@prefix rdf: <http://www.w3.org/1999/02/22-rdf-syntax-ns#> .
@prefix owl: <http://www.w3.org/2002/07/owl#> .
@prefix xsd: <http://www.w3.org/2001/XMLSchema#> .
@prefix rdfs: <http://www.w3.org/2000/01/rdf-schema#> .
@prefix dc: <http://purl.org/dc/elements/1.1/> .
@prefix pds4: <http://ontology.pds.nasa.gov/taxonomy/> .
###########################################
########## Class definitions
########## DateTime:2021-07-22T22:00:58
###########################################
 
pds4:subClassOf a rdfs:subClassOf;
  rdfs:label "is_a".
 
pds4:urn:nasa:pds:0001_nasa_pds_1:pds:tndo_context:pds:agency::1.0 rdf:type rdfs:Class;
  rdfs:label "Agency";
  pds4:subClassOf pds4:urn:nasa:pds:0001_nasa_pds_1:pds:tagged_nondigital_object:pds:tndo_context::1.0;
  rdfs:comment "The Agency class provides a description of an entity that provides regional or national level governance over nodes within the federated Planetary Data System.".
 
pds4:urn:nasa:pds:0001_nasa_pds_1:pds:tndo_context:pds:airborne::1.0 rdf:type rdfs:Class;
  rdfs:label "Airborne";
  pds4:subClassOf pds4:urn:nasa:pds:0001_nasa_pds_1:pds:tagged_nondigital_object:pds:tndo_context::1.0;
  rdfs:comment "The Airborne class provides a description of the physical object that transports a platform by or through air.".
 
pds4:urn:nasa:pds:0001_nasa_pds_1:pds:tndo_context:pds:airborne:aircraft::1.0 rdf:type rdfs:Class;
  rdfs:label "Aircraft";
  rdfs:subClassOf pds4:urn:nasa:pds:0001_nasa_pds_1:pds:tndo_context:pds:airborne::1.0;
  rdfs:comment "An airborne observatory carried on a powered, heavier than air vessel supporting observations, measurements, and scientific experiments during flight.".
 
pds4:urn:nasa:pds:0001_nasa_pds_1:pds:tndo_context:pds:airborne:balloon::1.0 rdf:type rdfs:Class;
  rdfs:label "Balloon";
  rdfs:subClassOf pds4:urn:nasa:pds:0001_nasa_pds_1:pds:tndo_context:pds:airborne::1.0;
  rdfs:comment "A balloon-borne observatory, typically consisting of a gondola structure carrying one or more telescopes and instruments, borne aloft by an unpowered or minimially powered lighter-than-atmosphere balloon for a limited observing period.".
 
pds4:urn:nasa:pds:0001_nasa_pds_1:pds:tndo_context:pds:airborne:suborbital_rocket::1.0 rdf:type rdfs:Class;
  rdfs:label "Suborbital Rocket";
  rdfs:subClassOf pds4:urn:nasa:pds:0001_nasa_pds_1:pds:tndo_context:pds:airborne::1.0;
  rdfs:comment "A Suborbital Rocket is an instrument-carrying rocket designed to take measurements and perform scientific experiments during its sub-orbital flight.".
 
pds4:urn:nasa:pds:0001_nasa_pds_1:pds:product_components:pds:alias::1.0 rdf:type rdfs:Class;
  rdfs:label "Alias";
  pds4:subClassOf pds4:urn:nasa:pds:0001_nasa_pds_1:all:user:pds:product_components::1.0;
  rdfs:comment "The Alias class provides a single alternate name and identification for this product in this or some other archive or data system.".
 
pds4:urn:nasa:pds:0001_nasa_pds_1:pds:product_components:pds:alias_list::1.0 rdf:type rdfs:Class;
  rdfs:label "Alias_List";
  pds4:subClassOf pds4:urn:nasa:pds:0001_nasa_pds_1:all:user:pds:product_components::1.0;
  rdfs:comment "The Alias_List class provides a list of paired alternate names and identifications for this product in this or some other archive or data system.".
 
pds4:urn:nasa:pds:0001_nasa_pds_1:all:user:speclib:ancillary_product::1.0 rdf:type rdfs:Class;
  rdfs:label "Ancillary_Product";
  pds4:subClassOf pds4:urn:nasa:pds:0001_nasa_pds_1:all:user::1.0;
  rdfs:comment "The Ancillary_Product class identifies an ancillary measurement related to a Spectral Library specimen.".
 
pds4:urn:nasa:pds:0001_nasa_pds_1:all:user:nucspec:applicable_records::1.0 rdf:type rdfs:Class;
  rdfs:label "Applicable_Records";
  pds4:subClassOf pds4:urn:nasa:pds:0001_nasa_pds_1:all:user::1.0;
  rdfs:comment "The records to which this state applies.".
 
pds4:urn:nasa:pds:0001_nasa_pds_1:pds:information_package:pds:archival_information_package::1.0 rdf:type rdfs:Class;
  rdfs:label "Archival_Information_Package";
  pds4:subClassOf pds4:urn:nasa:pds:0001_nasa_pds_1:pds:tndo_supplemental:pds:information_package::1.0;
  rdfs:comment "The Archival Information Package (AIP) class defines an Information Package consisting of the Content Information and the associated Preservation Description Information (PDI), which is preserved within an archive that conforms to the Open Archive Information System (OAIS) Reference Model.".
 
pds4:urn:nasa:pds:0001_nasa_pds_1:pds:byte_stream:pds:array::1.0 rdf:type rdfs:Class;
  rdfs:label "Array";
  pds4:subClassOf pds4:urn:nasa:pds:0001_nasa_pds_1:pds:tagged_digital_object:pds:byte_stream::1.0;
  rdfs:comment "The Array class defines a homogeneous N-dimensional array of scalars. The Array class is the parent class for all n-dimensional arrays of scalars.".
 
pds4:urn:nasa:pds:0001_nasa_pds_1:pds:array:pds:array_1d::1.0 rdf:type rdfs:Class;
  rdfs:label "Array_1D";
  pds4:subClassOf pds4:urn:nasa:pds:0001_nasa_pds_1:pds:byte_stream:pds:array::1.0;
  rdfs:comment "The Array 1D class is the parent class for all one dimensional array based classes.".
 
pds4:urn:nasa:pds:0001_nasa_pds_1:pds:array:pds:array_2d::1.0 rdf:type rdfs:Class;
  rdfs:label "Array_2D";
  pds4:subClassOf pds4:urn:nasa:pds:0001_nasa_pds_1:pds:byte_stream:pds:array::1.0;
  rdfs:comment "The Array 2D class is the parent class for all two dimensional array based classes.".
 
pds4:urn:nasa:pds:0001_nasa_pds_1:pds:array_2d:pds:array_2d_image::1.0 rdf:type rdfs:Class;
  rdfs:label "Array_2D_Image";
  pds4:subClassOf pds4:urn:nasa:pds:0001_nasa_pds_1:pds:array:pds:array_2d::1.0;
  rdfs:comment "The Array 2D Image class is an extension of the Array 2D class and defines a two dimensional image.".
 
pds4:urn:nasa:pds:0001_nasa_pds_1:pds:array_2d:pds:array_2d_map::1.0 rdf:type rdfs:Class;
  rdfs:label "Array_2D_Map";
  pds4:subClassOf pds4:urn:nasa:pds:0001_nasa_pds_1:pds:array:pds:array_2d::1.0;
  rdfs:comment "The Array 2D Map class is an extension of the Array 2D class and defines a  two dimensional map.".
 
pds4:urn:nasa:pds:0001_nasa_pds_1:pds:array_2d:pds:array_2d_spectrum::1.0 rdf:type rdfs:Class;
  rdfs:label "Array_2D_Spectrum";
  pds4:subClassOf pds4:urn:nasa:pds:0001_nasa_pds_1:pds:array:pds:array_2d::1.0;
  rdfs:comment "The Array 2D Spectrum class is an extension of the Array 2D class and defines a  two dimensional spectrum.".
 
pds4:urn:nasa:pds:0001_nasa_pds_1:pds:array:pds:array_3d::1.0 rdf:type rdfs:Class;
  rdfs:label "Array_3D";
  pds4:subClassOf pds4:urn:nasa:pds:0001_nasa_pds_1:pds:byte_stream:pds:array::1.0;
  rdfs:comment "The Array 3D class is the parent class for all three dimensional array based classes.".
 
pds4:urn:nasa:pds:0001_nasa_pds_1:pds:array_3d:pds:array_3d_image::1.0 rdf:type rdfs:Class;
  rdfs:label "Array_3D_Image";
  pds4:subClassOf pds4:urn:nasa:pds:0001_nasa_pds_1:pds:array:pds:array_3d::1.0;
  rdfs:comment "The Array 3D Image class is an extension of the Array 3D class and defines a  three dimensional image.".
 
pds4:urn:nasa:pds:0001_nasa_pds_1:pds:array_3d:pds:array_3d_movie::1.0 rdf:type rdfs:Class;
  rdfs:label "Array_3D_Movie";
  pds4:subClassOf pds4:urn:nasa:pds:0001_nasa_pds_1:pds:array:pds:array_3d::1.0;
  rdfs:comment "The Array 3D  Movie class is an extension of the Array 3D class and defines a  movie as a set of two dimensional images in a time series.".
 
pds4:urn:nasa:pds:0001_nasa_pds_1:pds:array_3d:pds:array_3d_spectrum::1.0 rdf:type rdfs:Class;
  rdfs:label "Array_3D_Spectrum";
  pds4:subClassOf pds4:urn:nasa:pds:0001_nasa_pds_1:pds:array:pds:array_3d::1.0;
  rdfs:comment "The Array 3D Spectrum class is an extension of the Array 3D class and defines a  three dimensional spectrum.".
 
pds4:urn:nasa:pds:0001_nasa_pds_1:all:user:geom:articulation_device_parameters::1.0 rdf:type rdfs:Class;
  rdfs:label "Articulation_Device_Parameters";
  pds4:subClassOf pds4:urn:nasa:pds:0001_nasa_pds_1:all:user::1.0;
  rdfs:comment "The Articulation_Device_Parameters class contains those attributes and sub-classes that describe an articulation device. An articulation device is anything that can move independently of the spacecraft to which it is attached. Examples include mast heads, wheel bogies, arms, filter wheel, scan platforms. ".
 
pds4:urn:nasa:pds:0001_nasa_pds_1:img:data_processing:img:autoexposure::1.0 rdf:type rdfs:Class;
  rdfs:label "Autoexposure";
  pds4:subClassOf pds4:urn:nasa:pds:0001_nasa_pds_1:all:user:img:data_processing::1.0;
  rdfs:comment "The Autoexposure class contains attributes used to identify or describe the algorithm used to automatically calculate the proper exposure time. This is generally based on some kind of histogram analysis. The specific autoexposure algorithm used is defined in the processing_algorithm attribute, and the specific set of attributes needed to describe it will vary based on the algorithm. Examples of autoexposure algorithms include \"Maki 2003\" used on MER, MSL ECAMs, M2020 ECAMS; \"Maurice 2012\" used on MSL ChemCam; \"Smith 1997\" used on Mars Pathfinder Imager.".
 
pds4:urn:nasa:pds:0001_nasa_pds_1:pds:tagged_digital_child:pds:axis_array::1.0 rdf:type rdfs:Class;
  rdfs:label "Axis_Array";
  pds4:subClassOf pds4:urn:nasa:pds:0001_nasa_pds_1:all:user:pds:tagged_digital_child::1.0;
  rdfs:comment "The Axis Array class is used as a component of the array class and defines an axis of the array.".
 
pds4:urn:nasa:pds:0001_nasa_pds_1:all:user:sp:axis_bin_set_energy::1.0 rdf:type rdfs:Class;
  rdfs:label "Axis_Bin_Set_Energy";
  pds4:subClassOf pds4:urn:nasa:pds:0001_nasa_pds_1:all:user::1.0;
  rdfs:comment " The Axis_Bin_Set_* classes describe the spectral characteristics of each band along the spectral dimension of the data object. This will be a literal \"axis\" in the case of 2D and 3D spectral arrays, or the \"Row\" axis of a spectral table (each row is a spectral bin), or the \"Field\" axis of table containing one spectrum per row. These classes are used in cases where the spectral information is not uniform along the spectral dimension. ".
 
pds4:urn:nasa:pds:0001_nasa_pds_1:all:user:sp:axis_bin_set_frequency::1.0 rdf:type rdfs:Class;
  rdfs:label "Axis_Bin_Set_Frequency";
  pds4:subClassOf pds4:urn:nasa:pds:0001_nasa_pds_1:all:user::1.0;
  rdfs:comment " The Axis_Bin_Set_* classes describe the spectral characteristics of each band along the spectral dimension of the data object. This will be a literal \"axis\" in the case of 2D and 3D spectral arrays, or the \"Row\" axis of a spectral table (each row is a spectral bin), or the \"Field\" axis of table containing one spectrum per row. These classes are used in cases where the spectral information is not uniform along the spectral dimension. ".
 
pds4:urn:nasa:pds:0001_nasa_pds_1:all:user:sp:axis_bin_set_wavelength::1.0 rdf:type rdfs:Class;
  rdfs:label "Axis_Bin_Set_Wavelength";
  pds4:subClassOf pds4:urn:nasa:pds:0001_nasa_pds_1:all:user::1.0;
  rdfs:comment " The Axis_Bin_Set_* classes describe the spectral characteristics of each band along the spectral dimension of the data object. This will be a literal \"axis\" in the case of 2D and 3D spectral arrays, or the \"Row\" axis of a spectral table (each row is a spectral bin), or the \"Field\" axis of table containing one spectrum per row. These classes are used in cases where the spectral information is not uniform along the spectral dimension. ".
 
pds4:urn:nasa:pds:0001_nasa_pds_1:all:user:sp:axis_bin_set_wavenumber::1.0 rdf:type rdfs:Class;
  rdfs:label "Axis_Bin_Set_Wavenumber";
  pds4:subClassOf pds4:urn:nasa:pds:0001_nasa_pds_1:all:user::1.0;
  rdfs:comment " The Axis_Bin_Set_* classes describe the spectral characteristics of each band along the spectral dimension of the data object. This will be a literal \"axis\" in the case of 2D and 3D spectral arrays, or the \"Row\" axis of a spectral table (each row is a spectral bin), or the \"Field\" axis of table containing one spectrum per row. These classes are used in cases where the spectral information is not uniform along the spectral dimension. ".
 
pds4:urn:nasa:pds:0001_nasa_pds_1:pds:tndo_supplemental:pds:band_bin::1.0 rdf:type rdfs:Class;
  rdfs:label "Band_Bin";
  pds4:subClassOf pds4:urn:nasa:pds:0001_nasa_pds_1:pds:tagged_nondigital_object:pds:tndo_supplemental::1.0;
  rdfs:comment "The Band_Bin class specifies the characteristics of an individual spectral band in a spectral qube.".
 
pds4:urn:nasa:pds:0001_nasa_pds_1:pds:tndo_supplemental:pds:band_bin_set::1.0 rdf:type rdfs:Class;
  rdfs:label "Band_Bin_Set";
  pds4:subClassOf pds4:urn:nasa:pds:0001_nasa_pds_1:pds:tagged_nondigital_object:pds:tndo_supplemental::1.0;
  rdfs:comment "The Band_Bin_Set class contains the spectral characteristics for all the spectral bands in a qube.".
 
pds4:urn:nasa:pds:0001_nasa_pds_1:all:user:sp:bin_center_lookup::1.0 rdf:type rdfs:Class;
  rdfs:label "Bin_Center_Lookup";
  pds4:subClassOf pds4:urn:nasa:pds:0001_nasa_pds_1:all:user::1.0;
  rdfs:comment " The Bin_Center_Lookup class provides a link to a map or list of bin center values - either to a field in a spectral table, or to a distinct data object that is part of the same product, or to a separate PDS product containing the information. ".
 
pds4:urn:nasa:pds:0001_nasa_pds_1:all:user:sp:bin_description::1.0 rdf:type rdfs:Class;
  rdfs:label "Bin_Description";
  pds4:subClassOf pds4:urn:nasa:pds:0001_nasa_pds_1:all:user::1.0;
  rdfs:comment " This class groups the various bin description options, allowing a user to choose one. ".
 
pds4:urn:nasa:pds:0001_nasa_pds_1:all:user:sp:bin_energy::1.0 rdf:type rdfs:Class;
  rdfs:label "Bin_Energy";
  pds4:subClassOf pds4:urn:nasa:pds:0001_nasa_pds_1:all:user::1.0;
  rdfs:comment " The Bin_Energy class specifies the characteristics of an individual bin along a spectral or other binned axis in an Array object, in units of energy. ".
 
pds4:urn:nasa:pds:0001_nasa_pds_1:all:user:sp:bin_frequency::1.0 rdf:type rdfs:Class;
  rdfs:label "Bin_Frequency";
  pds4:subClassOf pds4:urn:nasa:pds:0001_nasa_pds_1:all:user::1.0;
  rdfs:comment " The Bin_Frequency class specifies the characteristics of an individual bin along a spectral or other binned axis in an Array object, in units of frequency. ".
 
pds4:urn:nasa:pds:0001_nasa_pds_1:all:user:sp:bin_wavelength::1.0 rdf:type rdfs:Class;
  rdfs:label "Bin_Wavelength";
  pds4:subClassOf pds4:urn:nasa:pds:0001_nasa_pds_1:all:user::1.0;
  rdfs:comment " The Bin_Wavelength class specifies the characteristics of an individual bin along a spectral or other binned axis in an Array object, in units of wavelength. ".
 
pds4:urn:nasa:pds:0001_nasa_pds_1:all:user:sp:bin_wavenumber::1.0 rdf:type rdfs:Class;
  rdfs:label "Bin_Wavenumber";
  pds4:subClassOf pds4:urn:nasa:pds:0001_nasa_pds_1:all:user::1.0;
  rdfs:comment " The Bin_Wavenumber class specifies the characteristics of an individual bin along a spectral or other binned axis in an Array object, in units of wavenumber. ".
 
pds4:urn:nasa:pds:0001_nasa_pds_1:all:user:sp:bin_width_constant::1.0 rdf:type rdfs:Class;
  rdfs:label "Bin_Width_Constant";
  pds4:subClassOf pds4:urn:nasa:pds:0001_nasa_pds_1:all:user::1.0;
  rdfs:comment " The Bin_Width_Constant class is used inside a Bin_Width_Lookup class for those cases where the bin width is either not well known or unknown. It provides a way to specify a nominal constant width or indicate that there is no available information about the bin width. If the bin width is completely unknown, use the appropriate bin_width attribute for the spectral type (frequency, wavelength, wavenumber, or energy), and indicate that it is nil, with a reason of \"unknown\". When this class is used, a full explanation of the situation should be provided by the bin_width_desc attribute of the parent class. ".
 
pds4:urn:nasa:pds:0001_nasa_pds_1:all:user:sp:bin_width_lookup::1.0 rdf:type rdfs:Class;
  rdfs:label "Bin_Width_Lookup";
  pds4:subClassOf pds4:urn:nasa:pds:0001_nasa_pds_1:all:user::1.0;
  rdfs:comment " The Bin_Width_Lookup class provides a link to a map or list of bin width values - either to a field in a spectral table, or to a distinct data object that is part of the same product, or to a separate PDS product containing the information. ".
 
pds4:urn:nasa:pds:0001_nasa_pds_1:all:user:rings:body_ident_base::1.0 rdf:type rdfs:Class;
  rdfs:label "Body_Ident_Base";
  pds4:subClassOf pds4:urn:nasa:pds:0001_nasa_pds_1:all:user::1.0;
  rdfs:comment "The Body_Ident_Base class provides multiple attributes that can be used to identify a physical object (spacecraft, planet instrument, transmitter, system barycenter, etc.). At least one must be used. ".
 
pds4:urn:nasa:pds:0001_nasa_pds_1:all:user:geom:body_identification_base::1.0 rdf:type rdfs:Class;
  rdfs:label "Body_Identification_Base";
  pds4:subClassOf pds4:urn:nasa:pds:0001_nasa_pds_1:all:user::1.0;
  rdfs:comment "The Body_Identification_Base class provides multiple attributes that can be used to identify a physical object (spacecraft, planet instrument, transmitter, system barycenter, etc.). At least one must be used. ".
 
pds4:urn:nasa:pds:0001_nasa_pds_1:all:user:cart:bounding_coordinates::1.0 rdf:type rdfs:Class;
  rdfs:label "Bounding_Coordinates";
  pds4:subClassOf pds4:urn:nasa:pds:0001_nasa_pds_1:all:user::1.0;
  rdfs:comment "The Bounding_Coordinates class defines the limits of coverage of a set of data expressed by latitude and longitude values in the order western-most, eastern-most, northern-most, and southern-most. ".
 
pds4:urn:nasa:pds:0001_nasa_pds_1:img:data_processing:img:brightness_correction::1.0 rdf:type rdfs:Class;
  rdfs:label "Brightness_Correction";
  pds4:subClassOf pds4:urn:nasa:pds:0001_nasa_pds_1:all:user:img:data_processing::1.0;
  rdfs:comment "The Brightness_Correction class describes brightness corrections that were applied to an image or mosaic. Brightness correction is the process of adjusting the DN values of adjacent frames in a mosaic so they match visually. It may also involve contrast or vignetting adjustments. The result may no longer be radiometrically calibrated due to the adjustments. The processing_algorithm child of Brightness_Correction describes the type of brightness correction, and should correspond to the classes within Brightness_Correction_Image. If the algorithm is \"MIXED\", multiple algorithms were used, in which case the specific information in each Brightness_Correction_Image must be used.".
 
pds4:urn:nasa:pds:0001_nasa_pds_1:img:data_processing_file:img:brightness_correction_file::1.0 rdf:type rdfs:Class;
  rdfs:label "Brightness_Correction_File";
  pds4:subClassOf pds4:urn:nasa:pds:0001_nasa_pds_1:all:user:img:data_processing_file::1.0;
  rdfs:comment "The Brightness_Correction_File identifies a file containing brightness correction information. The project SIS should define the format of this file. Correction information may appear in the file, in instances of the Brightness_Correction_Image class, or both (if both, they should be consistent).".
 
pds4:urn:nasa:pds:0001_nasa_pds_1:all:user:img:brightness_correction_hsi_linear::1.0 rdf:type rdfs:Class;
  rdfs:label "Brightness_Correction_HSI_Linear";
  pds4:subClassOf pds4:urn:nasa:pds:0001_nasa_pds_1:all:user::1.0;
  rdfs:comment "The Brightness_Correction_HSI_Linear class works just like Brightness_Correction_Linear, except that the color image is first converted to HSI (Hue, Saturation, Intensity) space, the correction is applied only to Intensity, and then the result is converted back to RGB space.".
 
pds4:urn:nasa:pds:0001_nasa_pds_1:all:user:img:brightness_correction_image::1.0 rdf:type rdfs:Class;
  rdfs:label "Brightness_Correction_Image";
  pds4:subClassOf pds4:urn:nasa:pds:0001_nasa_pds_1:all:user::1.0;
  rdfs:comment "The Brighness_Correction_Image class describes the brightness correction that was applied to a single image, whether alone or part of a mosaic. The image this correction applies to may be identified via the enclosed Internal_Reference, or via the order in which the Brightness_Correction_Image objects appear (which matches the order given in Input_Product_List).".
 
pds4:urn:nasa:pds:0001_nasa_pds_1:all:user:img:brightness_correction_linear::1.0 rdf:type rdfs:Class;
  rdfs:label "Brightness_Correction_Linear";
  pds4:subClassOf pds4:urn:nasa:pds:0001_nasa_pds_1:all:user::1.0;
  rdfs:comment "The Brightness_Correction_Linear class describes a simple linear brightness correction, with an additive (brightness_offset) and multiplicative (brightness_scale) factor applied. The result is: output = input * brightness_scale + brightness_offset. If there are multiple bands, the same correction is applied to each band.".
 
pds4:urn:nasa:pds:0001_nasa_pds_1:pds:tndo_supplemental:pds:bundle::1.0 rdf:type rdfs:Class;
  rdfs:label "Bundle";
  pds4:subClassOf pds4:urn:nasa:pds:0001_nasa_pds_1:pds:tagged_nondigital_object:pds:tndo_supplemental::1.0;
  rdfs:comment "The Bundle class describes a collection of collections.".
 
pds4:urn:nasa:pds:0001_nasa_pds_1:pds:product_components:pds:bundle_member_entry::1.0 rdf:type rdfs:Class;
  rdfs:label "Bundle_Member_Entry";
  pds4:subClassOf pds4:urn:nasa:pds:0001_nasa_pds_1:all:user:pds:product_components::1.0;
  rdfs:comment "The Bundle Member Entry class provides a member reference to a collection.".
 
pds4:urn:nasa:pds:0001_nasa_pds_1:pds:tagged_digital_object:pds:byte_stream::1.0 rdf:type rdfs:Class;
  rdfs:label "Byte_Stream";
  pds4:subClassOf pds4:urn:nasa:pds:0001_nasa_pds_1:all:user:pds:tagged_digital_object::1.0;
  rdfs:comment "The Byte Stream class defines a stream of bytes.".
 
pds4:urn:nasa:pds:0001_nasa_pds_1:geom:cahvor_model:geom:cahvore_model::1.0 rdf:type rdfs:Class;
  rdfs:label "CAHVORE_Model";
  pds4:subClassOf pds4:urn:nasa:pds:0001_nasa_pds_1:geom:cahv_model:geom:cahvor_model::1.0;
  rdfs:comment "The CAHVORE model is built upon CAHVOR (see CAHVOR_Model), adding support for fisheye lenses. It adds one more 3-vector and two scalars to CAHVOR. E (Entrance_Terms) contains the coefficients of a polynomial function used to model movement of the entrance pupil. The two scalars, cahvore_model_type and cahvore_model_parameter, together specify the type of lens being modeled. ".
 
pds4:urn:nasa:pds:0001_nasa_pds_1:geom:cahv_model:geom:cahvor_model::1.0 rdf:type rdfs:Class;
  rdfs:label "CAHVOR_Model";
  pds4:subClassOf pds4:urn:nasa:pds:0001_nasa_pds_1:all:user:geom:cahv_model::1.0;
  rdfs:comment "The CAHVOR model is built upon CAHV (see CAHV_Model), adding radial (barrel or pincushion) distortion to the linear model. It adds two more 3-vectors to CAHV. O (Vector_Optical) is a unit vector representing the axis of symmetry for the radial distortion. R (Radial_Terms) contains the coefficients of a polynomial function that describes the radial distortion. ".
 
pds4:urn:nasa:pds:0001_nasa_pds_1:all:user:geom:cahv_model::1.0 rdf:type rdfs:Class;
  rdfs:label "CAHV_Model";
  pds4:subClassOf pds4:urn:nasa:pds:0001_nasa_pds_1:all:user::1.0;
  rdfs:comment "The CAHV model is a linear, perspective-projection camera model (equivalent to a pinhole camera). It consists of four 3-vectors (C,A,H,V) that describe the internal and external camera model parameters needed to translate between 2D image coordinates and 3D world coordinates. C (Vector_Center) is the 3D position of the pinhole (center of the entrance pupil). A (Vector_Axis) is a unit vector normal to the image plane pointing outward. H (Vector_Horizontal) is a composite vector encoding three quantities: H\\' (a vector in the image plane perpendicular to the vertical columns), Hs (the distance between the lens center and image plane, measured in horizontal pixels), and Hc (the horizontal image coordinate directly under C when moving parallel to A). V (Vector_Vertical) similarly composites the analogous V\\', Vs, and Vc in the vertical direction. ".
 
pds4:urn:nasa:pds:0001_nasa_pds_1:all:user:nucspec:calibration_reference::1.0 rdf:type rdfs:Class;
  rdfs:label "Calibration_Reference";
  pds4:subClassOf pds4:urn:nasa:pds:0001_nasa_pds_1:all:user::1.0;
  rdfs:comment "Contains a reference to a document that describes the energy calibration for the product.".
 
pds4:urn:nasa:pds:0001_nasa_pds_1:all:user:cart:camera_model_offset::1.0 rdf:type rdfs:Class;
  rdfs:label "Camera_Model_Offset";
  pds4:subClassOf pds4:urn:nasa:pds:0001_nasa_pds_1:all:user::1.0;
  rdfs:comment "The Camera_Model_Offset class specifies the location of the image origin with respect to the camera model\\'s origin. For CAHV\\//CAHVOR models, this origin is not the center of the camera, but is the upper-left corner of the \"standard\"-size image, which is encoded in the CAHV vectors. Applies to the Perspective lander map projection.".
 
pds4:urn:nasa:pds:0001_nasa_pds_1:all:user:geom:camera_model_parameters::1.0 rdf:type rdfs:Class;
  rdfs:label "Camera_Model_Parameters";
  pds4:subClassOf pds4:urn:nasa:pds:0001_nasa_pds_1:all:user::1.0;
  rdfs:comment "A camera model describes the mathematical relationship between the coordinates of a point in 3-dimensional space and its projection onto a 2-dimensional image plane. There are numerous types of camera models. ".
 
pds4:urn:nasa:pds:0001_nasa_pds_1:all:user:cart:cartography::1.0 rdf:type rdfs:Class;
  rdfs:label "Cartography";
  pds4:subClassOf pds4:urn:nasa:pds:0001_nasa_pds_1:all:user::1.0;
  rdfs:comment "The Cartography class provides a description of how a 3D sphere, spheroid, or elliptical spheroid or the celestial sphere is mapped onto a plane. ".
 
pds4:urn:nasa:pds:0001_nasa_pds_1:rings:body_ident_base:rings:central_body_ident::1.0 rdf:type rdfs:Class;
  rdfs:label "Central_Body_Ident";
  pds4:subClassOf pds4:urn:nasa:pds:0001_nasa_pds_1:all:user:rings:body_ident_base::1.0;
  rdfs:comment "The Central_Body_Ident class uniquely identifies the body that is the central body associated with an observation (e.g., Saturn for Saturn system observations). ".
 
pds4:urn:nasa:pds:0001_nasa_pds_1:geom:body_identification_base:geom:central_body_identification::1.0 rdf:type rdfs:Class;
  rdfs:label "Central_Body_Identification";
  pds4:subClassOf pds4:urn:nasa:pds:0001_nasa_pds_1:all:user:geom:body_identification_base::1.0;
  rdfs:comment "The Central_Body_Identification class uniquely identifies the body that is the central body associated with an observation (e.g., Saturn for Saturn system observations). ".
 
pds4:urn:nasa:pds:0001_nasa_pds_1:rings:central_body_ident:rings:central_body_parameters::1.0 rdf:type rdfs:Class;
  rdfs:label "Central_Body_Parameters";
  pds4:subClassOf pds4:urn:nasa:pds:0001_nasa_pds_1:rings:body_ident_base:rings:central_body_ident::1.0;
  rdfs:comment "This class provides the parameters used to generate a ring model which are specific to the central body.".
 
pds4:urn:nasa:pds:0001_nasa_pds_1:pds:parsable_byte_stream:pds:checksum_manifest::1.0 rdf:type rdfs:Class;
  rdfs:label "Checksum_Manifest";
  pds4:subClassOf pds4:urn:nasa:pds:0001_nasa_pds_1:pds:byte_stream:pds:parsable_byte_stream::1.0;
  rdfs:comment "The Checksum_Manifest class defines a two column table for file references and checksums.".
 
pds4:urn:nasa:pds:0001_nasa_pds_1:all:user:sp:circular_fov::1.0 rdf:type rdfs:Class;
  rdfs:label "Circular_FOV";
  pds4:subClassOf pds4:urn:nasa:pds:0001_nasa_pds_1:all:user::1.0;
  rdfs:comment " The Circular_FOV class contains attributes to describe a circular aperture\\//field of view. ".
 
pds4:urn:nasa:pds:0001_nasa_pds_1:pds:product_components:pds:citation_information::1.0 rdf:type rdfs:Class;
  rdfs:label "Citation_Information";
  pds4:subClassOf pds4:urn:nasa:pds:0001_nasa_pds_1:all:user:pds:product_components::1.0;
  rdfs:comment "The Citation_Information class provides specific fields often used in citing the product in journal articles, abstract services, and other reference contexts.".
 
pds4:urn:nasa:pds:0001_nasa_pds_1:all:user:img:col_sum::1.0 rdf:type rdfs:Class;
  rdfs:label "Col_Sum";
  pds4:subClassOf pds4:urn:nasa:pds:0001_nasa_pds_1:all:user::1.0;
  rdfs:comment "Describes a Column Summation product, which is a single row containing the sum of all pixels in each column of the image.".
 
pds4:urn:nasa:pds:0001_nasa_pds_1:pds:tndo_supplemental:pds:collection::1.0 rdf:type rdfs:Class;
  rdfs:label "Collection";
  pds4:subClassOf pds4:urn:nasa:pds:0001_nasa_pds_1:pds:tagged_nondigital_object:pds:tndo_supplemental::1.0;
  rdfs:comment "The Collection class provides a description of a set of products.".
 
pds4:urn:nasa:pds:0001_nasa_pds_1:all:user:disp:color_display_settings::1.0 rdf:type rdfs:Class;
  rdfs:label "Color_Display_Settings";
  pds4:subClassOf pds4:urn:nasa:pds:0001_nasa_pds_1:all:user::1.0;
  rdfs:comment "The Color_Display_Settings class provides guidance to data users on how to display a multi-banded Array object on a color-capable display device.".
 
pds4:urn:nasa:pds:0001_nasa_pds_1:img:data_processing:img:color_filter_array::1.0 rdf:type rdfs:Class;
  rdfs:label "Color_Filter_Array";
  pds4:subClassOf pds4:urn:nasa:pds:0001_nasa_pds_1:all:user:img:data_processing::1.0;
  rdfs:comment "The Color_Filter_Array class describes whether or not an image was acquired using a Color Filter Array (CFA) and if so, whether and how the CFA pattern was removed. A CFA is a method for making color images using one exposure on a single sensor plane, where microfilters of different wavelengths are put in front of pixels in a specific pattern. The most common pattern is the Bayer pattern, which has a red, blue, and two green pixels in every 2x2 pixel square. Although generally used for RGB color, CFA filters can be of any number and wavelength (see color_filter_array_type).".
 
pds4:urn:nasa:pds:0001_nasa_pds_1:img:data_processing:img:color_processing::1.0 rdf:type rdfs:Class;
  rdfs:label "Color_Processing";
  pds4:subClassOf pds4:urn:nasa:pds:0001_nasa_pds_1:all:user:img:data_processing::1.0;
  rdfs:comment "The Color_Processing class contains parameters describing color correction or processing and how the image is represented in color.".
 
pds4:urn:nasa:pds:0001_nasa_pds_1:all:user:msn_surface:command_execution::1.0 rdf:type rdfs:Class;
  rdfs:label "Command_Execution";
  pds4:subClassOf pds4:urn:nasa:pds:0001_nasa_pds_1:all:user::1.0;
  rdfs:comment "The Command_Execution class contains information about how the command that acquired this data was executed, such as sequence or activity.".
 
pds4:urn:nasa:pds:0001_nasa_pds_1:all:user:geom:commanded_geometry::1.0 rdf:type rdfs:Class;
  rdfs:label "Commanded_Geometry";
  pds4:subClassOf pds4:urn:nasa:pds:0001_nasa_pds_1:all:user::1.0;
  rdfs:comment " Specifies how the device was commanded in order to achieve the state represented in the enclosing Articulation_Device_Parameters. Commands are often at a higher level, e.g. point at this location or move to this XYZ, which is translated by flight software to the actual pose of the device. Certain forms of command are measured in a coordinate frame; this is specified by the Coordinate_Space_Reference in this class (if not present, the Coordinate_Space_Reference in the Articulation_Device_Parameters parent should be assumed). ".
 
pds4:urn:nasa:pds:0001_nasa_pds_1:all:user:img:commanded_parameters::1.0 rdf:type rdfs:Class;
  rdfs:label "Commanded_Parameters";
  pds4:subClassOf pds4:urn:nasa:pds:0001_nasa_pds_1:all:user::1.0;
  rdfs:comment "The Commanded_Parameters class contains attributes used to identify or describe the commands sent to a spacecraft to perform one or more actions resulting in the acquisition of the current data product. These are distinct from similar values in the root Imaging class which indicate the state of the image as acquired.".
 
pds4:urn:nasa:pds:0001_nasa_pds_1:all:user:img_surface:commanded_parameters::1.0 rdf:type rdfs:Class;
  rdfs:label "Commanded_Parameters";
  pds4:subClassOf pds4:urn:nasa:pds:0001_nasa_pds_1:all:user::1.0;
  rdfs:comment "The Commanded_Parameters class contains attributes used to identify or describe the commands sent to a spacecraft to perform one or more actions resulting in the acquisition of the current data product. These are distinct from similar values in the root Surface_Imaging class which indicate the state of the image as acquired".
 
pds4:urn:nasa:pds:0001_nasa_pds_1:all:user:msn_surface:commanded_parameters::1.0 rdf:type rdfs:Class;
  rdfs:label "Commanded_Parameters";
  pds4:subClassOf pds4:urn:nasa:pds:0001_nasa_pds_1:all:user::1.0;
  rdfs:comment "The Commanded_Parameters class contains attributes used to identify or describe the commands sent to a spacecraft to perform one or more actions resulting in the acquisition of the current data product. These are distinct from similar values in the root Surface_Mission_Information class which indicate the state of the data as acquired.".
 
pds4:urn:nasa:pds:0001_nasa_pds_1:geom:vector_cartesian_position_base:geom:commanded_position::1.0 rdf:type rdfs:Class;
  rdfs:label "Commanded_Position";
  pds4:subClassOf pds4:urn:nasa:pds:0001_nasa_pds_1:all:user:geom:vector_cartesian_position_base::1.0;
  rdfs:comment " Specifies a Cartesian position used in commanding the device. ".
 
pds4:urn:nasa:pds:0001_nasa_pds_1:img:data_processing:img:companding::1.0 rdf:type rdfs:Class;
  rdfs:label "Companding";
  pds4:subClassOf pds4:urn:nasa:pds:0001_nasa_pds_1:all:user:img:data_processing::1.0;
  rdfs:comment " The Companding class describes whether or not data is or has had its bit depth reduced (for example conversion from 12 to 8 bits via a lookup table or bit scaling), the venue where it occurred (Software or Hardware), and the method used to complete the companding. The processing_algorithm attribute specifies how data was companded. Generally this will either be via a lookup table (such as a square root encoding), or by shifting bits to preserve the high order bits and discard the low order bits. The value of this keyword is mission specific but there are recommended values that should apply across missions when possible: NONE - no scaling. LUTn - use the numbered lookup table. Lookup tables are defined in the mission SIS. It is preferred for \"n\" to be a number but it could be a name, for example LUT_MMM_3 to indicate LUT 3 for the MMM instruments (on MSL). MSB_BITn - Shift to make bit \"n\" the most significant. Bits start numbering at 0 so MSB_BIT7 means no shift for a 12->8 bit companding, while MSB_BIT11 means to shift right 4 bits for a 12->8 bit companding. AUTOSHIFT - Data should be shifted to preserve the highest value. This value should only appear in a command echo; one of the MSB_BITn values should be used in downlinked data to specify what the actual shift was.".
 
pds4:urn:nasa:pds:0001_nasa_pds_1:img:data_processing_file:img:companding_file::1.0 rdf:type rdfs:Class;
  rdfs:label "Companding_File";
  pds4:subClassOf pds4:urn:nasa:pds:0001_nasa_pds_1:all:user:img:data_processing_file::1.0;
  rdfs:comment "The Companding _File class specifies the file containing the decompanding (inverse LUT) table used to process the data.".
 
pds4:urn:nasa:pds:0001_nasa_pds_1:img:data_processing_file:img:companding_table::1.0 rdf:type rdfs:Class;
  rdfs:label "Companding_Table";
  pds4:subClassOf pds4:urn:nasa:pds:0001_nasa_pds_1:all:user:img:data_processing_file::1.0;
  rdfs:comment "The Companding_Table class specifies the look up table used to compand the data.".
 
pds4:urn:nasa:pds:0001_nasa_pds_1:all:user:img:companding_table_mapping::1.0 rdf:type rdfs:Class;
  rdfs:label "Companding_Table_Mapping";
  pds4:subClassOf pds4:urn:nasa:pds:0001_nasa_pds_1:all:user::1.0;
  rdfs:comment "The Companding_Table_Mapping class specifies the mapping between the input DN range and the output DN as the data are companded.".
 
pds4:urn:nasa:pds:0001_nasa_pds_1:all:user:sp:complex_fov::1.0 rdf:type rdfs:Class;
  rdfs:label "Complex_FOV";
  pds4:subClassOf pds4:urn:nasa:pds:0001_nasa_pds_1:all:user::1.0;
  rdfs:comment " The Complex_FOV class is used for apertures (slits) that are not either circular or a simple rectangular shape. ".
 
pds4:urn:nasa:pds:0001_nasa_pds_1:pds:tagged_digital_object:pds:composite_structure::1.0 rdf:type rdfs:Class;
  rdfs:label "Composite_Structure";
  pds4:subClassOf pds4:urn:nasa:pds:0001_nasa_pds_1:all:user:pds:tagged_digital_object::1.0;
  rdfs:comment "The Composite Structure class provides a general framework for defining a structure that consists of two or more simpler structures".
 
pds4:urn:nasa:pds:0001_nasa_pds_1:all:user:img_surface:configuration::1.0 rdf:type rdfs:Class;
  rdfs:label "Configuration";
  pds4:subClassOf pds4:urn:nasa:pds:0001_nasa_pds_1:all:user::1.0;
  rdfs:comment "Defines a single configuration for this reachability assessment.".
 
pds4:urn:nasa:pds:0001_nasa_pds_1:all:user:img_surface:configurations::1.0 rdf:type rdfs:Class;
  rdfs:label "Configurations";
  pds4:subClassOf pds4:urn:nasa:pds:0001_nasa_pds_1:all:user::1.0;
  rdfs:comment "Specifies the configurations of the device used for reachability assessment. The specific values will be device-dependent but could include e.g. shoulder in\\//out, elbow up\\//down, wrist up\\//down.".
 
pds4:urn:nasa:pds:0001_nasa_pds_1:pds:product_components:pds:context_area::1.0 rdf:type rdfs:Class;
  rdfs:label "Context_Area";
  pds4:subClassOf pds4:urn:nasa:pds:0001_nasa_pds_1:all:user:pds:product_components::1.0;
  rdfs:comment "The Context Area provides context information for a product.".
 
pds4:urn:nasa:pds:0001_nasa_pds_1:all:user:survey:coordinate::1.0 rdf:type rdfs:Class;
  rdfs:label "Coordinate";
  pds4:subClassOf pds4:urn:nasa:pds:0001_nasa_pds_1:all:user::1.0;
  rdfs:comment "A location on the celestial sphere, consisting of right ascension and declination.".
 
pds4:urn:nasa:pds:0001_nasa_pds_1:all:user:cart:coordinate_representation::1.0 rdf:type rdfs:Class;
  rdfs:label "Coordinate_Representation";
  pds4:subClassOf pds4:urn:nasa:pds:0001_nasa_pds_1:all:user::1.0;
  rdfs:comment "The Coordinate_Representation class provides the method of encoding the position of a point by measuring its distance from perpendicular reference axes (the \"coordinate pair\" and \"row and column\" methods). ".
 
pds4:urn:nasa:pds:0001_nasa_pds_1:all:user:geom:coordinate_space_definition::1.0 rdf:type rdfs:Class;
  rdfs:label "Coordinate_Space_Definition";
  pds4:subClassOf pds4:urn:nasa:pds:0001_nasa_pds_1:all:user::1.0;
  rdfs:comment "The Coordinate_Space classes are typically used for lander\\//rover geometry while the Coordinate_System construction is used for orbiter\\//flyby geometry. ".
 
pds4:urn:nasa:pds:0001_nasa_pds_1:all:user:geom:coordinate_space_identification::1.0 rdf:type rdfs:Class;
  rdfs:label "Coordinate_Space_Identification";
  pds4:subClassOf pds4:urn:nasa:pds:0001_nasa_pds_1:all:user::1.0;
  rdfs:comment "The Coordinate_Space_Identification class uniquely identifies a coordinate space (i.e., reference frame + position) with respect to which the values of the attributes in the containing class are defined. ".
 
pds4:urn:nasa:pds:0001_nasa_pds_1:geom:list_index_no_units:geom:coordinate_space_index::1.0 rdf:type rdfs:Class;
  rdfs:label "Coordinate_Space_Index";
  pds4:subClassOf pds4:urn:nasa:pds:0001_nasa_pds_1:geom:list_index_base:geom:list_index_no_units::1.0;
  rdfs:comment "Identifies a coordinate space using an index value given in an identified list. ".
 
pds4:urn:nasa:pds:0001_nasa_pds_1:all:user:geom:coordinate_space_indexed::1.0 rdf:type rdfs:Class;
  rdfs:label "Coordinate_Space_Indexed";
  pds4:subClassOf pds4:urn:nasa:pds:0001_nasa_pds_1:all:user::1.0;
  rdfs:comment "The Coordinate_Space_Indexed class contains the attributes and classes identifying the indexed coordinate space. ".
 
pds4:urn:nasa:pds:0001_nasa_pds_1:geom:coordinate_space_identification:geom:coordinate_space_present::1.0 rdf:type rdfs:Class;
  rdfs:label "Coordinate_Space_Present";
  pds4:subClassOf pds4:urn:nasa:pds:0001_nasa_pds_1:all:user:geom:coordinate_space_identification::1.0;
  rdfs:comment "The Coordinate_Space_Present class includes the attributes that identifies the coordinate space presently being defined. ".
 
pds4:urn:nasa:pds:0001_nasa_pds_1:all:user:geom:coordinate_space_quality::1.0 rdf:type rdfs:Class;
  rdfs:label "Coordinate_Space_Quality";
  pds4:subClassOf pds4:urn:nasa:pds:0001_nasa_pds_1:all:user::1.0;
  rdfs:comment "Parameters that indicate the quality of the coordinate space knowledge. ".
 
pds4:urn:nasa:pds:0001_nasa_pds_1:geom:coordinate_space_identification:geom:coordinate_space_reference::1.0 rdf:type rdfs:Class;
  rdfs:label "Coordinate_Space_Reference";
  pds4:subClassOf pds4:urn:nasa:pds:0001_nasa_pds_1:all:user:geom:coordinate_space_identification::1.0;
  rdfs:comment "The Coordinate_Space_Reference class includes the attributes that identify the coordinate space being used to express coordinates in the class in which it appears. ".
 
pds4:urn:nasa:pds:0001_nasa_pds_1:all:user:geom:coordinate_space_spice::1.0 rdf:type rdfs:Class;
  rdfs:label "Coordinate_Space_SPICE";
  pds4:subClassOf pds4:urn:nasa:pds:0001_nasa_pds_1:all:user::1.0;
  rdfs:comment "Identifies a coordinate space using SPICE names for the frame and origin.".
 
pds4:urn:nasa:pds:0001_nasa_pds_1:all:user:geom:coordinate_system_identification::1.0 rdf:type rdfs:Class;
  rdfs:label "Coordinate_System_Identification";
  pds4:subClassOf pds4:urn:nasa:pds:0001_nasa_pds_1:all:user::1.0;
  rdfs:comment "The Coordinate_System_Identification class fully describes a coordinate system. This class is typically used for orbiter\\//flyby geometry while the Coordinate_Space construction is used for lander\\//rover geometry. Coordinate_System_Identification provides the reference frame, coordinate system type (cartesian, planetocentric, etc.), origin, and the instantiation time of the system when appropriate. The instantiation time (coordinate_system_time_utc) is used when a rotating frame has been \\'frozen\\' at a particular epoch. Instantiation time is not needed for inertial or rotating frames. ".
 
pds4:urn:nasa:pds:0001_nasa_pds_1:geom:body_identification_base:geom:coordinate_system_origin_identification::1.0 rdf:type rdfs:Class;
  rdfs:label "Coordinate_System_Origin_Identification";
  pds4:subClassOf pds4:urn:nasa:pds:0001_nasa_pds_1:all:user:geom:body_identification_base::1.0;
  rdfs:comment "The Coordinate_System_Origin_Identification class uniquely identifies the \"body\" that is the origin of a coordinate system. Typically body centered coordinate systems place the origin at the center of mass of the body. In addition to physical bodies, the origin may be defined at a point in space such as a system barycenter. Note that the origin of coordinate system does not necessarily correspond to either end point of a vector. ".
 
pds4:urn:nasa:pds:0001_nasa_pds_1:all:user:survey:corner_position::1.0 rdf:type rdfs:Class;
  rdfs:label "Corner_Position";
  pds4:subClassOf pds4:urn:nasa:pds:0001_nasa_pds_1:all:user::1.0;
  rdfs:comment "The position of one corner of an image".
 
pds4:urn:nasa:pds:0001_nasa_pds_1:img:list_index_no_units_imaging:img:correction_parameter::1.0 rdf:type rdfs:Class;
  rdfs:label "Correction_Parameter";
  pds4:subClassOf pds4:urn:nasa:pds:0001_nasa_pds_1:all:user:img:list_index_no_units_imaging::1.0;
  rdfs:comment " The Correction_Parameter class specifies identifier(s) and value for a data correction parameter applicable to the parent class.".
 
pds4:urn:nasa:pds:0001_nasa_pds_1:all:user:cart:cylindrical::1.0 rdf:type rdfs:Class;
  rdfs:label "Cylindrical";
  pds4:subClassOf pds4:urn:nasa:pds:0001_nasa_pds_1:all:user::1.0;
  rdfs:comment "This is an in-situ projection used for (non-stereo) panoramas. Each image row represents a constant elevation and each image column represents a constant azimuth, from a given point of view. The image scale in degrees per pixel is constant across the image.".
 
pds4:urn:nasa:pds:0001_nasa_pds_1:all:user:cart:cylindrical_perspective::1.0 rdf:type rdfs:Class;
  rdfs:label "Cylindrical_Perspective";
  pds4:subClassOf pds4:urn:nasa:pds:0001_nasa_pds_1:all:user::1.0;
  rdfs:comment "This is an in-situ projection that is a hybrid. Each column is a vertical slice from a pinhole camera (Perspective projection), while the columns are spaced evenly in azimuth (Cylindrical projection). It is most useful for viewing panoramas in stereo.".
 
pds4:urn:nasa:pds:0001_nasa_pds_1:pds:tagged_nondigital_child:pds:dd_associate_external_class::1.0 rdf:type rdfs:Class;
  rdfs:label "DD_Associate_External_Class";
  pds4:subClassOf pds4:urn:nasa:pds:0001_nasa_pds_1:all:user:pds:tagged_nondigital_child::1.0;
  rdfs:comment "The DD_Associate_External_Class class allows the definition of permissible values in Ingest_LDD for attributes defined in external namespaces.".
 
pds4:urn:nasa:pds:0001_nasa_pds_1:pds:tagged_nondigital_child:pds:dd_association::1.0 rdf:type rdfs:Class;
  rdfs:label "DD_Association";
  pds4:subClassOf pds4:urn:nasa:pds:0001_nasa_pds_1:all:user:pds:tagged_nondigital_child::1.0;
  rdfs:comment "The DD_Association class defines the association between two classes or a class and an attribute in a data dictionary.".
 
pds4:urn:nasa:pds:0001_nasa_pds_1:pds:tagged_nondigital_child:pds:dd_association_external::1.0 rdf:type rdfs:Class;
  rdfs:label "DD_Association_External";
  pds4:subClassOf pds4:urn:nasa:pds:0001_nasa_pds_1:all:user:pds:tagged_nondigital_child::1.0;
  rdfs:comment "The DD_Association_External class defines the association between classes and attributes within the local data dictionary and those external to the local data dictionary.".
 
pds4:urn:nasa:pds:0001_nasa_pds_1:pds:tndo_supplemental:pds:dd_attribute::1.0 rdf:type rdfs:Class;
  rdfs:label "DD_Attribute";
  pds4:subClassOf pds4:urn:nasa:pds:0001_nasa_pds_1:pds:tagged_nondigital_object:pds:tndo_supplemental::1.0;
  rdfs:comment "The DD_Attribute class defines an attribute for a data dictionary.".
 
pds4:urn:nasa:pds:0001_nasa_pds_1:pds:tndo_supplemental:pds:dd_attribute_full::1.0 rdf:type rdfs:Class;
  rdfs:label "DD_Attribute_Full";
  pds4:subClassOf pds4:urn:nasa:pds:0001_nasa_pds_1:pds:tagged_nondigital_object:pds:tndo_supplemental::1.0;
  rdfs:comment "The DD_Attribute_Full class provides a more complete definition of an attribute in the data dictionary.".
 
pds4:urn:nasa:pds:0001_nasa_pds_1:pds:tndo_supplemental:pds:dd_attribute_full:pds3::1.0 rdf:type rdfs:Class;
  rdfs:label "PDS3";
  rdfs:subClassOf pds4:urn:nasa:pds:0001_nasa_pds_1:pds:tndo_supplemental:pds:dd_attribute_full::1.0;
  rdfs:comment "The attribute definition originated under PDS3".
 
pds4:urn:nasa:pds:0001_nasa_pds_1:pds:tndo_supplemental:pds:dd_attribute_full:pds4::1.0 rdf:type rdfs:Class;
  rdfs:label "PDS4";
  rdfs:subClassOf pds4:urn:nasa:pds:0001_nasa_pds_1:pds:tndo_supplemental:pds:dd_attribute_full::1.0;
  rdfs:comment "The attribute definition originated under PDS4".
 
pds4:urn:nasa:pds:0001_nasa_pds_1:pds:tagged_nondigital_child:pds:dd_attribute_reference::1.0 rdf:type rdfs:Class;
  rdfs:label "DD_Attribute_Reference";
  pds4:subClassOf pds4:urn:nasa:pds:0001_nasa_pds_1:all:user:pds:tagged_nondigital_child::1.0;
  rdfs:comment "The DD Attribute Reference class provides a reference to an attribute using a namespace identifier and the attribute name.".
 
pds4:urn:nasa:pds:0001_nasa_pds_1:pds:tndo_supplemental:pds:dd_class::1.0 rdf:type rdfs:Class;
  rdfs:label "DD_Class";
  pds4:subClassOf pds4:urn:nasa:pds:0001_nasa_pds_1:pds:tagged_nondigital_object:pds:tndo_supplemental::1.0;
  rdfs:comment "The DD_Class class defines a class for a data dictionary.".
 
pds4:urn:nasa:pds:0001_nasa_pds_1:pds:tndo_supplemental:pds:dd_class_full::1.0 rdf:type rdfs:Class;
  rdfs:label "DD_Class_Full";
  pds4:subClassOf pds4:urn:nasa:pds:0001_nasa_pds_1:pds:tagged_nondigital_object:pds:tndo_supplemental::1.0;
  rdfs:comment "The DD_Class_Full class provides a more complete definition of a class for a data dictionary.".
 
pds4:urn:nasa:pds:0001_nasa_pds_1:pds:tndo_supplemental:pds:dd_class_full:pds3::1.0 rdf:type rdfs:Class;
  rdfs:label "PDS3";
  rdfs:subClassOf pds4:urn:nasa:pds:0001_nasa_pds_1:pds:tndo_supplemental:pds:dd_class_full::1.0;
  rdfs:comment "The class definition originated under PDS3".
 
pds4:urn:nasa:pds:0001_nasa_pds_1:pds:tndo_supplemental:pds:dd_class_full:pds4::1.0 rdf:type rdfs:Class;
  rdfs:label "PDS4";
  rdfs:subClassOf pds4:urn:nasa:pds:0001_nasa_pds_1:pds:tndo_supplemental:pds:dd_class_full::1.0;
  rdfs:comment "The class definition originated under PDS4".
 
pds4:urn:nasa:pds:0001_nasa_pds_1:pds:tagged_nondigital_child:pds:dd_class_reference::1.0 rdf:type rdfs:Class;
  rdfs:label "DD_Class_Reference";
  pds4:subClassOf pds4:urn:nasa:pds:0001_nasa_pds_1:all:user:pds:tagged_nondigital_child::1.0;
  rdfs:comment "The DD Class Reference class provides a reference to a class using a namespace identifier and the class name.".
 
pds4:urn:nasa:pds:0001_nasa_pds_1:pds:tagged_nondigital_child:pds:dd_context_value_list::1.0 rdf:type rdfs:Class;
  rdfs:label "DD_Context_Value_List";
  pds4:subClassOf pds4:urn:nasa:pds:0001_nasa_pds_1:all:user:pds:tagged_nondigital_child::1.0;
  rdfs:comment "The DD_Context_Value_List class identifies an attribute and its relative xpath for the definition of permissible values and their meanings.".
 
pds4:urn:nasa:pds:0001_nasa_pds_1:pds:tagged_nondigital_child:pds:dd_permissible_value::1.0 rdf:type rdfs:Class;
  rdfs:label "DD_Permissible_Value";
  pds4:subClassOf pds4:urn:nasa:pds:0001_nasa_pds_1:all:user:pds:tagged_nondigital_child::1.0;
  rdfs:comment "The DD_Permissible_Value class lists permissible values and their meanings.".
 
pds4:urn:nasa:pds:0001_nasa_pds_1:pds:tagged_nondigital_child:pds:dd_permissible_value_full::1.0 rdf:type rdfs:Class;
  rdfs:label "DD_Permissible_Value_Full";
  pds4:subClassOf pds4:urn:nasa:pds:0001_nasa_pds_1:all:user:pds:tagged_nondigital_child::1.0;
  rdfs:comment "The DD_Permissible_Value_Full class lists permissible values, their meanings, and the dates when active.".
 
pds4:urn:nasa:pds:0001_nasa_pds_1:pds:tndo_supplemental:pds:dd_rule::1.0 rdf:type rdfs:Class;
  rdfs:label "DD_Rule";
  pds4:subClassOf pds4:urn:nasa:pds:0001_nasa_pds_1:pds:tagged_nondigital_object:pds:tndo_supplemental::1.0;
  rdfs:comment "The DD_Rule class defines a Schematron rule for a data dictionary.".
 
pds4:urn:nasa:pds:0001_nasa_pds_1:pds:tndo_supplemental:pds:dd_rule_statement::1.0 rdf:type rdfs:Class;
  rdfs:label "DD_Rule_Statement";
  pds4:subClassOf pds4:urn:nasa:pds:0001_nasa_pds_1:pds:tagged_nondigital_object:pds:tndo_supplemental::1.0;
  rdfs:comment "The DD_Rule_Statement class defines a Schematron rule statement.".
 
pds4:urn:nasa:pds:0001_nasa_pds_1:pds:tagged_nondigital_child:pds:dd_value_domain::1.0 rdf:type rdfs:Class;
  rdfs:label "DD_Value_Domain";
  pds4:subClassOf pds4:urn:nasa:pds:0001_nasa_pds_1:all:user:pds:tagged_nondigital_child::1.0;
  rdfs:comment "The DD_Value_Domain class defines an attribute\\'s permissible values and their constraints.".
 
pds4:urn:nasa:pds:0001_nasa_pds_1:pds:tagged_nondigital_child:pds:dd_value_domain_full::1.0 rdf:type rdfs:Class;
  rdfs:label "DD_Value_Domain_Full";
  pds4:subClassOf pds4:urn:nasa:pds:0001_nasa_pds_1:all:user:pds:tagged_nondigital_child::1.0;
  rdfs:comment "The DD_Value_Domain_Full class provides a more complete definition of a attribute\\'s value domain.".
 
pds4:urn:nasa:pds:0001_nasa_pds_1:pds:information_package:pds:dip_deep_archive::1.0 rdf:type rdfs:Class;
  rdfs:label "DIP_Deep_Archive";
  pds4:subClassOf pds4:urn:nasa:pds:0001_nasa_pds_1:pds:tndo_supplemental:pds:information_package::1.0;
  rdfs:comment "The Dissemination Information Package Deep Archive class is an Information Package derived from one or more AIPs and is received by the National Space Science Data Center (NSSDC).".
 
pds4:urn:nasa:pds:0001_nasa_pds_1:img:data_processing:img:dark_current_correction::1.0 rdf:type rdfs:Class;
  rdfs:label "Dark_Current_Correction";
  pds4:subClassOf pds4:urn:nasa:pds:0001_nasa_pds_1:all:user:img:data_processing::1.0;
  rdfs:comment "Specifies how dark current removal was performed on this image.".
 
pds4:urn:nasa:pds:0001_nasa_pds_1:all:user:img:data_processing::1.0 rdf:type rdfs:Class;
  rdfs:label "Data_Processing";
  pds4:subClassOf pds4:urn:nasa:pds:0001_nasa_pds_1:all:user::1.0;
  rdfs:comment "The Data_Processing class contains attributes describing how processing and\\//or calibration was performed on a data product. It is not intended to be used on its own; rather it is intended to be extended by classes specific to a particular type of processing, such as Shutter_Subtraction, Flat_Field_Correction, Companding, etc. The attributes of this class thus become attributes of the extension class. ".
 
pds4:urn:nasa:pds:0001_nasa_pds_1:all:user:img:data_processing_file::1.0 rdf:type rdfs:Class;
  rdfs:label "Data_Processing_File";
  pds4:subClassOf pds4:urn:nasa:pds:0001_nasa_pds_1:all:user::1.0;
  rdfs:comment "The Data_Processing_File class contain attributes which identify a file containing calibration data that was applied to the science data. It is not intended to be used on its own; rather it is intended to be extended by classes specific to a particular type of file, such as Flat_Field_File. Note that the \"name\" attribute is the name of the file; this attribute should only be used if the file is either not included in an archive, or if the delivery status is unknown by the data provider. The External_Reference or Internal_Reference class should be used instead of name if at all possible.".
 
pds4:urn:nasa:pds:0001_nasa_pds_1:pds:tndo_context_pds3:pds:data_set_pds3::1.0 rdf:type rdfs:Class;
  rdfs:label "Data_Set_PDS3";
  pds4:subClassOf pds4:urn:nasa:pds:0001_nasa_pds_1:pds:tagged_nondigital_object:pds:tndo_context_pds3::1.0;
  rdfs:comment "The Data Set PDS3 class is used to capture the data set information from the PDS3 Data Set Catalog.".
 
pds4:urn:nasa:pds:0001_nasa_pds_1:all:user:geom:derived_geometry::1.0 rdf:type rdfs:Class;
  rdfs:label "Derived_Geometry";
  pds4:subClassOf pds4:urn:nasa:pds:0001_nasa_pds_1:all:user::1.0;
  rdfs:comment "The Derived_Geometry class is a container for surface based observations (lander or rover). It is used to provide some geometric quantities relative to a specific Reference Coordinate Space. ".
 
pds4:urn:nasa:pds:0001_nasa_pds_1:all:user:img_surface:derived_product_parameters::1.0 rdf:type rdfs:Class;
  rdfs:label "Derived_Product_Parameters";
  pds4:subClassOf pds4:urn:nasa:pds:0001_nasa_pds_1:all:user::1.0;
  rdfs:comment "The Derived_Product_Parameters class contains attributes used to identify and describe processing performed on products in order to produce a higher level product.".
 
pds4:urn:nasa:pds:0001_nasa_pds_1:all:user:img:detector::1.0 rdf:type rdfs:Class;
  rdfs:label "Detector";
  pds4:subClassOf pds4:urn:nasa:pds:0001_nasa_pds_1:all:user::1.0;
  rdfs:comment "The Detector class contains attributes describing the state of the instrument detector. These are values directly read from the detector and do not necessarily reflect the state of the image after onboard processing. For example, the entire image may be read into memory and then subframed in software, in which case the subframe attributes in this class reflect the entire image (as read from the detector), whereas those in the Subframe class represent the final subframe results.".
 
pds4:urn:nasa:pds:0001_nasa_pds_1:all:user:nucspec:detector::1.0 rdf:type rdfs:Class;
  rdfs:label "Detector";
  pds4:subClassOf pds4:urn:nasa:pds:0001_nasa_pds_1:all:user::1.0;
  rdfs:comment "Specifies a single detector which was active at the time of observation.".
 
pds4:urn:nasa:pds:0001_nasa_pds_1:all:user:nucspec:detectors::1.0 rdf:type rdfs:Class;
  rdfs:label "Detectors";
  pds4:subClassOf pds4:urn:nasa:pds:0001_nasa_pds_1:all:user::1.0;
  rdfs:comment "Specifies which detectors were active on an instrument at the time of observation.".
 
pds4:urn:nasa:pds:0001_nasa_pds_1:all:user:geom:device_angle::1.0 rdf:type rdfs:Class;
  rdfs:label "Device_Angle";
  pds4:subClassOf pds4:urn:nasa:pds:0001_nasa_pds_1:all:user::1.0;
  rdfs:comment "The Device_Angle class is a container for the set of angles between the various components or devices of the spacecraft. ".
 
pds4:urn:nasa:pds:0001_nasa_pds_1:geom:list_index_angle:geom:device_angle_index::1.0 rdf:type rdfs:Class;
  rdfs:label "Device_Angle_Index";
  pds4:subClassOf pds4:urn:nasa:pds:0001_nasa_pds_1:geom:list_index_base:geom:list_index_angle::1.0;
  rdfs:comment "The Device_Angle class is a container for the set of angles the spacecraft device specified in the parent Articulation_Device_Parameters class. ".
 
pds4:urn:nasa:pds:0001_nasa_pds_1:all:user:geom:device_component_state::1.0 rdf:type rdfs:Class;
  rdfs:label "Device_Component_State";
  pds4:subClassOf pds4:urn:nasa:pds:0001_nasa_pds_1:all:user::1.0;
  rdfs:comment "The Device_Component_State class is a container for the states of the various components of the articulation device. ".
 
pds4:urn:nasa:pds:0001_nasa_pds_1:img:device_parameters:img:device_component_state::1.0 rdf:type rdfs:Class;
  rdfs:label "Device_Component_State";
  pds4:subClassOf pds4:urn:nasa:pds:0001_nasa_pds_1:all:user:img:device_parameters::1.0;
  rdfs:comment "The Device_Component_State class describes the state of one component of an imaging instrument or other imaging device. The meaning of \"state\" is device-specific.".
 
pds4:urn:nasa:pds:0001_nasa_pds_1:geom:list_index_text:geom:device_component_state_index::1.0 rdf:type rdfs:Class;
  rdfs:label "Device_Component_State_Index";
  pds4:subClassOf pds4:urn:nasa:pds:0001_nasa_pds_1:geom:list_index_base:geom:list_index_text::1.0;
  rdfs:comment "The Device_Component_State_Index class is a container for one state of a component of the articulation device. ".
 
pds4:urn:nasa:pds:0001_nasa_pds_1:all:user:img:device_component_states::1.0 rdf:type rdfs:Class;
  rdfs:label "Device_Component_States";
  pds4:subClassOf pds4:urn:nasa:pds:0001_nasa_pds_1:all:user::1.0;
  rdfs:comment "The Device_Component_States class provides a container for the set of states of a component of an imaging instrument or other imaging device.".
 
pds4:urn:nasa:pds:0001_nasa_pds_1:img:device_parameters:img:device_current::1.0 rdf:type rdfs:Class;
  rdfs:label "Device_Current";
  pds4:subClassOf pds4:urn:nasa:pds:0001_nasa_pds_1:all:user:img:device_parameters::1.0;
  rdfs:comment "The Device_Current class provides the current of some point on an imaging instrument or other imaging device.".
 
pds4:urn:nasa:pds:0001_nasa_pds_1:all:user:img:device_currents::1.0 rdf:type rdfs:Class;
  rdfs:label "Device_Currents";
  pds4:subClassOf pds4:urn:nasa:pds:0001_nasa_pds_1:all:user::1.0;
  rdfs:comment "The Device_Currents class provides a container for the set of currents of an imaging instrument or other imaging device.".
 
pds4:urn:nasa:pds:0001_nasa_pds_1:img:device_parameters:img:device_motor_count::1.0 rdf:type rdfs:Class;
  rdfs:label "Device_Motor_Count";
  pds4:subClassOf pds4:urn:nasa:pds:0001_nasa_pds_1:all:user:img:device_parameters::1.0;
  rdfs:comment "The Device_Motor_Count class describes the raw motor count of one actuator on an imaging instrument or other imaging device (such as a filter wheel, focus motor, or zoom motor). This information should typically be reported in a more specific and useable form in other classes, such as a filter number or wavelength in the Optical_Filter class or a focus distnace in the Focus class.".
 
pds4:urn:nasa:pds:0001_nasa_pds_1:all:user:geom:device_motor_counts::1.0 rdf:type rdfs:Class;
  rdfs:label "Device_Motor_Counts";
  pds4:subClassOf pds4:urn:nasa:pds:0001_nasa_pds_1:all:user::1.0;
  rdfs:comment "The Device_Motor_Counts class is a container for the classes that describe the motor step count information for device components. ".
 
pds4:urn:nasa:pds:0001_nasa_pds_1:all:user:img:device_motor_counts::1.0 rdf:type rdfs:Class;
  rdfs:label "Device_Motor_Counts";
  pds4:subClassOf pds4:urn:nasa:pds:0001_nasa_pds_1:all:user::1.0;
  rdfs:comment "The Device_Motor_Counts class provides a container for the set of raw motor counts of actuators on an imaging instrument or other imaging device (such as a filter wheel, focus motor, or zoom motor).".
 
pds4:urn:nasa:pds:0001_nasa_pds_1:geom:list_index_no_units:geom:device_motor_counts_index::1.0 rdf:type rdfs:Class;
  rdfs:label "Device_Motor_Counts_Index";
  pds4:subClassOf pds4:urn:nasa:pds:0001_nasa_pds_1:geom:list_index_base:geom:list_index_no_units::1.0;
  rdfs:comment "The Device_Motor_Counts_Index class is a container for the attributes that describe the motor step count information for a single motor on a device. ".
 
pds4:urn:nasa:pds:0001_nasa_pds_1:all:user:img:device_parameters::1.0 rdf:type rdfs:Class;
  rdfs:label "Device_Parameters";
  pds4:subClassOf pds4:urn:nasa:pds:0001_nasa_pds_1:all:user::1.0;
  rdfs:comment "The Device_Parameters class identifies where a measurement was made. It may refer to an individual imaging instrument, imaging instrument device, or some defined point on the instrument or device. The class is intended to be extended (for example, by Device_Temperature) to add the associated measurement rather than being used directly.".
 
pds4:urn:nasa:pds:0001_nasa_pds_1:all:user:geom:device_pose::1.0 rdf:type rdfs:Class;
  rdfs:label "Device_Pose";
  pds4:subClassOf pds4:urn:nasa:pds:0001_nasa_pds_1:all:user::1.0;
  rdfs:comment "Defines the pose of this articulation device. The name indicates what exactly is being measured and how, and disambiguates if there is more than one Device_Pose. For example, Mars 2020 has \"arm_attitude_reference\", which indicates the pose of the rover that was used to calculate gravity droop of the arm. The interpretation of the pose is mission-specific; see the mission documentation.".
 
pds4:urn:nasa:pds:0001_nasa_pds_1:all:user:geom:device_temperature::1.0 rdf:type rdfs:Class;
  rdfs:label "Device_Temperature";
  pds4:subClassOf pds4:urn:nasa:pds:0001_nasa_pds_1:all:user::1.0;
  rdfs:comment "The Device_Temperature class is a container for all available device temperatures of an articulated device and\\//or part(s) of a device. ".
 
pds4:urn:nasa:pds:0001_nasa_pds_1:img:device_parameters:img:device_temperature::1.0 rdf:type rdfs:Class;
  rdfs:label "Device_Temperature";
  pds4:subClassOf pds4:urn:nasa:pds:0001_nasa_pds_1:all:user:img:device_parameters::1.0;
  rdfs:comment "The Device_Temperature class provides a container for the temperature of some point on an imaging instrument or other imaging device. ".
 
pds4:urn:nasa:pds:0001_nasa_pds_1:geom:list_index_temperature:geom:device_temperature_index::1.0 rdf:type rdfs:Class;
  rdfs:label "Device_Temperature_Index";
  pds4:subClassOf pds4:urn:nasa:pds:0001_nasa_pds_1:geom:list_index_base:geom:list_index_temperature::1.0;
  rdfs:comment "The Device_Temperature_Index class specifies the attributes describing the temperature of one device or some part of a device. ".
 
pds4:urn:nasa:pds:0001_nasa_pds_1:all:user:img:device_temperatures::1.0 rdf:type rdfs:Class;
  rdfs:label "Device_Temperatures";
  pds4:subClassOf pds4:urn:nasa:pds:0001_nasa_pds_1:all:user::1.0;
  rdfs:comment "The Device_Temperatures class provides a container for the set of temperatures of an imaging instrument or other imaging device. ".
 
pds4:urn:nasa:pds:0001_nasa_pds_1:img:device_parameters:img:device_voltage::1.0 rdf:type rdfs:Class;
  rdfs:label "Device_Voltage";
  pds4:subClassOf pds4:urn:nasa:pds:0001_nasa_pds_1:all:user:img:device_parameters::1.0;
  rdfs:comment "The Device_Voltage class provides the voltage of some point on an imaging instrument or other imaging device. ".
 
pds4:urn:nasa:pds:0001_nasa_pds_1:all:user:img:device_voltages::1.0 rdf:type rdfs:Class;
  rdfs:label "Device_Voltages";
  pds4:subClassOf pds4:urn:nasa:pds:0001_nasa_pds_1:all:user::1.0;
  rdfs:comment "The Device_Voltage class provides a container for the set of voltages of an imaging instrument or other imaging device.".
 
pds4:urn:nasa:pds:0001_nasa_pds_1:pds:product_components:pds:discipline_area::1.0 rdf:type rdfs:Class;
  rdfs:label "Discipline_Area";
  pds4:subClassOf pds4:urn:nasa:pds:0001_nasa_pds_1:all:user:pds:product_components::1.0;
  rdfs:comment "The Discipline area allows the insertion of discipline specific metadata.".
 
pds4:urn:nasa:pds:0001_nasa_pds_1:pds:product_components:pds:discipline_facets::1.0 rdf:type rdfs:Class;
  rdfs:label "Discipline_Facets";
  pds4:subClassOf pds4:urn:nasa:pds:0001_nasa_pds_1:all:user:pds:product_components::1.0;
  rdfs:comment "The Discipline_Facets class contains the discipline-related search facets.  It is required and may not be repeated. Note that Science_Facets was modeled with Discipline_Facets as a component and Discipline_Facets was modeled with Group_Facet1 and Group_Facet2 as components. This dependency hierarchy was flattened and only Science_Facets exists in the schema.".
 
pds4:urn:nasa:pds:0001_nasa_pds_1:pds:tndo_supplemental:pds:display_2d_image::1.0 rdf:type rdfs:Class;
  rdfs:label "Display_2D_Image";
  pds4:subClassOf pds4:urn:nasa:pds:0001_nasa_pds_1:pds:tagged_nondigital_object:pds:tndo_supplemental::1.0;
  rdfs:comment "The Display_2D_Image class provides attributes to enable the display of a 2 dimensional image.".
 
pds4:urn:nasa:pds:0001_nasa_pds_1:all:user:disp:display_direction::1.0 rdf:type rdfs:Class;
  rdfs:label "Display_Direction";
  pds4:subClassOf pds4:urn:nasa:pds:0001_nasa_pds_1:all:user::1.0;
  rdfs:comment "The Display_Direction class specifies how two of the dimensions of an Array object should be displayed in the vertical (line) and horizontal (sample) dimensions of a display device.".
 
pds4:urn:nasa:pds:0001_nasa_pds_1:all:user:geom:display_direction::1.0 rdf:type rdfs:Class;
  rdfs:label "Display_Direction";
  pds4:subClassOf pds4:urn:nasa:pds:0001_nasa_pds_1:all:user::1.0;
  rdfs:comment "The Display_Direction class specifies which two of the dimensions of an Array object should be displayed and how they should be displayed in the vertical (line) and horizontal (sample) dimensions of a display device. This class is essentially the same as the class of the same name in the Display Dictionary, and is redefined here for convenience. ".
 
pds4:urn:nasa:pds:0001_nasa_pds_1:all:user:rings:display_direction::1.0 rdf:type rdfs:Class;
  rdfs:label "Display_Direction";
  pds4:subClassOf pds4:urn:nasa:pds:0001_nasa_pds_1:all:user::1.0;
  rdfs:comment "The Display_Direction class specifies which two of the dimensions of an Array object should be displayed and how they should be displayed in the vertical (line) and horizontal (sample) dimensions of a display device. This class is a modification of the corresponding class in the Display Dictionary, and is redefined here for convenience. The local_identifier_reference is used to identify the array or arrays to which this iteration of the class applies. Multiple entries are permitted the settings in the iteration of Display_Direction apply to all of the referenced arrays. ".
 
pds4:urn:nasa:pds:0001_nasa_pds_1:all:user:disp:display_settings::1.0 rdf:type rdfs:Class;
  rdfs:label "Display_Settings";
  pds4:subClassOf pds4:urn:nasa:pds:0001_nasa_pds_1:all:user::1.0;
  rdfs:comment "The Display_Settings class contains one or more classes describing how data should be displayed on a display device.".
 
pds4:urn:nasa:pds:0001_nasa_pds_1:pds:information_package:pds:dissemination_information_package::1.0 rdf:type rdfs:Class;
  rdfs:label "Dissemination_Information_Package";
  pds4:subClassOf pds4:urn:nasa:pds:0001_nasa_pds_1:pds:tndo_supplemental:pds:information_package::1.0;
  rdfs:comment "The Dissemination Information Package (DIP) class defines an Information Package, derived from one or more AIPs, that is received by a consumer.".
 
pds4:urn:nasa:pds:0001_nasa_pds_1:all:user:geom:distance_generic::1.0 rdf:type rdfs:Class;
  rdfs:label "Distance_Generic";
  pds4:subClassOf pds4:urn:nasa:pds:0001_nasa_pds_1:all:user::1.0;
  rdfs:comment "The distance between the two objects, both of which must be specified. ".
 
pds4:urn:nasa:pds:0001_nasa_pds_1:all:user:cart:distance_and_bearing_representation::1.0 rdf:type rdfs:Class;
  rdfs:label "Distance_and_Bearing_Representation";
  pds4:subClassOf pds4:urn:nasa:pds:0001_nasa_pds_1:all:user::1.0;
  rdfs:comment "The Distance_and_Bearing_Representation class provides a method of encoding the position of a point by measuring its distance and direction (azimuth angle) from another point.".
 
pds4:urn:nasa:pds:0001_nasa_pds_1:all:user:geom:distances::1.0 rdf:type rdfs:Class;
  rdfs:label "Distances";
  pds4:subClassOf pds4:urn:nasa:pds:0001_nasa_pds_1:all:user::1.0;
  rdfs:comment "The Distances class is a container of distance classes. ".
 
pds4:urn:nasa:pds:0001_nasa_pds_1:all:user:geom:distances_min_max::1.0 rdf:type rdfs:Class;
  rdfs:label "Distances_Min_Max";
  pds4:subClassOf pds4:urn:nasa:pds:0001_nasa_pds_1:all:user::1.0;
  rdfs:comment "The Distances_Min_Max class is a container class for named distances given as minimum-maximum pairs. For distance, if either the minimum or maximum parameter is given, both must be provided. ".
 
pds4:urn:nasa:pds:0001_nasa_pds_1:all:user:geom:distances_specific::1.0 rdf:type rdfs:Class;
  rdfs:label "Distances_Specific";
  pds4:subClassOf pds4:urn:nasa:pds:0001_nasa_pds_1:all:user::1.0;
  rdfs:comment "The Distances_Specific class is a container class for specific distances defined in this dictionary. ".
 
pds4:urn:nasa:pds:0001_nasa_pds_1:all:user:geom:distances_start_stop::1.0 rdf:type rdfs:Class;
  rdfs:label "Distances_Start_Stop";
  pds4:subClassOf pds4:urn:nasa:pds:0001_nasa_pds_1:all:user::1.0;
  rdfs:comment "The Distances_Start_Stop class is a container class for named distances given as pairs corresponding to the beginning and end of the observation. For a distance, if either the start or stop parameter is given, both must be provided. If any values from this class are included in the label, the parameters geometry_start_time_utc and geometry_stop_time_utc must be given in the enclosing Geometry_Orbiter class. ".
 
pds4:urn:nasa:pds:0001_nasa_pds_1:pds:tndo_supplemental:pds:document::1.0 rdf:type rdfs:Class;
  rdfs:label "Document";
  pds4:subClassOf pds4:urn:nasa:pds:0001_nasa_pds_1:pds:tagged_nondigital_object:pds:tndo_supplemental::1.0;
  rdfs:comment "The Document class describes a document.".
 
pds4:urn:nasa:pds:0001_nasa_pds_1:pds:tagged_nondigital_child:pds:document_edition::1.0 rdf:type rdfs:Class;
  rdfs:label "Document_Edition";
  pds4:subClassOf pds4:urn:nasa:pds:0001_nasa_pds_1:all:user:pds:tagged_nondigital_child::1.0;
  rdfs:comment "A Document Edition is one complete version of the document in a set of files that is distinguished by language, a unique assemblage of file formats, or some other criteria.".
 
pds4:urn:nasa:pds:0001_nasa_pds_1:pds:file:pds:document_file::1.0 rdf:type rdfs:Class;
  rdfs:label "Document_File";
  pds4:subClassOf pds4:urn:nasa:pds:0001_nasa_pds_1:pds:tagged_digital_object:pds:file::1.0;
  rdfs:comment "The Document File class describes a file which is a part of a document.".
 
pds4:urn:nasa:pds:0001_nasa_pds_1:img:data_processing:img:downsampling::1.0 rdf:type rdfs:Class;
  rdfs:label "Downsampling";
  pds4:subClassOf pds4:urn:nasa:pds:0001_nasa_pds_1:all:user:img:data_processing::1.0;
  rdfs:comment " The Downsampling class describes whether or not downsampling occurred, the venue where it occurred (Software or Hardware), the method used to downsample, and the pixel averaging dimensions. A downsampled image is a smaller version of the image, resulting in reduced resolution of the same coverage area. The processing_algorithm attribute specifies the pixel resolution downsample method used. This varies by mission, but examples from MSL include: \\'Mean\\' - Downsampling done in software by calculation of the mean., \\'Conditional\\' - Use hardware binning if downsampling (by mean calculation) and subframe arguments are consistent.".
 
pds4:urn:nasa:pds:0001_nasa_pds_1:pds:tagged_digital_child:pds:element_array::1.0 rdf:type rdfs:Class;
  rdfs:label "Element_Array";
  pds4:subClassOf pds4:urn:nasa:pds:0001_nasa_pds_1:all:user:pds:tagged_digital_child::1.0;
  rdfs:comment "The Element Array class is used as a component of the array class and defines an element of the array.".
 
pds4:urn:nasa:pds:0001_nasa_pds_1:pds:encoded_byte_stream:pds:encoded_audio::1.0 rdf:type rdfs:Class;
  rdfs:label "Encoded_Audio";
  pds4:subClassOf pds4:urn:nasa:pds:0001_nasa_pds_1:pds:byte_stream:pds:encoded_byte_stream::1.0;
  rdfs:comment "The Encoded_Audio class is used for files containing audio data in standard formats, such as WAV.".
 
pds4:urn:nasa:pds:0001_nasa_pds_1:pds:encoded_byte_stream:pds:encoded_binary::1.0 rdf:type rdfs:Class;
  rdfs:label "Encoded_Binary";
  pds4:subClassOf pds4:urn:nasa:pds:0001_nasa_pds_1:pds:byte_stream:pds:encoded_byte_stream::1.0;
  rdfs:comment "The Encoded Binary class describes a binary encoded byte stream. This class is used to describe files in the repository that are being registered using  Product_File_Repository.".
 
pds4:urn:nasa:pds:0001_nasa_pds_1:pds:byte_stream:pds:encoded_byte_stream::1.0 rdf:type rdfs:Class;
  rdfs:label "Encoded_Byte_Stream";
  pds4:subClassOf pds4:urn:nasa:pds:0001_nasa_pds_1:pds:tagged_digital_object:pds:byte_stream::1.0;
  rdfs:comment "The Encoded Byte Stream class defines byte streams that must be decoded by software before use. These byte streams must only use standard encodings. The Encoded Byte Stream class is the parent class for all encoded byte streams.".
 
pds4:urn:nasa:pds:0001_nasa_pds_1:pds:encoded_byte_stream:pds:encoded_header::1.0 rdf:type rdfs:Class;
  rdfs:label "Encoded_Header";
  pds4:subClassOf pds4:urn:nasa:pds:0001_nasa_pds_1:pds:byte_stream:pds:encoded_byte_stream::1.0;
  rdfs:comment "The Encoded Header class describes a header that has been encoded using an encoding scheme that is compliant to an external standard.".
 
pds4:urn:nasa:pds:0001_nasa_pds_1:pds:encoded_byte_stream:pds:encoded_image::1.0 rdf:type rdfs:Class;
  rdfs:label "Encoded_Image";
  pds4:subClassOf pds4:urn:nasa:pds:0001_nasa_pds_1:pds:byte_stream:pds:encoded_byte_stream::1.0;
  rdfs:comment "The Encoded Image class is used for ancillary images in standard formats, such as JPEG.".
 
pds4:urn:nasa:pds:0001_nasa_pds_1:pds:encoded_byte_stream:pds:encoded_native::1.0 rdf:type rdfs:Class;
  rdfs:label "Encoded_Native";
  pds4:subClassOf pds4:urn:nasa:pds:0001_nasa_pds_1:pds:byte_stream:pds:encoded_byte_stream::1.0;
  rdfs:comment "The Encoded Native class describes a binary encoded byte stream. This class is used to describe data objects for Product_Native.".
 
pds4:urn:nasa:pds:0001_nasa_pds_1:all:user:nucspec:energy_calibration::1.0 rdf:type rdfs:Class;
  rdfs:label "Energy_Calibration";
  pds4:subClassOf pds4:urn:nasa:pds:0001_nasa_pds_1:all:user::1.0;
  rdfs:comment "Specifies methods and data used to determine the pulse height in energy units (e.g. MeV) for each channel of a pulse height spectrum.".
 
pds4:urn:nasa:pds:0001_nasa_pds_1:geom:polynomial_coefficients_3:geom:entrance_terms::1.0 rdf:type rdfs:Class;
  rdfs:label "Entrance_Terms";
  pds4:subClassOf pds4:urn:nasa:pds:0001_nasa_pds_1:all:user:geom:polynomial_coefficients_3::1.0;
  rdfs:comment "The Entrance_Terms contains the coefficients of a polynomial function used to model movement of the entrance pupil. ".
 
pds4:urn:nasa:pds:0001_nasa_pds_1:all:user:cart:equirectangular::1.0 rdf:type rdfs:Class;
  rdfs:label "Equirectangular";
  pds4:subClassOf pds4:urn:nasa:pds:0001_nasa_pds_1:all:user::1.0;
  rdfs:comment "The Equirectangular class contains parameters for the Equirectangular map projection. Synder 1987, DOI:10.3133\\//pp1395, page 90: https:\\//\\//pubs.usgs.gov\\//pp\\//1395\\//report.pdf#page=102 PROJ: https:\\//\\//proj.org\\//operations\\//projections\\//eqc.html forward: x = R * (lambda - lambda_0) * cos(phi_1) y = R * (phi - phi_1) and reverse: lambda = (x \\// R cos(phi_1)) + lambda_0 phi = (y \\// R) + phi_1 where: lambda is the longitude of the location to project on the body; phi is the latitude of the location to project on the body; phi_1 is the standard parallel (north and south of the equator) where the scale of the projection is true; lambda_0 is the central meridian of the map; x is the horizontal coordinate of the projected location on the map; y is the vertical coordinate of the projected location on the map; R is the radius of the body. ".
 
pds4:urn:nasa:pds:0001_nasa_pds_1:all:user:img_surface:error_model::1.0 rdf:type rdfs:Class;
  rdfs:label "Error_Model";
  pds4:subClassOf pds4:urn:nasa:pds:0001_nasa_pds_1:all:user::1.0;
  rdfs:comment "The Error_Model class specifies the name of the error model used, a reference to the algorithm descriptions, and the parameters needed for that algorithm. The specific set of values is determined by each individual missions.".
 
pds4:urn:nasa:pds:0001_nasa_pds_1:all:user:img_surface:error_model_parameter::1.0 rdf:type rdfs:Class;
  rdfs:label "Error_Model_Parameter";
  pds4:subClassOf pds4:urn:nasa:pds:0001_nasa_pds_1:all:user::1.0;
  rdfs:comment "The Error_Model_Parameter class specifies name and value for a parameter defined by the error model described by the parent class.".
 
pds4:urn:nasa:pds:0001_nasa_pds_1:all:user:img_surface:error_pixel::1.0 rdf:type rdfs:Class;
  rdfs:label "Error_Pixel";
  pds4:subClassOf pds4:urn:nasa:pds:0001_nasa_pds_1:all:user::1.0;
  rdfs:comment " The Error_Pixel class specifies the line and sample in the image where an error occurred.".
 
pds4:urn:nasa:pds:0001_nasa_pds_1:all:user:geom:expanded_geometry::1.0 rdf:type rdfs:Class;
  rdfs:label "Expanded_Geometry";
  pds4:subClassOf pds4:urn:nasa:pds:0001_nasa_pds_1:all:user::1.0;
  rdfs:comment "The Expanded_Geometry class provides a mechanism to reference additional geometric metadata contained in a separate object or product (e.g., a table of metadata). ".
 
pds4:urn:nasa:pds:0001_nasa_pds_1:all:user:img:exposure::1.0 rdf:type rdfs:Class;
  rdfs:label "Exposure";
  pds4:subClassOf pds4:urn:nasa:pds:0001_nasa_pds_1:all:user::1.0;
  rdfs:comment "The Exposure class contains attributes identifying the image instrument exposure configuration and image exposure values. As a child of the Imaging class, these attribute values identify the actual exposure values when the image was taken. As a child of the Commanded_Parameters class, these attribute values are those that were commanded to the spacecraft at the time the image was taken.".
 
pds4:urn:nasa:pds:0001_nasa_pds_1:pds:product_components:pds:external_reference::1.0 rdf:type rdfs:Class;
  rdfs:label "External_Reference";
  pds4:subClassOf pds4:urn:nasa:pds:0001_nasa_pds_1:all:user:pds:product_components::1.0;
  rdfs:comment "The External_Reference class is used to reference a source outside the PDS registry system.".
 
pds4:urn:nasa:pds:0001_nasa_pds_1:pds:external_reference:pds:external_reference_extended::1.0 rdf:type rdfs:Class;
  rdfs:label "External_Reference_Extended";
  pds4:subClassOf pds4:urn:nasa:pds:0001_nasa_pds_1:pds:product_components:pds:external_reference::1.0;
  rdfs:comment "The External_Reference_Extended class is used to reference a source outside the PDS registry system. This extension is used in the local data dictionary.".
 
pds4:urn:nasa:pds:0001_nasa_pds_1:pds:tndo_context:pds:facility::1.0 rdf:type rdfs:Class;
  rdfs:label "Facility";
  pds4:subClassOf pds4:urn:nasa:pds:0001_nasa_pds_1:pds:tagged_nondigital_object:pds:tndo_context::1.0;
  rdfs:comment "The Facility class provides a name and address for a  terrestrial observatory or laboratory.".
 
pds4:urn:nasa:pds:0001_nasa_pds_1:pds:tndo_context:pds:facility:laboratory::1.0 rdf:type rdfs:Class;
  rdfs:label "Laboratory";
  rdfs:subClassOf pds4:urn:nasa:pds:0001_nasa_pds_1:pds:tndo_context:pds:facility::1.0;
  rdfs:comment "The facility is a laboratory".
 
pds4:urn:nasa:pds:0001_nasa_pds_1:pds:tndo_context:pds:facility:observatory::1.0 rdf:type rdfs:Class;
  rdfs:label "Observatory";
  rdfs:subClassOf pds4:urn:nasa:pds:0001_nasa_pds_1:pds:tndo_context:pds:facility::1.0;
  rdfs:comment "The facility is an observatory".
 
pds4:urn:nasa:pds:0001_nasa_pds_1:pds:tagged_digital_child:pds:field::1.0 rdf:type rdfs:Class;
  rdfs:label "Field";
  pds4:subClassOf pds4:urn:nasa:pds:0001_nasa_pds_1:all:user:pds:tagged_digital_child::1.0;
  rdfs:comment "The Field class defines a field of a record and is the parent class of all specific field classes.The Field class defines a field of a record or a field of a group and is the parent class of all specific field classes.".
 
pds4:urn:nasa:pds:0001_nasa_pds_1:pds:field:pds:field_binary::1.0 rdf:type rdfs:Class;
  rdfs:label "Field_Binary";
  pds4:subClassOf pds4:urn:nasa:pds:0001_nasa_pds_1:pds:tagged_digital_child:pds:field::1.0;
  rdfs:comment "The Field_Binary class defines a field of a binary record or a field of a binary group.".
 
pds4:urn:nasa:pds:0001_nasa_pds_1:pds:field:pds:field_bit::1.0 rdf:type rdfs:Class;
  rdfs:label "Field_Bit";
  pds4:subClassOf pds4:urn:nasa:pds:0001_nasa_pds_1:pds:tagged_digital_child:pds:field::1.0;
  rdfs:comment "The Field_Bit class provides parameters for extracting one field out of a string of bytes which contains packed data (that is, data values either smaller than a single byte, or crossing byte boundaries, or both.".
 
pds4:urn:nasa:pds:0001_nasa_pds_1:pds:field:pds:field_character::1.0 rdf:type rdfs:Class;
  rdfs:label "Field_Character";
  pds4:subClassOf pds4:urn:nasa:pds:0001_nasa_pds_1:pds:tagged_digital_child:pds:field::1.0;
  rdfs:comment "The Field_Character class defines a field of a character record or a field of a character group.".
 
pds4:urn:nasa:pds:0001_nasa_pds_1:pds:field:pds:field_delimited::1.0 rdf:type rdfs:Class;
  rdfs:label "Field_Delimited";
  pds4:subClassOf pds4:urn:nasa:pds:0001_nasa_pds_1:pds:tagged_digital_child:pds:field::1.0;
  rdfs:comment "The Field_Delimited class defines a field of a delimited record or a field of a delimited group.".
 
pds4:urn:nasa:pds:0001_nasa_pds_1:pds:tndo_supplemental:pds:field_statistics::1.0 rdf:type rdfs:Class;
  rdfs:label "Field_Statistics";
  pds4:subClassOf pds4:urn:nasa:pds:0001_nasa_pds_1:pds:tagged_nondigital_object:pds:tndo_supplemental::1.0;
  rdfs:comment "The Field Statistics class provides a set of metrics for a column formed by a field in a repeating record.".
 
pds4:urn:nasa:pds:0001_nasa_pds_1:all:user:sp:field_of_view::1.0 rdf:type rdfs:Class;
  rdfs:label "Field_of_View";
  pds4:subClassOf pds4:urn:nasa:pds:0001_nasa_pds_1:all:user::1.0;
  rdfs:comment " The Field_of_View class is used to describe the field of view corresponding to the spectral data object. This class should describe the aperture or slit used in making the spectral observation, when applicable, as opposed to the theoretical full field of view of a telescope or boresight (which should be defined in a Geometry Dictionary class). ".
 
pds4:urn:nasa:pds:0001_nasa_pds_1:pds:tagged_digital_object:pds:file::1.0 rdf:type rdfs:Class;
  rdfs:label "File";
  pds4:subClassOf pds4:urn:nasa:pds:0001_nasa_pds_1:all:user:pds:tagged_digital_object::1.0;
  rdfs:comment "The File class consists of attributes that describe a file in a data store.".
 
pds4:urn:nasa:pds:0001_nasa_pds_1:pds:product_components:pds:file_area::1.0 rdf:type rdfs:Class;
  rdfs:label "File_Area";
  pds4:subClassOf pds4:urn:nasa:pds:0001_nasa_pds_1:all:user:pds:product_components::1.0;
  rdfs:comment "The File_Area class defines a File and its component data objects.".
 
pds4:urn:nasa:pds:0001_nasa_pds_1:pds:file_area:pds:file_area_ancillary::1.0 rdf:type rdfs:Class;
  rdfs:label "File_Area_Ancillary";
  pds4:subClassOf pds4:urn:nasa:pds:0001_nasa_pds_1:pds:product_components:pds:file_area::1.0;
  rdfs:comment "The File Area Ancillary class describes a file and one or more tagged_data_objects contained within the file.".
 
pds4:urn:nasa:pds:0001_nasa_pds_1:pds:file_area:pds:file_area_binary::1.0 rdf:type rdfs:Class;
  rdfs:label "File_Area_Binary";
  pds4:subClassOf pds4:urn:nasa:pds:0001_nasa_pds_1:pds:product_components:pds:file_area::1.0;
  rdfs:comment "The File Area Binary class describes a file that contains an encoded byte stream.".
 
pds4:urn:nasa:pds:0001_nasa_pds_1:pds:file_area:pds:file_area_browse::1.0 rdf:type rdfs:Class;
  rdfs:label "File_Area_Browse";
  pds4:subClassOf pds4:urn:nasa:pds:0001_nasa_pds_1:pds:product_components:pds:file_area::1.0;
  rdfs:comment "The File Area Browse class describes a file and one or more tagged_data_objects contained within the file.".
 
pds4:urn:nasa:pds:0001_nasa_pds_1:pds:file_area:pds:file_area_checksum_manifest::1.0 rdf:type rdfs:Class;
  rdfs:label "File_Area_Checksum_Manifest";
  pds4:subClassOf pds4:urn:nasa:pds:0001_nasa_pds_1:pds:product_components:pds:file_area::1.0;
  rdfs:comment "The File Area Checksum Manifest class describes a file that contains a two column table for file references and checksums.".
 
pds4:urn:nasa:pds:0001_nasa_pds_1:pds:file_area:pds:file_area_encoded_image::1.0 rdf:type rdfs:Class;
  rdfs:label "File_Area_Encoded_Image";
  pds4:subClassOf pds4:urn:nasa:pds:0001_nasa_pds_1:pds:product_components:pds:file_area::1.0;
  rdfs:comment "The File Area Encoded Image class describes a file that contains an Encoded Image object.".
 
pds4:urn:nasa:pds:0001_nasa_pds_1:pds:file_area:pds:file_area_inventory::1.0 rdf:type rdfs:Class;
  rdfs:label "File_Area_Inventory";
  pds4:subClassOf pds4:urn:nasa:pds:0001_nasa_pds_1:pds:product_components:pds:file_area::1.0;
  rdfs:comment "The File Area Inventory class describes a file and an inventory consisting of references to  members.".
 
pds4:urn:nasa:pds:0001_nasa_pds_1:pds:file_area:pds:file_area_metadata::1.0 rdf:type rdfs:Class;
  rdfs:label "File_Area_Metadata";
  pds4:subClassOf pds4:urn:nasa:pds:0001_nasa_pds_1:pds:product_components:pds:file_area::1.0;
  rdfs:comment "The File Area Metadata class describes a table which provides new, and\\//or improved, metadata. All field names provided must be attributes defined in PDS4, either in the common dictionary, or in a PDS4 discipline or mission dictionary.".
 
pds4:urn:nasa:pds:0001_nasa_pds_1:pds:file_area:pds:file_area_native::1.0 rdf:type rdfs:Class;
  rdfs:label "File_Area_Native";
  pds4:subClassOf pds4:urn:nasa:pds:0001_nasa_pds_1:pds:product_components:pds:file_area::1.0;
  rdfs:comment "The File Area Native describes tagged_data_objects collected from an instrument.".
 
pds4:urn:nasa:pds:0001_nasa_pds_1:pds:file_area:pds:file_area_observational::1.0 rdf:type rdfs:Class;
  rdfs:label "File_Area_Observational";
  pds4:subClassOf pds4:urn:nasa:pds:0001_nasa_pds_1:pds:product_components:pds:file_area::1.0;
  rdfs:comment "The File Area Observational class describes, for an observational product, a file and one or more tagged_data_objects contained within the file.".
 
pds4:urn:nasa:pds:0001_nasa_pds_1:pds:file_area:pds:file_area_observational_supplemental::1.0 rdf:type rdfs:Class;
  rdfs:label "File_Area_Observational_Supplemental";
  pds4:subClassOf pds4:urn:nasa:pds:0001_nasa_pds_1:pds:product_components:pds:file_area::1.0;
  rdfs:comment "The File Area Observational Supplemental class describes, for an observational product, additional files and tagged_data_objects contained within the file.".
 
pds4:urn:nasa:pds:0001_nasa_pds_1:pds:file_area:pds:file_area_sip_deep_archive::1.0 rdf:type rdfs:Class;
  rdfs:label "File_Area_SIP_Deep_Archive";
  pds4:subClassOf pds4:urn:nasa:pds:0001_nasa_pds_1:pds:product_components:pds:file_area::1.0;
  rdfs:comment "The File Area SIP Deep Archive class describes the File Area for the Submission Information Package (SIP) for the NASA planetary science deep archive.".
 
pds4:urn:nasa:pds:0001_nasa_pds_1:pds:file_area:pds:file_area_spice_kernel::1.0 rdf:type rdfs:Class;
  rdfs:label "File_Area_SPICE_Kernel";
  pds4:subClassOf pds4:urn:nasa:pds:0001_nasa_pds_1:pds:product_components:pds:file_area::1.0;
  rdfs:comment "The File Area SPICE Kernel class describes a file that contains a SPICE Kernel object.".
 
pds4:urn:nasa:pds:0001_nasa_pds_1:pds:file_area:pds:file_area_service_description::1.0 rdf:type rdfs:Class;
  rdfs:label "File_Area_Service_Description";
  pds4:subClassOf pds4:urn:nasa:pds:0001_nasa_pds_1:pds:product_components:pds:file_area::1.0;
  rdfs:comment "The File Area Service Description class describes a file that contains a service description.".
 
pds4:urn:nasa:pds:0001_nasa_pds_1:pds:file_area:pds:file_area_text::1.0 rdf:type rdfs:Class;
  rdfs:label "File_Area_Text";
  pds4:subClassOf pds4:urn:nasa:pds:0001_nasa_pds_1:pds:product_components:pds:file_area::1.0;
  rdfs:comment "The File Area Text class describes a file that contains a text stream object.".
 
pds4:urn:nasa:pds:0001_nasa_pds_1:pds:file_area:pds:file_area_transfer_manifest::1.0 rdf:type rdfs:Class;
  rdfs:label "File_Area_Transfer_Manifest";
  pds4:subClassOf pds4:urn:nasa:pds:0001_nasa_pds_1:pds:product_components:pds:file_area::1.0;
  rdfs:comment "The File Area Transfer Manifest class describes a file that contains a two column table that maps the logical identifiers and version ids of products to their file specification names.".
 
pds4:urn:nasa:pds:0001_nasa_pds_1:pds:file_area:pds:file_area_update::1.0 rdf:type rdfs:Class;
  rdfs:label "File_Area_Update";
  pds4:subClassOf pds4:urn:nasa:pds:0001_nasa_pds_1:pds:product_components:pds:file_area::1.0;
  rdfs:comment "The File Area Update class is a File Area that describes a file that contains one or  more digital objects used to provide additional metadata for registered products.".
 
pds4:urn:nasa:pds:0001_nasa_pds_1:pds:file_area:pds:file_area_xml_schema::1.0 rdf:type rdfs:Class;
  rdfs:label "File_Area_XML_Schema";
  pds4:subClassOf pds4:urn:nasa:pds:0001_nasa_pds_1:pds:product_components:pds:file_area::1.0;
  rdfs:comment "The File Area XML Schema class describes a file that contains a resource used for the PDS4 implementation into XML.".
 
pds4:urn:nasa:pds:0001_nasa_pds_1:all:user:sp:filter::1.0 rdf:type rdfs:Class;
  rdfs:label "Filter";
  pds4:subClassOf pds4:urn:nasa:pds:0001_nasa_pds_1:all:user::1.0;
  rdfs:comment " The Filter class identifies the filter associated with a specific band or bin along a spectral axis in an Array object. The filter may be identified by either name, identifier, or number or some combination of these. ".
 
pds4:urn:nasa:pds:0001_nasa_pds_1:all:user:nucspec:first_count::1.0 rdf:type rdfs:Class;
  rdfs:label "First_Count";
  pds4:subClassOf pds4:urn:nasa:pds:0001_nasa_pds_1:all:user::1.0;
  rdfs:comment "Defines the records to which this state applies by identifying the first record (inclusive), and the number of contiguous records, including the first.".
 
pds4:urn:nasa:pds:0001_nasa_pds_1:all:user:nucspec:first_last::1.0 rdf:type rdfs:Class;
  rdfs:label "First_Last";
  pds4:subClassOf pds4:urn:nasa:pds:0001_nasa_pds_1:all:user::1.0;
  rdfs:comment "Defines the first and last records for which this state applies. The record numbers are one-based and inclusive.".
 
pds4:urn:nasa:pds:0001_nasa_pds_1:img:data_processing:img:flat_field_correction::1.0 rdf:type rdfs:Class;
  rdfs:label "Flat_Field_Correction";
  pds4:subClassOf pds4:urn:nasa:pds:0001_nasa_pds_1:all:user:img:data_processing::1.0;
  rdfs:comment " The Flat_Field_Correction class specifies how flat-field correction was performed on this image. This can be done either algorithmically, using a Radial_Flat_Field_Correction, or using a Flat_Field_File.".
 
pds4:urn:nasa:pds:0001_nasa_pds_1:img:data_processing_file:img:flat_field_file::1.0 rdf:type rdfs:Class;
  rdfs:label "Flat_Field_File";
  pds4:subClassOf pds4:urn:nasa:pds:0001_nasa_pds_1:all:user:img:data_processing_file::1.0;
  rdfs:comment "The Flat_Field_File class specifies the image used for flat field correction. The image is divided by this flat field image in order to apply the flat field correction (which is the opposite of Radial_Flat_Field_Function). ".
 
pds4:urn:nasa:pds:0001_nasa_pds_1:all:user:img:focus::1.0 rdf:type rdfs:Class;
  rdfs:label "Focus";
  pds4:subClassOf pds4:urn:nasa:pds:0001_nasa_pds_1:all:user::1.0;
  rdfs:comment "The Focus class contains attributes that describe the focus or autofocus parameters for an observation. As a child of Commanded_Parameters, these indicate the focus settings used to command the instrument. Otherwise, they indicate the actual focus used by the observation.".
 
pds4:urn:nasa:pds:0001_nasa_pds_1:img:data_processing:img:focus_stack::1.0 rdf:type rdfs:Class;
  rdfs:label "Focus_Stack";
  pds4:subClassOf pds4:urn:nasa:pds:0001_nasa_pds_1:all:user:img:data_processing::1.0;
  rdfs:comment "The Focus_Stack class contains attributes that describe a set of images taken at different focus settings, which are often merged to create a best-focus image or combined to extract range information. Focus stacks are also sometimes called ZStacks. ".
 
pds4:urn:nasa:pds:0001_nasa_pds_1:all:user:geom:footprint_vertices::1.0 rdf:type rdfs:Class;
  rdfs:label "Footprint_Vertices";
  pds4:subClassOf pds4:urn:nasa:pds:0001_nasa_pds_1:all:user::1.0;
  rdfs:comment "The Footprint_Vertices class provides a set of latitude and longitude pairs which are the vertices of a polygon representing the projected footprint of the field of view on the target surface (or on a map). Note this is intended for products such as maps, or where the target fills the field of view. The vertices should be listed either in clockwise or counterclockwise order. ".
 
pds4:urn:nasa:pds:0001_nasa_pds_1:all:user:img:frame::1.0 rdf:type rdfs:Class;
  rdfs:label "Frame";
  pds4:subClassOf pds4:urn:nasa:pds:0001_nasa_pds_1:all:user::1.0;
  rdfs:comment "The Frame class contains attributes providing information specific to an image frame. A frame consists of a sequence of measurements made over a specified time interval, and may include measurements from different instrument modes. In the context of Frame, product_flag refers to the actual image.".
 
pds4:urn:nasa:pds:0001_nasa_pds_1:all:user:rings:frame_ident_base::1.0 rdf:type rdfs:Class;
  rdfs:label "Frame_Ident_Base";
  pds4:subClassOf pds4:urn:nasa:pds:0001_nasa_pds_1:all:user::1.0;
  rdfs:comment "The Frame_Ident_Base class provides multiple attributes that can be used to identify a reference frame. At least one must be used. ".
 
pds4:urn:nasa:pds:0001_nasa_pds_1:all:user:geom:frame_identification_base::1.0 rdf:type rdfs:Class;
  rdfs:label "Frame_Identification_Base";
  pds4:subClassOf pds4:urn:nasa:pds:0001_nasa_pds_1:all:user::1.0;
  rdfs:comment "The Frame_Identification_Base class provides multiple attributes that can be used to identify a reference frame. At least one must be used. ".
 
pds4:urn:nasa:pds:0001_nasa_pds_1:all:user:geom:generic_vectors::1.0 rdf:type rdfs:Class;
  rdfs:label "Generic_Vectors";
  pds4:subClassOf pds4:urn:nasa:pds:0001_nasa_pds_1:all:user::1.0;
  rdfs:comment "The Generic_Vectors class is a container class for all of the build your own vector templates. ".
 
pds4:urn:nasa:pds:0001_nasa_pds_1:all:user:cart:geo_transformation::1.0 rdf:type rdfs:Class;
  rdfs:label "Geo_Transformation";
  pds4:subClassOf pds4:urn:nasa:pds:0001_nasa_pds_1:all:user::1.0;
  rdfs:comment "The GEO_Transformation describes the relationship between raster positions (in pixel\\//line coordinates) and georeferenced coordinates. This is defined by an affine transform. The affine transform consists of six coefficients which map pixel\\//line coordinates into georeferenced space using the following relationship: Xgeo = GT(0) + Xpixel*GT(1) + Yline*GT(2) Ygeo = GT(3) + Xpixel*GT(4) + Yline*GT(5) or also defined as: GT[0] = Xmin; \\//\\// upperleft_corner_y GT[1] = CellSize in X; \\//\\// W-E pixel size, pixel_resolution_x GT[2] = 0; \\//\\// rotation term, 0 if \\'North Up\\' GT[3] = Ymax; \\//\\// upperleft_corner_y GT[4] = 0; \\//\\// shear term, 0 if \\'North Up\\' GT[5] = CellSize in Y; \\//\\// N-S pixel size, pixel_resolution_y In case of north up images, the GT(2) and GT(4) coefficients are zero, and the GT(1) is pixel width (pixel_resolution_x), and GT(5) is pixel height (pixel_resolution_y). The (GT(0),GT(3)) position is the top left corner of the top left pixel of the raster. Note that the pixel\\//line coordinates in the above are from (0.5,0.5) at the top left corner of the top left pixel to (width_in_pixels,height_in_pixels) at the bottom right corner of the bottom right pixel. The pixel\\//line location of the center of the top left pixel would therefore be (1.0,1.0). ".
 
pds4:urn:nasa:pds:0001_nasa_pds_1:all:user:cart:geodetic_model::1.0 rdf:type rdfs:Class;
  rdfs:label "Geodetic_Model";
  pds4:subClassOf pds4:urn:nasa:pds:0001_nasa_pds_1:all:user::1.0;
  rdfs:comment "The Geodetic_Model class provides parameters describing the shape of the planet.".
 
pds4:urn:nasa:pds:0001_nasa_pds_1:all:user:cart:geographic::1.0 rdf:type rdfs:Class;
  rdfs:label "Geographic";
  pds4:subClassOf pds4:urn:nasa:pds:0001_nasa_pds_1:all:user::1.0;
  rdfs:comment "The Geographic class provides information about the quantities of latitude and longitude which define the position of a point on a planetary body\\'s surface with respect to a reference spheroid.".
 
pds4:urn:nasa:pds:0001_nasa_pds_1:all:user:geom:geometry::1.0 rdf:type rdfs:Class;
  rdfs:label "Geometry";
  pds4:subClassOf pds4:urn:nasa:pds:0001_nasa_pds_1:all:user::1.0;
  rdfs:comment "The Geometry class is a container for all geometric information in the label. The Image_Display_Geometry class should have one instance if the primary data object is an Array object for which two of the dimensions are suitable for display in the vertical (line) and horizontal (sample) dimensions of a display device. Multiple instances of the Image_Display_Geometry class are only appropriate if the data product contains multiple Array objects and the orientations of the various objects are not the same. ".
 
pds4:urn:nasa:pds:0001_nasa_pds_1:all:user:geom:geometry_lander::1.0 rdf:type rdfs:Class;
  rdfs:label "Geometry_Lander";
  pds4:subClassOf pds4:urn:nasa:pds:0001_nasa_pds_1:all:user::1.0;
  rdfs:comment "The Geometry_Lander class is a container for all geometric information in the label relating to a landed spacecraft, including rovers. ".
 
pds4:urn:nasa:pds:0001_nasa_pds_1:all:user:geom:geometry_orbiter::1.0 rdf:type rdfs:Class;
  rdfs:label "Geometry_Orbiter";
  pds4:subClassOf pds4:urn:nasa:pds:0001_nasa_pds_1:all:user::1.0;
  rdfs:comment "The Geometry_Orbiter class is a container for geometric information (positions, velocities, orientations, etc.) relevant to orbiter or flyby spacecraft observations. If any of the contained classes or attributes have central body, and or target in the class or attribute name (e.g., spacecraft_to_central_body_distance, Vector_Planetocentric_Position_Spacecraft_To_Target), then the central body and or target must be identified in this class. If more than one geometry_reference_time_utc, target or central body need to be identified to fully describe the data, use multiple instances of the Geometry_Orbiter class. Do not use Coordinate_System at this level if more than one coordinate system is used in the contained classes. If more than one coordinate system is used, specify Coordinate_System in each of the subordinate classes where it is appropriate. ".
 
pds4:urn:nasa:pds:0001_nasa_pds_1:all:user:img_surface:geometry_projection::1.0 rdf:type rdfs:Class;
  rdfs:label "Geometry_Projection";
  pds4:subClassOf pds4:urn:nasa:pds:0001_nasa_pds_1:all:user::1.0;
  rdfs:comment "The Geometry_Projection describes the geometric projection or warping the image has undergone. It is not the intent of this class to describe map projections, but rather image warps such as linearization (stereo epipolar alignment), geometric sensor correction, or rubber-sheeting. If present, a linearization partner image can be referenced using either an Internal_Reference or External_Reference.".
 
pds4:urn:nasa:pds:0001_nasa_pds_1:geom:body_identification_base:geom:geometry_target_identification::1.0 rdf:type rdfs:Class;
  rdfs:label "Geometry_Target_Identification";
  pds4:subClassOf pds4:urn:nasa:pds:0001_nasa_pds_1:all:user:geom:body_identification_base::1.0;
  rdfs:comment "The object to which the associated set of geometric parameters are given. Within the Geometry dictionary context, a \"Target\" is the body on the \"to\" end of a vector, or other translation through space. ".
 
pds4:urn:nasa:pds:0001_nasa_pds_1:all:user:rings:global_model_parameters::1.0 rdf:type rdfs:Class;
  rdfs:label "Global_Model_Parameters";
  pds4:subClassOf pds4:urn:nasa:pds:0001_nasa_pds_1:all:user::1.0;
  rdfs:comment "This class provides the general parameters used to generate a ring model.".
 
pds4:urn:nasa:pds:0001_nasa_pds_1:all:user:cart:grid_coordinate_system::1.0 rdf:type rdfs:Class;
  rdfs:label "Grid_Coordinate_System";
  pds4:subClassOf pds4:urn:nasa:pds:0001_nasa_pds_1:all:user::1.0;
  rdfs:comment "The Grid_Coordinate_System class defines a plane-rectangular coordinate system usually based on, and mathematically adjusted to, a map projection so that geographic positions can be readily transformed to and from plane coordinates.".
 
pds4:urn:nasa:pds:0001_nasa_pds_1:pds:tagged_digital_child:pds:group::1.0 rdf:type rdfs:Class;
  rdfs:label "Group";
  pds4:subClassOf pds4:urn:nasa:pds:0001_nasa_pds_1:all:user:pds:tagged_digital_child::1.0;
  rdfs:comment "The Group class defines a group of (repeating) fields and, possibly, (sub) groups; it is the parent class of all specific group classes.".
 
pds4:urn:nasa:pds:0001_nasa_pds_1:pds:product_components:pds:group_facet1::1.0 rdf:type rdfs:Class;
  rdfs:label "Group_Facet1";
  pds4:subClassOf pds4:urn:nasa:pds:0001_nasa_pds_1:all:user:pds:product_components::1.0;
  rdfs:comment "The Group_Facet1 class contains a single facet restricted according to the value of discipline_name. It also contains zero or more subfacets restricted according to the value of the facet. Note that Science_Facets was modeled with Discipline_Facets as a component and Discipline_Facets was modeled with Group_Facet1 and Group_Facet2 as components. This dependency hierarchy was flattened and only Science_Facets exists in the schema.".
 
pds4:urn:nasa:pds:0001_nasa_pds_1:pds:product_components:pds:group_facet2::1.0 rdf:type rdfs:Class;
  rdfs:label "Group_Facet2";
  pds4:subClassOf pds4:urn:nasa:pds:0001_nasa_pds_1:all:user:pds:product_components::1.0;
  rdfs:comment "The Group_Facet2 class contains a single facet restricted according to the value of discipline_name. It also contains zero or more subfacets restricted according to the value of the facet. Note that Science_Facets was modeled with Discipline_Facets as a component and Discipline_Facets was modeled with Group_Facet1 and Group_Facet2 as components. This dependency hierarchy was flattened and only Science_Facets exists in the schema.".
 
pds4:urn:nasa:pds:0001_nasa_pds_1:pds:group:pds:group_field_binary::1.0 rdf:type rdfs:Class;
  rdfs:label "Group_Field_Binary";
  pds4:subClassOf pds4:urn:nasa:pds:0001_nasa_pds_1:pds:tagged_digital_child:pds:group::1.0;
  rdfs:comment "The Group_Field_Binary class allows a group of table fields.".
 
pds4:urn:nasa:pds:0001_nasa_pds_1:pds:group:pds:group_field_character::1.0 rdf:type rdfs:Class;
  rdfs:label "Group_Field_Character";
  pds4:subClassOf pds4:urn:nasa:pds:0001_nasa_pds_1:pds:tagged_digital_child:pds:group::1.0;
  rdfs:comment "The Group_Field_Character class allows a group of table fields.".
 
pds4:urn:nasa:pds:0001_nasa_pds_1:pds:group:pds:group_field_delimited::1.0 rdf:type rdfs:Class;
  rdfs:label "Group_Field_Delimited";
  pds4:subClassOf pds4:urn:nasa:pds:0001_nasa_pds_1:pds:tagged_digital_child:pds:group::1.0;
  rdfs:comment "The Field_Group_Delimited class allows a group of delimited fields.".
 
pds4:urn:nasa:pds:0001_nasa_pds_1:pds:parsable_byte_stream:pds:header::1.0 rdf:type rdfs:Class;
  rdfs:label "Header";
  pds4:subClassOf pds4:urn:nasa:pds:0001_nasa_pds_1:pds:byte_stream:pds:parsable_byte_stream::1.0;
  rdfs:comment "The Header class describes a data object header.".
 
pds4:urn:nasa:pds:0001_nasa_pds_1:img:data_processing:img:high_dynamic_range::1.0 rdf:type rdfs:Class;
  rdfs:label "High_Dynamic_Range";
  pds4:subClassOf pds4:urn:nasa:pds:0001_nasa_pds_1:all:user:img:data_processing::1.0;
  rdfs:comment "Specifies parameters related to High Dynamic Range processing, which combines multiple exposures of different lengths into a single product with a greater dynamic range than any of the inputs.".
 
pds4:urn:nasa:pds:0001_nasa_pds_1:all:user:img:high_dynamic_range_exposure::1.0 rdf:type rdfs:Class;
  rdfs:label "High_Dynamic_Range_Exposure";
  pds4:subClassOf pds4:urn:nasa:pds:0001_nasa_pds_1:all:user::1.0;
  rdfs:comment "Specifies parameters for each individual exposure in an HDR image.".
 
pds4:urn:nasa:pds:0001_nasa_pds_1:all:user:img:histogram::1.0 rdf:type rdfs:Class;
  rdfs:label "Histogram";
  pds4:subClassOf pds4:urn:nasa:pds:0001_nasa_pds_1:all:user::1.0;
  rdfs:comment "Describes a Histogram product.".
 
pds4:urn:nasa:pds:0001_nasa_pds_1:all:user:cart:horizontal_coordinate_system_definition::1.0 rdf:type rdfs:Class;
  rdfs:label "Horizontal_Coordinate_System_Definition";
  pds4:subClassOf pds4:urn:nasa:pds:0001_nasa_pds_1:all:user::1.0;
  rdfs:comment "The Horizontal_Coordinate_System_Definition class provides the reference frame or system from which linear or angular quantities are measured and assigned to the position that a point occupies. ".
 
pds4:urn:nasa:pds:0001_nasa_pds_1:all:user:img:icer_parameters::1.0 rdf:type rdfs:Class;
  rdfs:label "ICER_Parameters";
  pds4:subClassOf pds4:urn:nasa:pds:0001_nasa_pds_1:all:user::1.0;
  rdfs:comment " The ICER_Parameters class contains attributes describing onboard compression parameters specific to Joint Photographic Experts Group (JPEG) image compression. ICER is a wavelet-based image compression file format used by the NASA Mars Rovers. ICER has both lossy and lossless compression modes.".
 
pds4:urn:nasa:pds:0001_nasa_pds_1:pds:product_components:pds:identification_area::1.0 rdf:type rdfs:Class;
  rdfs:label "Identification_Area";
  pds4:subClassOf pds4:urn:nasa:pds:0001_nasa_pds_1:all:user:pds:product_components::1.0;
  rdfs:comment "The identification area consists of attributes that identify and name an object.".
 
pds4:urn:nasa:pds:0001_nasa_pds_1:all:user:img:illumination::1.0 rdf:type rdfs:Class;
  rdfs:label "Illumination";
  pds4:subClassOf pds4:urn:nasa:pds:0001_nasa_pds_1:all:user::1.0;
  rdfs:comment " The Illumination class provides attributes describing the illumination sources used to illuminate the imaging target.".
 
pds4:urn:nasa:pds:0001_nasa_pds_1:all:user:geom:illumination_geometry::1.0 rdf:type rdfs:Class;
  rdfs:label "Illumination_Geometry";
  pds4:subClassOf pds4:urn:nasa:pds:0001_nasa_pds_1:all:user::1.0;
  rdfs:comment "The Illumination_Geometry class is a container for illumination geometry classes.".
 
pds4:urn:nasa:pds:0001_nasa_pds_1:all:user:geom:illumination_min_max::1.0 rdf:type rdfs:Class;
  rdfs:label "Illumination_Min_Max";
  pds4:subClassOf pds4:urn:nasa:pds:0001_nasa_pds_1:all:user::1.0;
  rdfs:comment "The Illumination_Min_Max class contains attributes providing illumination parameters as minimum\\//maximum pairs. For any given illumination parameter if one of minimum or maximum is given, both must be given. If a target is specified using the Geometry_Target_Identification class in the Orbiter_Identification class under the same parent Geometry_Orbiter class, the min-max pairs for each illumination parameter provide the range of that parameter in the observation on that target. Otherwise the pair provides the range for the entire field of view. ".
 
pds4:urn:nasa:pds:0001_nasa_pds_1:all:user:geom:illumination_specific::1.0 rdf:type rdfs:Class;
  rdfs:label "Illumination_Specific";
  pds4:subClassOf pds4:urn:nasa:pds:0001_nasa_pds_1:all:user::1.0;
  rdfs:comment "The Illumination_Specific class contains attributes providing illumination parameters at a single location in the field of view. That location is specified by using one, and only one of reference_location, reference_pixel_location, or Reference_Pixel, If reference_location is used, and indicates a point on a target, the target must be the one specified using Geometry_Target_Identification in the parent Geometry_Orbiter class. The provided value for each illumination attribute must correspond to the time given by geometry_reference_time_utc. ".
 
pds4:urn:nasa:pds:0001_nasa_pds_1:all:user:geom:illumination_start_stop::1.0 rdf:type rdfs:Class;
  rdfs:label "Illumination_Start_Stop";
  pds4:subClassOf pds4:urn:nasa:pds:0001_nasa_pds_1:all:user::1.0;
  rdfs:comment "The Illumination_Start_Stop class contains attributes providing illumination parameters as pairs corresponding to the beginning and end of the observation. If either the start or stop parameter is given, both must be provided. If any values from this class are included in the label, the parameters geometry_start_time_utc and geometry_stop_time_utc must be given in the enclosing Geometry_Orbiter class. If a target is specified using the Geometry_Target_Identification class in the Orbiter_Identification class under the parent Geometry_Orbiter class, the start-stop pairs for each illumination parameter provide the range of that parameter in the observation on that target. Otherwise the pair provides the range for the entire field of view. ".
 
pds4:urn:nasa:pds:0001_nasa_pds_1:all:user:img:image_compression_segment::1.0 rdf:type rdfs:Class;
  rdfs:label "Image_Compression_Segment";
  pds4:subClassOf pds4:urn:nasa:pds:0001_nasa_pds_1:all:user::1.0;
  rdfs:comment " The Image_Compression_Segment class provides attributes describing each segment into which data was partitioned for error containment purposes as part of the compression process. ".
 
pds4:urn:nasa:pds:0001_nasa_pds_1:all:user:survey:image_corners::1.0 rdf:type rdfs:Class;
  rdfs:label "Image_Corners";
  pds4:subClassOf pds4:urn:nasa:pds:0001_nasa_pds_1:all:user::1.0;
  rdfs:comment "The portion of the sky contained within an image, identified by its four corners".
 
pds4:urn:nasa:pds:0001_nasa_pds_1:all:user:geom:image_display_geometry::1.0 rdf:type rdfs:Class;
  rdfs:label "Image_Display_Geometry";
  pds4:subClassOf pds4:urn:nasa:pds:0001_nasa_pds_1:all:user::1.0;
  rdfs:comment "Image_Display_Geometry class provides an unambiguous description of the orientation of the image contents. Given an image, displayed as described by the Display_Direction class, any one of the Object_Orientation_* classes should allow unambiguous orientation of the contents of the image. The Local_Internal_Reference class is used to identify the object to which this instance of the Image_Display_Geometry class applies, and must be used if there is more than one instance of Image_Display_Geometry in the label. The appropriate value for local_reference_type is image_display_to_object. The Object_Orientation_North_East class is typically used for instruments for which the entire field of view is a portion of the target surface (e.g., instruments on Mars orbital spacecraft); otherwise use Object_Orientation_RA_Dec (e.g., flyby missions, missions with orbit radii much larger than the target radius such as Voyager or Cassini). At least one of these must be used. The two *_Identification classes used here are Central_Body (e.g., Saturn if you are using Planetocentric or planetographic coordinates in the Saturn system) and Target when the described object in the FoV is not the Central_Body. For example giving the orientation of the pole of Enceladus in Saturn Planetocentric coordinates, Central_Body = Saturn, Target = Enceladus. Bottom line: put in enough information so someone else can figure out the orientation of the field of view. We also offer an option to provide the pointing information as a quaternion. ".
 
pds4:urn:nasa:pds:0001_nasa_pds_1:img:data_processing:img:image_filter::1.0 rdf:type rdfs:Class;
  rdfs:label "Image_Filter";
  pds4:subClassOf pds4:urn:nasa:pds:0001_nasa_pds_1:all:user:img:data_processing::1.0;
  rdfs:comment "The Image_Filter class specifies what kind of image filtering has been done to the image. Image filtering looks at image intensity rather the geometry of pixels (cf. Spatial_Filter).".
 
pds4:urn:nasa:pds:0001_nasa_pds_1:all:user:img_surface:image_identifiers::1.0 rdf:type rdfs:Class;
  rdfs:label "Image_Identifiers";
  pds4:subClassOf pds4:urn:nasa:pds:0001_nasa_pds_1:all:user::1.0;
  rdfs:comment "The Image_Identifiers class contains items that help to identify the image or guide how processing should be done to the image.".
 
pds4:urn:nasa:pds:0001_nasa_pds_1:all:user:img:image_mask::1.0 rdf:type rdfs:Class;
  rdfs:label "Image_Mask";
  pds4:subClassOf pds4:urn:nasa:pds:0001_nasa_pds_1:all:user::1.0;
  rdfs:comment "The Image_Mask specifies how pixels were masked (removed) from an image. Masks are typically used to suppress results in areas where they don\\'t belong, for example masking off spacecraft hardware or removing pixels that did not meet some processing threshold. ".
 
pds4:urn:nasa:pds:0001_nasa_pds_1:all:user:img:image_mask_file::1.0 rdf:type rdfs:Class;
  rdfs:label "Image_Mask_File";
  pds4:subClassOf pds4:urn:nasa:pds:0001_nasa_pds_1:all:user::1.0;
  rdfs:comment "This class identifies a file used for image masking. The mask_type defines the type of file; if mask_type is missing then \"image\" is assumed.".
 
pds4:urn:nasa:pds:0001_nasa_pds_1:all:user:img:imaging::1.0 rdf:type rdfs:Class;
  rdfs:label "Imaging";
  pds4:subClassOf pds4:urn:nasa:pds:0001_nasa_pds_1:all:user::1.0;
  rdfs:comment "The Imaging class contains classes and attributes describing both the image product itself and the imaging instrument. Image product information can include exposure duration, filters, data correction, sampling, frame, sub-frames, and how the product was derived. For the imaging instrument, information can be provided describing the dynamic physical or operating characteristics of the imaging instrument.".
 
pds4:urn:nasa:pds:0001_nasa_pds_1:pds:tndo_supplemental:pds:information_package::1.0 rdf:type rdfs:Class;
  rdfs:label "Information_Package";
  pds4:subClassOf pds4:urn:nasa:pds:0001_nasa_pds_1:pds:tagged_nondigital_object:pds:tndo_supplemental::1.0;
  rdfs:comment "The Information Package class defines the Information Package as described in the OAIS Reference Model and is the parent class of all specific IP classes.".
 
pds4:urn:nasa:pds:0001_nasa_pds_1:pds:tndo_supplemental:pds:information_package_component::1.0 rdf:type rdfs:Class;
  rdfs:label "Information_Package_Component";
  pds4:subClassOf pds4:urn:nasa:pds:0001_nasa_pds_1:pds:tagged_nondigital_object:pds:tndo_supplemental::1.0;
  rdfs:comment "The Information_Package_Component class associates a Bundle, Collections or Basic Products with Checksum and Storage Manifests.".
 
pds4:urn:nasa:pds:0001_nasa_pds_1:pds:tndo_supplemental:pds:information_package_component_deep_archive::1.0 rdf:type rdfs:Class;
  rdfs:label "Information_Package_Component_Deep_Archive";
  pds4:subClassOf pds4:urn:nasa:pds:0001_nasa_pds_1:pds:tagged_nondigital_object:pds:tndo_supplemental::1.0;
  rdfs:comment "The Information Package Component Deep Archive class is an Information Package Component for the NASA planetary science deep archive.".
 
pds4:urn:nasa:pds:0001_nasa_pds_1:pds:tndo_supplemental:pds:ingest_ldd::1.0 rdf:type rdfs:Class;
  rdfs:label "Ingest_LDD";
  pds4:subClassOf pds4:urn:nasa:pds:0001_nasa_pds_1:pds:tagged_nondigital_object:pds:tndo_supplemental::1.0;
  rdfs:comment "The Ingest_LDD class provides a form for collecting class and attribute definitions.".
 
pds4:urn:nasa:pds:0001_nasa_pds_1:all:user:proc:input_product::1.0 rdf:type rdfs:Class;
  rdfs:label "Input_Product";
  pds4:subClassOf pds4:urn:nasa:pds:0001_nasa_pds_1:all:user::1.0;
  rdfs:comment "The Input_Product class describes one of the product most directly used as input to software for product creation, including raw, partially-processed, calibrated, or derived products.".
 
pds4:urn:nasa:pds:0001_nasa_pds_1:all:user:proc:input_product_list::1.0 rdf:type rdfs:Class;
  rdfs:label "Input_Product_List";
  pds4:subClassOf pds4:urn:nasa:pds:0001_nasa_pds_1:all:user::1.0;
  rdfs:comment "The Input_Product_List class describes all of the product(s) most directly used as input to software for product creation, including raw, partially-processed, calibrated, or derived products. These Input Products can be explicitly described in this label using the Input_Product class, and\\//or a list of products can be specified in another product referenced by the Internal_Reference or Local_Internal_Reference.".
 
pds4:urn:nasa:pds:0001_nasa_pds_1:pds:tndo_context:pds:instrument::1.0 rdf:type rdfs:Class;
  rdfs:label "Instrument";
  pds4:subClassOf pds4:urn:nasa:pds:0001_nasa_pds_1:pds:tagged_nondigital_object:pds:tndo_context::1.0;
  rdfs:comment "The Instrument class provides a description of a physical object that collects data.".
 
pds4:urn:nasa:pds:0001_nasa_pds_1:pds:tndo_context:pds:instrument:accelerometer::1.0 rdf:type rdfs:Class;
  rdfs:label "Accelerometer";
  rdfs:subClassOf pds4:urn:nasa:pds:0001_nasa_pds_1:pds:tndo_context:pds:instrument::1.0;
  rdfs:comment "An instrument that measures proper (i.e., its own) acceleration.".
 
pds4:urn:nasa:pds:0001_nasa_pds_1:pds:tndo_context:pds:instrument:alpha_particle_detector::1.0 rdf:type rdfs:Class;
  rdfs:label "Alpha Particle Detector";
  rdfs:subClassOf pds4:urn:nasa:pds:0001_nasa_pds_1:pds:tndo_context:pds:instrument::1.0;
  rdfs:comment "An instrument that measures the number and\\//or distribution of alpha particles.".
 
pds4:urn:nasa:pds:0001_nasa_pds_1:pds:tndo_context:pds:instrument:alpha_particle_x-ray_spectrometer::1.0 rdf:type rdfs:Class;
  rdfs:label "Alpha Particle X-Ray Spectrometer";
  rdfs:subClassOf pds4:urn:nasa:pds:0001_nasa_pds_1:pds:tndo_context:pds:instrument::1.0;
  rdfs:comment "An instrument that bombards a sample with alpha particles and X-rays and measures the energy spectrum of scattered alpha particles and X-rays to determine the sample\\'s elemental composition.".
 
pds4:urn:nasa:pds:0001_nasa_pds_1:pds:tndo_context:pds:instrument:altimeter::1.0 rdf:type rdfs:Class;
  rdfs:label "Altimeter";
  rdfs:subClassOf pds4:urn:nasa:pds:0001_nasa_pds_1:pds:tndo_context:pds:instrument::1.0;
  rdfs:comment "An instrument that measures its own altitude above a reference surface.".
 
pds4:urn:nasa:pds:0001_nasa_pds_1:pds:tndo_context:pds:instrument:anemometer::1.0 rdf:type rdfs:Class;
  rdfs:label "Anemometer";
  rdfs:subClassOf pds4:urn:nasa:pds:0001_nasa_pds_1:pds:tndo_context:pds:instrument::1.0;
  rdfs:comment "An in situ instrument that measures wind speed.".
 
pds4:urn:nasa:pds:0001_nasa_pds_1:pds:tndo_context:pds:instrument:atmospheric_sciences::1.0 rdf:type rdfs:Class;
  rdfs:label "Atmospheric Sciences";
  rdfs:subClassOf pds4:urn:nasa:pds:0001_nasa_pds_1:pds:tndo_context:pds:instrument::1.0;
  rdfs:comment "A top level category for atmospheric science instruments.".
 
pds4:urn:nasa:pds:0001_nasa_pds_1:pds:tndo_context:pds:instrument:atomic_force_microscope::1.0 rdf:type rdfs:Class;
  rdfs:label "Atomic Force Microscope";
  rdfs:subClassOf pds4:urn:nasa:pds:0001_nasa_pds_1:pds:tndo_context:pds:instrument::1.0;
  rdfs:comment "An instrument that uses atomic forces between a probe and a sample to produce high-resolution topographic scans of the sample.".
 
pds4:urn:nasa:pds:0001_nasa_pds_1:pds:tndo_context:pds:instrument:barometer::1.0 rdf:type rdfs:Class;
  rdfs:label "Barometer";
  rdfs:subClassOf pds4:urn:nasa:pds:0001_nasa_pds_1:pds:tndo_context:pds:instrument::1.0;
  rdfs:comment "An in situ instrument that measures atmospheric pressure.".
 
pds4:urn:nasa:pds:0001_nasa_pds_1:pds:tndo_context:pds:instrument:biology_experiments::1.0 rdf:type rdfs:Class;
  rdfs:label "Biology Experiments";
  rdfs:subClassOf pds4:urn:nasa:pds:0001_nasa_pds_1:pds:tndo_context:pds:instrument::1.0;
  rdfs:comment "An instrument that conducts one or more experiments on samples to determine their potential for biological activity.".
 
pds4:urn:nasa:pds:0001_nasa_pds_1:pds:tndo_context:pds:instrument:bolometer::1.0 rdf:type rdfs:Class;
  rdfs:label "Bolometer";
  rdfs:subClassOf pds4:urn:nasa:pds:0001_nasa_pds_1:pds:tndo_context:pds:instrument::1.0;
  rdfs:comment "An instrument that estimates radiation intensity by measuring changes in electrical resistivity as the temperature of its sensor varies in response to the incident power density.".
 
pds4:urn:nasa:pds:0001_nasa_pds_1:pds:tndo_context:pds:instrument:camera::1.0 rdf:type rdfs:Class;
  rdfs:label "Camera";
  rdfs:subClassOf pds4:urn:nasa:pds:0001_nasa_pds_1:pds:tndo_context:pds:instrument::1.0;
  rdfs:comment "An instrument that records and stores analog images (compare \\'imager\\').".
 
pds4:urn:nasa:pds:0001_nasa_pds_1:pds:tndo_context:pds:instrument:cosmic_ray_detector::1.0 rdf:type rdfs:Class;
  rdfs:label "Cosmic Ray Detector";
  rdfs:subClassOf pds4:urn:nasa:pds:0001_nasa_pds_1:pds:tndo_context:pds:instrument::1.0;
  rdfs:comment "An instrument that detects and\\//or measures cosmic rays.".
 
pds4:urn:nasa:pds:0001_nasa_pds_1:pds:tndo_context:pds:instrument:drilling_tool::1.0 rdf:type rdfs:Class;
  rdfs:label "Drilling Tool";
  rdfs:subClassOf pds4:urn:nasa:pds:0001_nasa_pds_1:pds:tndo_context:pds:instrument::1.0;
  rdfs:comment "A tool that drills into samples.".
 
pds4:urn:nasa:pds:0001_nasa_pds_1:pds:tndo_context:pds:instrument:dust::1.0 rdf:type rdfs:Class;
  rdfs:label "Dust";
  rdfs:subClassOf pds4:urn:nasa:pds:0001_nasa_pds_1:pds:tndo_context:pds:instrument::1.0;
  rdfs:comment "An instrument that detects and\\//or measures dust.".
 
pds4:urn:nasa:pds:0001_nasa_pds_1:pds:tndo_context:pds:instrument:dust_detector::1.0 rdf:type rdfs:Class;
  rdfs:label "Dust Detector";
  rdfs:subClassOf pds4:urn:nasa:pds:0001_nasa_pds_1:pds:tndo_context:pds:instrument::1.0;
  rdfs:comment "An instrument that detects and\\//or measures dust.".
 
pds4:urn:nasa:pds:0001_nasa_pds_1:pds:tndo_context:pds:instrument:electrical_probe::1.0 rdf:type rdfs:Class;
  rdfs:label "Electrical Probe";
  rdfs:subClassOf pds4:urn:nasa:pds:0001_nasa_pds_1:pds:tndo_context:pds:instrument::1.0;
  rdfs:comment "An in situ instrument that measures electrical properties (e.g., conductivity) of a medium into which it is inserted.".
 
pds4:urn:nasa:pds:0001_nasa_pds_1:pds:tndo_context:pds:instrument:energetic_particle_detector::1.0 rdf:type rdfs:Class;
  rdfs:label "Energetic Particle Detector";
  rdfs:subClassOf pds4:urn:nasa:pds:0001_nasa_pds_1:pds:tndo_context:pds:instrument::1.0;
  rdfs:comment " An instrument that detects and\\//or measures energetic charged particles.".
 
pds4:urn:nasa:pds:0001_nasa_pds_1:pds:tndo_context:pds:instrument:gamma_ray_detector::1.0 rdf:type rdfs:Class;
  rdfs:label "Gamma Ray Detector";
  rdfs:subClassOf pds4:urn:nasa:pds:0001_nasa_pds_1:pds:tndo_context:pds:instrument::1.0;
  rdfs:comment "An instrument that detects and\\//or measures gamma rays.".
 
pds4:urn:nasa:pds:0001_nasa_pds_1:pds:tndo_context:pds:instrument:gas_analyzer::1.0 rdf:type rdfs:Class;
  rdfs:label "Gas Analyzer";
  rdfs:subClassOf pds4:urn:nasa:pds:0001_nasa_pds_1:pds:tndo_context:pds:instrument::1.0;
  rdfs:comment "A high-temperature furnace combined with a mass spectrometer that heats a sample and analyzes the mass distribution of the evolved gases.".
 
pds4:urn:nasa:pds:0001_nasa_pds_1:pds:tndo_context:pds:instrument:gravimeter::1.0 rdf:type rdfs:Class;
  rdfs:label "Gravimeter";
  rdfs:subClassOf pds4:urn:nasa:pds:0001_nasa_pds_1:pds:tndo_context:pds:instrument::1.0;
  rdfs:comment "An instrument that measures the local gravitational field.".
 
pds4:urn:nasa:pds:0001_nasa_pds_1:pds:tndo_context:pds:instrument:grinding_tool::1.0 rdf:type rdfs:Class;
  rdfs:label "Grinding Tool";
  rdfs:subClassOf pds4:urn:nasa:pds:0001_nasa_pds_1:pds:tndo_context:pds:instrument::1.0;
  rdfs:comment "A tool that grinds into samples.".
 
pds4:urn:nasa:pds:0001_nasa_pds_1:pds:tndo_context:pds:instrument:hygrometer::1.0 rdf:type rdfs:Class;
  rdfs:label "Hygrometer";
  rdfs:subClassOf pds4:urn:nasa:pds:0001_nasa_pds_1:pds:tndo_context:pds:instrument::1.0;
  rdfs:comment "An instrument used to measure the moisture content of its environment.".
 
pds4:urn:nasa:pds:0001_nasa_pds_1:pds:tndo_context:pds:instrument:imager::1.0 rdf:type rdfs:Class;
  rdfs:label "Imager";
  rdfs:subClassOf pds4:urn:nasa:pds:0001_nasa_pds_1:pds:tndo_context:pds:instrument::1.0;
  rdfs:comment "An instrument that records and stores digital images.".
 
pds4:urn:nasa:pds:0001_nasa_pds_1:pds:tndo_context:pds:instrument:imaging_spectrometer::1.0 rdf:type rdfs:Class;
  rdfs:label "Imaging Spectrometer";
  rdfs:subClassOf pds4:urn:nasa:pds:0001_nasa_pds_1:pds:tndo_context:pds:instrument::1.0;
  rdfs:comment "An instrument that combines the functions of a spectrometer and an imager - i.e., it captures and stores multiple images, each at a slightly different wavelength.".
 
pds4:urn:nasa:pds:0001_nasa_pds_1:pds:tndo_context:pds:instrument:inertial_measurement_unit::1.0 rdf:type rdfs:Class;
  rdfs:label "Inertial Measurement Unit";
  rdfs:subClassOf pds4:urn:nasa:pds:0001_nasa_pds_1:pds:tndo_context:pds:instrument::1.0;
  rdfs:comment "An instrument that measures changes in its own velocity and orientation by using a combination of accelerometers, gyroscopes, and\\//or other devices.".
 
pds4:urn:nasa:pds:0001_nasa_pds_1:pds:tndo_context:pds:instrument:infrared_spectrometer::1.0 rdf:type rdfs:Class;
  rdfs:label "Infrared Spectrometer";
  rdfs:subClassOf pds4:urn:nasa:pds:0001_nasa_pds_1:pds:tndo_context:pds:instrument::1.0;
  rdfs:comment "An instrument that measures the spectral distribution of infrared radiation.".
 
pds4:urn:nasa:pds:0001_nasa_pds_1:pds:tndo_context:pds:instrument:interferometer::1.0 rdf:type rdfs:Class;
  rdfs:label "Interferometer";
  rdfs:subClassOf pds4:urn:nasa:pds:0001_nasa_pds_1:pds:tndo_context:pds:instrument::1.0;
  rdfs:comment "An instrument used to measure small displacements, refractive index changes and surface irregularities using interferometry.".
 
pds4:urn:nasa:pds:0001_nasa_pds_1:pds:tndo_context:pds:instrument:laser_induced_breakdown_spectrometer::1.0 rdf:type rdfs:Class;
  rdfs:label "Laser Induced Breakdown Spectrometer";
  rdfs:subClassOf pds4:urn:nasa:pds:0001_nasa_pds_1:pds:tndo_context:pds:instrument::1.0;
  rdfs:comment "An instrument that uses an active laser to generate a plasma from a target and then measures the energy spectrum of the evolved plasma.".
 
pds4:urn:nasa:pds:0001_nasa_pds_1:pds:tndo_context:pds:instrument:magnetometer::1.0 rdf:type rdfs:Class;
  rdfs:label "Magnetometer";
  rdfs:subClassOf pds4:urn:nasa:pds:0001_nasa_pds_1:pds:tndo_context:pds:instrument::1.0;
  rdfs:comment "An instrument that measures the strength and\\//or direction of a magnetic field.".
 
pds4:urn:nasa:pds:0001_nasa_pds_1:pds:tndo_context:pds:instrument:mass_spectrometer::1.0 rdf:type rdfs:Class;
  rdfs:label "Mass Spectrometer";
  rdfs:subClassOf pds4:urn:nasa:pds:0001_nasa_pds_1:pds:tndo_context:pds:instrument::1.0;
  rdfs:comment "An instrument that measures the number of particles in a sample as a function of their mass.".
 
pds4:urn:nasa:pds:0001_nasa_pds_1:pds:tndo_context:pds:instrument:microscope::1.0 rdf:type rdfs:Class;
  rdfs:label "Microscope";
  rdfs:subClassOf pds4:urn:nasa:pds:0001_nasa_pds_1:pds:tndo_context:pds:instrument::1.0;
  rdfs:comment "An instrument used to view objects that are too small to be seen by the naked eye.".
 
pds4:urn:nasa:pds:0001_nasa_pds_1:pds:tndo_context:pds:instrument:microwave_spectrometer::1.0 rdf:type rdfs:Class;
  rdfs:label "Microwave Spectrometer";
  rdfs:subClassOf pds4:urn:nasa:pds:0001_nasa_pds_1:pds:tndo_context:pds:instrument::1.0;
  rdfs:comment "An instrument that measures the spectral distribution of microwave radiation.".
 
pds4:urn:nasa:pds:0001_nasa_pds_1:pds:tndo_context:pds:instrument:moessbauer_spectrometer::1.0 rdf:type rdfs:Class;
  rdfs:label "Moessbauer Spectrometer";
  rdfs:subClassOf pds4:urn:nasa:pds:0001_nasa_pds_1:pds:tndo_context:pds:instrument::1.0;
  rdfs:comment "An instrument that uses the Mossbauer effect to determine the abundance of Fe-bearing minerals in a sample.".
 
pds4:urn:nasa:pds:0001_nasa_pds_1:pds:tndo_context:pds:instrument:naked_eye::1.0 rdf:type rdfs:Class;
  rdfs:label "Naked Eye";
  rdfs:subClassOf pds4:urn:nasa:pds:0001_nasa_pds_1:pds:tndo_context:pds:instrument::1.0;
  rdfs:comment "Observations made with the naked eye and recorded in a data product.".
 
pds4:urn:nasa:pds:0001_nasa_pds_1:pds:tndo_context:pds:instrument:neutral_particle_detector::1.0 rdf:type rdfs:Class;
  rdfs:label "Neutral Particle Detector";
  rdfs:subClassOf pds4:urn:nasa:pds:0001_nasa_pds_1:pds:tndo_context:pds:instrument::1.0;
  rdfs:comment "An instrument that detects and\\//or measures neutral particles.".
 
pds4:urn:nasa:pds:0001_nasa_pds_1:pds:tndo_context:pds:instrument:neutron_detector::1.0 rdf:type rdfs:Class;
  rdfs:label "Neutron Detector";
  rdfs:subClassOf pds4:urn:nasa:pds:0001_nasa_pds_1:pds:tndo_context:pds:instrument::1.0;
  rdfs:comment "An instrument that measures the number and\\//or energy distribution of neutrons.".
 
pds4:urn:nasa:pds:0001_nasa_pds_1:pds:tndo_context:pds:instrument:particle_detector::1.0 rdf:type rdfs:Class;
  rdfs:label "Particle Detector";
  rdfs:subClassOf pds4:urn:nasa:pds:0001_nasa_pds_1:pds:tndo_context:pds:instrument::1.0;
  rdfs:comment "An instrument that detects and\\//or measures charged particles.".
 
pds4:urn:nasa:pds:0001_nasa_pds_1:pds:tndo_context:pds:instrument:photometer::1.0 rdf:type rdfs:Class;
  rdfs:label "Photometer";
  rdfs:subClassOf pds4:urn:nasa:pds:0001_nasa_pds_1:pds:tndo_context:pds:instrument::1.0;
  rdfs:comment "An instrument that measures radiation intensity (e.g., of visible light), sometimes with the goal of inferring optical properties of materials.".
 
pds4:urn:nasa:pds:0001_nasa_pds_1:pds:tndo_context:pds:instrument:plasma_analyzer::1.0 rdf:type rdfs:Class;
  rdfs:label "Plasma Analyzer";
  rdfs:subClassOf pds4:urn:nasa:pds:0001_nasa_pds_1:pds:tndo_context:pds:instrument::1.0;
  rdfs:comment "An instrument that measures the spectral distribution of energy in a low-frequency plasma.".
 
pds4:urn:nasa:pds:0001_nasa_pds_1:pds:tndo_context:pds:instrument:plasma_detector::1.0 rdf:type rdfs:Class;
  rdfs:label "Plasma Detector";
  rdfs:subClassOf pds4:urn:nasa:pds:0001_nasa_pds_1:pds:tndo_context:pds:instrument::1.0;
  rdfs:comment "An instrument that detects and\\//or measures low energy charged particles.".
 
pds4:urn:nasa:pds:0001_nasa_pds_1:pds:tndo_context:pds:instrument:plasma_wave_spectrometer::1.0 rdf:type rdfs:Class;
  rdfs:label "Plasma Wave Spectrometer";
  rdfs:subClassOf pds4:urn:nasa:pds:0001_nasa_pds_1:pds:tndo_context:pds:instrument::1.0;
  rdfs:comment "An instrument that measures the energy distribution in a low-frequency plasma.".
 
pds4:urn:nasa:pds:0001_nasa_pds_1:pds:tndo_context:pds:instrument:polarimeter::1.0 rdf:type rdfs:Class;
  rdfs:label "Polarimeter";
  rdfs:subClassOf pds4:urn:nasa:pds:0001_nasa_pds_1:pds:tndo_context:pds:instrument::1.0;
  rdfs:comment "An instrument used to measure the angle of rotation caused by passing polarized electromagnetic radiation through an optically active substance.".
 
pds4:urn:nasa:pds:0001_nasa_pds_1:pds:tndo_context:pds:instrument:radar::1.0 rdf:type rdfs:Class;
  rdfs:label "Radar";
  rdfs:subClassOf pds4:urn:nasa:pds:0001_nasa_pds_1:pds:tndo_context:pds:instrument::1.0;
  rdfs:comment "An instrument that transmits and receives radio signals for the purpose of detecting, determining the range (distance) to, velocity of, and\\//or direction of one or more distant targets.".
 
pds4:urn:nasa:pds:0001_nasa_pds_1:pds:tndo_context:pds:instrument:radio_science::1.0 rdf:type rdfs:Class;
  rdfs:label "Radio Science";
  rdfs:subClassOf pds4:urn:nasa:pds:0001_nasa_pds_1:pds:tndo_context:pds:instrument::1.0;
  rdfs:comment "An instrument suite used to conduct measurements at radio frequencies.".
 
pds4:urn:nasa:pds:0001_nasa_pds_1:pds:tndo_context:pds:instrument:radio_spectrometer::1.0 rdf:type rdfs:Class;
  rdfs:label "Radio Spectrometer";
  rdfs:subClassOf pds4:urn:nasa:pds:0001_nasa_pds_1:pds:tndo_context:pds:instrument::1.0;
  rdfs:comment "An instrument that measures the spectral distribution of electromagnetic radiation at radio frequencies.".
 
pds4:urn:nasa:pds:0001_nasa_pds_1:pds:tndo_context:pds:instrument:radio_telescope::1.0 rdf:type rdfs:Class;
  rdfs:label "Radio Telescope";
  rdfs:subClassOf pds4:urn:nasa:pds:0001_nasa_pds_1:pds:tndo_context:pds:instrument::1.0;
  rdfs:comment " An instrument used to focus and capture radio waves.".
 
pds4:urn:nasa:pds:0001_nasa_pds_1:pds:tndo_context:pds:instrument:radio-radar::1.0 rdf:type rdfs:Class;
  rdfs:label "Radio-Radar";
  rdfs:subClassOf pds4:urn:nasa:pds:0001_nasa_pds_1:pds:tndo_context:pds:instrument::1.0;
  rdfs:comment "An instrument used to conduct measurements at radio frequencies.".
 
pds4:urn:nasa:pds:0001_nasa_pds_1:pds:tndo_context:pds:instrument:radiometer::1.0 rdf:type rdfs:Class;
  rdfs:label "Radiometer";
  rdfs:subClassOf pds4:urn:nasa:pds:0001_nasa_pds_1:pds:tndo_context:pds:instrument::1.0;
  rdfs:comment "An instrument which measures the radiant flux of electromagnetic radiation.".
 
pds4:urn:nasa:pds:0001_nasa_pds_1:pds:tndo_context:pds:instrument:reflectometer::1.0 rdf:type rdfs:Class;
  rdfs:label "Reflectometer";
  rdfs:subClassOf pds4:urn:nasa:pds:0001_nasa_pds_1:pds:tndo_context:pds:instrument::1.0;
  rdfs:comment "An instrument that measures the reflectance of surfaces.  An electron reflectometer measures the properties of electrons trapped along magnetic field lines to infer the strength and direction of the field remotely.".
 
pds4:urn:nasa:pds:0001_nasa_pds_1:pds:tndo_context:pds:instrument:regolith_properties::1.0 rdf:type rdfs:Class;
  rdfs:label "Regolith Properties";
  rdfs:subClassOf pds4:urn:nasa:pds:0001_nasa_pds_1:pds:tndo_context:pds:instrument::1.0;
  rdfs:comment "A top level category for the science instruments associated with the Geosciences.".
 
pds4:urn:nasa:pds:0001_nasa_pds_1:pds:tndo_context:pds:instrument:robotic_arm::1.0 rdf:type rdfs:Class;
  rdfs:label "Robotic Arm";
  rdfs:subClassOf pds4:urn:nasa:pds:0001_nasa_pds_1:pds:tndo_context:pds:instrument::1.0;
  rdfs:comment "A tool used to place in-situ instruments on surface rocks or soil, dig into a surface, and\\//or to collect surface samples for other instruments to analyze on a spacecraft.".
 
pds4:urn:nasa:pds:0001_nasa_pds_1:pds:tndo_context:pds:instrument:seismometer::1.0 rdf:type rdfs:Class;
  rdfs:label "Seismometer";
  rdfs:subClassOf pds4:urn:nasa:pds:0001_nasa_pds_1:pds:tndo_context:pds:instrument::1.0;
  rdfs:comment "An instrument that measure motion of the ground.".
 
pds4:urn:nasa:pds:0001_nasa_pds_1:pds:tndo_context:pds:instrument:small_bodies_sciences::1.0 rdf:type rdfs:Class;
  rdfs:label "Small Bodies Sciences";
  rdfs:subClassOf pds4:urn:nasa:pds:0001_nasa_pds_1:pds:tndo_context:pds:instrument::1.0;
  rdfs:comment "A top level category for the science instruments associated with Small Bodies.".
 
pds4:urn:nasa:pds:0001_nasa_pds_1:pds:tndo_context:pds:instrument:spectrograph::1.0 rdf:type rdfs:Class;
  rdfs:label "Spectrograph";
  rdfs:subClassOf pds4:urn:nasa:pds:0001_nasa_pds_1:pds:tndo_context:pds:instrument::1.0;
  rdfs:comment "An instrument that separates light into a frequency spectrum and records the signal using a camera.".
 
pds4:urn:nasa:pds:0001_nasa_pds_1:pds:tndo_context:pds:instrument:spectrograph_imager::1.0 rdf:type rdfs:Class;
  rdfs:label "Spectrograph Imager";
  rdfs:subClassOf pds4:urn:nasa:pds:0001_nasa_pds_1:pds:tndo_context:pds:instrument::1.0;
  rdfs:comment "See Imaging Spectrometer.".
 
pds4:urn:nasa:pds:0001_nasa_pds_1:pds:tndo_context:pds:instrument:spectrometer::1.0 rdf:type rdfs:Class;
  rdfs:label "Spectrometer";
  rdfs:subClassOf pds4:urn:nasa:pds:0001_nasa_pds_1:pds:tndo_context:pds:instrument::1.0;
  rdfs:comment "An instrument that measures a spectrum, reporting intensity as a function of wavelength, frequency, energy, momentum, or mass.".
 
pds4:urn:nasa:pds:0001_nasa_pds_1:pds:tndo_context:pds:instrument:thermal_imager::1.0 rdf:type rdfs:Class;
  rdfs:label "Thermal Imager";
  rdfs:subClassOf pds4:urn:nasa:pds:0001_nasa_pds_1:pds:tndo_context:pds:instrument::1.0;
  rdfs:comment "An instrument that captures an image at thermal infrared wavelengths.".
 
pds4:urn:nasa:pds:0001_nasa_pds_1:pds:tndo_context:pds:instrument:thermal_probe::1.0 rdf:type rdfs:Class;
  rdfs:label "Thermal Probe";
  rdfs:subClassOf pds4:urn:nasa:pds:0001_nasa_pds_1:pds:tndo_context:pds:instrument::1.0;
  rdfs:comment "An in situ instrument that measures thermal properties (e.g., temperature) at one or more points along its length.".
 
pds4:urn:nasa:pds:0001_nasa_pds_1:pds:tndo_context:pds:instrument:thermometer::1.0 rdf:type rdfs:Class;
  rdfs:label "Thermometer";
  rdfs:subClassOf pds4:urn:nasa:pds:0001_nasa_pds_1:pds:tndo_context:pds:instrument::1.0;
  rdfs:comment "An instrument that measures temperature.".
 
pds4:urn:nasa:pds:0001_nasa_pds_1:pds:tndo_context:pds:instrument:ultraviolet_spectrometer::1.0 rdf:type rdfs:Class;
  rdfs:label "Ultraviolet Spectrometer";
  rdfs:subClassOf pds4:urn:nasa:pds:0001_nasa_pds_1:pds:tndo_context:pds:instrument::1.0;
  rdfs:comment "An instrument that measures the spectral distribution of ultraviolet radiation.".
 
pds4:urn:nasa:pds:0001_nasa_pds_1:pds:tndo_context:pds:instrument:weather_station::1.0 rdf:type rdfs:Class;
  rdfs:label "Weather Station";
  rdfs:subClassOf pds4:urn:nasa:pds:0001_nasa_pds_1:pds:tndo_context:pds:instrument::1.0;
  rdfs:comment "An instrument that collects data for the scientific study of weather and weather-related phenomena such as (but not limited to) temperature, pressure, wind speed, wind direction, etc.".
 
pds4:urn:nasa:pds:0001_nasa_pds_1:pds:tndo_context:pds:instrument:wet_chemistry_laboratory::1.0 rdf:type rdfs:Class;
  rdfs:label "Wet Chemistry Laboratory";
  rdfs:subClassOf pds4:urn:nasa:pds:0001_nasa_pds_1:pds:tndo_context:pds:instrument::1.0;
  rdfs:comment "An instrument that mixes soil samples with solutions to measure material properties such as pH, conductivity, oxidation-reduction potential, etc.".
 
pds4:urn:nasa:pds:0001_nasa_pds_1:pds:tndo_context:pds:instrument:x-ray_detector::1.0 rdf:type rdfs:Class;
  rdfs:label "X-ray Detector";
  rdfs:subClassOf pds4:urn:nasa:pds:0001_nasa_pds_1:pds:tndo_context:pds:instrument::1.0;
  rdfs:comment "An instrument that detects and\\//or measures X-rays.".
 
pds4:urn:nasa:pds:0001_nasa_pds_1:pds:tndo_context:pds:instrument:x-ray_diffraction_spectrometer::1.0 rdf:type rdfs:Class;
  rdfs:label "X-ray Diffraction Spectrometer";
  rdfs:subClassOf pds4:urn:nasa:pds:0001_nasa_pds_1:pds:tndo_context:pds:instrument::1.0;
  rdfs:comment "An instrument that uses a beam of X-rays to probe the internal structure of a powdered sample and identify its mineral composition.".
 
pds4:urn:nasa:pds:0001_nasa_pds_1:pds:tndo_context:pds:instrument:x-ray_fluorescence_spectrometer::1.0 rdf:type rdfs:Class;
  rdfs:label "X-ray Fluorescence Spectrometer";
  rdfs:subClassOf pds4:urn:nasa:pds:0001_nasa_pds_1:pds:tndo_context:pds:instrument::1.0;
  rdfs:comment "An instrument that measures the emission of secondary X-rays to determine the elemental composition of a sample that has been irradiated with primary X-rays.".
 
pds4:urn:nasa:pds:0001_nasa_pds_1:pds:tndo_context:pds:instrument_host::1.0 rdf:type rdfs:Class;
  rdfs:label "Instrument_Host";
  pds4:subClassOf pds4:urn:nasa:pds:0001_nasa_pds_1:pds:tagged_nondigital_object:pds:tndo_context::1.0;
  rdfs:comment "The Instrument Host class provides a description of the physical object upon which an instrument is mounted.".
 
pds4:urn:nasa:pds:0001_nasa_pds_1:pds:tndo_context:pds:instrument_host:aircraft::1.0 rdf:type rdfs:Class;
  rdfs:label "Aircraft";
  rdfs:subClassOf pds4:urn:nasa:pds:0001_nasa_pds_1:pds:tndo_context:pds:instrument_host::1.0;
  rdfs:comment "An airborne observatory carried on a powered, heavier than air vessel supporting observations, measurements, and scientific experiments during flight.".
 
pds4:urn:nasa:pds:0001_nasa_pds_1:pds:tndo_context:pds:instrument_host:balloon::1.0 rdf:type rdfs:Class;
  rdfs:label "Balloon";
  rdfs:subClassOf pds4:urn:nasa:pds:0001_nasa_pds_1:pds:tndo_context:pds:instrument_host::1.0;
  rdfs:comment "A balloon-borne observatory, typically consisting of a gondola structure carrying one or more telescopes and instruments, borne aloft by an unpowered or minimially powered lighter-than-atmosphere balloon for a limited observing period.".
 
pds4:urn:nasa:pds:0001_nasa_pds_1:pds:tndo_context:pds:instrument_host:earth_based::1.0 rdf:type rdfs:Class;
  rdfs:label "Earth Based";
  rdfs:subClassOf pds4:urn:nasa:pds:0001_nasa_pds_1:pds:tndo_context:pds:instrument_host::1.0;
  rdfs:comment "The Instrument Host is classified as being of type Earth Based".
 
pds4:urn:nasa:pds:0001_nasa_pds_1:pds:tndo_context:pds:instrument_host:earth-based::1.0 rdf:type rdfs:Class;
  rdfs:label "Earth-based";
  rdfs:subClassOf pds4:urn:nasa:pds:0001_nasa_pds_1:pds:tndo_context:pds:instrument_host::1.0;
  rdfs:comment "The instrument host is on or near the surface of Earth (no more than 100 km altitude above the surface).".
 
pds4:urn:nasa:pds:0001_nasa_pds_1:pds:tndo_context:pds:instrument_host:lander::1.0 rdf:type rdfs:Class;
  rdfs:label "Lander";
  rdfs:subClassOf pds4:urn:nasa:pds:0001_nasa_pds_1:pds:tndo_context:pds:instrument_host::1.0;
  rdfs:comment "A spacecraft designed for descent to and operation at a single fixed point on the surface of a celestial body.".
 
pds4:urn:nasa:pds:0001_nasa_pds_1:pds:tndo_context:pds:instrument_host:rover::1.0 rdf:type rdfs:Class;
  rdfs:label "Rover";
  rdfs:subClassOf pds4:urn:nasa:pds:0001_nasa_pds_1:pds:tndo_context:pds:instrument_host::1.0;
  rdfs:comment "A spacecraft designed for descent to and mobile operation on the surface of a celestial body.".
 
pds4:urn:nasa:pds:0001_nasa_pds_1:pds:tndo_context:pds:instrument_host:spacecraft::1.0 rdf:type rdfs:Class;
  rdfs:label "Spacecraft";
  rdfs:subClassOf pds4:urn:nasa:pds:0001_nasa_pds_1:pds:tndo_context:pds:instrument_host::1.0;
  rdfs:comment "A vehicle designed for travel in outer space (\\'outer space\\' is the region more than 100 km above the Earth\\'s surface, a convention accepted in many contexts -- see http:\\//\\//en.wikipedia.org\\//wiki\\//Outer_space).".
 
pds4:urn:nasa:pds:0001_nasa_pds_1:pds:tndo_context:pds:instrument_host:suborbital_rocket::1.0 rdf:type rdfs:Class;
  rdfs:label "Suborbital Rocket";
  rdfs:subClassOf pds4:urn:nasa:pds:0001_nasa_pds_1:pds:tndo_context:pds:instrument_host::1.0;
  rdfs:comment "A Suborbital Rocket is an instrument-carrying rocket designed to take measurements and perform scientific experiments during its sub-orbital flight.".
 
pds4:urn:nasa:pds:0001_nasa_pds_1:pds:tndo_context_pds3:pds:instrument_host_pds3::1.0 rdf:type rdfs:Class;
  rdfs:label "Instrument_Host_PDS3";
  pds4:subClassOf pds4:urn:nasa:pds:0001_nasa_pds_1:pds:tagged_nondigital_object:pds:tndo_context_pds3::1.0;
  rdfs:comment "The Instrument Host class provides a description of the phyiscal object upon which an instrument is mounted. This class captures the PDS3 catalog Instrument Host information.".
 
pds4:urn:nasa:pds:0001_nasa_pds_1:all:user:img_surface:instrument_information::1.0 rdf:type rdfs:Class;
  rdfs:label "Instrument_Information";
  pds4:subClassOf pds4:urn:nasa:pds:0001_nasa_pds_1:all:user::1.0;
  rdfs:comment "The Instrument_Information class specifies information about the configuration of the instrument as it acquired this observation.".
 
pds4:urn:nasa:pds:0001_nasa_pds_1:pds:tndo_context_pds3:pds:instrument_pds3::1.0 rdf:type rdfs:Class;
  rdfs:label "Instrument_PDS3";
  pds4:subClassOf pds4:urn:nasa:pds:0001_nasa_pds_1:pds:tagged_nondigital_object:pds:tndo_context_pds3::1.0;
  rdfs:comment "The Instrument class provides a description of a phyiscal object that collects data. This class captures the PDS3 catalog Instrument information.".
 
pds4:urn:nasa:pds:0001_nasa_pds_1:all:user:nucspec:instrument_settings::1.0 rdf:type rdfs:Class;
  rdfs:label "Instrument_Settings";
  pds4:subClassOf pds4:urn:nasa:pds:0001_nasa_pds_1:all:user::1.0;
  rdfs:comment "This class specifies instrument settings. Instrument settings may be driven via a state table, which may be associated with specific observations within the data product, either by directly indicating those records, or indicating the observation times at which certain states apply.".
 
pds4:urn:nasa:pds:0001_nasa_pds_1:all:user:img:instrument_state::1.0 rdf:type rdfs:Class;
  rdfs:label "Instrument_State";
  pds4:subClassOf pds4:urn:nasa:pds:0001_nasa_pds_1:all:user::1.0;
  rdfs:comment "The Instrument_State class contains classes providing the values of any dynamic physical or operating characteristics of the imaging instruments.".
 
pds4:urn:nasa:pds:0001_nasa_pds_1:pds:product_components:pds:internal_reference::1.0 rdf:type rdfs:Class;
  rdfs:label "Internal_Reference";
  pds4:subClassOf pds4:urn:nasa:pds:0001_nasa_pds_1:all:user:pds:product_components::1.0;
  rdfs:comment "The Internal_Reference class is used to cross-reference other products in PDS4-compliant registries of PDS and its recognized international partners.".
 
pds4:urn:nasa:pds:0001_nasa_pds_1:all:user:geom:interpolation::1.0 rdf:type rdfs:Class;
  rdfs:label "Interpolation";
  pds4:subClassOf pds4:urn:nasa:pds:0001_nasa_pds_1:all:user::1.0;
  rdfs:comment "The Interpolation class defines how the camera model was interpolated from the calibration models. Interpolation is used to create models in a variable space (e.g., focus, zoom) between points at which calibration was performed. If more than one dimension of variables were interpolated, multiple Interpolation objects can exist, with interpolation_sequence defining the order. ".
 
pds4:urn:nasa:pds:0001_nasa_pds_1:pds:table_delimited:pds:inventory::1.0 rdf:type rdfs:Class;
  rdfs:label "Inventory";
  pds4:subClassOf pds4:urn:nasa:pds:0001_nasa_pds_1:pds:parsable_byte_stream:pds:table_delimited::1.0;
  rdfs:comment "The Inventory class defines the inventory for members of a collection.".
 
pds4:urn:nasa:pds:0001_nasa_pds_1:pds:tndo_context:pds:investigation::1.0 rdf:type rdfs:Class;
  rdfs:label "Investigation";
  pds4:subClassOf pds4:urn:nasa:pds:0001_nasa_pds_1:pds:tagged_nondigital_object:pds:tndo_context::1.0;
  rdfs:comment "A set of experiments and\\//or observations with a clearly defined purpose.".
 
pds4:urn:nasa:pds:0001_nasa_pds_1:pds:tndo_context:pds:investigation:field_campaign::1.0 rdf:type rdfs:Class;
  rdfs:label "Field Campaign";
  rdfs:subClassOf pds4:urn:nasa:pds:0001_nasa_pds_1:pds:tndo_context:pds:investigation::1.0;
  rdfs:comment "A set of experiments and\\//or observations with a clearly defined purpose that is coordinated among one or more individuals and\\//or one or more organizations. The campaign is characterized primarily by its in situ terrestrial field work.".
 
pds4:urn:nasa:pds:0001_nasa_pds_1:pds:tndo_context:pds:investigation:individual_investigation::1.0 rdf:type rdfs:Class;
  rdfs:label "Individual Investigation";
  rdfs:subClassOf pds4:urn:nasa:pds:0001_nasa_pds_1:pds:tndo_context:pds:investigation::1.0;
  rdfs:comment "A set of experiments and\\//or observations with a clearly defined purpose that is under the direction of a single individual. For example, a series of related laboratory experiments\\//observations conducted by a small university team and funded through a single proposal could be an Individual Investigation. Library research by one person on previously published results to distill common conclusions could also be an Individual Investigation.".
 
pds4:urn:nasa:pds:0001_nasa_pds_1:pds:tndo_context:pds:investigation:mission::1.0 rdf:type rdfs:Class;
  rdfs:label "Mission";
  rdfs:subClassOf pds4:urn:nasa:pds:0001_nasa_pds_1:pds:tndo_context:pds:investigation::1.0;
  rdfs:comment "A set of experiments and\\//or observations with a clearly defined purpose that is under the direction of an organization (such as a national space agency) and uses one or more vehicles of similar design. A mission is usually conducted by a national or international space agency using a small number (often one) of spacecraft especially designed and built for the purpose. For example: (1) the NASA Voyager mission launched two spacecraft to Jupiter and Saturn; (2) the Deep Impact (DI) mission launched a spacecraft, part of which impacted the comet Tempel 2; and (3) the EPOXI mission redefined the objectives of the surviving DI hardware for further exploration of the solar system.".
 
pds4:urn:nasa:pds:0001_nasa_pds_1:pds:tndo_context:pds:investigation:observing_campaign::1.0 rdf:type rdfs:Class;
  rdfs:label "Observing Campaign";
  rdfs:subClassOf pds4:urn:nasa:pds:0001_nasa_pds_1:pds:tndo_context:pds:investigation::1.0;
  rdfs:comment "A set of experiments and\\//or observations with a clearly defined purpose that is coordinated among one or more individuals and\\//or one or more organizations. The campaign is characterized primarily by its remote sensing observations. For example, the International Halley Watch mobilized observatories around the world for collection of data during the most recent apparition of Comet Halley. The Shoemaker-Levy-9 (SL9) campaign used both Earth-based and spacecraft instruments to monitor the SL9 impact on Jupiter.".
 
pds4:urn:nasa:pds:0001_nasa_pds_1:pds:tndo_context:pds:investigation:other_investigation::1.0 rdf:type rdfs:Class;
  rdfs:label "Other Investigation";
  rdfs:subClassOf pds4:urn:nasa:pds:0001_nasa_pds_1:pds:tndo_context:pds:investigation::1.0;
  rdfs:comment "Any other set of experiments and\\//or observations with a unifying theme.".
 
pds4:urn:nasa:pds:0001_nasa_pds_1:pds:product_components:pds:investigation_area::1.0 rdf:type rdfs:Class;
  rdfs:label "Investigation_Area";
  pds4:subClassOf pds4:urn:nasa:pds:0001_nasa_pds_1:all:user:pds:product_components::1.0;
  rdfs:comment "The Investigation_Area class provides information about an investigation (mission, observing campaign or other coordinated, large-scale data collection effort).".
 
pds4:urn:nasa:pds:0001_nasa_pds_1:pds:product_components:pds:investigation_area:field_campaign::1.0 rdf:type rdfs:Class;
  rdfs:label "Field Campaign";
  rdfs:subClassOf pds4:urn:nasa:pds:0001_nasa_pds_1:pds:product_components:pds:investigation_area::1.0;
  rdfs:comment "A set of experiments and\\//or observations with a clearly defined purpose that is coordinated among one or more individuals and\\//or one or more organizations. The campaign is characterized primarily by its in situ terrestrial field work.".
 
pds4:urn:nasa:pds:0001_nasa_pds_1:pds:product_components:pds:investigation_area:individual_investigation::1.0 rdf:type rdfs:Class;
  rdfs:label "Individual Investigation";
  rdfs:subClassOf pds4:urn:nasa:pds:0001_nasa_pds_1:pds:product_components:pds:investigation_area::1.0;
  rdfs:comment "A set of experiments and\\//or observations with a clearly defined purpose that uses existing facilities and is under the direction of a single individual. For example, a series of related laboratory experiments\\//observations conducted by a small university team and funded through a single proposal could be an Individual Investigation. Library research by one person on previously published results to distill common conclusions could also be an Individual Investigation.".
 
pds4:urn:nasa:pds:0001_nasa_pds_1:pds:product_components:pds:investigation_area:mission::1.0 rdf:type rdfs:Class;
  rdfs:label "Mission";
  rdfs:subClassOf pds4:urn:nasa:pds:0001_nasa_pds_1:pds:product_components:pds:investigation_area::1.0;
  rdfs:comment "A set of experiments and\\//or observations with a clearly defined purpose that occupies the designated resources for all (or at least a significant fraction) of the available time. A mission is usually conducted by a national or international space agency using a small number (often one) of spacecraft especially designed and built for the purpose. For example: (1) the NASA Voyager mission launched two spacecraft to Jupiter and Saturn; (2) the Deep Impact (DI) mission launched a spacecraft, part of which impacted the comet Tempel 2; and (3) the EPOXI mission redefined the objectives of the surviving DI hardware for further exploration of the solar system.".
 
pds4:urn:nasa:pds:0001_nasa_pds_1:pds:product_components:pds:investigation_area:observing_campaign::1.0 rdf:type rdfs:Class;
  rdfs:label "Observing Campaign";
  rdfs:subClassOf pds4:urn:nasa:pds:0001_nasa_pds_1:pds:product_components:pds:investigation_area::1.0;
  rdfs:comment "A set of experiments and\\//or observations with a clearly defined purpose that uses (primarily) existing facilities, but not exclusively. After (and possibly during) the campaign other investigations are carried out using the same facilities. For example, the International Halley Watch mobilized observatories around the world for collection of data during the most recent apparition of Comet Halley. The Shoemaker-Levy-9 (SL9) campaign used both Earth-based and spacecraft instruments to monitor the SL9 impact on Jupiter.".
 
pds4:urn:nasa:pds:0001_nasa_pds_1:pds:product_components:pds:investigation_area:other_investigation::1.0 rdf:type rdfs:Class;
  rdfs:label "Other Investigation";
  rdfs:subClassOf pds4:urn:nasa:pds:0001_nasa_pds_1:pds:product_components:pds:investigation_area::1.0;
  rdfs:comment "Any other set of experiments and\\//or observations with a unifying theme.".
 
pds4:urn:nasa:pds:0001_nasa_pds_1:all:user:img:jpeg_parameters::1.0 rdf:type rdfs:Class;
  rdfs:label "JPEG_Parameters";
  pds4:subClassOf pds4:urn:nasa:pds:0001_nasa_pds_1:all:user::1.0;
  rdfs:comment " The JPEG_Parameters class contains attributes describing onboard compression parameters specific to Joint Photographic Experts Group (JPEG) image compression.".
 
pds4:urn:nasa:pds:0001_nasa_pds_1:img:jpeg_parameters:img:jpeg_progressive_parameters::1.0 rdf:type rdfs:Class;
  rdfs:label "JPEG_Progressive_Parameters";
  pds4:subClassOf pds4:urn:nasa:pds:0001_nasa_pds_1:all:user:img:jpeg_parameters::1.0;
  rdfs:comment " The JPEG_Progressive_Parameters class contains attributes describing an interlaced progressive JPEG format, in which data is compressed in multiple passes of progressively higher detail. This is ideal for large images that will be displayed while downloading over a slow connection, allowing a reasonable preview after receiving only a portion of the data.".
 
pds4:urn:nasa:pds:0001_nasa_pds_1:all:user:img:led_illumination_source::1.0 rdf:type rdfs:Class;
  rdfs:label "LED_Illumination_Source";
  pds4:subClassOf pds4:urn:nasa:pds:0001_nasa_pds_1:all:user::1.0;
  rdfs:comment "The LED_Illumination_Source class provides attributes describing an individual LED used to illuminate an imaging target.".
 
pds4:urn:nasa:pds:0001_nasa_pds_1:all:user:img:loco_parameters::1.0 rdf:type rdfs:Class;
  rdfs:label "LOCO_Parameters";
  pds4:subClassOf pds4:urn:nasa:pds:0001_nasa_pds_1:all:user::1.0;
  rdfs:comment " The LOCO_Parameters class contains attributes describing onboard compression parameters specific to Low Complexity Lossless Compression (LOCO) image compression, a lossless submode of ICER".
 
pds4:urn:nasa:pds:0001_nasa_pds_1:all:user:cart:lambert_azimuthal_equal_area::1.0 rdf:type rdfs:Class;
  rdfs:label "Lambert_Azimuthal_Equal_Area";
  pds4:subClassOf pds4:urn:nasa:pds:0001_nasa_pds_1:all:user::1.0;
  rdfs:comment "The Lambert_Azimuthal_Equal_Area class contains parameters for the Lambert Azimuthal Equal-area projection. Synder 1987, DOI:10.3133\\//pp1395, page 182: https:\\//\\//pubs.usgs.gov\\//pp\\//1395\\//report.pdf#page=194 PROJ: https:\\//\\//proj.org\\//operations\\//projections\\//laea.html ".
 
pds4:urn:nasa:pds:0001_nasa_pds_1:all:user:cart:lambert_conformal_conic::1.0 rdf:type rdfs:Class;
  rdfs:label "Lambert_Conformal_Conic";
  pds4:subClassOf pds4:urn:nasa:pds:0001_nasa_pds_1:all:user::1.0;
  rdfs:comment "The Lambert_Conformal_Conic class contains parameters for the Lambert Conformal Conic projection. Synder 1987, DOI:10.3133\\//pp1395, page 104: https:\\//\\//pubs.usgs.gov\\//pp\\//1395\\//report.pdf#page=116 PROJ: https:\\//\\//proj.org\\//operations\\//projections\\//lcc.html ".
 
pds4:urn:nasa:pds:0001_nasa_pds_1:all:user:survey:limiting_magnitudes::1.0 rdf:type rdfs:Class;
  rdfs:label "Limiting_Magnitudes";
  pds4:subClassOf pds4:urn:nasa:pds:0001_nasa_pds_1:all:user::1.0;
  rdfs:comment "The limiting magnitude of the image".
 
pds4:urn:nasa:pds:0001_nasa_pds_1:geom:list_index_base:geom:list_index_angle::1.0 rdf:type rdfs:Class;
  rdfs:label "List_Index_Angle";
  pds4:subClassOf pds4:urn:nasa:pds:0001_nasa_pds_1:all:user:geom:list_index_base::1.0;
  rdfs:comment "Used when the list values are angles. ".
 
pds4:urn:nasa:pds:0001_nasa_pds_1:all:user:geom:list_index_base::1.0 rdf:type rdfs:Class;
  rdfs:label "List_Index_Base";
  pds4:subClassOf pds4:urn:nasa:pds:0001_nasa_pds_1:all:user::1.0;
  rdfs:comment "The List_Index class is an abstract class designed to enable the use of indexed lists. The minimum requirement is at least one of sequence number, name or \"id\", plus the set of values themselves. ".
 
pds4:urn:nasa:pds:0001_nasa_pds_1:geom:list_index_base:geom:list_index_length::1.0 rdf:type rdfs:Class;
  rdfs:label "List_Index_Length";
  pds4:subClassOf pds4:urn:nasa:pds:0001_nasa_pds_1:all:user:geom:list_index_base::1.0;
  rdfs:comment "Used when the list values are lengths.".
 
pds4:urn:nasa:pds:0001_nasa_pds_1:geom:list_index_base:geom:list_index_no_units::1.0 rdf:type rdfs:Class;
  rdfs:label "List_Index_No_Units";
  pds4:subClassOf pds4:urn:nasa:pds:0001_nasa_pds_1:all:user:geom:list_index_base::1.0;
  rdfs:comment "Used when the list values have no units.".
 
pds4:urn:nasa:pds:0001_nasa_pds_1:all:user:img:list_index_no_units_imaging::1.0 rdf:type rdfs:Class;
  rdfs:label "List_Index_No_Units_Imaging";
  pds4:subClassOf pds4:urn:nasa:pds:0001_nasa_pds_1:all:user::1.0;
  rdfs:comment "Used when the list values have no units. ".
 
pds4:urn:nasa:pds:0001_nasa_pds_1:geom:list_index_base:geom:list_index_temperature::1.0 rdf:type rdfs:Class;
  rdfs:label "List_Index_Temperature";
  pds4:subClassOf pds4:urn:nasa:pds:0001_nasa_pds_1:all:user:geom:list_index_base::1.0;
  rdfs:comment "Used when the list values are temperatures. They may also have accompanying temperature counts using index_value_number. ".
 
pds4:urn:nasa:pds:0001_nasa_pds_1:geom:list_index_base:geom:list_index_text::1.0 rdf:type rdfs:Class;
  rdfs:label "List_Index_Text";
  pds4:subClassOf pds4:urn:nasa:pds:0001_nasa_pds_1:all:user:geom:list_index_base::1.0;
  rdfs:comment "Used when the list values are strings.".
 
pds4:urn:nasa:pds:0001_nasa_pds_1:all:user:cart:local::1.0 rdf:type rdfs:Class;
  rdfs:label "Local";
  pds4:subClassOf pds4:urn:nasa:pds:0001_nasa_pds_1:all:user::1.0;
  rdfs:comment "The Local class provides a description of any coordinate system that is not aligned with the surface of the planet. ".
 
pds4:urn:nasa:pds:0001_nasa_pds_1:pds:tagged_digital_child:pds:local_id_reference::1.0 rdf:type rdfs:Class;
  rdfs:label "Local_ID_Reference";
  pds4:subClassOf pds4:urn:nasa:pds:0001_nasa_pds_1:all:user:pds:tagged_digital_child::1.0;
  rdfs:comment "The Local_ID_Reference class defines a one directional relationship by referencing another description object in the label.".
 
pds4:urn:nasa:pds:0001_nasa_pds_1:pds:tagged_digital_child:pds:local_id_relation::1.0 rdf:type rdfs:Class;
  rdfs:label "Local_ID_Relation";
  pds4:subClassOf pds4:urn:nasa:pds:0001_nasa_pds_1:all:user:pds:tagged_digital_child::1.0;
  rdfs:comment "The Local_ID_Relation class defines a one directional relationship between two description objects in the label.".
 
pds4:urn:nasa:pds:0001_nasa_pds_1:pds:product_components:pds:local_internal_reference::1.0 rdf:type rdfs:Class;
  rdfs:label "Local_Internal_Reference";
  pds4:subClassOf pds4:urn:nasa:pds:0001_nasa_pds_1:all:user:pds:product_components::1.0;
  rdfs:comment "The Local Internal_Reference class is used to cross-reference other Description Objects in a PDS4 label.".
 
pds4:urn:nasa:pds:0001_nasa_pds_1:all:user:cart:local_planar::1.0 rdf:type rdfs:Class;
  rdfs:label "Local_Planar";
  pds4:subClassOf pds4:urn:nasa:pds:0001_nasa_pds_1:all:user::1.0;
  rdfs:comment "The Local_Planar class defines any right-handed planar coordinate system of which the z-axis coincides with a plumb line through the origin that locally is aligned with the surface of the planet. ".
 
pds4:urn:nasa:pds:0001_nasa_pds_1:all:user:msss_cam_mh:msss_camera_mini_header::1.0 rdf:type rdfs:Class;
  rdfs:label "MSSS_Camera_Mini_Header";
  pds4:subClassOf pds4:urn:nasa:pds:0001_nasa_pds_1:all:user::1.0;
  rdfs:comment "The MSSS_Camera_Mini_Header class contains information for cameras developed by Malin Space Science Systems (MSSS) that share a common architecture or digital electronics assembly. Example cameras include Mastcam, MAHLI, MARDI, Mastcam-Z, SHERLOC-Watson and SHERLOC-ACI.".
 
pds4:urn:nasa:pds:0001_nasa_pds_1:pds:table_delimited:pds:manifest_sip_deep_archive::1.0 rdf:type rdfs:Class;
  rdfs:label "Manifest_SIP_Deep_Archive";
  pds4:subClassOf pds4:urn:nasa:pds:0001_nasa_pds_1:pds:parsable_byte_stream:pds:table_delimited::1.0;
  rdfs:comment "The Manifest SIP Deep Archive class is a Table Delimited for the NASA planetary science deep archive\\'s Submission Information Package (SIP).".
 
pds4:urn:nasa:pds:0001_nasa_pds_1:all:user:cart:map_projection::1.0 rdf:type rdfs:Class;
  rdfs:label "Map_Projection";
  pds4:subClassOf pds4:urn:nasa:pds:0001_nasa_pds_1:all:user::1.0;
  rdfs:comment "The Map_Projection class provides the systematic representation of all or part of the surface of a planet on a plane (or Cartesian system). ".
 
pds4:urn:nasa:pds:0001_nasa_pds_1:all:user:cart:map_projection_lander::1.0 rdf:type rdfs:Class;
  rdfs:label "Map_Projection_Lander";
  pds4:subClassOf pds4:urn:nasa:pds:0001_nasa_pds_1:all:user::1.0;
  rdfs:comment "The Map_Projection class provides the systematic representation of all or part of the surface of a planet on a plane or developable surface from the perspective of an in-situ spacecraft.".
 
pds4:urn:nasa:pds:0001_nasa_pds_1:all:user:cart:map_projection_rings::1.0 rdf:type rdfs:Class;
  rdfs:label "Map_Projection_Rings";
  pds4:subClassOf pds4:urn:nasa:pds:0001_nasa_pds_1:all:user::1.0;
  rdfs:comment "The Map_Projection_Rings class provides the systematic representation of all or part of the rings of a planet on a plane.".
 
pds4:urn:nasa:pds:0001_nasa_pds_1:all:user:speclib:measurement_instrument::1.0 rdf:type rdfs:Class;
  rdfs:label "Measurement_Instrument";
  pds4:subClassOf pds4:urn:nasa:pds:0001_nasa_pds_1:all:user::1.0;
  rdfs:comment "The Measurement_Instrument class contains attributes that identify the instrument that made the measurement. ".
 
pds4:urn:nasa:pds:0001_nasa_pds_1:all:user:speclib:measurement_parameters::1.0 rdf:type rdfs:Class;
  rdfs:label "Measurement_Parameters";
  pds4:subClassOf pds4:urn:nasa:pds:0001_nasa_pds_1:all:user::1.0;
  rdfs:comment "The Measurement_Parameters class contains attributes relevant to a single measurement of a specimen. ".
 
pds4:urn:nasa:pds:0001_nasa_pds_1:all:user:cart:mercator::1.0 rdf:type rdfs:Class;
  rdfs:label "Mercator";
  pds4:subClassOf pds4:urn:nasa:pds:0001_nasa_pds_1:all:user::1.0;
  rdfs:comment "The Mercator class contains parameters for the Mercator projection. Synder 1987, DOI:10.3133\\//pp1395, page 38: https:\\//\\//pubs.usgs.gov\\//pp\\//1395\\//report.pdf#page=50 PROJ: https:\\//\\//proj.org\\//operations\\//projections\\//merc.html ".
 
pds4:urn:nasa:pds:0001_nasa_pds_1:pds:product_components:pds:mission_area::1.0 rdf:type rdfs:Class;
  rdfs:label "Mission_Area";
  pds4:subClassOf pds4:urn:nasa:pds:0001_nasa_pds_1:all:user:pds:product_components::1.0;
  rdfs:comment "The mission area allows the insertion of mission specific metadata.".
 
pds4:urn:nasa:pds:0001_nasa_pds_1:all:user:msn:mission_information::1.0 rdf:type rdfs:Class;
  rdfs:label "Mission_Information";
  pds4:subClassOf pds4:urn:nasa:pds:0001_nasa_pds_1:all:user::1.0;
  rdfs:comment "The Mission_Information class provides information about a mission.".
 
pds4:urn:nasa:pds:0001_nasa_pds_1:pds:tndo_context_pds3:pds:mission_pds3::1.0 rdf:type rdfs:Class;
  rdfs:label "Mission_PDS3";
  pds4:subClassOf pds4:urn:nasa:pds:0001_nasa_pds_1:pds:tagged_nondigital_object:pds:tndo_context_pds3::1.0;
  rdfs:comment "The Mission PDS3 class describes an activity involved in the collection of data. This class captures the PDS3 catalog Mission information.".
 
pds4:urn:nasa:pds:0001_nasa_pds_1:pds:product_components:pds:modification_detail::1.0 rdf:type rdfs:Class;
  rdfs:label "Modification_Detail";
  pds4:subClassOf pds4:urn:nasa:pds:0001_nasa_pds_1:all:user:pds:product_components::1.0;
  rdfs:comment "The Modification_Detail class provides the details of one round of modification for the product.  The first, required, instance of this class documents the date the product was first registered.".
 
pds4:urn:nasa:pds:0001_nasa_pds_1:pds:product_components:pds:modification_history::1.0 rdf:type rdfs:Class;
  rdfs:label "Modification_History";
  pds4:subClassOf pds4:urn:nasa:pds:0001_nasa_pds_1:all:user:pds:product_components::1.0;
  rdfs:comment "The Modification_History class tracks the history of changes made to the product once it enters the registry system.".
 
pds4:urn:nasa:pds:0001_nasa_pds_1:all:user:geom:motion_counter::1.0 rdf:type rdfs:Class;
  rdfs:label "Motion_Counter";
  pds4:subClassOf pds4:urn:nasa:pds:0001_nasa_pds_1:all:user::1.0;
  rdfs:comment "The Motion_Counter class provides a set of integers that describe a (potentially) unique location (position \\// orientation) for a rover or other movable object. Each time an event occurs that results in a movement, a new motion counter value is created. This includes intentional motion due to drive commands, as well as potential motion due to other articulating devices, such as arms or antennae. This motion counter (or part of it) is used as a reference to define instances of coordinate systems that can move such as SITE or ROVER frames. The motion counter is defined in a mission-specific manner. Although the original intent was to have incrementing indices (e.g., MER), the motion counter could also contain any integer values that conform to the above definition, such as time or spacecraft clock values. ".
 
pds4:urn:nasa:pds:0001_nasa_pds_1:geom:list_index_no_units:geom:motion_counter_index::1.0 rdf:type rdfs:Class;
  rdfs:label "Motion_Counter_Index";
  pds4:subClassOf pds4:urn:nasa:pds:0001_nasa_pds_1:geom:list_index_base:geom:list_index_no_units::1.0;
  rdfs:comment "The Motion_Counter_Index class identifies and populates one element of a Motion_Counter list. The class should be repeated for each element of the list. ".
 
pds4:urn:nasa:pds:0001_nasa_pds_1:all:user:disp:movie_display_settings::1.0 rdf:type rdfs:Class;
  rdfs:label "Movie_Display_Settings";
  pds4:subClassOf pds4:urn:nasa:pds:0001_nasa_pds_1:all:user::1.0;
  rdfs:comment "The Movie_Display_Settings class provides default values for the display of a multi-banded Array using a software application capable of displaying video content.".
 
pds4:urn:nasa:pds:0001_nasa_pds_1:pds:tagged_nondigital_child:pds:nssdc::1.0 rdf:type rdfs:Class;
  rdfs:label "NSSDC";
  pds4:subClassOf pds4:urn:nasa:pds:0001_nasa_pds_1:all:user:pds:tagged_nondigital_child::1.0;
  rdfs:comment "The NSSDC Information class provides identification information for data submitted to the NSSDC.".
 
pds4:urn:nasa:pds:0001_nasa_pds_1:all:user:survey:n_sigma_limit::1.0 rdf:type rdfs:Class;
  rdfs:label "N_Sigma_Limit";
  pds4:subClassOf pds4:urn:nasa:pds:0001_nasa_pds_1:all:user::1.0;
  rdfs:comment "The limiting magnitude of a point source at a significance of n-sigma (i.e. a S\\//N of n)".
 
pds4:urn:nasa:pds:0001_nasa_pds_1:pds:tndo_context:pds:node::1.0 rdf:type rdfs:Class;
  rdfs:label "Node";
  pds4:subClassOf pds4:urn:nasa:pds:0001_nasa_pds_1:pds:tagged_nondigital_object:pds:tndo_context::1.0;
  rdfs:comment "The Node class provides a description of an entity that provides local governance within the federated Planetary Data System.".
 
pds4:urn:nasa:pds:0001_nasa_pds_1:all:user:rings:normal_mode_parameters::1.0 rdf:type rdfs:Class;
  rdfs:label "Normal_Mode_Parameters";
  pds4:subClassOf pds4:urn:nasa:pds:0001_nasa_pds_1:all:user::1.0;
  rdfs:comment "This class provides the normal mode parameters is one is present in the described ring.".
 
pds4:urn:nasa:pds:0001_nasa_pds_1:all:user:nucspec:nucspec_observation_properties::1.0 rdf:type rdfs:Class;
  rdfs:label "NucSpec_Observation_Properties";
  pds4:subClassOf pds4:urn:nasa:pds:0001_nasa_pds_1:all:user::1.0;
  rdfs:comment "This class specifies properties pertaining to a nuclear spectroscopy observation.".
 
pds4:urn:nasa:pds:0001_nasa_pds_1:all:user:geom:object_orientation_clock_angles::1.0 rdf:type rdfs:Class;
  rdfs:label "Object_Orientation_Clock_Angles";
  pds4:subClassOf pds4:urn:nasa:pds:0001_nasa_pds_1:all:user::1.0;
  rdfs:comment "The Object_Orientation_Clock_Angles class provides several clock angles which can be used to describe the orientation of the field of view with respect to various external references such as Celestial or Equatorial North. ".
 
pds4:urn:nasa:pds:0001_nasa_pds_1:all:user:geom:object_orientation_north_east::1.0 rdf:type rdfs:Class;
  rdfs:label "Object_Orientation_North_East";
  pds4:subClassOf pds4:urn:nasa:pds:0001_nasa_pds_1:all:user::1.0;
  rdfs:comment "The Object_Orientation_North_East class provides the parameters needed to describe the orientation of an external coordinate system relative to the image coordinate frame as described by the Display_Direction class. ".
 
pds4:urn:nasa:pds:0001_nasa_pds_1:all:user:geom:object_orientation_ra_dec::1.0 rdf:type rdfs:Class;
  rdfs:label "Object_Orientation_RA_Dec";
  pds4:subClassOf pds4:urn:nasa:pds:0001_nasa_pds_1:all:user::1.0;
  rdfs:comment "The Object_Orientation_RA_Dec class provides the parameters needed to describe the orientation of the celestial reference frame relative to the image coordinate frame as described by the Display_Direction class. ".
 
pds4:urn:nasa:pds:0001_nasa_pds_1:pds:tndo_supplemental:pds:object_statistics::1.0 rdf:type rdfs:Class;
  rdfs:label "Object_Statistics";
  pds4:subClassOf pds4:urn:nasa:pds:0001_nasa_pds_1:pds:tagged_nondigital_object:pds:tndo_supplemental::1.0;
  rdfs:comment "The Object Statistics class provides a set of values that provide metrics about the object.".
 
pds4:urn:nasa:pds:0001_nasa_pds_1:all:user:cart:oblique_cylindrical::1.0 rdf:type rdfs:Class;
  rdfs:label "Oblique_Cylindrical";
  pds4:subClassOf pds4:urn:nasa:pds:0001_nasa_pds_1:all:user::1.0;
  rdfs:comment "The Oblique_Cylindrical class contains parameters for the Oblique Cylindrical projection. Synder 1987, DOI:10.3133\\//pp1395, page 93: https:\\//\\//pubs.usgs.gov\\//pp\\//1395\\//report.pdf#page=105 ".
 
pds4:urn:nasa:pds:0001_nasa_pds_1:all:user:cart:oblique_line_azimuth::1.0 rdf:type rdfs:Class;
  rdfs:label "Oblique_Line_Azimuth";
  pds4:subClassOf pds4:urn:nasa:pds:0001_nasa_pds_1:all:user::1.0;
  rdfs:comment "The Oblique_Line_Azimuth class defines the method used to describe the line along which an Oblique Mercator map projection is centered using the map projection origin and an azimuth. Synder 1987, DOI:10.3133\\//pp1395, page 195: https:\\//\\//pubs.usgs.gov\\//pp\\//1395\\//report.pdf#page=207 PROJ: https:\\//\\//proj.org\\//operations\\//projections\\//omerc.html ".
 
pds4:urn:nasa:pds:0001_nasa_pds_1:all:user:cart:oblique_line_point::1.0 rdf:type rdfs:Class;
  rdfs:label "Oblique_Line_Point";
  pds4:subClassOf pds4:urn:nasa:pds:0001_nasa_pds_1:all:user::1.0;
  rdfs:comment "The Oblique_Line_Point class defines the method used to describe the line along which an Oblique Mercator map projection is centered using two points near the limits of the mapped region that define the center line. Synder 1987, DOI:10.3133\\//pp1395, page 195: https:\\//\\//pubs.usgs.gov\\//pp\\//1395\\//report.pdf#page=207 PROJ: https:\\//\\//proj.org\\//operations\\//projections\\//omerc.html ".
 
pds4:urn:nasa:pds:0001_nasa_pds_1:all:user:cart:oblique_line_point_group::1.0 rdf:type rdfs:Class;
  rdfs:label "Oblique_Line_Point_Group";
  pds4:subClassOf pds4:urn:nasa:pds:0001_nasa_pds_1:all:user::1.0;
  rdfs:comment "The Oblique_Line_Point_Group class provides the coordinates in latitude and longitude of one end point of the line along which an oblique mercator map projection is centered.".
 
pds4:urn:nasa:pds:0001_nasa_pds_1:all:user:cart:oblique_mercator::1.0 rdf:type rdfs:Class;
  rdfs:label "Oblique_Mercator";
  pds4:subClassOf pds4:urn:nasa:pds:0001_nasa_pds_1:all:user::1.0;
  rdfs:comment "The Oblique_Mercator class contains parameters for the Oblique Mercator projection. Synder 1987, DOI:10.3133\\//pp1395, page 66: https:\\//\\//pubs.usgs.gov\\//pp\\//1395\\//report.pdf#page=78 PROJ: https:\\//\\//proj.org\\//operations\\//projections\\//omerc.html ".
 
pds4:urn:nasa:pds:0001_nasa_pds_1:pds:context_area:pds:observation_area::1.0 rdf:type rdfs:Class;
  rdfs:label "Observation_Area";
  pds4:subClassOf pds4:urn:nasa:pds:0001_nasa_pds_1:pds:product_components:pds:context_area::1.0;
  rdfs:comment "The observation area consists of attributes that provide information about the circumstances under which the data were collected.".
 
pds4:urn:nasa:pds:0001_nasa_pds_1:all:user:msn:observation_context::1.0 rdf:type rdfs:Class;
  rdfs:label "Observation_Context";
  pds4:subClassOf pds4:urn:nasa:pds:0001_nasa_pds_1:all:user::1.0;
  rdfs:comment "Describes the vehicle context at the time the observation was taken.".
 
pds4:urn:nasa:pds:0001_nasa_pds_1:all:user:sp:observation_parameters::1.0 rdf:type rdfs:Class;
  rdfs:label "Observation_Parameters";
  pds4:subClassOf pds4:urn:nasa:pds:0001_nasa_pds_1:all:user::1.0;
  rdfs:comment " The Observation_Parameters class collects various values related to the observational circumstances. In general, this class should be present, and all parameters applicable to the situation should be included, even though optional. In some complex cases or for high-level derived products this class may not be applicable, in which case it may be omitted. Use the \\'comment\\' attribute to describe any special circumstances users should be aware of. ".
 
pds4:urn:nasa:pds:0001_nasa_pds_1:all:user:msn_surface:observational_intent::1.0 rdf:type rdfs:Class;
  rdfs:label "Observational_Intent";
  pds4:subClassOf pds4:urn:nasa:pds:0001_nasa_pds_1:all:user::1.0;
  rdfs:comment "Describes the intent and context of the observation.".
 
pds4:urn:nasa:pds:0001_nasa_pds_1:geom:body_identification_base:geom:observer_identification::1.0 rdf:type rdfs:Class;
  rdfs:label "Observer_Identification";
  pds4:subClassOf pds4:urn:nasa:pds:0001_nasa_pds_1:all:user:geom:body_identification_base::1.0;
  rdfs:comment "Within the Geometry dictionary context, an \"Observer\" is the body on the \"from\" end of a vector, or other translation through space. ".
 
pds4:urn:nasa:pds:0001_nasa_pds_1:all:user:nucspec:observing_condition::1.0 rdf:type rdfs:Class;
  rdfs:label "Observing_Condition";
  pds4:subClassOf pds4:urn:nasa:pds:0001_nasa_pds_1:all:user::1.0;
  rdfs:comment "Describes the times that the activity affecting nuclear spectroscopy observations was in effect, along with the sources of the activity, if applicable.".
 
pds4:urn:nasa:pds:0001_nasa_pds_1:all:user:nucspec:observing_conditions::1.0 rdf:type rdfs:Class;
  rdfs:label "Observing_Conditions";
  pds4:subClassOf pds4:urn:nasa:pds:0001_nasa_pds_1:all:user::1.0;
  rdfs:comment "Describes activity that may affect nuclear spectroscopy observations.".
 
pds4:urn:nasa:pds:0001_nasa_pds_1:pds:tndo_context:pds:observing_system::1.0 rdf:type rdfs:Class;
  rdfs:label "Observing_System";
  pds4:subClassOf pds4:urn:nasa:pds:0001_nasa_pds_1:pds:tagged_nondigital_object:pds:tndo_context::1.0;
  rdfs:comment "The Observing System class describes the entire suite used to collect the data.".
 
pds4:urn:nasa:pds:0001_nasa_pds_1:pds:tagged_nondigital_child:pds:observing_system_component::1.0 rdf:type rdfs:Class;
  rdfs:label "Observing_System_Component";
  pds4:subClassOf pds4:urn:nasa:pds:0001_nasa_pds_1:all:user:pds:tagged_nondigital_child::1.0;
  rdfs:comment "The Observing System Component class describes one or more subsystems used to collect data.".
 
pds4:urn:nasa:pds:0001_nasa_pds_1:pds:tagged_nondigital_child:pds:observing_system_component:airborne::1.0 rdf:type rdfs:Class;
  rdfs:label "Airborne";
  rdfs:subClassOf pds4:urn:nasa:pds:0001_nasa_pds_1:pds:tagged_nondigital_child:pds:observing_system_component::1.0;
  rdfs:comment "The physical object that transports a platform by or through air.".
 
pds4:urn:nasa:pds:0001_nasa_pds_1:pds:tagged_nondigital_child:pds:observing_system_component:aircraft::1.0 rdf:type rdfs:Class;
  rdfs:label "Aircraft";
  rdfs:subClassOf pds4:urn:nasa:pds:0001_nasa_pds_1:pds:tagged_nondigital_child:pds:observing_system_component::1.0;
  rdfs:comment "An airborne observatory carried on a powered, heavier than air vessel supporting observations, measurements, and scientific experiments during flight.".
 
pds4:urn:nasa:pds:0001_nasa_pds_1:pds:tagged_nondigital_child:pds:observing_system_component:artificial_illumination::1.0 rdf:type rdfs:Class;
  rdfs:label "Artificial Illumination";
  rdfs:subClassOf pds4:urn:nasa:pds:0001_nasa_pds_1:pds:tagged_nondigital_child:pds:observing_system_component::1.0;
  rdfs:comment "The observing system component provides artificial illumination".
 
pds4:urn:nasa:pds:0001_nasa_pds_1:pds:tagged_nondigital_child:pds:observing_system_component:balloon::1.0 rdf:type rdfs:Class;
  rdfs:label "Balloon";
  rdfs:subClassOf pds4:urn:nasa:pds:0001_nasa_pds_1:pds:tagged_nondigital_child:pds:observing_system_component::1.0;
  rdfs:comment "A balloon-borne observatory, typically consisting of a gondola structure carrying one or more telescopes and instruments, borne aloft by an unpowered or minimially powered lighter-than-atmosphere balloon for a limited observing period.".
 
pds4:urn:nasa:pds:0001_nasa_pds_1:pds:tagged_nondigital_child:pds:observing_system_component:computer::1.0 rdf:type rdfs:Class;
  rdfs:label "Computer";
  rdfs:subClassOf pds4:urn:nasa:pds:0001_nasa_pds_1:pds:tagged_nondigital_child:pds:observing_system_component::1.0;
  rdfs:comment "The observing system component is a processor embedded in the observing configuration, that manipulates or regulates the data prior to downlink.".
 
pds4:urn:nasa:pds:0001_nasa_pds_1:pds:tagged_nondigital_child:pds:observing_system_component:facility::1.0 rdf:type rdfs:Class;
  rdfs:label "Facility";
  rdfs:subClassOf pds4:urn:nasa:pds:0001_nasa_pds_1:pds:tagged_nondigital_child:pds:observing_system_component::1.0;
  rdfs:comment "The observing system component is a facility.".
 
pds4:urn:nasa:pds:0001_nasa_pds_1:pds:tagged_nondigital_child:pds:observing_system_component:host::1.0 rdf:type rdfs:Class;
  rdfs:label "Host";
  rdfs:subClassOf pds4:urn:nasa:pds:0001_nasa_pds_1:pds:tagged_nondigital_child:pds:observing_system_component::1.0;
  rdfs:comment "The observing system component is a host or a member in a chain of hosts that ultimately contains an instrument that collects data.".
 
pds4:urn:nasa:pds:0001_nasa_pds_1:pds:tagged_nondigital_child:pds:observing_system_component:instrument::1.0 rdf:type rdfs:Class;
  rdfs:label "Instrument";
  rdfs:subClassOf pds4:urn:nasa:pds:0001_nasa_pds_1:pds:tagged_nondigital_child:pds:observing_system_component::1.0;
  rdfs:comment "The observing system component is an instrument".
 
pds4:urn:nasa:pds:0001_nasa_pds_1:pds:tagged_nondigital_child:pds:observing_system_component:laboratory::1.0 rdf:type rdfs:Class;
  rdfs:label "Laboratory";
  rdfs:subClassOf pds4:urn:nasa:pds:0001_nasa_pds_1:pds:tagged_nondigital_child:pds:observing_system_component::1.0;
  rdfs:comment "The observing system component is a laboratory".
 
pds4:urn:nasa:pds:0001_nasa_pds_1:pds:tagged_nondigital_child:pds:observing_system_component:literature_search::1.0 rdf:type rdfs:Class;
  rdfs:label "Literature Search";
  rdfs:subClassOf pds4:urn:nasa:pds:0001_nasa_pds_1:pds:tagged_nondigital_child:pds:observing_system_component::1.0;
  rdfs:comment "The observing system component is a literature search".
 
pds4:urn:nasa:pds:0001_nasa_pds_1:pds:tagged_nondigital_child:pds:observing_system_component:naked_eye::1.0 rdf:type rdfs:Class;
  rdfs:label "Naked Eye";
  rdfs:subClassOf pds4:urn:nasa:pds:0001_nasa_pds_1:pds:tagged_nondigital_child:pds:observing_system_component::1.0;
  rdfs:comment "The observing system component is the unaided eye of a person".
 
pds4:urn:nasa:pds:0001_nasa_pds_1:pds:tagged_nondigital_child:pds:observing_system_component:observatory::1.0 rdf:type rdfs:Class;
  rdfs:label "Observatory";
  rdfs:subClassOf pds4:urn:nasa:pds:0001_nasa_pds_1:pds:tagged_nondigital_child:pds:observing_system_component::1.0;
  rdfs:comment "The observing system component is an observatory".
 
pds4:urn:nasa:pds:0001_nasa_pds_1:pds:tagged_nondigital_child:pds:observing_system_component:spacecraft::1.0 rdf:type rdfs:Class;
  rdfs:label "Spacecraft";
  rdfs:subClassOf pds4:urn:nasa:pds:0001_nasa_pds_1:pds:tagged_nondigital_child:pds:observing_system_component::1.0;
  rdfs:comment "The observing system component is a spacecraft".
 
pds4:urn:nasa:pds:0001_nasa_pds_1:pds:tagged_nondigital_child:pds:observing_system_component:suborbital_rocket::1.0 rdf:type rdfs:Class;
  rdfs:label "Suborbital Rocket";
  rdfs:subClassOf pds4:urn:nasa:pds:0001_nasa_pds_1:pds:tagged_nondigital_child:pds:observing_system_component::1.0;
  rdfs:comment "A Suborbital Rocket is an instrument-carrying rocket designed to take measurements and perform scientific experiments during its sub-orbital flight.".
 
pds4:urn:nasa:pds:0001_nasa_pds_1:pds:tagged_nondigital_child:pds:observing_system_component:telescope::1.0 rdf:type rdfs:Class;
  rdfs:label "Telescope";
  rdfs:subClassOf pds4:urn:nasa:pds:0001_nasa_pds_1:pds:tagged_nondigital_child:pds:observing_system_component::1.0;
  rdfs:comment "The observing system component is a telescope".
 
pds4:urn:nasa:pds:0001_nasa_pds_1:all:user:rings:occultation_ring_profile::1.0 rdf:type rdfs:Class;
  rdfs:label "Occultation_Ring_Profile";
  pds4:subClassOf pds4:urn:nasa:pds:0001_nasa_pds_1:all:user::1.0;
  rdfs:comment "This class replaces the Radio_Occultation and Stellar_Occultation classes. It is used for all ring occultation profiles regardless of the occultation type. ".
 
pds4:urn:nasa:pds:0001_nasa_pds_1:all:user:rings:occultation_supplement::1.0 rdf:type rdfs:Class;
  rdfs:label "Occultation_Supplement";
  pds4:subClassOf pds4:urn:nasa:pds:0001_nasa_pds_1:all:user::1.0;
  rdfs:comment "This class is required for all radio ring occultation calibration and geometry supplemental files.".
 
pds4:urn:nasa:pds:0001_nasa_pds_1:all:user:rings:occultation_time_series::1.0 rdf:type rdfs:Class;
  rdfs:label "Occultation_Time_Series";
  pds4:subClassOf pds4:urn:nasa:pds:0001_nasa_pds_1:all:user::1.0;
  rdfs:comment "This class supports occultation data organized as a time series.".
 
pds4:urn:nasa:pds:0001_nasa_pds_1:all:user:img:onboard_color_matrix::1.0 rdf:type rdfs:Class;
  rdfs:label "Onboard_Color_Matrix";
  pds4:subClassOf pds4:urn:nasa:pds:0001_nasa_pds_1:all:user::1.0;
  rdfs:comment "The Onboard_Color_Matrix class represents a 3x3 matrix that is used onboard to perform color correction. It is done after de-Bayering, as all three color bands are needed for each pixel. The first three elements are multiplied by the R,G,B (respectively) pixel values and summed to get the output Red pixel value. Similarly, the second three create the output Green, and the last three the output Blue. If the label is not present, no correction was performed.".
 
pds4:urn:nasa:pds:0001_nasa_pds_1:all:user:img:onboard_compression::1.0 rdf:type rdfs:Class;
  rdfs:label "Onboard_Compression";
  pds4:subClassOf pds4:urn:nasa:pds:0001_nasa_pds_1:all:user::1.0;
  rdfs:comment "The Onboard_Compression class contains attributes describing the compression performed onboard a spacecraft or instrument for data storage and transmission.".
 
pds4:urn:nasa:pds:0001_nasa_pds_1:all:user:img:onboard_responsivity::1.0 rdf:type rdfs:Class;
  rdfs:label "Onboard_Responsivity";
  pds4:subClassOf pds4:urn:nasa:pds:0001_nasa_pds_1:all:user::1.0;
  rdfs:comment "The Onboard_Responsivity class specifies factors that have been applied to the R, G, and B cells (respectively) of the Bayer pattern, before de-Bayering (demosaicking) takes place. The intent of these is to approximately balance the filters so the de-Bayering process is not skewed, and EDR\\//ILT products look reasonable before full radiometric or color correction is done on the ground. If these factors are not present, no correction was performed.".
 
pds4:urn:nasa:pds:0001_nasa_pds_1:all:user:img:optical_filter::1.0 rdf:type rdfs:Class;
  rdfs:label "Optical_Filter";
  pds4:subClassOf pds4:urn:nasa:pds:0001_nasa_pds_1:all:user::1.0;
  rdfs:comment "The Optical_Filter class defines the filters used by the camera optics (not to be confused with image processing software filters). The filter may be identified by name, identifier, number, or some combination of these.".
 
pds4:urn:nasa:pds:0001_nasa_pds_1:all:user:img:optical_properties::1.0 rdf:type rdfs:Class;
  rdfs:label "Optical_Properties";
  pds4:subClassOf pds4:urn:nasa:pds:0001_nasa_pds_1:all:user::1.0;
  rdfs:comment "The Optical_Properties class describes properties of the optics used in acquiring the image.".
 
pds4:urn:nasa:pds:0001_nasa_pds_1:all:user:msn:orbital_mission::1.0 rdf:type rdfs:Class;
  rdfs:label "Orbital_Mission";
  pds4:subClassOf pds4:urn:nasa:pds:0001_nasa_pds_1:all:user::1.0;
  rdfs:comment "The Orbital_Mission class provides information about an orbital mission.".
 
pds4:urn:nasa:pds:0001_nasa_pds_1:all:user:geom:orbiter_identification::1.0 rdf:type rdfs:Class;
  rdfs:label "Orbiter_Identification";
  pds4:subClassOf pds4:urn:nasa:pds:0001_nasa_pds_1:all:user::1.0;
  rdfs:comment "The Orbiter_Identification class is a container of classes used to establish global identifications for the Geometry_Orbiter class. ".
 
pds4:urn:nasa:pds:0001_nasa_pds_1:all:user:cart:orthographic::1.0 rdf:type rdfs:Class;
  rdfs:label "Orthographic";
  pds4:subClassOf pds4:urn:nasa:pds:0001_nasa_pds_1:all:user::1.0;
  rdfs:comment "The Orthographic class contains parameters for the Orthographic projection. Synder 1987, DOI:10.3133\\//pp1395, page 145: https:\\//\\//pubs.usgs.gov\\//pp\\//1395\\//report.pdf#page=157 PROJ: https:\\//\\//proj.org\\//operations\\//projections\\//ortho.html ".
 
pds4:urn:nasa:pds:0001_nasa_pds_1:all:user:cart:orthographic_lander::1.0 rdf:type rdfs:Class;
  rdfs:label "Orthographic_Lander";
  pds4:subClassOf pds4:urn:nasa:pds:0001_nasa_pds_1:all:user::1.0;
  rdfs:comment "This is an in-situ projection that is a generalization of the Vertical projection, in that any arbitrary projection plane can be specified.".
 
pds4:urn:nasa:pds:0001_nasa_pds_1:all:user:cart:orthorectified::1.0 rdf:type rdfs:Class;
  rdfs:label "Orthorectified";
  pds4:subClassOf pds4:urn:nasa:pds:0001_nasa_pds_1:all:user::1.0;
  rdfs:comment "This is an in-situ projection that provides a true overhead view of the scene. Range data is required to create this projection, meaning there is no parallax distortion. It has a constant scale in meters\\//pixel.".
 
pds4:urn:nasa:pds:0001_nasa_pds_1:pds:tndo_context:pds:other::1.0 rdf:type rdfs:Class;
  rdfs:label "Other";
  pds4:subClassOf pds4:urn:nasa:pds:0001_nasa_pds_1:pds:tagged_nondigital_object:pds:tndo_context::1.0;
  rdfs:comment "The Other class provides a description of activities involved in the collection of data which are not otherwise modeled.".
 
pds4:urn:nasa:pds:0001_nasa_pds_1:pds:tndo_context:pds:pds_affiliate::1.0 rdf:type rdfs:Class;
  rdfs:label "PDS_Affiliate";
  pds4:subClassOf pds4:urn:nasa:pds:0001_nasa_pds_1:pds:tagged_nondigital_object:pds:tndo_context::1.0;
  rdfs:comment "The PDS Affiliate class provides a description of a person who has an association with the planetary science community and has access to PDS resources not normally allowed to the general public.".
 
pds4:urn:nasa:pds:0001_nasa_pds_1:pds:tndo_context:pds:pds_guest::1.0 rdf:type rdfs:Class;
  rdfs:label "PDS_Guest";
  pds4:subClassOf pds4:urn:nasa:pds:0001_nasa_pds_1:pds:tagged_nondigital_object:pds:tndo_context::1.0;
  rdfs:comment "The PDS_Guest class is the default description of a person who has an association with the planetary science community and who has the most limited access to PDS resources.".
 
pds4:urn:nasa:pds:0001_nasa_pds_1:all:user:geom:psph_model::1.0 rdf:type rdfs:Class;
  rdfs:label "PSPH_Model";
  pds4:subClassOf pds4:urn:nasa:pds:0001_nasa_pds_1:all:user::1.0;
  rdfs:comment " A new camera model designed to perform better fisheye-image rectification prior to 1D stereo correlation. The primary innovation is the use of a unit projection sphere rather than an image plane. For epipolar alignment between stereo cameras the rows (for a left\\//right pair) or the columns (for an up\\//down pair) of both must lie along the same plane. Thus we use a pair of planes to define the rows and columns. Each plane will rotate around a static dedicated axis passing through the sphere center. Pixels will be located where the planes intersect with each other and the unit sphere. ".
 
pds4:urn:nasa:pds:0001_nasa_pds_1:pds:tagged_digital_child:pds:packed_data_fields::1.0 rdf:type rdfs:Class;
  rdfs:label "Packed_Data_Fields";
  pds4:subClassOf pds4:urn:nasa:pds:0001_nasa_pds_1:all:user:pds:tagged_digital_child::1.0;
  rdfs:comment "The Packed_Data_Fields class contains field definitions for extracting packed data from the associated byte string field.".
 
pds4:urn:nasa:pds:0001_nasa_pds_1:all:user:proc:parameter::1.0 rdf:type rdfs:Class;
  rdfs:label "Parameter";
  pds4:subClassOf pds4:urn:nasa:pds:0001_nasa_pds_1:all:user::1.0;
  rdfs:comment "The Parameter class describes any information about software program execution. Examples of information that can be captured here are software input arguments, software output arguments, log information, and references to specific data products. This class is intended to be freeform to allow data providers the ability to specify information they determine applicable and useful for their data processing software and data products.".
 
pds4:urn:nasa:pds:0001_nasa_pds_1:pds:byte_stream:pds:parsable_byte_stream::1.0 rdf:type rdfs:Class;
  rdfs:label "Parsable_Byte_Stream";
  pds4:subClassOf pds4:urn:nasa:pds:0001_nasa_pds_1:pds:tagged_digital_object:pds:byte_stream::1.0;
  rdfs:comment "The Parsable Byte Stream class defines byte streams that have standard parsing rules. The Parsable Byte Stream class is the parent class for all parsable byte streams.".
 
pds4:urn:nasa:pds:0001_nasa_pds_1:all:user:survey:percentage_limit::1.0 rdf:type rdfs:Class;
  rdfs:label "Percentage_Limit";
  pds4:subClassOf pds4:urn:nasa:pds:0001_nasa_pds_1:all:user::1.0;
  rdfs:comment "The limiting magnitude of the image, expressed as a magnitude, and the percentage of known objects detected at that magnitude".
 
pds4:urn:nasa:pds:0001_nasa_pds_1:all:user:cart:perspective::1.0 rdf:type rdfs:Class;
  rdfs:label "Perspective";
  pds4:subClassOf pds4:urn:nasa:pds:0001_nasa_pds_1:all:user::1.0;
  rdfs:comment "This is an in-situ projection that models a pinhole camera. ".
 
pds4:urn:nasa:pds:0001_nasa_pds_1:all:user:img:pixel_averaging_dimensions::1.0 rdf:type rdfs:Class;
  rdfs:label "Pixel_Averaging_Dimensions";
  pds4:subClassOf pds4:urn:nasa:pds:0001_nasa_pds_1:all:user::1.0;
  rdfs:comment "The Pixel_Averaging_Dimensions class provides the height and width, in pixels, of the area over which pixels were averaged prior to image compression.".
 
pds4:urn:nasa:pds:0001_nasa_pds_1:all:user:geom:pixel_dimensions::1.0 rdf:type rdfs:Class;
  rdfs:label "Pixel_Dimensions";
  pds4:subClassOf pds4:urn:nasa:pds:0001_nasa_pds_1:all:user::1.0;
  rdfs:comment "The Pixel_Dimensions class contains information regarding pixel size. ".
 
pds4:urn:nasa:pds:0001_nasa_pds_1:all:user:geom:pixel_intercept::1.0 rdf:type rdfs:Class;
  rdfs:label "Pixel_Intercept";
  pds4:subClassOf pds4:urn:nasa:pds:0001_nasa_pds_1:all:user::1.0;
  rdfs:comment "The Pixel_Intercept class provides the latitude and longitude on the surface of the target for the projection of the specified pixel. The pixel is specified using either reference_pixel_location or Reference_Pixel. Although each of these is optional, one must be used. ".
 
pds4:urn:nasa:pds:0001_nasa_pds_1:all:user:cart:pixel_position_nadir_polar::1.0 rdf:type rdfs:Class;
  rdfs:label "Pixel_Position_Nadir_Polar";
  pds4:subClassOf pds4:urn:nasa:pds:0001_nasa_pds_1:all:user::1.0;
  rdfs:comment "The Pixel_Position_Nadir_Polar class specifies the sample coordinate of the location in the image of the \"special\" point of the mosaic. For Polar projections, this is the nadir of the polar projection. In PDS3, this information was specified using the LINE_PROJECTION_OFFSET and SAMPLE_PROJECTION_OFFSET keywords.".
 
pds4:urn:nasa:pds:0001_nasa_pds_1:all:user:cart:pixel_position_origin::1.0 rdf:type rdfs:Class;
  rdfs:label "Pixel_Position_Origin";
  pds4:subClassOf pds4:urn:nasa:pds:0001_nasa_pds_1:all:user::1.0;
  rdfs:comment "The Pixel_Position_Origin class specifies the sample coordinate of the location in the image of the \"special\" point of the mosaic. For Vertical, Orthographic and Orthorectified projections, this is the origin of the projected coordinate system, corresponding to the Vector_Projection_Origin. In PDS3, this information was specified using the LINE_PROJECTION_OFFSET and SAMPLE_PROJECTION_OFFSET keywords.".
 
pds4:urn:nasa:pds:0001_nasa_pds_1:all:user:geom:pixel_size_projected::1.0 rdf:type rdfs:Class;
  rdfs:label "Pixel_Size_Projected";
  pds4:subClassOf pds4:urn:nasa:pds:0001_nasa_pds_1:all:user::1.0;
  rdfs:comment "The Pixel_Size_Projected class gives the size, in units of length (e.g., kilometers) of the projection of a pixel onto the surface of the target which is specified in the parent Geometry_Orbiter class. The reference_location attribute is used to identify the specific point on the target. ".
 
pds4:urn:nasa:pds:0001_nasa_pds_1:all:user:img_surface:placement_target_instrument::1.0 rdf:type rdfs:Class;
  rdfs:label "Placement_Target_Instrument";
  pds4:subClassOf pds4:urn:nasa:pds:0001_nasa_pds_1:all:user::1.0;
  rdfs:comment "Indicates the instrument that is referred to by the product. This is not the same as the instrument that acquired the product. For example, on InSight instrument placement products, it defines which instrument is being placed.".
 
pds4:urn:nasa:pds:0001_nasa_pds_1:all:user:cart:planar::1.0 rdf:type rdfs:Class;
  rdfs:label "Planar";
  pds4:subClassOf pds4:urn:nasa:pds:0001_nasa_pds_1:all:user::1.0;
  rdfs:comment "The Planar class provides the quantities of distances, or distances and angles, which define the position of a point on a reference plane to which the surface of a planet has been projected.".
 
pds4:urn:nasa:pds:0001_nasa_pds_1:all:user:cart:planar_coordinate_information::1.0 rdf:type rdfs:Class;
  rdfs:label "Planar_Coordinate_Information";
  pds4:subClassOf pds4:urn:nasa:pds:0001_nasa_pds_1:all:user::1.0;
  rdfs:comment "The Planar_Coordinate_Information class provides information about the coordinate system developed on the planar surface.".
 
pds4:urn:nasa:pds:0001_nasa_pds_1:all:user:cart:point_perspective::1.0 rdf:type rdfs:Class;
  rdfs:label "Point_Perspective";
  pds4:subClassOf pds4:urn:nasa:pds:0001_nasa_pds_1:all:user::1.0;
  rdfs:comment "The Point Perspective class contains parameters for the Point Perspective (fundamental definition) projection. Synder 1987, DOI:10.3133\\//pp1395, page 169: https:\\//\\//pubs.usgs.gov\\//pp\\//1395\\//report.pdf#page=181 ".
 
pds4:urn:nasa:pds:0001_nasa_pds_1:all:user:img:pointing_correction::1.0 rdf:type rdfs:Class;
  rdfs:label "Pointing_Correction";
  pds4:subClassOf pds4:urn:nasa:pds:0001_nasa_pds_1:all:user::1.0;
  rdfs:comment "The Pointing_Correction class contains attributes used to identify and describe the camera model transformations completed in order to update pointing information of an image or mosaic.".
 
pds4:urn:nasa:pds:0001_nasa_pds_1:img:data_processing_file:img:pointing_correction_file::1.0 rdf:type rdfs:Class;
  rdfs:label "Pointing_Correction_File";
  pds4:subClassOf pds4:urn:nasa:pds:0001_nasa_pds_1:all:user:img:data_processing_file::1.0;
  rdfs:comment "The Pointing_Correction_File class identifies a file containing pointing correction information.".
 
pds4:urn:nasa:pds:0001_nasa_pds_1:all:user:img:pointing_correction_image::1.0 rdf:type rdfs:Class;
  rdfs:label "Pointing_Correction_Image";
  pds4:subClassOf pds4:urn:nasa:pds:0001_nasa_pds_1:all:user::1.0;
  rdfs:comment "The Pointing_Correction_Image class contains attributes used to identify and describe the camera model transformations completed in order to update pointing information of a single image, whether alone or part of a mosaic.".
 
pds4:urn:nasa:pds:0001_nasa_pds_1:all:user:img:pointing_model_parameter::1.0 rdf:type rdfs:Class;
  rdfs:label "Pointing_Model_Parameter";
  pds4:subClassOf pds4:urn:nasa:pds:0001_nasa_pds_1:all:user::1.0;
  rdfs:comment "The Pointing_Model_Parameter class specifies the name and value (numeric) parameters needed by the pointing model identified by the pointing_model_name attribute in the Pointing_Correction parent class. The meaning of any given parameter is defined by the pointing model. ".
 
pds4:urn:nasa:pds:0001_nasa_pds_1:all:user:cart:polar::1.0 rdf:type rdfs:Class;
  rdfs:label "Polar";
  pds4:subClassOf pds4:urn:nasa:pds:0001_nasa_pds_1:all:user::1.0;
  rdfs:comment "This is an in-situ projection that provides a quasi-overhead view that extends to the horizon. Elevation is measured radially outward from the nadir location, with a constant pixel scale. Azimuth is measured along concentric circles centered at the nadir.".
 
pds4:urn:nasa:pds:0001_nasa_pds_1:all:user:cart:polar_stereographic::1.0 rdf:type rdfs:Class;
  rdfs:label "Polar_Stereographic";
  pds4:subClassOf pds4:urn:nasa:pds:0001_nasa_pds_1:all:user::1.0;
  rdfs:comment "The Polar_Stereographic class contains parameters for the Polar Stereographic projection. Synder 1987, DOI:10.3133\\//pp1395, page 154: https:\\//\\//pubs.usgs.gov\\//pp\\//1395\\//report.pdf#page=166 PROJ: https:\\//\\//proj.org\\//operations\\//projections\\//stere.html Note that most applications will either define latitude_of_projection_origin or scale_factor_at_projection_origin, but not both. Here we define latitude_of_projection_origin as mandatory and at CART LDD versoin 1934 have made scale_factor_at_projection_origin optional. For context, these two keywords have the same impact on the final product but are just different ways to define it. Thus, for example in the PROJ library, if both are made available, the latitude_of_projection_origin (+lat_ts) will be used instead of scale_factor_at_projection_origin (+k_0). Note, if you do supply the optional attribute scale_factor_at_projection_origin, the default scale (+k_0) for planetary polar data will mostly likely be set to 1.0. ".
 
pds4:urn:nasa:pds:0001_nasa_pds_1:all:user:cart:polyconic::1.0 rdf:type rdfs:Class;
  rdfs:label "Polyconic";
  pds4:subClassOf pds4:urn:nasa:pds:0001_nasa_pds_1:all:user::1.0;
  rdfs:comment "The Polyconic class contains parameters for the Polyconic projection. Synder 1987, DOI:10.3133\\//pp1395, page 124: https:\\//\\//pubs.usgs.gov\\//pp\\//1395\\//report.pdf#page=136 PROJ: https:\\//\\//proj.org\\//operations\\//projections\\//poly.html ".
 
pds4:urn:nasa:pds:0001_nasa_pds_1:all:user:nucspec:polynomial::1.0 rdf:type rdfs:Class;
  rdfs:label "Polynomial";
  pds4:subClassOf pds4:urn:nasa:pds:0001_nasa_pds_1:all:user::1.0;
  rdfs:comment "The pulse height in energy units (e.g. MeV) is determined for a given channel number using the polynomial: H(x) = a0 + a1 x + a2 x^2 + ..., where H is pulse height with energy units and x is channel number.".
 
pds4:urn:nasa:pds:0001_nasa_pds_1:all:user:geom:polynomial_coefficients_1::1.0 rdf:type rdfs:Class;
  rdfs:label "Polynomial_Coefficients_1";
  pds4:subClassOf pds4:urn:nasa:pds:0001_nasa_pds_1:all:user::1.0;
  rdfs:comment "The Polynomial_Coefficients_1 class provides a one polynomial coefficient. ".
 
pds4:urn:nasa:pds:0001_nasa_pds_1:all:user:geom:polynomial_coefficients_2::1.0 rdf:type rdfs:Class;
  rdfs:label "Polynomial_Coefficients_2";
  pds4:subClassOf pds4:urn:nasa:pds:0001_nasa_pds_1:all:user::1.0;
  rdfs:comment "The Polynomial_Coefficients_2 class provides two polynomial coefficients. ".
 
pds4:urn:nasa:pds:0001_nasa_pds_1:all:user:geom:polynomial_coefficients_3::1.0 rdf:type rdfs:Class;
  rdfs:label "Polynomial_Coefficients_3";
  pds4:subClassOf pds4:urn:nasa:pds:0001_nasa_pds_1:all:user::1.0;
  rdfs:comment "The Polynomial_Coefficients_3 class provides three polynomial coefficients. ".
 
pds4:urn:nasa:pds:0001_nasa_pds_1:all:user:nucspec:polynomial_term::1.0 rdf:type rdfs:Class;
  rdfs:label "Polynomial_Term";
  pds4:subClassOf pds4:urn:nasa:pds:0001_nasa_pds_1:all:user::1.0;
  rdfs:comment "Describes a single term in the polynomial function.".
 
pds4:urn:nasa:pds:0001_nasa_pds_1:pds:product_components:pds:primary_result_summary::1.0 rdf:type rdfs:Class;
  rdfs:label "Primary_Result_Summary";
  pds4:subClassOf pds4:urn:nasa:pds:0001_nasa_pds_1:all:user:pds:product_components::1.0;
  rdfs:comment "The Primary_Result_Summary class provides a high-level description of the types of products included in the collection or bundle".
 
pds4:urn:nasa:pds:0001_nasa_pds_1:pds:product_components:pds:primary_result_summary:altimetry::1.0 rdf:type rdfs:Class;
  rdfs:label "Altimetry";
  rdfs:subClassOf pds4:urn:nasa:pds:0001_nasa_pds_1:pds:product_components:pds:primary_result_summary::1.0;
  rdfs:comment "Measurement of altitude.".
 
pds4:urn:nasa:pds:0001_nasa_pds_1:pds:product_components:pds:primary_result_summary:astrometry::1.0 rdf:type rdfs:Class;
  rdfs:label "Astrometry";
  rdfs:subClassOf pds4:urn:nasa:pds:0001_nasa_pds_1:pds:product_components:pds:primary_result_summary::1.0;
  rdfs:comment "Precise measurement of positions of heavenly bodies.".
 
pds4:urn:nasa:pds:0001_nasa_pds_1:pds:product_components:pds:primary_result_summary:count::1.0 rdf:type rdfs:Class;
  rdfs:label "Count";
  rdfs:subClassOf pds4:urn:nasa:pds:0001_nasa_pds_1:pds:product_components:pds:primary_result_summary::1.0;
  rdfs:comment "A recording of the number of discrete events".
 
pds4:urn:nasa:pds:0001_nasa_pds_1:pds:product_components:pds:primary_result_summary:e\/b-field_vectors::1.0 rdf:type rdfs:Class;
  rdfs:label "E\\//B-Field Vectors";
  rdfs:subClassOf pds4:urn:nasa:pds:0001_nasa_pds_1:pds:product_components:pds:primary_result_summary::1.0;
  rdfs:comment "Arrays populated by values of the electric\\//magnetic field in three orthogonal directions.".
 
pds4:urn:nasa:pds:0001_nasa_pds_1:pds:product_components:pds:primary_result_summary:gravity_model::1.0 rdf:type rdfs:Class;
  rdfs:label "Gravity Model";
  rdfs:subClassOf pds4:urn:nasa:pds:0001_nasa_pds_1:pds:product_components:pds:primary_result_summary::1.0;
  rdfs:comment "An approximation to the gravity field of an object derived from measurement and\\//or theory".
 
pds4:urn:nasa:pds:0001_nasa_pds_1:pds:product_components:pds:primary_result_summary:image::1.0 rdf:type rdfs:Class;
  rdfs:label "Image";
  rdfs:subClassOf pds4:urn:nasa:pds:0001_nasa_pds_1:pds:product_components:pds:primary_result_summary::1.0;
  rdfs:comment "A two-dimensional representation of a field of view".
 
pds4:urn:nasa:pds:0001_nasa_pds_1:pds:product_components:pds:primary_result_summary:lightcurves::1.0 rdf:type rdfs:Class;
  rdfs:label "Lightcurves";
  rdfs:subClassOf pds4:urn:nasa:pds:0001_nasa_pds_1:pds:product_components:pds:primary_result_summary::1.0;
  rdfs:comment "This value indicates data products containing time-sequences of magnitude measurements for one or more individual targets (typically asteroids or comets).".
 
pds4:urn:nasa:pds:0001_nasa_pds_1:pds:product_components:pds:primary_result_summary:map::1.0 rdf:type rdfs:Class;
  rdfs:label "Map";
  rdfs:subClassOf pds4:urn:nasa:pds:0001_nasa_pds_1:pds:product_components:pds:primary_result_summary::1.0;
  rdfs:comment "A two-dimensional representation of the plan view of a surface".
 
pds4:urn:nasa:pds:0001_nasa_pds_1:pds:product_components:pds:primary_result_summary:meteorology::1.0 rdf:type rdfs:Class;
  rdfs:label "Meteorology";
  rdfs:subClassOf pds4:urn:nasa:pds:0001_nasa_pds_1:pds:product_components:pds:primary_result_summary::1.0;
  rdfs:comment "Measurements of the meteorological conditions of an atmosphere such as pressure, temperature, wind speed, etc.".
 
pds4:urn:nasa:pds:0001_nasa_pds_1:pds:product_components:pds:primary_result_summary:null_result::1.0 rdf:type rdfs:Class;
  rdfs:label "Null Result";
  rdfs:subClassOf pds4:urn:nasa:pds:0001_nasa_pds_1:pds:product_components:pds:primary_result_summary::1.0;
  rdfs:comment "Measurements which failed.".
 
pds4:urn:nasa:pds:0001_nasa_pds_1:pds:product_components:pds:primary_result_summary:occultation::1.0 rdf:type rdfs:Class;
  rdfs:label "Occultation";
  rdfs:subClassOf pds4:urn:nasa:pds:0001_nasa_pds_1:pds:product_components:pds:primary_result_summary::1.0;
  rdfs:comment "Measurements conducted when one celestial body progressively hides another".
 
pds4:urn:nasa:pds:0001_nasa_pds_1:pds:product_components:pds:primary_result_summary:photometry::1.0 rdf:type rdfs:Class;
  rdfs:label "Photometry";
  rdfs:subClassOf pds4:urn:nasa:pds:0001_nasa_pds_1:pds:product_components:pds:primary_result_summary::1.0;
  rdfs:comment "Measurement of light flux".
 
pds4:urn:nasa:pds:0001_nasa_pds_1:pds:product_components:pds:primary_result_summary:physical_parameters::1.0 rdf:type rdfs:Class;
  rdfs:label "Physical Parameters";
  rdfs:subClassOf pds4:urn:nasa:pds:0001_nasa_pds_1:pds:product_components:pds:primary_result_summary::1.0;
  rdfs:comment "This value indicates data products containing compilations of one or more physical parameters - like albedo, density, absolute magnitude, etc. It is generally used for data that combines these highly-derived results from multiple sources.".
 
pds4:urn:nasa:pds:0001_nasa_pds_1:pds:product_components:pds:primary_result_summary:polarimetry::1.0 rdf:type rdfs:Class;
  rdfs:label "Polarimetry";
  rdfs:subClassOf pds4:urn:nasa:pds:0001_nasa_pds_1:pds:product_components:pds:primary_result_summary::1.0;
  rdfs:comment "Measurement of the polarization state of radiation.".
 
pds4:urn:nasa:pds:0001_nasa_pds_1:pds:product_components:pds:primary_result_summary:radiometry::1.0 rdf:type rdfs:Class;
  rdfs:label "Radiometry";
  rdfs:subClassOf pds4:urn:nasa:pds:0001_nasa_pds_1:pds:product_components:pds:primary_result_summary::1.0;
  rdfs:comment "Measurement of the radiation coming from a body, usually at infrared and longer wavelengths".
 
pds4:urn:nasa:pds:0001_nasa_pds_1:pds:product_components:pds:primary_result_summary:reference::1.0 rdf:type rdfs:Class;
  rdfs:label "Reference";
  rdfs:subClassOf pds4:urn:nasa:pds:0001_nasa_pds_1:pds:product_components:pds:primary_result_summary::1.0;
  rdfs:comment "A Reference product provides ancillary information needed to support the use of another data product.  Reference products include things like tables of foot notes or lists of detailed citations, and are usually associated with data products compiled from the published literature.".
 
pds4:urn:nasa:pds:0001_nasa_pds_1:pds:product_components:pds:primary_result_summary:shape_model::1.0 rdf:type rdfs:Class;
  rdfs:label "Shape Model";
  rdfs:subClassOf pds4:urn:nasa:pds:0001_nasa_pds_1:pds:product_components:pds:primary_result_summary::1.0;
  rdfs:comment "An approximation to the shape of an object derived from measurements and\\//or theory".
 
pds4:urn:nasa:pds:0001_nasa_pds_1:pds:product_components:pds:primary_result_summary:spectrum::1.0 rdf:type rdfs:Class;
  rdfs:label "Spectrum";
  rdfs:subClassOf pds4:urn:nasa:pds:0001_nasa_pds_1:pds:product_components:pds:primary_result_summary::1.0;
  rdfs:comment "An array containing values of a dependent variable as a function of an independent variable.".
 
pds4:urn:nasa:pds:0001_nasa_pds_1:all:user:proc:process::1.0 rdf:type rdfs:Class;
  rdfs:label "Process";
  pds4:subClassOf pds4:urn:nasa:pds:0001_nasa_pds_1:all:user::1.0;
  rdfs:comment "The Process class describes one of the software processes used to produce the data product referenced in the parent Processing_Information class. This class includes descriptions of the process owner as well as the data processing software used to create the data product.".
 
pds4:urn:nasa:pds:0001_nasa_pds_1:all:user:proc:processing_information::1.0 rdf:type rdfs:Class;
  rdfs:label "Processing_Information";
  pds4:subClassOf pds4:urn:nasa:pds:0001_nasa_pds_1:all:user::1.0;
  rdfs:comment "The Processing_Information class contains detailed information regarding the history of processing of the data product(s) described in the label. Information that can be specified using this class includes input products used to create a specific data product and the software and processes used to produce that product.".
 
pds4:urn:nasa:pds:0001_nasa_pds_1:all:user:pds:product::1.0 rdf:type rdfs:Class;
  rdfs:label "Product";
  pds4:subClassOf pds4:urn:nasa:pds:0001_nasa_pds_1:all:user::1.0;
  rdfs:comment "A Product is a uniquely identified object that is managed by a registry\\//repository. It consists of one or more tagged data objects.".
 
pds4:urn:nasa:pds:0001_nasa_pds_1:pds:product:pds:product_aip::1.0 rdf:type rdfs:Class;
  rdfs:label "Product_AIP";
  pds4:subClassOf pds4:urn:nasa:pds:0001_nasa_pds_1:all:user:pds:product::1.0;
  rdfs:comment "The Product AIP class defines a product for the Archival Information Package.".
 
pds4:urn:nasa:pds:0001_nasa_pds_1:pds:product:pds:product_ancillary::1.0 rdf:type rdfs:Class;
  rdfs:label "Product_Ancillary";
  pds4:subClassOf pds4:urn:nasa:pds:0001_nasa_pds_1:all:user:pds:product::1.0;
  rdfs:comment "The Product_Ancillary class defines a product that contains data that are supplementary to observational data and cannot reasonably be associated with any other non-observational data class. Use of Product_Ancillary must be approved by the curating node.".
 
pds4:urn:nasa:pds:0001_nasa_pds_1:pds:product:pds:product_attribute_definition::1.0 rdf:type rdfs:Class;
  rdfs:label "Product_Attribute_Definition";
  pds4:subClassOf pds4:urn:nasa:pds:0001_nasa_pds_1:all:user:pds:product::1.0;
  rdfs:comment "The Product Attribute Definition provides an attribute definition in XML encoding.".
 
pds4:urn:nasa:pds:0001_nasa_pds_1:pds:product:pds:product_browse::1.0 rdf:type rdfs:Class;
  rdfs:label "Product_Browse";
  pds4:subClassOf pds4:urn:nasa:pds:0001_nasa_pds_1:all:user:pds:product::1.0;
  rdfs:comment "The Product Browse class defines a product consisting of one  encoded byte stream digital object.".
 
pds4:urn:nasa:pds:0001_nasa_pds_1:pds:product:pds:product_bundle::1.0 rdf:type rdfs:Class;
  rdfs:label "Product_Bundle";
  pds4:subClassOf pds4:urn:nasa:pds:0001_nasa_pds_1:all:user:pds:product::1.0;
  rdfs:comment "A Product_Bundle is an aggregate product and has a table of references to one or more collections.".
 
pds4:urn:nasa:pds:0001_nasa_pds_1:pds:product:pds:product_class_definition::1.0 rdf:type rdfs:Class;
  rdfs:label "Product_Class_Definition";
  pds4:subClassOf pds4:urn:nasa:pds:0001_nasa_pds_1:all:user:pds:product::1.0;
  rdfs:comment "The Product Class Definition provides a class definition in XML encoding.".
 
pds4:urn:nasa:pds:0001_nasa_pds_1:pds:product:pds:product_collection::1.0 rdf:type rdfs:Class;
  rdfs:label "Product_Collection";
  pds4:subClassOf pds4:urn:nasa:pds:0001_nasa_pds_1:all:user:pds:product::1.0;
  rdfs:comment "A Product_Collection has a table of references to one or more basic products. The references are stored in a table called the inventory.".
 
pds4:urn:nasa:pds:0001_nasa_pds_1:pds:product:pds:product_context::1.0 rdf:type rdfs:Class;
  rdfs:label "Product_Context";
  pds4:subClassOf pds4:urn:nasa:pds:0001_nasa_pds_1:all:user:pds:product::1.0;
  rdfs:comment "The Product Context class describes something that provides context and provenance for an observational product.".
 
pds4:urn:nasa:pds:0001_nasa_pds_1:pds:product:pds:product_dip::1.0 rdf:type rdfs:Class;
  rdfs:label "Product_DIP";
  pds4:subClassOf pds4:urn:nasa:pds:0001_nasa_pds_1:all:user:pds:product::1.0;
  rdfs:comment "The Product DIP class defines a product for the Dissemination Information Package.".
 
pds4:urn:nasa:pds:0001_nasa_pds_1:pds:product:pds:product_dip_deep_archive::1.0 rdf:type rdfs:Class;
  rdfs:label "Product_DIP_Deep_Archive";
  pds4:subClassOf pds4:urn:nasa:pds:0001_nasa_pds_1:all:user:pds:product::1.0;
  rdfs:comment "The Product DIP_Deep_Archive class defines a product for the Dissemination Information Package for the deep archive.".
 
pds4:urn:nasa:pds:0001_nasa_pds_1:pds:product:pds:product_data_set_pds3::1.0 rdf:type rdfs:Class;
  rdfs:label "Product_Data_Set_PDS3";
  pds4:subClassOf pds4:urn:nasa:pds:0001_nasa_pds_1:all:user:pds:product::1.0;
  rdfs:comment "The Data Set PDS3 product  is used to create proxy labels for the data sets in the PDS3 Data Set catalog.".
 
pds4:urn:nasa:pds:0001_nasa_pds_1:pds:product:pds:product_document::1.0 rdf:type rdfs:Class;
  rdfs:label "Product_Document";
  pds4:subClassOf pds4:urn:nasa:pds:0001_nasa_pds_1:all:user:pds:product::1.0;
  rdfs:comment "A Product Document is a product consisting of a single logical document that may comprise one or more document editions.".
 
pds4:urn:nasa:pds:0001_nasa_pds_1:pds:product:pds:product_file_repository::1.0 rdf:type rdfs:Class;
  rdfs:label "Product_File_Repository";
  pds4:subClassOf pds4:urn:nasa:pds:0001_nasa_pds_1:all:user:pds:product::1.0;
  rdfs:comment "The Product File Repository class consists of a single text file. This product is used to register a file in a repository.".
 
pds4:urn:nasa:pds:0001_nasa_pds_1:pds:product:pds:product_file_text::1.0 rdf:type rdfs:Class;
  rdfs:label "Product_File_Text";
  pds4:subClassOf pds4:urn:nasa:pds:0001_nasa_pds_1:all:user:pds:product::1.0;
  rdfs:comment "The Product File Text consists of a single text file with ASCII character encoding.".
 
pds4:urn:nasa:pds:0001_nasa_pds_1:pds:product:pds:product_instrument_host_pds3::1.0 rdf:type rdfs:Class;
  rdfs:label "Product_Instrument_Host_PDS3";
  pds4:subClassOf pds4:urn:nasa:pds:0001_nasa_pds_1:all:user:pds:product::1.0;
  rdfs:comment "An Instrument Host product describes an instrument host. This product captures the PDS3 catalog instrument host information.".
 
pds4:urn:nasa:pds:0001_nasa_pds_1:pds:product:pds:product_instrument_pds3::1.0 rdf:type rdfs:Class;
  rdfs:label "Product_Instrument_PDS3";
  pds4:subClassOf pds4:urn:nasa:pds:0001_nasa_pds_1:all:user:pds:product::1.0;
  rdfs:comment "An Instrument product describes an instrument. This product captures the PDS3 catalog instrument information.".
 
pds4:urn:nasa:pds:0001_nasa_pds_1:pds:product:pds:product_metadata_supplemental::1.0 rdf:type rdfs:Class;
  rdfs:label "Product_Metadata_Supplemental";
  pds4:subClassOf pds4:urn:nasa:pds:0001_nasa_pds_1:all:user:pds:product::1.0;
  rdfs:comment "The Product_Metadata_Supplemental class is used to provide new, and\\//or improved, metadata for some or all of the basic products in a single collection. More than one Product_Metadata_Supplemental may apply to any given collection, but a Product_Metadata_Supplemental may only be associated with a single collection. Each Product_Metadata_Supplemental will be a primary member of the collection to which it applies.".
 
pds4:urn:nasa:pds:0001_nasa_pds_1:pds:product:pds:product_mission_pds3::1.0 rdf:type rdfs:Class;
  rdfs:label "Product_Mission_PDS3";
  pds4:subClassOf pds4:urn:nasa:pds:0001_nasa_pds_1:all:user:pds:product::1.0;
  rdfs:comment "An Mission product describes a mission. This product captures the PDS3 catalog mission information.".
 
pds4:urn:nasa:pds:0001_nasa_pds_1:pds:product:pds:product_native::1.0 rdf:type rdfs:Class;
  rdfs:label "Product_Native";
  pds4:subClassOf pds4:urn:nasa:pds:0001_nasa_pds_1:all:user:pds:product::1.0;
  rdfs:comment "Product_Native is used to describe digital objects in the original format returned by the spacecraft or experimental system when that format  cannot be described using one of the PDS4 formats specified for observational data (tables or arrays,  excluding Array_1D).".
 
pds4:urn:nasa:pds:0001_nasa_pds_1:pds:product:pds:product_observational::1.0 rdf:type rdfs:Class;
  rdfs:label "Product_Observational";
  pds4:subClassOf pds4:urn:nasa:pds:0001_nasa_pds_1:all:user:pds:product::1.0;
  rdfs:comment "A Product_Observational is a set of one or more information objects produced by an observing system.".
 
pds4:urn:nasa:pds:0001_nasa_pds_1:pds:product:pds:product_proxy_pds3::1.0 rdf:type rdfs:Class;
  rdfs:label "Product_Proxy_PDS3";
  pds4:subClassOf pds4:urn:nasa:pds:0001_nasa_pds_1:all:user:pds:product::1.0;
  rdfs:comment "The Product Proxy PDS3 class defines a product with enough information to register a PDS3 data product.".
 
pds4:urn:nasa:pds:0001_nasa_pds_1:pds:product:pds:product_sip::1.0 rdf:type rdfs:Class;
  rdfs:label "Product_SIP";
  pds4:subClassOf pds4:urn:nasa:pds:0001_nasa_pds_1:all:user:pds:product::1.0;
  rdfs:comment "The Product SIP class defines a product for the Submission Information Package.".
 
pds4:urn:nasa:pds:0001_nasa_pds_1:pds:product:pds:product_sip_deep_archive::1.0 rdf:type rdfs:Class;
  rdfs:label "Product_SIP_Deep_Archive";
  pds4:subClassOf pds4:urn:nasa:pds:0001_nasa_pds_1:all:user:pds:product::1.0;
  rdfs:comment "The Product SIP Deep Archive class defines a Submission Information Package (SIP) for the NASA planetary science deep archive.".
 
pds4:urn:nasa:pds:0001_nasa_pds_1:pds:product:pds:product_spice_kernel::1.0 rdf:type rdfs:Class;
  rdfs:label "Product_SPICE_Kernel";
  pds4:subClassOf pds4:urn:nasa:pds:0001_nasa_pds_1:all:user:pds:product::1.0;
  rdfs:comment "The Product SPICE Kernel class defines a SPICE kernel product.".
 
pds4:urn:nasa:pds:0001_nasa_pds_1:pds:product:pds:product_service::1.0 rdf:type rdfs:Class;
  rdfs:label "Product_Service";
  pds4:subClassOf pds4:urn:nasa:pds:0001_nasa_pds_1:all:user:pds:product::1.0;
  rdfs:comment "The Product Service class defines a product for registering services. Service descriptions from this product are used to register services as intrinsic registry objects.".
 
pds4:urn:nasa:pds:0001_nasa_pds_1:pds:product:pds:product_software::1.0 rdf:type rdfs:Class;
  rdfs:label "Product_Software";
  pds4:subClassOf pds4:urn:nasa:pds:0001_nasa_pds_1:all:user:pds:product::1.0;
  rdfs:comment "Product Software is a product consisting of a set of one or more software formats.".
 
pds4:urn:nasa:pds:0001_nasa_pds_1:pds:product:pds:product_subscription_pds3::1.0 rdf:type rdfs:Class;
  rdfs:label "Product_Subscription_PDS3";
  pds4:subClassOf pds4:urn:nasa:pds:0001_nasa_pds_1:all:user:pds:product::1.0;
  rdfs:comment "The Product_Subscription_PDS3 class provides the list of subscriptions for a PDS3 subscriber.".
 
pds4:urn:nasa:pds:0001_nasa_pds_1:pds:product:pds:product_target_pds3::1.0 rdf:type rdfs:Class;
  rdfs:label "Product_Target_PDS3";
  pds4:subClassOf pds4:urn:nasa:pds:0001_nasa_pds_1:all:user:pds:product::1.0;
  rdfs:comment "A target product describes a target. This product captures a reduced set of the PDS3 catalog target information.".
 
pds4:urn:nasa:pds:0001_nasa_pds_1:pds:product:pds:product_thumbnail::1.0 rdf:type rdfs:Class;
  rdfs:label "Product_Thumbnail";
  pds4:subClassOf pds4:urn:nasa:pds:0001_nasa_pds_1:all:user:pds:product::1.0;
  rdfs:comment "The Product Thumbnail class defines a product consisting of one encoded byte stream digital object.".
 
pds4:urn:nasa:pds:0001_nasa_pds_1:pds:product:pds:product_update::1.0 rdf:type rdfs:Class;
  rdfs:label "Product_Update";
  pds4:subClassOf pds4:urn:nasa:pds:0001_nasa_pds_1:all:user:pds:product::1.0;
  rdfs:comment "The Product Update class defines a product consisting of update information and optional references to other products.".
 
pds4:urn:nasa:pds:0001_nasa_pds_1:pds:product:pds:product_volume_pds3::1.0 rdf:type rdfs:Class;
  rdfs:label "Product_Volume_PDS3";
  pds4:subClassOf pds4:urn:nasa:pds:0001_nasa_pds_1:all:user:pds:product::1.0;
  rdfs:comment "A Product Volume PDS3 product captures the PDS3 volume information.".
 
pds4:urn:nasa:pds:0001_nasa_pds_1:pds:product:pds:product_volume_set_pds3::1.0 rdf:type rdfs:Class;
  rdfs:label "Product_Volume_Set_PDS3";
  pds4:subClassOf pds4:urn:nasa:pds:0001_nasa_pds_1:all:user:pds:product::1.0;
  rdfs:comment "A Product Volume Set PDS3 product captures the PDS3 volume set information.".
 
pds4:urn:nasa:pds:0001_nasa_pds_1:pds:product:pds:product_xml_schema::1.0 rdf:type rdfs:Class;
  rdfs:label "Product_XML_Schema";
  pds4:subClassOf pds4:urn:nasa:pds:0001_nasa_pds_1:all:user:pds:product::1.0;
  rdfs:comment "The Product_XML_Schema  describes a resource used for the PDS4 implementation into XML.".
 
pds4:urn:nasa:pds:0001_nasa_pds_1:pds:product:pds:product_zipped::1.0 rdf:type rdfs:Class;
  rdfs:label "Product_Zipped";
  pds4:subClassOf pds4:urn:nasa:pds:0001_nasa_pds_1:all:user:pds:product::1.0;
  rdfs:comment "The Product_Zipped  is a product with references to other products. The referenced products and all associated products and files are packaged into a single ZIP file.".
 
pds4:urn:nasa:pds:0001_nasa_pds_1:pds:tndo_supplemental:pds:property_map::1.0 rdf:type rdfs:Class;
  rdfs:label "Property_Map";
  pds4:subClassOf pds4:urn:nasa:pds:0001_nasa_pds_1:pds:tagged_nondigital_object:pds:tndo_supplemental::1.0;
  rdfs:comment "The Property Map class defines a table consisting of a set of data elements and their values. The data elements in this table are considered to be locally defined and not subject to standards except for nomenclature rules.".
 
pds4:urn:nasa:pds:0001_nasa_pds_1:pds:tndo_supplemental:pds:property_map_entry::1.0 rdf:type rdfs:Class;
  rdfs:label "Property_Map_Entry";
  pds4:subClassOf pds4:urn:nasa:pds:0001_nasa_pds_1:pds:tagged_nondigital_object:pds:tndo_supplemental::1.0;
  rdfs:comment "The property map entry consists of a property name and one or more values.".
 
pds4:urn:nasa:pds:0001_nasa_pds_1:pds:tndo_supplemental:pds:property_maps::1.0 rdf:type rdfs:Class;
  rdfs:label "Property_Maps";
  pds4:subClassOf pds4:urn:nasa:pds:0001_nasa_pds_1:pds:tagged_nondigital_object:pds:tndo_supplemental::1.0;
  rdfs:comment "The Property Maps class defines a collection of one or more related Property Maps.".
 
pds4:urn:nasa:pds:0001_nasa_pds_1:pds:tndo_supplemental:pds:quaternion::1.0 rdf:type rdfs:Class;
  rdfs:label "Quaternion";
  pds4:subClassOf pds4:urn:nasa:pds:0001_nasa_pds_1:pds:tagged_nondigital_object:pds:tndo_supplemental::1.0;
  rdfs:comment "The Quaternion class models a mathematical construct that consists of four individual numeric components.  Quaternions are a convenient mechanism for encapsulating orientation information since they require only four units of numeric storage, as opposed to the nine needed for a rotation matrix.".
 
pds4:urn:nasa:pds:0001_nasa_pds_1:pds:tndo_supplemental:pds:quaternion:spice::1.0 rdf:type rdfs:Class;
  rdfs:label "SPICE";
  rdfs:subClassOf pds4:urn:nasa:pds:0001_nasa_pds_1:pds:tndo_supplemental:pds:quaternion::1.0;
  rdfs:comment "The quaternion has components zero through three, with the 0th component being the scalar, and the 1st, 2nd and 3rd being the vector components.".
 
pds4:urn:nasa:pds:0001_nasa_pds_1:pds:tndo_supplemental:pds:quaternion:spacecraft_telemetry::1.0 rdf:type rdfs:Class;
  rdfs:label "Spacecraft Telemetry";
  rdfs:subClassOf pds4:urn:nasa:pds:0001_nasa_pds_1:pds:tndo_supplemental:pds:quaternion::1.0;
  rdfs:comment "The quaternion has components one through four, with the 4th component being the scalar, and the 1st, 2nd and 3rd being the vector components.".
 
pds4:urn:nasa:pds:0001_nasa_pds_1:all:user:geom:quaternion_base::1.0 rdf:type rdfs:Class;
  rdfs:label "Quaternion_Base";
  pds4:subClassOf pds4:urn:nasa:pds:0001_nasa_pds_1:all:user::1.0;
  rdfs:comment "The Quaternion_Base class defines a quaternion that represents rotation between two right-handed reference frames. In this dictionary, quaternions are always constructed so that the application of the quaternion describes the rotation of one frame to a second frame. The two frames and the direction of rotation must be identified unambiguously in the enclosing classes. Quaternions are expressed as a set of four numbers in the order (qcos, qsin1, qsin2, qsin3), where qcos = cos(theta\\//2) and qsin(n) = sin(theta\\//2)*a(n). Theta is the angle of rotation and a is the unit vector (x,y,z) around which the rotation occurs. A document providing the full mathematical basis for this construction, along with examples, and a summary of common pitfalls, is in preparation. The current version can be obtained by contacting the PDS Engineering Node. In application you need to know the four elements of the quaternion, the two end point frames, and the direction of the rotation. This dictionary provides two extensions to this Base class. In the Quaternion_Plus_Direction class we require the direction of rotation. This class can only be used if the two end point frames are identified in the enclosing class. This is generally the case in the Lander section. The Quaternion_Plus_To_From class requires the two frames be identified explicitly with one designated as the \"from frame\" and the other as the \"to frame\". ".
 
pds4:urn:nasa:pds:0001_nasa_pds_1:pds:tagged_nondigital_child:pds:quaternion_component::1.0 rdf:type rdfs:Class;
  rdfs:label "Quaternion_Component";
  pds4:subClassOf pds4:urn:nasa:pds:0001_nasa_pds_1:all:user:pds:tagged_nondigital_child::1.0;
  rdfs:comment "The Quaternion_Component class provides a component of a quaternion.".
 
pds4:urn:nasa:pds:0001_nasa_pds_1:geom:quaternion_base:geom:quaternion_model_transform::1.0 rdf:type rdfs:Class;
  rdfs:label "Quaternion_Model_Transform";
  pds4:subClassOf pds4:urn:nasa:pds:0001_nasa_pds_1:all:user:geom:quaternion_base::1.0;
  rdfs:comment "The Quaternion_Model_Transform class specifies, along with Vector_Model_Transform class, the transform used for the camera model in an image. Camera models created by the calibration process have associated with them a pose, comprised of the position (offset) and orientation (quaternion) of the camera at the time it was calibrated. The model is transformed (\"pointed\") for a specific image by computing, generally using articulation device kinematics, a final pose for the image. The camera model is then translated and rotated from the calibration to final pose. This class specifies the quaternion portion of the final pose. ".
 
pds4:urn:nasa:pds:0001_nasa_pds_1:geom:quaternion_base:geom:quaternion_plus_direction::1.0 rdf:type rdfs:Class;
  rdfs:label "Quaternion_Plus_Direction";
  pds4:subClassOf pds4:urn:nasa:pds:0001_nasa_pds_1:all:user:geom:quaternion_base::1.0;
  rdfs:comment "Quaternion_Plus_Direction provides the four elements of a quaternion and its direction of rotation. The two end point frames must be identified in the enclosing class. See the definition of Quaternion_Base for more details on the quaternion classes in this dictionary. ".
 
pds4:urn:nasa:pds:0001_nasa_pds_1:geom:quaternion_base:geom:quaternion_plus_to_from::1.0 rdf:type rdfs:Class;
  rdfs:label "Quaternion_Plus_To_From";
  pds4:subClassOf pds4:urn:nasa:pds:0001_nasa_pds_1:all:user:geom:quaternion_base::1.0;
  rdfs:comment "Quaternion_Plus_To_From provides the four elements of a quaternion, plus attributes which identify the initial (Rotate_From) and final (Rotate_To) frames of the rotation. See the defintion of Quaternion_Base for more details on the quaternion classes in this dictionary. ".
 
pds4:urn:nasa:pds:0001_nasa_pds_1:all:user:img:radial_flat_field_function::1.0 rdf:type rdfs:Class;
  rdfs:label "Radial_Flat_Field_Function";
  pds4:subClassOf pds4:urn:nasa:pds:0001_nasa_pds_1:all:user::1.0;
  rdfs:comment "The Radial_Flat_Field_Function class pecifies parameters used to generate a synthetic flat field using a simple radial function of the form: r = (x-x_center)^2 + (y-y_center)^2 ; flat_field(x,y) = 1 + r0 + r1*r + r2*r^2 + r3*r^3 . Note that x is in the sample direction of the image, and y is in the line direction. The image is multiplied by this function in order to perform a flat field correction (which is the opposite of Flat_Field_File). ".
 
pds4:urn:nasa:pds:0001_nasa_pds_1:geom:polynomial_coefficients_3:geom:radial_terms::1.0 rdf:type rdfs:Class;
  rdfs:label "Radial_Terms";
  pds4:subClassOf pds4:urn:nasa:pds:0001_nasa_pds_1:all:user:geom:polynomial_coefficients_3::1.0;
  rdfs:comment "Radial_Terms contains the coefficients of a polynomial function used to describe the radial distortion of the camera. ".
 
pds4:urn:nasa:pds:0001_nasa_pds_1:img:data_processing:img:radiometric_correction::1.0 rdf:type rdfs:Class;
  rdfs:label "Radiometric_Correction";
  pds4:subClassOf pds4:urn:nasa:pds:0001_nasa_pds_1:all:user:img:data_processing::1.0;
  rdfs:comment " The Radiometric_Correction class is a container for the type and details of the radiometric calibration performed on the product.".
 
pds4:urn:nasa:pds:0001_nasa_pds_1:all:user:img_surface:reach_instrument::1.0 rdf:type rdfs:Class;
  rdfs:label "Reach_Instrument";
  pds4:subClassOf pds4:urn:nasa:pds:0001_nasa_pds_1:all:user::1.0;
  rdfs:comment "Defines a single instrument for this reachability assessment. For products where each instrument is associated with a band in the output, the \"band\" attribute specifies which band it is. For products where instruments are involved in the computation but not represented individually in the output, the band should be omitted.".
 
pds4:urn:nasa:pds:0001_nasa_pds_1:all:user:img_surface:reach_instruments::1.0 rdf:type rdfs:Class;
  rdfs:label "Reach_Instruments";
  pds4:subClassOf pds4:urn:nasa:pds:0001_nasa_pds_1:all:user::1.0;
  rdfs:comment "Lists the instruments involved in this reachability assesment.".
 
pds4:urn:nasa:pds:0001_nasa_pds_1:all:user:img_surface:reachability::1.0 rdf:type rdfs:Class;
  rdfs:label "Reachability";
  pds4:subClassOf pds4:urn:nasa:pds:0001_nasa_pds_1:all:user::1.0;
  rdfs:comment "This class describes Reachability products, which define whether and how a moving device (such as an arm) can contact, view, or otherwise interact with the world at each pixel of an image.".
 
pds4:urn:nasa:pds:0001_nasa_pds_1:pds:tagged_digital_child:pds:record::1.0 rdf:type rdfs:Class;
  rdfs:label "Record";
  pds4:subClassOf pds4:urn:nasa:pds:0001_nasa_pds_1:all:user:pds:tagged_digital_child::1.0;
  rdfs:comment "The Record class defines a record of a file and is the parent class of all specific record classes.".
 
pds4:urn:nasa:pds:0001_nasa_pds_1:pds:record:pds:record_binary::1.0 rdf:type rdfs:Class;
  rdfs:label "Record_Binary";
  pds4:subClassOf pds4:urn:nasa:pds:0001_nasa_pds_1:pds:tagged_digital_child:pds:record::1.0;
  rdfs:comment "The Record_Binary class is a component of the table class and defines a record of the table.".
 
pds4:urn:nasa:pds:0001_nasa_pds_1:pds:record:pds:record_character::1.0 rdf:type rdfs:Class;
  rdfs:label "Record_Character";
  pds4:subClassOf pds4:urn:nasa:pds:0001_nasa_pds_1:pds:tagged_digital_child:pds:record::1.0;
  rdfs:comment "The Record_Character class is a component of the table class and defines a record of the table.".
 
pds4:urn:nasa:pds:0001_nasa_pds_1:pds:record:pds:record_delimited::1.0 rdf:type rdfs:Class;
  rdfs:label "Record_Delimited";
  pds4:subClassOf pds4:urn:nasa:pds:0001_nasa_pds_1:pds:tagged_digital_child:pds:record::1.0;
  rdfs:comment "The Record_Delimited class is a component of the delimited table (spreadsheet) class and defines a record of the delimited table.".
 
pds4:urn:nasa:pds:0001_nasa_pds_1:all:user:sp:rectangular_fov::1.0 rdf:type rdfs:Class;
  rdfs:label "Rectangular_FOV";
  pds4:subClassOf pds4:urn:nasa:pds:0001_nasa_pds_1:all:user::1.0;
  rdfs:comment " This class is used to describe a rectangular (i.e., slit) aperture. ".
 
pds4:urn:nasa:pds:0001_nasa_pds_1:rings:frame_ident_base:rings:reference_frame_ident::1.0 rdf:type rdfs:Class;
  rdfs:label "Reference_Frame_Ident";
  pds4:subClassOf pds4:urn:nasa:pds:0001_nasa_pds_1:all:user:rings:frame_ident_base::1.0;
  rdfs:comment "The Reference_Frame_Ident class is a base class for identifying reference frames. These are frames in the NAIF sense, i.e., three orthogonal axes with a specified orientation, but without a fixed origin. ".
 
pds4:urn:nasa:pds:0001_nasa_pds_1:geom:frame_identification_base:geom:reference_frame_identification::1.0 rdf:type rdfs:Class;
  rdfs:label "Reference_Frame_Identification";
  pds4:subClassOf pds4:urn:nasa:pds:0001_nasa_pds_1:all:user:geom:frame_identification_base::1.0;
  rdfs:comment "The Reference_Frame_Identification class is a base class for identifying reference frames. These are frames in the NAIF sense, i.e., three orthogonal axes with a specified orientation, but without a fixed origin. ".
 
pds4:urn:nasa:pds:0001_nasa_pds_1:pds:product_components:pds:reference_list::1.0 rdf:type rdfs:Class;
  rdfs:label "Reference_List";
  pds4:subClassOf pds4:urn:nasa:pds:0001_nasa_pds_1:all:user:pds:product_components::1.0;
  rdfs:comment "The Reference_List class provides general references, cross-references, and source products for the product. References cited elsewhere in the label need not be repeated here.".
 
pds4:urn:nasa:pds:0001_nasa_pds_1:all:user:geom:reference_pixel::1.0 rdf:type rdfs:Class;
  rdfs:label "Reference_Pixel";
  pds4:subClassOf pds4:urn:nasa:pds:0001_nasa_pds_1:all:user::1.0;
  rdfs:comment "The Reference_Pixel class provides the pixel coordinates, line and sample, to which values in the containing class apply. Integer values indicate the center of the pixel. Sub-pixel values are permitted. For pixel_sample, the leading edge (left edge for sample increasing to the right) has a value 0.5 less than the integer value at the center, and the value for the trailing edge is the center integer value + 0.5. For pixel_line, the leading and trailing edges (top and bottom respectively for line increasing downward) again are -0.5 and +0.5 with respect to the center integer value. ".
 
pds4:urn:nasa:pds:0001_nasa_pds_1:all:user:img:reference_pixel::1.0 rdf:type rdfs:Class;
  rdfs:label "Reference_Pixel";
  pds4:subClassOf pds4:urn:nasa:pds:0001_nasa_pds_1:all:user::1.0;
  rdfs:comment "Describes a Reference Pixel product, which is a set of dark, non-imaging pixels used to monitor electronics. product_flag.".
 
pds4:urn:nasa:pds:0001_nasa_pds_1:all:user:rings:reprojection_geometry::1.0 rdf:type rdfs:Class;
  rdfs:label "Reprojection_Geometry";
  pds4:subClassOf pds4:urn:nasa:pds:0001_nasa_pds_1:all:user::1.0;
  rdfs:comment "This class provides the parameters describing reprojection geometry when the ring(s) is reprojected based on a fixed grid of coordinates (.g., radius vs. longitude).".
 
pds4:urn:nasa:pds:0001_nasa_pds_1:pds:tndo_context:pds:resource::1.0 rdf:type rdfs:Class;
  rdfs:label "Resource";
  pds4:subClassOf pds4:urn:nasa:pds:0001_nasa_pds_1:pds:tagged_nondigital_object:pds:tndo_context::1.0;
  rdfs:comment "The Resource class provides a description of a web resource.".
 
pds4:urn:nasa:pds:0001_nasa_pds_1:pds:tndo_context:pds:resource:information.agency::1.0 rdf:type rdfs:Class;
  rdfs:label "Information.Agency";
  rdfs:subClassOf pds4:urn:nasa:pds:0001_nasa_pds_1:pds:tndo_context:pds:resource::1.0;
  rdfs:comment "The web resource provides information about an agency.".
 
pds4:urn:nasa:pds:0001_nasa_pds_1:pds:tndo_context:pds:resource:information.instrument::1.0 rdf:type rdfs:Class;
  rdfs:label "Information.Instrument";
  rdfs:subClassOf pds4:urn:nasa:pds:0001_nasa_pds_1:pds:tndo_context:pds:resource::1.0;
  rdfs:comment "The web resource provides information about an instrument".
 
pds4:urn:nasa:pds:0001_nasa_pds_1:pds:tndo_context:pds:resource:information.instrument_host::1.0 rdf:type rdfs:Class;
  rdfs:label "Information.Instrument_Host";
  rdfs:subClassOf pds4:urn:nasa:pds:0001_nasa_pds_1:pds:tndo_context:pds:resource::1.0;
  rdfs:comment "The web resource provides information about an instrument host".
 
pds4:urn:nasa:pds:0001_nasa_pds_1:pds:tndo_context:pds:resource:information.investigation::1.0 rdf:type rdfs:Class;
  rdfs:label "Information.Investigation";
  rdfs:subClassOf pds4:urn:nasa:pds:0001_nasa_pds_1:pds:tndo_context:pds:resource::1.0;
  rdfs:comment "The web resource provides information about an investigation".
 
pds4:urn:nasa:pds:0001_nasa_pds_1:pds:tndo_context:pds:resource:information.node::1.0 rdf:type rdfs:Class;
  rdfs:label "Information.Node";
  rdfs:subClassOf pds4:urn:nasa:pds:0001_nasa_pds_1:pds:tndo_context:pds:resource::1.0;
  rdfs:comment "The web resource provides information about a node".
 
pds4:urn:nasa:pds:0001_nasa_pds_1:pds:tndo_context:pds:resource:information.person::1.0 rdf:type rdfs:Class;
  rdfs:label "Information.Person";
  rdfs:subClassOf pds4:urn:nasa:pds:0001_nasa_pds_1:pds:tndo_context:pds:resource::1.0;
  rdfs:comment "The web resource provides information about a person".
 
pds4:urn:nasa:pds:0001_nasa_pds_1:pds:tndo_context:pds:resource:information.resource::1.0 rdf:type rdfs:Class;
  rdfs:label "Information.Resource";
  rdfs:subClassOf pds4:urn:nasa:pds:0001_nasa_pds_1:pds:tndo_context:pds:resource::1.0;
  rdfs:comment "The web resource provides information about a generic resource".
 
pds4:urn:nasa:pds:0001_nasa_pds_1:pds:tndo_context:pds:resource:information.science_portal::1.0 rdf:type rdfs:Class;
  rdfs:label "Information.Science_Portal";
  rdfs:subClassOf pds4:urn:nasa:pds:0001_nasa_pds_1:pds:tndo_context:pds:resource::1.0;
  rdfs:comment "The web resource provides information about a science portal".
 
pds4:urn:nasa:pds:0001_nasa_pds_1:pds:tndo_context:pds:resource:information.target::1.0 rdf:type rdfs:Class;
  rdfs:label "Information.Target";
  rdfs:subClassOf pds4:urn:nasa:pds:0001_nasa_pds_1:pds:tndo_context:pds:resource::1.0;
  rdfs:comment "The web resource provides information about a target".
 
pds4:urn:nasa:pds:0001_nasa_pds_1:pds:tndo_context:pds:resource:system.browse::1.0 rdf:type rdfs:Class;
  rdfs:label "System.Browse";
  rdfs:subClassOf pds4:urn:nasa:pds:0001_nasa_pds_1:pds:tndo_context:pds:resource::1.0;
  rdfs:comment "The system resource provides browse functionality.".
 
pds4:urn:nasa:pds:0001_nasa_pds_1:pds:tndo_context:pds:resource:system.directory_listing::1.0 rdf:type rdfs:Class;
  rdfs:label "System.Directory_Listing";
  rdfs:subClassOf pds4:urn:nasa:pds:0001_nasa_pds_1:pds:tndo_context:pds:resource::1.0;
  rdfs:comment "The system resource provides a directory listing.".
 
pds4:urn:nasa:pds:0001_nasa_pds_1:pds:tndo_context:pds:resource:system.registry_query::1.0 rdf:type rdfs:Class;
  rdfs:label "System.Registry_Query";
  rdfs:subClassOf pds4:urn:nasa:pds:0001_nasa_pds_1:pds:tndo_context:pds:resource::1.0;
  rdfs:comment "The system resource provides registry query functionality.".
 
pds4:urn:nasa:pds:0001_nasa_pds_1:pds:tndo_context:pds:resource:system.search::1.0 rdf:type rdfs:Class;
  rdfs:label "System.Search";
  rdfs:subClassOf pds4:urn:nasa:pds:0001_nasa_pds_1:pds:tndo_context:pds:resource::1.0;
  rdfs:comment "The system resource provides search functionality.".
 
pds4:urn:nasa:pds:0001_nasa_pds_1:pds:tndo_context:pds:resource:system.transform::1.0 rdf:type rdfs:Class;
  rdfs:label "System.Transform";
  rdfs:subClassOf pds4:urn:nasa:pds:0001_nasa_pds_1:pds:tndo_context:pds:resource::1.0;
  rdfs:comment "The system resource provides transform functionality.".
 
pds4:urn:nasa:pds:0001_nasa_pds_1:pds:tndo_context:pds:resource:system.transport::1.0 rdf:type rdfs:Class;
  rdfs:label "System.Transport";
  rdfs:subClassOf pds4:urn:nasa:pds:0001_nasa_pds_1:pds:tndo_context:pds:resource::1.0;
  rdfs:comment "The system resource provides transport functionality.".
 
pds4:urn:nasa:pds:0001_nasa_pds_1:rings:body_ident_base:rings:ring_identification::1.0 rdf:type rdfs:Class;
  rdfs:label "Ring_Identification";
  pds4:subClassOf pds4:urn:nasa:pds:0001_nasa_pds_1:all:user:rings:body_ident_base::1.0;
  rdfs:comment "This class identifies the specific ring to which the parameters given in the enclosing class apply.".
 
pds4:urn:nasa:pds:0001_nasa_pds_1:all:user:rings:ring_model::1.0 rdf:type rdfs:Class;
  rdfs:label "Ring_Model";
  pds4:subClassOf pds4:urn:nasa:pds:0001_nasa_pds_1:all:user::1.0;
  rdfs:comment "This class provides the parameters used to generate a ring model.".
 
pds4:urn:nasa:pds:0001_nasa_pds_1:all:user:rings:ring_moon_systems::1.0 rdf:type rdfs:Class;
  rdfs:label "Ring_Moon_Systems";
  pds4:subClassOf pds4:urn:nasa:pds:0001_nasa_pds_1:all:user::1.0;
  rdfs:comment "This is an umbrella class for all of the classes and attributes in this dictionary.".
 
pds4:urn:nasa:pds:0001_nasa_pds_1:all:user:rings:ring_orbital_elements::1.0 rdf:type rdfs:Class;
  rdfs:label "Ring_Orbital_Elements";
  pds4:subClassOf pds4:urn:nasa:pds:0001_nasa_pds_1:all:user::1.0;
  rdfs:comment "This class provides the orbital element values for a specific ring which were generated in a ring model.".
 
pds4:urn:nasa:pds:0001_nasa_pds_1:all:user:cart:ring_polar::1.0 rdf:type rdfs:Class;
  rdfs:label "Ring_Polar";
  pds4:subClassOf pds4:urn:nasa:pds:0001_nasa_pds_1:all:user::1.0;
  rdfs:comment "The representation of ring data requires a unique projection. The rings are modeled by a thin disk centered on the body and in its equatorial plane. For Saturn, the thin disk is centered on Saturn and in its equatorial plane, with an outer radius of 500,000km. If the field of view falls partially or completely beyond this limit or if it intersects the primary body before intersecting the rings, the data will not be included. Plotted coordinates are derived as follows. If A is the location of the intersection of the CIRS field of view with the body\\'s equatorial plane, the X coordinate is the distance of A from the center of the body (e.g. Saturn), and the Y coordinate is the local time on on the body at the intersection with the body\\'s surface of the line between A and the body\\'s center. Local time is expressed in fractional hours, from 0.0 (at midnight) to 12.0 (at noon), to 24.0 (at midnight). ".
 
pds4:urn:nasa:pds:0001_nasa_pds_1:all:user:rings:ring_reprojection::1.0 rdf:type rdfs:Class;
  rdfs:label "Ring_Reprojection";
  pds4:subClassOf pds4:urn:nasa:pds:0001_nasa_pds_1:all:user::1.0;
  rdfs:comment "This class provides the parameters used to describe ring reprojection geometry.".
 
pds4:urn:nasa:pds:0001_nasa_pds_1:all:user:rings:ring_spectrum::1.0 rdf:type rdfs:Class;
  rdfs:label "Ring_Spectrum";
  pds4:subClassOf pds4:urn:nasa:pds:0001_nasa_pds_1:all:user::1.0;
  rdfs:comment "This class provides the parameters used to describe ring spectra or spectrograms.".
 
pds4:urn:nasa:pds:0001_nasa_pds_1:all:user:survey:rollover::1.0 rdf:type rdfs:Class;
  rdfs:label "Rollover";
  pds4:subClassOf pds4:urn:nasa:pds:0001_nasa_pds_1:all:user::1.0;
  rdfs:comment "The properties of the peak of the histogram of stellar magnitudes within the image.".
 
pds4:urn:nasa:pds:0001_nasa_pds_1:geom:frame_identification_base:geom:rotate_from::1.0 rdf:type rdfs:Class;
  rdfs:label "Rotate_From";
  pds4:subClassOf pds4:urn:nasa:pds:0001_nasa_pds_1:all:user:geom:frame_identification_base::1.0;
  rdfs:comment "A quaternion rotates one reference frame to another reference frame. The Rotate_From class identifies the initial frame. ".
 
pds4:urn:nasa:pds:0001_nasa_pds_1:geom:frame_identification_base:geom:rotate_to::1.0 rdf:type rdfs:Class;
  rdfs:label "Rotate_To";
  pds4:subClassOf pds4:urn:nasa:pds:0001_nasa_pds_1:all:user:geom:frame_identification_base::1.0;
  rdfs:comment "A quaternion rotates a one reference frame to another reference frame. The Rotate_To class identifies the destination frame. ".
 
pds4:urn:nasa:pds:0001_nasa_pds_1:all:user:img:row_sum::1.0 rdf:type rdfs:Class;
  rdfs:label "Row_Sum";
  pds4:subClassOf pds4:urn:nasa:pds:0001_nasa_pds_1:all:user::1.0;
  rdfs:comment "Describes a Row Summation product, which is a single column containing the sum of all pixels in each row of the image.".
 
pds4:urn:nasa:pds:0001_nasa_pds_1:pds:information_package:pds:sip_deep_archive::1.0 rdf:type rdfs:Class;
  rdfs:label "SIP_Deep_Archive";
  pds4:subClassOf pds4:urn:nasa:pds:0001_nasa_pds_1:pds:tndo_supplemental:pds:information_package::1.0;
  rdfs:comment "The SIP Deep Archive class is a Submission Information Package (SIP)  for the NASA planetary science deep archive.".
 
pds4:urn:nasa:pds:0001_nasa_pds_1:pds:parsable_byte_stream:pds:spice_kernel::1.0 rdf:type rdfs:Class;
  rdfs:label "SPICE_Kernel";
  pds4:subClassOf pds4:urn:nasa:pds:0001_nasa_pds_1:pds:byte_stream:pds:parsable_byte_stream::1.0;
  rdfs:comment "The SPICE Kernel class describes a SPICE object.".
 
pds4:urn:nasa:pds:0001_nasa_pds_1:all:user:geom:spice_kernel_files::1.0 rdf:type rdfs:Class;
  rdfs:label "SPICE_Kernel_Files";
  pds4:subClassOf pds4:urn:nasa:pds:0001_nasa_pds_1:all:user::1.0;
  rdfs:comment "The SPICE_Kernel_Files class provides references to the SPICE files used when calculating geometric values. ".
 
pds4:urn:nasa:pds:0001_nasa_pds_1:all:user:geom:spice_kernel_identification::1.0 rdf:type rdfs:Class;
  rdfs:label "SPICE_Kernel_Identification";
  pds4:subClassOf pds4:urn:nasa:pds:0001_nasa_pds_1:all:user::1.0;
  rdfs:comment "The SPICE_Kernel_Identification class optionally includes the SPICE kernel type and provides two alternatives for identifying the product: LIDVID using Internal_Reference, and the file name of the kernel file. Although optional, LIDVID should be given if one is available. The optional kernel_provenance attribute indicates whether the kernel is a predict or reconstructed kernel, or some combination of the two, or if it is a kernel type for which such distinctions do not apply. ".
 
pds4:urn:nasa:pds:0001_nasa_pds_1:all:user:img:sampling::1.0 rdf:type rdfs:Class;
  rdfs:label "Sampling";
  pds4:subClassOf pds4:urn:nasa:pds:0001_nasa_pds_1:all:user::1.0;
  rdfs:comment " The Sampling class contains attributes and classes related to the sampling, scaling, companding, and compression or reduction in resolution of data.".
 
pds4:urn:nasa:pds:0001_nasa_pds_1:rings:body_ident_base:rings:satellite_identification::1.0 rdf:type rdfs:Class;
  rdfs:label "Satellite_Identification";
  pds4:subClassOf pds4:urn:nasa:pds:0001_nasa_pds_1:all:user:rings:body_ident_base::1.0;
  rdfs:comment "This class identifies the specific satellite to which the parameters given in the enclosing class apply.".
 
pds4:urn:nasa:pds:0001_nasa_pds_1:all:user:rings:satellite_parameters::1.0 rdf:type rdfs:Class;
  rdfs:label "Satellite_Parameters";
  pds4:subClassOf pds4:urn:nasa:pds:0001_nasa_pds_1:all:user::1.0;
  rdfs:comment "This class provides the parameters used to generate a ring model which are specific to a single satellite.".
 
pds4:urn:nasa:pds:0001_nasa_pds_1:pds:product_components:pds:science_facets::1.0 rdf:type rdfs:Class;
  rdfs:label "Science_Facets";
  pds4:subClassOf pds4:urn:nasa:pds:0001_nasa_pds_1:all:user:pds:product_components::1.0;
  rdfs:comment "The Science_Facets class contains the science-related search facets.  It is optional and may be repeated if an product has facets related to, for example, two different disciplines (as defined by the discipline_name facet). Note that Science_Facets was modeled with Discipline_Facets as a component and Discipline_Facets was modeled with Group_Facet1 and Group_Facet2 as components. This dependency hierarchy was flattened and only Science_Facets exists in the schema.".
 
pds4:urn:nasa:pds:0001_nasa_pds_1:all:user:cart:secondary_spatial_domain::1.0 rdf:type rdfs:Class;
  rdfs:label "Secondary_Spatial_Domain";
  pds4:subClassOf pds4:urn:nasa:pds:0001_nasa_pds_1:all:user::1.0;
  rdfs:comment "The Secondary_Spatial_Domain class describes an alternative longitude and latitude bounds to better support IAU approved or historically used geographic areal coordinates. This is only needed if the Spatial_Domain does not meet IAU recommendations or historical uses for the body. ".
 
pds4:urn:nasa:pds:0001_nasa_pds_1:pds:tndo_context:pds:service::1.0 rdf:type rdfs:Class;
  rdfs:label "Service";
  pds4:subClassOf pds4:urn:nasa:pds:0001_nasa_pds_1:pds:tagged_nondigital_object:pds:tndo_context::1.0;
  rdfs:comment "The Service class provides a description of a web service or tool.".
 
pds4:urn:nasa:pds:0001_nasa_pds_1:pds:parsable_byte_stream:pds:service_description::1.0 rdf:type rdfs:Class;
  rdfs:label "Service_Description";
  pds4:subClassOf pds4:urn:nasa:pds:0001_nasa_pds_1:pds:byte_stream:pds:parsable_byte_stream::1.0;
  rdfs:comment "The Service Description class defines a file that contains a standardized service specification.".
 
pds4:urn:nasa:pds:0001_nasa_pds_1:img:data_processing:img:shutter_subtraction::1.0 rdf:type rdfs:Class;
  rdfs:label "Shutter_Subtraction";
  pds4:subClassOf pds4:urn:nasa:pds:0001_nasa_pds_1:all:user:img:data_processing::1.0;
  rdfs:comment " The Shutter_Subtraction class specifies attributes describing the removal from the image of the shutter, or fixed-pattern.".
 
pds4:urn:nasa:pds:0001_nasa_pds_1:all:user:cart:sinusoidal::1.0 rdf:type rdfs:Class;
  rdfs:label "Sinusoidal";
  pds4:subClassOf pds4:urn:nasa:pds:0001_nasa_pds_1:all:user::1.0;
  rdfs:comment "The Sinusoidal class contains parameters for the Sinusoidal projection. Synder 1987, DOI:10.3133\\//pp1395, page 243: https:\\//\\//pubs.usgs.gov\\//pp\\//1395\\//report.pdf#page=255 PROJ: https:\\//\\//proj.org\\//operations\\//projections\\//sinu.html ".
 
pds4:urn:nasa:pds:0001_nasa_pds_1:pds:tndo_supplemental:pds:software::1.0 rdf:type rdfs:Class;
  rdfs:label "Software";
  pds4:subClassOf pds4:urn:nasa:pds:0001_nasa_pds_1:pds:tagged_nondigital_object:pds:tndo_supplemental::1.0;
  rdfs:comment "The Software class describes a software product".
 
pds4:urn:nasa:pds:0001_nasa_pds_1:all:user:proc:software::1.0 rdf:type rdfs:Class;
  rdfs:label "Software";
  pds4:subClassOf pds4:urn:nasa:pds:0001_nasa_pds_1:all:user::1.0;
  rdfs:comment "The Software class describes the data processing software used in order to produce the data product.".
 
pds4:urn:nasa:pds:0001_nasa_pds_1:pds:tndo_supplemental:pds:software_binary::1.0 rdf:type rdfs:Class;
  rdfs:label "Software_Binary";
  pds4:subClassOf pds4:urn:nasa:pds:0001_nasa_pds_1:pds:tagged_nondigital_object:pds:tndo_supplemental::1.0;
  rdfs:comment "The Software Binary class provides a description of a software code that is stored as a compiled binary file.".
 
pds4:urn:nasa:pds:0001_nasa_pds_1:all:user:proc:software_program::1.0 rdf:type rdfs:Class;
  rdfs:label "Software_Program";
  pds4:subClassOf pds4:urn:nasa:pds:0001_nasa_pds_1:all:user::1.0;
  rdfs:comment "The Software_Program class describes the specific components or tasks of the Software executed in producing the data product.".
 
pds4:urn:nasa:pds:0001_nasa_pds_1:all:user:proc:software_program_parameters::1.0 rdf:type rdfs:Class;
  rdfs:label "Software_Program_Parameters";
  pds4:subClassOf pds4:urn:nasa:pds:0001_nasa_pds_1:all:user::1.0;
  rdfs:comment "The Software_Program_Parameters class specifies the set of 1 or more parameters for the software program. These parameters can be input, output, or log information. The premise being a way to capture as much information as possible about the software program execution.".
 
pds4:urn:nasa:pds:0001_nasa_pds_1:pds:tndo_supplemental:pds:software_script::1.0 rdf:type rdfs:Class;
  rdfs:label "Software_Script";
  pds4:subClassOf pds4:urn:nasa:pds:0001_nasa_pds_1:pds:tagged_nondigital_object:pds:tndo_supplemental::1.0;
  rdfs:comment "The Software Script class provides a description of a software code that is stored as a script.".
 
pds4:urn:nasa:pds:0001_nasa_pds_1:pds:tndo_supplemental:pds:software_source::1.0 rdf:type rdfs:Class;
  rdfs:label "Software_Source";
  pds4:subClassOf pds4:urn:nasa:pds:0001_nasa_pds_1:pds:tagged_nondigital_object:pds:tndo_supplemental::1.0;
  rdfs:comment "The Software Source class provides a description of a software code that is stored as source code.".
 
pds4:urn:nasa:pds:0001_nasa_pds_1:pds:tagged_nondigital_child:pds:source_product_external::1.0 rdf:type rdfs:Class;
  rdfs:label "Source_Product_External";
  pds4:subClassOf pds4:urn:nasa:pds:0001_nasa_pds_1:all:user:pds:tagged_nondigital_child::1.0;
  rdfs:comment "The Source_Product_External class is used to reference one or more source products (a product containing input data for the creation of this product) outside the PDS4 Registry that have a common reference_type, doi, curating facility, and\\//or description. At least one of doi or curating facility must be provided. All source products listed within a single Source_Product_External class must correspond to the same doi and\\//or curating facility.".
 
pds4:urn:nasa:pds:0001_nasa_pds_1:pds:tagged_nondigital_child:pds:source_product_internal::1.0 rdf:type rdfs:Class;
  rdfs:label "Source_Product_Internal";
  pds4:subClassOf pds4:urn:nasa:pds:0001_nasa_pds_1:all:user:pds:tagged_nondigital_child::1.0;
  rdfs:comment "The Source_Product _Internal class is used to reference one or more source products in the PDS4 registry system. A source product contains input data for the creation of this product.".
 
pds4:urn:nasa:pds:0001_nasa_pds_1:all:user:cart:spatial_domain::1.0 rdf:type rdfs:Class;
  rdfs:label "Spatial_Domain";
  pds4:subClassOf pds4:urn:nasa:pds:0001_nasa_pds_1:all:user::1.0;
  rdfs:comment "The Spatial_Domain class describes the geographic areal domain of the data set. ".
 
pds4:urn:nasa:pds:0001_nasa_pds_1:img:data_processing:img:spatial_filter::1.0 rdf:type rdfs:Class;
  rdfs:label "Spatial_Filter";
  pds4:subClassOf pds4:urn:nasa:pds:0001_nasa_pds_1:all:user:img:data_processing::1.0;
  rdfs:comment "The Spatial_Filter class specifies what kind of spatial filtering has been done on the image. Spatial filtering looks at the geometry of pixels (e.g. XYZ or range values) rather than their intensity (cf. Image_Filter).".
 
pds4:urn:nasa:pds:0001_nasa_pds_1:all:user:cart:spatial_reference_information::1.0 rdf:type rdfs:Class;
  rdfs:label "Spatial_Reference_Information";
  pds4:subClassOf pds4:urn:nasa:pds:0001_nasa_pds_1:all:user::1.0;
  rdfs:comment "The Spatial_Reference_Information class provides a description of the reference frame for, and the means to encode, coordinates in a data set. ".
 
pds4:urn:nasa:pds:0001_nasa_pds_1:pds:tagged_digital_child:pds:special_constants::1.0 rdf:type rdfs:Class;
  rdfs:label "Special_Constants";
  pds4:subClassOf pds4:urn:nasa:pds:0001_nasa_pds_1:all:user:pds:tagged_digital_child::1.0;
  rdfs:comment "The Special Constants class provides a set of values used to indicate special cases that occur in the data.".
 
pds4:urn:nasa:pds:0001_nasa_pds_1:all:user:img:special_point::1.0 rdf:type rdfs:Class;
  rdfs:label "Special_Point";
  pds4:subClassOf pds4:urn:nasa:pds:0001_nasa_pds_1:all:user::1.0;
  rdfs:comment "Defines a special point on the image detector, such as the location in pixel space that a co-boresighted instrument measures.".
 
pds4:urn:nasa:pds:0001_nasa_pds_1:all:user:speclib:specimen_classification::1.0 rdf:type rdfs:Class;
  rdfs:label "Specimen_Classification";
  pds4:subClassOf pds4:urn:nasa:pds:0001_nasa_pds_1:all:user::1.0;
  rdfs:comment "The Specimen_Classification class provides information about how a specimen has been classified.".
 
pds4:urn:nasa:pds:0001_nasa_pds_1:all:user:speclib:specimen_parameters::1.0 rdf:type rdfs:Class;
  rdfs:label "Specimen_Parameters";
  pds4:subClassOf pds4:urn:nasa:pds:0001_nasa_pds_1:all:user::1.0;
  rdfs:comment "The Specimen_Parameters class provides information about a specimen for which measurements have been made.".
 
pds4:urn:nasa:pds:0001_nasa_pds_1:all:user:sp:spectral_characteristics::1.0 rdf:type rdfs:Class;
  rdfs:label "Spectral_Characteristics";
  pds4:subClassOf pds4:urn:nasa:pds:0001_nasa_pds_1:all:user::1.0;
  rdfs:comment " The Spectral_Characteristics class provides information about the spectral characteristics of a 1D, 2D, or 3D spectral data object. It is note used for tabulated spectra - tables in which each row ".
 
pds4:urn:nasa:pds:0001_nasa_pds_1:all:user:speclib:spectral_library_product::1.0 rdf:type rdfs:Class;
  rdfs:label "Spectral_Library_Product";
  pds4:subClassOf pds4:urn:nasa:pds:0001_nasa_pds_1:all:user::1.0;
  rdfs:comment "The Spectral_Library_Product class provides information about a data product in the Spectral Library.".
 
pds4:urn:nasa:pds:0001_nasa_pds_1:all:user:sp:spectral_lookup::1.0 rdf:type rdfs:Class;
  rdfs:label "Spectral_Lookup";
  pds4:subClassOf pds4:urn:nasa:pds:0001_nasa_pds_1:all:user::1.0;
  rdfs:comment " The Spectral_Lookup class references either specific Fields included in a spectral table (for 1D and tabulated spectra), or a 2-dimensional lookup map providing spectral characteristics for a corresponding spectral Array object. In the latter case, the referenced lookup map may either be to the referencing product, or an external stand-alone product. ".
 
pds4:urn:nasa:pds:0001_nasa_pds_1:all:user:cart:state_plane_coordinate_system::1.0 rdf:type rdfs:Class;
  rdfs:label "State_Plane_Coordinate_System";
  pds4:subClassOf pds4:urn:nasa:pds:0001_nasa_pds_1:all:user::1.0;
  rdfs:comment "The State_Plane_Coordinate_System class defines a plane-rectangular coordinate system established for each state in the United States by the National Geodetic Survey. Synder 1987, DOI:10.3133\\//pp1395, page 52: https:\\//\\//pubs.usgs.gov\\//pp\\//1395\\//report.pdf#page=64 ".
 
pds4:urn:nasa:pds:0001_nasa_pds_1:all:user:nucspec:state_table::1.0 rdf:type rdfs:Class;
  rdfs:label "State_Table";
  pds4:subClassOf pds4:urn:nasa:pds:0001_nasa_pds_1:all:user::1.0;
  rdfs:comment "Specifies an additional look-up table that provides additional information about specific observations within the product.".
 
pds4:urn:nasa:pds:0001_nasa_pds_1:all:user:nucspec:state_table_entry::1.0 rdf:type rdfs:Class;
  rdfs:label "State_Table_Entry";
  pds4:subClassOf pds4:urn:nasa:pds:0001_nasa_pds_1:all:user::1.0;
  rdfs:comment "Associates individual observations in the data product with a record in the state table, providing additonal information on those observations.".
 
pds4:urn:nasa:pds:0001_nasa_pds_1:all:user:nucspec:state_time::1.0 rdf:type rdfs:Class;
  rdfs:label "State_Time";
  pds4:subClassOf pds4:urn:nasa:pds:0001_nasa_pds_1:all:user::1.0;
  rdfs:comment "The time during which this state was applicable. The state table entry is applicable to records in the referenced data table if the time of the data record, as given by state_time_field_name, is between the start time and stop time given in State_Time.".
 
pds4:urn:nasa:pds:0001_nasa_pds_1:all:user:img_surface:stereo_product_parameters::1.0 rdf:type rdfs:Class;
  rdfs:label "Stereo_Product_Parameters";
  pds4:subClassOf pds4:urn:nasa:pds:0001_nasa_pds_1:all:user::1.0;
  rdfs:comment "The Stereo_Product_Parameters class describes the conditions under which stereo analysis was performed. This includes items such as the stereo baseline (separation between the cameras) and what partner image(s) were used for stereo analysis. If present, stereo partner images can be referenced using either an Internal_Reference or External_Reference.".
 
pds4:urn:nasa:pds:0001_nasa_pds_1:pds:parsable_byte_stream:pds:stream_text::1.0 rdf:type rdfs:Class;
  rdfs:label "Stream_Text";
  pds4:subClassOf pds4:urn:nasa:pds:0001_nasa_pds_1:pds:byte_stream:pds:parsable_byte_stream::1.0;
  rdfs:comment "The Stream text class defines a text object.".
 
pds4:urn:nasa:pds:0001_nasa_pds_1:all:user:img:subframe::1.0 rdf:type rdfs:Class;
  rdfs:label "Subframe";
  pds4:subClassOf pds4:urn:nasa:pds:0001_nasa_pds_1:all:user::1.0;
  rdfs:comment " The Subframe class describes the position and other optional characteristics of an image subframe, relative to the original image. ".
 
pds4:urn:nasa:pds:0001_nasa_pds_1:pds:information_package:pds:submission_information_package::1.0 rdf:type rdfs:Class;
  rdfs:label "Submission_Information_Package";
  pds4:subClassOf pds4:urn:nasa:pds:0001_nasa_pds_1:pds:tndo_supplemental:pds:information_package::1.0;
  rdfs:comment "The Submission Information Package (SIP) class is an Information Package that is delivered by a Data Provider to an archive that conforms to the Open Archive Information System (OAIS) Reference Model for use in the construction of one or more AIPs.".
 
pds4:urn:nasa:pds:0001_nasa_pds_1:pds:tndo_context_pds3:pds:subscriber_pds3::1.0 rdf:type rdfs:Class;
  rdfs:label "Subscriber_PDS3";
  pds4:subClassOf pds4:urn:nasa:pds:0001_nasa_pds_1:pds:tagged_nondigital_object:pds:tndo_context_pds3::1.0;
  rdfs:comment "The Subscriber PDS3 class provides the name of the subscriber and their subscription list.".
 
pds4:urn:nasa:pds:0001_nasa_pds_1:all:user:geom:surface_geometry::1.0 rdf:type rdfs:Class;
  rdfs:label "Surface_Geometry";
  pds4:subClassOf pds4:urn:nasa:pds:0001_nasa_pds_1:all:user::1.0;
  rdfs:comment "The Surface_Geometry class is a container for surface geometry classes. ".
 
pds4:urn:nasa:pds:0001_nasa_pds_1:all:user:geom:surface_geometry_min_max::1.0 rdf:type rdfs:Class;
  rdfs:label "Surface_Geometry_Min_Max";
  pds4:subClassOf pds4:urn:nasa:pds:0001_nasa_pds_1:all:user::1.0;
  rdfs:comment "The Surface_Geometry_Min_Max class contains attributes providing surface geometry parameters as minimum\\//maximum pairs. For any given parameter if one of minimum or maximum is given, both must be given. The min-max pairs for each parameter provide the range of that parameter in the observation for the target specified using the Geometry_Target_Identification class in the Orbiter_Identification class under the parent Geometry_Orbiter class. ".
 
pds4:urn:nasa:pds:0001_nasa_pds_1:all:user:geom:surface_geometry_specific::1.0 rdf:type rdfs:Class;
  rdfs:label "Surface_Geometry_Specific";
  pds4:subClassOf pds4:urn:nasa:pds:0001_nasa_pds_1:all:user::1.0;
  rdfs:comment "The Surface_Geometry_Specific class contains classes and attributes for various points on the surface of the target designated in the enclosing Geometry_Orbiter. ".
 
pds4:urn:nasa:pds:0001_nasa_pds_1:all:user:geom:surface_geometry_start_stop::1.0 rdf:type rdfs:Class;
  rdfs:label "Surface_Geometry_Start_Stop";
  pds4:subClassOf pds4:urn:nasa:pds:0001_nasa_pds_1:all:user::1.0;
  rdfs:comment "The Surface_Geometry_Start_Stop class contains attributes providing surface geometry parameters given as pairs corresponding to the beginning and end of the observation. For a parameter, if either the start or stop parameter is given, both must be provided. If any values from this class are included in the label, the parameters geometry_start_time_utc and geometry_stop_time_utc must be given in the enclosing Geometry_Orbiter class. ".
 
pds4:urn:nasa:pds:0001_nasa_pds_1:all:user:img_surface:surface_imaging::1.0 rdf:type rdfs:Class;
  rdfs:label "Surface_Imaging";
  pds4:subClassOf pds4:urn:nasa:pds:0001_nasa_pds_1:all:user::1.0;
  rdfs:comment "Attributes specific to imaging instruments on surface missions.".
 
pds4:urn:nasa:pds:0001_nasa_pds_1:all:user:msn:surface_mission::1.0 rdf:type rdfs:Class;
  rdfs:label "Surface_Mission";
  pds4:subClassOf pds4:urn:nasa:pds:0001_nasa_pds_1:all:user::1.0;
  rdfs:comment "The Surface_Mission class provides information about a surface mission.".
 
pds4:urn:nasa:pds:0001_nasa_pds_1:all:user:msn_surface:surface_mission_information::1.0 rdf:type rdfs:Class;
  rdfs:label "Surface_Mission_Information";
  pds4:subClassOf pds4:urn:nasa:pds:0001_nasa_pds_1:all:user::1.0;
  rdfs:comment "The Surface_Mission_Information class contains attributes specific to surface missions which apply across instrument types.".
 
pds4:urn:nasa:pds:0001_nasa_pds_1:all:user:cart:surface_model_parameters::1.0 rdf:type rdfs:Class;
  rdfs:label "Surface_Model_Parameters";
  pds4:subClassOf pds4:urn:nasa:pds:0001_nasa_pds_1:all:user::1.0;
  rdfs:comment "This class describes the surface model used by the projection. For in-situ mosaics, the surface model describes the surface upon which input images are projected in order to create a unified point of view in a mosaic. To the extent the surface model does not match the actual surface, parallax errors typically occur at seams between images.".
 
pds4:urn:nasa:pds:0001_nasa_pds_1:all:user:cart:surface_model_planar::1.0 rdf:type rdfs:Class;
  rdfs:label "Surface_Model_Planar";
  pds4:subClassOf pds4:urn:nasa:pds:0001_nasa_pds_1:all:user::1.0;
  rdfs:comment "This is a specific type of surface model that treats the surface as a flat plane, with a specified orientation (Vector_Surface_Normal) and location (Vector_Surface_Ground_Location). ".
 
pds4:urn:nasa:pds:0001_nasa_pds_1:all:user:cart:surface_model_spherical::1.0 rdf:type rdfs:Class;
  rdfs:label "Surface_Model_Spherical";
  pds4:subClassOf pds4:urn:nasa:pds:0001_nasa_pds_1:all:user::1.0;
  rdfs:comment "This is a specific type of surface model that treats the surface as a sphere, with a specified center and radius.".
 
pds4:urn:nasa:pds:0001_nasa_pds_1:all:user:survey:survey::1.0 rdf:type rdfs:Class;
  rdfs:label "Survey";
  pds4:subClassOf pds4:urn:nasa:pds:0001_nasa_pds_1:all:user::1.0;
  rdfs:comment "Sky Survey related properties.".
 
pds4:urn:nasa:pds:0001_nasa_pds_1:pds:byte_stream:pds:table_base::1.0 rdf:type rdfs:Class;
  rdfs:label "Table_Base";
  pds4:subClassOf pds4:urn:nasa:pds:0001_nasa_pds_1:pds:tagged_digital_object:pds:byte_stream::1.0;
  rdfs:comment "The Table Base class defines a heterogeneous repeating record of scalars. The Table Base class is the parent class for all heterogeneous repeating record of scalars.".
 
pds4:urn:nasa:pds:0001_nasa_pds_1:pds:table_base:pds:table_binary::1.0 rdf:type rdfs:Class;
  rdfs:label "Table_Binary";
  pds4:subClassOf pds4:urn:nasa:pds:0001_nasa_pds_1:pds:byte_stream:pds:table_base::1.0;
  rdfs:comment "The Table Binary class is an extension of table base and defines a simple binary table.".
 
pds4:urn:nasa:pds:0001_nasa_pds_1:pds:table_base:pds:table_character::1.0 rdf:type rdfs:Class;
  rdfs:label "Table_Character";
  pds4:subClassOf pds4:urn:nasa:pds:0001_nasa_pds_1:pds:byte_stream:pds:table_base::1.0;
  rdfs:comment "The Table Character class is an extension of table base and defines a simple character table.".
 
pds4:urn:nasa:pds:0001_nasa_pds_1:pds:parsable_byte_stream:pds:table_delimited::1.0 rdf:type rdfs:Class;
  rdfs:label "Table_Delimited";
  pds4:subClassOf pds4:urn:nasa:pds:0001_nasa_pds_1:pds:byte_stream:pds:parsable_byte_stream::1.0;
  rdfs:comment "The Table_Delimited class defines a simple table (spreadsheet) with delimited fields and records.".
 
pds4:urn:nasa:pds:0001_nasa_pds_1:pds:table_delimited:pds:table_delimited_source_product_external::1.0 rdf:type rdfs:Class;
  rdfs:label "Table_Delimited_Source_Product_External";
  pds4:subClassOf pds4:urn:nasa:pds:0001_nasa_pds_1:pds:parsable_byte_stream:pds:table_delimited::1.0;
  rdfs:comment "The Table_Delimited_Source_Product_External class defines a table that references many source products (products containing input data for the creation of this product) outside the PDS4 Registry that have a common reference_type, doi, curating facility, and\\//or description. At least one of doi or curating facility must be provided for each source product.".
 
pds4:urn:nasa:pds:0001_nasa_pds_1:pds:table_delimited:pds:table_delimited_source_product_internal::1.0 rdf:type rdfs:Class;
  rdfs:label "Table_Delimited_Source_Product_Internal";
  pds4:subClassOf pds4:urn:nasa:pds:0001_nasa_pds_1:pds:parsable_byte_stream:pds:table_delimited::1.0;
  rdfs:comment "The Table_Delimited_Source_Product_Internal class defines a table that references many source products (products containing input data for the creation of this product) in the PDS4 registry system. A source product contains input data for the creation of this product.".
 
pds4:urn:nasa:pds:0001_nasa_pds_1:pds:tndo_context:pds:target::1.0 rdf:type rdfs:Class;
  rdfs:label "Target";
  pds4:subClassOf pds4:urn:nasa:pds:0001_nasa_pds_1:pds:tagged_nondigital_object:pds:tndo_context::1.0;
  rdfs:comment "The Target class provides a description of a physical object that is the object of data collection.".
 
pds4:urn:nasa:pds:0001_nasa_pds_1:pds:tndo_context:pds:target:asteroid::1.0 rdf:type rdfs:Class;
  rdfs:label "Asteroid";
  rdfs:subClassOf pds4:urn:nasa:pds:0001_nasa_pds_1:pds:tndo_context:pds:target::1.0;
  rdfs:comment "The target is classified as an asteroid".
 
pds4:urn:nasa:pds:0001_nasa_pds_1:pds:tndo_context:pds:target:astrophysical::1.0 rdf:type rdfs:Class;
  rdfs:label "Astrophysical";
  rdfs:subClassOf pds4:urn:nasa:pds:0001_nasa_pds_1:pds:tndo_context:pds:target::1.0;
  rdfs:comment "The target is classified as of interest to the astrophysics community.".
 
pds4:urn:nasa:pds:0001_nasa_pds_1:pds:tndo_context:pds:target:calibration::1.0 rdf:type rdfs:Class;
  rdfs:label "Calibration";
  rdfs:subClassOf pds4:urn:nasa:pds:0001_nasa_pds_1:pds:tndo_context:pds:target::1.0;
  rdfs:comment "The Target is classified as calibration".
 
pds4:urn:nasa:pds:0001_nasa_pds_1:pds:tndo_context:pds:target:calibration_field::1.0 rdf:type rdfs:Class;
  rdfs:label "Calibration Field";
  rdfs:subClassOf pds4:urn:nasa:pds:0001_nasa_pds_1:pds:tndo_context:pds:target::1.0;
  rdfs:comment "This type indicates a star field observed to be used for calibration purposes. Typically, this will correspond to a field defined in a published work like the Landolt photometric catalog.".
 
pds4:urn:nasa:pds:0001_nasa_pds_1:pds:tndo_context:pds:target:calibrator::1.0 rdf:type rdfs:Class;
  rdfs:label "Calibrator";
  rdfs:subClassOf pds4:urn:nasa:pds:0001_nasa_pds_1:pds:tndo_context:pds:target::1.0;
  rdfs:comment "This type indicates a piece of equipment specifically designed to generate a signal to be used for calibration.".
 
pds4:urn:nasa:pds:0001_nasa_pds_1:pds:tndo_context:pds:target:centaur::1.0 rdf:type rdfs:Class;
  rdfs:label "Centaur";
  rdfs:subClassOf pds4:urn:nasa:pds:0001_nasa_pds_1:pds:tndo_context:pds:target::1.0;
  rdfs:comment "The target is classified as a Centaur. A Centaur is a minor planet orbiting beyond the orbit of Jupiter and interior to the orbit of Neptune. Its semimajor axis range is greater than 5.4 AU and less than 30.1 AU.".
 
pds4:urn:nasa:pds:0001_nasa_pds_1:pds:tndo_context:pds:target:comet::1.0 rdf:type rdfs:Class;
  rdfs:label "Comet";
  rdfs:subClassOf pds4:urn:nasa:pds:0001_nasa_pds_1:pds:tndo_context:pds:target::1.0;
  rdfs:comment "The target is classified as a comet".
 
pds4:urn:nasa:pds:0001_nasa_pds_1:pds:tndo_context:pds:target:dust::1.0 rdf:type rdfs:Class;
  rdfs:label "Dust";
  rdfs:subClassOf pds4:urn:nasa:pds:0001_nasa_pds_1:pds:tndo_context:pds:target::1.0;
  rdfs:comment "The target is classified as dust".
 
pds4:urn:nasa:pds:0001_nasa_pds_1:pds:tndo_context:pds:target:dwarf_planet::1.0 rdf:type rdfs:Class;
  rdfs:label "Dwarf Planet";
  rdfs:subClassOf pds4:urn:nasa:pds:0001_nasa_pds_1:pds:tndo_context:pds:target::1.0;
  rdfs:comment "The target is classified as a dwarf planet".
 
pds4:urn:nasa:pds:0001_nasa_pds_1:pds:tndo_context:pds:target:equipment::1.0 rdf:type rdfs:Class;
  rdfs:label "Equipment";
  rdfs:subClassOf pds4:urn:nasa:pds:0001_nasa_pds_1:pds:tndo_context:pds:target::1.0;
  rdfs:comment "Target is classified as a part of the host spacecraft or another (human) artifact".
 
pds4:urn:nasa:pds:0001_nasa_pds_1:pds:tndo_context:pds:target:exoplanet_system::1.0 rdf:type rdfs:Class;
  rdfs:label "Exoplanet System";
  rdfs:subClassOf pds4:urn:nasa:pds:0001_nasa_pds_1:pds:tndo_context:pds:target::1.0;
  rdfs:comment "This type indicates a target that is a star or stellar system (binary, trinary, etc.) with a known or suspected planetary system around it.".
 
pds4:urn:nasa:pds:0001_nasa_pds_1:pds:tndo_context:pds:target:galaxy::1.0 rdf:type rdfs:Class;
  rdfs:label "Galaxy";
  rdfs:subClassOf pds4:urn:nasa:pds:0001_nasa_pds_1:pds:tndo_context:pds:target::1.0;
  rdfs:comment "The target is classified as a galaxy".
 
pds4:urn:nasa:pds:0001_nasa_pds_1:pds:tndo_context:pds:target:globular_cluster::1.0 rdf:type rdfs:Class;
  rdfs:label "Globular Cluster";
  rdfs:subClassOf pds4:urn:nasa:pds:0001_nasa_pds_1:pds:tndo_context:pds:target::1.0;
  rdfs:comment "The target is classified as a globular cluster".
 
pds4:urn:nasa:pds:0001_nasa_pds_1:pds:tndo_context:pds:target:laboratory_analog::1.0 rdf:type rdfs:Class;
  rdfs:label "Laboratory Analog";
  rdfs:subClassOf pds4:urn:nasa:pds:0001_nasa_pds_1:pds:tndo_context:pds:target::1.0;
  rdfs:comment "The target is classified as a laboratory analog approximating a planetary environment.".
 
pds4:urn:nasa:pds:0001_nasa_pds_1:pds:tndo_context:pds:target:lunar_sample::1.0 rdf:type rdfs:Class;
  rdfs:label "Lunar Sample";
  rdfs:subClassOf pds4:urn:nasa:pds:0001_nasa_pds_1:pds:tndo_context:pds:target::1.0;
  rdfs:comment "The target is a sample collected on the Earth\\'s Moon".
 
pds4:urn:nasa:pds:0001_nasa_pds_1:pds:tndo_context:pds:target:magnetic_field::1.0 rdf:type rdfs:Class;
  rdfs:label "Magnetic Field";
  rdfs:subClassOf pds4:urn:nasa:pds:0001_nasa_pds_1:pds:tndo_context:pds:target::1.0;
  rdfs:comment "The target is classified as a magnetic field.".
 
pds4:urn:nasa:pds:0001_nasa_pds_1:pds:tndo_context:pds:target:meteorite::1.0 rdf:type rdfs:Class;
  rdfs:label "Meteorite";
  rdfs:subClassOf pds4:urn:nasa:pds:0001_nasa_pds_1:pds:tndo_context:pds:target::1.0;
  rdfs:comment "The target is classified as a meteorite".
 
pds4:urn:nasa:pds:0001_nasa_pds_1:pds:tndo_context:pds:target:meteoroid::1.0 rdf:type rdfs:Class;
  rdfs:label "Meteoroid";
  rdfs:subClassOf pds4:urn:nasa:pds:0001_nasa_pds_1:pds:tndo_context:pds:target::1.0;
  rdfs:comment "The target is classified as a meteoroid".
 
pds4:urn:nasa:pds:0001_nasa_pds_1:pds:tndo_context:pds:target:meteoroid_stream::1.0 rdf:type rdfs:Class;
  rdfs:label "Meteoroid Stream";
  rdfs:subClassOf pds4:urn:nasa:pds:0001_nasa_pds_1:pds:tndo_context:pds:target::1.0;
  rdfs:comment "The target is classified as a meteoroid stream".
 
pds4:urn:nasa:pds:0001_nasa_pds_1:pds:tndo_context:pds:target:nebula::1.0 rdf:type rdfs:Class;
  rdfs:label "Nebula";
  rdfs:subClassOf pds4:urn:nasa:pds:0001_nasa_pds_1:pds:tndo_context:pds:target::1.0;
  rdfs:comment "The target is classified as a nebula".
 
pds4:urn:nasa:pds:0001_nasa_pds_1:pds:tndo_context:pds:target:open_cluster::1.0 rdf:type rdfs:Class;
  rdfs:label "Open Cluster";
  rdfs:subClassOf pds4:urn:nasa:pds:0001_nasa_pds_1:pds:tndo_context:pds:target::1.0;
  rdfs:comment "The target is classified as an open cluster".
 
pds4:urn:nasa:pds:0001_nasa_pds_1:pds:tndo_context:pds:target:planet::1.0 rdf:type rdfs:Class;
  rdfs:label "Planet";
  rdfs:subClassOf pds4:urn:nasa:pds:0001_nasa_pds_1:pds:tndo_context:pds:target::1.0;
  rdfs:comment "The target is classified as a planet".
 
pds4:urn:nasa:pds:0001_nasa_pds_1:pds:tndo_context:pds:target:planetary_nebula::1.0 rdf:type rdfs:Class;
  rdfs:label "Planetary Nebula";
  rdfs:subClassOf pds4:urn:nasa:pds:0001_nasa_pds_1:pds:tndo_context:pds:target::1.0;
  rdfs:comment "The target is classified as a planetary nebula".
 
pds4:urn:nasa:pds:0001_nasa_pds_1:pds:tndo_context:pds:target:planetary_system::1.0 rdf:type rdfs:Class;
  rdfs:label "Planetary System";
  rdfs:subClassOf pds4:urn:nasa:pds:0001_nasa_pds_1:pds:tndo_context:pds:target::1.0;
  rdfs:comment "This type indicates a target consisting of a primary body and its satellite(s), ring(s), or similarly associated objects.  For example: Saturn and its rings, Jupiter and its moons, etc.".
 
pds4:urn:nasa:pds:0001_nasa_pds_1:pds:tndo_context:pds:target:plasma_cloud::1.0 rdf:type rdfs:Class;
  rdfs:label "Plasma Cloud";
  rdfs:subClassOf pds4:urn:nasa:pds:0001_nasa_pds_1:pds:tndo_context:pds:target::1.0;
  rdfs:comment "The target is classified as a plasma cloud".
 
pds4:urn:nasa:pds:0001_nasa_pds_1:pds:tndo_context:pds:target:plasma_stream::1.0 rdf:type rdfs:Class;
  rdfs:label "Plasma Stream";
  rdfs:subClassOf pds4:urn:nasa:pds:0001_nasa_pds_1:pds:tndo_context:pds:target::1.0;
  rdfs:comment "Target is classified as a plasma stream.".
 
pds4:urn:nasa:pds:0001_nasa_pds_1:pds:tndo_context:pds:target:ring::1.0 rdf:type rdfs:Class;
  rdfs:label "Ring";
  rdfs:subClassOf pds4:urn:nasa:pds:0001_nasa_pds_1:pds:tndo_context:pds:target::1.0;
  rdfs:comment "The target is classified as a ring".
 
pds4:urn:nasa:pds:0001_nasa_pds_1:pds:tndo_context:pds:target:sample::1.0 rdf:type rdfs:Class;
  rdfs:label "Sample";
  rdfs:subClassOf pds4:urn:nasa:pds:0001_nasa_pds_1:pds:tndo_context:pds:target::1.0;
  rdfs:comment "The target is classified as a physical sample representative of a larger whole. Samples may include but are not confined to rocks, minerals, fluids, or synthetic approximations of those types of materials.".
 
pds4:urn:nasa:pds:0001_nasa_pds_1:pds:tndo_context:pds:target:satellite::1.0 rdf:type rdfs:Class;
  rdfs:label "Satellite";
  rdfs:subClassOf pds4:urn:nasa:pds:0001_nasa_pds_1:pds:tndo_context:pds:target::1.0;
  rdfs:comment "The target is classified as a satellite".
 
pds4:urn:nasa:pds:0001_nasa_pds_1:pds:tndo_context:pds:target:star::1.0 rdf:type rdfs:Class;
  rdfs:label "Star";
  rdfs:subClassOf pds4:urn:nasa:pds:0001_nasa_pds_1:pds:tndo_context:pds:target::1.0;
  rdfs:comment "The target is classified as a star".
 
pds4:urn:nasa:pds:0001_nasa_pds_1:pds:tndo_context:pds:target:star_cluster::1.0 rdf:type rdfs:Class;
  rdfs:label "Star Cluster";
  rdfs:subClassOf pds4:urn:nasa:pds:0001_nasa_pds_1:pds:tndo_context:pds:target::1.0;
  rdfs:comment "The target is classified as a star cluster".
 
pds4:urn:nasa:pds:0001_nasa_pds_1:pds:tndo_context:pds:target:synthetic_sample::1.0 rdf:type rdfs:Class;
  rdfs:label "Synthetic Sample";
  rdfs:subClassOf pds4:urn:nasa:pds:0001_nasa_pds_1:pds:tndo_context:pds:target::1.0;
  rdfs:comment "The target is a sample created in a laboratory.".
 
pds4:urn:nasa:pds:0001_nasa_pds_1:pds:tndo_context:pds:target:terrestrial_sample::1.0 rdf:type rdfs:Class;
  rdfs:label "Terrestrial Sample";
  rdfs:subClassOf pds4:urn:nasa:pds:0001_nasa_pds_1:pds:tndo_context:pds:target::1.0;
  rdfs:comment "The target is classified as a terrestrial sample".
 
pds4:urn:nasa:pds:0001_nasa_pds_1:pds:tndo_context:pds:target:trans-neptunian_object::1.0 rdf:type rdfs:Class;
  rdfs:label "Trans-Neptunian Object";
  rdfs:subClassOf pds4:urn:nasa:pds:0001_nasa_pds_1:pds:tndo_context:pds:target::1.0;
  rdfs:comment "The target is classified as a trans-Neptunian object".
 
pds4:urn:nasa:pds:0001_nasa_pds_1:pds:product_components:pds:target_identification::1.0 rdf:type rdfs:Class;
  rdfs:label "Target_Identification";
  pds4:subClassOf pds4:urn:nasa:pds:0001_nasa_pds_1:all:user:pds:product_components::1.0;
  rdfs:comment "The Target_Identification class provides detailed target identification information.".
 
pds4:urn:nasa:pds:0001_nasa_pds_1:pds:product_components:pds:target_identification:asteroid::1.0 rdf:type rdfs:Class;
  rdfs:label "Asteroid";
  rdfs:subClassOf pds4:urn:nasa:pds:0001_nasa_pds_1:pds:product_components:pds:target_identification::1.0;
  rdfs:comment "The target is classified as an asteroid".
 
pds4:urn:nasa:pds:0001_nasa_pds_1:pds:product_components:pds:target_identification:astrophysical::1.0 rdf:type rdfs:Class;
  rdfs:label "Astrophysical";
  rdfs:subClassOf pds4:urn:nasa:pds:0001_nasa_pds_1:pds:product_components:pds:target_identification::1.0;
  rdfs:comment "The target is classified as of interest to the astrophysics community.".
 
pds4:urn:nasa:pds:0001_nasa_pds_1:pds:product_components:pds:target_identification:calibration::1.0 rdf:type rdfs:Class;
  rdfs:label "Calibration";
  rdfs:subClassOf pds4:urn:nasa:pds:0001_nasa_pds_1:pds:product_components:pds:target_identification::1.0;
  rdfs:comment "The Target is classified as calibration".
 
pds4:urn:nasa:pds:0001_nasa_pds_1:pds:product_components:pds:target_identification:calibration_field::1.0 rdf:type rdfs:Class;
  rdfs:label "Calibration Field";
  rdfs:subClassOf pds4:urn:nasa:pds:0001_nasa_pds_1:pds:product_components:pds:target_identification::1.0;
  rdfs:comment "This type indicates a star field observed to be used for calibration purposes. Typically, this will correspond to a field defined in a published work like the Landolt photometric catalog.".
 
pds4:urn:nasa:pds:0001_nasa_pds_1:pds:product_components:pds:target_identification:calibrator::1.0 rdf:type rdfs:Class;
  rdfs:label "Calibrator";
  rdfs:subClassOf pds4:urn:nasa:pds:0001_nasa_pds_1:pds:product_components:pds:target_identification::1.0;
  rdfs:comment "This type indicates a piece of equipment specifically designed to generate a signal to be used for calibration.".
 
pds4:urn:nasa:pds:0001_nasa_pds_1:pds:product_components:pds:target_identification:centaur::1.0 rdf:type rdfs:Class;
  rdfs:label "Centaur";
  rdfs:subClassOf pds4:urn:nasa:pds:0001_nasa_pds_1:pds:product_components:pds:target_identification::1.0;
  rdfs:comment "The target is classified as a Centaur. A Centaur is a minor planet orbiting beyond the orbit of Jupiter and interior to the orbit of Neptune. Its semimajor axis range is greater than 5.4 AU and less than 30.1 AU.".
 
pds4:urn:nasa:pds:0001_nasa_pds_1:pds:product_components:pds:target_identification:comet::1.0 rdf:type rdfs:Class;
  rdfs:label "Comet";
  rdfs:subClassOf pds4:urn:nasa:pds:0001_nasa_pds_1:pds:product_components:pds:target_identification::1.0;
  rdfs:comment "The target is classified as a comet".
 
pds4:urn:nasa:pds:0001_nasa_pds_1:pds:product_components:pds:target_identification:dust::1.0 rdf:type rdfs:Class;
  rdfs:label "Dust";
  rdfs:subClassOf pds4:urn:nasa:pds:0001_nasa_pds_1:pds:product_components:pds:target_identification::1.0;
  rdfs:comment "The target is classified as dust".
 
pds4:urn:nasa:pds:0001_nasa_pds_1:pds:product_components:pds:target_identification:dwarf_planet::1.0 rdf:type rdfs:Class;
  rdfs:label "Dwarf Planet";
  rdfs:subClassOf pds4:urn:nasa:pds:0001_nasa_pds_1:pds:product_components:pds:target_identification::1.0;
  rdfs:comment "The target is classified as a dwarf planet".
 
pds4:urn:nasa:pds:0001_nasa_pds_1:pds:product_components:pds:target_identification:equipment::1.0 rdf:type rdfs:Class;
  rdfs:label "Equipment";
  rdfs:subClassOf pds4:urn:nasa:pds:0001_nasa_pds_1:pds:product_components:pds:target_identification::1.0;
  rdfs:comment "Target is classified as a part of the host spacecraft or another (human) artifact".
 
pds4:urn:nasa:pds:0001_nasa_pds_1:pds:product_components:pds:target_identification:exoplanet_system::1.0 rdf:type rdfs:Class;
  rdfs:label "Exoplanet System";
  rdfs:subClassOf pds4:urn:nasa:pds:0001_nasa_pds_1:pds:product_components:pds:target_identification::1.0;
  rdfs:comment "This type indicates a target that is a star or stellar system (binary, trinary, etc.) with a known or suspected planetary system around it.".
 
pds4:urn:nasa:pds:0001_nasa_pds_1:pds:product_components:pds:target_identification:galaxy::1.0 rdf:type rdfs:Class;
  rdfs:label "Galaxy";
  rdfs:subClassOf pds4:urn:nasa:pds:0001_nasa_pds_1:pds:product_components:pds:target_identification::1.0;
  rdfs:comment "The target is classified as a galaxy".
 
pds4:urn:nasa:pds:0001_nasa_pds_1:pds:product_components:pds:target_identification:globular_cluster::1.0 rdf:type rdfs:Class;
  rdfs:label "Globular Cluster";
  rdfs:subClassOf pds4:urn:nasa:pds:0001_nasa_pds_1:pds:product_components:pds:target_identification::1.0;
  rdfs:comment "The target is classified as a globular cluster".
 
pds4:urn:nasa:pds:0001_nasa_pds_1:pds:product_components:pds:target_identification:laboratory_analog::1.0 rdf:type rdfs:Class;
  rdfs:label "Laboratory Analog";
  rdfs:subClassOf pds4:urn:nasa:pds:0001_nasa_pds_1:pds:product_components:pds:target_identification::1.0;
  rdfs:comment "The target is classified as a laboratory analog approximating a planetary environment.".
 
pds4:urn:nasa:pds:0001_nasa_pds_1:pds:product_components:pds:target_identification:lunar_sample::1.0 rdf:type rdfs:Class;
  rdfs:label "Lunar Sample";
  rdfs:subClassOf pds4:urn:nasa:pds:0001_nasa_pds_1:pds:product_components:pds:target_identification::1.0;
  rdfs:comment "The target is a sample collected on the Earth\\'s Moon".
 
pds4:urn:nasa:pds:0001_nasa_pds_1:pds:product_components:pds:target_identification:magnetic_field::1.0 rdf:type rdfs:Class;
  rdfs:label "Magnetic Field";
  rdfs:subClassOf pds4:urn:nasa:pds:0001_nasa_pds_1:pds:product_components:pds:target_identification::1.0;
  rdfs:comment "The target is classified as a magnetic field.".
 
pds4:urn:nasa:pds:0001_nasa_pds_1:pds:product_components:pds:target_identification:meteorite::1.0 rdf:type rdfs:Class;
  rdfs:label "Meteorite";
  rdfs:subClassOf pds4:urn:nasa:pds:0001_nasa_pds_1:pds:product_components:pds:target_identification::1.0;
  rdfs:comment "The target is classified as a meteorite".
 
pds4:urn:nasa:pds:0001_nasa_pds_1:pds:product_components:pds:target_identification:meteoroid::1.0 rdf:type rdfs:Class;
  rdfs:label "Meteoroid";
  rdfs:subClassOf pds4:urn:nasa:pds:0001_nasa_pds_1:pds:product_components:pds:target_identification::1.0;
  rdfs:comment "The target is classified as a meteoroid".
 
pds4:urn:nasa:pds:0001_nasa_pds_1:pds:product_components:pds:target_identification:meteoroid_stream::1.0 rdf:type rdfs:Class;
  rdfs:label "Meteoroid Stream";
  rdfs:subClassOf pds4:urn:nasa:pds:0001_nasa_pds_1:pds:product_components:pds:target_identification::1.0;
  rdfs:comment "The target is classified as a meteoroid stream".
 
pds4:urn:nasa:pds:0001_nasa_pds_1:pds:product_components:pds:target_identification:nebula::1.0 rdf:type rdfs:Class;
  rdfs:label "Nebula";
  rdfs:subClassOf pds4:urn:nasa:pds:0001_nasa_pds_1:pds:product_components:pds:target_identification::1.0;
  rdfs:comment "The target is classified as a nebula".
 
pds4:urn:nasa:pds:0001_nasa_pds_1:pds:product_components:pds:target_identification:open_cluster::1.0 rdf:type rdfs:Class;
  rdfs:label "Open Cluster";
  rdfs:subClassOf pds4:urn:nasa:pds:0001_nasa_pds_1:pds:product_components:pds:target_identification::1.0;
  rdfs:comment "The target is classified as an open cluster".
 
pds4:urn:nasa:pds:0001_nasa_pds_1:pds:product_components:pds:target_identification:planet::1.0 rdf:type rdfs:Class;
  rdfs:label "Planet";
  rdfs:subClassOf pds4:urn:nasa:pds:0001_nasa_pds_1:pds:product_components:pds:target_identification::1.0;
  rdfs:comment "The target is classified as a planet".
 
pds4:urn:nasa:pds:0001_nasa_pds_1:pds:product_components:pds:target_identification:planetary_nebula::1.0 rdf:type rdfs:Class;
  rdfs:label "Planetary Nebula";
  rdfs:subClassOf pds4:urn:nasa:pds:0001_nasa_pds_1:pds:product_components:pds:target_identification::1.0;
  rdfs:comment "The target is classified as a planetary nebula".
 
pds4:urn:nasa:pds:0001_nasa_pds_1:pds:product_components:pds:target_identification:planetary_system::1.0 rdf:type rdfs:Class;
  rdfs:label "Planetary System";
  rdfs:subClassOf pds4:urn:nasa:pds:0001_nasa_pds_1:pds:product_components:pds:target_identification::1.0;
  rdfs:comment "This type indicates a target consisting of a primary body and its satellite(s), ring(s), or similarly associated objects.  For example: Saturn and its rings, Jupiter and its moons, etc.".
 
pds4:urn:nasa:pds:0001_nasa_pds_1:pds:product_components:pds:target_identification:plasma_cloud::1.0 rdf:type rdfs:Class;
  rdfs:label "Plasma Cloud";
  rdfs:subClassOf pds4:urn:nasa:pds:0001_nasa_pds_1:pds:product_components:pds:target_identification::1.0;
  rdfs:comment "The target is classified as a plasma cloud".
 
pds4:urn:nasa:pds:0001_nasa_pds_1:pds:product_components:pds:target_identification:plasma_stream::1.0 rdf:type rdfs:Class;
  rdfs:label "Plasma Stream";
  rdfs:subClassOf pds4:urn:nasa:pds:0001_nasa_pds_1:pds:product_components:pds:target_identification::1.0;
  rdfs:comment "Target is classified as a plasma stream.".
 
pds4:urn:nasa:pds:0001_nasa_pds_1:pds:product_components:pds:target_identification:ring::1.0 rdf:type rdfs:Class;
  rdfs:label "Ring";
  rdfs:subClassOf pds4:urn:nasa:pds:0001_nasa_pds_1:pds:product_components:pds:target_identification::1.0;
  rdfs:comment "The target is classified as a ring".
 
pds4:urn:nasa:pds:0001_nasa_pds_1:pds:product_components:pds:target_identification:sample::1.0 rdf:type rdfs:Class;
  rdfs:label "Sample";
  rdfs:subClassOf pds4:urn:nasa:pds:0001_nasa_pds_1:pds:product_components:pds:target_identification::1.0;
  rdfs:comment "The target is classified as a physical sample representative of a larger whole. Samples may include but are not confined to rocks, minerals, fluids, or synthetic approximations of those types of materials.".
 
pds4:urn:nasa:pds:0001_nasa_pds_1:pds:product_components:pds:target_identification:satellite::1.0 rdf:type rdfs:Class;
  rdfs:label "Satellite";
  rdfs:subClassOf pds4:urn:nasa:pds:0001_nasa_pds_1:pds:product_components:pds:target_identification::1.0;
  rdfs:comment "The target is classified as a satellite".
 
pds4:urn:nasa:pds:0001_nasa_pds_1:pds:product_components:pds:target_identification:star::1.0 rdf:type rdfs:Class;
  rdfs:label "Star";
  rdfs:subClassOf pds4:urn:nasa:pds:0001_nasa_pds_1:pds:product_components:pds:target_identification::1.0;
  rdfs:comment "The target is classified as a star".
 
pds4:urn:nasa:pds:0001_nasa_pds_1:pds:product_components:pds:target_identification:star_cluster::1.0 rdf:type rdfs:Class;
  rdfs:label "Star Cluster";
  rdfs:subClassOf pds4:urn:nasa:pds:0001_nasa_pds_1:pds:product_components:pds:target_identification::1.0;
  rdfs:comment "The target is classified as a star cluster".
 
pds4:urn:nasa:pds:0001_nasa_pds_1:pds:product_components:pds:target_identification:synthetic_sample::1.0 rdf:type rdfs:Class;
  rdfs:label "Synthetic Sample";
  rdfs:subClassOf pds4:urn:nasa:pds:0001_nasa_pds_1:pds:product_components:pds:target_identification::1.0;
  rdfs:comment "The target is a sample created in a laboratory".
 
pds4:urn:nasa:pds:0001_nasa_pds_1:pds:product_components:pds:target_identification:terrestrial_sample::1.0 rdf:type rdfs:Class;
  rdfs:label "Terrestrial Sample";
  rdfs:subClassOf pds4:urn:nasa:pds:0001_nasa_pds_1:pds:product_components:pds:target_identification::1.0;
  rdfs:comment "The target is classified as a terrestrial sample".
 
pds4:urn:nasa:pds:0001_nasa_pds_1:pds:product_components:pds:target_identification:trans-neptunian_object::1.0 rdf:type rdfs:Class;
  rdfs:label "Trans-Neptunian Object";
  rdfs:subClassOf pds4:urn:nasa:pds:0001_nasa_pds_1:pds:product_components:pds:target_identification::1.0;
  rdfs:comment "The target is classified as a trans-Neptunian object".
 
pds4:urn:nasa:pds:0001_nasa_pds_1:pds:tndo_context_pds3:pds:target_pds3::1.0 rdf:type rdfs:Class;
  rdfs:label "Target_PDS3";
  pds4:subClassOf pds4:urn:nasa:pds:0001_nasa_pds_1:pds:tagged_nondigital_object:pds:tndo_context_pds3::1.0;
  rdfs:comment "The Target class provides a description of a phyiscal object that is the object of data collection. This class captures the PDS3 catalog Target information.".
 
pds4:urn:nasa:pds:0001_nasa_pds_1:all:user:msn_surface:telemetry::1.0 rdf:type rdfs:Class;
  rdfs:label "Telemetry";
  pds4:subClassOf pds4:urn:nasa:pds:0001_nasa_pds_1:all:user::1.0;
  rdfs:comment "The Telemetry class contains downlink-related attributes used primarily during mission operations.".
 
pds4:urn:nasa:pds:0001_nasa_pds_1:pds:tndo_context:pds:telescope::1.0 rdf:type rdfs:Class;
  rdfs:label "Telescope";
  pds4:subClassOf pds4:urn:nasa:pds:0001_nasa_pds_1:pds:tagged_nondigital_object:pds:tndo_context::1.0;
  rdfs:comment "The Telescope class provides coordinates and parameters for terrestrial, ground-based telescopes.".
 
pds4:urn:nasa:pds:0001_nasa_pds_1:pds:tndo_supplemental:pds:term_map_skos::1.0 rdf:type rdfs:Class;
  rdfs:label "Term_Map_SKOS";
  pds4:subClassOf pds4:urn:nasa:pds:0001_nasa_pds_1:pds:tagged_nondigital_object:pds:tndo_supplemental::1.0;
  rdfs:comment "TheTerm_Map_SKOS class is used to collect a set of terms and definitions for a SKOS ontology.".
 
pds4:urn:nasa:pds:0001_nasa_pds_1:pds:tagged_nondigital_child:pds:terminological_entry::1.0 rdf:type rdfs:Class;
  rdfs:label "Terminological_Entry";
  pds4:subClassOf pds4:urn:nasa:pds:0001_nasa_pds_1:all:user:pds:tagged_nondigital_child::1.0;
  rdfs:comment "The terminological_entry class provides the name (designation) and definition of the attribute in a specified natural language.".
 
pds4:urn:nasa:pds:0001_nasa_pds_1:pds:tagged_nondigital_child:pds:terminological_entry_skos::1.0 rdf:type rdfs:Class;
  rdfs:label "Terminological_Entry_SKOS";
  pds4:subClassOf pds4:urn:nasa:pds:0001_nasa_pds_1:all:user:pds:tagged_nondigital_child::1.0;
  rdfs:comment "The terminological_entry_SKOS class provides terms and definitions for a SKOS ontology.".
 
pds4:urn:nasa:pds:0001_nasa_pds_1:all:user:img:thumbnail::1.0 rdf:type rdfs:Class;
  rdfs:label "Thumbnail";
  pds4:subClassOf pds4:urn:nasa:pds:0001_nasa_pds_1:all:user::1.0;
  rdfs:comment "Describes a Thumbnail product, which is a greatly reduced resolution version of the image.".
 
pds4:urn:nasa:pds:0001_nasa_pds_1:all:user:img:tile::1.0 rdf:type rdfs:Class;
  rdfs:label "Tile";
  pds4:subClassOf pds4:urn:nasa:pds:0001_nasa_pds_1:all:user::1.0;
  rdfs:comment "Contains parameters that describe how an image was or will be broken into tiles, before reassembly into a whole. This is generally intended for cameras that break up an exposure into tiles for transmission, but can also be used to describe tiling done by a ground system (e.g. for display purposes) if needed. Tiles need not be regular nor do they need to cover the entire area, and irregular tiles may overlap. Note that the image in which this class appears is expected to contain all the tiles (i.e. not just a single tile).".
 
pds4:urn:nasa:pds:0001_nasa_pds_1:all:user:img:tiling::1.0 rdf:type rdfs:Class;
  rdfs:label "Tiling";
  pds4:subClassOf pds4:urn:nasa:pds:0001_nasa_pds_1:all:user::1.0;
  rdfs:comment "Contains parameters that describe how an image was or will be broken into tiles, before reassembly into a whole. This is generally intended for cameras that break up an exposure into tiles for transmission, but can also be used to describe tiling done by a ground system (e.g. for display purposes) if needed. Tiles need not be regular nor do they need to cover the entire area, and irregular tiles may overlap. Note that the image in which this class appears is expected to contain all the tiles (i.e. not just a single tile).".
 
pds4:urn:nasa:pds:0001_nasa_pds_1:pds:product_components:pds:time_coordinates::1.0 rdf:type rdfs:Class;
  rdfs:label "Time_Coordinates";
  pds4:subClassOf pds4:urn:nasa:pds:0001_nasa_pds_1:all:user:pds:product_components::1.0;
  rdfs:comment "The Time_Coordinates class provides a list of time coordinates.".
 
pds4:urn:nasa:pds:0001_nasa_pds_1:all:user:nucspec:time_range_et::1.0 rdf:type rdfs:Class;
  rdfs:label "Time_Range_ET";
  pds4:subClassOf pds4:urn:nasa:pds:0001_nasa_pds_1:all:user::1.0;
  rdfs:comment "Ephemeris time, as defined by the referenced field, for the first and last science data records for a temporally contiguous block of records with the same state or affected by the same conditions. These records need not be contiguous within the file, but there must be no records with a different state between the start and stop time.".
 
pds4:urn:nasa:pds:0001_nasa_pds_1:all:user:nucspec:time_range_sclk::1.0 rdf:type rdfs:Class;
  rdfs:label "Time_Range_SCLK";
  pds4:subClassOf pds4:urn:nasa:pds:0001_nasa_pds_1:all:user::1.0;
  rdfs:comment "Spacecraft clock time in ticks since spacecraft clock start for the first and last science data records for a temporally contiguous block of records with the same state or affected by the same conditions. These records need not be contiguous within the file, but there must be no records with a different state between the start and stop time.".
 
pds4:urn:nasa:pds:0001_nasa_pds_1:all:user:nucspec:time_range_utc::1.0 rdf:type rdfs:Class;
  rdfs:label "Time_Range_UTC";
  pds4:subClassOf pds4:urn:nasa:pds:0001_nasa_pds_1:all:user::1.0;
  rdfs:comment "Universal Coordinated Time for the first and last science data records for a temporally contiguous block of records with the same state or affected by the same conditions. These records need not be contiguous within the file, but there must be no records with a different state between the start and stop time.".
 
pds4:urn:nasa:pds:0001_nasa_pds_1:pds:table_character:pds:transfer_manifest::1.0 rdf:type rdfs:Class;
  rdfs:label "Transfer_Manifest";
  pds4:subClassOf pds4:urn:nasa:pds:0001_nasa_pds_1:pds:table_base:pds:table_character::1.0;
  rdfs:comment "The Transfer_Manifest class defines a table that maps product LIDVIDs to the file_specificaition_names of the products\\' XML label files.".
 
pds4:urn:nasa:pds:0001_nasa_pds_1:all:user:cart:transverse_mercator::1.0 rdf:type rdfs:Class;
  rdfs:label "Transverse_Mercator";
  pds4:subClassOf pds4:urn:nasa:pds:0001_nasa_pds_1:all:user::1.0;
  rdfs:comment "The Transverse_Mercator class contains parameters for the Transverse Mercator projection. Synder 1987, DOI:10.3133\\//pp1395, page 48: https:\\//\\//pubs.usgs.gov\\//pp\\//1395\\//report.pdf#page=60 PROJ: https:\\//\\//proj.org\\//operations\\//projections\\//tmerc.html ".
 
pds4:urn:nasa:pds:0001_nasa_pds_1:all:user:ctli:type_list::1.0 rdf:type rdfs:Class;
  rdfs:label "Type_List";
  pds4:subClassOf pds4:urn:nasa:pds:0001_nasa_pds_1:all:user::1.0;
  rdfs:comment "The Type List class provides a list of values and their value meanings.".
 
pds4:urn:nasa:pds:0001_nasa_pds_1:all:user:ctli:type_list:accelerometer::1.0 rdf:type rdfs:Class;
  rdfs:label "Accelerometer";
  rdfs:subClassOf pds4:urn:nasa:pds:0001_nasa_pds_1:all:user:ctli:type_list::1.0;
  rdfs:comment " An accelerometer measures acceleration -- rate of change of velocity -- in its own rest frame. ".
 
pds4:urn:nasa:pds:0001_nasa_pds_1:all:user:ctli:type_list:altimeter::1.0 rdf:type rdfs:Class;
  rdfs:label "Altimeter";
  rdfs:subClassOf pds4:urn:nasa:pds:0001_nasa_pds_1:all:user:ctli:type_list::1.0;
  rdfs:comment " An altimeter measures distance above a surface. ".
 
pds4:urn:nasa:pds:0001_nasa_pds_1:all:user:ctli:type_list:atmospheric_structure_instrument::1.0 rdf:type rdfs:Class;
  rdfs:label "Atmospheric Structure Instrument";
  rdfs:subClassOf pds4:urn:nasa:pds:0001_nasa_pds_1:all:user:ctli:type_list::1.0;
  rdfs:comment " An atmospheric structure instrument measures one or more structural properties of an atmosphere. These properties may include -- but are not limited to -- pressure, temperature, density, wind speed, and wind direction. ".
 
pds4:urn:nasa:pds:0001_nasa_pds_1:all:user:ctli:type_list:camera::1.0 rdf:type rdfs:Class;
  rdfs:label "Camera";
  rdfs:subClassOf pds4:urn:nasa:pds:0001_nasa_pds_1:all:user:ctli:type_list::1.0;
  rdfs:comment " A camera is an optical instrument that captures a still image or a sequence of images on physical media. ".
 
pds4:urn:nasa:pds:0001_nasa_pds_1:all:user:ctli:type_list:charged_particle_detector::1.0 rdf:type rdfs:Class;
  rdfs:label "Charged Particle Detector";
  rdfs:subClassOf pds4:urn:nasa:pds:0001_nasa_pds_1:all:user:ctli:type_list::1.0;
  rdfs:comment " A charged particle detector detects and\\//or counts charged particles, and provides information about particle properties and distributions. ".
 
pds4:urn:nasa:pds:0001_nasa_pds_1:all:user:ctli:type_list:dust_analyzer::1.0 rdf:type rdfs:Class;
  rdfs:label "Dust Analyzer";
  rdfs:subClassOf pds4:urn:nasa:pds:0001_nasa_pds_1:all:user:ctli:type_list::1.0;
  rdfs:comment " A dust analyzer measures the size and\\//or energy distribution of dust particles. ".
 
pds4:urn:nasa:pds:0001_nasa_pds_1:all:user:ctli:type_list:electric_field_instrument::1.0 rdf:type rdfs:Class;
  rdfs:label "Electric Field Instrument";
  rdfs:subClassOf pds4:urn:nasa:pds:0001_nasa_pds_1:all:user:ctli:type_list::1.0;
  rdfs:comment " An electric field instrument measures the direction and\\//or strength of an electric field. ".
 
pds4:urn:nasa:pds:0001_nasa_pds_1:all:user:ctli:type_list:gamma_ray_detector::1.0 rdf:type rdfs:Class;
  rdfs:label "Gamma Ray Detector";
  rdfs:subClassOf pds4:urn:nasa:pds:0001_nasa_pds_1:all:user:ctli:type_list::1.0;
  rdfs:comment " A gamma ray detector is an instrument that detects gamma rays. ".
 
pds4:urn:nasa:pds:0001_nasa_pds_1:all:user:ctli:type_list:gas_analyzer::1.0 rdf:type rdfs:Class;
  rdfs:label "Gas Analyzer";
  rdfs:subClassOf pds4:urn:nasa:pds:0001_nasa_pds_1:all:user:ctli:type_list::1.0;
  rdfs:comment " A gas analyzer measures the concentration of one or more species in a mixture of neutral gases. ".
 
pds4:urn:nasa:pds:0001_nasa_pds_1:all:user:ctli:type_list:gravimeter::1.0 rdf:type rdfs:Class;
  rdfs:label "Gravimeter";
  rdfs:subClassOf pds4:urn:nasa:pds:0001_nasa_pds_1:all:user:ctli:type_list::1.0;
  rdfs:comment " A gravimeter measures gravitational acceleration. ".
 
pds4:urn:nasa:pds:0001_nasa_pds_1:all:user:ctli:type_list:imager::1.0 rdf:type rdfs:Class;
  rdfs:label "Imager";
  rdfs:subClassOf pds4:urn:nasa:pds:0001_nasa_pds_1:all:user:ctli:type_list::1.0;
  rdfs:comment " An imager detects and converts information into a digital image. ".
 
pds4:urn:nasa:pds:0001_nasa_pds_1:all:user:ctli:type_list:imaging_spectrometer::1.0 rdf:type rdfs:Class;
  rdfs:label "Imaging Spectrometer";
  rdfs:subClassOf pds4:urn:nasa:pds:0001_nasa_pds_1:all:user:ctli:type_list::1.0;
  rdfs:comment " An imaging spectrometer acquires a spectrally-resolved image of an object or scene. Two axes of the image correspond to orthogonal spatial dimensions and the third corresponds to wavelength. ".
 
pds4:urn:nasa:pds:0001_nasa_pds_1:all:user:ctli:type_list:interferometer::1.0 rdf:type rdfs:Class;
  rdfs:label "Interferometer";
  rdfs:subClassOf pds4:urn:nasa:pds:0001_nasa_pds_1:all:user:ctli:type_list::1.0;
  rdfs:comment " An interferometer superposes waves such that constructive and destructive interference results in patterns that can be interpreted as very small displacements at the signal source. ".
 
pds4:urn:nasa:pds:0001_nasa_pds_1:all:user:ctli:type_list:langmuir_probe::1.0 rdf:type rdfs:Class;
  rdfs:label "Langmuir Probe";
  rdfs:subClassOf pds4:urn:nasa:pds:0001_nasa_pds_1:all:user:ctli:type_list::1.0;
  rdfs:comment " A Langmuir probe consists of one or more electrodes used to determine in-situ plasma properties such as density and temperature from the measured potentials and currents. ".
 
pds4:urn:nasa:pds:0001_nasa_pds_1:all:user:ctli:type_list:lidar::1.0 rdf:type rdfs:Class;
  rdfs:label "Lidar";
  rdfs:subClassOf pds4:urn:nasa:pds:0001_nasa_pds_1:all:user:ctli:type_list::1.0;
  rdfs:comment " A lidar measures distance to a target by illuminating it with a pulsed laser and measuring the time delay of the reflected signal. ".
 
pds4:urn:nasa:pds:0001_nasa_pds_1:all:user:ctli:type_list:magnetometer::1.0 rdf:type rdfs:Class;
  rdfs:label "Magnetometer";
  rdfs:subClassOf pds4:urn:nasa:pds:0001_nasa_pds_1:all:user:ctli:type_list::1.0;
  rdfs:comment " A magnetometer measures the direction and\\//or strength of a magnetic field. ".
 
pds4:urn:nasa:pds:0001_nasa_pds_1:all:user:ctli:type_list:mass_spectrometer::1.0 rdf:type rdfs:Class;
  rdfs:label "Mass Spectrometer";
  rdfs:subClassOf pds4:urn:nasa:pds:0001_nasa_pds_1:all:user:ctli:type_list::1.0;
  rdfs:comment " A mass spectrometer sorts and counts atoms, ions, and\\//or molecules based on their masses. ".
 
pds4:urn:nasa:pds:0001_nasa_pds_1:all:user:ctli:type_list:meteorology::1.0 rdf:type rdfs:Class;
  rdfs:label "Meteorology";
  rdfs:subClassOf pds4:urn:nasa:pds:0001_nasa_pds_1:all:user:ctli:type_list::1.0;
  rdfs:comment " A meteorology instrument measures in situ meteorological conditions. These may include -- but are not limited to -- pressure, temperature, wind speed, and wind direction. ".
 
pds4:urn:nasa:pds:0001_nasa_pds_1:all:user:ctli:type_list:microphone::1.0 rdf:type rdfs:Class;
  rdfs:label "Microphone";
  rdfs:subClassOf pds4:urn:nasa:pds:0001_nasa_pds_1:all:user:ctli:type_list::1.0;
  rdfs:comment " A microphone converts sound waves into electrical signals. ".
 
pds4:urn:nasa:pds:0001_nasa_pds_1:all:user:ctli:type_list:microscope::1.0 rdf:type rdfs:Class;
  rdfs:label "Microscope";
  rdfs:subClassOf pds4:urn:nasa:pds:0001_nasa_pds_1:all:user:ctli:type_list::1.0;
  rdfs:comment " A microscope magnifies objects that are too small to be seen with the naked eye. ".
 
pds4:urn:nasa:pds:0001_nasa_pds_1:all:user:ctli:type_list:mutual_impedance_probe::1.0 rdf:type rdfs:Class;
  rdfs:label "Mutual Impedance Probe";
  rdfs:subClassOf pds4:urn:nasa:pds:0001_nasa_pds_1:all:user:ctli:type_list::1.0;
  rdfs:comment " A mutual impedance probe measures in situ bulk plasma properties at radio frequencies. ".
 
pds4:urn:nasa:pds:0001_nasa_pds_1:all:user:ctli:type_list:nephelometer::1.0 rdf:type rdfs:Class;
  rdfs:label "Nephelometer";
  rdfs:subClassOf pds4:urn:nasa:pds:0001_nasa_pds_1:all:user:ctli:type_list::1.0;
  rdfs:comment " A nephelometer measures the concentration of suspended (cloud) particulates. ".
 
pds4:urn:nasa:pds:0001_nasa_pds_1:all:user:ctli:type_list:neutral_particle_detector::1.0 rdf:type rdfs:Class;
  rdfs:label "Neutral Particle Detector";
  rdfs:subClassOf pds4:urn:nasa:pds:0001_nasa_pds_1:all:user:ctli:type_list::1.0;
  rdfs:comment " A neutral particle detector detects and\\//or counts neutral particles, and provides information about particle properties and distributions. ".
 
pds4:urn:nasa:pds:0001_nasa_pds_1:all:user:ctli:type_list:neutron_detector::1.0 rdf:type rdfs:Class;
  rdfs:label "Neutron Detector";
  rdfs:subClassOf pds4:urn:nasa:pds:0001_nasa_pds_1:all:user:ctli:type_list::1.0;
  rdfs:comment " A neutron detector detects and\\//or counts neutrons. ".
 
pds4:urn:nasa:pds:0001_nasa_pds_1:all:user:ctli:type_list:photometer::1.0 rdf:type rdfs:Class;
  rdfs:label "Photometer";
  rdfs:subClassOf pds4:urn:nasa:pds:0001_nasa_pds_1:all:user:ctli:type_list::1.0;
  rdfs:comment " A photometer measures the intensity of electromagnetic radiation over a wavelength range at infrared and shorter wavelengths. ".
 
pds4:urn:nasa:pds:0001_nasa_pds_1:all:user:ctli:type_list:polarimeter::1.0 rdf:type rdfs:Class;
  rdfs:label "Polarimeter";
  rdfs:subClassOf pds4:urn:nasa:pds:0001_nasa_pds_1:all:user:ctli:type_list::1.0;
  rdfs:comment " A polarimeter measures the polarization of an electromagnetic wave. ".
 
pds4:urn:nasa:pds:0001_nasa_pds_1:all:user:ctli:type_list:radar::1.0 rdf:type rdfs:Class;
  rdfs:label "Radar";
  rdfs:subClassOf pds4:urn:nasa:pds:0001_nasa_pds_1:all:user:ctli:type_list::1.0;
  rdfs:comment " A radar transmits an electromagnetic wave, then measures amplitude, time delay, frequency shift, phase shift, and\\//or polarization of the echo from a distant target. ".
 
pds4:urn:nasa:pds:0001_nasa_pds_1:all:user:ctli:type_list:radio_receiver::1.0 rdf:type rdfs:Class;
  rdfs:label "Radio Receiver";
  rdfs:subClassOf pds4:urn:nasa:pds:0001_nasa_pds_1:all:user:ctli:type_list::1.0;
  rdfs:comment " A radio receiver detects the information in propagating electromagnetic waves collected by an antenna. ".
 
pds4:urn:nasa:pds:0001_nasa_pds_1:all:user:ctli:type_list:radio_science::1.0 rdf:type rdfs:Class;
  rdfs:label "Radio Science";
  rdfs:subClassOf pds4:urn:nasa:pds:0001_nasa_pds_1:all:user:ctli:type_list::1.0;
  rdfs:comment " Radio science is the use of active and\\//or passive electromagnetic waves to probe the environment. ".
 
pds4:urn:nasa:pds:0001_nasa_pds_1:all:user:ctli:type_list:radiometer::1.0 rdf:type rdfs:Class;
  rdfs:label "Radiometer";
  rdfs:subClassOf pds4:urn:nasa:pds:0001_nasa_pds_1:all:user:ctli:type_list::1.0;
  rdfs:comment " A radiometer measures radiant flux (power) of electromagnetic radiation. ".
 
pds4:urn:nasa:pds:0001_nasa_pds_1:all:user:ctli:type_list:relaxation_sounder::1.0 rdf:type rdfs:Class;
  rdfs:label "Relaxation Sounder";
  rdfs:subClassOf pds4:urn:nasa:pds:0001_nasa_pds_1:all:user:ctli:type_list::1.0;
  rdfs:comment "A relaxation sounder determines the properties of a plasma by actively probing at radio frequencies at and near the plasma frequency.".
 
pds4:urn:nasa:pds:0001_nasa_pds_1:all:user:ctli:type_list:seismometer::1.0 rdf:type rdfs:Class;
  rdfs:label "Seismometer";
  rdfs:subClassOf pds4:urn:nasa:pds:0001_nasa_pds_1:all:user:ctli:type_list::1.0;
  rdfs:comment " A seismometer measures ground motions such as might be caused by earthquakes, volcanic eruptions, or explosions. ".
 
pds4:urn:nasa:pds:0001_nasa_pds_1:all:user:ctli:type_list:spacecraft_sensor::1.0 rdf:type rdfs:Class;
  rdfs:label "Spacecraft Sensor";
  rdfs:subClassOf pds4:urn:nasa:pds:0001_nasa_pds_1:all:user:ctli:type_list::1.0;
  rdfs:comment " A spacecraft sensor captures information on the status or physical condition of a spacecraft or its components. These may include, but are not limited to, temperatures, mechanical friction, currents, voltages, etc. ".
 
pds4:urn:nasa:pds:0001_nasa_pds_1:all:user:ctli:type_list:spectrometer::1.0 rdf:type rdfs:Class;
  rdfs:label "Spectrometer";
  rdfs:subClassOf pds4:urn:nasa:pds:0001_nasa_pds_1:all:user:ctli:type_list::1.0;
  rdfs:comment " A spectrometer measures an energy spectrum. ".
 
pds4:urn:nasa:pds:0001_nasa_pds_1:all:user:ctli:type_list:spectrum_analyzer::1.0 rdf:type rdfs:Class;
  rdfs:label "Spectrum Analyzer";
  rdfs:subClassOf pds4:urn:nasa:pds:0001_nasa_pds_1:all:user:ctli:type_list::1.0;
  rdfs:comment " A spectrum analyzer measures the properties of photons, charged particles, or electrical signals as a function of frequency or energy. ".
 
pds4:urn:nasa:pds:0001_nasa_pds_1:all:user:ctli:type_list:sub-surface_tool::1.0 rdf:type rdfs:Class;
  rdfs:label "Sub-Surface Tool";
  rdfs:subClassOf pds4:urn:nasa:pds:0001_nasa_pds_1:all:user:ctli:type_list::1.0;
  rdfs:comment " A sub-surface tool probes the upper few meters of a surface to infer its properties. Examples include (but are not limited to) drills and penetrators. ".
 
pds4:urn:nasa:pds:0001_nasa_pds_1:all:user:ctli:type_list:surface_tool::1.0 rdf:type rdfs:Class;
  rdfs:label "Surface Tool";
  rdfs:subClassOf pds4:urn:nasa:pds:0001_nasa_pds_1:all:user:ctli:type_list::1.0;
  rdfs:comment " A surface tool physically probes a surface to infer its properties. Examples include (but are not limited to) brush and deployment systems. ".
 
pds4:urn:nasa:pds:0001_nasa_pds_1:all:user:ctli:type_list:temperature_sensor::1.0 rdf:type rdfs:Class;
  rdfs:label "Temperature Sensor";
  rdfs:subClassOf pds4:urn:nasa:pds:0001_nasa_pds_1:all:user:ctli:type_list::1.0;
  rdfs:comment "A temperature sensor measures temperature.".
 
pds4:urn:nasa:pds:0001_nasa_pds_1:all:user:ctli:type_list:weather_station::1.0 rdf:type rdfs:Class;
  rdfs:label "Weather Station";
  rdfs:subClassOf pds4:urn:nasa:pds:0001_nasa_pds_1:all:user:ctli:type_list::1.0;
  rdfs:comment " A weather station is a suite of instruments that measures in situ meteorological conditions. These may include -- but are not limited to -- pressure, temperature, wind speed and wind direction. ".
 
pds4:urn:nasa:pds:0001_nasa_pds_1:all:user:ctli:type_list:wind_tunnel::1.0 rdf:type rdfs:Class;
  rdfs:label "Wind Tunnel";
  rdfs:subClassOf pds4:urn:nasa:pds:0001_nasa_pds_1:all:user:ctli:type_list::1.0;
  rdfs:comment " A wind tunnel is used to study the effects of air moving past solid objects. ".
 
pds4:urn:nasa:pds:0001_nasa_pds_1:pds:tndo_context:pds:type_list_area::1.0 rdf:type rdfs:Class;
  rdfs:label "Type_List_Area";
  pds4:subClassOf pds4:urn:nasa:pds:0001_nasa_pds_1:pds:tagged_nondigital_object:pds:tndo_context::1.0;
  rdfs:comment "The Type_List_Area allows the insertion of a Type List.".
 
pds4:urn:nasa:pds:0001_nasa_pds_1:pds:tagged_digital_child:pds:uniformly_sampled::1.0 rdf:type rdfs:Class;
  rdfs:label "Uniformly_Sampled";
  pds4:subClassOf pds4:urn:nasa:pds:0001_nasa_pds_1:all:user:pds:tagged_digital_child::1.0;
  rdfs:comment "The Uniformly_Sampled class provides parameters for a uniformly sampled table.".
 
pds4:urn:nasa:pds:0001_nasa_pds_1:all:user:sp:uniformly_sampled_energy::1.0 rdf:type rdfs:Class;
  rdfs:label "Uniformly_Sampled_Energy";
  pds4:subClassOf pds4:urn:nasa:pds:0001_nasa_pds_1:all:user::1.0;
  rdfs:comment " The Uniformly_Sampled_Energy class provides attributes describing the spectral characteristics of a named axis of an Array object or the rows or fields of a Table object, in cases where the spectral sampling interval is regular and the sampling parameters are in energy units. ".
 
pds4:urn:nasa:pds:0001_nasa_pds_1:all:user:sp:uniformly_sampled_frequency::1.0 rdf:type rdfs:Class;
  rdfs:label "Uniformly_Sampled_Frequency";
  pds4:subClassOf pds4:urn:nasa:pds:0001_nasa_pds_1:all:user::1.0;
  rdfs:comment " The Uniformly_Sampled_Frequency class provides attributes describing the spectral characteristics of a named axis of an Array object or the rows or fields of a Table object, in cases where the spectral sampling interval is regular and the sampling parameters are in frequency units. ".
 
pds4:urn:nasa:pds:0001_nasa_pds_1:all:user:rings:uniformly_sampled_radius::1.0 rdf:type rdfs:Class;
  rdfs:label "Uniformly_Sampled_Radius";
  pds4:subClassOf pds4:urn:nasa:pds:0001_nasa_pds_1:all:user::1.0;
  rdfs:comment " The Uniformly_Sampled_Radius class provides attributes describing the spectral characteristics of an axis of an Array object or the rows of a Table object, in cases where the spectral sampling interval is regular and the sampling parameters are in wavelength units. The axis is identified either by using Local_Internal_Reference, or by using axis name. The latter may be simpler to use if this class applies to multiple Array objects. ".
 
pds4:urn:nasa:pds:0001_nasa_pds_1:all:user:sp:uniformly_sampled_wavelength::1.0 rdf:type rdfs:Class;
  rdfs:label "Uniformly_Sampled_Wavelength";
  pds4:subClassOf pds4:urn:nasa:pds:0001_nasa_pds_1:all:user::1.0;
  rdfs:comment " The Uniformly_Sampled_Wavelength class provides attributes describing the spectral characteristics of a named axis of an Array object or the rows or fields of a Table object, in cases where the spectral sampling interval is regular and the sampling parameters are in wavelength units. ".
 
pds4:urn:nasa:pds:0001_nasa_pds_1:all:user:sp:uniformly_sampled_wavenumber::1.0 rdf:type rdfs:Class;
  rdfs:label "Uniformly_Sampled_Wavenumber";
  pds4:subClassOf pds4:urn:nasa:pds:0001_nasa_pds_1:all:user::1.0;
  rdfs:comment " The Uniformly_Sampled_Wavenumber class provides attributes describing the spectral characteristics of a named axis of an Array object or the rows or fields of a Table object, in cases where the spectral sampling interval is regular and the sampling parameters are in wavenumber units. ".
 
pds4:urn:nasa:pds:0001_nasa_pds_1:all:user:cart:universal_polar_stereographic::1.0 rdf:type rdfs:Class;
  rdfs:label "Universal_Polar_Stereographic";
  pds4:subClassOf pds4:urn:nasa:pds:0001_nasa_pds_1:all:user::1.0;
  rdfs:comment "The Universal_Polar_Stereographic class, generally used for Earth data sets, defines a grid system based on the polar stereographic projection, applied to the planet\\'s polar regions north of 84 degrees north and south of 80 degrees south. Synder 1987, DOI:10.3133\\//pp1395, page 157: https:\\//\\//pubs.usgs.gov\\//pp\\//1395\\//report.pdf#page=169 PROJ: https:\\//\\//proj.org\\//operations\\//projections\\//ups.html ".
 
pds4:urn:nasa:pds:0001_nasa_pds_1:all:user:cart:universal_transverse_mercator::1.0 rdf:type rdfs:Class;
  rdfs:label "Universal_Transverse_Mercator";
  pds4:subClassOf pds4:urn:nasa:pds:0001_nasa_pds_1:all:user::1.0;
  rdfs:comment "The Universal_Transverse_Mercator class defines a grid system based on the Transverse Mercator projection, applied between latitudes 84 degrees north and 80 degrees south on the planet\\'s surface. Synder 1987, DOI:10.3133\\//pp1395, page 57: https:\\//\\//pubs.usgs.gov\\//pp\\//1395\\//report.pdf#page=69 PROJ: https:\\//\\//proj.org\\//operations\\//projections\\//utm.html ".
 
pds4:urn:nasa:pds:0001_nasa_pds_1:pds:tndo_supplemental:pds:update::1.0 rdf:type rdfs:Class;
  rdfs:label "Update";
  pds4:subClassOf pds4:urn:nasa:pds:0001_nasa_pds_1:pds:tagged_nondigital_object:pds:tndo_supplemental::1.0;
  rdfs:comment "The Update class consists of update information.".
 
pds4:urn:nasa:pds:0001_nasa_pds_1:pds:product_components:pds:update_entry::1.0 rdf:type rdfs:Class;
  rdfs:label "Update_Entry";
  pds4:subClassOf pds4:urn:nasa:pds:0001_nasa_pds_1:all:user:pds:product_components::1.0;
  rdfs:comment "The Update Entry class provides the date and description of an update.".
 
pds4:urn:nasa:pds:0001_nasa_pds_1:pds:tndo_supplemental:pds:vector::1.0 rdf:type rdfs:Class;
  rdfs:label "Vector";
  pds4:subClassOf pds4:urn:nasa:pds:0001_nasa_pds_1:pds:tagged_nondigital_object:pds:tndo_supplemental::1.0;
  rdfs:comment "The Vector class provides the components of either a velocity or position vector.".
 
pds4:urn:nasa:pds:0001_nasa_pds_1:pds:tndo_supplemental:pds:vector:acceleration::1.0 rdf:type rdfs:Class;
  rdfs:label "Acceleration";
  rdfs:subClassOf pds4:urn:nasa:pds:0001_nasa_pds_1:pds:tndo_supplemental:pds:vector::1.0;
  rdfs:comment "Vector contains the components of an acceleration".
 
pds4:urn:nasa:pds:0001_nasa_pds_1:pds:tndo_supplemental:pds:vector:pointing::1.0 rdf:type rdfs:Class;
  rdfs:label "Pointing";
  rdfs:subClassOf pds4:urn:nasa:pds:0001_nasa_pds_1:pds:tndo_supplemental:pds:vector::1.0;
  rdfs:comment "Vector contains the components of a direction".
 
pds4:urn:nasa:pds:0001_nasa_pds_1:pds:tndo_supplemental:pds:vector:position::1.0 rdf:type rdfs:Class;
  rdfs:label "Position";
  rdfs:subClassOf pds4:urn:nasa:pds:0001_nasa_pds_1:pds:tndo_supplemental:pds:vector::1.0;
  rdfs:comment "Vector contains the components of a position".
 
pds4:urn:nasa:pds:0001_nasa_pds_1:pds:tndo_supplemental:pds:vector:velocity::1.0 rdf:type rdfs:Class;
  rdfs:label "Velocity";
  rdfs:subClassOf pds4:urn:nasa:pds:0001_nasa_pds_1:pds:tndo_supplemental:pds:vector::1.0;
  rdfs:comment "Vector contains the components of a velocity".
 
pds4:urn:nasa:pds:0001_nasa_pds_1:geom:vector_cartesian_unit:geom:vector_axis::1.0 rdf:type rdfs:Class;
  rdfs:label "Vector_Axis";
  pds4:subClassOf pds4:urn:nasa:pds:0001_nasa_pds_1:all:user:geom:vector_cartesian_unit::1.0;
  rdfs:comment "The Vector_Axis is a unit vector that describes the axis of the camera, defined as the normal to the image plane. ".
 
pds4:urn:nasa:pds:0001_nasa_pds_1:geom:vector_cartesian_unit:geom:vector_axis_x::1.0 rdf:type rdfs:Class;
  rdfs:label "Vector_Axis_X";
  pds4:subClassOf pds4:urn:nasa:pds:0001_nasa_pds_1:all:user:geom:vector_cartesian_unit::1.0;
  rdfs:comment " Unit column-plane rotation axis, passing through the sphere center, typically vertical and pointing down so that positive rotations (by the right-hand rule) will rotate the forward half of the plane in the (rightward) direction of increasing column (as projected on the forward hemisphere). ".
 
pds4:urn:nasa:pds:0001_nasa_pds_1:geom:vector_cartesian_unit:geom:vector_axis_y::1.0 rdf:type rdfs:Class;
  rdfs:label "Vector_Axis_Y";
  pds4:subClassOf pds4:urn:nasa:pds:0001_nasa_pds_1:all:user:geom:vector_cartesian_unit::1.0;
  rdfs:comment " Unit row-plane rotation axis, passing through the sphere center, typically horizontal and pointing left so that positive rotations (by the right-hand rule) will rotate the forward half of the plane in the (downward) direction of increasing row (as projected on the forward hemisphere). ".
 
pds4:urn:nasa:pds:0001_nasa_pds_1:pds:tndo_supplemental:pds:vector_cartesian_3::1.0 rdf:type rdfs:Class;
  rdfs:label "Vector_Cartesian_3";
  pds4:subClassOf pds4:urn:nasa:pds:0001_nasa_pds_1:pds:tagged_nondigital_object:pds:tndo_supplemental::1.0;
  rdfs:comment "The Vector_Cartesian_3_Base class is the parent class of 3 element Cartesian vectors.".
 
pds4:urn:nasa:pds:0001_nasa_pds_1:pds:vector_cartesian_3:pds:vector_cartesian_3_acceleration::1.0 rdf:type rdfs:Class;
  rdfs:label "Vector_Cartesian_3_Acceleration";
  pds4:subClassOf pds4:urn:nasa:pds:0001_nasa_pds_1:pds:tndo_supplemental:pds:vector_cartesian_3::1.0;
  rdfs:comment "The Vector_Cartesian_3_Acceleration class is a 3 element Cartesian vector for acceleration coordinates.".
 
pds4:urn:nasa:pds:0001_nasa_pds_1:pds:vector_cartesian_3:pds:vector_cartesian_3_pointing::1.0 rdf:type rdfs:Class;
  rdfs:label "Vector_Cartesian_3_Pointing";
  pds4:subClassOf pds4:urn:nasa:pds:0001_nasa_pds_1:pds:tndo_supplemental:pds:vector_cartesian_3::1.0;
  rdfs:comment "The Vector_Cartesian_3_Pointing class is a 3 element normalized Cartesian vector for pointing.".
 
pds4:urn:nasa:pds:0001_nasa_pds_1:pds:vector_cartesian_3:pds:vector_cartesian_3_position::1.0 rdf:type rdfs:Class;
  rdfs:label "Vector_Cartesian_3_Position";
  pds4:subClassOf pds4:urn:nasa:pds:0001_nasa_pds_1:pds:tndo_supplemental:pds:vector_cartesian_3::1.0;
  rdfs:comment "The Vector_Cartesian_3_Position class is a 3 element Cartesian vector for position coordinates.".
 
pds4:urn:nasa:pds:0001_nasa_pds_1:pds:vector_cartesian_3:pds:vector_cartesian_3_velocity::1.0 rdf:type rdfs:Class;
  rdfs:label "Vector_Cartesian_3_Velocity";
  pds4:subClassOf pds4:urn:nasa:pds:0001_nasa_pds_1:pds:tndo_supplemental:pds:vector_cartesian_3::1.0;
  rdfs:comment "The Vector_Cartesian_3_Velocity class is a 3 element Cartesian vector for velocity coordinates.".
 
pds4:urn:nasa:pds:0001_nasa_pds_1:all:user:geom:vector_cartesian_acceleration_base::1.0 rdf:type rdfs:Class;
  rdfs:label "Vector_Cartesian_Acceleration_Base";
  pds4:subClassOf pds4:urn:nasa:pds:0001_nasa_pds_1:all:user::1.0;
  rdfs:comment "The Vector_Cartesian_Acceleration_Base is a three dimensional, rectangular coordinates vector. Uses units of linear acceleration. The included attributes are not sufficient to identify the endpoints of the vector. ".
 
pds4:urn:nasa:pds:0001_nasa_pds_1:geom:vector_cartesian_acceleration_base:geom:vector_cartesian_acceleration_extended_base::1.0 rdf:type rdfs:Class;
  rdfs:label "Vector_Cartesian_Acceleration_Extended_Base";
  pds4:subClassOf pds4:urn:nasa:pds:0001_nasa_pds_1:all:user:geom:vector_cartesian_acceleration_base::1.0;
  rdfs:comment "The Vector_Cartesian_Acceleration_Extended_Base is a three dimensional, rectangular coordinates vector. Uses units of linear acceleration. The included attributes are not sufficient to identify the endpoints of the vector. While the class Coordinate_System_Identification is optional, it must be used here if the coordinate system has not been specified in the enclosing class. ".
 
pds4:urn:nasa:pds:0001_nasa_pds_1:geom:vector_cartesian_acceleration_extended_base:geom:vector_cartesian_acceleration_generic::1.0 rdf:type rdfs:Class;
  rdfs:label "Vector_Cartesian_Acceleration_Generic";
  pds4:subClassOf pds4:urn:nasa:pds:0001_nasa_pds_1:geom:vector_cartesian_acceleration_base:geom:vector_cartesian_acceleration_extended_base::1.0;
  rdfs:comment "Vector_Cartesian_Acceleration_Generic is a three dimensional, rectangular coordinates vector. Uses units of linear acceleration. Includes attributes to identify the endpoints of the vector. While the class Coordinate_System_Identification is optional, it must be used here if the coordinate system has not been specified in the enclosing class. ".
 
pds4:urn:nasa:pds:0001_nasa_pds_1:all:user:cart:vector_cartesian_no_units::1.0 rdf:type rdfs:Class;
  rdfs:label "Vector_Cartesian_No_Units";
  pds4:subClassOf pds4:urn:nasa:pds:0001_nasa_pds_1:all:user::1.0;
  rdfs:comment "This is a generic vector in Cartesian space. The \"x\", \"y\", and \"z\" component have no units. ".
 
pds4:urn:nasa:pds:0001_nasa_pds_1:all:user:geom:vector_cartesian_no_units::1.0 rdf:type rdfs:Class;
  rdfs:label "Vector_Cartesian_No_Units";
  pds4:subClassOf pds4:urn:nasa:pds:0001_nasa_pds_1:all:user::1.0;
  rdfs:comment "This is a generic vector in Cartesian space. The \"x\", \"y\", and \"z\" component have no units. ".
 
pds4:urn:nasa:pds:0001_nasa_pds_1:all:user:geom:vector_cartesian_pixel::1.0 rdf:type rdfs:Class;
  rdfs:label "Vector_Cartesian_Pixel";
  pds4:subClassOf pds4:urn:nasa:pds:0001_nasa_pds_1:all:user::1.0;
  rdfs:comment "This a Cartesian pixel vector generally used in camera models. ".
 
pds4:urn:nasa:pds:0001_nasa_pds_1:all:user:cart:vector_cartesian_position_base::1.0 rdf:type rdfs:Class;
  rdfs:label "Vector_Cartesian_Position_Base";
  pds4:subClassOf pds4:urn:nasa:pds:0001_nasa_pds_1:all:user::1.0;
  rdfs:comment "The Vector_Cartesian_Position_Base is a three dimensional, rectangular coordinates vector. Uses units of length. The included attributes are not sufficient to identify the endpoints of the vector. ".
 
pds4:urn:nasa:pds:0001_nasa_pds_1:all:user:geom:vector_cartesian_position_base::1.0 rdf:type rdfs:Class;
  rdfs:label "Vector_Cartesian_Position_Base";
  pds4:subClassOf pds4:urn:nasa:pds:0001_nasa_pds_1:all:user::1.0;
  rdfs:comment "The Vector_Cartesian_Position_Base is a three dimensional, rectangular coordinates vector. Uses units of length. The included attributes are not sufficient to identify the endpoints of the vector. ".
 
pds4:urn:nasa:pds:0001_nasa_pds_1:geom:vector_cartesian_position_extended_base:geom:vector_cartesian_position_central_body_to_spacecraft::1.0 rdf:type rdfs:Class;
  rdfs:label "Vector_Cartesian_Position_Central_Body_To_Spacecraft";
  pds4:subClassOf pds4:urn:nasa:pds:0001_nasa_pds_1:geom:vector_cartesian_position_base:geom:vector_cartesian_position_extended_base::1.0;
  rdfs:comment "The Vector_Cartesian_Position_Central_Body_To_Spacecraft is a linear, rectangular coordinates vector from the center of mass of the central body (e.g., planet) to the spacecraft. While the class Coordinate_System_Identification is optional, it must be used here if the coordinate system has not been specified in the enclosing class. ".
 
pds4:urn:nasa:pds:0001_nasa_pds_1:geom:vector_cartesian_position_extended_base:geom:vector_cartesian_position_central_body_to_target::1.0 rdf:type rdfs:Class;
  rdfs:label "Vector_Cartesian_Position_Central_Body_To_Target";
  pds4:subClassOf pds4:urn:nasa:pds:0001_nasa_pds_1:geom:vector_cartesian_position_base:geom:vector_cartesian_position_extended_base::1.0;
  rdfs:comment "The Vector_Cartesian_Position_Central_Body_To_Target is a linear, rectangular coordinates vector from the center of mass of the central body (e.g., planet) to the target specified in the parent Geometry_Orbiter class. While the class Coordinate_System_Identification is optional, it must be used here if the coordinate system has not been specified in the enclosing class. ".
 
pds4:urn:nasa:pds:0001_nasa_pds_1:geom:vector_cartesian_position_extended_base:geom:vector_cartesian_position_earth_to_central_body::1.0 rdf:type rdfs:Class;
  rdfs:label "Vector_Cartesian_Position_Earth_To_Central_Body";
  pds4:subClassOf pds4:urn:nasa:pds:0001_nasa_pds_1:geom:vector_cartesian_position_base:geom:vector_cartesian_position_extended_base::1.0;
  rdfs:comment "The Vector_Cartesian_Position_Earth_To_Central_Body is a linear, rectangular coordinates vector from the Earth to the central body (e.g., planet). While the class Coordinate_System_Identification is optional, it must be used here if the coordinate system has not been specified in the enclosing class. ".
 
pds4:urn:nasa:pds:0001_nasa_pds_1:geom:vector_cartesian_position_extended_base:geom:vector_cartesian_position_earth_to_spacecraft::1.0 rdf:type rdfs:Class;
  rdfs:label "Vector_Cartesian_Position_Earth_To_Spacecraft";
  pds4:subClassOf pds4:urn:nasa:pds:0001_nasa_pds_1:geom:vector_cartesian_position_base:geom:vector_cartesian_position_extended_base::1.0;
  rdfs:comment "The Vector_Cartesian_Position_Earth_To_Spacecraft is a linear, rectangular coordinates vector from the Earth to the spacecraft. While the class Coordinate_System_Identification is optional, it must be used here if the coordinate system has not been specified in the enclosing class. ".
 
pds4:urn:nasa:pds:0001_nasa_pds_1:geom:vector_cartesian_position_extended_base:geom:vector_cartesian_position_earth_to_target::1.0 rdf:type rdfs:Class;
  rdfs:label "Vector_Cartesian_Position_Earth_To_Target";
  pds4:subClassOf pds4:urn:nasa:pds:0001_nasa_pds_1:geom:vector_cartesian_position_base:geom:vector_cartesian_position_extended_base::1.0;
  rdfs:comment "The Vector_Cartesian_Position_Earth_To_Target is a linear, rectangular coordinates vector from the Earth to the target specified in the parent Geometry_Orbiter class. While the class Coordinate_System_Identification is optional, it must be used here if the coordinate system has not been specified in the enclosing class. ".
 
pds4:urn:nasa:pds:0001_nasa_pds_1:geom:vector_cartesian_position_base:geom:vector_cartesian_position_extended_base::1.0 rdf:type rdfs:Class;
  rdfs:label "Vector_Cartesian_Position_Extended_Base";
  pds4:subClassOf pds4:urn:nasa:pds:0001_nasa_pds_1:all:user:geom:vector_cartesian_position_base::1.0;
  rdfs:comment "The Vector_Cartesian_Position_Extended_Base is a three dimensional, rectangular coordinates vector. Uses units of length. The included attributes are not sufficient to identify the endpoints of the vector. While the class Coordinate_System_Identification is optional, it must be used here if the coordinate system has not been specified in the enclosing class. ".
 
pds4:urn:nasa:pds:0001_nasa_pds_1:geom:vector_cartesian_position_extended_base:geom:vector_cartesian_position_generic::1.0 rdf:type rdfs:Class;
  rdfs:label "Vector_Cartesian_Position_Generic";
  pds4:subClassOf pds4:urn:nasa:pds:0001_nasa_pds_1:geom:vector_cartesian_position_base:geom:vector_cartesian_position_extended_base::1.0;
  rdfs:comment "Vector_Cartesian_Position_Generic is a three dimensional, rectangular coordinates vector. Uses units of length. Includes attributes to identify the endpoints of the vector. While the class Coordinate_System_Identification is optional, it must be used here if the coordinate system has not been specified in the enclosing class. ".
 
pds4:urn:nasa:pds:0001_nasa_pds_1:geom:vector_cartesian_position_extended_base:geom:vector_cartesian_position_ssb_to_central_body::1.0 rdf:type rdfs:Class;
  rdfs:label "Vector_Cartesian_Position_SSB_To_Central_Body";
  pds4:subClassOf pds4:urn:nasa:pds:0001_nasa_pds_1:geom:vector_cartesian_position_base:geom:vector_cartesian_position_extended_base::1.0;
  rdfs:comment "The Vector_Cartesian_Position_SSB_To_Central_Body is a linear, rectangular coordinates vector from the Solar System Barycenter to the central body (e.g., planet). While the class Coordinate_System_Identification is optional, it must be used here if the coordinate system has not been specified in the enclosing class. ".
 
pds4:urn:nasa:pds:0001_nasa_pds_1:geom:vector_cartesian_position_extended_base:geom:vector_cartesian_position_ssb_to_spacecraft::1.0 rdf:type rdfs:Class;
  rdfs:label "Vector_Cartesian_Position_SSB_To_Spacecraft";
  pds4:subClassOf pds4:urn:nasa:pds:0001_nasa_pds_1:geom:vector_cartesian_position_base:geom:vector_cartesian_position_extended_base::1.0;
  rdfs:comment "The Vector_Cartesian_Position_SSB_To_Spacecraft is a linear, rectangular coordinates vector from the Solar System Barycenter to the spacecraft. While the class Coordinate_System_Identification is optional, it must be used here if the coordinate system has not been specified in the enclosing class. ".
 
pds4:urn:nasa:pds:0001_nasa_pds_1:geom:vector_cartesian_position_extended_base:geom:vector_cartesian_position_ssb_to_target::1.0 rdf:type rdfs:Class;
  rdfs:label "Vector_Cartesian_Position_SSB_To_Target";
  pds4:subClassOf pds4:urn:nasa:pds:0001_nasa_pds_1:geom:vector_cartesian_position_base:geom:vector_cartesian_position_extended_base::1.0;
  rdfs:comment "The Vector_Cartesian_Position_SSB_To_Target is a linear, rectangular coordinates vector from the Solar System Barycenter to the target specified in the parent Geometry_Orbiter class. While the class Coordinate_System_Identification is optional, it must be used here if the coordinate system has not been specified in the enclosing class. ".
 
pds4:urn:nasa:pds:0001_nasa_pds_1:geom:vector_cartesian_position_extended_base:geom:vector_cartesian_position_spacecraft_to_target::1.0 rdf:type rdfs:Class;
  rdfs:label "Vector_Cartesian_Position_Spacecraft_To_Target";
  pds4:subClassOf pds4:urn:nasa:pds:0001_nasa_pds_1:geom:vector_cartesian_position_base:geom:vector_cartesian_position_extended_base::1.0;
  rdfs:comment "The Vector_Cartesian_Position_Spacecraft_To_Target is a linear, rectangular coordinates vector from the spacecraft to the target specified in the parent Geometry_Orbiter class. While the class Coordinate_System_Identification is optional, it must be used here if the coordinate system has not been specified in the enclosing class. ".
 
pds4:urn:nasa:pds:0001_nasa_pds_1:geom:vector_cartesian_position_extended_base:geom:vector_cartesian_position_sun_to_central_body::1.0 rdf:type rdfs:Class;
  rdfs:label "Vector_Cartesian_Position_Sun_To_Central_Body";
  pds4:subClassOf pds4:urn:nasa:pds:0001_nasa_pds_1:geom:vector_cartesian_position_base:geom:vector_cartesian_position_extended_base::1.0;
  rdfs:comment "The Vector_Cartesian_Position_Sun_To_Central_Body is a linear, rectangular coordinates vector from the Sun to the central body (e.g., planet). While the class Coordinate_System_Identification is optional, it must be used here if the coordinate system has not been specified in the enclosing class. ".
 
pds4:urn:nasa:pds:0001_nasa_pds_1:geom:vector_cartesian_position_extended_base:geom:vector_cartesian_position_sun_to_spacecraft::1.0 rdf:type rdfs:Class;
  rdfs:label "Vector_Cartesian_Position_Sun_To_Spacecraft";
  pds4:subClassOf pds4:urn:nasa:pds:0001_nasa_pds_1:geom:vector_cartesian_position_base:geom:vector_cartesian_position_extended_base::1.0;
  rdfs:comment "The Vector_Cartesian_Position_Sun_To_Spacecraft is a linear, rectangular coordinates vector from the Sun to the spacecraft. While the class Coordinate_System_Identification is optional, it must be used here if the coordinate system has not been specified in the enclosing class. ".
 
pds4:urn:nasa:pds:0001_nasa_pds_1:geom:vector_cartesian_position_extended_base:geom:vector_cartesian_position_sun_to_target::1.0 rdf:type rdfs:Class;
  rdfs:label "Vector_Cartesian_Position_Sun_To_Target";
  pds4:subClassOf pds4:urn:nasa:pds:0001_nasa_pds_1:geom:vector_cartesian_position_base:geom:vector_cartesian_position_extended_base::1.0;
  rdfs:comment "The Vector_Cartesian_Position_Sun_To_Target is a linear, rectangular coordinates vector from the Sun to the target specified in the parent Geometry_Orbiter class. While the class Coordinate_System_Identification is optional, it must be used here if the coordinate system has not been specified in the enclosing class. ".
 
pds4:urn:nasa:pds:0001_nasa_pds_1:all:user:geom:vector_cartesian_unit::1.0 rdf:type rdfs:Class;
  rdfs:label "Vector_Cartesian_Unit";
  pds4:subClassOf pds4:urn:nasa:pds:0001_nasa_pds_1:all:user::1.0;
  rdfs:comment "This is a generic unit vector in Cartesian space. The \"x\", \"y\", and \"z\" component have no units and are restricted to values between -1.0 and 1.0 inclusive. Further the length of the vector square root of the (sum of the squares of the components) must be 1.0. ".
 
pds4:urn:nasa:pds:0001_nasa_pds_1:all:user:cart:vector_cartesian_unit_base::1.0 rdf:type rdfs:Class;
  rdfs:label "Vector_Cartesian_Unit_Base";
  pds4:subClassOf pds4:urn:nasa:pds:0001_nasa_pds_1:all:user::1.0;
  rdfs:comment "This is a generic unit vector in Cartesian space. The \"x\", \"y\", and \"z\" component have no units and are restricted to values between -1.0 and 1.0 inclusive. Further the length of the vector square root of the (sum of the squares of the components) must be 1.0. ".
 
pds4:urn:nasa:pds:0001_nasa_pds_1:all:user:geom:vector_cartesian_velocity_base::1.0 rdf:type rdfs:Class;
  rdfs:label "Vector_Cartesian_Velocity_Base";
  pds4:subClassOf pds4:urn:nasa:pds:0001_nasa_pds_1:all:user::1.0;
  rdfs:comment "The Vector_Cartesian_Velocity_Base is a three dimensional, rectangular coordinates vector. Uses units of linear velocity. The included attributes are not sufficient to identify the endpoints of the vector. ".
 
pds4:urn:nasa:pds:0001_nasa_pds_1:geom:vector_cartesian_velocity_base:geom:vector_cartesian_velocity_extended_base::1.0 rdf:type rdfs:Class;
  rdfs:label "Vector_Cartesian_Velocity_Extended_Base";
  pds4:subClassOf pds4:urn:nasa:pds:0001_nasa_pds_1:all:user:geom:vector_cartesian_velocity_base::1.0;
  rdfs:comment "The Vector_Cartesian_Velocity_Extended_Base is a three dimensional, rectangular coordinates vector. Uses units of linear velocity. The included attributes are not sufficient to identify the endpoints of the vector. While the class Coordinate_System_Identification is optional, it must be used here if the coordinate system has not been specified in the enclosing class. ".
 
pds4:urn:nasa:pds:0001_nasa_pds_1:geom:vector_cartesian_velocity_extended_base:geom:vector_cartesian_velocity_generic::1.0 rdf:type rdfs:Class;
  rdfs:label "Vector_Cartesian_Velocity_Generic";
  pds4:subClassOf pds4:urn:nasa:pds:0001_nasa_pds_1:geom:vector_cartesian_velocity_base:geom:vector_cartesian_velocity_extended_base::1.0;
  rdfs:comment "Vector_Cartesian_Velocity_Generic is a three dimensional, rectangular coordinates vector. Uses units of linear velocity. Includes attributes to identify the endpoints of the vector. While the class Coordinate_System_Identification is optional, it must be used here if the coordinate system has not been specified in the enclosing class. ".
 
pds4:urn:nasa:pds:0001_nasa_pds_1:geom:vector_cartesian_velocity_extended_base:geom:vector_cartesian_velocity_spacecraft_relative_to_central_body::1.0 rdf:type rdfs:Class;
  rdfs:label "Vector_Cartesian_Velocity_Spacecraft_Relative_To_Central_Body";
  pds4:subClassOf pds4:urn:nasa:pds:0001_nasa_pds_1:geom:vector_cartesian_velocity_base:geom:vector_cartesian_velocity_extended_base::1.0;
  rdfs:comment "The Vector_Cartesian_Velocity_Spacecraft_Relative_To_Central_Body is a velocity vector in rectangular coordinates that gives the velocity of the spacecraft with respect to the central body (e.g., planet). While the class Coordinate_System_Identification is optional, it must be used here if the coordinate system has not been specified in the enclosing class. ".
 
pds4:urn:nasa:pds:0001_nasa_pds_1:geom:vector_cartesian_velocity_extended_base:geom:vector_cartesian_velocity_spacecraft_relative_to_earth::1.0 rdf:type rdfs:Class;
  rdfs:label "Vector_Cartesian_Velocity_Spacecraft_Relative_To_Earth";
  pds4:subClassOf pds4:urn:nasa:pds:0001_nasa_pds_1:geom:vector_cartesian_velocity_base:geom:vector_cartesian_velocity_extended_base::1.0;
  rdfs:comment "The Vector_Cartesian_Velocity_Spacecraft_Relative_To_Earth is a velocity vector in rectangular coordinates that gives the velocity of the spacecraft with respect to Earth. While the class Coordinate_System_Identification is optional, it must be used here if the coordinate system has not been specified in the enclosing class. ".
 
pds4:urn:nasa:pds:0001_nasa_pds_1:geom:vector_cartesian_velocity_extended_base:geom:vector_cartesian_velocity_spacecraft_relative_to_ssb::1.0 rdf:type rdfs:Class;
  rdfs:label "Vector_Cartesian_Velocity_Spacecraft_Relative_To_SSB";
  pds4:subClassOf pds4:urn:nasa:pds:0001_nasa_pds_1:geom:vector_cartesian_velocity_base:geom:vector_cartesian_velocity_extended_base::1.0;
  rdfs:comment "The Vector_Cartesian_Velocity_Spacecraft_Relative_To_SSB is a velocity vector in rectangular coordinates that gives the velocity of the spacecraft with respect to the Solar System Barycenter. While the class Coordinate_System_Identification is optional, it must be used here if the coordinate system has not been specified in the enclosing class. ".
 
pds4:urn:nasa:pds:0001_nasa_pds_1:geom:vector_cartesian_velocity_extended_base:geom:vector_cartesian_velocity_spacecraft_relative_to_sun::1.0 rdf:type rdfs:Class;
  rdfs:label "Vector_Cartesian_Velocity_Spacecraft_Relative_To_Sun";
  pds4:subClassOf pds4:urn:nasa:pds:0001_nasa_pds_1:geom:vector_cartesian_velocity_base:geom:vector_cartesian_velocity_extended_base::1.0;
  rdfs:comment " Vector_Cartesian_Velocity_Spacecraft_Relative_To_Sun is a velocity vector in rectangular coordinates that gives the velocity of the spacecraft with respect to the center of the Sun. While the class Coordinate_System_Identification is optional, it must be used here if the coordinate system has not been specified in the enclosing class. ".
 
pds4:urn:nasa:pds:0001_nasa_pds_1:geom:vector_cartesian_velocity_extended_base:geom:vector_cartesian_velocity_spacecraft_relative_to_target::1.0 rdf:type rdfs:Class;
  rdfs:label "Vector_Cartesian_Velocity_Spacecraft_Relative_To_Target";
  pds4:subClassOf pds4:urn:nasa:pds:0001_nasa_pds_1:geom:vector_cartesian_velocity_base:geom:vector_cartesian_velocity_extended_base::1.0;
  rdfs:comment "The Vector_Cartesian_Velocity_Spacecraft_Relative_To_Target is a velocity vector in rectangular coordinates that gives the velocity of the spacecraft with respect to the target specified in the parent Geometry_Orbiter class. While the class Coordinate_System_Identification is optional, it must be used here if the coordinate system has not been specified in the enclosing class. ".
 
pds4:urn:nasa:pds:0001_nasa_pds_1:geom:vector_cartesian_velocity_extended_base:geom:vector_cartesian_velocity_target_relative_to_central_body::1.0 rdf:type rdfs:Class;
  rdfs:label "Vector_Cartesian_Velocity_Target_Relative_To_Central_Body";
  pds4:subClassOf pds4:urn:nasa:pds:0001_nasa_pds_1:geom:vector_cartesian_velocity_base:geom:vector_cartesian_velocity_extended_base::1.0;
  rdfs:comment "The Vector_Cartesian_Velocity_Target_Relative_To_Central_Body is a velocity vector in rectangular coordinates that gives the velocity of the designated target with respect to the central body (e.g., planet). While the class Coordinate_System_Identification is optional, it must be used here if the coordinate system has not been specified in the enclosing class. ".
 
pds4:urn:nasa:pds:0001_nasa_pds_1:geom:vector_cartesian_velocity_extended_base:geom:vector_cartesian_velocity_target_relative_to_earth::1.0 rdf:type rdfs:Class;
  rdfs:label "Vector_Cartesian_Velocity_Target_Relative_To_Earth";
  pds4:subClassOf pds4:urn:nasa:pds:0001_nasa_pds_1:geom:vector_cartesian_velocity_base:geom:vector_cartesian_velocity_extended_base::1.0;
  rdfs:comment "The Vector_Cartesian_Velocity_Target_Relative_To_Earth is a velocity vector in rectangular coordinates that gives the velocity of the designated target with respect to Earth. While the class Coordinate_System_Identification is optional, it must be used here if the coordinate system has not been specified in the enclosing class. ".
 
pds4:urn:nasa:pds:0001_nasa_pds_1:geom:vector_cartesian_velocity_extended_base:geom:vector_cartesian_velocity_target_relative_to_ssb::1.0 rdf:type rdfs:Class;
  rdfs:label "Vector_Cartesian_Velocity_Target_Relative_To_SSB";
  pds4:subClassOf pds4:urn:nasa:pds:0001_nasa_pds_1:geom:vector_cartesian_velocity_base:geom:vector_cartesian_velocity_extended_base::1.0;
  rdfs:comment "The Vector_Cartesian_Velocity_Target_Relative_To_SSB is a velocity vector in rectangular coordinates that gives the velocity of the designated target with respect to the Solar System Barycenter. While the class Coordinate_System_Identification is optional, it must be used here if the coordinate system has not been specified in the enclosing class. ".
 
pds4:urn:nasa:pds:0001_nasa_pds_1:geom:vector_cartesian_velocity_extended_base:geom:vector_cartesian_velocity_target_relative_to_spacecraft::1.0 rdf:type rdfs:Class;
  rdfs:label "Vector_Cartesian_Velocity_Target_Relative_To_Spacecraft";
  pds4:subClassOf pds4:urn:nasa:pds:0001_nasa_pds_1:geom:vector_cartesian_velocity_base:geom:vector_cartesian_velocity_extended_base::1.0;
  rdfs:comment "The Vector_Cartesian_Velocity_Target_Relative_To_Spacecraft is a velocity vector in rectangular coordinates that gives the velocity of the designated target with respect to the spacecraft. While the class Coordinate_System_Identification is optional, it must be used here if the coordinate system has not been specified in the enclosing class. ".
 
pds4:urn:nasa:pds:0001_nasa_pds_1:geom:vector_cartesian_velocity_extended_base:geom:vector_cartesian_velocity_target_relative_to_sun::1.0 rdf:type rdfs:Class;
  rdfs:label "Vector_Cartesian_Velocity_Target_Relative_To_Sun";
  pds4:subClassOf pds4:urn:nasa:pds:0001_nasa_pds_1:geom:vector_cartesian_velocity_base:geom:vector_cartesian_velocity_extended_base::1.0;
  rdfs:comment " Vector_Cartesian_Velocity_Target_Relative_To_Sun is a velocity vector in rectangular coordinates that gives the velocity of the designated target with respect to the center of the sun. While the class Coordinate_System_Identification is optional, it must be used here if the coordinate system has not been specified in the enclosing class. ".
 
pds4:urn:nasa:pds:0001_nasa_pds_1:geom:vector_cartesian_position_base:geom:vector_center::1.0 rdf:type rdfs:Class;
  rdfs:label "Vector_Center";
  pds4:subClassOf pds4:urn:nasa:pds:0001_nasa_pds_1:all:user:geom:vector_cartesian_position_base::1.0;
  rdfs:comment "The Vector_Center describes the location of the entrance pupil of a camera. ".
 
pds4:urn:nasa:pds:0001_nasa_pds_1:pds:tagged_nondigital_child:pds:vector_component::1.0 rdf:type rdfs:Class;
  rdfs:label "Vector_Component";
  pds4:subClassOf pds4:urn:nasa:pds:0001_nasa_pds_1:all:user:pds:tagged_nondigital_child::1.0;
  rdfs:comment "The Vector_Component class provides a component of a vector.".
 
pds4:urn:nasa:pds:0001_nasa_pds_1:geom:vector_cartesian_unit:geom:vector_device_gravity::1.0 rdf:type rdfs:Class;
  rdfs:label "Vector_Device_Gravity";
  pds4:subClassOf pds4:urn:nasa:pds:0001_nasa_pds_1:all:user:geom:vector_cartesian_unit::1.0;
  rdfs:comment "The Vector_Device_Gravity class is a unit vector that specifies the direction of an external force acting on the articulation device, in the spacecraft\\'s coordinate system, at the time the pose was computed. ".
 
pds4:urn:nasa:pds:0001_nasa_pds_1:geom:vector_cartesian_acceleration_base:geom:vector_device_gravity_magnitude::1.0 rdf:type rdfs:Class;
  rdfs:label "Vector_Device_Gravity_Magnitude";
  pds4:subClassOf pds4:urn:nasa:pds:0001_nasa_pds_1:all:user:geom:vector_cartesian_acceleration_base::1.0;
  rdfs:comment "The Vector_Device_Gravity_Magnitude class is a vector (with magnitude) that specifies the direction of an external force acting on the articulation device, in the spacecraft\\'s coordinate system, at the time the pose was computed. ".
 
pds4:urn:nasa:pds:0001_nasa_pds_1:geom:vector_cartesian_pixel:geom:vector_horizontal::1.0 rdf:type rdfs:Class;
  rdfs:label "Vector_Horizontal";
  pds4:subClassOf pds4:urn:nasa:pds:0001_nasa_pds_1:all:user:geom:vector_cartesian_pixel::1.0;
  rdfs:comment "The Vector_Horizonal is a composite vector encoding three quantities: H\\' (a vector in the image plane perpendicular to the vertical columns), Hs (the distance between the lens center and image plane, measured in horizontal pixels), and Hc (the horizontal image coordinate directly under C when moving parallel to A). H\\' is often thought of as describing the orientation of rows in space, but is actually perpendicular to the columns. ".
 
pds4:urn:nasa:pds:0001_nasa_pds_1:all:user:cart:vector_length_base::1.0 rdf:type rdfs:Class;
  rdfs:label "Vector_Length_Base";
  pds4:subClassOf pds4:urn:nasa:pds:0001_nasa_pds_1:all:user::1.0;
  rdfs:comment "The Vector_Length_Base is an abstract class that forms the base of length-based x, y, z vectors.".
 
pds4:urn:nasa:pds:0001_nasa_pds_1:geom:vector_cartesian_no_units:geom:vector_model_transform::1.0 rdf:type rdfs:Class;
  rdfs:label "Vector_Model_Transform";
  pds4:subClassOf pds4:urn:nasa:pds:0001_nasa_pds_1:all:user:geom:vector_cartesian_no_units::1.0;
  rdfs:comment "The Vector_Model_Transform class specifies, along with the Quaternion_Model_Transform class, the transform used for the camera model in this image. Camera models created by the calibration process have associated with them a pose, comprised of the position (offset) and orientation (quaternion) of the camera at the time it was calibrated. The model is transformed (\"pointed\") for a specific image by computing, generally using articulation device kinematics, a final pose for the image. The camera model is then translated and rotated from the calibration to final pose. This class specifies the offset portion of the final pose. ".
 
pds4:urn:nasa:pds:0001_nasa_pds_1:geom:vector_cartesian_unit:geom:vector_normal_x::1.0 rdf:type rdfs:Class;
  rdfs:label "Vector_Normal_X";
  pds4:subClassOf pds4:urn:nasa:pds:0001_nasa_pds_1:all:user:geom:vector_cartesian_unit::1.0;
  rdfs:comment " Unit normal vector to the column plane when x equals zero, pointing in the same direction as the cross product of axis x with an outward-pointing vector that also lies in the plane. ".
 
pds4:urn:nasa:pds:0001_nasa_pds_1:geom:vector_cartesian_unit:geom:vector_normal_y::1.0 rdf:type rdfs:Class;
  rdfs:label "Vector_Normal_Y";
  pds4:subClassOf pds4:urn:nasa:pds:0001_nasa_pds_1:all:user:geom:vector_cartesian_unit::1.0;
  rdfs:comment " Unit normal vector to the row plane when y equals zero, pointing in the same direction as the cross product of axis x with an outward-pointing vector that also lies in the plane. ".
 
pds4:urn:nasa:pds:0001_nasa_pds_1:geom:vector_cartesian_unit:geom:vector_optical::1.0 rdf:type rdfs:Class;
  rdfs:label "Vector_Optical";
  pds4:subClassOf pds4:urn:nasa:pds:0001_nasa_pds_1:all:user:geom:vector_cartesian_unit::1.0;
  rdfs:comment "The Vector_Optical is a unit vector that describes the axis of symmetry for radial distortion in the camera. ".
 
pds4:urn:nasa:pds:0001_nasa_pds_1:geom:vector_cartesian_position_base:geom:vector_origin_offset::1.0 rdf:type rdfs:Class;
  rdfs:label "Vector_Origin_Offset";
  pds4:subClassOf pds4:urn:nasa:pds:0001_nasa_pds_1:all:user:geom:vector_cartesian_position_base::1.0;
  rdfs:comment "The Vector_Origin_Offset class contains attributes that specify the offset from the reference coordinate system\\'s origin to the origin of the coordinate system. It is the location of the current system\\'s origin as measured in the reference system. ".
 
pds4:urn:nasa:pds:0001_nasa_pds_1:all:user:geom:vector_planetocentric_position_base::1.0 rdf:type rdfs:Class;
  rdfs:label "Vector_Planetocentric_Position_Base";
  pds4:subClassOf pds4:urn:nasa:pds:0001_nasa_pds_1:all:user::1.0;
  rdfs:comment "The Vector_Planetocentric_Position_Base is a three dimensional spherical vector (radius, longitude, latitude) with the angular coordinates defined to be consistent with the Planetocentric coordinate system. Uses linear units for the radius dimension, and angular units for the other two dimensions. The included attributes are not sufficient to identify the endpoints of the vector. ".
 
pds4:urn:nasa:pds:0001_nasa_pds_1:geom:vector_planetocentric_position_extended_base:geom:vector_planetocentric_position_central_body_to_spacecraft::1.0 rdf:type rdfs:Class;
  rdfs:label "Vector_Planetocentric_Position_Central_Body_To_Spacecraft";
  pds4:subClassOf pds4:urn:nasa:pds:0001_nasa_pds_1:geom:vector_planetocentric_position_base:geom:vector_planetocentric_position_extended_base::1.0;
  rdfs:comment "The Vector_Planetocentric_Position_Central_Body_To_Spacecraft is a spherical position vector in Planetocentric coordinates. It extends from the center of mass of the central body (e.g., planet) to the spacecraft. While the class Coordinate_System_Identification is optional, it must be used here if the coordinate system has not been specified in the enclosing class. ".
 
pds4:urn:nasa:pds:0001_nasa_pds_1:geom:vector_planetocentric_position_extended_base:geom:vector_planetocentric_position_central_body_to_target::1.0 rdf:type rdfs:Class;
  rdfs:label "Vector_Planetocentric_Position_Central_Body_To_Target";
  pds4:subClassOf pds4:urn:nasa:pds:0001_nasa_pds_1:geom:vector_planetocentric_position_base:geom:vector_planetocentric_position_extended_base::1.0;
  rdfs:comment "The Vector_Planetocentric_Position_Central_Body_To_Target is a spherical position vector in Planetocentric coordinates. It extends from the center of mass of the central body (e.g., planet) to the target specified in the parent Geometry_Orbiter class. While the class Coordinate_System_Identification is optional, it must be used here if the coordinate system has not been specified in the enclosing class. ".
 
pds4:urn:nasa:pds:0001_nasa_pds_1:geom:vector_planetocentric_position_base:geom:vector_planetocentric_position_extended_base::1.0 rdf:type rdfs:Class;
  rdfs:label "Vector_Planetocentric_Position_Extended_Base";
  pds4:subClassOf pds4:urn:nasa:pds:0001_nasa_pds_1:all:user:geom:vector_planetocentric_position_base::1.0;
  rdfs:comment "The Vector_Planetocentric_Position_Extended_Base is a three dimensional spherical vector (radius, longitude, latitude) with the angular coordinates defined to be consistent with the Planetocentric coordinate system. Uses linear units for the radius dimension, and angular units for the other two dimensions. The included attributes are not sufficient to identify the endpoints of the vector. While the class Coordinate_System_Identification is optional, it must be used here if the coordinate system has not been specified in the enclosing class. ".
 
pds4:urn:nasa:pds:0001_nasa_pds_1:geom:vector_planetocentric_position_extended_base:geom:vector_planetocentric_position_generic::1.0 rdf:type rdfs:Class;
  rdfs:label "Vector_Planetocentric_Position_Generic";
  pds4:subClassOf pds4:urn:nasa:pds:0001_nasa_pds_1:geom:vector_planetocentric_position_base:geom:vector_planetocentric_position_extended_base::1.0;
  rdfs:comment "The Vector_Planetocentric_Position_Generic is a three dimensional spherical vector (radius, longitude, latitude) with the angular coordinates defined to be consistent with the Planetocentric coordinate system. Uses linear units for the radius dimension, and angular units for the other two dimensions. Includes attributes to identify the endpoints of the vector. While the class Coordinate_System_Identification is optional, it must be used here if the coordinate system has not been specified in the enclosing class. ".
 
pds4:urn:nasa:pds:0001_nasa_pds_1:geom:vector_planetocentric_position_extended_base:geom:vector_planetocentric_position_spacecraft_to_target::1.0 rdf:type rdfs:Class;
  rdfs:label "Vector_Planetocentric_Position_Spacecraft_To_Target";
  pds4:subClassOf pds4:urn:nasa:pds:0001_nasa_pds_1:geom:vector_planetocentric_position_base:geom:vector_planetocentric_position_extended_base::1.0;
  rdfs:comment "The Vector_Planetocentric_Position_Spacecraft_To_Target is a spherical position vector in Planetocentric coordinates. It extends from the spacecraft to the target specified in the parent Geometry_Orbiter class. While the class Coordinate_System_Identification is optional, it must be used here if the coordinate system has not been specified in the enclosing class. ".
 
pds4:urn:nasa:pds:0001_nasa_pds_1:all:user:geom:vector_planetocentric_velocity_base::1.0 rdf:type rdfs:Class;
  rdfs:label "Vector_Planetocentric_Velocity_Base";
  pds4:subClassOf pds4:urn:nasa:pds:0001_nasa_pds_1:all:user::1.0;
  rdfs:comment "The Vector_Planetocentric_Velocity_Base is a three dimensional spherical vector (radius, longitude, latitude) with the angular coordinates defined to be consistent with the Planetocentric coordinate system. Uses linear velocity units for the radius dimension, and angular velocity units for the other two dimensions. The included attributes are not sufficient to identify the endpoints of the vector. ".
 
pds4:urn:nasa:pds:0001_nasa_pds_1:geom:vector_planetocentric_velocity_base:geom:vector_planetocentric_velocity_extended_base::1.0 rdf:type rdfs:Class;
  rdfs:label "Vector_Planetocentric_Velocity_Extended_Base";
  pds4:subClassOf pds4:urn:nasa:pds:0001_nasa_pds_1:all:user:geom:vector_planetocentric_velocity_base::1.0;
  rdfs:comment "The Vector_Planetocentric_Velocity_Extended_Base is a three dimensional spherical vector (radius, longitude, latitude) with the angular coordinates defined to be consistent with the Planetocentric coordinate system. Uses linear velocity units for the radius dimension, and angular velocity units for the other two dimensions. The included attributes are not sufficient to identify the endpoints of the vector. While the class Coordinate_System_Identification is optional, it must be used here if the coordinate system has not been specified in the enclosing class. ".
 
pds4:urn:nasa:pds:0001_nasa_pds_1:geom:vector_planetocentric_velocity_extended_base:geom:vector_planetocentric_velocity_generic::1.0 rdf:type rdfs:Class;
  rdfs:label "Vector_Planetocentric_Velocity_Generic";
  pds4:subClassOf pds4:urn:nasa:pds:0001_nasa_pds_1:geom:vector_planetocentric_velocity_base:geom:vector_planetocentric_velocity_extended_base::1.0;
  rdfs:comment "The Vector_Planetocentric_Velocity_Generic is a three dimensional spherical vector (radius, longitude, latitude) with the angular coordinates defined to be consistent with the Planetocentric coordinate system. Uses linear velocity units for the radius dimension, and angular velocity units for the other two dimensions. Includes attributes to identify the endpoints of the vector. While the class Coordinate_System_Identification is optional, it must be used here if the coordinate system has not been specified in the enclosing class. ".
 
pds4:urn:nasa:pds:0001_nasa_pds_1:geom:vector_planetocentric_velocity_extended_base:geom:vector_planetocentric_velocity_spacecraft_relative_to_target::1.0 rdf:type rdfs:Class;
  rdfs:label "Vector_Planetocentric_Velocity_Spacecraft_Relative_To_Target";
  pds4:subClassOf pds4:urn:nasa:pds:0001_nasa_pds_1:geom:vector_planetocentric_velocity_base:geom:vector_planetocentric_velocity_extended_base::1.0;
  rdfs:comment "The Vector_Planetocentric_Velocity_Spacecraft_Relative_To_Target is a spherical velocity vector in Planetocentric coordinates that gives the velocity of the spacecraft with respect to the designated target. While the class Coordinate_System_Identification is optional, it must be used here if the coordinate system has not been specified in the enclosing class. ".
 
pds4:urn:nasa:pds:0001_nasa_pds_1:geom:vector_planetocentric_velocity_extended_base:geom:vector_planetocentric_velocity_target_relative_to_central_body::1.0 rdf:type rdfs:Class;
  rdfs:label "Vector_Planetocentric_Velocity_Target_Relative_To_Central_Body";
  pds4:subClassOf pds4:urn:nasa:pds:0001_nasa_pds_1:geom:vector_planetocentric_velocity_base:geom:vector_planetocentric_velocity_extended_base::1.0;
  rdfs:comment "The Vector_Planetocentric_Velocity_Target_Relative_To_Central_Body is a spherical velocity vector in Planetocentric coordinates that gives the velocity of the target with respect to the central body. While the class Coordinate_System_Identification is optional, it must be used here if the coordinate system has not been specified in the enclosing class. ".
 
pds4:urn:nasa:pds:0001_nasa_pds_1:geom:vector_planetocentric_velocity_extended_base:geom:vector_planetocentric_velocity_target_relative_to_spacecraft::1.0 rdf:type rdfs:Class;
  rdfs:label "Vector_Planetocentric_Velocity_Target_Relative_To_Spacecraft";
  pds4:subClassOf pds4:urn:nasa:pds:0001_nasa_pds_1:geom:vector_planetocentric_velocity_base:geom:vector_planetocentric_velocity_extended_base::1.0;
  rdfs:comment "The Vector_Planetocentric_Velocity_Target_Relative_To_Spacecraft is a spherical velocity vector in Planetocentric coordinates that gives the velocity of the target with respect to the spacecraft. While the class Coordinate_System_Identification is optional, it must be used here if the coordinate system has not been specified in the enclosing class. ".
 
pds4:urn:nasa:pds:0001_nasa_pds_1:geom:vector_cartesian_position_base:cart:vector_projection_origin::1.0 rdf:type rdfs:Class;
  rdfs:label "Vector_Projection_Origin";
  pds4:subClassOf pds4:urn:nasa:pds:0001_nasa_pds_1:all:user:geom:vector_cartesian_position_base::1.0;
  rdfs:comment "The Vector_Projection_Origin class specifies the location of the origin of the projection. For Polar and Cylindrical projections, this is the XYZ point from which all the azimuth\\//elevation rays emanate. For the Cylindrical-Perspective projection, this defines the center of the circle around which the synthetic camera orbits. For Orthographic, Orthorectified, and Vertical projections, this optional keyword specifies the point on the projection plane that serves as the origin of the projection (i.e. all points on a line through this point in the direction of PROJECTION_Z_AXIS_VECTOR will be located at X=Y=0 in the projection). If not present, (0,0,0) should be assumed. This translation is generally not necessary and not often used; the (X|Y)_AXIS_MINIMUM and (X|Y)_AXIS_MAXIMUM fields allow the mosaic to be located arbitrarily in the projection plane.".
 
pds4:urn:nasa:pds:0001_nasa_pds_1:cart:vector_cartesian_unit_base:cart:vector_projection_x_axis::1.0 rdf:type rdfs:Class;
  rdfs:label "Vector_Projection_X_Axis";
  pds4:subClassOf pds4:urn:nasa:pds:0001_nasa_pds_1:all:user:cart:vector_cartesian_unit_base::1.0;
  rdfs:comment "The Vector_Projection_X_Axis class specifies a unit vector defining the X-axis for a given projection. For Orthographic, Orthorectified, and Vertical projections, this vector defines how the * axis in the mosaic is oriented in space. The X and Y axis vectors together define the rotation of the projection plane around the projection axis.".
 
pds4:urn:nasa:pds:0001_nasa_pds_1:cart:vector_cartesian_unit_base:cart:vector_projection_y_axis::1.0 rdf:type rdfs:Class;
  rdfs:label "Vector_Projection_Y_Axis";
  pds4:subClassOf pds4:urn:nasa:pds:0001_nasa_pds_1:all:user:cart:vector_cartesian_unit_base::1.0;
  rdfs:comment "The Vector_Projection_Y_Axis class specifies a unit vector defining the Y-axis for a given projection. For Orthographic, Orthorectified, and Vertical projections, this vector defines how the * axis in the mosaic is oriented in space. The X and Y axis vectors together define the rotation of the projection plane around the projection axis.".
 
pds4:urn:nasa:pds:0001_nasa_pds_1:cart:vector_cartesian_unit_base:cart:vector_projection_z_axis::1.0 rdf:type rdfs:Class;
  rdfs:label "Vector_Projection_Z_Axis";
  pds4:subClassOf pds4:urn:nasa:pds:0001_nasa_pds_1:all:user:cart:vector_cartesian_unit_base::1.0;
  rdfs:comment "The Vector_Projection_Z_Axis class specifies a unit vector defining the Z axis for a given projection. For Orthographic, Orthorectified, and Vertical projections, this vector defines the projection axis for the mosaic. All points along a line parallel to this axis are projected to the same spot in the projection plane. For the Cylindrical-Perspective projections, this defines the new axis of the circle around which the synthetic camera orbits (i.e. the normal to the circle), after the cameras have been rotated to correct for rover tilt. Vector_Projection_Z_Axis_Initial contains the axis before rotation; the difference in these two indicate the rotation amount.".
 
pds4:urn:nasa:pds:0001_nasa_pds_1:cart:vector_cartesian_unit_base:cart:vector_projection_z_axis_initial::1.0 rdf:type rdfs:Class;
  rdfs:label "Vector_Projection_Z_Axis_Initial";
  pds4:subClassOf pds4:urn:nasa:pds:0001_nasa_pds_1:all:user:cart:vector_cartesian_unit_base::1.0;
  rdfs:comment "The Vector_Projection_Z_Axis_Initial class specifies the initial unit vector defining the Z axis for a given projection. For Cylindrical-Perspective projections, this defines the original axis of the circle around which the synthetic camera orbits, before the cameras have been rotated to correct for rover tilt. Vector_Projection_Z_Axis contains the axis after rotation; the difference in these two indicate the rotation amount.".
 
pds4:urn:nasa:pds:0001_nasa_pds_1:all:user:img_surface:vector_range_origin::1.0 rdf:type rdfs:Class;
  rdfs:label "Vector_Range_Origin";
  pds4:subClassOf pds4:urn:nasa:pds:0001_nasa_pds_1:all:user::1.0;
  rdfs:comment "The Vector_Range_Origin class specifies the 3-D space from which the Range values are measured in a Range RDR. This will normally be the same as the C point of the camera. It is expressed in the coordinate system specified by the Coordinate_Space_Reference class.".
 
pds4:urn:nasa:pds:0001_nasa_pds_1:geom:vector_cartesian_unit:geom:vector_solar_direction::1.0 rdf:type rdfs:Class;
  rdfs:label "Vector_Solar_Direction";
  pds4:subClassOf pds4:urn:nasa:pds:0001_nasa_pds_1:all:user:geom:vector_cartesian_unit::1.0;
  rdfs:comment " Unit vector pointing in the direction of the Sun at the time of the observation. ".
 
pds4:urn:nasa:pds:0001_nasa_pds_1:geom:vector_cartesian_position_base:cart:vector_sphere_center::1.0 rdf:type rdfs:Class;
  rdfs:label "Vector_Sphere_Center";
  pds4:subClassOf pds4:urn:nasa:pds:0001_nasa_pds_1:all:user:geom:vector_cartesian_position_base::1.0;
  rdfs:comment "The Vector_Sphere_Center class specifies the center of the sphere. This point is measured in the coordinates specified by the Coordinate_Space reference in the Surface_Model_Parameters class.".
 
pds4:urn:nasa:pds:0001_nasa_pds_1:geom:vector_cartesian_position_base:cart:vector_surface_ground_location::1.0 rdf:type rdfs:Class;
  rdfs:label "Vector_Surface_Ground_Location";
  pds4:subClassOf pds4:urn:nasa:pds:0001_nasa_pds_1:all:user:geom:vector_cartesian_position_base::1.0;
  rdfs:comment "The Vector_Surface_Ground_Location class specifies any point on the surface model, in order to fix the model in space. This point is measured in the coordinates specified by the Coordinate_Space reference in the Surface_Model_Parameters class.".
 
pds4:urn:nasa:pds:0001_nasa_pds_1:cart:vector_cartesian_unit_base:cart:vector_surface_normal::1.0 rdf:type rdfs:Class;
  rdfs:label "Vector_Surface_Normal";
  pds4:subClassOf pds4:urn:nasa:pds:0001_nasa_pds_1:all:user:cart:vector_cartesian_unit_base::1.0;
  rdfs:comment "The Vector_Surface_Normal class specifies a vector normal to the planar surface model. This vector is measured in the coordinates specified by the Coordinate_Space reference in the Surface_Model_Parameters class.".
 
pds4:urn:nasa:pds:0001_nasa_pds_1:geom:vector_cartesian_pixel:geom:vector_vertical::1.0 rdf:type rdfs:Class;
  rdfs:label "Vector_Vertical";
  pds4:subClassOf pds4:urn:nasa:pds:0001_nasa_pds_1:all:user:geom:vector_cartesian_pixel::1.0;
  rdfs:comment "The Vector_Vertical is a composite vector encoding three quantities: V\\' (a vector in the image plane perpendicular to the horizontal rows), Vs (the distance between the lens center and image plane, measured in vertical pixels), and Vc (the vertical image coordinate directly under C when moving parallel to A). V\\' is often thought of as describing the orientation of columns in space, but is actually perpendicular to the rows. ".
 
pds4:urn:nasa:pds:0001_nasa_pds_1:all:user:geom:vectors::1.0 rdf:type rdfs:Class;
  rdfs:label "Vectors";
  pds4:subClassOf pds4:urn:nasa:pds:0001_nasa_pds_1:all:user::1.0;
  rdfs:comment "The Vectors class is a container of vector classes. ".
 
pds4:urn:nasa:pds:0001_nasa_pds_1:all:user:geom:vectors_cartesian_specific::1.0 rdf:type rdfs:Class;
  rdfs:label "Vectors_Cartesian_Specific";
  pds4:subClassOf pds4:urn:nasa:pds:0001_nasa_pds_1:all:user::1.0;
  rdfs:comment "The Vectors_Cartesian_Specific class is a container class for all cartesian vectors with pre-identified endpoints. ".
 
pds4:urn:nasa:pds:0001_nasa_pds_1:all:user:geom:vectors_planetocentric_specific::1.0 rdf:type rdfs:Class;
  rdfs:label "Vectors_Planetocentric_Specific";
  pds4:subClassOf pds4:urn:nasa:pds:0001_nasa_pds_1:all:user::1.0;
  rdfs:comment "The Vectors_Planetocentric_Specific class is a container class for all planetocentric vectors with pre-identified endpoints. ".
 
pds4:urn:nasa:pds:0001_nasa_pds_1:all:user:cart:vertical::1.0 rdf:type rdfs:Class;
  rdfs:label "Vertical";
  pds4:subClassOf pds4:urn:nasa:pds:0001_nasa_pds_1:all:user::1.0;
  rdfs:comment "This is an in-situ projection that provides an overhead view. By projecting to a surface model, the need for range data is eliminated, but significant layover effects can happen when the actual geometry does not match the surface model. It has a constant scale in meters\\//pixel, subject to layover distortion.".
 
pds4:urn:nasa:pds:0001_nasa_pds_1:all:user:img:video::1.0 rdf:type rdfs:Class;
  rdfs:label "Video";
  pds4:subClassOf pds4:urn:nasa:pds:0001_nasa_pds_1:all:user::1.0;
  rdfs:comment "The Video class contains attributes related to video observations, defined as a regular time series of frames. The class can be used to describe a single frame within the video, or the video as a whole.".
 
pds4:urn:nasa:pds:0001_nasa_pds_1:pds:tndo_context_pds3:pds:volume_pds3::1.0 rdf:type rdfs:Class;
  rdfs:label "Volume_PDS3";
  pds4:subClassOf pds4:urn:nasa:pds:0001_nasa_pds_1:pds:tagged_nondigital_object:pds:tndo_context_pds3::1.0;
  rdfs:comment "The Volume_PDS3 class is used to capture the volume information from the PDS3 Data Set Catalog.".
 
pds4:urn:nasa:pds:0001_nasa_pds_1:pds:tndo_context_pds3:pds:volume_set_pds3::1.0 rdf:type rdfs:Class;
  rdfs:label "Volume_Set_PDS3";
  pds4:subClassOf pds4:urn:nasa:pds:0001_nasa_pds_1:pds:tagged_nondigital_object:pds:tndo_context_pds3::1.0;
  rdfs:comment "The Volume_Set_PDS3 class is used to capture the volume set information from the PDS3 Data Set Catalog.".
 
pds4:urn:nasa:pds:0001_nasa_pds_1:pds:parsable_byte_stream:pds:xml_schema::1.0 rdf:type rdfs:Class;
  rdfs:label "XML_Schema";
  pds4:subClassOf pds4:urn:nasa:pds:0001_nasa_pds_1:pds:byte_stream:pds:parsable_byte_stream::1.0;
  rdfs:comment "The XML Schema class defines a resource used for the PDS4 implementation into XML.".
 
pds4:urn:nasa:pds:0001_nasa_pds_1:pds:tndo_supplemental:pds:zip::1.0 rdf:type rdfs:Class;
  rdfs:label "Zip";
  pds4:subClassOf pds4:urn:nasa:pds:0001_nasa_pds_1:pds:tagged_nondigital_object:pds:tndo_supplemental::1.0;
  rdfs:comment "The Zip class describes a zip file.".
 
pds4:urn:nasa:pds:0001_nasa_pds_1:pds:product:pds:product_attribute_definition::attribute_to_image:1.0 rdf:type rdf:Property;
  rdfs:label "attribute_to_image";
  rdfs:domain pds4:urn:nasa:pds:0001_nasa_pds_1:pds:product:pds:product_attribute_definition::1.0;
  rdfs:range pds4:urn:nasa:pds:0001_nasa_pds_1:pds:product:pds:product_observational::1.0.
 
pds4:urn:nasa:pds:0001_nasa_pds_1:pds:product:pds:product_attribute_definition::attribute_to_document:1.0 rdf:type rdf:Property;
  rdfs:label "attribute_to_document";
  rdfs:domain pds4:urn:nasa:pds:0001_nasa_pds_1:pds:product:pds:product_attribute_definition::1.0;
  rdfs:range pds4:urn:nasa:pds:0001_nasa_pds_1:pds:product:pds:product_document::1.0.
 
pds4:urn:nasa:pds:0001_nasa_pds_1:pds:product:pds:product_class_definition::class_to_image:1.0 rdf:type rdf:Property;
  rdfs:label "class_to_image";
  rdfs:domain pds4:urn:nasa:pds:0001_nasa_pds_1:pds:product:pds:product_class_definition::1.0;
  rdfs:range pds4:urn:nasa:pds:0001_nasa_pds_1:pds:product:pds:product_observational::1.0.
 
pds4:urn:nasa:pds:0001_nasa_pds_1:pds:product:pds:product_class_definition::class_to_document:1.0 rdf:type rdf:Property;
  rdfs:label "class_to_document";
  rdfs:domain pds4:urn:nasa:pds:0001_nasa_pds_1:pds:product:pds:product_class_definition::1.0;
  rdfs:range pds4:urn:nasa:pds:0001_nasa_pds_1:pds:product:pds:product_document::1.0.
 
pds4:urn:nasa:pds:0001_nasa_pds_1:pds:product:pds:product_aip::package_has_collection:1.0 rdf:type rdf:Property;
  rdfs:label "package_has_collection";
  rdfs:domain pds4:urn:nasa:pds:0001_nasa_pds_1:pds:product:pds:product_aip::1.0;
  rdfs:range pds4:urn:nasa:pds:0001_nasa_pds_1:pds:product:pds:product_collection::1.0.
 
pds4:urn:nasa:pds:0001_nasa_pds_1:pds:product:pds:product_aip::package_has_bundle:1.0 rdf:type rdf:Property;
  rdfs:label "package_has_bundle";
  rdfs:domain pds4:urn:nasa:pds:0001_nasa_pds_1:pds:product:pds:product_aip::1.0;
  rdfs:range pds4:urn:nasa:pds:0001_nasa_pds_1:pds:product:pds:product_bundle::1.0.
 
pds4:urn:nasa:pds:0001_nasa_pds_1:pds:product:pds:product_aip::package_has_product:1.0 rdf:type rdf:Property;
  rdfs:label "package_has_product";
  rdfs:domain pds4:urn:nasa:pds:0001_nasa_pds_1:pds:product:pds:product_aip::1.0;
  rdfs:range pds4:urn:nasa:pds:0001_nasa_pds_1:pds:product:pds:product_observational::1.0.
 
pds4:urn:nasa:pds:0001_nasa_pds_1:pds:product:pds:product_aip::package_compiled_from_package:1.0 rdf:type rdf:Property;
  rdfs:label "package_compiled_from_package";
  rdfs:domain pds4:urn:nasa:pds:0001_nasa_pds_1:pds:product:pds:product_aip::1.0;
  rdfs:range pds4:urn:nasa:pds:0001_nasa_pds_1:pds:product:pds:product_aip::1.0.
 
pds4:urn:nasa:pds:0001_nasa_pds_1:pds:product:pds:product_ancillary::ancillary_to_investigation:1.0 rdf:type rdf:Property;
  rdfs:label "ancillary_to_investigation";
  rdfs:domain pds4:urn:nasa:pds:0001_nasa_pds_1:pds:product:pds:product_ancillary::1.0;
  rdfs:range pds4:urn:nasa:pds:0001_nasa_pds_1:pds:tndo_context:pds:investigation::1.0.
 
pds4:urn:nasa:pds:0001_nasa_pds_1:pds:product:pds:product_ancillary::ancillary_to_target:1.0 rdf:type rdf:Property;
  rdfs:label "ancillary_to_target";
  rdfs:domain pds4:urn:nasa:pds:0001_nasa_pds_1:pds:product:pds:product_ancillary::1.0;
  rdfs:range pds4:urn:nasa:pds:0001_nasa_pds_1:pds:tndo_context:pds:target::1.0.
 
pds4:urn:nasa:pds:0001_nasa_pds_1:pds:product:pds:product_ancillary::ancillary_to_data:1.0 rdf:type rdf:Property;
  rdfs:label "ancillary_to_data";
  rdfs:domain pds4:urn:nasa:pds:0001_nasa_pds_1:pds:product:pds:product_ancillary::1.0;
  rdfs:range pds4:urn:nasa:pds:0001_nasa_pds_1:pds:product:pds:product_observational::1.0.
 
pds4:urn:nasa:pds:0001_nasa_pds_1:pds:product:pds:product_ancillary::ancillary_to_document:1.0 rdf:type rdf:Property;
  rdfs:label "ancillary_to_document";
  rdfs:domain pds4:urn:nasa:pds:0001_nasa_pds_1:pds:product:pds:product_ancillary::1.0;
  rdfs:range pds4:urn:nasa:pds:0001_nasa_pds_1:pds:product:pds:product_document::1.0.
 
pds4:urn:nasa:pds:0001_nasa_pds_1:pds:product:pds:product_ancillary::ancillary_to_browse:1.0 rdf:type rdf:Property;
  rdfs:label "ancillary_to_browse";
  rdfs:domain pds4:urn:nasa:pds:0001_nasa_pds_1:pds:product:pds:product_ancillary::1.0;
  rdfs:range pds4:urn:nasa:pds:0001_nasa_pds_1:pds:product:pds:product_browse::1.0.
 
pds4:urn:nasa:pds:0001_nasa_pds_1:pds:product:pds:product_browse::browse_to_data:1.0 rdf:type rdf:Property;
  rdfs:label "browse_to_data";
  rdfs:domain pds4:urn:nasa:pds:0001_nasa_pds_1:pds:product:pds:product_browse::1.0;
  rdfs:range pds4:urn:nasa:pds:0001_nasa_pds_1:pds:product:pds:product_observational::1.0.
 
pds4:urn:nasa:pds:0001_nasa_pds_1:pds:product:pds:product_browse::browse_to_thumbnail:1.0 rdf:type rdf:Property;
  rdfs:label "browse_to_thumbnail";
  rdfs:domain pds4:urn:nasa:pds:0001_nasa_pds_1:pds:product:pds:product_browse::1.0;
  rdfs:range pds4:urn:nasa:pds:0001_nasa_pds_1:pds:product:pds:product_thumbnail::1.0.
 
pds4:urn:nasa:pds:0001_nasa_pds_1:pds:product:pds:product_browse::browse_to_browse:1.0 rdf:type rdf:Property;
  rdfs:label "browse_to_browse";
  rdfs:domain pds4:urn:nasa:pds:0001_nasa_pds_1:pds:product:pds:product_browse::1.0;
  rdfs:range pds4:urn:nasa:pds:0001_nasa_pds_1:pds:product:pds:product_browse::1.0.
 
pds4:urn:nasa:pds:0001_nasa_pds_1:pds:product:pds:product_browse::browse_to_document:1.0 rdf:type rdf:Property;
  rdfs:label "browse_to_document";
  rdfs:domain pds4:urn:nasa:pds:0001_nasa_pds_1:pds:product:pds:product_browse::1.0;
  rdfs:range pds4:urn:nasa:pds:0001_nasa_pds_1:pds:product:pds:product_document::1.0.
 
pds4:urn:nasa:pds:0001_nasa_pds_1:pds:product:pds:product_browse::browse_to_ancillary:1.0 rdf:type rdf:Property;
  rdfs:label "browse_to_ancillary";
  rdfs:domain pds4:urn:nasa:pds:0001_nasa_pds_1:pds:product:pds:product_browse::1.0;
  rdfs:range pds4:urn:nasa:pds:0001_nasa_pds_1:pds:product:pds:product_ancillary::1.0.
 
pds4:urn:nasa:pds:0001_nasa_pds_1:pds:product:pds:product_bundle::bundle_to_investigation:1.0 rdf:type rdf:Property;
  rdfs:label "bundle_to_investigation";
  rdfs:domain pds4:urn:nasa:pds:0001_nasa_pds_1:pds:product:pds:product_bundle::1.0;
  rdfs:range pds4:urn:nasa:pds:0001_nasa_pds_1:pds:tndo_context:pds:investigation::1.0.
 
pds4:urn:nasa:pds:0001_nasa_pds_1:pds:product:pds:product_bundle::bundle_to_errata:1.0 rdf:type rdf:Property;
  rdfs:label "bundle_to_errata";
  rdfs:domain pds4:urn:nasa:pds:0001_nasa_pds_1:pds:product:pds:product_bundle::1.0;
  rdfs:range pds4:urn:nasa:pds:0001_nasa_pds_1:pds:product:pds:product_document::1.0.
 
pds4:urn:nasa:pds:0001_nasa_pds_1:pds:product:pds:product_bundle::bundle_to_document:1.0 rdf:type rdf:Property;
  rdfs:label "bundle_to_document";
  rdfs:domain pds4:urn:nasa:pds:0001_nasa_pds_1:pds:product:pds:product_bundle::1.0;
  rdfs:range pds4:urn:nasa:pds:0001_nasa_pds_1:pds:product:pds:product_document::1.0.
 
pds4:urn:nasa:pds:0001_nasa_pds_1:pds:product:pds:product_bundle::bundle_to_investigation:1.0 rdf:type rdf:Property;
  rdfs:label "bundle_to_investigation";
  rdfs:domain pds4:urn:nasa:pds:0001_nasa_pds_1:pds:product:pds:product_bundle::1.0;
  rdfs:range pds4:urn:nasa:pds:0001_nasa_pds_1:pds:tndo_context:pds:investigation::1.0.
 
pds4:urn:nasa:pds:0001_nasa_pds_1:pds:product:pds:product_bundle::bundle_to_instrument:1.0 rdf:type rdf:Property;
  rdfs:label "bundle_to_instrument";
  rdfs:domain pds4:urn:nasa:pds:0001_nasa_pds_1:pds:product:pds:product_bundle::1.0;
  rdfs:range pds4:urn:nasa:pds:0001_nasa_pds_1:pds:tndo_context:pds:instrument::1.0.
 
pds4:urn:nasa:pds:0001_nasa_pds_1:pds:product:pds:product_bundle::bundle_to_instrument_host:1.0 rdf:type rdf:Property;
  rdfs:label "bundle_to_instrument_host";
  rdfs:domain pds4:urn:nasa:pds:0001_nasa_pds_1:pds:product:pds:product_bundle::1.0;
  rdfs:range pds4:urn:nasa:pds:0001_nasa_pds_1:pds:tndo_context:pds:instrument_host::1.0.
 
pds4:urn:nasa:pds:0001_nasa_pds_1:pds:product:pds:product_bundle::bundle_to_target:1.0 rdf:type rdf:Property;
  rdfs:label "bundle_to_target";
  rdfs:domain pds4:urn:nasa:pds:0001_nasa_pds_1:pds:product:pds:product_bundle::1.0;
  rdfs:range pds4:urn:nasa:pds:0001_nasa_pds_1:pds:tndo_context:pds:target::1.0.
 
pds4:urn:nasa:pds:0001_nasa_pds_1:pds:product:pds:product_bundle::bundle_to_resource:1.0 rdf:type rdf:Property;
  rdfs:label "bundle_to_resource";
  rdfs:domain pds4:urn:nasa:pds:0001_nasa_pds_1:pds:product:pds:product_bundle::1.0;
  rdfs:range pds4:urn:nasa:pds:0001_nasa_pds_1:pds:tndo_context:pds:resource::1.0.
 
pds4:urn:nasa:pds:0001_nasa_pds_1:pds:product:pds:product_bundle::bundle_to_associate:1.0 rdf:type rdf:Property;
  rdfs:label "bundle_to_associate";
  rdfs:domain pds4:urn:nasa:pds:0001_nasa_pds_1:pds:product:pds:product_bundle::1.0;
  rdfs:range pds4:urn:nasa:pds:0001_nasa_pds_1:all:user:pds:product::1.0.
 
pds4:urn:nasa:pds:0001_nasa_pds_1:pds:product:pds:product_collection::collection_to_investigation:1.0 rdf:type rdf:Property;
  rdfs:label "collection_to_investigation";
  rdfs:domain pds4:urn:nasa:pds:0001_nasa_pds_1:pds:product:pds:product_collection::1.0;
  rdfs:range pds4:urn:nasa:pds:0001_nasa_pds_1:pds:tndo_context:pds:investigation::1.0.
 
pds4:urn:nasa:pds:0001_nasa_pds_1:pds:product:pds:product_collection::collection_to_resource:1.0 rdf:type rdf:Property;
  rdfs:label "collection_to_resource";
  rdfs:domain pds4:urn:nasa:pds:0001_nasa_pds_1:pds:product:pds:product_collection::1.0;
  rdfs:range pds4:urn:nasa:pds:0001_nasa_pds_1:pds:tndo_context:pds:resource::1.0.
 
pds4:urn:nasa:pds:0001_nasa_pds_1:pds:product:pds:product_collection::collection_to_associate:1.0 rdf:type rdf:Property;
  rdfs:label "collection_to_associate";
  rdfs:domain pds4:urn:nasa:pds:0001_nasa_pds_1:pds:product:pds:product_collection::1.0;
  rdfs:range pds4:urn:nasa:pds:0001_nasa_pds_1:all:user:pds:product::1.0.
 
pds4:urn:nasa:pds:0001_nasa_pds_1:pds:product:pds:product_collection::collection_to_calibration:1.0 rdf:type rdf:Property;
  rdfs:label "collection_to_calibration";
  rdfs:domain pds4:urn:nasa:pds:0001_nasa_pds_1:pds:product:pds:product_collection::1.0;
  rdfs:range pds4:urn:nasa:pds:0001_nasa_pds_1:pds:product:pds:product_metadata_supplemental::1.0.
 
pds4:urn:nasa:pds:0001_nasa_pds_1:pds:product:pds:product_collection::collection_to_geometry:1.0 rdf:type rdf:Property;
  rdfs:label "collection_to_geometry";
  rdfs:domain pds4:urn:nasa:pds:0001_nasa_pds_1:pds:product:pds:product_collection::1.0;
  rdfs:range pds4:urn:nasa:pds:0001_nasa_pds_1:pds:product:pds:product_metadata_supplemental::1.0.
 
pds4:urn:nasa:pds:0001_nasa_pds_1:pds:product:pds:product_collection::collection_to_spice_kernel:1.0 rdf:type rdf:Property;
  rdfs:label "collection_to_spice_kernel";
  rdfs:domain pds4:urn:nasa:pds:0001_nasa_pds_1:pds:product:pds:product_collection::1.0;
  rdfs:range pds4:urn:nasa:pds:0001_nasa_pds_1:pds:product:pds:product_spice_kernel::1.0.
 
pds4:urn:nasa:pds:0001_nasa_pds_1:pds:product:pds:product_collection::collection_curated_by_node:1.0 rdf:type rdf:Property;
  rdfs:label "collection_curated_by_node";
  rdfs:domain pds4:urn:nasa:pds:0001_nasa_pds_1:pds:product:pds:product_collection::1.0;
  rdfs:range pds4:urn:nasa:pds:0001_nasa_pds_1:pds:tndo_context:pds:node::1.0.
 
pds4:urn:nasa:pds:0001_nasa_pds_1:pds:product:pds:product_collection::collection_to_document:1.0 rdf:type rdf:Property;
  rdfs:label "collection_to_document";
  rdfs:domain pds4:urn:nasa:pds:0001_nasa_pds_1:pds:product:pds:product_collection::1.0;
  rdfs:range pds4:urn:nasa:pds:0001_nasa_pds_1:pds:product:pds:product_document::1.0.
 
pds4:urn:nasa:pds:0001_nasa_pds_1:pds:product:pds:product_collection::collection_to_browse:1.0 rdf:type rdf:Property;
  rdfs:label "collection_to_browse";
  rdfs:domain pds4:urn:nasa:pds:0001_nasa_pds_1:pds:product:pds:product_collection::1.0;
  rdfs:range pds4:urn:nasa:pds:0001_nasa_pds_1:pds:product:pds:product_browse::1.0.
 
pds4:urn:nasa:pds:0001_nasa_pds_1:pds:product:pds:product_collection::collection_to_context:1.0 rdf:type rdf:Property;
  rdfs:label "collection_to_context";
  rdfs:domain pds4:urn:nasa:pds:0001_nasa_pds_1:pds:product:pds:product_collection::1.0;
  rdfs:range pds4:urn:nasa:pds:0001_nasa_pds_1:pds:product:pds:product_context::1.0.
 
pds4:urn:nasa:pds:0001_nasa_pds_1:pds:product:pds:product_collection::collection_to_data:1.0 rdf:type rdf:Property;
  rdfs:label "collection_to_data";
  rdfs:domain pds4:urn:nasa:pds:0001_nasa_pds_1:pds:product:pds:product_collection::1.0;
  rdfs:range pds4:urn:nasa:pds:0001_nasa_pds_1:pds:product:pds:product_observational::1.0.
 
pds4:urn:nasa:pds:0001_nasa_pds_1:pds:product:pds:product_collection::collection_to_ancillary:1.0 rdf:type rdf:Property;
  rdfs:label "collection_to_ancillary";
  rdfs:domain pds4:urn:nasa:pds:0001_nasa_pds_1:pds:product:pds:product_collection::1.0;
  rdfs:range pds4:urn:nasa:pds:0001_nasa_pds_1:pds:product:pds:product_ancillary::1.0.
 
pds4:urn:nasa:pds:0001_nasa_pds_1:pds:product:pds:product_collection::collection_to_schema:1.0 rdf:type rdf:Property;
  rdfs:label "collection_to_schema";
  rdfs:domain pds4:urn:nasa:pds:0001_nasa_pds_1:pds:product:pds:product_collection::1.0;
  rdfs:range pds4:urn:nasa:pds:0001_nasa_pds_1:pds:product:pds:product_xml_schema::1.0.
 
pds4:urn:nasa:pds:0001_nasa_pds_1:pds:product:pds:product_collection::collection_to_errata:1.0 rdf:type rdf:Property;
  rdfs:label "collection_to_errata";
  rdfs:domain pds4:urn:nasa:pds:0001_nasa_pds_1:pds:product:pds:product_collection::1.0;
  rdfs:range pds4:urn:nasa:pds:0001_nasa_pds_1:pds:product:pds:product_document::1.0.
 
pds4:urn:nasa:pds:0001_nasa_pds_1:pds:product:pds:product_collection::collection_to_bundle:1.0 rdf:type rdf:Property;
  rdfs:label "collection_to_bundle";
  rdfs:domain pds4:urn:nasa:pds:0001_nasa_pds_1:pds:product:pds:product_collection::1.0;
  rdfs:range pds4:urn:nasa:pds:0001_nasa_pds_1:pds:product:pds:product_bundle::1.0.
 
pds4:urn:nasa:pds:0001_nasa_pds_1:pds:product:pds:product_collection::collection_to_personnel:1.0 rdf:type rdf:Property;
  rdfs:label "collection_to_personnel";
  rdfs:domain pds4:urn:nasa:pds:0001_nasa_pds_1:pds:product:pds:product_collection::1.0;
  rdfs:range pds4:urn:nasa:pds:0001_nasa_pds_1:pds:tndo_context:pds:pds_affiliate::1.0.
 
pds4:urn:nasa:pds:0001_nasa_pds_1:pds:product:pds:product_collection::collection_to_investigation:1.0 rdf:type rdf:Property;
  rdfs:label "collection_to_investigation";
  rdfs:domain pds4:urn:nasa:pds:0001_nasa_pds_1:pds:product:pds:product_collection::1.0;
  rdfs:range pds4:urn:nasa:pds:0001_nasa_pds_1:pds:tndo_context:pds:investigation::1.0.
 
pds4:urn:nasa:pds:0001_nasa_pds_1:pds:product:pds:product_collection::collection_to_instrument:1.0 rdf:type rdf:Property;
  rdfs:label "collection_to_instrument";
  rdfs:domain pds4:urn:nasa:pds:0001_nasa_pds_1:pds:product:pds:product_collection::1.0;
  rdfs:range pds4:urn:nasa:pds:0001_nasa_pds_1:pds:tndo_context:pds:instrument::1.0.
 
pds4:urn:nasa:pds:0001_nasa_pds_1:pds:product:pds:product_collection::collection_to_instrument_host:1.0 rdf:type rdf:Property;
  rdfs:label "collection_to_instrument_host";
  rdfs:domain pds4:urn:nasa:pds:0001_nasa_pds_1:pds:product:pds:product_collection::1.0;
  rdfs:range pds4:urn:nasa:pds:0001_nasa_pds_1:pds:tndo_context:pds:instrument_host::1.0.
 
pds4:urn:nasa:pds:0001_nasa_pds_1:pds:product:pds:product_collection::collection_to_target:1.0 rdf:type rdf:Property;
  rdfs:label "collection_to_target";
  rdfs:domain pds4:urn:nasa:pds:0001_nasa_pds_1:pds:product:pds:product_collection::1.0;
  rdfs:range pds4:urn:nasa:pds:0001_nasa_pds_1:pds:tndo_context:pds:target::1.0.
 
pds4:urn:nasa:pds:0001_nasa_pds_1:pds:product:pds:product_context::context_to_associate:1.0 rdf:type rdf:Property;
  rdfs:label "context_to_associate";
  rdfs:domain pds4:urn:nasa:pds:0001_nasa_pds_1:pds:product:pds:product_context::1.0;
  rdfs:range pds4:urn:nasa:pds:0001_nasa_pds_1:all:user:pds:product::1.0.
 
pds4:urn:nasa:pds:0001_nasa_pds_1:pds:tndo_context:pds:instrument::instrument_to_document:1.0 rdf:type rdf:Property;
  rdfs:label "instrument_to_document";
  rdfs:domain pds4:urn:nasa:pds:0001_nasa_pds_1:pds:tndo_context:pds:instrument::1.0;
  rdfs:range pds4:urn:nasa:pds:0001_nasa_pds_1:pds:product:pds:product_document::1.0.
 
pds4:urn:nasa:pds:0001_nasa_pds_1:pds:tndo_context:pds:instrument::instrument_to_instrument_host:1.0 rdf:type rdf:Property;
  rdfs:label "instrument_to_instrument_host";
  rdfs:domain pds4:urn:nasa:pds:0001_nasa_pds_1:pds:tndo_context:pds:instrument::1.0;
  rdfs:range pds4:urn:nasa:pds:0001_nasa_pds_1:pds:tndo_context:pds:instrument_host::1.0.
 
pds4:urn:nasa:pds:0001_nasa_pds_1:pds:tndo_context:pds:instrument_host::instrument_host_to_document:1.0 rdf:type rdf:Property;
  rdfs:label "instrument_host_to_document";
  rdfs:domain pds4:urn:nasa:pds:0001_nasa_pds_1:pds:tndo_context:pds:instrument_host::1.0;
  rdfs:range pds4:urn:nasa:pds:0001_nasa_pds_1:pds:product:pds:product_document::1.0.
 
pds4:urn:nasa:pds:0001_nasa_pds_1:pds:tndo_context:pds:instrument_host::instrument_host_to_instrument:1.0 rdf:type rdf:Property;
  rdfs:label "instrument_host_to_instrument";
  rdfs:domain pds4:urn:nasa:pds:0001_nasa_pds_1:pds:tndo_context:pds:instrument_host::1.0;
  rdfs:range pds4:urn:nasa:pds:0001_nasa_pds_1:pds:tndo_context:pds:instrument::1.0.
 
pds4:urn:nasa:pds:0001_nasa_pds_1:pds:tndo_context:pds:instrument_host::instrument_host_to_investigation:1.0 rdf:type rdf:Property;
  rdfs:label "instrument_host_to_investigation";
  rdfs:domain pds4:urn:nasa:pds:0001_nasa_pds_1:pds:tndo_context:pds:instrument_host::1.0;
  rdfs:range pds4:urn:nasa:pds:0001_nasa_pds_1:pds:tndo_context:pds:investigation::1.0.
 
pds4:urn:nasa:pds:0001_nasa_pds_1:pds:tndo_context:pds:instrument_host::instrument_host_to_target:1.0 rdf:type rdf:Property;
  rdfs:label "instrument_host_to_target";
  rdfs:domain pds4:urn:nasa:pds:0001_nasa_pds_1:pds:tndo_context:pds:instrument_host::1.0;
  rdfs:range pds4:urn:nasa:pds:0001_nasa_pds_1:pds:tndo_context:pds:target::1.0.
 
pds4:urn:nasa:pds:0001_nasa_pds_1:pds:tndo_context:pds:investigation::investigation_to_document:1.0 rdf:type rdf:Property;
  rdfs:label "investigation_to_document";
  rdfs:domain pds4:urn:nasa:pds:0001_nasa_pds_1:pds:tndo_context:pds:investigation::1.0;
  rdfs:range pds4:urn:nasa:pds:0001_nasa_pds_1:pds:product:pds:product_document::1.0.
 
pds4:urn:nasa:pds:0001_nasa_pds_1:pds:tndo_context:pds:investigation::investigation_to_instrument:1.0 rdf:type rdf:Property;
  rdfs:label "investigation_to_instrument";
  rdfs:domain pds4:urn:nasa:pds:0001_nasa_pds_1:pds:tndo_context:pds:investigation::1.0;
  rdfs:range pds4:urn:nasa:pds:0001_nasa_pds_1:pds:tndo_context:pds:instrument::1.0.
 
pds4:urn:nasa:pds:0001_nasa_pds_1:pds:tndo_context:pds:investigation::investigation_to_instrument_host:1.0 rdf:type rdf:Property;
  rdfs:label "investigation_to_instrument_host";
  rdfs:domain pds4:urn:nasa:pds:0001_nasa_pds_1:pds:tndo_context:pds:investigation::1.0;
  rdfs:range pds4:urn:nasa:pds:0001_nasa_pds_1:pds:tndo_context:pds:instrument_host::1.0.
 
pds4:urn:nasa:pds:0001_nasa_pds_1:pds:tndo_context:pds:investigation::investigation_to_target:1.0 rdf:type rdf:Property;
  rdfs:label "investigation_to_target";
  rdfs:domain pds4:urn:nasa:pds:0001_nasa_pds_1:pds:tndo_context:pds:investigation::1.0;
  rdfs:range pds4:urn:nasa:pds:0001_nasa_pds_1:pds:tndo_context:pds:target::1.0.
 
pds4:urn:nasa:pds:0001_nasa_pds_1:pds:tndo_context:pds:node::node_to_personnel:1.0 rdf:type rdf:Property;
  rdfs:label "node_to_personnel";
  rdfs:domain pds4:urn:nasa:pds:0001_nasa_pds_1:pds:tndo_context:pds:node::1.0;
  rdfs:range pds4:urn:nasa:pds:0001_nasa_pds_1:pds:tndo_context:pds:pds_affiliate::1.0.
 
pds4:urn:nasa:pds:0001_nasa_pds_1:pds:tndo_context:pds:node::node_to_agency:1.0 rdf:type rdf:Property;
  rdfs:label "node_to_agency";
  rdfs:domain pds4:urn:nasa:pds:0001_nasa_pds_1:pds:tndo_context:pds:node::1.0;
  rdfs:range pds4:urn:nasa:pds:0001_nasa_pds_1:pds:tndo_context:pds:agency::1.0.
 
pds4:urn:nasa:pds:0001_nasa_pds_1:pds:tndo_context:pds:node::node_to_manager:1.0 rdf:type rdf:Property;
  rdfs:label "node_to_manager";
  rdfs:domain pds4:urn:nasa:pds:0001_nasa_pds_1:pds:tndo_context:pds:node::1.0;
  rdfs:range pds4:urn:nasa:pds:0001_nasa_pds_1:pds:tndo_context:pds:pds_affiliate::1.0.
 
pds4:urn:nasa:pds:0001_nasa_pds_1:pds:tndo_context:pds:node::node_to_operator:1.0 rdf:type rdf:Property;
  rdfs:label "node_to_operator";
  rdfs:domain pds4:urn:nasa:pds:0001_nasa_pds_1:pds:tndo_context:pds:node::1.0;
  rdfs:range pds4:urn:nasa:pds:0001_nasa_pds_1:pds:tndo_context:pds:pds_affiliate::1.0.
 
pds4:urn:nasa:pds:0001_nasa_pds_1:pds:tndo_context:pds:node::node_to_data_archivist:1.0 rdf:type rdf:Property;
  rdfs:label "node_to_data_archivist";
  rdfs:domain pds4:urn:nasa:pds:0001_nasa_pds_1:pds:tndo_context:pds:node::1.0;
  rdfs:range pds4:urn:nasa:pds:0001_nasa_pds_1:pds:tndo_context:pds:pds_affiliate::1.0.
 
pds4:urn:nasa:pds:0001_nasa_pds_1:pds:tndo_context:pds:resource::resource_to_instrument:1.0 rdf:type rdf:Property;
  rdfs:label "resource_to_instrument";
  rdfs:domain pds4:urn:nasa:pds:0001_nasa_pds_1:pds:tndo_context:pds:resource::1.0;
  rdfs:range pds4:urn:nasa:pds:0001_nasa_pds_1:pds:tndo_context:pds:instrument::1.0.
 
pds4:urn:nasa:pds:0001_nasa_pds_1:pds:tndo_context:pds:resource::resource_to_instrument_host:1.0 rdf:type rdf:Property;
  rdfs:label "resource_to_instrument_host";
  rdfs:domain pds4:urn:nasa:pds:0001_nasa_pds_1:pds:tndo_context:pds:resource::1.0;
  rdfs:range pds4:urn:nasa:pds:0001_nasa_pds_1:pds:tndo_context:pds:instrument_host::1.0.
 
pds4:urn:nasa:pds:0001_nasa_pds_1:pds:tndo_context:pds:resource::resource_to_investigation:1.0 rdf:type rdf:Property;
  rdfs:label "resource_to_investigation";
  rdfs:domain pds4:urn:nasa:pds:0001_nasa_pds_1:pds:tndo_context:pds:resource::1.0;
  rdfs:range pds4:urn:nasa:pds:0001_nasa_pds_1:pds:tndo_context:pds:investigation::1.0.
 
pds4:urn:nasa:pds:0001_nasa_pds_1:pds:tndo_context:pds:resource::resource_to_target:1.0 rdf:type rdf:Property;
  rdfs:label "resource_to_target";
  rdfs:domain pds4:urn:nasa:pds:0001_nasa_pds_1:pds:tndo_context:pds:resource::1.0;
  rdfs:range pds4:urn:nasa:pds:0001_nasa_pds_1:pds:tndo_context:pds:target::1.0.
 
pds4:urn:nasa:pds:0001_nasa_pds_1:pds:tndo_context:pds:target::target_to_document:1.0 rdf:type rdf:Property;
  rdfs:label "target_to_document";
  rdfs:domain pds4:urn:nasa:pds:0001_nasa_pds_1:pds:tndo_context:pds:target::1.0;
  rdfs:range pds4:urn:nasa:pds:0001_nasa_pds_1:pds:product:pds:product_document::1.0.
 
pds4:urn:nasa:pds:0001_nasa_pds_1:pds:tndo_context:pds:target::target_to_instrument:1.0 rdf:type rdf:Property;
  rdfs:label "target_to_instrument";
  rdfs:domain pds4:urn:nasa:pds:0001_nasa_pds_1:pds:tndo_context:pds:target::1.0;
  rdfs:range pds4:urn:nasa:pds:0001_nasa_pds_1:pds:tndo_context:pds:instrument::1.0.
 
pds4:urn:nasa:pds:0001_nasa_pds_1:pds:tndo_context:pds:target::target_to_instrument_host:1.0 rdf:type rdf:Property;
  rdfs:label "target_to_instrument_host";
  rdfs:domain pds4:urn:nasa:pds:0001_nasa_pds_1:pds:tndo_context:pds:target::1.0;
  rdfs:range pds4:urn:nasa:pds:0001_nasa_pds_1:pds:tndo_context:pds:instrument_host::1.0.
 
pds4:urn:nasa:pds:0001_nasa_pds_1:pds:tndo_context:pds:target::target_to_investigation:1.0 rdf:type rdf:Property;
  rdfs:label "target_to_investigation";
  rdfs:domain pds4:urn:nasa:pds:0001_nasa_pds_1:pds:tndo_context:pds:target::1.0;
  rdfs:range pds4:urn:nasa:pds:0001_nasa_pds_1:pds:tndo_context:pds:investigation::1.0.
 
pds4:urn:nasa:pds:0001_nasa_pds_1:pds:tndo_context:pds:instrument::instrument_to_telescope:1.0 rdf:type rdf:Property;
  rdfs:label "instrument_to_telescope";
  rdfs:domain pds4:urn:nasa:pds:0001_nasa_pds_1:pds:tndo_context:pds:instrument::1.0;
  rdfs:range pds4:urn:nasa:pds:0001_nasa_pds_1:pds:tndo_context:pds:telescope::1.0.
 
pds4:urn:nasa:pds:0001_nasa_pds_1:pds:tndo_context:pds:instrument::instrument_to_observatory:1.0 rdf:type rdf:Property;
  rdfs:label "instrument_to_observatory";
  rdfs:domain pds4:urn:nasa:pds:0001_nasa_pds_1:pds:tndo_context:pds:instrument::1.0;
  rdfs:range pds4:urn:nasa:pds:0001_nasa_pds_1:pds:product:pds:product_context::1.0.
 
pds4:urn:nasa:pds:0001_nasa_pds_1:pds:tndo_context:pds:instrument::instrument_to_facility:1.0 rdf:type rdf:Property;
  rdfs:label "instrument_to_facility";
  rdfs:domain pds4:urn:nasa:pds:0001_nasa_pds_1:pds:tndo_context:pds:instrument::1.0;
  rdfs:range pds4:urn:nasa:pds:0001_nasa_pds_1:pds:tndo_context:pds:facility::1.0.
 
pds4:urn:nasa:pds:0001_nasa_pds_1:pds:tndo_context:pds:telescope::telescope_to_observatory:1.0 rdf:type rdf:Property;
  rdfs:label "telescope_to_observatory";
  rdfs:domain pds4:urn:nasa:pds:0001_nasa_pds_1:pds:tndo_context:pds:telescope::1.0;
  rdfs:range pds4:urn:nasa:pds:0001_nasa_pds_1:pds:product:pds:product_context::1.0.
 
pds4:urn:nasa:pds:0001_nasa_pds_1:pds:tndo_context:pds:telescope::telescope_to_facility:1.0 rdf:type rdf:Property;
  rdfs:label "telescope_to_facility";
  rdfs:domain pds4:urn:nasa:pds:0001_nasa_pds_1:pds:tndo_context:pds:telescope::1.0;
  rdfs:range pds4:urn:nasa:pds:0001_nasa_pds_1:pds:tndo_context:pds:facility::1.0.
 
pds4:urn:nasa:pds:0001_nasa_pds_1:pds:tndo_context:pds:telescope::telescope_to_airborne:1.0 rdf:type rdf:Property;
  rdfs:label "telescope_to_airborne";
  rdfs:domain pds4:urn:nasa:pds:0001_nasa_pds_1:pds:tndo_context:pds:telescope::1.0;
  rdfs:range pds4:urn:nasa:pds:0001_nasa_pds_1:pds:tndo_context:pds:airborne::1.0.
 
pds4:urn:nasa:pds:0001_nasa_pds_1:pds:tndo_context:pds:investigation::investigation_to_telescope:1.0 rdf:type rdf:Property;
  rdfs:label "investigation_to_telescope";
  rdfs:domain pds4:urn:nasa:pds:0001_nasa_pds_1:pds:tndo_context:pds:investigation::1.0;
  rdfs:range pds4:urn:nasa:pds:0001_nasa_pds_1:pds:tndo_context:pds:telescope::1.0.
 
pds4:urn:nasa:pds:0001_nasa_pds_1:pds:tndo_context:pds:facility::facility_to_investigation:1.0 rdf:type rdf:Property;
  rdfs:label "facility_to_investigation";
  rdfs:domain pds4:urn:nasa:pds:0001_nasa_pds_1:pds:tndo_context:pds:facility::1.0;
  rdfs:range pds4:urn:nasa:pds:0001_nasa_pds_1:pds:tndo_context:pds:investigation::1.0.
 
pds4:urn:nasa:pds:0001_nasa_pds_1:pds:tndo_context:pds:facility::facility_to_instrument:1.0 rdf:type rdf:Property;
  rdfs:label "facility_to_instrument";
  rdfs:domain pds4:urn:nasa:pds:0001_nasa_pds_1:pds:tndo_context:pds:facility::1.0;
  rdfs:range pds4:urn:nasa:pds:0001_nasa_pds_1:pds:tndo_context:pds:instrument::1.0.
 
pds4:urn:nasa:pds:0001_nasa_pds_1:pds:tndo_context:pds:facility::facility_to_telescope:1.0 rdf:type rdf:Property;
  rdfs:label "facility_to_telescope";
  rdfs:domain pds4:urn:nasa:pds:0001_nasa_pds_1:pds:tndo_context:pds:facility::1.0;
  rdfs:range pds4:urn:nasa:pds:0001_nasa_pds_1:pds:tndo_context:pds:telescope::1.0.
 
pds4:urn:nasa:pds:0001_nasa_pds_1:pds:tndo_context:pds:investigation::investigation_to_facility:1.0 rdf:type rdf:Property;
  rdfs:label "investigation_to_facility";
  rdfs:domain pds4:urn:nasa:pds:0001_nasa_pds_1:pds:tndo_context:pds:investigation::1.0;
  rdfs:range pds4:urn:nasa:pds:0001_nasa_pds_1:pds:tndo_context:pds:facility::1.0.
 
pds4:urn:nasa:pds:0001_nasa_pds_1:pds:tndo_context:pds:telescope::telescope_to_instrument:1.0 rdf:type rdf:Property;
  rdfs:label "telescope_to_instrument";
  rdfs:domain pds4:urn:nasa:pds:0001_nasa_pds_1:pds:tndo_context:pds:telescope::1.0;
  rdfs:range pds4:urn:nasa:pds:0001_nasa_pds_1:pds:tndo_context:pds:instrument::1.0.
 
pds4:urn:nasa:pds:0001_nasa_pds_1:pds:product:pds:product_aip::package_has_collection:1.0 rdf:type rdf:Property;
  rdfs:label "package_has_collection";
  rdfs:domain pds4:urn:nasa:pds:0001_nasa_pds_1:pds:product:pds:product_aip::1.0;
  rdfs:range pds4:urn:nasa:pds:0001_nasa_pds_1:pds:product:pds:product_collection::1.0.
 
pds4:urn:nasa:pds:0001_nasa_pds_1:pds:product:pds:product_aip::package_has_bundle:1.0 rdf:type rdf:Property;
  rdfs:label "package_has_bundle";
  rdfs:domain pds4:urn:nasa:pds:0001_nasa_pds_1:pds:product:pds:product_aip::1.0;
  rdfs:range pds4:urn:nasa:pds:0001_nasa_pds_1:pds:product:pds:product_bundle::1.0.
 
pds4:urn:nasa:pds:0001_nasa_pds_1:pds:product:pds:product_aip::package_has_product:1.0 rdf:type rdf:Property;
  rdfs:label "package_has_product";
  rdfs:domain pds4:urn:nasa:pds:0001_nasa_pds_1:pds:product:pds:product_aip::1.0;
  rdfs:range pds4:urn:nasa:pds:0001_nasa_pds_1:pds:product:pds:product_observational::1.0.
 
pds4:urn:nasa:pds:0001_nasa_pds_1:pds:product:pds:product_aip::package_compiled_from_package:1.0 rdf:type rdf:Property;
  rdfs:label "package_compiled_from_package";
  rdfs:domain pds4:urn:nasa:pds:0001_nasa_pds_1:pds:product:pds:product_aip::1.0;
  rdfs:range pds4:urn:nasa:pds:0001_nasa_pds_1:pds:product:pds:product_aip::1.0.
 
pds4:urn:nasa:pds:0001_nasa_pds_1:pds:product:pds:product_aip::package_has_collection:1.0 rdf:type rdf:Property;
  rdfs:label "package_has_collection";
  rdfs:domain pds4:urn:nasa:pds:0001_nasa_pds_1:pds:product:pds:product_aip::1.0;
  rdfs:range pds4:urn:nasa:pds:0001_nasa_pds_1:pds:product:pds:product_collection::1.0.
 
pds4:urn:nasa:pds:0001_nasa_pds_1:pds:product:pds:product_aip::package_has_bundle:1.0 rdf:type rdf:Property;
  rdfs:label "package_has_bundle";
  rdfs:domain pds4:urn:nasa:pds:0001_nasa_pds_1:pds:product:pds:product_aip::1.0;
  rdfs:range pds4:urn:nasa:pds:0001_nasa_pds_1:pds:product:pds:product_bundle::1.0.
 
pds4:urn:nasa:pds:0001_nasa_pds_1:pds:product:pds:product_aip::package_has_product:1.0 rdf:type rdf:Property;
  rdfs:label "package_has_product";
  rdfs:domain pds4:urn:nasa:pds:0001_nasa_pds_1:pds:product:pds:product_aip::1.0;
  rdfs:range pds4:urn:nasa:pds:0001_nasa_pds_1:pds:product:pds:product_observational::1.0.
 
pds4:urn:nasa:pds:0001_nasa_pds_1:pds:product:pds:product_aip::package_compiled_from_package:1.0 rdf:type rdf:Property;
  rdfs:label "package_compiled_from_package";
  rdfs:domain pds4:urn:nasa:pds:0001_nasa_pds_1:pds:product:pds:product_aip::1.0;
  rdfs:range pds4:urn:nasa:pds:0001_nasa_pds_1:pds:product:pds:product_aip::1.0.
 
pds4:urn:nasa:pds:0001_nasa_pds_1:pds:product:pds:product_document::document_to_investigation:1.0 rdf:type rdf:Property;
  rdfs:label "document_to_investigation";
  rdfs:domain pds4:urn:nasa:pds:0001_nasa_pds_1:pds:product:pds:product_document::1.0;
  rdfs:range pds4:urn:nasa:pds:0001_nasa_pds_1:pds:tndo_context:pds:investigation::1.0.
 
pds4:urn:nasa:pds:0001_nasa_pds_1:pds:product:pds:product_document::document_to_target:1.0 rdf:type rdf:Property;
  rdfs:label "document_to_target";
  rdfs:domain pds4:urn:nasa:pds:0001_nasa_pds_1:pds:product:pds:product_document::1.0;
  rdfs:range pds4:urn:nasa:pds:0001_nasa_pds_1:pds:tndo_context:pds:target::1.0.
 
pds4:urn:nasa:pds:0001_nasa_pds_1:pds:product:pds:product_document::document_to_associate:1.0 rdf:type rdf:Property;
  rdfs:label "document_to_associate";
  rdfs:domain pds4:urn:nasa:pds:0001_nasa_pds_1:pds:product:pds:product_document::1.0;
  rdfs:range pds4:urn:nasa:pds:0001_nasa_pds_1:all:user:pds:product::1.0.
 
pds4:urn:nasa:pds:0001_nasa_pds_1:pds:product:pds:product_document::document_to_investigation:1.0 rdf:type rdf:Property;
  rdfs:label "document_to_investigation";
  rdfs:domain pds4:urn:nasa:pds:0001_nasa_pds_1:pds:product:pds:product_document::1.0;
  rdfs:range pds4:urn:nasa:pds:0001_nasa_pds_1:pds:tndo_context:pds:investigation::1.0.
 
pds4:urn:nasa:pds:0001_nasa_pds_1:pds:product:pds:product_document::document_to_instrument_host:1.0 rdf:type rdf:Property;
  rdfs:label "document_to_instrument_host";
  rdfs:domain pds4:urn:nasa:pds:0001_nasa_pds_1:pds:product:pds:product_document::1.0;
  rdfs:range pds4:urn:nasa:pds:0001_nasa_pds_1:pds:tndo_context:pds:instrument_host::1.0.
 
pds4:urn:nasa:pds:0001_nasa_pds_1:pds:product:pds:product_document::document_to_instrument:1.0 rdf:type rdf:Property;
  rdfs:label "document_to_instrument";
  rdfs:domain pds4:urn:nasa:pds:0001_nasa_pds_1:pds:product:pds:product_document::1.0;
  rdfs:range pds4:urn:nasa:pds:0001_nasa_pds_1:pds:tndo_context:pds:instrument::1.0.
 
pds4:urn:nasa:pds:0001_nasa_pds_1:pds:product:pds:product_document::document_to_target:1.0 rdf:type rdf:Property;
  rdfs:label "document_to_target";
  rdfs:domain pds4:urn:nasa:pds:0001_nasa_pds_1:pds:product:pds:product_document::1.0;
  rdfs:range pds4:urn:nasa:pds:0001_nasa_pds_1:pds:tndo_context:pds:target::1.0.
 
pds4:urn:nasa:pds:0001_nasa_pds_1:pds:product:pds:product_observational::data_to_investigation:1.0 rdf:type rdf:Property;
  rdfs:label "data_to_investigation";
  rdfs:domain pds4:urn:nasa:pds:0001_nasa_pds_1:pds:product:pds:product_observational::1.0;
  rdfs:range pds4:urn:nasa:pds:0001_nasa_pds_1:pds:tndo_context:pds:investigation::1.0.
 
pds4:urn:nasa:pds:0001_nasa_pds_1:pds:product:pds:product_observational::data_to_target:1.0 rdf:type rdf:Property;
  rdfs:label "data_to_target";
  rdfs:domain pds4:urn:nasa:pds:0001_nasa_pds_1:pds:product:pds:product_observational::1.0;
  rdfs:range pds4:urn:nasa:pds:0001_nasa_pds_1:pds:tndo_context:pds:target::1.0.
 
pds4:urn:nasa:pds:0001_nasa_pds_1:pds:product:pds:product_observational::data_to_associate:1.0 rdf:type rdf:Property;
  rdfs:label "data_to_associate";
  rdfs:domain pds4:urn:nasa:pds:0001_nasa_pds_1:pds:product:pds:product_observational::1.0;
  rdfs:range pds4:urn:nasa:pds:0001_nasa_pds_1:all:user:pds:product::1.0.
 
pds4:urn:nasa:pds:0001_nasa_pds_1:pds:product:pds:product_observational::data_to_resource:1.0 rdf:type rdf:Property;
  rdfs:label "data_to_resource";
  rdfs:domain pds4:urn:nasa:pds:0001_nasa_pds_1:pds:product:pds:product_observational::1.0;
  rdfs:range pds4:urn:nasa:pds:0001_nasa_pds_1:pds:tndo_context:pds:resource::1.0.
 
pds4:urn:nasa:pds:0001_nasa_pds_1:pds:product:pds:product_observational::data_to_calibration_document:1.0 rdf:type rdf:Property;
  rdfs:label "data_to_calibration_document";
  rdfs:domain pds4:urn:nasa:pds:0001_nasa_pds_1:pds:product:pds:product_observational::1.0;
  rdfs:range pds4:urn:nasa:pds:0001_nasa_pds_1:pds:product:pds:product_document::1.0.
 
pds4:urn:nasa:pds:0001_nasa_pds_1:pds:product:pds:product_observational::data_to_calibration_product:1.0 rdf:type rdf:Property;
  rdfs:label "data_to_calibration_product";
  rdfs:domain pds4:urn:nasa:pds:0001_nasa_pds_1:pds:product:pds:product_observational::1.0;
  rdfs:range pds4:urn:nasa:pds:0001_nasa_pds_1:pds:product:pds:product_observational::1.0.
 
pds4:urn:nasa:pds:0001_nasa_pds_1:pds:product:pds:product_observational::data_to_raw_product:1.0 rdf:type rdf:Property;
  rdfs:label "data_to_raw_product";
  rdfs:domain pds4:urn:nasa:pds:0001_nasa_pds_1:pds:product:pds:product_observational::1.0;
  rdfs:range pds4:urn:nasa:pds:0001_nasa_pds_1:pds:product:pds:product_observational::1.0.
 
pds4:urn:nasa:pds:0001_nasa_pds_1:pds:product:pds:product_observational::data_to_calibrated_product:1.0 rdf:type rdf:Property;
  rdfs:label "data_to_calibrated_product";
  rdfs:domain pds4:urn:nasa:pds:0001_nasa_pds_1:pds:product:pds:product_observational::1.0;
  rdfs:range pds4:urn:nasa:pds:0001_nasa_pds_1:pds:product:pds:product_observational::1.0.
 
pds4:urn:nasa:pds:0001_nasa_pds_1:pds:product:pds:product_observational::data_to_derived_product:1.0 rdf:type rdf:Property;
  rdfs:label "data_to_derived_product";
  rdfs:domain pds4:urn:nasa:pds:0001_nasa_pds_1:pds:product:pds:product_observational::1.0;
  rdfs:range pds4:urn:nasa:pds:0001_nasa_pds_1:pds:product:pds:product_observational::1.0.
 
pds4:urn:nasa:pds:0001_nasa_pds_1:pds:product:pds:product_observational::data_to_geometry:1.0 rdf:type rdf:Property;
  rdfs:label "data_to_geometry";
  rdfs:domain pds4:urn:nasa:pds:0001_nasa_pds_1:pds:product:pds:product_observational::1.0;
  rdfs:range pds4:urn:nasa:pds:0001_nasa_pds_1:pds:product:pds:product_metadata_supplemental::1.0.
 
pds4:urn:nasa:pds:0001_nasa_pds_1:pds:product:pds:product_observational::data_to_spice_kernel:1.0 rdf:type rdf:Property;
  rdfs:label "data_to_spice_kernel";
  rdfs:domain pds4:urn:nasa:pds:0001_nasa_pds_1:pds:product:pds:product_observational::1.0;
  rdfs:range pds4:urn:nasa:pds:0001_nasa_pds_1:pds:product:pds:product_spice_kernel::1.0.
 
pds4:urn:nasa:pds:0001_nasa_pds_1:pds:product:pds:product_observational::data_to_thumbnail:1.0 rdf:type rdf:Property;
  rdfs:label "data_to_thumbnail";
  rdfs:domain pds4:urn:nasa:pds:0001_nasa_pds_1:pds:product:pds:product_observational::1.0;
  rdfs:range pds4:urn:nasa:pds:0001_nasa_pds_1:pds:product:pds:product_thumbnail::1.0.
 
pds4:urn:nasa:pds:0001_nasa_pds_1:pds:product:pds:product_observational::data_to_document:1.0 rdf:type rdf:Property;
  rdfs:label "data_to_document";
  rdfs:domain pds4:urn:nasa:pds:0001_nasa_pds_1:pds:product:pds:product_observational::1.0;
  rdfs:range pds4:urn:nasa:pds:0001_nasa_pds_1:pds:product:pds:product_document::1.0.
 
pds4:urn:nasa:pds:0001_nasa_pds_1:pds:product:pds:product_observational::data_curated_by_node:1.0 rdf:type rdf:Property;
  rdfs:label "data_curated_by_node";
  rdfs:domain pds4:urn:nasa:pds:0001_nasa_pds_1:pds:product:pds:product_observational::1.0;
  rdfs:range pds4:urn:nasa:pds:0001_nasa_pds_1:pds:tndo_context:pds:node::1.0.
 
pds4:urn:nasa:pds:0001_nasa_pds_1:pds:product:pds:product_observational::data_to_browse:1.0 rdf:type rdf:Property;
  rdfs:label "data_to_browse";
  rdfs:domain pds4:urn:nasa:pds:0001_nasa_pds_1:pds:product:pds:product_observational::1.0;
  rdfs:range pds4:urn:nasa:pds:0001_nasa_pds_1:pds:product:pds:product_browse::1.0.
 
pds4:urn:nasa:pds:0001_nasa_pds_1:pds:product:pds:product_observational::data_to_ancillary_data:1.0 rdf:type rdf:Property;
  rdfs:label "data_to_ancillary_data";
  rdfs:domain pds4:urn:nasa:pds:0001_nasa_pds_1:pds:product:pds:product_observational::1.0;
  rdfs:range pds4:urn:nasa:pds:0001_nasa_pds_1:pds:product:pds:product_ancillary::1.0.
 
pds4:urn:nasa:pds:0001_nasa_pds_1:pds:product:pds:product_aip::package_has_collection:1.0 rdf:type rdf:Property;
  rdfs:label "package_has_collection";
  rdfs:domain pds4:urn:nasa:pds:0001_nasa_pds_1:pds:product:pds:product_aip::1.0;
  rdfs:range pds4:urn:nasa:pds:0001_nasa_pds_1:pds:product:pds:product_collection::1.0.
 
pds4:urn:nasa:pds:0001_nasa_pds_1:pds:product:pds:product_aip::package_has_bundle:1.0 rdf:type rdf:Property;
  rdfs:label "package_has_bundle";
  rdfs:domain pds4:urn:nasa:pds:0001_nasa_pds_1:pds:product:pds:product_aip::1.0;
  rdfs:range pds4:urn:nasa:pds:0001_nasa_pds_1:pds:product:pds:product_bundle::1.0.
 
pds4:urn:nasa:pds:0001_nasa_pds_1:pds:product:pds:product_aip::package_has_product:1.0 rdf:type rdf:Property;
  rdfs:label "package_has_product";
  rdfs:domain pds4:urn:nasa:pds:0001_nasa_pds_1:pds:product:pds:product_aip::1.0;
  rdfs:range pds4:urn:nasa:pds:0001_nasa_pds_1:pds:product:pds:product_observational::1.0.
 
pds4:urn:nasa:pds:0001_nasa_pds_1:pds:product:pds:product_aip::package_has_bundle:1.0 rdf:type rdf:Property;
  rdfs:label "package_has_bundle";
  rdfs:domain pds4:urn:nasa:pds:0001_nasa_pds_1:pds:product:pds:product_aip::1.0;
  rdfs:range pds4:urn:nasa:pds:0001_nasa_pds_1:pds:product:pds:product_bundle::1.0.
 
pds4:urn:nasa:pds:0001_nasa_pds_1:pds:product:pds:product_thumbnail::thumbnail_to_data:1.0 rdf:type rdf:Property;
  rdfs:label "thumbnail_to_data";
  rdfs:domain pds4:urn:nasa:pds:0001_nasa_pds_1:pds:product:pds:product_thumbnail::1.0;
  rdfs:range pds4:urn:nasa:pds:0001_nasa_pds_1:pds:product:pds:product_observational::1.0.
 
pds4:urn:nasa:pds:0001_nasa_pds_1:pds:product:pds:product_thumbnail::thumbnail_to_browse:1.0 rdf:type rdf:Property;
  rdfs:label "thumbnail_to_browse";
  rdfs:domain pds4:urn:nasa:pds:0001_nasa_pds_1:pds:product:pds:product_thumbnail::1.0;
  rdfs:range pds4:urn:nasa:pds:0001_nasa_pds_1:pds:product:pds:product_browse::1.0.
 
pds4:urn:nasa:pds:0001_nasa_pds_1:pds:product:pds:product_thumbnail::thumbnail_to_document:1.0 rdf:type rdf:Property;
  rdfs:label "thumbnail_to_document";
  rdfs:domain pds4:urn:nasa:pds:0001_nasa_pds_1:pds:product:pds:product_thumbnail::1.0;
  rdfs:range pds4:urn:nasa:pds:0001_nasa_pds_1:pds:product:pds:product_document::1.0.
 
pds4:urn:nasa:pds:0001_nasa_pds_1:pds:product:pds:product_update::update_to_collection:1.0 rdf:type rdf:Property;
  rdfs:label "update_to_collection";
  rdfs:domain pds4:urn:nasa:pds:0001_nasa_pds_1:pds:product:pds:product_update::1.0;
  rdfs:range pds4:urn:nasa:pds:0001_nasa_pds_1:pds:product:pds:product_collection::1.0.
 
pds4:urn:nasa:pds:0001_nasa_pds_1:pds:product:pds:product_zipped::zip_to_package:1.0 rdf:type rdf:Property;
  rdfs:label "zip_to_package";
  rdfs:domain pds4:urn:nasa:pds:0001_nasa_pds_1:pds:product:pds:product_zipped::1.0;
  rdfs:range pds4:urn:nasa:pds:0001_nasa_pds_1:pds:product:pds:product_aip::1.0.
 
pds4:urn:nasa:pds:0001_nasa_pds_1:all:user:cart:cartography::local_internal_reference::1.0 rdf:type rdf:Property;
  rdfs:label "Local_Internal_Reference";
  rdfs:domain pds4:urn:nasa:pds:0001_nasa_pds_1:all:user:cart:cartography::1.0;
  rdfs:range pds4:urn:nasa:pds:0001_nasa_pds_1:pds:product_components:pds:local_internal_reference::1.0.
 
pds4:urn:nasa:pds:0001_nasa_pds_1:all:user:cart:cartography::spatial_domain::1.0 rdf:type rdf:Property;
  rdfs:label "Spatial_Domain";
  rdfs:domain pds4:urn:nasa:pds:0001_nasa_pds_1:all:user:cart:cartography::1.0;
  rdfs:range pds4:urn:nasa:pds:0001_nasa_pds_1:all:user:cart:spatial_domain::1.0.
 
pds4:urn:nasa:pds:0001_nasa_pds_1:all:user:cart:cartography::secondary_spatial_domain::1.0 rdf:type rdf:Property;
  rdfs:label "Secondary_Spatial_Domain";
  rdfs:domain pds4:urn:nasa:pds:0001_nasa_pds_1:all:user:cart:cartography::1.0;
  rdfs:range pds4:urn:nasa:pds:0001_nasa_pds_1:all:user:cart:secondary_spatial_domain::1.0.
 
pds4:urn:nasa:pds:0001_nasa_pds_1:all:user:cart:cartography::spatial_reference_information::1.0 rdf:type rdf:Property;
  rdfs:label "Spatial_Reference_Information";
  rdfs:domain pds4:urn:nasa:pds:0001_nasa_pds_1:all:user:cart:cartography::1.0;
  rdfs:range pds4:urn:nasa:pds:0001_nasa_pds_1:all:user:cart:spatial_reference_information::1.0.
 
pds4:urn:nasa:pds:0001_nasa_pds_1:all:user:cart:cylindrical::vector_projection_origin::1.0 rdf:type rdf:Property;
  rdfs:label "Vector_Projection_Origin";
  rdfs:domain pds4:urn:nasa:pds:0001_nasa_pds_1:all:user:cart:cylindrical::1.0;
  rdfs:range pds4:urn:nasa:pds:0001_nasa_pds_1:geom:vector_cartesian_position_base:cart:vector_projection_origin::1.0.
 
pds4:urn:nasa:pds:0001_nasa_pds_1:all:user:cart:cylindrical_perspective::vector_projection_origin::1.0 rdf:type rdf:Property;
  rdfs:label "Vector_Projection_Origin";
  rdfs:domain pds4:urn:nasa:pds:0001_nasa_pds_1:all:user:cart:cylindrical_perspective::1.0;
  rdfs:range pds4:urn:nasa:pds:0001_nasa_pds_1:geom:vector_cartesian_position_base:cart:vector_projection_origin::1.0.
 
pds4:urn:nasa:pds:0001_nasa_pds_1:all:user:cart:cylindrical_perspective::vector_projection_z_axis::1.0 rdf:type rdf:Property;
  rdfs:label "Vector_Projection_Z_Axis";
  rdfs:domain pds4:urn:nasa:pds:0001_nasa_pds_1:all:user:cart:cylindrical_perspective::1.0;
  rdfs:range pds4:urn:nasa:pds:0001_nasa_pds_1:cart:vector_cartesian_unit_base:cart:vector_projection_z_axis::1.0.
 
pds4:urn:nasa:pds:0001_nasa_pds_1:all:user:cart:cylindrical_perspective::vector_projection_z_axis_initial::1.0 rdf:type rdf:Property;
  rdfs:label "Vector_Projection_Z_Axis_Initial";
  rdfs:domain pds4:urn:nasa:pds:0001_nasa_pds_1:all:user:cart:cylindrical_perspective::1.0;
  rdfs:range pds4:urn:nasa:pds:0001_nasa_pds_1:cart:vector_cartesian_unit_base:cart:vector_projection_z_axis_initial::1.0.
 
pds4:urn:nasa:pds:0001_nasa_pds_1:all:user:cart:grid_coordinate_system::universal_transverse_mercator::1.0 rdf:type rdf:Property;
  rdfs:label "Universal_Transverse_Mercator";
  rdfs:domain pds4:urn:nasa:pds:0001_nasa_pds_1:all:user:cart:grid_coordinate_system::1.0;
  rdfs:range pds4:urn:nasa:pds:0001_nasa_pds_1:all:user:cart:universal_transverse_mercator::1.0.
 
pds4:urn:nasa:pds:0001_nasa_pds_1:all:user:cart:grid_coordinate_system::universal_polar_stereographic::1.0 rdf:type rdf:Property;
  rdfs:label "Universal_Polar_Stereographic";
  rdfs:domain pds4:urn:nasa:pds:0001_nasa_pds_1:all:user:cart:grid_coordinate_system::1.0;
  rdfs:range pds4:urn:nasa:pds:0001_nasa_pds_1:all:user:cart:universal_polar_stereographic::1.0.
 
pds4:urn:nasa:pds:0001_nasa_pds_1:all:user:cart:grid_coordinate_system::state_plane_coordinate_system::1.0 rdf:type rdf:Property;
  rdfs:label "State_Plane_Coordinate_System";
  rdfs:domain pds4:urn:nasa:pds:0001_nasa_pds_1:all:user:cart:grid_coordinate_system::1.0;
  rdfs:range pds4:urn:nasa:pds:0001_nasa_pds_1:all:user:cart:state_plane_coordinate_system::1.0.
 
pds4:urn:nasa:pds:0001_nasa_pds_1:all:user:cart:horizontal_coordinate_system_definition::geographic::1.0 rdf:type rdf:Property;
  rdfs:label "Geographic";
  rdfs:domain pds4:urn:nasa:pds:0001_nasa_pds_1:all:user:cart:horizontal_coordinate_system_definition::1.0;
  rdfs:range pds4:urn:nasa:pds:0001_nasa_pds_1:all:user:cart:geographic::1.0.
 
pds4:urn:nasa:pds:0001_nasa_pds_1:all:user:cart:horizontal_coordinate_system_definition::planar::1.0 rdf:type rdf:Property;
  rdfs:label "Planar";
  rdfs:domain pds4:urn:nasa:pds:0001_nasa_pds_1:all:user:cart:horizontal_coordinate_system_definition::1.0;
  rdfs:range pds4:urn:nasa:pds:0001_nasa_pds_1:all:user:cart:planar::1.0.
 
pds4:urn:nasa:pds:0001_nasa_pds_1:all:user:cart:horizontal_coordinate_system_definition::local::1.0 rdf:type rdf:Property;
  rdfs:label "Local";
  rdfs:domain pds4:urn:nasa:pds:0001_nasa_pds_1:all:user:cart:horizontal_coordinate_system_definition::1.0;
  rdfs:range pds4:urn:nasa:pds:0001_nasa_pds_1:all:user:cart:local::1.0.
 
pds4:urn:nasa:pds:0001_nasa_pds_1:all:user:cart:horizontal_coordinate_system_definition::geodetic_model::1.0 rdf:type rdf:Property;
  rdfs:label "Geodetic_Model";
  rdfs:domain pds4:urn:nasa:pds:0001_nasa_pds_1:all:user:cart:horizontal_coordinate_system_definition::1.0;
  rdfs:range pds4:urn:nasa:pds:0001_nasa_pds_1:all:user:cart:geodetic_model::1.0.
 
pds4:urn:nasa:pds:0001_nasa_pds_1:all:user:cart:local::map_projection_lander::1.0 rdf:type rdf:Property;
  rdfs:label "Map_Projection_Lander";
  rdfs:domain pds4:urn:nasa:pds:0001_nasa_pds_1:all:user:cart:local::1.0;
  rdfs:range pds4:urn:nasa:pds:0001_nasa_pds_1:all:user:cart:map_projection_lander::1.0.
 
pds4:urn:nasa:pds:0001_nasa_pds_1:all:user:cart:local::map_projection_rings::1.0 rdf:type rdf:Property;
  rdfs:label "Map_Projection_Rings";
  rdfs:domain pds4:urn:nasa:pds:0001_nasa_pds_1:all:user:cart:local::1.0;
  rdfs:range pds4:urn:nasa:pds:0001_nasa_pds_1:all:user:cart:map_projection_rings::1.0.
 
pds4:urn:nasa:pds:0001_nasa_pds_1:all:user:cart:local::surface_model_parameters::1.0 rdf:type rdf:Property;
  rdfs:label "Surface_Model_Parameters";
  rdfs:domain pds4:urn:nasa:pds:0001_nasa_pds_1:all:user:cart:local::1.0;
  rdfs:range pds4:urn:nasa:pds:0001_nasa_pds_1:all:user:cart:surface_model_parameters::1.0.
 
pds4:urn:nasa:pds:0001_nasa_pds_1:all:user:cart:map_projection::equirectangular::1.0 rdf:type rdf:Property;
  rdfs:label "Equirectangular";
  rdfs:domain pds4:urn:nasa:pds:0001_nasa_pds_1:all:user:cart:map_projection::1.0;
  rdfs:range pds4:urn:nasa:pds:0001_nasa_pds_1:all:user:cart:equirectangular::1.0.
 
pds4:urn:nasa:pds:0001_nasa_pds_1:all:user:cart:map_projection::lambert_azimuthal_equal_area::1.0 rdf:type rdf:Property;
  rdfs:label "Lambert_Azimuthal_Equal_Area";
  rdfs:domain pds4:urn:nasa:pds:0001_nasa_pds_1:all:user:cart:map_projection::1.0;
  rdfs:range pds4:urn:nasa:pds:0001_nasa_pds_1:all:user:cart:lambert_azimuthal_equal_area::1.0.
 
pds4:urn:nasa:pds:0001_nasa_pds_1:all:user:cart:map_projection::lambert_conformal_conic::1.0 rdf:type rdf:Property;
  rdfs:label "Lambert_Conformal_Conic";
  rdfs:domain pds4:urn:nasa:pds:0001_nasa_pds_1:all:user:cart:map_projection::1.0;
  rdfs:range pds4:urn:nasa:pds:0001_nasa_pds_1:all:user:cart:lambert_conformal_conic::1.0.
 
pds4:urn:nasa:pds:0001_nasa_pds_1:all:user:cart:map_projection::mercator::1.0 rdf:type rdf:Property;
  rdfs:label "Mercator";
  rdfs:domain pds4:urn:nasa:pds:0001_nasa_pds_1:all:user:cart:map_projection::1.0;
  rdfs:range pds4:urn:nasa:pds:0001_nasa_pds_1:all:user:cart:mercator::1.0.
 
pds4:urn:nasa:pds:0001_nasa_pds_1:all:user:cart:map_projection::oblique_cylindrical::1.0 rdf:type rdf:Property;
  rdfs:label "Oblique_Cylindrical";
  rdfs:domain pds4:urn:nasa:pds:0001_nasa_pds_1:all:user:cart:map_projection::1.0;
  rdfs:range pds4:urn:nasa:pds:0001_nasa_pds_1:all:user:cart:oblique_cylindrical::1.0.
 
pds4:urn:nasa:pds:0001_nasa_pds_1:all:user:cart:map_projection::oblique_mercator::1.0 rdf:type rdf:Property;
  rdfs:label "Oblique_Mercator";
  rdfs:domain pds4:urn:nasa:pds:0001_nasa_pds_1:all:user:cart:map_projection::1.0;
  rdfs:range pds4:urn:nasa:pds:0001_nasa_pds_1:all:user:cart:oblique_mercator::1.0.
 
pds4:urn:nasa:pds:0001_nasa_pds_1:all:user:cart:map_projection::orthographic::1.0 rdf:type rdf:Property;
  rdfs:label "Orthographic";
  rdfs:domain pds4:urn:nasa:pds:0001_nasa_pds_1:all:user:cart:map_projection::1.0;
  rdfs:range pds4:urn:nasa:pds:0001_nasa_pds_1:all:user:cart:orthographic::1.0.
 
pds4:urn:nasa:pds:0001_nasa_pds_1:all:user:cart:map_projection::point_perspective::1.0 rdf:type rdf:Property;
  rdfs:label "Point_Perspective";
  rdfs:domain pds4:urn:nasa:pds:0001_nasa_pds_1:all:user:cart:map_projection::1.0;
  rdfs:range pds4:urn:nasa:pds:0001_nasa_pds_1:all:user:cart:point_perspective::1.0.
 
pds4:urn:nasa:pds:0001_nasa_pds_1:all:user:cart:map_projection::polar_stereographic::1.0 rdf:type rdf:Property;
  rdfs:label "Polar_Stereographic";
  rdfs:domain pds4:urn:nasa:pds:0001_nasa_pds_1:all:user:cart:map_projection::1.0;
  rdfs:range pds4:urn:nasa:pds:0001_nasa_pds_1:all:user:cart:polar_stereographic::1.0.
 
pds4:urn:nasa:pds:0001_nasa_pds_1:all:user:cart:map_projection::polyconic::1.0 rdf:type rdf:Property;
  rdfs:label "Polyconic";
  rdfs:domain pds4:urn:nasa:pds:0001_nasa_pds_1:all:user:cart:map_projection::1.0;
  rdfs:range pds4:urn:nasa:pds:0001_nasa_pds_1:all:user:cart:polyconic::1.0.
 
pds4:urn:nasa:pds:0001_nasa_pds_1:all:user:cart:map_projection::sinusoidal::1.0 rdf:type rdf:Property;
  rdfs:label "Sinusoidal";
  rdfs:domain pds4:urn:nasa:pds:0001_nasa_pds_1:all:user:cart:map_projection::1.0;
  rdfs:range pds4:urn:nasa:pds:0001_nasa_pds_1:all:user:cart:sinusoidal::1.0.
 
pds4:urn:nasa:pds:0001_nasa_pds_1:all:user:cart:map_projection::transverse_mercator::1.0 rdf:type rdf:Property;
  rdfs:label "Transverse_Mercator";
  rdfs:domain pds4:urn:nasa:pds:0001_nasa_pds_1:all:user:cart:map_projection::1.0;
  rdfs:range pds4:urn:nasa:pds:0001_nasa_pds_1:all:user:cart:transverse_mercator::1.0.
 
pds4:urn:nasa:pds:0001_nasa_pds_1:all:user:cart:map_projection_lander::cylindrical::1.0 rdf:type rdf:Property;
  rdfs:label "Cylindrical";
  rdfs:domain pds4:urn:nasa:pds:0001_nasa_pds_1:all:user:cart:map_projection_lander::1.0;
  rdfs:range pds4:urn:nasa:pds:0001_nasa_pds_1:all:user:cart:cylindrical::1.0.
 
pds4:urn:nasa:pds:0001_nasa_pds_1:all:user:cart:map_projection_lander::perspective::1.0 rdf:type rdf:Property;
  rdfs:label "Perspective";
  rdfs:domain pds4:urn:nasa:pds:0001_nasa_pds_1:all:user:cart:map_projection_lander::1.0;
  rdfs:range pds4:urn:nasa:pds:0001_nasa_pds_1:all:user:cart:perspective::1.0.
 
pds4:urn:nasa:pds:0001_nasa_pds_1:all:user:cart:map_projection_lander::cylindrical_perspective::1.0 rdf:type rdf:Property;
  rdfs:label "Cylindrical_Perspective";
  rdfs:domain pds4:urn:nasa:pds:0001_nasa_pds_1:all:user:cart:map_projection_lander::1.0;
  rdfs:range pds4:urn:nasa:pds:0001_nasa_pds_1:all:user:cart:cylindrical_perspective::1.0.
 
pds4:urn:nasa:pds:0001_nasa_pds_1:all:user:cart:map_projection_lander::polar::1.0 rdf:type rdf:Property;
  rdfs:label "Polar";
  rdfs:domain pds4:urn:nasa:pds:0001_nasa_pds_1:all:user:cart:map_projection_lander::1.0;
  rdfs:range pds4:urn:nasa:pds:0001_nasa_pds_1:all:user:cart:polar::1.0.
 
pds4:urn:nasa:pds:0001_nasa_pds_1:all:user:cart:map_projection_lander::vertical::1.0 rdf:type rdf:Property;
  rdfs:label "Vertical";
  rdfs:domain pds4:urn:nasa:pds:0001_nasa_pds_1:all:user:cart:map_projection_lander::1.0;
  rdfs:range pds4:urn:nasa:pds:0001_nasa_pds_1:all:user:cart:vertical::1.0.
 
pds4:urn:nasa:pds:0001_nasa_pds_1:all:user:cart:map_projection_lander::orthographic_lander::1.0 rdf:type rdf:Property;
  rdfs:label "Orthographic_Lander";
  rdfs:domain pds4:urn:nasa:pds:0001_nasa_pds_1:all:user:cart:map_projection_lander::1.0;
  rdfs:range pds4:urn:nasa:pds:0001_nasa_pds_1:all:user:cart:orthographic_lander::1.0.
 
pds4:urn:nasa:pds:0001_nasa_pds_1:all:user:cart:map_projection_lander::orthorectified::1.0 rdf:type rdf:Property;
  rdfs:label "Orthorectified";
  rdfs:domain pds4:urn:nasa:pds:0001_nasa_pds_1:all:user:cart:map_projection_lander::1.0;
  rdfs:range pds4:urn:nasa:pds:0001_nasa_pds_1:all:user:cart:orthorectified::1.0.
 
pds4:urn:nasa:pds:0001_nasa_pds_1:all:user:cart:map_projection_rings::ring_polar::1.0 rdf:type rdf:Property;
  rdfs:label "Ring_Polar";
  rdfs:domain pds4:urn:nasa:pds:0001_nasa_pds_1:all:user:cart:map_projection_rings::1.0;
  rdfs:range pds4:urn:nasa:pds:0001_nasa_pds_1:all:user:cart:ring_polar::1.0.
 
pds4:urn:nasa:pds:0001_nasa_pds_1:all:user:cart:oblique_line_point::oblique_line_point_group::1.0 rdf:type rdf:Property;
  rdfs:label "Oblique_Line_Point_Group";
  rdfs:domain pds4:urn:nasa:pds:0001_nasa_pds_1:all:user:cart:oblique_line_point::1.0;
  rdfs:range pds4:urn:nasa:pds:0001_nasa_pds_1:all:user:cart:oblique_line_point_group::1.0.
 
pds4:urn:nasa:pds:0001_nasa_pds_1:all:user:cart:oblique_mercator::oblique_line_azimuth::1.0 rdf:type rdf:Property;
  rdfs:label "Oblique_Line_Azimuth";
  rdfs:domain pds4:urn:nasa:pds:0001_nasa_pds_1:all:user:cart:oblique_mercator::1.0;
  rdfs:range pds4:urn:nasa:pds:0001_nasa_pds_1:all:user:cart:oblique_line_azimuth::1.0.
 
pds4:urn:nasa:pds:0001_nasa_pds_1:all:user:cart:oblique_mercator::oblique_line_point::1.0 rdf:type rdf:Property;
  rdfs:label "Oblique_Line_Point";
  rdfs:domain pds4:urn:nasa:pds:0001_nasa_pds_1:all:user:cart:oblique_mercator::1.0;
  rdfs:range pds4:urn:nasa:pds:0001_nasa_pds_1:all:user:cart:oblique_line_point::1.0.
 
pds4:urn:nasa:pds:0001_nasa_pds_1:all:user:cart:orthographic_lander::pixel_position_origin::1.0 rdf:type rdf:Property;
  rdfs:label "Pixel_Position_Origin";
  rdfs:domain pds4:urn:nasa:pds:0001_nasa_pds_1:all:user:cart:orthographic_lander::1.0;
  rdfs:range pds4:urn:nasa:pds:0001_nasa_pds_1:all:user:cart:pixel_position_origin::1.0.
 
pds4:urn:nasa:pds:0001_nasa_pds_1:all:user:cart:orthographic_lander::vector_projection_origin::1.0 rdf:type rdf:Property;
  rdfs:label "Vector_Projection_Origin";
  rdfs:domain pds4:urn:nasa:pds:0001_nasa_pds_1:all:user:cart:orthographic_lander::1.0;
  rdfs:range pds4:urn:nasa:pds:0001_nasa_pds_1:geom:vector_cartesian_position_base:cart:vector_projection_origin::1.0.
 
pds4:urn:nasa:pds:0001_nasa_pds_1:all:user:cart:orthographic_lander::vector_projection_x_axis::1.0 rdf:type rdf:Property;
  rdfs:label "Vector_Projection_X_Axis";
  rdfs:domain pds4:urn:nasa:pds:0001_nasa_pds_1:all:user:cart:orthographic_lander::1.0;
  rdfs:range pds4:urn:nasa:pds:0001_nasa_pds_1:cart:vector_cartesian_unit_base:cart:vector_projection_x_axis::1.0.
 
pds4:urn:nasa:pds:0001_nasa_pds_1:all:user:cart:orthographic_lander::vector_projection_y_axis::1.0 rdf:type rdf:Property;
  rdfs:label "Vector_Projection_Y_Axis";
  rdfs:domain pds4:urn:nasa:pds:0001_nasa_pds_1:all:user:cart:orthographic_lander::1.0;
  rdfs:range pds4:urn:nasa:pds:0001_nasa_pds_1:cart:vector_cartesian_unit_base:cart:vector_projection_y_axis::1.0.
 
pds4:urn:nasa:pds:0001_nasa_pds_1:all:user:cart:orthographic_lander::vector_projection_z_axis::1.0 rdf:type rdf:Property;
  rdfs:label "Vector_Projection_Z_Axis";
  rdfs:domain pds4:urn:nasa:pds:0001_nasa_pds_1:all:user:cart:orthographic_lander::1.0;
  rdfs:range pds4:urn:nasa:pds:0001_nasa_pds_1:cart:vector_cartesian_unit_base:cart:vector_projection_z_axis::1.0.
 
pds4:urn:nasa:pds:0001_nasa_pds_1:all:user:cart:orthorectified::pixel_position_origin::1.0 rdf:type rdf:Property;
  rdfs:label "Pixel_Position_Origin";
  rdfs:domain pds4:urn:nasa:pds:0001_nasa_pds_1:all:user:cart:orthorectified::1.0;
  rdfs:range pds4:urn:nasa:pds:0001_nasa_pds_1:all:user:cart:pixel_position_origin::1.0.
 
pds4:urn:nasa:pds:0001_nasa_pds_1:all:user:cart:orthorectified::vector_projection_origin::1.0 rdf:type rdf:Property;
  rdfs:label "Vector_Projection_Origin";
  rdfs:domain pds4:urn:nasa:pds:0001_nasa_pds_1:all:user:cart:orthorectified::1.0;
  rdfs:range pds4:urn:nasa:pds:0001_nasa_pds_1:geom:vector_cartesian_position_base:cart:vector_projection_origin::1.0.
 
pds4:urn:nasa:pds:0001_nasa_pds_1:all:user:cart:orthorectified::vector_projection_x_axis::1.0 rdf:type rdf:Property;
  rdfs:label "Vector_Projection_X_Axis";
  rdfs:domain pds4:urn:nasa:pds:0001_nasa_pds_1:all:user:cart:orthorectified::1.0;
  rdfs:range pds4:urn:nasa:pds:0001_nasa_pds_1:cart:vector_cartesian_unit_base:cart:vector_projection_x_axis::1.0.
 
pds4:urn:nasa:pds:0001_nasa_pds_1:all:user:cart:orthorectified::vector_projection_y_axis::1.0 rdf:type rdf:Property;
  rdfs:label "Vector_Projection_Y_Axis";
  rdfs:domain pds4:urn:nasa:pds:0001_nasa_pds_1:all:user:cart:orthorectified::1.0;
  rdfs:range pds4:urn:nasa:pds:0001_nasa_pds_1:cart:vector_cartesian_unit_base:cart:vector_projection_y_axis::1.0.
 
pds4:urn:nasa:pds:0001_nasa_pds_1:all:user:cart:orthorectified::vector_projection_z_axis::1.0 rdf:type rdf:Property;
  rdfs:label "Vector_Projection_Z_Axis";
  rdfs:domain pds4:urn:nasa:pds:0001_nasa_pds_1:all:user:cart:orthorectified::1.0;
  rdfs:range pds4:urn:nasa:pds:0001_nasa_pds_1:cart:vector_cartesian_unit_base:cart:vector_projection_z_axis::1.0.
 
pds4:urn:nasa:pds:0001_nasa_pds_1:all:user:cart:perspective::camera_model_offset::1.0 rdf:type rdf:Property;
  rdfs:label "Camera_Model_Offset";
  rdfs:domain pds4:urn:nasa:pds:0001_nasa_pds_1:all:user:cart:perspective::1.0;
  rdfs:range pds4:urn:nasa:pds:0001_nasa_pds_1:all:user:cart:camera_model_offset::1.0.
 
pds4:urn:nasa:pds:0001_nasa_pds_1:all:user:cart:planar::map_projection::1.0 rdf:type rdf:Property;
  rdfs:label "Map_Projection";
  rdfs:domain pds4:urn:nasa:pds:0001_nasa_pds_1:all:user:cart:planar::1.0;
  rdfs:range pds4:urn:nasa:pds:0001_nasa_pds_1:all:user:cart:map_projection::1.0.
 
pds4:urn:nasa:pds:0001_nasa_pds_1:all:user:cart:planar::grid_coordinate_system::1.0 rdf:type rdf:Property;
  rdfs:label "Grid_Coordinate_System";
  rdfs:domain pds4:urn:nasa:pds:0001_nasa_pds_1:all:user:cart:planar::1.0;
  rdfs:range pds4:urn:nasa:pds:0001_nasa_pds_1:all:user:cart:grid_coordinate_system::1.0.
 
pds4:urn:nasa:pds:0001_nasa_pds_1:all:user:cart:planar::local_planar::1.0 rdf:type rdf:Property;
  rdfs:label "Local_Planar";
  rdfs:domain pds4:urn:nasa:pds:0001_nasa_pds_1:all:user:cart:planar::1.0;
  rdfs:range pds4:urn:nasa:pds:0001_nasa_pds_1:all:user:cart:local_planar::1.0.
 
pds4:urn:nasa:pds:0001_nasa_pds_1:all:user:cart:planar::planar_coordinate_information::1.0 rdf:type rdf:Property;
  rdfs:label "Planar_Coordinate_Information";
  rdfs:domain pds4:urn:nasa:pds:0001_nasa_pds_1:all:user:cart:planar::1.0;
  rdfs:range pds4:urn:nasa:pds:0001_nasa_pds_1:all:user:cart:planar_coordinate_information::1.0.
 
pds4:urn:nasa:pds:0001_nasa_pds_1:all:user:cart:planar::geo_transformation::1.0 rdf:type rdf:Property;
  rdfs:label "Geo_Transformation";
  rdfs:domain pds4:urn:nasa:pds:0001_nasa_pds_1:all:user:cart:planar::1.0;
  rdfs:range pds4:urn:nasa:pds:0001_nasa_pds_1:all:user:cart:geo_transformation::1.0.
 
pds4:urn:nasa:pds:0001_nasa_pds_1:all:user:cart:planar_coordinate_information::coordinate_representation::1.0 rdf:type rdf:Property;
  rdfs:label "Coordinate_Representation";
  rdfs:domain pds4:urn:nasa:pds:0001_nasa_pds_1:all:user:cart:planar_coordinate_information::1.0;
  rdfs:range pds4:urn:nasa:pds:0001_nasa_pds_1:all:user:cart:coordinate_representation::1.0.
 
pds4:urn:nasa:pds:0001_nasa_pds_1:all:user:cart:planar_coordinate_information::distance_and_bearing_representation::1.0 rdf:type rdf:Property;
  rdfs:label "Distance_and_Bearing_Representation";
  rdfs:domain pds4:urn:nasa:pds:0001_nasa_pds_1:all:user:cart:planar_coordinate_information::1.0;
  rdfs:range pds4:urn:nasa:pds:0001_nasa_pds_1:all:user:cart:distance_and_bearing_representation::1.0.
 
pds4:urn:nasa:pds:0001_nasa_pds_1:all:user:cart:polar::pixel_position_nadir_polar::1.0 rdf:type rdf:Property;
  rdfs:label "Pixel_Position_Nadir_Polar";
  rdfs:domain pds4:urn:nasa:pds:0001_nasa_pds_1:all:user:cart:polar::1.0;
  rdfs:range pds4:urn:nasa:pds:0001_nasa_pds_1:all:user:cart:pixel_position_nadir_polar::1.0.
 
pds4:urn:nasa:pds:0001_nasa_pds_1:all:user:cart:polar::vector_projection_origin::1.0 rdf:type rdf:Property;
  rdfs:label "Vector_Projection_Origin";
  rdfs:domain pds4:urn:nasa:pds:0001_nasa_pds_1:all:user:cart:polar::1.0;
  rdfs:range pds4:urn:nasa:pds:0001_nasa_pds_1:geom:vector_cartesian_position_base:cart:vector_projection_origin::1.0.
 
pds4:urn:nasa:pds:0001_nasa_pds_1:all:user:cart:secondary_spatial_domain::bounding_coordinates::1.0 rdf:type rdf:Property;
  rdfs:label "Bounding_Coordinates";
  rdfs:domain pds4:urn:nasa:pds:0001_nasa_pds_1:all:user:cart:secondary_spatial_domain::1.0;
  rdfs:range pds4:urn:nasa:pds:0001_nasa_pds_1:all:user:cart:bounding_coordinates::1.0.
 
pds4:urn:nasa:pds:0001_nasa_pds_1:all:user:cart:spatial_domain::bounding_coordinates::1.0 rdf:type rdf:Property;
  rdfs:label "Bounding_Coordinates";
  rdfs:domain pds4:urn:nasa:pds:0001_nasa_pds_1:all:user:cart:spatial_domain::1.0;
  rdfs:range pds4:urn:nasa:pds:0001_nasa_pds_1:all:user:cart:bounding_coordinates::1.0.
 
pds4:urn:nasa:pds:0001_nasa_pds_1:all:user:cart:spatial_reference_information::horizontal_coordinate_system_definition::1.0 rdf:type rdf:Property;
  rdfs:label "Horizontal_Coordinate_System_Definition";
  rdfs:domain pds4:urn:nasa:pds:0001_nasa_pds_1:all:user:cart:spatial_reference_information::1.0;
  rdfs:range pds4:urn:nasa:pds:0001_nasa_pds_1:all:user:cart:horizontal_coordinate_system_definition::1.0.
 
pds4:urn:nasa:pds:0001_nasa_pds_1:all:user:cart:state_plane_coordinate_system::lambert_conformal_conic::1.0 rdf:type rdf:Property;
  rdfs:label "Lambert_Conformal_Conic";
  rdfs:domain pds4:urn:nasa:pds:0001_nasa_pds_1:all:user:cart:state_plane_coordinate_system::1.0;
  rdfs:range pds4:urn:nasa:pds:0001_nasa_pds_1:all:user:cart:lambert_conformal_conic::1.0.
 
pds4:urn:nasa:pds:0001_nasa_pds_1:all:user:cart:state_plane_coordinate_system::transverse_mercator::1.0 rdf:type rdf:Property;
  rdfs:label "Transverse_Mercator";
  rdfs:domain pds4:urn:nasa:pds:0001_nasa_pds_1:all:user:cart:state_plane_coordinate_system::1.0;
  rdfs:range pds4:urn:nasa:pds:0001_nasa_pds_1:all:user:cart:transverse_mercator::1.0.
 
pds4:urn:nasa:pds:0001_nasa_pds_1:all:user:cart:state_plane_coordinate_system::oblique_mercator::1.0 rdf:type rdf:Property;
  rdfs:label "Oblique_Mercator";
  rdfs:domain pds4:urn:nasa:pds:0001_nasa_pds_1:all:user:cart:state_plane_coordinate_system::1.0;
  rdfs:range pds4:urn:nasa:pds:0001_nasa_pds_1:all:user:cart:oblique_mercator::1.0.
 
pds4:urn:nasa:pds:0001_nasa_pds_1:all:user:cart:state_plane_coordinate_system::polyconic::1.0 rdf:type rdf:Property;
  rdfs:label "Polyconic";
  rdfs:domain pds4:urn:nasa:pds:0001_nasa_pds_1:all:user:cart:state_plane_coordinate_system::1.0;
  rdfs:range pds4:urn:nasa:pds:0001_nasa_pds_1:all:user:cart:polyconic::1.0.
 
pds4:urn:nasa:pds:0001_nasa_pds_1:all:user:cart:surface_model_parameters::surface_model_planar::1.0 rdf:type rdf:Property;
  rdfs:label "Surface_Model_Planar";
  rdfs:domain pds4:urn:nasa:pds:0001_nasa_pds_1:all:user:cart:surface_model_parameters::1.0;
  rdfs:range pds4:urn:nasa:pds:0001_nasa_pds_1:all:user:cart:surface_model_planar::1.0.
 
pds4:urn:nasa:pds:0001_nasa_pds_1:all:user:cart:surface_model_parameters::surface_model_spherical::1.0 rdf:type rdf:Property;
  rdfs:label "Surface_Model_Spherical";
  rdfs:domain pds4:urn:nasa:pds:0001_nasa_pds_1:all:user:cart:surface_model_parameters::1.0;
  rdfs:range pds4:urn:nasa:pds:0001_nasa_pds_1:all:user:cart:surface_model_spherical::1.0.
 
pds4:urn:nasa:pds:0001_nasa_pds_1:all:user:cart:surface_model_planar::vector_surface_normal::1.0 rdf:type rdf:Property;
  rdfs:label "Vector_Surface_Normal";
  rdfs:domain pds4:urn:nasa:pds:0001_nasa_pds_1:all:user:cart:surface_model_planar::1.0;
  rdfs:range pds4:urn:nasa:pds:0001_nasa_pds_1:cart:vector_cartesian_unit_base:cart:vector_surface_normal::1.0.
 
pds4:urn:nasa:pds:0001_nasa_pds_1:all:user:cart:surface_model_planar::vector_surface_ground_location::1.0 rdf:type rdf:Property;
  rdfs:label "Vector_Surface_Ground_Location";
  rdfs:domain pds4:urn:nasa:pds:0001_nasa_pds_1:all:user:cart:surface_model_planar::1.0;
  rdfs:range pds4:urn:nasa:pds:0001_nasa_pds_1:geom:vector_cartesian_position_base:cart:vector_surface_ground_location::1.0.
 
pds4:urn:nasa:pds:0001_nasa_pds_1:all:user:cart:surface_model_spherical::vector_sphere_center::1.0 rdf:type rdf:Property;
  rdfs:label "Vector_Sphere_Center";
  rdfs:domain pds4:urn:nasa:pds:0001_nasa_pds_1:all:user:cart:surface_model_spherical::1.0;
  rdfs:range pds4:urn:nasa:pds:0001_nasa_pds_1:geom:vector_cartesian_position_base:cart:vector_sphere_center::1.0.
 
pds4:urn:nasa:pds:0001_nasa_pds_1:all:user:cart:universal_polar_stereographic::polar_stereographic::1.0 rdf:type rdf:Property;
  rdfs:label "Polar_Stereographic";
  rdfs:domain pds4:urn:nasa:pds:0001_nasa_pds_1:all:user:cart:universal_polar_stereographic::1.0;
  rdfs:range pds4:urn:nasa:pds:0001_nasa_pds_1:all:user:cart:polar_stereographic::1.0.
 
pds4:urn:nasa:pds:0001_nasa_pds_1:all:user:cart:universal_transverse_mercator::transverse_mercator::1.0 rdf:type rdf:Property;
  rdfs:label "Transverse_Mercator";
  rdfs:domain pds4:urn:nasa:pds:0001_nasa_pds_1:all:user:cart:universal_transverse_mercator::1.0;
  rdfs:range pds4:urn:nasa:pds:0001_nasa_pds_1:all:user:cart:transverse_mercator::1.0.
 
pds4:urn:nasa:pds:0001_nasa_pds_1:all:user:cart:vertical::pixel_position_origin::1.0 rdf:type rdf:Property;
  rdfs:label "Pixel_Position_Origin";
  rdfs:domain pds4:urn:nasa:pds:0001_nasa_pds_1:all:user:cart:vertical::1.0;
  rdfs:range pds4:urn:nasa:pds:0001_nasa_pds_1:all:user:cart:pixel_position_origin::1.0.
 
pds4:urn:nasa:pds:0001_nasa_pds_1:all:user:cart:vertical::vector_projection_origin::1.0 rdf:type rdf:Property;
  rdfs:label "Vector_Projection_Origin";
  rdfs:domain pds4:urn:nasa:pds:0001_nasa_pds_1:all:user:cart:vertical::1.0;
  rdfs:range pds4:urn:nasa:pds:0001_nasa_pds_1:geom:vector_cartesian_position_base:cart:vector_projection_origin::1.0.
 
pds4:urn:nasa:pds:0001_nasa_pds_1:all:user:disp:display_settings::local_internal_reference::1.0 rdf:type rdf:Property;
  rdfs:label "Local_Internal_Reference";
  rdfs:domain pds4:urn:nasa:pds:0001_nasa_pds_1:all:user:disp:display_settings::1.0;
  rdfs:range pds4:urn:nasa:pds:0001_nasa_pds_1:pds:product_components:pds:local_internal_reference::1.0.
 
pds4:urn:nasa:pds:0001_nasa_pds_1:all:user:disp:display_settings::display_direction::1.0 rdf:type rdf:Property;
  rdfs:label "Display_Direction";
  rdfs:domain pds4:urn:nasa:pds:0001_nasa_pds_1:all:user:disp:display_settings::1.0;
  rdfs:range pds4:urn:nasa:pds:0001_nasa_pds_1:all:user:disp:display_direction::1.0.
 
pds4:urn:nasa:pds:0001_nasa_pds_1:all:user:disp:display_settings::color_display_settings::1.0 rdf:type rdf:Property;
  rdfs:label "Color_Display_Settings";
  rdfs:domain pds4:urn:nasa:pds:0001_nasa_pds_1:all:user:disp:display_settings::1.0;
  rdfs:range pds4:urn:nasa:pds:0001_nasa_pds_1:all:user:disp:color_display_settings::1.0.
 
pds4:urn:nasa:pds:0001_nasa_pds_1:all:user:disp:display_settings::movie_display_settings::1.0 rdf:type rdf:Property;
  rdfs:label "Movie_Display_Settings";
  rdfs:domain pds4:urn:nasa:pds:0001_nasa_pds_1:all:user:disp:display_settings::1.0;
  rdfs:range pds4:urn:nasa:pds:0001_nasa_pds_1:all:user:disp:movie_display_settings::1.0.
 
pds4:urn:nasa:pds:0001_nasa_pds_1:all:user:geom:articulation_device_parameters::device_angle::1.0 rdf:type rdf:Property;
  rdfs:label "Device_Angle";
  rdfs:domain pds4:urn:nasa:pds:0001_nasa_pds_1:all:user:geom:articulation_device_parameters::1.0;
  rdfs:range pds4:urn:nasa:pds:0001_nasa_pds_1:all:user:geom:device_angle::1.0.
 
pds4:urn:nasa:pds:0001_nasa_pds_1:all:user:geom:articulation_device_parameters::device_component_state::1.0 rdf:type rdf:Property;
  rdfs:label "Device_Component_State";
  rdfs:domain pds4:urn:nasa:pds:0001_nasa_pds_1:all:user:geom:articulation_device_parameters::1.0;
  rdfs:range pds4:urn:nasa:pds:0001_nasa_pds_1:all:user:geom:device_component_state::1.0.
 
pds4:urn:nasa:pds:0001_nasa_pds_1:all:user:geom:articulation_device_parameters::device_motor_counts::1.0 rdf:type rdf:Property;
  rdfs:label "Device_Motor_Counts";
  rdfs:domain pds4:urn:nasa:pds:0001_nasa_pds_1:all:user:geom:articulation_device_parameters::1.0;
  rdfs:range pds4:urn:nasa:pds:0001_nasa_pds_1:all:user:geom:device_motor_counts::1.0.
 
pds4:urn:nasa:pds:0001_nasa_pds_1:all:user:geom:articulation_device_parameters::device_pose::1.0 rdf:type rdf:Property;
  rdfs:label "Device_Pose";
  rdfs:domain pds4:urn:nasa:pds:0001_nasa_pds_1:all:user:geom:articulation_device_parameters::1.0;
  rdfs:range pds4:urn:nasa:pds:0001_nasa_pds_1:all:user:geom:device_pose::1.0.
 
pds4:urn:nasa:pds:0001_nasa_pds_1:all:user:geom:articulation_device_parameters::vector_device_gravity::1.0 rdf:type rdf:Property;
  rdfs:label "Vector_Device_Gravity";
  rdfs:domain pds4:urn:nasa:pds:0001_nasa_pds_1:all:user:geom:articulation_device_parameters::1.0;
  rdfs:range pds4:urn:nasa:pds:0001_nasa_pds_1:geom:vector_cartesian_unit:geom:vector_device_gravity::1.0.
 
pds4:urn:nasa:pds:0001_nasa_pds_1:all:user:geom:articulation_device_parameters::vector_device_gravity_magnitude::1.0 rdf:type rdf:Property;
  rdfs:label "Vector_Device_Gravity_Magnitude";
  rdfs:domain pds4:urn:nasa:pds:0001_nasa_pds_1:all:user:geom:articulation_device_parameters::1.0;
  rdfs:range pds4:urn:nasa:pds:0001_nasa_pds_1:geom:vector_cartesian_acceleration_base:geom:vector_device_gravity_magnitude::1.0.
 
pds4:urn:nasa:pds:0001_nasa_pds_1:all:user:geom:articulation_device_parameters::device_temperature::1.0 rdf:type rdf:Property;
  rdfs:label "Device_Temperature";
  rdfs:domain pds4:urn:nasa:pds:0001_nasa_pds_1:all:user:geom:articulation_device_parameters::1.0;
  rdfs:range pds4:urn:nasa:pds:0001_nasa_pds_1:all:user:geom:device_temperature::1.0.
 
pds4:urn:nasa:pds:0001_nasa_pds_1:all:user:geom:articulation_device_parameters::coordinate_space_present::1.0 rdf:type rdf:Property;
  rdfs:label "Coordinate_Space_Present";
  rdfs:domain pds4:urn:nasa:pds:0001_nasa_pds_1:all:user:geom:articulation_device_parameters::1.0;
  rdfs:range pds4:urn:nasa:pds:0001_nasa_pds_1:geom:coordinate_space_identification:geom:coordinate_space_present::1.0.
 
pds4:urn:nasa:pds:0001_nasa_pds_1:all:user:geom:articulation_device_parameters::coordinate_space_reference::1.0 rdf:type rdf:Property;
  rdfs:label "Coordinate_Space_Reference";
  rdfs:domain pds4:urn:nasa:pds:0001_nasa_pds_1:all:user:geom:articulation_device_parameters::1.0;
  rdfs:range pds4:urn:nasa:pds:0001_nasa_pds_1:geom:coordinate_space_identification:geom:coordinate_space_reference::1.0.
 
pds4:urn:nasa:pds:0001_nasa_pds_1:all:user:geom:articulation_device_parameters::commanded_geometry::1.0 rdf:type rdf:Property;
  rdfs:label "Commanded_Geometry";
  rdfs:domain pds4:urn:nasa:pds:0001_nasa_pds_1:all:user:geom:articulation_device_parameters::1.0;
  rdfs:range pds4:urn:nasa:pds:0001_nasa_pds_1:all:user:geom:commanded_geometry::1.0.
 
pds4:urn:nasa:pds:0001_nasa_pds_1:all:user:geom:body_identification_base::internal_reference::1.0 rdf:type rdf:Property;
  rdfs:label "Internal_Reference";
  rdfs:domain pds4:urn:nasa:pds:0001_nasa_pds_1:all:user:geom:body_identification_base::1.0;
  rdfs:range pds4:urn:nasa:pds:0001_nasa_pds_1:pds:product_components:pds:internal_reference::1.0.
 
pds4:urn:nasa:pds:0001_nasa_pds_1:geom:cahvor_model:geom:cahvore_model::entrance_terms::1.0 rdf:type rdf:Property;
  rdfs:label "Entrance_Terms";
  rdfs:domain pds4:urn:nasa:pds:0001_nasa_pds_1:geom:cahvor_model:geom:cahvore_model::1.0;
  rdfs:range pds4:urn:nasa:pds:0001_nasa_pds_1:geom:polynomial_coefficients_3:geom:entrance_terms::1.0.
 
pds4:urn:nasa:pds:0001_nasa_pds_1:geom:cahv_model:geom:cahvor_model::vector_optical::1.0 rdf:type rdf:Property;
  rdfs:label "Vector_Optical";
  rdfs:domain pds4:urn:nasa:pds:0001_nasa_pds_1:geom:cahv_model:geom:cahvor_model::1.0;
  rdfs:range pds4:urn:nasa:pds:0001_nasa_pds_1:geom:vector_cartesian_unit:geom:vector_optical::1.0.
 
pds4:urn:nasa:pds:0001_nasa_pds_1:geom:cahv_model:geom:cahvor_model::radial_terms::1.0 rdf:type rdf:Property;
  rdfs:label "Radial_Terms";
  rdfs:domain pds4:urn:nasa:pds:0001_nasa_pds_1:geom:cahv_model:geom:cahvor_model::1.0;
  rdfs:range pds4:urn:nasa:pds:0001_nasa_pds_1:geom:polynomial_coefficients_3:geom:radial_terms::1.0.
 
pds4:urn:nasa:pds:0001_nasa_pds_1:all:user:geom:cahv_model::vector_center::1.0 rdf:type rdf:Property;
  rdfs:label "Vector_Center";
  rdfs:domain pds4:urn:nasa:pds:0001_nasa_pds_1:all:user:geom:cahv_model::1.0;
  rdfs:range pds4:urn:nasa:pds:0001_nasa_pds_1:geom:vector_cartesian_position_base:geom:vector_center::1.0.
 
pds4:urn:nasa:pds:0001_nasa_pds_1:all:user:geom:cahv_model::vector_axis::1.0 rdf:type rdf:Property;
  rdfs:label "Vector_Axis";
  rdfs:domain pds4:urn:nasa:pds:0001_nasa_pds_1:all:user:geom:cahv_model::1.0;
  rdfs:range pds4:urn:nasa:pds:0001_nasa_pds_1:geom:vector_cartesian_unit:geom:vector_axis::1.0.
 
pds4:urn:nasa:pds:0001_nasa_pds_1:all:user:geom:cahv_model::vector_horizontal::1.0 rdf:type rdf:Property;
  rdfs:label "Vector_Horizontal";
  rdfs:domain pds4:urn:nasa:pds:0001_nasa_pds_1:all:user:geom:cahv_model::1.0;
  rdfs:range pds4:urn:nasa:pds:0001_nasa_pds_1:geom:vector_cartesian_pixel:geom:vector_horizontal::1.0.
 
pds4:urn:nasa:pds:0001_nasa_pds_1:all:user:geom:cahv_model::vector_vertical::1.0 rdf:type rdf:Property;
  rdfs:label "Vector_Vertical";
  rdfs:domain pds4:urn:nasa:pds:0001_nasa_pds_1:all:user:geom:cahv_model::1.0;
  rdfs:range pds4:urn:nasa:pds:0001_nasa_pds_1:geom:vector_cartesian_pixel:geom:vector_vertical::1.0.
 
pds4:urn:nasa:pds:0001_nasa_pds_1:all:user:geom:camera_model_parameters::internal_reference::1.0 rdf:type rdf:Property;
  rdfs:label "Internal_Reference";
  rdfs:domain pds4:urn:nasa:pds:0001_nasa_pds_1:all:user:geom:camera_model_parameters::1.0;
  rdfs:range pds4:urn:nasa:pds:0001_nasa_pds_1:pds:product_components:pds:internal_reference::1.0.
 
pds4:urn:nasa:pds:0001_nasa_pds_1:all:user:geom:camera_model_parameters::cahv_model::1.0 rdf:type rdf:Property;
  rdfs:label "CAHV_Model";
  rdfs:domain pds4:urn:nasa:pds:0001_nasa_pds_1:all:user:geom:camera_model_parameters::1.0;
  rdfs:range pds4:urn:nasa:pds:0001_nasa_pds_1:all:user:geom:cahv_model::1.0.
 
pds4:urn:nasa:pds:0001_nasa_pds_1:all:user:geom:camera_model_parameters::cahvor_model::1.0 rdf:type rdf:Property;
  rdfs:label "CAHVOR_Model";
  rdfs:domain pds4:urn:nasa:pds:0001_nasa_pds_1:all:user:geom:camera_model_parameters::1.0;
  rdfs:range pds4:urn:nasa:pds:0001_nasa_pds_1:geom:cahv_model:geom:cahvor_model::1.0.
 
pds4:urn:nasa:pds:0001_nasa_pds_1:all:user:geom:camera_model_parameters::cahvore_model::1.0 rdf:type rdf:Property;
  rdfs:label "CAHVORE_Model";
  rdfs:domain pds4:urn:nasa:pds:0001_nasa_pds_1:all:user:geom:camera_model_parameters::1.0;
  rdfs:range pds4:urn:nasa:pds:0001_nasa_pds_1:geom:cahvor_model:geom:cahvore_model::1.0.
 
pds4:urn:nasa:pds:0001_nasa_pds_1:all:user:geom:camera_model_parameters::psph_model::1.0 rdf:type rdf:Property;
  rdfs:label "PSPH_Model";
  rdfs:domain pds4:urn:nasa:pds:0001_nasa_pds_1:all:user:geom:camera_model_parameters::1.0;
  rdfs:range pds4:urn:nasa:pds:0001_nasa_pds_1:all:user:geom:psph_model::1.0.
 
pds4:urn:nasa:pds:0001_nasa_pds_1:all:user:geom:camera_model_parameters::reference_frame_identification::1.0 rdf:type rdf:Property;
  rdfs:label "Reference_Frame_Identification";
  rdfs:domain pds4:urn:nasa:pds:0001_nasa_pds_1:all:user:geom:camera_model_parameters::1.0;
  rdfs:range pds4:urn:nasa:pds:0001_nasa_pds_1:geom:frame_identification_base:geom:reference_frame_identification::1.0.
 
pds4:urn:nasa:pds:0001_nasa_pds_1:all:user:geom:camera_model_parameters::coordinate_space_reference::1.0 rdf:type rdf:Property;
  rdfs:label "Coordinate_Space_Reference";
  rdfs:domain pds4:urn:nasa:pds:0001_nasa_pds_1:all:user:geom:camera_model_parameters::1.0;
  rdfs:range pds4:urn:nasa:pds:0001_nasa_pds_1:geom:coordinate_space_identification:geom:coordinate_space_reference::1.0.
 
pds4:urn:nasa:pds:0001_nasa_pds_1:all:user:geom:camera_model_parameters::quaternion_model_transform::1.0 rdf:type rdf:Property;
  rdfs:label "Quaternion_Model_Transform";
  rdfs:domain pds4:urn:nasa:pds:0001_nasa_pds_1:all:user:geom:camera_model_parameters::1.0;
  rdfs:range pds4:urn:nasa:pds:0001_nasa_pds_1:geom:quaternion_base:geom:quaternion_model_transform::1.0.
 
pds4:urn:nasa:pds:0001_nasa_pds_1:all:user:geom:camera_model_parameters::vector_model_transform::1.0 rdf:type rdf:Property;
  rdfs:label "Vector_Model_Transform";
  rdfs:domain pds4:urn:nasa:pds:0001_nasa_pds_1:all:user:geom:camera_model_parameters::1.0;
  rdfs:range pds4:urn:nasa:pds:0001_nasa_pds_1:geom:vector_cartesian_no_units:geom:vector_model_transform::1.0.
 
pds4:urn:nasa:pds:0001_nasa_pds_1:all:user:geom:camera_model_parameters::interpolation::1.0 rdf:type rdf:Property;
  rdfs:label "Interpolation";
  rdfs:domain pds4:urn:nasa:pds:0001_nasa_pds_1:all:user:geom:camera_model_parameters::1.0;
  rdfs:range pds4:urn:nasa:pds:0001_nasa_pds_1:all:user:geom:interpolation::1.0.
 
pds4:urn:nasa:pds:0001_nasa_pds_1:all:user:geom:commanded_geometry::device_angle::1.0 rdf:type rdf:Property;
  rdfs:label "Device_Angle";
  rdfs:domain pds4:urn:nasa:pds:0001_nasa_pds_1:all:user:geom:commanded_geometry::1.0;
  rdfs:range pds4:urn:nasa:pds:0001_nasa_pds_1:all:user:geom:device_angle::1.0.
 
pds4:urn:nasa:pds:0001_nasa_pds_1:all:user:geom:commanded_geometry::commanded_position::1.0 rdf:type rdf:Property;
  rdfs:label "Commanded_Position";
  rdfs:domain pds4:urn:nasa:pds:0001_nasa_pds_1:all:user:geom:commanded_geometry::1.0;
  rdfs:range pds4:urn:nasa:pds:0001_nasa_pds_1:geom:vector_cartesian_position_base:geom:commanded_position::1.0.
 
pds4:urn:nasa:pds:0001_nasa_pds_1:all:user:geom:commanded_geometry::coordinate_space_reference::1.0 rdf:type rdf:Property;
  rdfs:label "Coordinate_Space_Reference";
  rdfs:domain pds4:urn:nasa:pds:0001_nasa_pds_1:all:user:geom:commanded_geometry::1.0;
  rdfs:range pds4:urn:nasa:pds:0001_nasa_pds_1:geom:coordinate_space_identification:geom:coordinate_space_reference::1.0.
 
pds4:urn:nasa:pds:0001_nasa_pds_1:all:user:geom:coordinate_space_definition::coordinate_space_present::1.0 rdf:type rdf:Property;
  rdfs:label "Coordinate_Space_Present";
  rdfs:domain pds4:urn:nasa:pds:0001_nasa_pds_1:all:user:geom:coordinate_space_definition::1.0;
  rdfs:range pds4:urn:nasa:pds:0001_nasa_pds_1:geom:coordinate_space_identification:geom:coordinate_space_present::1.0.
 
pds4:urn:nasa:pds:0001_nasa_pds_1:all:user:geom:coordinate_space_definition::vector_origin_offset::1.0 rdf:type rdf:Property;
  rdfs:label "Vector_Origin_Offset";
  rdfs:domain pds4:urn:nasa:pds:0001_nasa_pds_1:all:user:geom:coordinate_space_definition::1.0;
  rdfs:range pds4:urn:nasa:pds:0001_nasa_pds_1:geom:vector_cartesian_position_base:geom:vector_origin_offset::1.0.
 
pds4:urn:nasa:pds:0001_nasa_pds_1:all:user:geom:coordinate_space_definition::quaternion_plus_direction::1.0 rdf:type rdf:Property;
  rdfs:label "Quaternion_Plus_Direction";
  rdfs:domain pds4:urn:nasa:pds:0001_nasa_pds_1:all:user:geom:coordinate_space_definition::1.0;
  rdfs:range pds4:urn:nasa:pds:0001_nasa_pds_1:geom:quaternion_base:geom:quaternion_plus_direction::1.0.
 
pds4:urn:nasa:pds:0001_nasa_pds_1:all:user:geom:coordinate_space_definition::coordinate_space_reference::1.0 rdf:type rdf:Property;
  rdfs:label "Coordinate_Space_Reference";
  rdfs:domain pds4:urn:nasa:pds:0001_nasa_pds_1:all:user:geom:coordinate_space_definition::1.0;
  rdfs:range pds4:urn:nasa:pds:0001_nasa_pds_1:geom:coordinate_space_identification:geom:coordinate_space_reference::1.0.
 
pds4:urn:nasa:pds:0001_nasa_pds_1:all:user:geom:coordinate_space_definition::coordinate_space_quality::1.0 rdf:type rdf:Property;
  rdfs:label "Coordinate_Space_Quality";
  rdfs:domain pds4:urn:nasa:pds:0001_nasa_pds_1:all:user:geom:coordinate_space_definition::1.0;
  rdfs:range pds4:urn:nasa:pds:0001_nasa_pds_1:all:user:geom:coordinate_space_quality::1.0.
 
pds4:urn:nasa:pds:0001_nasa_pds_1:all:user:geom:coordinate_space_identification::coordinate_space_indexed::1.0 rdf:type rdf:Property;
  rdfs:label "Coordinate_Space_Indexed";
  rdfs:domain pds4:urn:nasa:pds:0001_nasa_pds_1:all:user:geom:coordinate_space_identification::1.0;
  rdfs:range pds4:urn:nasa:pds:0001_nasa_pds_1:all:user:geom:coordinate_space_indexed::1.0.
 
pds4:urn:nasa:pds:0001_nasa_pds_1:all:user:geom:coordinate_space_identification::coordinate_space_spice::1.0 rdf:type rdf:Property;
  rdfs:label "Coordinate_Space_SPICE";
  rdfs:domain pds4:urn:nasa:pds:0001_nasa_pds_1:all:user:geom:coordinate_space_identification::1.0;
  rdfs:range pds4:urn:nasa:pds:0001_nasa_pds_1:all:user:geom:coordinate_space_spice::1.0.
 
pds4:urn:nasa:pds:0001_nasa_pds_1:all:user:geom:coordinate_space_identification::local_internal_reference::1.0 rdf:type rdf:Property;
  rdfs:label "Local_Internal_Reference";
  rdfs:domain pds4:urn:nasa:pds:0001_nasa_pds_1:all:user:geom:coordinate_space_identification::1.0;
  rdfs:range pds4:urn:nasa:pds:0001_nasa_pds_1:pds:product_components:pds:local_internal_reference::1.0.
 
pds4:urn:nasa:pds:0001_nasa_pds_1:all:user:geom:coordinate_space_indexed::coordinate_space_index::1.0 rdf:type rdf:Property;
  rdfs:label "Coordinate_Space_Index";
  rdfs:domain pds4:urn:nasa:pds:0001_nasa_pds_1:all:user:geom:coordinate_space_indexed::1.0;
  rdfs:range pds4:urn:nasa:pds:0001_nasa_pds_1:geom:list_index_no_units:geom:coordinate_space_index::1.0.
 
pds4:urn:nasa:pds:0001_nasa_pds_1:all:user:geom:coordinate_system_identification::coordinate_system_origin_identification::1.0 rdf:type rdf:Property;
  rdfs:label "Coordinate_System_Origin_Identification";
  rdfs:domain pds4:urn:nasa:pds:0001_nasa_pds_1:all:user:geom:coordinate_system_identification::1.0;
  rdfs:range pds4:urn:nasa:pds:0001_nasa_pds_1:geom:body_identification_base:geom:coordinate_system_origin_identification::1.0.
 
pds4:urn:nasa:pds:0001_nasa_pds_1:all:user:geom:coordinate_system_identification::reference_frame_identification::1.0 rdf:type rdf:Property;
  rdfs:label "Reference_Frame_Identification";
  rdfs:domain pds4:urn:nasa:pds:0001_nasa_pds_1:all:user:geom:coordinate_system_identification::1.0;
  rdfs:range pds4:urn:nasa:pds:0001_nasa_pds_1:geom:frame_identification_base:geom:reference_frame_identification::1.0.
 
pds4:urn:nasa:pds:0001_nasa_pds_1:all:user:geom:derived_geometry::vector_solar_direction::1.0 rdf:type rdf:Property;
  rdfs:label "Vector_Solar_Direction";
  rdfs:domain pds4:urn:nasa:pds:0001_nasa_pds_1:all:user:geom:derived_geometry::1.0;
  rdfs:range pds4:urn:nasa:pds:0001_nasa_pds_1:geom:vector_cartesian_unit:geom:vector_solar_direction::1.0.
 
pds4:urn:nasa:pds:0001_nasa_pds_1:all:user:geom:derived_geometry::coordinate_space_reference::1.0 rdf:type rdf:Property;
  rdfs:label "Coordinate_Space_Reference";
  rdfs:domain pds4:urn:nasa:pds:0001_nasa_pds_1:all:user:geom:derived_geometry::1.0;
  rdfs:range pds4:urn:nasa:pds:0001_nasa_pds_1:geom:coordinate_space_identification:geom:coordinate_space_reference::1.0.
 
pds4:urn:nasa:pds:0001_nasa_pds_1:all:user:geom:device_angle::device_angle_index::1.0 rdf:type rdf:Property;
  rdfs:label "Device_Angle_Index";
  rdfs:domain pds4:urn:nasa:pds:0001_nasa_pds_1:all:user:geom:device_angle::1.0;
  rdfs:range pds4:urn:nasa:pds:0001_nasa_pds_1:geom:list_index_angle:geom:device_angle_index::1.0.
 
pds4:urn:nasa:pds:0001_nasa_pds_1:all:user:geom:device_component_state::device_component_state_index::1.0 rdf:type rdf:Property;
  rdfs:label "Device_Component_State_Index";
  rdfs:domain pds4:urn:nasa:pds:0001_nasa_pds_1:all:user:geom:device_component_state::1.0;
  rdfs:range pds4:urn:nasa:pds:0001_nasa_pds_1:geom:list_index_text:geom:device_component_state_index::1.0.
 
pds4:urn:nasa:pds:0001_nasa_pds_1:all:user:geom:device_motor_counts::device_motor_counts_index::1.0 rdf:type rdf:Property;
  rdfs:label "Device_Motor_Counts_Index";
  rdfs:domain pds4:urn:nasa:pds:0001_nasa_pds_1:all:user:geom:device_motor_counts::1.0;
  rdfs:range pds4:urn:nasa:pds:0001_nasa_pds_1:geom:list_index_no_units:geom:device_motor_counts_index::1.0.
 
pds4:urn:nasa:pds:0001_nasa_pds_1:all:user:geom:device_pose::quaternion_plus_direction::1.0 rdf:type rdf:Property;
  rdfs:label "Quaternion_Plus_Direction";
  rdfs:domain pds4:urn:nasa:pds:0001_nasa_pds_1:all:user:geom:device_pose::1.0;
  rdfs:range pds4:urn:nasa:pds:0001_nasa_pds_1:geom:quaternion_base:geom:quaternion_plus_direction::1.0.
 
pds4:urn:nasa:pds:0001_nasa_pds_1:all:user:geom:device_pose::vector_origin_offset::1.0 rdf:type rdf:Property;
  rdfs:label "Vector_Origin_Offset";
  rdfs:domain pds4:urn:nasa:pds:0001_nasa_pds_1:all:user:geom:device_pose::1.0;
  rdfs:range pds4:urn:nasa:pds:0001_nasa_pds_1:geom:vector_cartesian_position_base:geom:vector_origin_offset::1.0.
 
pds4:urn:nasa:pds:0001_nasa_pds_1:all:user:geom:device_temperature::device_temperature_index::1.0 rdf:type rdf:Property;
  rdfs:label "Device_Temperature_Index";
  rdfs:domain pds4:urn:nasa:pds:0001_nasa_pds_1:all:user:geom:device_temperature::1.0;
  rdfs:range pds4:urn:nasa:pds:0001_nasa_pds_1:geom:list_index_temperature:geom:device_temperature_index::1.0.
 
pds4:urn:nasa:pds:0001_nasa_pds_1:all:user:geom:distance_generic::observer_identification::1.0 rdf:type rdf:Property;
  rdfs:label "Observer_Identification";
  rdfs:domain pds4:urn:nasa:pds:0001_nasa_pds_1:all:user:geom:distance_generic::1.0;
  rdfs:range pds4:urn:nasa:pds:0001_nasa_pds_1:geom:body_identification_base:geom:observer_identification::1.0.
 
pds4:urn:nasa:pds:0001_nasa_pds_1:all:user:geom:distance_generic::geometry_target_identification::1.0 rdf:type rdf:Property;
  rdfs:label "Geometry_Target_Identification";
  rdfs:domain pds4:urn:nasa:pds:0001_nasa_pds_1:all:user:geom:distance_generic::1.0;
  rdfs:range pds4:urn:nasa:pds:0001_nasa_pds_1:geom:body_identification_base:geom:geometry_target_identification::1.0.
 
pds4:urn:nasa:pds:0001_nasa_pds_1:all:user:geom:distances::distances_specific::1.0 rdf:type rdf:Property;
  rdfs:label "Distances_Specific";
  rdfs:domain pds4:urn:nasa:pds:0001_nasa_pds_1:all:user:geom:distances::1.0;
  rdfs:range pds4:urn:nasa:pds:0001_nasa_pds_1:all:user:geom:distances_specific::1.0.
 
pds4:urn:nasa:pds:0001_nasa_pds_1:all:user:geom:distances::distances_min_max::1.0 rdf:type rdf:Property;
  rdfs:label "Distances_Min_Max";
  rdfs:domain pds4:urn:nasa:pds:0001_nasa_pds_1:all:user:geom:distances::1.0;
  rdfs:range pds4:urn:nasa:pds:0001_nasa_pds_1:all:user:geom:distances_min_max::1.0.
 
pds4:urn:nasa:pds:0001_nasa_pds_1:all:user:geom:distances::distances_start_stop::1.0 rdf:type rdf:Property;
  rdfs:label "Distances_Start_Stop";
  rdfs:domain pds4:urn:nasa:pds:0001_nasa_pds_1:all:user:geom:distances::1.0;
  rdfs:range pds4:urn:nasa:pds:0001_nasa_pds_1:all:user:geom:distances_start_stop::1.0.
 
pds4:urn:nasa:pds:0001_nasa_pds_1:all:user:geom:distances::distance_generic::1.0 rdf:type rdf:Property;
  rdfs:label "Distance_Generic";
  rdfs:domain pds4:urn:nasa:pds:0001_nasa_pds_1:all:user:geom:distances::1.0;
  rdfs:range pds4:urn:nasa:pds:0001_nasa_pds_1:all:user:geom:distance_generic::1.0.
 
pds4:urn:nasa:pds:0001_nasa_pds_1:all:user:geom:expanded_geometry::local_internal_reference::1.0 rdf:type rdf:Property;
  rdfs:label "Local_Internal_Reference";
  rdfs:domain pds4:urn:nasa:pds:0001_nasa_pds_1:all:user:geom:expanded_geometry::1.0;
  rdfs:range pds4:urn:nasa:pds:0001_nasa_pds_1:pds:product_components:pds:local_internal_reference::1.0.
 
pds4:urn:nasa:pds:0001_nasa_pds_1:all:user:geom:expanded_geometry::internal_reference::1.0 rdf:type rdf:Property;
  rdfs:label "Internal_Reference";
  rdfs:domain pds4:urn:nasa:pds:0001_nasa_pds_1:all:user:geom:expanded_geometry::1.0;
  rdfs:range pds4:urn:nasa:pds:0001_nasa_pds_1:pds:product_components:pds:internal_reference::1.0.
 
pds4:urn:nasa:pds:0001_nasa_pds_1:all:user:geom:footprint_vertices::pixel_intercept::1.0 rdf:type rdf:Property;
  rdfs:label "Pixel_Intercept";
  rdfs:domain pds4:urn:nasa:pds:0001_nasa_pds_1:all:user:geom:footprint_vertices::1.0;
  rdfs:range pds4:urn:nasa:pds:0001_nasa_pds_1:all:user:geom:pixel_intercept::1.0.
 
pds4:urn:nasa:pds:0001_nasa_pds_1:all:user:geom:frame_identification_base::internal_reference::1.0 rdf:type rdf:Property;
  rdfs:label "Internal_Reference";
  rdfs:domain pds4:urn:nasa:pds:0001_nasa_pds_1:all:user:geom:frame_identification_base::1.0;
  rdfs:range pds4:urn:nasa:pds:0001_nasa_pds_1:pds:product_components:pds:internal_reference::1.0.
 
pds4:urn:nasa:pds:0001_nasa_pds_1:all:user:geom:generic_vectors::vector_cartesian_position_generic::1.0 rdf:type rdf:Property;
  rdfs:label "Vector_Cartesian_Position_Generic";
  rdfs:domain pds4:urn:nasa:pds:0001_nasa_pds_1:all:user:geom:generic_vectors::1.0;
  rdfs:range pds4:urn:nasa:pds:0001_nasa_pds_1:geom:vector_cartesian_position_extended_base:geom:vector_cartesian_position_generic::1.0.
 
pds4:urn:nasa:pds:0001_nasa_pds_1:all:user:geom:generic_vectors::vector_cartesian_velocity_generic::1.0 rdf:type rdf:Property;
  rdfs:label "Vector_Cartesian_Velocity_Generic";
  rdfs:domain pds4:urn:nasa:pds:0001_nasa_pds_1:all:user:geom:generic_vectors::1.0;
  rdfs:range pds4:urn:nasa:pds:0001_nasa_pds_1:geom:vector_cartesian_velocity_extended_base:geom:vector_cartesian_velocity_generic::1.0.
 
pds4:urn:nasa:pds:0001_nasa_pds_1:all:user:geom:generic_vectors::vector_cartesian_acceleration_generic::1.0 rdf:type rdf:Property;
  rdfs:label "Vector_Cartesian_Acceleration_Generic";
  rdfs:domain pds4:urn:nasa:pds:0001_nasa_pds_1:all:user:geom:generic_vectors::1.0;
  rdfs:range pds4:urn:nasa:pds:0001_nasa_pds_1:geom:vector_cartesian_acceleration_extended_base:geom:vector_cartesian_acceleration_generic::1.0.
 
pds4:urn:nasa:pds:0001_nasa_pds_1:all:user:geom:generic_vectors::vector_planetocentric_position_generic::1.0 rdf:type rdf:Property;
  rdfs:label "Vector_Planetocentric_Position_Generic";
  rdfs:domain pds4:urn:nasa:pds:0001_nasa_pds_1:all:user:geom:generic_vectors::1.0;
  rdfs:range pds4:urn:nasa:pds:0001_nasa_pds_1:geom:vector_planetocentric_position_extended_base:geom:vector_planetocentric_position_generic::1.0.
 
pds4:urn:nasa:pds:0001_nasa_pds_1:all:user:geom:generic_vectors::vector_planetocentric_velocity_generic::1.0 rdf:type rdf:Property;
  rdfs:label "Vector_Planetocentric_Velocity_Generic";
  rdfs:domain pds4:urn:nasa:pds:0001_nasa_pds_1:all:user:geom:generic_vectors::1.0;
  rdfs:range pds4:urn:nasa:pds:0001_nasa_pds_1:geom:vector_planetocentric_velocity_extended_base:geom:vector_planetocentric_velocity_generic::1.0.
 
pds4:urn:nasa:pds:0001_nasa_pds_1:all:user:geom:geometry::spice_kernel_files::1.0 rdf:type rdf:Property;
  rdfs:label "SPICE_Kernel_Files";
  rdfs:domain pds4:urn:nasa:pds:0001_nasa_pds_1:all:user:geom:geometry::1.0;
  rdfs:range pds4:urn:nasa:pds:0001_nasa_pds_1:all:user:geom:spice_kernel_files::1.0.
 
pds4:urn:nasa:pds:0001_nasa_pds_1:all:user:geom:geometry::expanded_geometry::1.0 rdf:type rdf:Property;
  rdfs:label "Expanded_Geometry";
  rdfs:domain pds4:urn:nasa:pds:0001_nasa_pds_1:all:user:geom:geometry::1.0;
  rdfs:range pds4:urn:nasa:pds:0001_nasa_pds_1:all:user:geom:expanded_geometry::1.0.
 
pds4:urn:nasa:pds:0001_nasa_pds_1:all:user:geom:geometry::image_display_geometry::1.0 rdf:type rdf:Property;
  rdfs:label "Image_Display_Geometry";
  rdfs:domain pds4:urn:nasa:pds:0001_nasa_pds_1:all:user:geom:geometry::1.0;
  rdfs:range pds4:urn:nasa:pds:0001_nasa_pds_1:all:user:geom:image_display_geometry::1.0.
 
pds4:urn:nasa:pds:0001_nasa_pds_1:all:user:geom:geometry::geometry_orbiter::1.0 rdf:type rdf:Property;
  rdfs:label "Geometry_Orbiter";
  rdfs:domain pds4:urn:nasa:pds:0001_nasa_pds_1:all:user:geom:geometry::1.0;
  rdfs:range pds4:urn:nasa:pds:0001_nasa_pds_1:all:user:geom:geometry_orbiter::1.0.
 
pds4:urn:nasa:pds:0001_nasa_pds_1:all:user:geom:geometry::geometry_lander::1.0 rdf:type rdf:Property;
  rdfs:label "Geometry_Lander";
  rdfs:domain pds4:urn:nasa:pds:0001_nasa_pds_1:all:user:geom:geometry::1.0;
  rdfs:range pds4:urn:nasa:pds:0001_nasa_pds_1:all:user:geom:geometry_lander::1.0.
 
pds4:urn:nasa:pds:0001_nasa_pds_1:all:user:geom:geometry_lander::articulation_device_parameters::1.0 rdf:type rdf:Property;
  rdfs:label "Articulation_Device_Parameters";
  rdfs:domain pds4:urn:nasa:pds:0001_nasa_pds_1:all:user:geom:geometry_lander::1.0;
  rdfs:range pds4:urn:nasa:pds:0001_nasa_pds_1:all:user:geom:articulation_device_parameters::1.0.
 
pds4:urn:nasa:pds:0001_nasa_pds_1:all:user:geom:geometry_lander::camera_model_parameters::1.0 rdf:type rdf:Property;
  rdfs:label "Camera_Model_Parameters";
  rdfs:domain pds4:urn:nasa:pds:0001_nasa_pds_1:all:user:geom:geometry_lander::1.0;
  rdfs:range pds4:urn:nasa:pds:0001_nasa_pds_1:all:user:geom:camera_model_parameters::1.0.
 
pds4:urn:nasa:pds:0001_nasa_pds_1:all:user:geom:geometry_lander::coordinate_space_definition::1.0 rdf:type rdf:Property;
  rdfs:label "Coordinate_Space_Definition";
  rdfs:domain pds4:urn:nasa:pds:0001_nasa_pds_1:all:user:geom:geometry_lander::1.0;
  rdfs:range pds4:urn:nasa:pds:0001_nasa_pds_1:all:user:geom:coordinate_space_definition::1.0.
 
pds4:urn:nasa:pds:0001_nasa_pds_1:all:user:geom:geometry_lander::derived_geometry::1.0 rdf:type rdf:Property;
  rdfs:label "Derived_Geometry";
  rdfs:domain pds4:urn:nasa:pds:0001_nasa_pds_1:all:user:geom:geometry_lander::1.0;
  rdfs:range pds4:urn:nasa:pds:0001_nasa_pds_1:all:user:geom:derived_geometry::1.0.
 
pds4:urn:nasa:pds:0001_nasa_pds_1:all:user:geom:geometry_lander::motion_counter::1.0 rdf:type rdf:Property;
  rdfs:label "Motion_Counter";
  rdfs:domain pds4:urn:nasa:pds:0001_nasa_pds_1:all:user:geom:geometry_lander::1.0;
  rdfs:range pds4:urn:nasa:pds:0001_nasa_pds_1:all:user:geom:motion_counter::1.0.
 
pds4:urn:nasa:pds:0001_nasa_pds_1:all:user:geom:geometry_orbiter::orbiter_identification::1.0 rdf:type rdf:Property;
  rdfs:label "Orbiter_Identification";
  rdfs:domain pds4:urn:nasa:pds:0001_nasa_pds_1:all:user:geom:geometry_orbiter::1.0;
  rdfs:range pds4:urn:nasa:pds:0001_nasa_pds_1:all:user:geom:orbiter_identification::1.0.
 
pds4:urn:nasa:pds:0001_nasa_pds_1:all:user:geom:geometry_orbiter::pixel_dimensions::1.0 rdf:type rdf:Property;
  rdfs:label "Pixel_Dimensions";
  rdfs:domain pds4:urn:nasa:pds:0001_nasa_pds_1:all:user:geom:geometry_orbiter::1.0;
  rdfs:range pds4:urn:nasa:pds:0001_nasa_pds_1:all:user:geom:pixel_dimensions::1.0.
 
pds4:urn:nasa:pds:0001_nasa_pds_1:all:user:geom:geometry_orbiter::distances::1.0 rdf:type rdf:Property;
  rdfs:label "Distances";
  rdfs:domain pds4:urn:nasa:pds:0001_nasa_pds_1:all:user:geom:geometry_orbiter::1.0;
  rdfs:range pds4:urn:nasa:pds:0001_nasa_pds_1:all:user:geom:distances::1.0.
 
pds4:urn:nasa:pds:0001_nasa_pds_1:all:user:geom:geometry_orbiter::surface_geometry::1.0 rdf:type rdf:Property;
  rdfs:label "Surface_Geometry";
  rdfs:domain pds4:urn:nasa:pds:0001_nasa_pds_1:all:user:geom:geometry_orbiter::1.0;
  rdfs:range pds4:urn:nasa:pds:0001_nasa_pds_1:all:user:geom:surface_geometry::1.0.
 
pds4:urn:nasa:pds:0001_nasa_pds_1:all:user:geom:geometry_orbiter::illumination_geometry::1.0 rdf:type rdf:Property;
  rdfs:label "Illumination_Geometry";
  rdfs:domain pds4:urn:nasa:pds:0001_nasa_pds_1:all:user:geom:geometry_orbiter::1.0;
  rdfs:range pds4:urn:nasa:pds:0001_nasa_pds_1:all:user:geom:illumination_geometry::1.0.
 
pds4:urn:nasa:pds:0001_nasa_pds_1:all:user:geom:geometry_orbiter::vectors::1.0 rdf:type rdf:Property;
  rdfs:label "Vectors";
  rdfs:domain pds4:urn:nasa:pds:0001_nasa_pds_1:all:user:geom:geometry_orbiter::1.0;
  rdfs:range pds4:urn:nasa:pds:0001_nasa_pds_1:all:user:geom:vectors::1.0.
 
pds4:urn:nasa:pds:0001_nasa_pds_1:all:user:geom:illumination_geometry::illumination_specific::1.0 rdf:type rdf:Property;
  rdfs:label "Illumination_Specific";
  rdfs:domain pds4:urn:nasa:pds:0001_nasa_pds_1:all:user:geom:illumination_geometry::1.0;
  rdfs:range pds4:urn:nasa:pds:0001_nasa_pds_1:all:user:geom:illumination_specific::1.0.
 
pds4:urn:nasa:pds:0001_nasa_pds_1:all:user:geom:illumination_geometry::illumination_min_max::1.0 rdf:type rdf:Property;
  rdfs:label "Illumination_Min_Max";
  rdfs:domain pds4:urn:nasa:pds:0001_nasa_pds_1:all:user:geom:illumination_geometry::1.0;
  rdfs:range pds4:urn:nasa:pds:0001_nasa_pds_1:all:user:geom:illumination_min_max::1.0.
 
pds4:urn:nasa:pds:0001_nasa_pds_1:all:user:geom:illumination_geometry::illumination_start_stop::1.0 rdf:type rdf:Property;
  rdfs:label "Illumination_Start_Stop";
  rdfs:domain pds4:urn:nasa:pds:0001_nasa_pds_1:all:user:geom:illumination_geometry::1.0;
  rdfs:range pds4:urn:nasa:pds:0001_nasa_pds_1:all:user:geom:illumination_start_stop::1.0.
 
pds4:urn:nasa:pds:0001_nasa_pds_1:all:user:geom:illumination_specific::reference_pixel::1.0 rdf:type rdf:Property;
  rdfs:label "Reference_Pixel";
  rdfs:domain pds4:urn:nasa:pds:0001_nasa_pds_1:all:user:geom:illumination_specific::1.0;
  rdfs:range pds4:urn:nasa:pds:0001_nasa_pds_1:all:user:geom:reference_pixel::1.0.
 
pds4:urn:nasa:pds:0001_nasa_pds_1:all:user:geom:image_display_geometry::local_internal_reference::1.0 rdf:type rdf:Property;
  rdfs:label "Local_Internal_Reference";
  rdfs:domain pds4:urn:nasa:pds:0001_nasa_pds_1:all:user:geom:image_display_geometry::1.0;
  rdfs:range pds4:urn:nasa:pds:0001_nasa_pds_1:pds:product_components:pds:local_internal_reference::1.0.
 
pds4:urn:nasa:pds:0001_nasa_pds_1:all:user:geom:image_display_geometry::display_direction::1.0 rdf:type rdf:Property;
  rdfs:label "Display_Direction";
  rdfs:domain pds4:urn:nasa:pds:0001_nasa_pds_1:all:user:geom:image_display_geometry::1.0;
  rdfs:range pds4:urn:nasa:pds:0001_nasa_pds_1:all:user:geom:display_direction::1.0.
 
pds4:urn:nasa:pds:0001_nasa_pds_1:all:user:geom:image_display_geometry::central_body_identification::1.0 rdf:type rdf:Property;
  rdfs:label "Central_Body_Identification";
  rdfs:domain pds4:urn:nasa:pds:0001_nasa_pds_1:all:user:geom:image_display_geometry::1.0;
  rdfs:range pds4:urn:nasa:pds:0001_nasa_pds_1:geom:body_identification_base:geom:central_body_identification::1.0.
 
pds4:urn:nasa:pds:0001_nasa_pds_1:all:user:geom:image_display_geometry::geometry_target_identification::1.0 rdf:type rdf:Property;
  rdfs:label "Geometry_Target_Identification";
  rdfs:domain pds4:urn:nasa:pds:0001_nasa_pds_1:all:user:geom:image_display_geometry::1.0;
  rdfs:range pds4:urn:nasa:pds:0001_nasa_pds_1:geom:body_identification_base:geom:geometry_target_identification::1.0.
 
pds4:urn:nasa:pds:0001_nasa_pds_1:all:user:geom:image_display_geometry::object_orientation_north_east::1.0 rdf:type rdf:Property;
  rdfs:label "Object_Orientation_North_East";
  rdfs:domain pds4:urn:nasa:pds:0001_nasa_pds_1:all:user:geom:image_display_geometry::1.0;
  rdfs:range pds4:urn:nasa:pds:0001_nasa_pds_1:all:user:geom:object_orientation_north_east::1.0.
 
pds4:urn:nasa:pds:0001_nasa_pds_1:all:user:geom:image_display_geometry::object_orientation_ra_dec::1.0 rdf:type rdf:Property;
  rdfs:label "Object_Orientation_RA_Dec";
  rdfs:domain pds4:urn:nasa:pds:0001_nasa_pds_1:all:user:geom:image_display_geometry::1.0;
  rdfs:range pds4:urn:nasa:pds:0001_nasa_pds_1:all:user:geom:object_orientation_ra_dec::1.0.
 
pds4:urn:nasa:pds:0001_nasa_pds_1:all:user:geom:image_display_geometry::object_orientation_clock_angles::1.0 rdf:type rdf:Property;
  rdfs:label "Object_Orientation_Clock_Angles";
  rdfs:domain pds4:urn:nasa:pds:0001_nasa_pds_1:all:user:geom:image_display_geometry::1.0;
  rdfs:range pds4:urn:nasa:pds:0001_nasa_pds_1:all:user:geom:object_orientation_clock_angles::1.0.
 
pds4:urn:nasa:pds:0001_nasa_pds_1:all:user:geom:image_display_geometry::quaternion_plus_to_from::1.0 rdf:type rdf:Property;
  rdfs:label "Quaternion_Plus_To_From";
  rdfs:domain pds4:urn:nasa:pds:0001_nasa_pds_1:all:user:geom:image_display_geometry::1.0;
  rdfs:range pds4:urn:nasa:pds:0001_nasa_pds_1:geom:quaternion_base:geom:quaternion_plus_to_from::1.0.
 
pds4:urn:nasa:pds:0001_nasa_pds_1:all:user:geom:motion_counter::motion_counter_index::1.0 rdf:type rdf:Property;
  rdfs:label "Motion_Counter_Index";
  rdfs:domain pds4:urn:nasa:pds:0001_nasa_pds_1:all:user:geom:motion_counter::1.0;
  rdfs:range pds4:urn:nasa:pds:0001_nasa_pds_1:geom:list_index_no_units:geom:motion_counter_index::1.0.
 
pds4:urn:nasa:pds:0001_nasa_pds_1:all:user:geom:object_orientation_north_east::reference_frame_identification::1.0 rdf:type rdf:Property;
  rdfs:label "Reference_Frame_Identification";
  rdfs:domain pds4:urn:nasa:pds:0001_nasa_pds_1:all:user:geom:object_orientation_north_east::1.0;
  rdfs:range pds4:urn:nasa:pds:0001_nasa_pds_1:geom:frame_identification_base:geom:reference_frame_identification::1.0.
 
pds4:urn:nasa:pds:0001_nasa_pds_1:all:user:geom:object_orientation_ra_dec::reference_pixel::1.0 rdf:type rdf:Property;
  rdfs:label "Reference_Pixel";
  rdfs:domain pds4:urn:nasa:pds:0001_nasa_pds_1:all:user:geom:object_orientation_ra_dec::1.0;
  rdfs:range pds4:urn:nasa:pds:0001_nasa_pds_1:all:user:geom:reference_pixel::1.0.
 
pds4:urn:nasa:pds:0001_nasa_pds_1:all:user:geom:object_orientation_ra_dec::reference_frame_identification::1.0 rdf:type rdf:Property;
  rdfs:label "Reference_Frame_Identification";
  rdfs:domain pds4:urn:nasa:pds:0001_nasa_pds_1:all:user:geom:object_orientation_ra_dec::1.0;
  rdfs:range pds4:urn:nasa:pds:0001_nasa_pds_1:geom:frame_identification_base:geom:reference_frame_identification::1.0.
 
pds4:urn:nasa:pds:0001_nasa_pds_1:all:user:geom:orbiter_identification::central_body_identification::1.0 rdf:type rdf:Property;
  rdfs:label "Central_Body_Identification";
  rdfs:domain pds4:urn:nasa:pds:0001_nasa_pds_1:all:user:geom:orbiter_identification::1.0;
  rdfs:range pds4:urn:nasa:pds:0001_nasa_pds_1:geom:body_identification_base:geom:central_body_identification::1.0.
 
pds4:urn:nasa:pds:0001_nasa_pds_1:all:user:geom:orbiter_identification::geometry_target_identification::1.0 rdf:type rdf:Property;
  rdfs:label "Geometry_Target_Identification";
  rdfs:domain pds4:urn:nasa:pds:0001_nasa_pds_1:all:user:geom:orbiter_identification::1.0;
  rdfs:range pds4:urn:nasa:pds:0001_nasa_pds_1:geom:body_identification_base:geom:geometry_target_identification::1.0.
 
pds4:urn:nasa:pds:0001_nasa_pds_1:all:user:geom:orbiter_identification::coordinate_system_identification::1.0 rdf:type rdf:Property;
  rdfs:label "Coordinate_System_Identification";
  rdfs:domain pds4:urn:nasa:pds:0001_nasa_pds_1:all:user:geom:orbiter_identification::1.0;
  rdfs:range pds4:urn:nasa:pds:0001_nasa_pds_1:all:user:geom:coordinate_system_identification::1.0.
 
pds4:urn:nasa:pds:0001_nasa_pds_1:all:user:geom:psph_model::vector_center::1.0 rdf:type rdf:Property;
  rdfs:label "Vector_Center";
  rdfs:domain pds4:urn:nasa:pds:0001_nasa_pds_1:all:user:geom:psph_model::1.0;
  rdfs:range pds4:urn:nasa:pds:0001_nasa_pds_1:geom:vector_cartesian_position_base:geom:vector_center::1.0.
 
pds4:urn:nasa:pds:0001_nasa_pds_1:all:user:geom:psph_model::vector_axis_x::1.0 rdf:type rdf:Property;
  rdfs:label "Vector_Axis_X";
  rdfs:domain pds4:urn:nasa:pds:0001_nasa_pds_1:all:user:geom:psph_model::1.0;
  rdfs:range pds4:urn:nasa:pds:0001_nasa_pds_1:geom:vector_cartesian_unit:geom:vector_axis_x::1.0.
 
pds4:urn:nasa:pds:0001_nasa_pds_1:all:user:geom:psph_model::vector_axis_y::1.0 rdf:type rdf:Property;
  rdfs:label "Vector_Axis_Y";
  rdfs:domain pds4:urn:nasa:pds:0001_nasa_pds_1:all:user:geom:psph_model::1.0;
  rdfs:range pds4:urn:nasa:pds:0001_nasa_pds_1:geom:vector_cartesian_unit:geom:vector_axis_y::1.0.
 
pds4:urn:nasa:pds:0001_nasa_pds_1:all:user:geom:psph_model::vector_normal_x::1.0 rdf:type rdf:Property;
  rdfs:label "Vector_Normal_X";
  rdfs:domain pds4:urn:nasa:pds:0001_nasa_pds_1:all:user:geom:psph_model::1.0;
  rdfs:range pds4:urn:nasa:pds:0001_nasa_pds_1:geom:vector_cartesian_unit:geom:vector_normal_x::1.0.
 
pds4:urn:nasa:pds:0001_nasa_pds_1:all:user:geom:psph_model::vector_normal_y::1.0 rdf:type rdf:Property;
  rdfs:label "Vector_Normal_Y";
  rdfs:domain pds4:urn:nasa:pds:0001_nasa_pds_1:all:user:geom:psph_model::1.0;
  rdfs:range pds4:urn:nasa:pds:0001_nasa_pds_1:geom:vector_cartesian_unit:geom:vector_normal_y::1.0.
 
pds4:urn:nasa:pds:0001_nasa_pds_1:all:user:geom:pixel_dimensions::pixel_size_projected::1.0 rdf:type rdf:Property;
  rdfs:label "Pixel_Size_Projected";
  rdfs:domain pds4:urn:nasa:pds:0001_nasa_pds_1:all:user:geom:pixel_dimensions::1.0;
  rdfs:range pds4:urn:nasa:pds:0001_nasa_pds_1:all:user:geom:pixel_size_projected::1.0.
 
pds4:urn:nasa:pds:0001_nasa_pds_1:all:user:geom:pixel_intercept::reference_pixel::1.0 rdf:type rdf:Property;
  rdfs:label "Reference_Pixel";
  rdfs:domain pds4:urn:nasa:pds:0001_nasa_pds_1:all:user:geom:pixel_intercept::1.0;
  rdfs:range pds4:urn:nasa:pds:0001_nasa_pds_1:all:user:geom:reference_pixel::1.0.
 
pds4:urn:nasa:pds:0001_nasa_pds_1:geom:quaternion_base:geom:quaternion_plus_to_from::rotate_from::1.0 rdf:type rdf:Property;
  rdfs:label "Rotate_From";
  rdfs:domain pds4:urn:nasa:pds:0001_nasa_pds_1:geom:quaternion_base:geom:quaternion_plus_to_from::1.0;
  rdfs:range pds4:urn:nasa:pds:0001_nasa_pds_1:geom:frame_identification_base:geom:rotate_from::1.0.
 
pds4:urn:nasa:pds:0001_nasa_pds_1:geom:quaternion_base:geom:quaternion_plus_to_from::rotate_to::1.0 rdf:type rdf:Property;
  rdfs:label "Rotate_To";
  rdfs:domain pds4:urn:nasa:pds:0001_nasa_pds_1:geom:quaternion_base:geom:quaternion_plus_to_from::1.0;
  rdfs:range pds4:urn:nasa:pds:0001_nasa_pds_1:geom:frame_identification_base:geom:rotate_to::1.0.
 
pds4:urn:nasa:pds:0001_nasa_pds_1:all:user:geom:spice_kernel_files::spice_kernel_identification::1.0 rdf:type rdf:Property;
  rdfs:label "SPICE_Kernel_Identification";
  rdfs:domain pds4:urn:nasa:pds:0001_nasa_pds_1:all:user:geom:spice_kernel_files::1.0;
  rdfs:range pds4:urn:nasa:pds:0001_nasa_pds_1:all:user:geom:spice_kernel_identification::1.0.
 
pds4:urn:nasa:pds:0001_nasa_pds_1:all:user:geom:spice_kernel_identification::internal_reference::1.0 rdf:type rdf:Property;
  rdfs:label "Internal_Reference";
  rdfs:domain pds4:urn:nasa:pds:0001_nasa_pds_1:all:user:geom:spice_kernel_identification::1.0;
  rdfs:range pds4:urn:nasa:pds:0001_nasa_pds_1:pds:product_components:pds:internal_reference::1.0.
 
pds4:urn:nasa:pds:0001_nasa_pds_1:all:user:geom:surface_geometry::surface_geometry_specific::1.0 rdf:type rdf:Property;
  rdfs:label "Surface_Geometry_Specific";
  rdfs:domain pds4:urn:nasa:pds:0001_nasa_pds_1:all:user:geom:surface_geometry::1.0;
  rdfs:range pds4:urn:nasa:pds:0001_nasa_pds_1:all:user:geom:surface_geometry_specific::1.0.
 
pds4:urn:nasa:pds:0001_nasa_pds_1:all:user:geom:surface_geometry::surface_geometry_min_max::1.0 rdf:type rdf:Property;
  rdfs:label "Surface_Geometry_Min_Max";
  rdfs:domain pds4:urn:nasa:pds:0001_nasa_pds_1:all:user:geom:surface_geometry::1.0;
  rdfs:range pds4:urn:nasa:pds:0001_nasa_pds_1:all:user:geom:surface_geometry_min_max::1.0.
 
pds4:urn:nasa:pds:0001_nasa_pds_1:all:user:geom:surface_geometry::surface_geometry_start_stop::1.0 rdf:type rdf:Property;
  rdfs:label "Surface_Geometry_Start_Stop";
  rdfs:domain pds4:urn:nasa:pds:0001_nasa_pds_1:all:user:geom:surface_geometry::1.0;
  rdfs:range pds4:urn:nasa:pds:0001_nasa_pds_1:all:user:geom:surface_geometry_start_stop::1.0.
 
pds4:urn:nasa:pds:0001_nasa_pds_1:all:user:geom:surface_geometry_specific::pixel_intercept::1.0 rdf:type rdf:Property;
  rdfs:label "Pixel_Intercept";
  rdfs:domain pds4:urn:nasa:pds:0001_nasa_pds_1:all:user:geom:surface_geometry_specific::1.0;
  rdfs:range pds4:urn:nasa:pds:0001_nasa_pds_1:all:user:geom:pixel_intercept::1.0.
 
pds4:urn:nasa:pds:0001_nasa_pds_1:all:user:geom:surface_geometry_specific::footprint_vertices::1.0 rdf:type rdf:Property;
  rdfs:label "Footprint_Vertices";
  rdfs:domain pds4:urn:nasa:pds:0001_nasa_pds_1:all:user:geom:surface_geometry_specific::1.0;
  rdfs:range pds4:urn:nasa:pds:0001_nasa_pds_1:all:user:geom:footprint_vertices::1.0.
 
pds4:urn:nasa:pds:0001_nasa_pds_1:geom:vector_cartesian_acceleration_base:geom:vector_cartesian_acceleration_extended_base::coordinate_system_identification::1.0 rdf:type rdf:Property;
  rdfs:label "Coordinate_System_Identification";
  rdfs:domain pds4:urn:nasa:pds:0001_nasa_pds_1:geom:vector_cartesian_acceleration_base:geom:vector_cartesian_acceleration_extended_base::1.0;
  rdfs:range pds4:urn:nasa:pds:0001_nasa_pds_1:all:user:geom:coordinate_system_identification::1.0.
 
pds4:urn:nasa:pds:0001_nasa_pds_1:geom:vector_cartesian_acceleration_extended_base:geom:vector_cartesian_acceleration_generic::observer_identification::1.0 rdf:type rdf:Property;
  rdfs:label "Observer_Identification";
  rdfs:domain pds4:urn:nasa:pds:0001_nasa_pds_1:geom:vector_cartesian_acceleration_extended_base:geom:vector_cartesian_acceleration_generic::1.0;
  rdfs:range pds4:urn:nasa:pds:0001_nasa_pds_1:geom:body_identification_base:geom:observer_identification::1.0.
 
pds4:urn:nasa:pds:0001_nasa_pds_1:geom:vector_cartesian_acceleration_extended_base:geom:vector_cartesian_acceleration_generic::geometry_target_identification::1.0 rdf:type rdf:Property;
  rdfs:label "Geometry_Target_Identification";
  rdfs:domain pds4:urn:nasa:pds:0001_nasa_pds_1:geom:vector_cartesian_acceleration_extended_base:geom:vector_cartesian_acceleration_generic::1.0;
  rdfs:range pds4:urn:nasa:pds:0001_nasa_pds_1:geom:body_identification_base:geom:geometry_target_identification::1.0.
 
pds4:urn:nasa:pds:0001_nasa_pds_1:geom:vector_cartesian_position_base:geom:vector_cartesian_position_extended_base::coordinate_system_identification::1.0 rdf:type rdf:Property;
  rdfs:label "Coordinate_System_Identification";
  rdfs:domain pds4:urn:nasa:pds:0001_nasa_pds_1:geom:vector_cartesian_position_base:geom:vector_cartesian_position_extended_base::1.0;
  rdfs:range pds4:urn:nasa:pds:0001_nasa_pds_1:all:user:geom:coordinate_system_identification::1.0.
 
pds4:urn:nasa:pds:0001_nasa_pds_1:geom:vector_cartesian_position_extended_base:geom:vector_cartesian_position_generic::observer_identification::1.0 rdf:type rdf:Property;
  rdfs:label "Observer_Identification";
  rdfs:domain pds4:urn:nasa:pds:0001_nasa_pds_1:geom:vector_cartesian_position_extended_base:geom:vector_cartesian_position_generic::1.0;
  rdfs:range pds4:urn:nasa:pds:0001_nasa_pds_1:geom:body_identification_base:geom:observer_identification::1.0.
 
pds4:urn:nasa:pds:0001_nasa_pds_1:geom:vector_cartesian_position_extended_base:geom:vector_cartesian_position_generic::geometry_target_identification::1.0 rdf:type rdf:Property;
  rdfs:label "Geometry_Target_Identification";
  rdfs:domain pds4:urn:nasa:pds:0001_nasa_pds_1:geom:vector_cartesian_position_extended_base:geom:vector_cartesian_position_generic::1.0;
  rdfs:range pds4:urn:nasa:pds:0001_nasa_pds_1:geom:body_identification_base:geom:geometry_target_identification::1.0.
 
pds4:urn:nasa:pds:0001_nasa_pds_1:geom:vector_cartesian_velocity_base:geom:vector_cartesian_velocity_extended_base::coordinate_system_identification::1.0 rdf:type rdf:Property;
  rdfs:label "Coordinate_System_Identification";
  rdfs:domain pds4:urn:nasa:pds:0001_nasa_pds_1:geom:vector_cartesian_velocity_base:geom:vector_cartesian_velocity_extended_base::1.0;
  rdfs:range pds4:urn:nasa:pds:0001_nasa_pds_1:all:user:geom:coordinate_system_identification::1.0.
 
pds4:urn:nasa:pds:0001_nasa_pds_1:geom:vector_cartesian_velocity_extended_base:geom:vector_cartesian_velocity_generic::observer_identification::1.0 rdf:type rdf:Property;
  rdfs:label "Observer_Identification";
  rdfs:domain pds4:urn:nasa:pds:0001_nasa_pds_1:geom:vector_cartesian_velocity_extended_base:geom:vector_cartesian_velocity_generic::1.0;
  rdfs:range pds4:urn:nasa:pds:0001_nasa_pds_1:geom:body_identification_base:geom:observer_identification::1.0.
 
pds4:urn:nasa:pds:0001_nasa_pds_1:geom:vector_cartesian_velocity_extended_base:geom:vector_cartesian_velocity_generic::geometry_target_identification::1.0 rdf:type rdf:Property;
  rdfs:label "Geometry_Target_Identification";
  rdfs:domain pds4:urn:nasa:pds:0001_nasa_pds_1:geom:vector_cartesian_velocity_extended_base:geom:vector_cartesian_velocity_generic::1.0;
  rdfs:range pds4:urn:nasa:pds:0001_nasa_pds_1:geom:body_identification_base:geom:geometry_target_identification::1.0.
 
pds4:urn:nasa:pds:0001_nasa_pds_1:geom:vector_planetocentric_position_base:geom:vector_planetocentric_position_extended_base::coordinate_system_identification::1.0 rdf:type rdf:Property;
  rdfs:label "Coordinate_System_Identification";
  rdfs:domain pds4:urn:nasa:pds:0001_nasa_pds_1:geom:vector_planetocentric_position_base:geom:vector_planetocentric_position_extended_base::1.0;
  rdfs:range pds4:urn:nasa:pds:0001_nasa_pds_1:all:user:geom:coordinate_system_identification::1.0.
 
pds4:urn:nasa:pds:0001_nasa_pds_1:geom:vector_planetocentric_position_extended_base:geom:vector_planetocentric_position_generic::observer_identification::1.0 rdf:type rdf:Property;
  rdfs:label "Observer_Identification";
  rdfs:domain pds4:urn:nasa:pds:0001_nasa_pds_1:geom:vector_planetocentric_position_extended_base:geom:vector_planetocentric_position_generic::1.0;
  rdfs:range pds4:urn:nasa:pds:0001_nasa_pds_1:geom:body_identification_base:geom:observer_identification::1.0.
 
pds4:urn:nasa:pds:0001_nasa_pds_1:geom:vector_planetocentric_position_extended_base:geom:vector_planetocentric_position_generic::geometry_target_identification::1.0 rdf:type rdf:Property;
  rdfs:label "Geometry_Target_Identification";
  rdfs:domain pds4:urn:nasa:pds:0001_nasa_pds_1:geom:vector_planetocentric_position_extended_base:geom:vector_planetocentric_position_generic::1.0;
  rdfs:range pds4:urn:nasa:pds:0001_nasa_pds_1:geom:body_identification_base:geom:geometry_target_identification::1.0.
 
pds4:urn:nasa:pds:0001_nasa_pds_1:geom:vector_planetocentric_velocity_base:geom:vector_planetocentric_velocity_extended_base::coordinate_system_identification::1.0 rdf:type rdf:Property;
  rdfs:label "Coordinate_System_Identification";
  rdfs:domain pds4:urn:nasa:pds:0001_nasa_pds_1:geom:vector_planetocentric_velocity_base:geom:vector_planetocentric_velocity_extended_base::1.0;
  rdfs:range pds4:urn:nasa:pds:0001_nasa_pds_1:all:user:geom:coordinate_system_identification::1.0.
 
pds4:urn:nasa:pds:0001_nasa_pds_1:geom:vector_planetocentric_velocity_extended_base:geom:vector_planetocentric_velocity_generic::observer_identification::1.0 rdf:type rdf:Property;
  rdfs:label "Observer_Identification";
  rdfs:domain pds4:urn:nasa:pds:0001_nasa_pds_1:geom:vector_planetocentric_velocity_extended_base:geom:vector_planetocentric_velocity_generic::1.0;
  rdfs:range pds4:urn:nasa:pds:0001_nasa_pds_1:geom:body_identification_base:geom:observer_identification::1.0.
 
pds4:urn:nasa:pds:0001_nasa_pds_1:geom:vector_planetocentric_velocity_extended_base:geom:vector_planetocentric_velocity_generic::geometry_target_identification::1.0 rdf:type rdf:Property;
  rdfs:label "Geometry_Target_Identification";
  rdfs:domain pds4:urn:nasa:pds:0001_nasa_pds_1:geom:vector_planetocentric_velocity_extended_base:geom:vector_planetocentric_velocity_generic::1.0;
  rdfs:range pds4:urn:nasa:pds:0001_nasa_pds_1:geom:body_identification_base:geom:geometry_target_identification::1.0.
 
pds4:urn:nasa:pds:0001_nasa_pds_1:all:user:geom:vectors::vectors_cartesian_specific::1.0 rdf:type rdf:Property;
  rdfs:label "Vectors_Cartesian_Specific";
  rdfs:domain pds4:urn:nasa:pds:0001_nasa_pds_1:all:user:geom:vectors::1.0;
  rdfs:range pds4:urn:nasa:pds:0001_nasa_pds_1:all:user:geom:vectors_cartesian_specific::1.0.
 
pds4:urn:nasa:pds:0001_nasa_pds_1:all:user:geom:vectors::vectors_planetocentric_specific::1.0 rdf:type rdf:Property;
  rdfs:label "Vectors_Planetocentric_Specific";
  rdfs:domain pds4:urn:nasa:pds:0001_nasa_pds_1:all:user:geom:vectors::1.0;
  rdfs:range pds4:urn:nasa:pds:0001_nasa_pds_1:all:user:geom:vectors_planetocentric_specific::1.0.
 
pds4:urn:nasa:pds:0001_nasa_pds_1:all:user:geom:vectors::generic_vectors::1.0 rdf:type rdf:Property;
  rdfs:label "Generic_Vectors";
  rdfs:domain pds4:urn:nasa:pds:0001_nasa_pds_1:all:user:geom:vectors::1.0;
  rdfs:range pds4:urn:nasa:pds:0001_nasa_pds_1:all:user:geom:generic_vectors::1.0.
 
pds4:urn:nasa:pds:0001_nasa_pds_1:all:user:geom:vectors_cartesian_specific::vector_cartesian_position_central_body_to_spacecraft::1.0 rdf:type rdf:Property;
  rdfs:label "Vector_Cartesian_Position_Central_Body_To_Spacecraft";
  rdfs:domain pds4:urn:nasa:pds:0001_nasa_pds_1:all:user:geom:vectors_cartesian_specific::1.0;
  rdfs:range pds4:urn:nasa:pds:0001_nasa_pds_1:geom:vector_cartesian_position_extended_base:geom:vector_cartesian_position_central_body_to_spacecraft::1.0.
 
pds4:urn:nasa:pds:0001_nasa_pds_1:all:user:geom:vectors_cartesian_specific::vector_cartesian_position_central_body_to_target::1.0 rdf:type rdf:Property;
  rdfs:label "Vector_Cartesian_Position_Central_Body_To_Target";
  rdfs:domain pds4:urn:nasa:pds:0001_nasa_pds_1:all:user:geom:vectors_cartesian_specific::1.0;
  rdfs:range pds4:urn:nasa:pds:0001_nasa_pds_1:geom:vector_cartesian_position_extended_base:geom:vector_cartesian_position_central_body_to_target::1.0.
 
pds4:urn:nasa:pds:0001_nasa_pds_1:all:user:geom:vectors_cartesian_specific::vector_cartesian_position_spacecraft_to_target::1.0 rdf:type rdf:Property;
  rdfs:label "Vector_Cartesian_Position_Spacecraft_To_Target";
  rdfs:domain pds4:urn:nasa:pds:0001_nasa_pds_1:all:user:geom:vectors_cartesian_specific::1.0;
  rdfs:range pds4:urn:nasa:pds:0001_nasa_pds_1:geom:vector_cartesian_position_extended_base:geom:vector_cartesian_position_spacecraft_to_target::1.0.
 
pds4:urn:nasa:pds:0001_nasa_pds_1:all:user:geom:vectors_cartesian_specific::vector_cartesian_position_ssb_to_central_body::1.0 rdf:type rdf:Property;
  rdfs:label "Vector_Cartesian_Position_SSB_To_Central_Body";
  rdfs:domain pds4:urn:nasa:pds:0001_nasa_pds_1:all:user:geom:vectors_cartesian_specific::1.0;
  rdfs:range pds4:urn:nasa:pds:0001_nasa_pds_1:geom:vector_cartesian_position_extended_base:geom:vector_cartesian_position_ssb_to_central_body::1.0.
 
pds4:urn:nasa:pds:0001_nasa_pds_1:all:user:geom:vectors_cartesian_specific::vector_cartesian_position_ssb_to_spacecraft::1.0 rdf:type rdf:Property;
  rdfs:label "Vector_Cartesian_Position_SSB_To_Spacecraft";
  rdfs:domain pds4:urn:nasa:pds:0001_nasa_pds_1:all:user:geom:vectors_cartesian_specific::1.0;
  rdfs:range pds4:urn:nasa:pds:0001_nasa_pds_1:geom:vector_cartesian_position_extended_base:geom:vector_cartesian_position_ssb_to_spacecraft::1.0.
 
pds4:urn:nasa:pds:0001_nasa_pds_1:all:user:geom:vectors_cartesian_specific::vector_cartesian_position_ssb_to_target::1.0 rdf:type rdf:Property;
  rdfs:label "Vector_Cartesian_Position_SSB_To_Target";
  rdfs:domain pds4:urn:nasa:pds:0001_nasa_pds_1:all:user:geom:vectors_cartesian_specific::1.0;
  rdfs:range pds4:urn:nasa:pds:0001_nasa_pds_1:geom:vector_cartesian_position_extended_base:geom:vector_cartesian_position_ssb_to_target::1.0.
 
pds4:urn:nasa:pds:0001_nasa_pds_1:all:user:geom:vectors_cartesian_specific::vector_cartesian_position_sun_to_central_body::1.0 rdf:type rdf:Property;
  rdfs:label "Vector_Cartesian_Position_Sun_To_Central_Body";
  rdfs:domain pds4:urn:nasa:pds:0001_nasa_pds_1:all:user:geom:vectors_cartesian_specific::1.0;
  rdfs:range pds4:urn:nasa:pds:0001_nasa_pds_1:geom:vector_cartesian_position_extended_base:geom:vector_cartesian_position_sun_to_central_body::1.0.
 
pds4:urn:nasa:pds:0001_nasa_pds_1:all:user:geom:vectors_cartesian_specific::vector_cartesian_position_sun_to_spacecraft::1.0 rdf:type rdf:Property;
  rdfs:label "Vector_Cartesian_Position_Sun_To_Spacecraft";
  rdfs:domain pds4:urn:nasa:pds:0001_nasa_pds_1:all:user:geom:vectors_cartesian_specific::1.0;
  rdfs:range pds4:urn:nasa:pds:0001_nasa_pds_1:geom:vector_cartesian_position_extended_base:geom:vector_cartesian_position_sun_to_spacecraft::1.0.
 
pds4:urn:nasa:pds:0001_nasa_pds_1:all:user:geom:vectors_cartesian_specific::vector_cartesian_position_sun_to_target::1.0 rdf:type rdf:Property;
  rdfs:label "Vector_Cartesian_Position_Sun_To_Target";
  rdfs:domain pds4:urn:nasa:pds:0001_nasa_pds_1:all:user:geom:vectors_cartesian_specific::1.0;
  rdfs:range pds4:urn:nasa:pds:0001_nasa_pds_1:geom:vector_cartesian_position_extended_base:geom:vector_cartesian_position_sun_to_target::1.0.
 
pds4:urn:nasa:pds:0001_nasa_pds_1:all:user:geom:vectors_cartesian_specific::vector_cartesian_position_earth_to_central_body::1.0 rdf:type rdf:Property;
  rdfs:label "Vector_Cartesian_Position_Earth_To_Central_Body";
  rdfs:domain pds4:urn:nasa:pds:0001_nasa_pds_1:all:user:geom:vectors_cartesian_specific::1.0;
  rdfs:range pds4:urn:nasa:pds:0001_nasa_pds_1:geom:vector_cartesian_position_extended_base:geom:vector_cartesian_position_earth_to_central_body::1.0.
 
pds4:urn:nasa:pds:0001_nasa_pds_1:all:user:geom:vectors_cartesian_specific::vector_cartesian_position_earth_to_spacecraft::1.0 rdf:type rdf:Property;
  rdfs:label "Vector_Cartesian_Position_Earth_To_Spacecraft";
  rdfs:domain pds4:urn:nasa:pds:0001_nasa_pds_1:all:user:geom:vectors_cartesian_specific::1.0;
  rdfs:range pds4:urn:nasa:pds:0001_nasa_pds_1:geom:vector_cartesian_position_extended_base:geom:vector_cartesian_position_earth_to_spacecraft::1.0.
 
pds4:urn:nasa:pds:0001_nasa_pds_1:all:user:geom:vectors_cartesian_specific::vector_cartesian_position_earth_to_target::1.0 rdf:type rdf:Property;
  rdfs:label "Vector_Cartesian_Position_Earth_To_Target";
  rdfs:domain pds4:urn:nasa:pds:0001_nasa_pds_1:all:user:geom:vectors_cartesian_specific::1.0;
  rdfs:range pds4:urn:nasa:pds:0001_nasa_pds_1:geom:vector_cartesian_position_extended_base:geom:vector_cartesian_position_earth_to_target::1.0.
 
pds4:urn:nasa:pds:0001_nasa_pds_1:all:user:geom:vectors_cartesian_specific::vector_cartesian_velocity_spacecraft_relative_to_central_body::1.0 rdf:type rdf:Property;
  rdfs:label "Vector_Cartesian_Velocity_Spacecraft_Relative_To_Central_Body";
  rdfs:domain pds4:urn:nasa:pds:0001_nasa_pds_1:all:user:geom:vectors_cartesian_specific::1.0;
  rdfs:range pds4:urn:nasa:pds:0001_nasa_pds_1:geom:vector_cartesian_velocity_extended_base:geom:vector_cartesian_velocity_spacecraft_relative_to_central_body::1.0.
 
pds4:urn:nasa:pds:0001_nasa_pds_1:all:user:geom:vectors_cartesian_specific::vector_cartesian_velocity_spacecraft_relative_to_target::1.0 rdf:type rdf:Property;
  rdfs:label "Vector_Cartesian_Velocity_Spacecraft_Relative_To_Target";
  rdfs:domain pds4:urn:nasa:pds:0001_nasa_pds_1:all:user:geom:vectors_cartesian_specific::1.0;
  rdfs:range pds4:urn:nasa:pds:0001_nasa_pds_1:geom:vector_cartesian_velocity_extended_base:geom:vector_cartesian_velocity_spacecraft_relative_to_target::1.0.
 
pds4:urn:nasa:pds:0001_nasa_pds_1:all:user:geom:vectors_cartesian_specific::vector_cartesian_velocity_spacecraft_relative_to_earth::1.0 rdf:type rdf:Property;
  rdfs:label "Vector_Cartesian_Velocity_Spacecraft_Relative_To_Earth";
  rdfs:domain pds4:urn:nasa:pds:0001_nasa_pds_1:all:user:geom:vectors_cartesian_specific::1.0;
  rdfs:range pds4:urn:nasa:pds:0001_nasa_pds_1:geom:vector_cartesian_velocity_extended_base:geom:vector_cartesian_velocity_spacecraft_relative_to_earth::1.0.
 
pds4:urn:nasa:pds:0001_nasa_pds_1:all:user:geom:vectors_cartesian_specific::vector_cartesian_velocity_spacecraft_relative_to_ssb::1.0 rdf:type rdf:Property;
  rdfs:label "Vector_Cartesian_Velocity_Spacecraft_Relative_To_SSB";
  rdfs:domain pds4:urn:nasa:pds:0001_nasa_pds_1:all:user:geom:vectors_cartesian_specific::1.0;
  rdfs:range pds4:urn:nasa:pds:0001_nasa_pds_1:geom:vector_cartesian_velocity_extended_base:geom:vector_cartesian_velocity_spacecraft_relative_to_ssb::1.0.
 
pds4:urn:nasa:pds:0001_nasa_pds_1:all:user:geom:vectors_cartesian_specific::vector_cartesian_velocity_spacecraft_relative_to_sun::1.0 rdf:type rdf:Property;
  rdfs:label "Vector_Cartesian_Velocity_Spacecraft_Relative_To_Sun";
  rdfs:domain pds4:urn:nasa:pds:0001_nasa_pds_1:all:user:geom:vectors_cartesian_specific::1.0;
  rdfs:range pds4:urn:nasa:pds:0001_nasa_pds_1:geom:vector_cartesian_velocity_extended_base:geom:vector_cartesian_velocity_spacecraft_relative_to_sun::1.0.
 
pds4:urn:nasa:pds:0001_nasa_pds_1:all:user:geom:vectors_cartesian_specific::vector_cartesian_velocity_target_relative_to_central_body::1.0 rdf:type rdf:Property;
  rdfs:label "Vector_Cartesian_Velocity_Target_Relative_To_Central_Body";
  rdfs:domain pds4:urn:nasa:pds:0001_nasa_pds_1:all:user:geom:vectors_cartesian_specific::1.0;
  rdfs:range pds4:urn:nasa:pds:0001_nasa_pds_1:geom:vector_cartesian_velocity_extended_base:geom:vector_cartesian_velocity_target_relative_to_central_body::1.0.
 
pds4:urn:nasa:pds:0001_nasa_pds_1:all:user:geom:vectors_cartesian_specific::vector_cartesian_velocity_target_relative_to_spacecraft::1.0 rdf:type rdf:Property;
  rdfs:label "Vector_Cartesian_Velocity_Target_Relative_To_Spacecraft";
  rdfs:domain pds4:urn:nasa:pds:0001_nasa_pds_1:all:user:geom:vectors_cartesian_specific::1.0;
  rdfs:range pds4:urn:nasa:pds:0001_nasa_pds_1:geom:vector_cartesian_velocity_extended_base:geom:vector_cartesian_velocity_target_relative_to_spacecraft::1.0.
 
pds4:urn:nasa:pds:0001_nasa_pds_1:all:user:geom:vectors_cartesian_specific::vector_cartesian_velocity_target_relative_to_earth::1.0 rdf:type rdf:Property;
  rdfs:label "Vector_Cartesian_Velocity_Target_Relative_To_Earth";
  rdfs:domain pds4:urn:nasa:pds:0001_nasa_pds_1:all:user:geom:vectors_cartesian_specific::1.0;
  rdfs:range pds4:urn:nasa:pds:0001_nasa_pds_1:geom:vector_cartesian_velocity_extended_base:geom:vector_cartesian_velocity_target_relative_to_earth::1.0.
 
pds4:urn:nasa:pds:0001_nasa_pds_1:all:user:geom:vectors_cartesian_specific::vector_cartesian_velocity_target_relative_to_ssb::1.0 rdf:type rdf:Property;
  rdfs:label "Vector_Cartesian_Velocity_Target_Relative_To_SSB";
  rdfs:domain pds4:urn:nasa:pds:0001_nasa_pds_1:all:user:geom:vectors_cartesian_specific::1.0;
  rdfs:range pds4:urn:nasa:pds:0001_nasa_pds_1:geom:vector_cartesian_velocity_extended_base:geom:vector_cartesian_velocity_target_relative_to_ssb::1.0.
 
pds4:urn:nasa:pds:0001_nasa_pds_1:all:user:geom:vectors_cartesian_specific::vector_cartesian_velocity_target_relative_to_sun::1.0 rdf:type rdf:Property;
  rdfs:label "Vector_Cartesian_Velocity_Target_Relative_To_Sun";
  rdfs:domain pds4:urn:nasa:pds:0001_nasa_pds_1:all:user:geom:vectors_cartesian_specific::1.0;
  rdfs:range pds4:urn:nasa:pds:0001_nasa_pds_1:geom:vector_cartesian_velocity_extended_base:geom:vector_cartesian_velocity_target_relative_to_sun::1.0.
 
pds4:urn:nasa:pds:0001_nasa_pds_1:all:user:geom:vectors_planetocentric_specific::vector_planetocentric_position_central_body_to_spacecraft::1.0 rdf:type rdf:Property;
  rdfs:label "Vector_Planetocentric_Position_Central_Body_To_Spacecraft";
  rdfs:domain pds4:urn:nasa:pds:0001_nasa_pds_1:all:user:geom:vectors_planetocentric_specific::1.0;
  rdfs:range pds4:urn:nasa:pds:0001_nasa_pds_1:geom:vector_planetocentric_position_extended_base:geom:vector_planetocentric_position_central_body_to_spacecraft::1.0.
 
pds4:urn:nasa:pds:0001_nasa_pds_1:all:user:geom:vectors_planetocentric_specific::vector_planetocentric_position_central_body_to_target::1.0 rdf:type rdf:Property;
  rdfs:label "Vector_Planetocentric_Position_Central_Body_To_Target";
  rdfs:domain pds4:urn:nasa:pds:0001_nasa_pds_1:all:user:geom:vectors_planetocentric_specific::1.0;
  rdfs:range pds4:urn:nasa:pds:0001_nasa_pds_1:geom:vector_planetocentric_position_extended_base:geom:vector_planetocentric_position_central_body_to_target::1.0.
 
pds4:urn:nasa:pds:0001_nasa_pds_1:all:user:geom:vectors_planetocentric_specific::vector_planetocentric_position_spacecraft_to_target::1.0 rdf:type rdf:Property;
  rdfs:label "Vector_Planetocentric_Position_Spacecraft_To_Target";
  rdfs:domain pds4:urn:nasa:pds:0001_nasa_pds_1:all:user:geom:vectors_planetocentric_specific::1.0;
  rdfs:range pds4:urn:nasa:pds:0001_nasa_pds_1:geom:vector_planetocentric_position_extended_base:geom:vector_planetocentric_position_spacecraft_to_target::1.0.
 
pds4:urn:nasa:pds:0001_nasa_pds_1:all:user:geom:vectors_planetocentric_specific::vector_planetocentric_velocity_spacecraft_relative_to_target::1.0 rdf:type rdf:Property;
  rdfs:label "Vector_Planetocentric_Velocity_Spacecraft_Relative_To_Target";
  rdfs:domain pds4:urn:nasa:pds:0001_nasa_pds_1:all:user:geom:vectors_planetocentric_specific::1.0;
  rdfs:range pds4:urn:nasa:pds:0001_nasa_pds_1:geom:vector_planetocentric_velocity_extended_base:geom:vector_planetocentric_velocity_spacecraft_relative_to_target::1.0.
 
pds4:urn:nasa:pds:0001_nasa_pds_1:all:user:geom:vectors_planetocentric_specific::vector_planetocentric_velocity_target_relative_to_central_body::1.0 rdf:type rdf:Property;
  rdfs:label "Vector_Planetocentric_Velocity_Target_Relative_To_Central_Body";
  rdfs:domain pds4:urn:nasa:pds:0001_nasa_pds_1:all:user:geom:vectors_planetocentric_specific::1.0;
  rdfs:range pds4:urn:nasa:pds:0001_nasa_pds_1:geom:vector_planetocentric_velocity_extended_base:geom:vector_planetocentric_velocity_target_relative_to_central_body::1.0.
 
pds4:urn:nasa:pds:0001_nasa_pds_1:all:user:geom:vectors_planetocentric_specific::vector_planetocentric_velocity_target_relative_to_spacecraft::1.0 rdf:type rdf:Property;
  rdfs:label "Vector_Planetocentric_Velocity_Target_Relative_To_Spacecraft";
  rdfs:domain pds4:urn:nasa:pds:0001_nasa_pds_1:all:user:geom:vectors_planetocentric_specific::1.0;
  rdfs:range pds4:urn:nasa:pds:0001_nasa_pds_1:geom:vector_planetocentric_velocity_extended_base:geom:vector_planetocentric_velocity_target_relative_to_spacecraft::1.0.
 
pds4:urn:nasa:pds:0001_nasa_pds_1:img:data_processing:img:brightness_correction::brightness_correction_file::1.0 rdf:type rdf:Property;
  rdfs:label "Brightness_Correction_File";
  rdfs:domain pds4:urn:nasa:pds:0001_nasa_pds_1:img:data_processing:img:brightness_correction::1.0;
  rdfs:range pds4:urn:nasa:pds:0001_nasa_pds_1:img:data_processing_file:img:brightness_correction_file::1.0.
 
pds4:urn:nasa:pds:0001_nasa_pds_1:img:data_processing:img:brightness_correction::brightness_correction_image::1.0 rdf:type rdf:Property;
  rdfs:label "Brightness_Correction_Image";
  rdfs:domain pds4:urn:nasa:pds:0001_nasa_pds_1:img:data_processing:img:brightness_correction::1.0;
  rdfs:range pds4:urn:nasa:pds:0001_nasa_pds_1:all:user:img:brightness_correction_image::1.0.
 
pds4:urn:nasa:pds:0001_nasa_pds_1:all:user:img:brightness_correction_image::internal_reference::1.0 rdf:type rdf:Property;
  rdfs:label "Internal_Reference";
  rdfs:domain pds4:urn:nasa:pds:0001_nasa_pds_1:all:user:img:brightness_correction_image::1.0;
  rdfs:range pds4:urn:nasa:pds:0001_nasa_pds_1:pds:product_components:pds:internal_reference::1.0.
 
pds4:urn:nasa:pds:0001_nasa_pds_1:all:user:img:brightness_correction_image::brightness_correction_linear::1.0 rdf:type rdf:Property;
  rdfs:label "Brightness_Correction_Linear";
  rdfs:domain pds4:urn:nasa:pds:0001_nasa_pds_1:all:user:img:brightness_correction_image::1.0;
  rdfs:range pds4:urn:nasa:pds:0001_nasa_pds_1:all:user:img:brightness_correction_linear::1.0.
 
pds4:urn:nasa:pds:0001_nasa_pds_1:all:user:img:brightness_correction_image::brightness_correction_hsi_linear::1.0 rdf:type rdf:Property;
  rdfs:label "Brightness_Correction_HSI_Linear";
  rdfs:domain pds4:urn:nasa:pds:0001_nasa_pds_1:all:user:img:brightness_correction_image::1.0;
  rdfs:range pds4:urn:nasa:pds:0001_nasa_pds_1:all:user:img:brightness_correction_hsi_linear::1.0.
 
pds4:urn:nasa:pds:0001_nasa_pds_1:img:data_processing:img:color_processing::onboard_responsivity::1.0 rdf:type rdf:Property;
  rdfs:label "Onboard_Responsivity";
  rdfs:domain pds4:urn:nasa:pds:0001_nasa_pds_1:img:data_processing:img:color_processing::1.0;
  rdfs:range pds4:urn:nasa:pds:0001_nasa_pds_1:all:user:img:onboard_responsivity::1.0.
 
pds4:urn:nasa:pds:0001_nasa_pds_1:img:data_processing:img:color_processing::onboard_color_matrix::1.0 rdf:type rdf:Property;
  rdfs:label "Onboard_Color_Matrix";
  rdfs:domain pds4:urn:nasa:pds:0001_nasa_pds_1:img:data_processing:img:color_processing::1.0;
  rdfs:range pds4:urn:nasa:pds:0001_nasa_pds_1:all:user:img:onboard_color_matrix::1.0.
 
pds4:urn:nasa:pds:0001_nasa_pds_1:all:user:img:commanded_parameters::brightness_correction::1.0 rdf:type rdf:Property;
  rdfs:label "Brightness_Correction";
  rdfs:domain pds4:urn:nasa:pds:0001_nasa_pds_1:all:user:img:commanded_parameters::1.0;
  rdfs:range pds4:urn:nasa:pds:0001_nasa_pds_1:img:data_processing:img:brightness_correction::1.0.
 
pds4:urn:nasa:pds:0001_nasa_pds_1:all:user:img:commanded_parameters::col_sum::1.0 rdf:type rdf:Property;
  rdfs:label "Col_Sum";
  rdfs:domain pds4:urn:nasa:pds:0001_nasa_pds_1:all:user:img:commanded_parameters::1.0;
  rdfs:range pds4:urn:nasa:pds:0001_nasa_pds_1:all:user:img:col_sum::1.0.
 
pds4:urn:nasa:pds:0001_nasa_pds_1:all:user:img:commanded_parameters::color_filter_array::1.0 rdf:type rdf:Property;
  rdfs:label "Color_Filter_Array";
  rdfs:domain pds4:urn:nasa:pds:0001_nasa_pds_1:all:user:img:commanded_parameters::1.0;
  rdfs:range pds4:urn:nasa:pds:0001_nasa_pds_1:img:data_processing:img:color_filter_array::1.0.
 
pds4:urn:nasa:pds:0001_nasa_pds_1:all:user:img:commanded_parameters::color_processing::1.0 rdf:type rdf:Property;
  rdfs:label "Color_Processing";
  rdfs:domain pds4:urn:nasa:pds:0001_nasa_pds_1:all:user:img:commanded_parameters::1.0;
  rdfs:range pds4:urn:nasa:pds:0001_nasa_pds_1:img:data_processing:img:color_processing::1.0.
 
pds4:urn:nasa:pds:0001_nasa_pds_1:all:user:img:commanded_parameters::dark_current_correction::1.0 rdf:type rdf:Property;
  rdfs:label "Dark_Current_Correction";
  rdfs:domain pds4:urn:nasa:pds:0001_nasa_pds_1:all:user:img:commanded_parameters::1.0;
  rdfs:range pds4:urn:nasa:pds:0001_nasa_pds_1:img:data_processing:img:dark_current_correction::1.0.
 
pds4:urn:nasa:pds:0001_nasa_pds_1:all:user:img:commanded_parameters::detector::1.0 rdf:type rdf:Property;
  rdfs:label "Detector";
  rdfs:domain pds4:urn:nasa:pds:0001_nasa_pds_1:all:user:img:commanded_parameters::1.0;
  rdfs:range pds4:urn:nasa:pds:0001_nasa_pds_1:all:user:img:detector::1.0.
 
pds4:urn:nasa:pds:0001_nasa_pds_1:all:user:img:commanded_parameters::downsampling::1.0 rdf:type rdf:Property;
  rdfs:label "Downsampling";
  rdfs:domain pds4:urn:nasa:pds:0001_nasa_pds_1:all:user:img:commanded_parameters::1.0;
  rdfs:range pds4:urn:nasa:pds:0001_nasa_pds_1:img:data_processing:img:downsampling::1.0.
 
pds4:urn:nasa:pds:0001_nasa_pds_1:all:user:img:commanded_parameters::exposure::1.0 rdf:type rdf:Property;
  rdfs:label "Exposure";
  rdfs:domain pds4:urn:nasa:pds:0001_nasa_pds_1:all:user:img:commanded_parameters::1.0;
  rdfs:range pds4:urn:nasa:pds:0001_nasa_pds_1:all:user:img:exposure::1.0.
 
pds4:urn:nasa:pds:0001_nasa_pds_1:all:user:img:commanded_parameters::flat_field_correction::1.0 rdf:type rdf:Property;
  rdfs:label "Flat_Field_Correction";
  rdfs:domain pds4:urn:nasa:pds:0001_nasa_pds_1:all:user:img:commanded_parameters::1.0;
  rdfs:range pds4:urn:nasa:pds:0001_nasa_pds_1:img:data_processing:img:flat_field_correction::1.0.
 
pds4:urn:nasa:pds:0001_nasa_pds_1:all:user:img:commanded_parameters::focus::1.0 rdf:type rdf:Property;
  rdfs:label "Focus";
  rdfs:domain pds4:urn:nasa:pds:0001_nasa_pds_1:all:user:img:commanded_parameters::1.0;
  rdfs:range pds4:urn:nasa:pds:0001_nasa_pds_1:all:user:img:focus::1.0.
 
pds4:urn:nasa:pds:0001_nasa_pds_1:all:user:img:commanded_parameters::focus_stack::1.0 rdf:type rdf:Property;
  rdfs:label "Focus_Stack";
  rdfs:domain pds4:urn:nasa:pds:0001_nasa_pds_1:all:user:img:commanded_parameters::1.0;
  rdfs:range pds4:urn:nasa:pds:0001_nasa_pds_1:img:data_processing:img:focus_stack::1.0.
 
pds4:urn:nasa:pds:0001_nasa_pds_1:all:user:img:commanded_parameters::frame::1.0 rdf:type rdf:Property;
  rdfs:label "Frame";
  rdfs:domain pds4:urn:nasa:pds:0001_nasa_pds_1:all:user:img:commanded_parameters::1.0;
  rdfs:range pds4:urn:nasa:pds:0001_nasa_pds_1:all:user:img:frame::1.0.
 
pds4:urn:nasa:pds:0001_nasa_pds_1:all:user:img:commanded_parameters::high_dynamic_range::1.0 rdf:type rdf:Property;
  rdfs:label "High_Dynamic_Range";
  rdfs:domain pds4:urn:nasa:pds:0001_nasa_pds_1:all:user:img:commanded_parameters::1.0;
  rdfs:range pds4:urn:nasa:pds:0001_nasa_pds_1:img:data_processing:img:high_dynamic_range::1.0.
 
pds4:urn:nasa:pds:0001_nasa_pds_1:all:user:img:commanded_parameters::histogram::1.0 rdf:type rdf:Property;
  rdfs:label "Histogram";
  rdfs:domain pds4:urn:nasa:pds:0001_nasa_pds_1:all:user:img:commanded_parameters::1.0;
  rdfs:range pds4:urn:nasa:pds:0001_nasa_pds_1:all:user:img:histogram::1.0.
 
pds4:urn:nasa:pds:0001_nasa_pds_1:all:user:img:commanded_parameters::illumination::1.0 rdf:type rdf:Property;
  rdfs:label "Illumination";
  rdfs:domain pds4:urn:nasa:pds:0001_nasa_pds_1:all:user:img:commanded_parameters::1.0;
  rdfs:range pds4:urn:nasa:pds:0001_nasa_pds_1:all:user:img:illumination::1.0.
 
pds4:urn:nasa:pds:0001_nasa_pds_1:all:user:img:commanded_parameters::image_filter::1.0 rdf:type rdf:Property;
  rdfs:label "Image_Filter";
  rdfs:domain pds4:urn:nasa:pds:0001_nasa_pds_1:all:user:img:commanded_parameters::1.0;
  rdfs:range pds4:urn:nasa:pds:0001_nasa_pds_1:img:data_processing:img:image_filter::1.0.
 
pds4:urn:nasa:pds:0001_nasa_pds_1:all:user:img:commanded_parameters::image_mask::1.0 rdf:type rdf:Property;
  rdfs:label "Image_Mask";
  rdfs:domain pds4:urn:nasa:pds:0001_nasa_pds_1:all:user:img:commanded_parameters::1.0;
  rdfs:range pds4:urn:nasa:pds:0001_nasa_pds_1:all:user:img:image_mask::1.0.
 
pds4:urn:nasa:pds:0001_nasa_pds_1:all:user:img:commanded_parameters::onboard_compression::1.0 rdf:type rdf:Property;
  rdfs:label "Onboard_Compression";
  rdfs:domain pds4:urn:nasa:pds:0001_nasa_pds_1:all:user:img:commanded_parameters::1.0;
  rdfs:range pds4:urn:nasa:pds:0001_nasa_pds_1:all:user:img:onboard_compression::1.0.
 
pds4:urn:nasa:pds:0001_nasa_pds_1:all:user:img:commanded_parameters::optical_filter::1.0 rdf:type rdf:Property;
  rdfs:label "Optical_Filter";
  rdfs:domain pds4:urn:nasa:pds:0001_nasa_pds_1:all:user:img:commanded_parameters::1.0;
  rdfs:range pds4:urn:nasa:pds:0001_nasa_pds_1:all:user:img:optical_filter::1.0.
 
pds4:urn:nasa:pds:0001_nasa_pds_1:all:user:img:commanded_parameters::optical_properties::1.0 rdf:type rdf:Property;
  rdfs:label "Optical_Properties";
  rdfs:domain pds4:urn:nasa:pds:0001_nasa_pds_1:all:user:img:commanded_parameters::1.0;
  rdfs:range pds4:urn:nasa:pds:0001_nasa_pds_1:all:user:img:optical_properties::1.0.
 
pds4:urn:nasa:pds:0001_nasa_pds_1:all:user:img:commanded_parameters::pointing_correction::1.0 rdf:type rdf:Property;
  rdfs:label "Pointing_Correction";
  rdfs:domain pds4:urn:nasa:pds:0001_nasa_pds_1:all:user:img:commanded_parameters::1.0;
  rdfs:range pds4:urn:nasa:pds:0001_nasa_pds_1:all:user:img:pointing_correction::1.0.
 
pds4:urn:nasa:pds:0001_nasa_pds_1:all:user:img:commanded_parameters::radiometric_correction::1.0 rdf:type rdf:Property;
  rdfs:label "Radiometric_Correction";
  rdfs:domain pds4:urn:nasa:pds:0001_nasa_pds_1:all:user:img:commanded_parameters::1.0;
  rdfs:range pds4:urn:nasa:pds:0001_nasa_pds_1:img:data_processing:img:radiometric_correction::1.0.
 
pds4:urn:nasa:pds:0001_nasa_pds_1:all:user:img:commanded_parameters::reference_pixel::1.0 rdf:type rdf:Property;
  rdfs:label "Reference_Pixel";
  rdfs:domain pds4:urn:nasa:pds:0001_nasa_pds_1:all:user:img:commanded_parameters::1.0;
  rdfs:range pds4:urn:nasa:pds:0001_nasa_pds_1:all:user:img:reference_pixel::1.0.
 
pds4:urn:nasa:pds:0001_nasa_pds_1:all:user:img:commanded_parameters::row_sum::1.0 rdf:type rdf:Property;
  rdfs:label "Row_Sum";
  rdfs:domain pds4:urn:nasa:pds:0001_nasa_pds_1:all:user:img:commanded_parameters::1.0;
  rdfs:range pds4:urn:nasa:pds:0001_nasa_pds_1:all:user:img:row_sum::1.0.
 
pds4:urn:nasa:pds:0001_nasa_pds_1:all:user:img:commanded_parameters::sampling::1.0 rdf:type rdf:Property;
  rdfs:label "Sampling";
  rdfs:domain pds4:urn:nasa:pds:0001_nasa_pds_1:all:user:img:commanded_parameters::1.0;
  rdfs:range pds4:urn:nasa:pds:0001_nasa_pds_1:all:user:img:sampling::1.0.
 
pds4:urn:nasa:pds:0001_nasa_pds_1:all:user:img:commanded_parameters::shutter_subtraction::1.0 rdf:type rdf:Property;
  rdfs:label "Shutter_Subtraction";
  rdfs:domain pds4:urn:nasa:pds:0001_nasa_pds_1:all:user:img:commanded_parameters::1.0;
  rdfs:range pds4:urn:nasa:pds:0001_nasa_pds_1:img:data_processing:img:shutter_subtraction::1.0.
 
pds4:urn:nasa:pds:0001_nasa_pds_1:all:user:img:commanded_parameters::spatial_filter::1.0 rdf:type rdf:Property;
  rdfs:label "Spatial_Filter";
  rdfs:domain pds4:urn:nasa:pds:0001_nasa_pds_1:all:user:img:commanded_parameters::1.0;
  rdfs:range pds4:urn:nasa:pds:0001_nasa_pds_1:img:data_processing:img:spatial_filter::1.0.
 
pds4:urn:nasa:pds:0001_nasa_pds_1:all:user:img:commanded_parameters::subframe::1.0 rdf:type rdf:Property;
  rdfs:label "Subframe";
  rdfs:domain pds4:urn:nasa:pds:0001_nasa_pds_1:all:user:img:commanded_parameters::1.0;
  rdfs:range pds4:urn:nasa:pds:0001_nasa_pds_1:all:user:img:subframe::1.0.
 
pds4:urn:nasa:pds:0001_nasa_pds_1:all:user:img:commanded_parameters::thumbnail::1.0 rdf:type rdf:Property;
  rdfs:label "Thumbnail";
  rdfs:domain pds4:urn:nasa:pds:0001_nasa_pds_1:all:user:img:commanded_parameters::1.0;
  rdfs:range pds4:urn:nasa:pds:0001_nasa_pds_1:all:user:img:thumbnail::1.0.
 
pds4:urn:nasa:pds:0001_nasa_pds_1:all:user:img:commanded_parameters::tiling::1.0 rdf:type rdf:Property;
  rdfs:label "Tiling";
  rdfs:domain pds4:urn:nasa:pds:0001_nasa_pds_1:all:user:img:commanded_parameters::1.0;
  rdfs:range pds4:urn:nasa:pds:0001_nasa_pds_1:all:user:img:tiling::1.0.
 
pds4:urn:nasa:pds:0001_nasa_pds_1:all:user:img:commanded_parameters::video::1.0 rdf:type rdf:Property;
  rdfs:label "Video";
  rdfs:domain pds4:urn:nasa:pds:0001_nasa_pds_1:all:user:img:commanded_parameters::1.0;
  rdfs:range pds4:urn:nasa:pds:0001_nasa_pds_1:all:user:img:video::1.0.
 
pds4:urn:nasa:pds:0001_nasa_pds_1:img:data_processing:img:companding::companding_file::1.0 rdf:type rdf:Property;
  rdfs:label "Companding_File";
  rdfs:domain pds4:urn:nasa:pds:0001_nasa_pds_1:img:data_processing:img:companding::1.0;
  rdfs:range pds4:urn:nasa:pds:0001_nasa_pds_1:img:data_processing_file:img:companding_file::1.0.
 
pds4:urn:nasa:pds:0001_nasa_pds_1:img:data_processing:img:companding::companding_table::1.0 rdf:type rdf:Property;
  rdfs:label "Companding_Table";
  rdfs:domain pds4:urn:nasa:pds:0001_nasa_pds_1:img:data_processing:img:companding::1.0;
  rdfs:range pds4:urn:nasa:pds:0001_nasa_pds_1:img:data_processing_file:img:companding_table::1.0.
 
pds4:urn:nasa:pds:0001_nasa_pds_1:img:data_processing_file:img:companding_table::companding_table_mapping::1.0 rdf:type rdf:Property;
  rdfs:label "Companding_Table_Mapping";
  rdfs:domain pds4:urn:nasa:pds:0001_nasa_pds_1:img:data_processing_file:img:companding_table::1.0;
  rdfs:range pds4:urn:nasa:pds:0001_nasa_pds_1:all:user:img:companding_table_mapping::1.0.
 
pds4:urn:nasa:pds:0001_nasa_pds_1:all:user:img:data_processing_file::internal_reference::1.0 rdf:type rdf:Property;
  rdfs:label "Internal_Reference";
  rdfs:domain pds4:urn:nasa:pds:0001_nasa_pds_1:all:user:img:data_processing_file::1.0;
  rdfs:range pds4:urn:nasa:pds:0001_nasa_pds_1:pds:product_components:pds:internal_reference::1.0.
 
pds4:urn:nasa:pds:0001_nasa_pds_1:all:user:img:data_processing_file::external_reference::1.0 rdf:type rdf:Property;
  rdfs:label "External_Reference";
  rdfs:domain pds4:urn:nasa:pds:0001_nasa_pds_1:all:user:img:data_processing_file::1.0;
  rdfs:range pds4:urn:nasa:pds:0001_nasa_pds_1:pds:product_components:pds:external_reference::1.0.
 
pds4:urn:nasa:pds:0001_nasa_pds_1:all:user:img:detector::special_point::1.0 rdf:type rdf:Property;
  rdfs:label "Special_Point";
  rdfs:domain pds4:urn:nasa:pds:0001_nasa_pds_1:all:user:img:detector::1.0;
  rdfs:range pds4:urn:nasa:pds:0001_nasa_pds_1:all:user:img:special_point::1.0.
 
pds4:urn:nasa:pds:0001_nasa_pds_1:all:user:img:detector::internal_reference::1.0 rdf:type rdf:Property;
  rdfs:label "Internal_Reference";
  rdfs:domain pds4:urn:nasa:pds:0001_nasa_pds_1:all:user:img:detector::1.0;
  rdfs:range pds4:urn:nasa:pds:0001_nasa_pds_1:pds:product_components:pds:internal_reference::1.0.
 
pds4:urn:nasa:pds:0001_nasa_pds_1:all:user:img:device_component_states::device_component_state::1.0 rdf:type rdf:Property;
  rdfs:label "Device_Component_State";
  rdfs:domain pds4:urn:nasa:pds:0001_nasa_pds_1:all:user:img:device_component_states::1.0;
  rdfs:range pds4:urn:nasa:pds:0001_nasa_pds_1:img:device_parameters:img:device_component_state::1.0.
 
pds4:urn:nasa:pds:0001_nasa_pds_1:all:user:img:device_currents::device_current::1.0 rdf:type rdf:Property;
  rdfs:label "Device_Current";
  rdfs:domain pds4:urn:nasa:pds:0001_nasa_pds_1:all:user:img:device_currents::1.0;
  rdfs:range pds4:urn:nasa:pds:0001_nasa_pds_1:img:device_parameters:img:device_current::1.0.
 
pds4:urn:nasa:pds:0001_nasa_pds_1:all:user:img:device_motor_counts::device_motor_count::1.0 rdf:type rdf:Property;
  rdfs:label "Device_Motor_Count";
  rdfs:domain pds4:urn:nasa:pds:0001_nasa_pds_1:all:user:img:device_motor_counts::1.0;
  rdfs:range pds4:urn:nasa:pds:0001_nasa_pds_1:img:device_parameters:img:device_motor_count::1.0.
 
pds4:urn:nasa:pds:0001_nasa_pds_1:all:user:img:device_temperatures::device_temperature::1.0 rdf:type rdf:Property;
  rdfs:label "Device_Temperature";
  rdfs:domain pds4:urn:nasa:pds:0001_nasa_pds_1:all:user:img:device_temperatures::1.0;
  rdfs:range pds4:urn:nasa:pds:0001_nasa_pds_1:img:device_parameters:img:device_temperature::1.0.
 
pds4:urn:nasa:pds:0001_nasa_pds_1:all:user:img:device_voltages::device_voltage::1.0 rdf:type rdf:Property;
  rdfs:label "Device_Voltage";
  rdfs:domain pds4:urn:nasa:pds:0001_nasa_pds_1:all:user:img:device_voltages::1.0;
  rdfs:range pds4:urn:nasa:pds:0001_nasa_pds_1:img:device_parameters:img:device_voltage::1.0.
 
pds4:urn:nasa:pds:0001_nasa_pds_1:img:data_processing:img:downsampling::pixel_averaging_dimensions::1.0 rdf:type rdf:Property;
  rdfs:label "Pixel_Averaging_Dimensions";
  rdfs:domain pds4:urn:nasa:pds:0001_nasa_pds_1:img:data_processing:img:downsampling::1.0;
  rdfs:range pds4:urn:nasa:pds:0001_nasa_pds_1:all:user:img:pixel_averaging_dimensions::1.0.
 
pds4:urn:nasa:pds:0001_nasa_pds_1:all:user:img:exposure::autoexposure::1.0 rdf:type rdf:Property;
  rdfs:label "Autoexposure";
  rdfs:domain pds4:urn:nasa:pds:0001_nasa_pds_1:all:user:img:exposure::1.0;
  rdfs:range pds4:urn:nasa:pds:0001_nasa_pds_1:img:data_processing:img:autoexposure::1.0.
 
pds4:urn:nasa:pds:0001_nasa_pds_1:img:data_processing:img:flat_field_correction::radial_flat_field_function::1.0 rdf:type rdf:Property;
  rdfs:label "Radial_Flat_Field_Function";
  rdfs:domain pds4:urn:nasa:pds:0001_nasa_pds_1:img:data_processing:img:flat_field_correction::1.0;
  rdfs:range pds4:urn:nasa:pds:0001_nasa_pds_1:all:user:img:radial_flat_field_function::1.0.
 
pds4:urn:nasa:pds:0001_nasa_pds_1:img:data_processing:img:flat_field_correction::flat_field_file::1.0 rdf:type rdf:Property;
  rdfs:label "Flat_Field_File";
  rdfs:domain pds4:urn:nasa:pds:0001_nasa_pds_1:img:data_processing:img:flat_field_correction::1.0;
  rdfs:range pds4:urn:nasa:pds:0001_nasa_pds_1:img:data_processing_file:img:flat_field_file::1.0.
 
pds4:urn:nasa:pds:0001_nasa_pds_1:img:data_processing:img:high_dynamic_range::high_dynamic_range_exposure::1.0 rdf:type rdf:Property;
  rdfs:label "High_Dynamic_Range_Exposure";
  rdfs:domain pds4:urn:nasa:pds:0001_nasa_pds_1:img:data_processing:img:high_dynamic_range::1.0;
  rdfs:range pds4:urn:nasa:pds:0001_nasa_pds_1:all:user:img:high_dynamic_range_exposure::1.0.
 
pds4:urn:nasa:pds:0001_nasa_pds_1:all:user:img:high_dynamic_range_exposure::internal_reference::1.0 rdf:type rdf:Property;
  rdfs:label "Internal_Reference";
  rdfs:domain pds4:urn:nasa:pds:0001_nasa_pds_1:all:user:img:high_dynamic_range_exposure::1.0;
  rdfs:range pds4:urn:nasa:pds:0001_nasa_pds_1:pds:product_components:pds:internal_reference::1.0.
 
pds4:urn:nasa:pds:0001_nasa_pds_1:all:user:img:icer_parameters::image_compression_segment::1.0 rdf:type rdf:Property;
  rdfs:label "Image_Compression_Segment";
  rdfs:domain pds4:urn:nasa:pds:0001_nasa_pds_1:all:user:img:icer_parameters::1.0;
  rdfs:range pds4:urn:nasa:pds:0001_nasa_pds_1:all:user:img:image_compression_segment::1.0.
 
pds4:urn:nasa:pds:0001_nasa_pds_1:all:user:img:illumination::led_illumination_source::1.0 rdf:type rdf:Property;
  rdfs:label "LED_Illumination_Source";
  rdfs:domain pds4:urn:nasa:pds:0001_nasa_pds_1:all:user:img:illumination::1.0;
  rdfs:range pds4:urn:nasa:pds:0001_nasa_pds_1:all:user:img:led_illumination_source::1.0.
 
pds4:urn:nasa:pds:0001_nasa_pds_1:all:user:img:image_mask::image_mask_file::1.0 rdf:type rdf:Property;
  rdfs:label "Image_Mask_File";
  rdfs:domain pds4:urn:nasa:pds:0001_nasa_pds_1:all:user:img:image_mask::1.0;
  rdfs:range pds4:urn:nasa:pds:0001_nasa_pds_1:all:user:img:image_mask_file::1.0.
 
pds4:urn:nasa:pds:0001_nasa_pds_1:all:user:img:image_mask_file::internal_reference::1.0 rdf:type rdf:Property;
  rdfs:label "Internal_Reference";
  rdfs:domain pds4:urn:nasa:pds:0001_nasa_pds_1:all:user:img:image_mask_file::1.0;
  rdfs:range pds4:urn:nasa:pds:0001_nasa_pds_1:pds:product_components:pds:internal_reference::1.0.
 
pds4:urn:nasa:pds:0001_nasa_pds_1:all:user:img:image_mask_file::external_reference::1.0 rdf:type rdf:Property;
  rdfs:label "External_Reference";
  rdfs:domain pds4:urn:nasa:pds:0001_nasa_pds_1:all:user:img:image_mask_file::1.0;
  rdfs:range pds4:urn:nasa:pds:0001_nasa_pds_1:pds:product_components:pds:external_reference::1.0.
 
pds4:urn:nasa:pds:0001_nasa_pds_1:all:user:img:imaging::local_internal_reference::1.0 rdf:type rdf:Property;
  rdfs:label "Local_Internal_Reference";
  rdfs:domain pds4:urn:nasa:pds:0001_nasa_pds_1:all:user:img:imaging::1.0;
  rdfs:range pds4:urn:nasa:pds:0001_nasa_pds_1:pds:product_components:pds:local_internal_reference::1.0.
 
pds4:urn:nasa:pds:0001_nasa_pds_1:all:user:img:imaging::brightness_correction::1.0 rdf:type rdf:Property;
  rdfs:label "Brightness_Correction";
  rdfs:domain pds4:urn:nasa:pds:0001_nasa_pds_1:all:user:img:imaging::1.0;
  rdfs:range pds4:urn:nasa:pds:0001_nasa_pds_1:img:data_processing:img:brightness_correction::1.0.
 
pds4:urn:nasa:pds:0001_nasa_pds_1:all:user:img:imaging::col_sum::1.0 rdf:type rdf:Property;
  rdfs:label "Col_Sum";
  rdfs:domain pds4:urn:nasa:pds:0001_nasa_pds_1:all:user:img:imaging::1.0;
  rdfs:range pds4:urn:nasa:pds:0001_nasa_pds_1:all:user:img:col_sum::1.0.
 
pds4:urn:nasa:pds:0001_nasa_pds_1:all:user:img:imaging::color_filter_array::1.0 rdf:type rdf:Property;
  rdfs:label "Color_Filter_Array";
  rdfs:domain pds4:urn:nasa:pds:0001_nasa_pds_1:all:user:img:imaging::1.0;
  rdfs:range pds4:urn:nasa:pds:0001_nasa_pds_1:img:data_processing:img:color_filter_array::1.0.
 
pds4:urn:nasa:pds:0001_nasa_pds_1:all:user:img:imaging::color_processing::1.0 rdf:type rdf:Property;
  rdfs:label "Color_Processing";
  rdfs:domain pds4:urn:nasa:pds:0001_nasa_pds_1:all:user:img:imaging::1.0;
  rdfs:range pds4:urn:nasa:pds:0001_nasa_pds_1:img:data_processing:img:color_processing::1.0.
 
pds4:urn:nasa:pds:0001_nasa_pds_1:all:user:img:imaging::dark_current_correction::1.0 rdf:type rdf:Property;
  rdfs:label "Dark_Current_Correction";
  rdfs:domain pds4:urn:nasa:pds:0001_nasa_pds_1:all:user:img:imaging::1.0;
  rdfs:range pds4:urn:nasa:pds:0001_nasa_pds_1:img:data_processing:img:dark_current_correction::1.0.
 
pds4:urn:nasa:pds:0001_nasa_pds_1:all:user:img:imaging::detector::1.0 rdf:type rdf:Property;
  rdfs:label "Detector";
  rdfs:domain pds4:urn:nasa:pds:0001_nasa_pds_1:all:user:img:imaging::1.0;
  rdfs:range pds4:urn:nasa:pds:0001_nasa_pds_1:all:user:img:detector::1.0.
 
pds4:urn:nasa:pds:0001_nasa_pds_1:all:user:img:imaging::downsampling::1.0 rdf:type rdf:Property;
  rdfs:label "Downsampling";
  rdfs:domain pds4:urn:nasa:pds:0001_nasa_pds_1:all:user:img:imaging::1.0;
  rdfs:range pds4:urn:nasa:pds:0001_nasa_pds_1:img:data_processing:img:downsampling::1.0.
 
pds4:urn:nasa:pds:0001_nasa_pds_1:all:user:img:imaging::exposure::1.0 rdf:type rdf:Property;
  rdfs:label "Exposure";
  rdfs:domain pds4:urn:nasa:pds:0001_nasa_pds_1:all:user:img:imaging::1.0;
  rdfs:range pds4:urn:nasa:pds:0001_nasa_pds_1:all:user:img:exposure::1.0.
 
pds4:urn:nasa:pds:0001_nasa_pds_1:all:user:img:imaging::flat_field_correction::1.0 rdf:type rdf:Property;
  rdfs:label "Flat_Field_Correction";
  rdfs:domain pds4:urn:nasa:pds:0001_nasa_pds_1:all:user:img:imaging::1.0;
  rdfs:range pds4:urn:nasa:pds:0001_nasa_pds_1:img:data_processing:img:flat_field_correction::1.0.
 
pds4:urn:nasa:pds:0001_nasa_pds_1:all:user:img:imaging::focus::1.0 rdf:type rdf:Property;
  rdfs:label "Focus";
  rdfs:domain pds4:urn:nasa:pds:0001_nasa_pds_1:all:user:img:imaging::1.0;
  rdfs:range pds4:urn:nasa:pds:0001_nasa_pds_1:all:user:img:focus::1.0.
 
pds4:urn:nasa:pds:0001_nasa_pds_1:all:user:img:imaging::focus_stack::1.0 rdf:type rdf:Property;
  rdfs:label "Focus_Stack";
  rdfs:domain pds4:urn:nasa:pds:0001_nasa_pds_1:all:user:img:imaging::1.0;
  rdfs:range pds4:urn:nasa:pds:0001_nasa_pds_1:img:data_processing:img:focus_stack::1.0.
 
pds4:urn:nasa:pds:0001_nasa_pds_1:all:user:img:imaging::frame::1.0 rdf:type rdf:Property;
  rdfs:label "Frame";
  rdfs:domain pds4:urn:nasa:pds:0001_nasa_pds_1:all:user:img:imaging::1.0;
  rdfs:range pds4:urn:nasa:pds:0001_nasa_pds_1:all:user:img:frame::1.0.
 
pds4:urn:nasa:pds:0001_nasa_pds_1:all:user:img:imaging::high_dynamic_range::1.0 rdf:type rdf:Property;
  rdfs:label "High_Dynamic_Range";
  rdfs:domain pds4:urn:nasa:pds:0001_nasa_pds_1:all:user:img:imaging::1.0;
  rdfs:range pds4:urn:nasa:pds:0001_nasa_pds_1:img:data_processing:img:high_dynamic_range::1.0.
 
pds4:urn:nasa:pds:0001_nasa_pds_1:all:user:img:imaging::histogram::1.0 rdf:type rdf:Property;
  rdfs:label "Histogram";
  rdfs:domain pds4:urn:nasa:pds:0001_nasa_pds_1:all:user:img:imaging::1.0;
  rdfs:range pds4:urn:nasa:pds:0001_nasa_pds_1:all:user:img:histogram::1.0.
 
pds4:urn:nasa:pds:0001_nasa_pds_1:all:user:img:imaging::illumination::1.0 rdf:type rdf:Property;
  rdfs:label "Illumination";
  rdfs:domain pds4:urn:nasa:pds:0001_nasa_pds_1:all:user:img:imaging::1.0;
  rdfs:range pds4:urn:nasa:pds:0001_nasa_pds_1:all:user:img:illumination::1.0.
 
pds4:urn:nasa:pds:0001_nasa_pds_1:all:user:img:imaging::image_filter::1.0 rdf:type rdf:Property;
  rdfs:label "Image_Filter";
  rdfs:domain pds4:urn:nasa:pds:0001_nasa_pds_1:all:user:img:imaging::1.0;
  rdfs:range pds4:urn:nasa:pds:0001_nasa_pds_1:img:data_processing:img:image_filter::1.0.
 
pds4:urn:nasa:pds:0001_nasa_pds_1:all:user:img:imaging::image_mask::1.0 rdf:type rdf:Property;
  rdfs:label "Image_Mask";
  rdfs:domain pds4:urn:nasa:pds:0001_nasa_pds_1:all:user:img:imaging::1.0;
  rdfs:range pds4:urn:nasa:pds:0001_nasa_pds_1:all:user:img:image_mask::1.0.
 
pds4:urn:nasa:pds:0001_nasa_pds_1:all:user:img:imaging::onboard_compression::1.0 rdf:type rdf:Property;
  rdfs:label "Onboard_Compression";
  rdfs:domain pds4:urn:nasa:pds:0001_nasa_pds_1:all:user:img:imaging::1.0;
  rdfs:range pds4:urn:nasa:pds:0001_nasa_pds_1:all:user:img:onboard_compression::1.0.
 
pds4:urn:nasa:pds:0001_nasa_pds_1:all:user:img:imaging::optical_filter::1.0 rdf:type rdf:Property;
  rdfs:label "Optical_Filter";
  rdfs:domain pds4:urn:nasa:pds:0001_nasa_pds_1:all:user:img:imaging::1.0;
  rdfs:range pds4:urn:nasa:pds:0001_nasa_pds_1:all:user:img:optical_filter::1.0.
 
pds4:urn:nasa:pds:0001_nasa_pds_1:all:user:img:imaging::optical_properties::1.0 rdf:type rdf:Property;
  rdfs:label "Optical_Properties";
  rdfs:domain pds4:urn:nasa:pds:0001_nasa_pds_1:all:user:img:imaging::1.0;
  rdfs:range pds4:urn:nasa:pds:0001_nasa_pds_1:all:user:img:optical_properties::1.0.
 
pds4:urn:nasa:pds:0001_nasa_pds_1:all:user:img:imaging::pointing_correction::1.0 rdf:type rdf:Property;
  rdfs:label "Pointing_Correction";
  rdfs:domain pds4:urn:nasa:pds:0001_nasa_pds_1:all:user:img:imaging::1.0;
  rdfs:range pds4:urn:nasa:pds:0001_nasa_pds_1:all:user:img:pointing_correction::1.0.
 
pds4:urn:nasa:pds:0001_nasa_pds_1:all:user:img:imaging::radiometric_correction::1.0 rdf:type rdf:Property;
  rdfs:label "Radiometric_Correction";
  rdfs:domain pds4:urn:nasa:pds:0001_nasa_pds_1:all:user:img:imaging::1.0;
  rdfs:range pds4:urn:nasa:pds:0001_nasa_pds_1:img:data_processing:img:radiometric_correction::1.0.
 
pds4:urn:nasa:pds:0001_nasa_pds_1:all:user:img:imaging::reference_pixel::1.0 rdf:type rdf:Property;
  rdfs:label "Reference_Pixel";
  rdfs:domain pds4:urn:nasa:pds:0001_nasa_pds_1:all:user:img:imaging::1.0;
  rdfs:range pds4:urn:nasa:pds:0001_nasa_pds_1:all:user:img:reference_pixel::1.0.
 
pds4:urn:nasa:pds:0001_nasa_pds_1:all:user:img:imaging::row_sum::1.0 rdf:type rdf:Property;
  rdfs:label "Row_Sum";
  rdfs:domain pds4:urn:nasa:pds:0001_nasa_pds_1:all:user:img:imaging::1.0;
  rdfs:range pds4:urn:nasa:pds:0001_nasa_pds_1:all:user:img:row_sum::1.0.
 
pds4:urn:nasa:pds:0001_nasa_pds_1:all:user:img:imaging::sampling::1.0 rdf:type rdf:Property;
  rdfs:label "Sampling";
  rdfs:domain pds4:urn:nasa:pds:0001_nasa_pds_1:all:user:img:imaging::1.0;
  rdfs:range pds4:urn:nasa:pds:0001_nasa_pds_1:all:user:img:sampling::1.0.
 
pds4:urn:nasa:pds:0001_nasa_pds_1:all:user:img:imaging::shutter_subtraction::1.0 rdf:type rdf:Property;
  rdfs:label "Shutter_Subtraction";
  rdfs:domain pds4:urn:nasa:pds:0001_nasa_pds_1:all:user:img:imaging::1.0;
  rdfs:range pds4:urn:nasa:pds:0001_nasa_pds_1:img:data_processing:img:shutter_subtraction::1.0.
 
pds4:urn:nasa:pds:0001_nasa_pds_1:all:user:img:imaging::spatial_filter::1.0 rdf:type rdf:Property;
  rdfs:label "Spatial_Filter";
  rdfs:domain pds4:urn:nasa:pds:0001_nasa_pds_1:all:user:img:imaging::1.0;
  rdfs:range pds4:urn:nasa:pds:0001_nasa_pds_1:img:data_processing:img:spatial_filter::1.0.
 
pds4:urn:nasa:pds:0001_nasa_pds_1:all:user:img:imaging::subframe::1.0 rdf:type rdf:Property;
  rdfs:label "Subframe";
  rdfs:domain pds4:urn:nasa:pds:0001_nasa_pds_1:all:user:img:imaging::1.0;
  rdfs:range pds4:urn:nasa:pds:0001_nasa_pds_1:all:user:img:subframe::1.0.
 
pds4:urn:nasa:pds:0001_nasa_pds_1:all:user:img:imaging::tiling::1.0 rdf:type rdf:Property;
  rdfs:label "Tiling";
  rdfs:domain pds4:urn:nasa:pds:0001_nasa_pds_1:all:user:img:imaging::1.0;
  rdfs:range pds4:urn:nasa:pds:0001_nasa_pds_1:all:user:img:tiling::1.0.
 
pds4:urn:nasa:pds:0001_nasa_pds_1:all:user:img:imaging::thumbnail::1.0 rdf:type rdf:Property;
  rdfs:label "Thumbnail";
  rdfs:domain pds4:urn:nasa:pds:0001_nasa_pds_1:all:user:img:imaging::1.0;
  rdfs:range pds4:urn:nasa:pds:0001_nasa_pds_1:all:user:img:thumbnail::1.0.
 
pds4:urn:nasa:pds:0001_nasa_pds_1:all:user:img:imaging::video::1.0 rdf:type rdf:Property;
  rdfs:label "Video";
  rdfs:domain pds4:urn:nasa:pds:0001_nasa_pds_1:all:user:img:imaging::1.0;
  rdfs:range pds4:urn:nasa:pds:0001_nasa_pds_1:all:user:img:video::1.0.
 
pds4:urn:nasa:pds:0001_nasa_pds_1:all:user:img:imaging::instrument_state::1.0 rdf:type rdf:Property;
  rdfs:label "Instrument_State";
  rdfs:domain pds4:urn:nasa:pds:0001_nasa_pds_1:all:user:img:imaging::1.0;
  rdfs:range pds4:urn:nasa:pds:0001_nasa_pds_1:all:user:img:instrument_state::1.0.
 
pds4:urn:nasa:pds:0001_nasa_pds_1:all:user:img:imaging::commanded_parameters::1.0 rdf:type rdf:Property;
  rdfs:label "Commanded_Parameters";
  rdfs:domain pds4:urn:nasa:pds:0001_nasa_pds_1:all:user:img:imaging::1.0;
  rdfs:range pds4:urn:nasa:pds:0001_nasa_pds_1:all:user:img:commanded_parameters::1.0.
 
pds4:urn:nasa:pds:0001_nasa_pds_1:all:user:img:instrument_state::device_component_states::1.0 rdf:type rdf:Property;
  rdfs:label "Device_Component_States";
  rdfs:domain pds4:urn:nasa:pds:0001_nasa_pds_1:all:user:img:instrument_state::1.0;
  rdfs:range pds4:urn:nasa:pds:0001_nasa_pds_1:all:user:img:device_component_states::1.0.
 
pds4:urn:nasa:pds:0001_nasa_pds_1:all:user:img:instrument_state::device_currents::1.0 rdf:type rdf:Property;
  rdfs:label "Device_Currents";
  rdfs:domain pds4:urn:nasa:pds:0001_nasa_pds_1:all:user:img:instrument_state::1.0;
  rdfs:range pds4:urn:nasa:pds:0001_nasa_pds_1:all:user:img:device_currents::1.0.
 
pds4:urn:nasa:pds:0001_nasa_pds_1:all:user:img:instrument_state::device_motor_counts::1.0 rdf:type rdf:Property;
  rdfs:label "Device_Motor_Counts";
  rdfs:domain pds4:urn:nasa:pds:0001_nasa_pds_1:all:user:img:instrument_state::1.0;
  rdfs:range pds4:urn:nasa:pds:0001_nasa_pds_1:all:user:img:device_motor_counts::1.0.
 
pds4:urn:nasa:pds:0001_nasa_pds_1:all:user:img:instrument_state::device_temperatures::1.0 rdf:type rdf:Property;
  rdfs:label "Device_Temperatures";
  rdfs:domain pds4:urn:nasa:pds:0001_nasa_pds_1:all:user:img:instrument_state::1.0;
  rdfs:range pds4:urn:nasa:pds:0001_nasa_pds_1:all:user:img:device_temperatures::1.0.
 
pds4:urn:nasa:pds:0001_nasa_pds_1:all:user:img:instrument_state::device_voltages::1.0 rdf:type rdf:Property;
  rdfs:label "Device_Voltages";
  rdfs:domain pds4:urn:nasa:pds:0001_nasa_pds_1:all:user:img:instrument_state::1.0;
  rdfs:range pds4:urn:nasa:pds:0001_nasa_pds_1:all:user:img:device_voltages::1.0.
 
pds4:urn:nasa:pds:0001_nasa_pds_1:all:user:img:jpeg_parameters::image_compression_segment::1.0 rdf:type rdf:Property;
  rdfs:label "Image_Compression_Segment";
  rdfs:domain pds4:urn:nasa:pds:0001_nasa_pds_1:all:user:img:jpeg_parameters::1.0;
  rdfs:range pds4:urn:nasa:pds:0001_nasa_pds_1:all:user:img:image_compression_segment::1.0.
 
pds4:urn:nasa:pds:0001_nasa_pds_1:all:user:img:loco_parameters::image_compression_segment::1.0 rdf:type rdf:Property;
  rdfs:label "Image_Compression_Segment";
  rdfs:domain pds4:urn:nasa:pds:0001_nasa_pds_1:all:user:img:loco_parameters::1.0;
  rdfs:range pds4:urn:nasa:pds:0001_nasa_pds_1:all:user:img:image_compression_segment::1.0.
 
pds4:urn:nasa:pds:0001_nasa_pds_1:all:user:img:onboard_compression::icer_parameters::1.0 rdf:type rdf:Property;
  rdfs:label "ICER_Parameters";
  rdfs:domain pds4:urn:nasa:pds:0001_nasa_pds_1:all:user:img:onboard_compression::1.0;
  rdfs:range pds4:urn:nasa:pds:0001_nasa_pds_1:all:user:img:icer_parameters::1.0.
 
pds4:urn:nasa:pds:0001_nasa_pds_1:all:user:img:onboard_compression::loco_parameters::1.0 rdf:type rdf:Property;
  rdfs:label "LOCO_Parameters";
  rdfs:domain pds4:urn:nasa:pds:0001_nasa_pds_1:all:user:img:onboard_compression::1.0;
  rdfs:range pds4:urn:nasa:pds:0001_nasa_pds_1:all:user:img:loco_parameters::1.0.
 
pds4:urn:nasa:pds:0001_nasa_pds_1:all:user:img:onboard_compression::jpeg_parameters::1.0 rdf:type rdf:Property;
  rdfs:label "JPEG_Parameters";
  rdfs:domain pds4:urn:nasa:pds:0001_nasa_pds_1:all:user:img:onboard_compression::1.0;
  rdfs:range pds4:urn:nasa:pds:0001_nasa_pds_1:all:user:img:jpeg_parameters::1.0.
 
pds4:urn:nasa:pds:0001_nasa_pds_1:all:user:img:onboard_compression::jpeg_progressive_parameters::1.0 rdf:type rdf:Property;
  rdfs:label "JPEG_Progressive_Parameters";
  rdfs:domain pds4:urn:nasa:pds:0001_nasa_pds_1:all:user:img:onboard_compression::1.0;
  rdfs:range pds4:urn:nasa:pds:0001_nasa_pds_1:img:jpeg_parameters:img:jpeg_progressive_parameters::1.0.
 
pds4:urn:nasa:pds:0001_nasa_pds_1:all:user:img:optical_filter::local_internal_reference::1.0 rdf:type rdf:Property;
  rdfs:label "Local_Internal_Reference";
  rdfs:domain pds4:urn:nasa:pds:0001_nasa_pds_1:all:user:img:optical_filter::1.0;
  rdfs:range pds4:urn:nasa:pds:0001_nasa_pds_1:pds:product_components:pds:local_internal_reference::1.0.
 
pds4:urn:nasa:pds:0001_nasa_pds_1:all:user:img:pointing_correction::pointing_correction_file::1.0 rdf:type rdf:Property;
  rdfs:label "Pointing_Correction_File";
  rdfs:domain pds4:urn:nasa:pds:0001_nasa_pds_1:all:user:img:pointing_correction::1.0;
  rdfs:range pds4:urn:nasa:pds:0001_nasa_pds_1:img:data_processing_file:img:pointing_correction_file::1.0.
 
pds4:urn:nasa:pds:0001_nasa_pds_1:all:user:img:pointing_correction::pointing_correction_image::1.0 rdf:type rdf:Property;
  rdfs:label "Pointing_Correction_Image";
  rdfs:domain pds4:urn:nasa:pds:0001_nasa_pds_1:all:user:img:pointing_correction::1.0;
  rdfs:range pds4:urn:nasa:pds:0001_nasa_pds_1:all:user:img:pointing_correction_image::1.0.
 
pds4:urn:nasa:pds:0001_nasa_pds_1:all:user:img:pointing_correction_image::pointing_model_parameter::1.0 rdf:type rdf:Property;
  rdfs:label "Pointing_Model_Parameter";
  rdfs:domain pds4:urn:nasa:pds:0001_nasa_pds_1:all:user:img:pointing_correction_image::1.0;
  rdfs:range pds4:urn:nasa:pds:0001_nasa_pds_1:all:user:img:pointing_model_parameter::1.0.
 
pds4:urn:nasa:pds:0001_nasa_pds_1:all:user:img:radial_flat_field_function::flat_field_file::1.0 rdf:type rdf:Property;
  rdfs:label "Flat_Field_File";
  rdfs:domain pds4:urn:nasa:pds:0001_nasa_pds_1:all:user:img:radial_flat_field_function::1.0;
  rdfs:range pds4:urn:nasa:pds:0001_nasa_pds_1:img:data_processing_file:img:flat_field_file::1.0.
 
pds4:urn:nasa:pds:0001_nasa_pds_1:all:user:img:reference_pixel::onboard_compression::1.0 rdf:type rdf:Property;
  rdfs:label "Onboard_Compression";
  rdfs:domain pds4:urn:nasa:pds:0001_nasa_pds_1:all:user:img:reference_pixel::1.0;
  rdfs:range pds4:urn:nasa:pds:0001_nasa_pds_1:all:user:img:onboard_compression::1.0.
 
pds4:urn:nasa:pds:0001_nasa_pds_1:all:user:img:sampling::companding::1.0 rdf:type rdf:Property;
  rdfs:label "Companding";
  rdfs:domain pds4:urn:nasa:pds:0001_nasa_pds_1:all:user:img:sampling::1.0;
  rdfs:range pds4:urn:nasa:pds:0001_nasa_pds_1:img:data_processing:img:companding::1.0.
 
pds4:urn:nasa:pds:0001_nasa_pds_1:all:user:img:thumbnail::onboard_compression::1.0 rdf:type rdf:Property;
  rdfs:label "Onboard_Compression";
  rdfs:domain pds4:urn:nasa:pds:0001_nasa_pds_1:all:user:img:thumbnail::1.0;
  rdfs:range pds4:urn:nasa:pds:0001_nasa_pds_1:all:user:img:onboard_compression::1.0.
 
pds4:urn:nasa:pds:0001_nasa_pds_1:all:user:img:thumbnail::sampling::1.0 rdf:type rdf:Property;
  rdfs:label "Sampling";
  rdfs:domain pds4:urn:nasa:pds:0001_nasa_pds_1:all:user:img:thumbnail::1.0;
  rdfs:range pds4:urn:nasa:pds:0001_nasa_pds_1:all:user:img:sampling::1.0.
 
pds4:urn:nasa:pds:0001_nasa_pds_1:all:user:img:thumbnail::subframe::1.0 rdf:type rdf:Property;
  rdfs:label "Subframe";
  rdfs:domain pds4:urn:nasa:pds:0001_nasa_pds_1:all:user:img:thumbnail::1.0;
  rdfs:range pds4:urn:nasa:pds:0001_nasa_pds_1:all:user:img:subframe::1.0.
 
pds4:urn:nasa:pds:0001_nasa_pds_1:all:user:img:tile::internal_reference::1.0 rdf:type rdf:Property;
  rdfs:label "Internal_Reference";
  rdfs:domain pds4:urn:nasa:pds:0001_nasa_pds_1:all:user:img:tile::1.0;
  rdfs:range pds4:urn:nasa:pds:0001_nasa_pds_1:pds:product_components:pds:internal_reference::1.0.
 
pds4:urn:nasa:pds:0001_nasa_pds_1:all:user:img:tile::local_internal_reference::1.0 rdf:type rdf:Property;
  rdfs:label "Local_Internal_Reference";
  rdfs:domain pds4:urn:nasa:pds:0001_nasa_pds_1:all:user:img:tile::1.0;
  rdfs:range pds4:urn:nasa:pds:0001_nasa_pds_1:pds:product_components:pds:local_internal_reference::1.0.
 
pds4:urn:nasa:pds:0001_nasa_pds_1:all:user:img:tile::external_reference::1.0 rdf:type rdf:Property;
  rdfs:label "External_Reference";
  rdfs:domain pds4:urn:nasa:pds:0001_nasa_pds_1:all:user:img:tile::1.0;
  rdfs:range pds4:urn:nasa:pds:0001_nasa_pds_1:pds:product_components:pds:external_reference::1.0.
 
pds4:urn:nasa:pds:0001_nasa_pds_1:all:user:img:tile::pixel_averaging_dimensions::1.0 rdf:type rdf:Property;
  rdfs:label "Pixel_Averaging_Dimensions";
  rdfs:domain pds4:urn:nasa:pds:0001_nasa_pds_1:all:user:img:tile::1.0;
  rdfs:range pds4:urn:nasa:pds:0001_nasa_pds_1:all:user:img:pixel_averaging_dimensions::1.0.
 
pds4:urn:nasa:pds:0001_nasa_pds_1:all:user:img:tile::subframe::1.0 rdf:type rdf:Property;
  rdfs:label "Subframe";
  rdfs:domain pds4:urn:nasa:pds:0001_nasa_pds_1:all:user:img:tile::1.0;
  rdfs:range pds4:urn:nasa:pds:0001_nasa_pds_1:all:user:img:subframe::1.0.
 
pds4:urn:nasa:pds:0001_nasa_pds_1:all:user:img:tiling::tile::1.0 rdf:type rdf:Property;
  rdfs:label "Tile";
  rdfs:domain pds4:urn:nasa:pds:0001_nasa_pds_1:all:user:img:tiling::1.0;
  rdfs:range pds4:urn:nasa:pds:0001_nasa_pds_1:all:user:img:tile::1.0.
 
pds4:urn:nasa:pds:0001_nasa_pds_1:all:user:img:video::internal_reference::1.0 rdf:type rdf:Property;
  rdfs:label "Internal_Reference";
  rdfs:domain pds4:urn:nasa:pds:0001_nasa_pds_1:all:user:img:video::1.0;
  rdfs:range pds4:urn:nasa:pds:0001_nasa_pds_1:pds:product_components:pds:internal_reference::1.0.
 
pds4:urn:nasa:pds:0001_nasa_pds_1:all:user:img:video::external_reference::1.0 rdf:type rdf:Property;
  rdfs:label "External_Reference";
  rdfs:domain pds4:urn:nasa:pds:0001_nasa_pds_1:all:user:img:video::1.0;
  rdfs:range pds4:urn:nasa:pds:0001_nasa_pds_1:pds:product_components:pds:external_reference::1.0.
 
pds4:urn:nasa:pds:0001_nasa_pds_1:all:user:img_surface:commanded_parameters::instrument_information::1.0 rdf:type rdf:Property;
  rdfs:label "Instrument_Information";
  rdfs:domain pds4:urn:nasa:pds:0001_nasa_pds_1:all:user:img_surface:commanded_parameters::1.0;
  rdfs:range pds4:urn:nasa:pds:0001_nasa_pds_1:all:user:img_surface:instrument_information::1.0.
 
pds4:urn:nasa:pds:0001_nasa_pds_1:all:user:img_surface:commanded_parameters::image_identifiers::1.0 rdf:type rdf:Property;
  rdfs:label "Image_Identifiers";
  rdfs:domain pds4:urn:nasa:pds:0001_nasa_pds_1:all:user:img_surface:commanded_parameters::1.0;
  rdfs:range pds4:urn:nasa:pds:0001_nasa_pds_1:all:user:img_surface:image_identifiers::1.0.
 
pds4:urn:nasa:pds:0001_nasa_pds_1:all:user:img_surface:configurations::configuration::1.0 rdf:type rdf:Property;
  rdfs:label "Configuration";
  rdfs:domain pds4:urn:nasa:pds:0001_nasa_pds_1:all:user:img_surface:configurations::1.0;
  rdfs:range pds4:urn:nasa:pds:0001_nasa_pds_1:all:user:img_surface:configuration::1.0.
 
pds4:urn:nasa:pds:0001_nasa_pds_1:all:user:img_surface:derived_product_parameters::placement_target_instrument::1.0 rdf:type rdf:Property;
  rdfs:label "Placement_Target_Instrument";
  rdfs:domain pds4:urn:nasa:pds:0001_nasa_pds_1:all:user:img_surface:derived_product_parameters::1.0;
  rdfs:range pds4:urn:nasa:pds:0001_nasa_pds_1:all:user:img_surface:placement_target_instrument::1.0.
 
pds4:urn:nasa:pds:0001_nasa_pds_1:all:user:img_surface:derived_product_parameters::vector_range_origin::1.0 rdf:type rdf:Property;
  rdfs:label "Vector_Range_Origin";
  rdfs:domain pds4:urn:nasa:pds:0001_nasa_pds_1:all:user:img_surface:derived_product_parameters::1.0;
  rdfs:range pds4:urn:nasa:pds:0001_nasa_pds_1:all:user:img_surface:vector_range_origin::1.0.
 
pds4:urn:nasa:pds:0001_nasa_pds_1:all:user:img_surface:derived_product_parameters::coordinate_space_reference::1.0 rdf:type rdf:Property;
  rdfs:label "Coordinate_Space_Reference";
  rdfs:domain pds4:urn:nasa:pds:0001_nasa_pds_1:all:user:img_surface:derived_product_parameters::1.0;
  rdfs:range pds4:urn:nasa:pds:0001_nasa_pds_1:geom:coordinate_space_identification:geom:coordinate_space_reference::1.0.
 
pds4:urn:nasa:pds:0001_nasa_pds_1:all:user:img_surface:error_model::error_model_parameter::1.0 rdf:type rdf:Property;
  rdfs:label "Error_Model_Parameter";
  rdfs:domain pds4:urn:nasa:pds:0001_nasa_pds_1:all:user:img_surface:error_model::1.0;
  rdfs:range pds4:urn:nasa:pds:0001_nasa_pds_1:all:user:img_surface:error_model_parameter::1.0.
 
pds4:urn:nasa:pds:0001_nasa_pds_1:all:user:img_surface:error_model::internal_reference::1.0 rdf:type rdf:Property;
  rdfs:label "Internal_Reference";
  rdfs:domain pds4:urn:nasa:pds:0001_nasa_pds_1:all:user:img_surface:error_model::1.0;
  rdfs:range pds4:urn:nasa:pds:0001_nasa_pds_1:pds:product_components:pds:internal_reference::1.0.
 
pds4:urn:nasa:pds:0001_nasa_pds_1:all:user:img_surface:geometry_projection::internal_reference::1.0 rdf:type rdf:Property;
  rdfs:label "Internal_Reference";
  rdfs:domain pds4:urn:nasa:pds:0001_nasa_pds_1:all:user:img_surface:geometry_projection::1.0;
  rdfs:range pds4:urn:nasa:pds:0001_nasa_pds_1:pds:product_components:pds:internal_reference::1.0.
 
pds4:urn:nasa:pds:0001_nasa_pds_1:all:user:img_surface:geometry_projection::external_reference::1.0 rdf:type rdf:Property;
  rdfs:label "External_Reference";
  rdfs:domain pds4:urn:nasa:pds:0001_nasa_pds_1:all:user:img_surface:geometry_projection::1.0;
  rdfs:range pds4:urn:nasa:pds:0001_nasa_pds_1:pds:product_components:pds:external_reference::1.0.
 
pds4:urn:nasa:pds:0001_nasa_pds_1:all:user:img_surface:placement_target_instrument::internal_reference::1.0 rdf:type rdf:Property;
  rdfs:label "Internal_Reference";
  rdfs:domain pds4:urn:nasa:pds:0001_nasa_pds_1:all:user:img_surface:placement_target_instrument::1.0;
  rdfs:range pds4:urn:nasa:pds:0001_nasa_pds_1:pds:product_components:pds:internal_reference::1.0.
 
pds4:urn:nasa:pds:0001_nasa_pds_1:all:user:img_surface:reach_instruments::reach_instrument::1.0 rdf:type rdf:Property;
  rdfs:label "Reach_Instrument";
  rdfs:domain pds4:urn:nasa:pds:0001_nasa_pds_1:all:user:img_surface:reach_instruments::1.0;
  rdfs:range pds4:urn:nasa:pds:0001_nasa_pds_1:all:user:img_surface:reach_instrument::1.0.
 
pds4:urn:nasa:pds:0001_nasa_pds_1:all:user:img_surface:reachability::reach_instruments::1.0 rdf:type rdf:Property;
  rdfs:label "Reach_Instruments";
  rdfs:domain pds4:urn:nasa:pds:0001_nasa_pds_1:all:user:img_surface:reachability::1.0;
  rdfs:range pds4:urn:nasa:pds:0001_nasa_pds_1:all:user:img_surface:reach_instruments::1.0.
 
pds4:urn:nasa:pds:0001_nasa_pds_1:all:user:img_surface:reachability::configurations::1.0 rdf:type rdf:Property;
  rdfs:label "Configurations";
  rdfs:domain pds4:urn:nasa:pds:0001_nasa_pds_1:all:user:img_surface:reachability::1.0;
  rdfs:range pds4:urn:nasa:pds:0001_nasa_pds_1:all:user:img_surface:configurations::1.0.
 
pds4:urn:nasa:pds:0001_nasa_pds_1:all:user:img_surface:stereo_product_parameters::internal_reference::1.0 rdf:type rdf:Property;
  rdfs:label "Internal_Reference";
  rdfs:domain pds4:urn:nasa:pds:0001_nasa_pds_1:all:user:img_surface:stereo_product_parameters::1.0;
  rdfs:range pds4:urn:nasa:pds:0001_nasa_pds_1:pds:product_components:pds:internal_reference::1.0.
 
pds4:urn:nasa:pds:0001_nasa_pds_1:all:user:img_surface:stereo_product_parameters::external_reference::1.0 rdf:type rdf:Property;
  rdfs:label "External_Reference";
  rdfs:domain pds4:urn:nasa:pds:0001_nasa_pds_1:all:user:img_surface:stereo_product_parameters::1.0;
  rdfs:range pds4:urn:nasa:pds:0001_nasa_pds_1:pds:product_components:pds:external_reference::1.0.
 
pds4:urn:nasa:pds:0001_nasa_pds_1:all:user:img_surface:surface_imaging::image_identifiers::1.0 rdf:type rdf:Property;
  rdfs:label "Image_Identifiers";
  rdfs:domain pds4:urn:nasa:pds:0001_nasa_pds_1:all:user:img_surface:surface_imaging::1.0;
  rdfs:range pds4:urn:nasa:pds:0001_nasa_pds_1:all:user:img_surface:image_identifiers::1.0.
 
pds4:urn:nasa:pds:0001_nasa_pds_1:all:user:img_surface:surface_imaging::instrument_information::1.0 rdf:type rdf:Property;
  rdfs:label "Instrument_Information";
  rdfs:domain pds4:urn:nasa:pds:0001_nasa_pds_1:all:user:img_surface:surface_imaging::1.0;
  rdfs:range pds4:urn:nasa:pds:0001_nasa_pds_1:all:user:img_surface:instrument_information::1.0.
 
pds4:urn:nasa:pds:0001_nasa_pds_1:all:user:img_surface:surface_imaging::derived_product_parameters::1.0 rdf:type rdf:Property;
  rdfs:label "Derived_Product_Parameters";
  rdfs:domain pds4:urn:nasa:pds:0001_nasa_pds_1:all:user:img_surface:surface_imaging::1.0;
  rdfs:range pds4:urn:nasa:pds:0001_nasa_pds_1:all:user:img_surface:derived_product_parameters::1.0.
 
pds4:urn:nasa:pds:0001_nasa_pds_1:all:user:img_surface:surface_imaging::error_model::1.0 rdf:type rdf:Property;
  rdfs:label "Error_Model";
  rdfs:domain pds4:urn:nasa:pds:0001_nasa_pds_1:all:user:img_surface:surface_imaging::1.0;
  rdfs:range pds4:urn:nasa:pds:0001_nasa_pds_1:all:user:img_surface:error_model::1.0.
 
pds4:urn:nasa:pds:0001_nasa_pds_1:all:user:img_surface:surface_imaging::geometry_projection::1.0 rdf:type rdf:Property;
  rdfs:label "Geometry_Projection";
  rdfs:domain pds4:urn:nasa:pds:0001_nasa_pds_1:all:user:img_surface:surface_imaging::1.0;
  rdfs:range pds4:urn:nasa:pds:0001_nasa_pds_1:all:user:img_surface:geometry_projection::1.0.
 
pds4:urn:nasa:pds:0001_nasa_pds_1:all:user:img_surface:surface_imaging::reachability::1.0 rdf:type rdf:Property;
  rdfs:label "Reachability";
  rdfs:domain pds4:urn:nasa:pds:0001_nasa_pds_1:all:user:img_surface:surface_imaging::1.0;
  rdfs:range pds4:urn:nasa:pds:0001_nasa_pds_1:all:user:img_surface:reachability::1.0.
 
pds4:urn:nasa:pds:0001_nasa_pds_1:all:user:img_surface:surface_imaging::stereo_product_parameters::1.0 rdf:type rdf:Property;
  rdfs:label "Stereo_Product_Parameters";
  rdfs:domain pds4:urn:nasa:pds:0001_nasa_pds_1:all:user:img_surface:surface_imaging::1.0;
  rdfs:range pds4:urn:nasa:pds:0001_nasa_pds_1:all:user:img_surface:stereo_product_parameters::1.0.
 
pds4:urn:nasa:pds:0001_nasa_pds_1:all:user:img_surface:surface_imaging::coordinate_space_reference::1.0 rdf:type rdf:Property;
  rdfs:label "Coordinate_Space_Reference";
  rdfs:domain pds4:urn:nasa:pds:0001_nasa_pds_1:all:user:img_surface:surface_imaging::1.0;
  rdfs:range pds4:urn:nasa:pds:0001_nasa_pds_1:geom:coordinate_space_identification:geom:coordinate_space_reference::1.0.
 
pds4:urn:nasa:pds:0001_nasa_pds_1:all:user:img_surface:surface_imaging::error_pixel::1.0 rdf:type rdf:Property;
  rdfs:label "Error_Pixel";
  rdfs:domain pds4:urn:nasa:pds:0001_nasa_pds_1:all:user:img_surface:surface_imaging::1.0;
  rdfs:range pds4:urn:nasa:pds:0001_nasa_pds_1:all:user:img_surface:error_pixel::1.0.
 
pds4:urn:nasa:pds:0001_nasa_pds_1:all:user:img_surface:surface_imaging::commanded_parameters::1.0 rdf:type rdf:Property;
  rdfs:label "Commanded_Parameters";
  rdfs:domain pds4:urn:nasa:pds:0001_nasa_pds_1:all:user:img_surface:surface_imaging::1.0;
  rdfs:range pds4:urn:nasa:pds:0001_nasa_pds_1:all:user:img_surface:commanded_parameters::1.0.
 
pds4:urn:nasa:pds:0001_nasa_pds_1:all:user:msn:mission_information::orbital_mission::1.0 rdf:type rdf:Property;
  rdfs:label "Orbital_Mission";
  rdfs:domain pds4:urn:nasa:pds:0001_nasa_pds_1:all:user:msn:mission_information::1.0;
  rdfs:range pds4:urn:nasa:pds:0001_nasa_pds_1:all:user:msn:orbital_mission::1.0.
 
pds4:urn:nasa:pds:0001_nasa_pds_1:all:user:msn:mission_information::surface_mission::1.0 rdf:type rdf:Property;
  rdfs:label "Surface_Mission";
  rdfs:domain pds4:urn:nasa:pds:0001_nasa_pds_1:all:user:msn:mission_information::1.0;
  rdfs:range pds4:urn:nasa:pds:0001_nasa_pds_1:all:user:msn:surface_mission::1.0.
 
pds4:urn:nasa:pds:0001_nasa_pds_1:all:user:msn:mission_information::observation_context::1.0 rdf:type rdf:Property;
  rdfs:label "Observation_Context";
  rdfs:domain pds4:urn:nasa:pds:0001_nasa_pds_1:all:user:msn:mission_information::1.0;
  rdfs:range pds4:urn:nasa:pds:0001_nasa_pds_1:all:user:msn:observation_context::1.0.
 
pds4:urn:nasa:pds:0001_nasa_pds_1:all:user:msn_surface:surface_mission_information::command_execution::1.0 rdf:type rdf:Property;
  rdfs:label "Command_Execution";
  rdfs:domain pds4:urn:nasa:pds:0001_nasa_pds_1:all:user:msn_surface:surface_mission_information::1.0;
  rdfs:range pds4:urn:nasa:pds:0001_nasa_pds_1:all:user:msn_surface:command_execution::1.0.
 
pds4:urn:nasa:pds:0001_nasa_pds_1:all:user:msn_surface:surface_mission_information::telemetry::1.0 rdf:type rdf:Property;
  rdfs:label "Telemetry";
  rdfs:domain pds4:urn:nasa:pds:0001_nasa_pds_1:all:user:msn_surface:surface_mission_information::1.0;
  rdfs:range pds4:urn:nasa:pds:0001_nasa_pds_1:all:user:msn_surface:telemetry::1.0.
 
pds4:urn:nasa:pds:0001_nasa_pds_1:all:user:msn_surface:surface_mission_information::observational_intent::1.0 rdf:type rdf:Property;
  rdfs:label "Observational_Intent";
  rdfs:domain pds4:urn:nasa:pds:0001_nasa_pds_1:all:user:msn_surface:surface_mission_information::1.0;
  rdfs:range pds4:urn:nasa:pds:0001_nasa_pds_1:all:user:msn_surface:observational_intent::1.0.
 
pds4:urn:nasa:pds:0001_nasa_pds_1:all:user:msn_surface:surface_mission_information::commanded_parameters::1.0 rdf:type rdf:Property;
  rdfs:label "Commanded_Parameters";
  rdfs:domain pds4:urn:nasa:pds:0001_nasa_pds_1:all:user:msn_surface:surface_mission_information::1.0;
  rdfs:range pds4:urn:nasa:pds:0001_nasa_pds_1:all:user:msn_surface:commanded_parameters::1.0.
 
pds4:urn:nasa:pds:0001_nasa_pds_1:all:user:msss_cam_mh:msss_camera_mini_header::detector::1.0 rdf:type rdf:Property;
  rdfs:label "Detector";
  rdfs:domain pds4:urn:nasa:pds:0001_nasa_pds_1:all:user:msss_cam_mh:msss_camera_mini_header::1.0;
  rdfs:range pds4:urn:nasa:pds:0001_nasa_pds_1:all:user:img:detector::1.0.
 
pds4:urn:nasa:pds:0001_nasa_pds_1:all:user:msss_cam_mh:msss_camera_mini_header::exposure::1.0 rdf:type rdf:Property;
  rdfs:label "Exposure";
  rdfs:domain pds4:urn:nasa:pds:0001_nasa_pds_1:all:user:msss_cam_mh:msss_camera_mini_header::1.0;
  rdfs:range pds4:urn:nasa:pds:0001_nasa_pds_1:all:user:img:exposure::1.0.
 
pds4:urn:nasa:pds:0001_nasa_pds_1:all:user:msss_cam_mh:msss_camera_mini_header::focus::1.0 rdf:type rdf:Property;
  rdfs:label "Focus";
  rdfs:domain pds4:urn:nasa:pds:0001_nasa_pds_1:all:user:msss_cam_mh:msss_camera_mini_header::1.0;
  rdfs:range pds4:urn:nasa:pds:0001_nasa_pds_1:all:user:img:focus::1.0.
 
pds4:urn:nasa:pds:0001_nasa_pds_1:all:user:msss_cam_mh:msss_camera_mini_header::onboard_compression::1.0 rdf:type rdf:Property;
  rdfs:label "Onboard_Compression";
  rdfs:domain pds4:urn:nasa:pds:0001_nasa_pds_1:all:user:msss_cam_mh:msss_camera_mini_header::1.0;
  rdfs:range pds4:urn:nasa:pds:0001_nasa_pds_1:all:user:img:onboard_compression::1.0.
 
pds4:urn:nasa:pds:0001_nasa_pds_1:all:user:msss_cam_mh:msss_camera_mini_header::optical_filter::1.0 rdf:type rdf:Property;
  rdfs:label "Optical_Filter";
  rdfs:domain pds4:urn:nasa:pds:0001_nasa_pds_1:all:user:msss_cam_mh:msss_camera_mini_header::1.0;
  rdfs:range pds4:urn:nasa:pds:0001_nasa_pds_1:all:user:img:optical_filter::1.0.
 
pds4:urn:nasa:pds:0001_nasa_pds_1:all:user:msss_cam_mh:msss_camera_mini_header::sampling::1.0 rdf:type rdf:Property;
  rdfs:label "Sampling";
  rdfs:domain pds4:urn:nasa:pds:0001_nasa_pds_1:all:user:msss_cam_mh:msss_camera_mini_header::1.0;
  rdfs:range pds4:urn:nasa:pds:0001_nasa_pds_1:all:user:img:sampling::1.0.
 
pds4:urn:nasa:pds:0001_nasa_pds_1:all:user:msss_cam_mh:msss_camera_mini_header::subframe::1.0 rdf:type rdf:Property;
  rdfs:label "Subframe";
  rdfs:domain pds4:urn:nasa:pds:0001_nasa_pds_1:all:user:msss_cam_mh:msss_camera_mini_header::1.0;
  rdfs:range pds4:urn:nasa:pds:0001_nasa_pds_1:all:user:img:subframe::1.0.
 
pds4:urn:nasa:pds:0001_nasa_pds_1:all:user:msss_cam_mh:msss_camera_mini_header::instrument_state::1.0 rdf:type rdf:Property;
  rdfs:label "Instrument_State";
  rdfs:domain pds4:urn:nasa:pds:0001_nasa_pds_1:all:user:msss_cam_mh:msss_camera_mini_header::1.0;
  rdfs:range pds4:urn:nasa:pds:0001_nasa_pds_1:all:user:img:instrument_state::1.0.
 
pds4:urn:nasa:pds:0001_nasa_pds_1:all:user:nucspec:applicable_records::first_last::1.0 rdf:type rdf:Property;
  rdfs:label "First_Last";
  rdfs:domain pds4:urn:nasa:pds:0001_nasa_pds_1:all:user:nucspec:applicable_records::1.0;
  rdfs:range pds4:urn:nasa:pds:0001_nasa_pds_1:all:user:nucspec:first_last::1.0.
 
pds4:urn:nasa:pds:0001_nasa_pds_1:all:user:nucspec:applicable_records::first_count::1.0 rdf:type rdf:Property;
  rdfs:label "First_Count";
  rdfs:domain pds4:urn:nasa:pds:0001_nasa_pds_1:all:user:nucspec:applicable_records::1.0;
  rdfs:range pds4:urn:nasa:pds:0001_nasa_pds_1:all:user:nucspec:first_count::1.0.
 
pds4:urn:nasa:pds:0001_nasa_pds_1:all:user:nucspec:calibration_reference::internal_reference::1.0 rdf:type rdf:Property;
  rdfs:label "Internal_Reference";
  rdfs:domain pds4:urn:nasa:pds:0001_nasa_pds_1:all:user:nucspec:calibration_reference::1.0;
  rdfs:range pds4:urn:nasa:pds:0001_nasa_pds_1:pds:product_components:pds:internal_reference::1.0.
 
pds4:urn:nasa:pds:0001_nasa_pds_1:all:user:nucspec:detectors::detector::1.0 rdf:type rdf:Property;
  rdfs:label "Detector";
  rdfs:domain pds4:urn:nasa:pds:0001_nasa_pds_1:all:user:nucspec:detectors::1.0;
  rdfs:range pds4:urn:nasa:pds:0001_nasa_pds_1:all:user:nucspec:detector::1.0.
 
pds4:urn:nasa:pds:0001_nasa_pds_1:all:user:nucspec:energy_calibration::polynomial::1.0 rdf:type rdf:Property;
  rdfs:label "Polynomial";
  rdfs:domain pds4:urn:nasa:pds:0001_nasa_pds_1:all:user:nucspec:energy_calibration::1.0;
  rdfs:range pds4:urn:nasa:pds:0001_nasa_pds_1:all:user:nucspec:polynomial::1.0.
 
pds4:urn:nasa:pds:0001_nasa_pds_1:all:user:nucspec:energy_calibration::calibration_reference::1.0 rdf:type rdf:Property;
  rdfs:label "Calibration_Reference";
  rdfs:domain pds4:urn:nasa:pds:0001_nasa_pds_1:all:user:nucspec:energy_calibration::1.0;
  rdfs:range pds4:urn:nasa:pds:0001_nasa_pds_1:all:user:nucspec:calibration_reference::1.0.
 
pds4:urn:nasa:pds:0001_nasa_pds_1:all:user:nucspec:instrument_settings::state_table::1.0 rdf:type rdf:Property;
  rdfs:label "State_Table";
  rdfs:domain pds4:urn:nasa:pds:0001_nasa_pds_1:all:user:nucspec:instrument_settings::1.0;
  rdfs:range pds4:urn:nasa:pds:0001_nasa_pds_1:all:user:nucspec:state_table::1.0.
 
pds4:urn:nasa:pds:0001_nasa_pds_1:all:user:nucspec:nucspec_observation_properties::energy_calibration::1.0 rdf:type rdf:Property;
  rdfs:label "Energy_Calibration";
  rdfs:domain pds4:urn:nasa:pds:0001_nasa_pds_1:all:user:nucspec:nucspec_observation_properties::1.0;
  rdfs:range pds4:urn:nasa:pds:0001_nasa_pds_1:all:user:nucspec:energy_calibration::1.0.
 
pds4:urn:nasa:pds:0001_nasa_pds_1:all:user:nucspec:nucspec_observation_properties::instrument_settings::1.0 rdf:type rdf:Property;
  rdfs:label "Instrument_Settings";
  rdfs:domain pds4:urn:nasa:pds:0001_nasa_pds_1:all:user:nucspec:nucspec_observation_properties::1.0;
  rdfs:range pds4:urn:nasa:pds:0001_nasa_pds_1:all:user:nucspec:instrument_settings::1.0.
 
pds4:urn:nasa:pds:0001_nasa_pds_1:all:user:nucspec:nucspec_observation_properties::detectors::1.0 rdf:type rdf:Property;
  rdfs:label "Detectors";
  rdfs:domain pds4:urn:nasa:pds:0001_nasa_pds_1:all:user:nucspec:nucspec_observation_properties::1.0;
  rdfs:range pds4:urn:nasa:pds:0001_nasa_pds_1:all:user:nucspec:detectors::1.0.
 
pds4:urn:nasa:pds:0001_nasa_pds_1:all:user:nucspec:nucspec_observation_properties::observing_conditions::1.0 rdf:type rdf:Property;
  rdfs:label "Observing_Conditions";
  rdfs:domain pds4:urn:nasa:pds:0001_nasa_pds_1:all:user:nucspec:nucspec_observation_properties::1.0;
  rdfs:range pds4:urn:nasa:pds:0001_nasa_pds_1:all:user:nucspec:observing_conditions::1.0.
 
pds4:urn:nasa:pds:0001_nasa_pds_1:all:user:nucspec:observing_condition::time_range_utc::1.0 rdf:type rdf:Property;
  rdfs:label "Time_Range_UTC";
  rdfs:domain pds4:urn:nasa:pds:0001_nasa_pds_1:all:user:nucspec:observing_condition::1.0;
  rdfs:range pds4:urn:nasa:pds:0001_nasa_pds_1:all:user:nucspec:time_range_utc::1.0.
 
pds4:urn:nasa:pds:0001_nasa_pds_1:all:user:nucspec:observing_condition::time_range_et::1.0 rdf:type rdf:Property;
  rdfs:label "Time_Range_ET";
  rdfs:domain pds4:urn:nasa:pds:0001_nasa_pds_1:all:user:nucspec:observing_condition::1.0;
  rdfs:range pds4:urn:nasa:pds:0001_nasa_pds_1:all:user:nucspec:time_range_et::1.0.
 
pds4:urn:nasa:pds:0001_nasa_pds_1:all:user:nucspec:observing_condition::time_range_sclk::1.0 rdf:type rdf:Property;
  rdfs:label "Time_Range_SCLK";
  rdfs:domain pds4:urn:nasa:pds:0001_nasa_pds_1:all:user:nucspec:observing_condition::1.0;
  rdfs:range pds4:urn:nasa:pds:0001_nasa_pds_1:all:user:nucspec:time_range_sclk::1.0.
 
pds4:urn:nasa:pds:0001_nasa_pds_1:all:user:nucspec:observing_conditions::observing_condition::1.0 rdf:type rdf:Property;
  rdfs:label "Observing_Condition";
  rdfs:domain pds4:urn:nasa:pds:0001_nasa_pds_1:all:user:nucspec:observing_conditions::1.0;
  rdfs:range pds4:urn:nasa:pds:0001_nasa_pds_1:all:user:nucspec:observing_condition::1.0.
 
pds4:urn:nasa:pds:0001_nasa_pds_1:all:user:nucspec:polynomial::polynomial_term::1.0 rdf:type rdf:Property;
  rdfs:label "Polynomial_Term";
  rdfs:domain pds4:urn:nasa:pds:0001_nasa_pds_1:all:user:nucspec:polynomial::1.0;
  rdfs:range pds4:urn:nasa:pds:0001_nasa_pds_1:all:user:nucspec:polynomial_term::1.0.
 
pds4:urn:nasa:pds:0001_nasa_pds_1:all:user:nucspec:state_table::internal_reference::1.0 rdf:type rdf:Property;
  rdfs:label "Internal_Reference";
  rdfs:domain pds4:urn:nasa:pds:0001_nasa_pds_1:all:user:nucspec:state_table::1.0;
  rdfs:range pds4:urn:nasa:pds:0001_nasa_pds_1:pds:product_components:pds:internal_reference::1.0.
 
pds4:urn:nasa:pds:0001_nasa_pds_1:all:user:nucspec:state_table::local_internal_reference::1.0 rdf:type rdf:Property;
  rdfs:label "Local_Internal_Reference";
  rdfs:domain pds4:urn:nasa:pds:0001_nasa_pds_1:all:user:nucspec:state_table::1.0;
  rdfs:range pds4:urn:nasa:pds:0001_nasa_pds_1:pds:product_components:pds:local_internal_reference::1.0.
 
pds4:urn:nasa:pds:0001_nasa_pds_1:all:user:nucspec:state_table::state_table_entry::1.0 rdf:type rdf:Property;
  rdfs:label "State_Table_Entry";
  rdfs:domain pds4:urn:nasa:pds:0001_nasa_pds_1:all:user:nucspec:state_table::1.0;
  rdfs:range pds4:urn:nasa:pds:0001_nasa_pds_1:all:user:nucspec:state_table_entry::1.0.
 
pds4:urn:nasa:pds:0001_nasa_pds_1:all:user:nucspec:state_table_entry::applicable_records::1.0 rdf:type rdf:Property;
  rdfs:label "Applicable_Records";
  rdfs:domain pds4:urn:nasa:pds:0001_nasa_pds_1:all:user:nucspec:state_table_entry::1.0;
  rdfs:range pds4:urn:nasa:pds:0001_nasa_pds_1:all:user:nucspec:applicable_records::1.0.
 
pds4:urn:nasa:pds:0001_nasa_pds_1:all:user:nucspec:state_table_entry::state_time::1.0 rdf:type rdf:Property;
  rdfs:label "State_Time";
  rdfs:domain pds4:urn:nasa:pds:0001_nasa_pds_1:all:user:nucspec:state_table_entry::1.0;
  rdfs:range pds4:urn:nasa:pds:0001_nasa_pds_1:all:user:nucspec:state_time::1.0.
 
pds4:urn:nasa:pds:0001_nasa_pds_1:all:user:nucspec:state_time::time_range_et::1.0 rdf:type rdf:Property;
  rdfs:label "Time_Range_ET";
  rdfs:domain pds4:urn:nasa:pds:0001_nasa_pds_1:all:user:nucspec:state_time::1.0;
  rdfs:range pds4:urn:nasa:pds:0001_nasa_pds_1:all:user:nucspec:time_range_et::1.0.
 
pds4:urn:nasa:pds:0001_nasa_pds_1:all:user:nucspec:state_time::time_range_sclk::1.0 rdf:type rdf:Property;
  rdfs:label "Time_Range_SCLK";
  rdfs:domain pds4:urn:nasa:pds:0001_nasa_pds_1:all:user:nucspec:state_time::1.0;
  rdfs:range pds4:urn:nasa:pds:0001_nasa_pds_1:all:user:nucspec:time_range_sclk::1.0.
 
pds4:urn:nasa:pds:0001_nasa_pds_1:all:user:nucspec:state_time::time_range_utc::1.0 rdf:type rdf:Property;
  rdfs:label "Time_Range_UTC";
  rdfs:domain pds4:urn:nasa:pds:0001_nasa_pds_1:all:user:nucspec:state_time::1.0;
  rdfs:range pds4:urn:nasa:pds:0001_nasa_pds_1:all:user:nucspec:time_range_utc::1.0.
 
pds4:urn:nasa:pds:0001_nasa_pds_1:pds:tndo_context:pds:agency::data_object::1.0 rdf:type rdf:Property;
  rdfs:label "data_object";
  rdfs:domain pds4:urn:nasa:pds:0001_nasa_pds_1:pds:tndo_context:pds:agency::1.0;
  rdfs:range pds4:urn:nasa:pds:0001_nasa_pds_1:pds:tndo_context:pds:other::1.0.
 
pds4:urn:nasa:pds:0001_nasa_pds_1:pds:product_components:pds:alias_list::alias::1.0 rdf:type rdf:Property;
  rdfs:label "alias";
  rdfs:domain pds4:urn:nasa:pds:0001_nasa_pds_1:pds:product_components:pds:alias_list::1.0;
  rdfs:range pds4:urn:nasa:pds:0001_nasa_pds_1:pds:product_components:pds:alias::1.0.
 
pds4:urn:nasa:pds:0001_nasa_pds_1:pds:byte_stream:pds:array::associated_statistics::1.0 rdf:type rdf:Property;
  rdfs:label "associated_Statistics";
  rdfs:domain pds4:urn:nasa:pds:0001_nasa_pds_1:pds:byte_stream:pds:array::1.0;
  rdfs:range pds4:urn:nasa:pds:0001_nasa_pds_1:pds:tndo_supplemental:pds:object_statistics::1.0.
 
pds4:urn:nasa:pds:0001_nasa_pds_1:pds:byte_stream:pds:array::data_object::1.0 rdf:type rdf:Property;
  rdfs:label "data_object";
  rdfs:domain pds4:urn:nasa:pds:0001_nasa_pds_1:pds:byte_stream:pds:array::1.0;
  rdfs:range pds4:urn:nasa:pds:0001_nasa_pds_1:pds:tndo_context:pds:other::1.0.
 
pds4:urn:nasa:pds:0001_nasa_pds_1:pds:byte_stream:pds:array::local_internal_reference::1.0 rdf:type rdf:Property;
  rdfs:label "local_internal_reference";
  rdfs:domain pds4:urn:nasa:pds:0001_nasa_pds_1:pds:byte_stream:pds:array::1.0;
  rdfs:range pds4:urn:nasa:pds:0001_nasa_pds_1:pds:product_components:pds:local_internal_reference::1.0.
 
pds4:urn:nasa:pds:0001_nasa_pds_1:pds:byte_stream:pds:array::has_element_array::1.0 rdf:type rdf:Property;
  rdfs:label "has_Element_Array";
  rdfs:domain pds4:urn:nasa:pds:0001_nasa_pds_1:pds:byte_stream:pds:array::1.0;
  rdfs:range pds4:urn:nasa:pds:0001_nasa_pds_1:pds:tagged_digital_child:pds:element_array::1.0.
 
pds4:urn:nasa:pds:0001_nasa_pds_1:pds:byte_stream:pds:array::associated_special_constants::1.0 rdf:type rdf:Property;
  rdfs:label "associated_Special_Constants";
  rdfs:domain pds4:urn:nasa:pds:0001_nasa_pds_1:pds:byte_stream:pds:array::1.0;
  rdfs:range pds4:urn:nasa:pds:0001_nasa_pds_1:pds:tagged_digital_child:pds:special_constants::1.0.
 
pds4:urn:nasa:pds:0001_nasa_pds_1:pds:byte_stream:pds:array::has_axis_array::1.0 rdf:type rdf:Property;
  rdfs:label "has_Axis_Array";
  rdfs:domain pds4:urn:nasa:pds:0001_nasa_pds_1:pds:byte_stream:pds:array::1.0;
  rdfs:range pds4:urn:nasa:pds:0001_nasa_pds_1:pds:tagged_digital_child:pds:axis_array::1.0.
 
pds4:urn:nasa:pds:0001_nasa_pds_1:pds:array:pds:array_1d::has_axis_array::1.0 rdf:type rdf:Property;
  rdfs:label "has_Axis_Array";
  rdfs:domain pds4:urn:nasa:pds:0001_nasa_pds_1:pds:array:pds:array_1d::1.0;
  rdfs:range pds4:urn:nasa:pds:0001_nasa_pds_1:pds:tagged_digital_child:pds:axis_array::1.0.
 
pds4:urn:nasa:pds:0001_nasa_pds_1:pds:array:pds:array_2d::has_axis_array::1.0 rdf:type rdf:Property;
  rdfs:label "has_Axis_Array";
  rdfs:domain pds4:urn:nasa:pds:0001_nasa_pds_1:pds:array:pds:array_2d::1.0;
  rdfs:range pds4:urn:nasa:pds:0001_nasa_pds_1:pds:tagged_digital_child:pds:axis_array::1.0.
 
pds4:urn:nasa:pds:0001_nasa_pds_1:pds:array_2d:pds:array_2d_image::has_display_2d_image::1.0 rdf:type rdf:Property;
  rdfs:label "has_Display_2d_Image";
  rdfs:domain pds4:urn:nasa:pds:0001_nasa_pds_1:pds:array_2d:pds:array_2d_image::1.0;
  rdfs:range pds4:urn:nasa:pds:0001_nasa_pds_1:pds:tndo_supplemental:pds:display_2d_image::1.0.
 
pds4:urn:nasa:pds:0001_nasa_pds_1:pds:array_2d:pds:array_2d_map::has_display_2d_image::1.0 rdf:type rdf:Property;
  rdfs:label "has_Display_2d_Image";
  rdfs:domain pds4:urn:nasa:pds:0001_nasa_pds_1:pds:array_2d:pds:array_2d_map::1.0;
  rdfs:range pds4:urn:nasa:pds:0001_nasa_pds_1:pds:tndo_supplemental:pds:display_2d_image::1.0.
 
pds4:urn:nasa:pds:0001_nasa_pds_1:pds:array_2d:pds:array_2d_spectrum::has_display_2d_image::1.0 rdf:type rdf:Property;
  rdfs:label "has_Display_2d_Image";
  rdfs:domain pds4:urn:nasa:pds:0001_nasa_pds_1:pds:array_2d:pds:array_2d_spectrum::1.0;
  rdfs:range pds4:urn:nasa:pds:0001_nasa_pds_1:pds:tndo_supplemental:pds:display_2d_image::1.0.
 
pds4:urn:nasa:pds:0001_nasa_pds_1:pds:array:pds:array_3d::has_axis_array::1.0 rdf:type rdf:Property;
  rdfs:label "has_Axis_Array";
  rdfs:domain pds4:urn:nasa:pds:0001_nasa_pds_1:pds:array:pds:array_3d::1.0;
  rdfs:range pds4:urn:nasa:pds:0001_nasa_pds_1:pds:tagged_digital_child:pds:axis_array::1.0.
 
pds4:urn:nasa:pds:0001_nasa_pds_1:pds:tagged_digital_child:pds:axis_array::has_band_bin_set::1.0 rdf:type rdf:Property;
  rdfs:label "has_Band_Bin_Set";
  rdfs:domain pds4:urn:nasa:pds:0001_nasa_pds_1:pds:tagged_digital_child:pds:axis_array::1.0;
  rdfs:range pds4:urn:nasa:pds:0001_nasa_pds_1:pds:tndo_supplemental:pds:band_bin_set::1.0.
 
pds4:urn:nasa:pds:0001_nasa_pds_1:pds:tndo_supplemental:pds:band_bin_set::has_band_bin::1.0 rdf:type rdf:Property;
  rdfs:label "has_band_bin";
  rdfs:domain pds4:urn:nasa:pds:0001_nasa_pds_1:pds:tndo_supplemental:pds:band_bin_set::1.0;
  rdfs:range pds4:urn:nasa:pds:0001_nasa_pds_1:pds:tndo_supplemental:pds:band_bin::1.0.
 
pds4:urn:nasa:pds:0001_nasa_pds_1:pds:tndo_supplemental:pds:bundle::data_object::1.0 rdf:type rdf:Property;
  rdfs:label "data_object";
  rdfs:domain pds4:urn:nasa:pds:0001_nasa_pds_1:pds:tndo_supplemental:pds:bundle::1.0;
  rdfs:range pds4:urn:nasa:pds:0001_nasa_pds_1:pds:tndo_context:pds:other::1.0.
 
pds4:urn:nasa:pds:0001_nasa_pds_1:pds:tagged_digital_object:pds:composite_structure::has_local_id_relation::1.0 rdf:type rdf:Property;
  rdfs:label "has_Local_ID_Relation";
  rdfs:domain pds4:urn:nasa:pds:0001_nasa_pds_1:pds:tagged_digital_object:pds:composite_structure::1.0;
  rdfs:range pds4:urn:nasa:pds:0001_nasa_pds_1:pds:tagged_digital_child:pds:local_id_relation::1.0.
 
pds4:urn:nasa:pds:0001_nasa_pds_1:pds:tagged_digital_object:pds:composite_structure::has_local_id_reference::1.0 rdf:type rdf:Property;
  rdfs:label "has_Local_ID_Reference";
  rdfs:domain pds4:urn:nasa:pds:0001_nasa_pds_1:pds:tagged_digital_object:pds:composite_structure::1.0;
  rdfs:range pds4:urn:nasa:pds:0001_nasa_pds_1:pds:tagged_digital_child:pds:local_id_reference::1.0.
 
pds4:urn:nasa:pds:0001_nasa_pds_1:pds:product_components:pds:context_area::has_investigation_area::1.0 rdf:type rdf:Property;
  rdfs:label "has_investigation_area";
  rdfs:domain pds4:urn:nasa:pds:0001_nasa_pds_1:pds:product_components:pds:context_area::1.0;
  rdfs:range pds4:urn:nasa:pds:0001_nasa_pds_1:pds:product_components:pds:investigation_area::1.0.
 
pds4:urn:nasa:pds:0001_nasa_pds_1:pds:product_components:pds:context_area::has_primary_result_description::1.0 rdf:type rdf:Property;
  rdfs:label "has_primary_result_description";
  rdfs:domain pds4:urn:nasa:pds:0001_nasa_pds_1:pds:product_components:pds:context_area::1.0;
  rdfs:range pds4:urn:nasa:pds:0001_nasa_pds_1:pds:product_components:pds:primary_result_summary::1.0.
 
pds4:urn:nasa:pds:0001_nasa_pds_1:pds:product_components:pds:context_area::has_time_coordinates::1.0 rdf:type rdf:Property;
  rdfs:label "has_time_coordinates";
  rdfs:domain pds4:urn:nasa:pds:0001_nasa_pds_1:pds:product_components:pds:context_area::1.0;
  rdfs:range pds4:urn:nasa:pds:0001_nasa_pds_1:pds:product_components:pds:time_coordinates::1.0.
 
pds4:urn:nasa:pds:0001_nasa_pds_1:pds:product_components:pds:context_area::has_observing_system::1.0 rdf:type rdf:Property;
  rdfs:label "has_observing_system";
  rdfs:domain pds4:urn:nasa:pds:0001_nasa_pds_1:pds:product_components:pds:context_area::1.0;
  rdfs:range pds4:urn:nasa:pds:0001_nasa_pds_1:pds:tndo_context:pds:observing_system::1.0.
 
pds4:urn:nasa:pds:0001_nasa_pds_1:pds:product_components:pds:context_area::has_mission_area::1.0 rdf:type rdf:Property;
  rdfs:label "has_mission_area";
  rdfs:domain pds4:urn:nasa:pds:0001_nasa_pds_1:pds:product_components:pds:context_area::1.0;
  rdfs:range pds4:urn:nasa:pds:0001_nasa_pds_1:pds:product_components:pds:mission_area::1.0.
 
pds4:urn:nasa:pds:0001_nasa_pds_1:pds:product_components:pds:context_area::has_target_identification::1.0 rdf:type rdf:Property;
  rdfs:label "has_target_identification";
  rdfs:domain pds4:urn:nasa:pds:0001_nasa_pds_1:pds:product_components:pds:context_area::1.0;
  rdfs:range pds4:urn:nasa:pds:0001_nasa_pds_1:pds:product_components:pds:target_identification::1.0.
 
pds4:urn:nasa:pds:0001_nasa_pds_1:pds:product_components:pds:context_area::has_discipline_area::1.0 rdf:type rdf:Property;
  rdfs:label "has_discipline_area";
  rdfs:domain pds4:urn:nasa:pds:0001_nasa_pds_1:pds:product_components:pds:context_area::1.0;
  rdfs:range pds4:urn:nasa:pds:0001_nasa_pds_1:pds:product_components:pds:discipline_area::1.0.
 
pds4:urn:nasa:pds:0001_nasa_pds_1:pds:tagged_nondigital_child:pds:dd_associate_external_class::dd_context_value_list::1.0 rdf:type rdf:Property;
  rdfs:label "dd_Context_Value_List";
  rdfs:domain pds4:urn:nasa:pds:0001_nasa_pds_1:pds:tagged_nondigital_child:pds:dd_associate_external_class::1.0;
  rdfs:range pds4:urn:nasa:pds:0001_nasa_pds_1:pds:tagged_nondigital_child:pds:dd_context_value_list::1.0.
 
pds4:urn:nasa:pds:0001_nasa_pds_1:pds:tagged_nondigital_child:pds:dd_association::dd_attribute_reference::1.0 rdf:type rdf:Property;
  rdfs:label "dd_attribute_reference";
  rdfs:domain pds4:urn:nasa:pds:0001_nasa_pds_1:pds:tagged_nondigital_child:pds:dd_association::1.0;
  rdfs:range pds4:urn:nasa:pds:0001_nasa_pds_1:pds:tagged_nondigital_child:pds:dd_attribute_reference::1.0.
 
pds4:urn:nasa:pds:0001_nasa_pds_1:pds:tagged_nondigital_child:pds:dd_association::dd_class_reference::1.0 rdf:type rdf:Property;
  rdfs:label "dd_class_reference";
  rdfs:domain pds4:urn:nasa:pds:0001_nasa_pds_1:pds:tagged_nondigital_child:pds:dd_association::1.0;
  rdfs:range pds4:urn:nasa:pds:0001_nasa_pds_1:pds:tagged_nondigital_child:pds:dd_class_reference::1.0.
 
pds4:urn:nasa:pds:0001_nasa_pds_1:pds:tndo_supplemental:pds:dd_attribute::value_domain_entry::1.0 rdf:type rdf:Property;
  rdfs:label "value_domain_entry";
  rdfs:domain pds4:urn:nasa:pds:0001_nasa_pds_1:pds:tndo_supplemental:pds:dd_attribute::1.0;
  rdfs:range pds4:urn:nasa:pds:0001_nasa_pds_1:pds:tagged_nondigital_child:pds:dd_value_domain::1.0.
 
pds4:urn:nasa:pds:0001_nasa_pds_1:pds:tndo_supplemental:pds:dd_attribute::terminological_entry::1.0 rdf:type rdf:Property;
  rdfs:label "terminological_entry";
  rdfs:domain pds4:urn:nasa:pds:0001_nasa_pds_1:pds:tndo_supplemental:pds:dd_attribute::1.0;
  rdfs:range pds4:urn:nasa:pds:0001_nasa_pds_1:pds:tagged_nondigital_child:pds:terminological_entry::1.0.
 
pds4:urn:nasa:pds:0001_nasa_pds_1:pds:tndo_supplemental:pds:dd_attribute::internal_reference::1.0 rdf:type rdf:Property;
  rdfs:label "internal_reference";
  rdfs:domain pds4:urn:nasa:pds:0001_nasa_pds_1:pds:tndo_supplemental:pds:dd_attribute::1.0;
  rdfs:range pds4:urn:nasa:pds:0001_nasa_pds_1:pds:product_components:pds:internal_reference::1.0.
 
pds4:urn:nasa:pds:0001_nasa_pds_1:pds:tndo_supplemental:pds:dd_attribute::data_object::1.0 rdf:type rdf:Property;
  rdfs:label "data_object";
  rdfs:domain pds4:urn:nasa:pds:0001_nasa_pds_1:pds:tndo_supplemental:pds:dd_attribute::1.0;
  rdfs:range pds4:urn:nasa:pds:0001_nasa_pds_1:pds:tndo_context:pds:other::1.0.
 
pds4:urn:nasa:pds:0001_nasa_pds_1:pds:tndo_supplemental:pds:dd_attribute_full::value_domain_entry::1.0 rdf:type rdf:Property;
  rdfs:label "value_domain_entry";
  rdfs:domain pds4:urn:nasa:pds:0001_nasa_pds_1:pds:tndo_supplemental:pds:dd_attribute_full::1.0;
  rdfs:range pds4:urn:nasa:pds:0001_nasa_pds_1:pds:tagged_nondigital_child:pds:dd_value_domain_full::1.0.
 
pds4:urn:nasa:pds:0001_nasa_pds_1:pds:tndo_supplemental:pds:dd_attribute_full::terminological_entry::1.0 rdf:type rdf:Property;
  rdfs:label "terminological_entry";
  rdfs:domain pds4:urn:nasa:pds:0001_nasa_pds_1:pds:tndo_supplemental:pds:dd_attribute_full::1.0;
  rdfs:range pds4:urn:nasa:pds:0001_nasa_pds_1:pds:tagged_nondigital_child:pds:terminological_entry::1.0.
 
pds4:urn:nasa:pds:0001_nasa_pds_1:pds:tndo_supplemental:pds:dd_attribute_full::data_object::1.0 rdf:type rdf:Property;
  rdfs:label "data_object";
  rdfs:domain pds4:urn:nasa:pds:0001_nasa_pds_1:pds:tndo_supplemental:pds:dd_attribute_full::1.0;
  rdfs:range pds4:urn:nasa:pds:0001_nasa_pds_1:pds:tndo_context:pds:other::1.0.
 
pds4:urn:nasa:pds:0001_nasa_pds_1:pds:tndo_supplemental:pds:dd_class::terminological_entry::1.0 rdf:type rdf:Property;
  rdfs:label "terminological_entry";
  rdfs:domain pds4:urn:nasa:pds:0001_nasa_pds_1:pds:tndo_supplemental:pds:dd_class::1.0;
  rdfs:range pds4:urn:nasa:pds:0001_nasa_pds_1:pds:tagged_nondigital_child:pds:terminological_entry::1.0.
 
pds4:urn:nasa:pds:0001_nasa_pds_1:pds:tndo_supplemental:pds:dd_class::internal_reference::1.0 rdf:type rdf:Property;
  rdfs:label "internal_reference";
  rdfs:domain pds4:urn:nasa:pds:0001_nasa_pds_1:pds:tndo_supplemental:pds:dd_class::1.0;
  rdfs:range pds4:urn:nasa:pds:0001_nasa_pds_1:pds:product_components:pds:internal_reference::1.0.
 
pds4:urn:nasa:pds:0001_nasa_pds_1:pds:tndo_supplemental:pds:dd_class::data_object::1.0 rdf:type rdf:Property;
  rdfs:label "data_object";
  rdfs:domain pds4:urn:nasa:pds:0001_nasa_pds_1:pds:tndo_supplemental:pds:dd_class::1.0;
  rdfs:range pds4:urn:nasa:pds:0001_nasa_pds_1:pds:tndo_context:pds:other::1.0.
 
pds4:urn:nasa:pds:0001_nasa_pds_1:pds:tndo_supplemental:pds:dd_class::dd_association::1.0 rdf:type rdf:Property;
  rdfs:label "dd_association";
  rdfs:domain pds4:urn:nasa:pds:0001_nasa_pds_1:pds:tndo_supplemental:pds:dd_class::1.0;
  rdfs:range pds4:urn:nasa:pds:0001_nasa_pds_1:pds:tagged_nondigital_child:pds:dd_associate_external_class::1.0.
 
pds4:urn:nasa:pds:0001_nasa_pds_1:pds:tndo_supplemental:pds:dd_class::dd_association::1.0 rdf:type rdf:Property;
  rdfs:label "dd_association";
  rdfs:domain pds4:urn:nasa:pds:0001_nasa_pds_1:pds:tndo_supplemental:pds:dd_class::1.0;
  rdfs:range pds4:urn:nasa:pds:0001_nasa_pds_1:pds:tagged_nondigital_child:pds:dd_association::1.0.
 
pds4:urn:nasa:pds:0001_nasa_pds_1:pds:tndo_supplemental:pds:dd_class::dd_association::1.0 rdf:type rdf:Property;
  rdfs:label "dd_association";
  rdfs:domain pds4:urn:nasa:pds:0001_nasa_pds_1:pds:tndo_supplemental:pds:dd_class::1.0;
  rdfs:range pds4:urn:nasa:pds:0001_nasa_pds_1:pds:tagged_nondigital_child:pds:dd_association_external::1.0.
 
pds4:urn:nasa:pds:0001_nasa_pds_1:pds:tndo_supplemental:pds:dd_class_full::terminological_entry::1.0 rdf:type rdf:Property;
  rdfs:label "terminological_entry";
  rdfs:domain pds4:urn:nasa:pds:0001_nasa_pds_1:pds:tndo_supplemental:pds:dd_class_full::1.0;
  rdfs:range pds4:urn:nasa:pds:0001_nasa_pds_1:pds:tagged_nondigital_child:pds:terminological_entry::1.0.
 
pds4:urn:nasa:pds:0001_nasa_pds_1:pds:tndo_supplemental:pds:dd_class_full::dd_association::1.0 rdf:type rdf:Property;
  rdfs:label "dd_association";
  rdfs:domain pds4:urn:nasa:pds:0001_nasa_pds_1:pds:tndo_supplemental:pds:dd_class_full::1.0;
  rdfs:range pds4:urn:nasa:pds:0001_nasa_pds_1:pds:tagged_nondigital_child:pds:dd_association::1.0.
 
pds4:urn:nasa:pds:0001_nasa_pds_1:pds:tndo_supplemental:pds:dd_class_full::data_object::1.0 rdf:type rdf:Property;
  rdfs:label "data_object";
  rdfs:domain pds4:urn:nasa:pds:0001_nasa_pds_1:pds:tndo_supplemental:pds:dd_class_full::1.0;
  rdfs:range pds4:urn:nasa:pds:0001_nasa_pds_1:pds:tndo_context:pds:other::1.0.
 
pds4:urn:nasa:pds:0001_nasa_pds_1:pds:tagged_nondigital_child:pds:dd_context_value_list::permissible_value::1.0 rdf:type rdf:Property;
  rdfs:label "permissible_value";
  rdfs:domain pds4:urn:nasa:pds:0001_nasa_pds_1:pds:tagged_nondigital_child:pds:dd_context_value_list::1.0;
  rdfs:range pds4:urn:nasa:pds:0001_nasa_pds_1:pds:tagged_nondigital_child:pds:dd_permissible_value::1.0.
 
pds4:urn:nasa:pds:0001_nasa_pds_1:pds:tagged_nondigital_child:pds:dd_permissible_value::terminological_entry::1.0 rdf:type rdf:Property;
  rdfs:label "terminological_entry";
  rdfs:domain pds4:urn:nasa:pds:0001_nasa_pds_1:pds:tagged_nondigital_child:pds:dd_permissible_value::1.0;
  rdfs:range pds4:urn:nasa:pds:0001_nasa_pds_1:pds:tagged_nondigital_child:pds:terminological_entry::1.0.
 
pds4:urn:nasa:pds:0001_nasa_pds_1:pds:tagged_nondigital_child:pds:dd_permissible_value_full::terminological_entry::1.0 rdf:type rdf:Property;
  rdfs:label "terminological_entry";
  rdfs:domain pds4:urn:nasa:pds:0001_nasa_pds_1:pds:tagged_nondigital_child:pds:dd_permissible_value_full::1.0;
  rdfs:range pds4:urn:nasa:pds:0001_nasa_pds_1:pds:tagged_nondigital_child:pds:terminological_entry::1.0.
 
pds4:urn:nasa:pds:0001_nasa_pds_1:pds:tndo_supplemental:pds:dd_rule::rule_statement::1.0 rdf:type rdf:Property;
  rdfs:label "rule_statement";
  rdfs:domain pds4:urn:nasa:pds:0001_nasa_pds_1:pds:tndo_supplemental:pds:dd_rule::1.0;
  rdfs:range pds4:urn:nasa:pds:0001_nasa_pds_1:pds:tndo_supplemental:pds:dd_rule_statement::1.0.
 
pds4:urn:nasa:pds:0001_nasa_pds_1:pds:tndo_supplemental:pds:dd_rule::dd_attribute_reference::1.0 rdf:type rdf:Property;
  rdfs:label "dd_attribute_reference";
  rdfs:domain pds4:urn:nasa:pds:0001_nasa_pds_1:pds:tndo_supplemental:pds:dd_rule::1.0;
  rdfs:range pds4:urn:nasa:pds:0001_nasa_pds_1:pds:tagged_nondigital_child:pds:dd_attribute_reference::1.0.
 
pds4:urn:nasa:pds:0001_nasa_pds_1:pds:tndo_supplemental:pds:dd_rule::dd_class_reference::1.0 rdf:type rdf:Property;
  rdfs:label "dd_class_reference";
  rdfs:domain pds4:urn:nasa:pds:0001_nasa_pds_1:pds:tndo_supplemental:pds:dd_rule::1.0;
  rdfs:range pds4:urn:nasa:pds:0001_nasa_pds_1:pds:tagged_nondigital_child:pds:dd_class_reference::1.0.
 
pds4:urn:nasa:pds:0001_nasa_pds_1:pds:tagged_nondigital_child:pds:dd_value_domain::permissible_value::1.0 rdf:type rdf:Property;
  rdfs:label "permissible_value";
  rdfs:domain pds4:urn:nasa:pds:0001_nasa_pds_1:pds:tagged_nondigital_child:pds:dd_value_domain::1.0;
  rdfs:range pds4:urn:nasa:pds:0001_nasa_pds_1:pds:tagged_nondigital_child:pds:dd_permissible_value::1.0.
 
pds4:urn:nasa:pds:0001_nasa_pds_1:pds:tagged_nondigital_child:pds:dd_value_domain_full::permissible_value::1.0 rdf:type rdf:Property;
  rdfs:label "permissible_value";
  rdfs:domain pds4:urn:nasa:pds:0001_nasa_pds_1:pds:tagged_nondigital_child:pds:dd_value_domain_full::1.0;
  rdfs:range pds4:urn:nasa:pds:0001_nasa_pds_1:pds:tagged_nondigital_child:pds:dd_permissible_value_full::1.0.
 
pds4:urn:nasa:pds:0001_nasa_pds_1:pds:tndo_context_pds3:pds:data_set_pds3::nssdc::1.0 rdf:type rdf:Property;
  rdfs:label "nssdc";
  rdfs:domain pds4:urn:nasa:pds:0001_nasa_pds_1:pds:tndo_context_pds3:pds:data_set_pds3::1.0;
  rdfs:range pds4:urn:nasa:pds:0001_nasa_pds_1:pds:tagged_nondigital_child:pds:nssdc::1.0.
 
pds4:urn:nasa:pds:0001_nasa_pds_1:pds:tndo_context_pds3:pds:data_set_pds3::data_object::1.0 rdf:type rdf:Property;
  rdfs:label "data_object";
  rdfs:domain pds4:urn:nasa:pds:0001_nasa_pds_1:pds:tndo_context_pds3:pds:data_set_pds3::1.0;
  rdfs:range pds4:urn:nasa:pds:0001_nasa_pds_1:pds:tndo_context:pds:other::1.0.
 
pds4:urn:nasa:pds:0001_nasa_pds_1:pds:tndo_context_pds3:pds:data_set_pds3::data_object::1.0 rdf:type rdf:Property;
  rdfs:label "data_object";
  rdfs:domain pds4:urn:nasa:pds:0001_nasa_pds_1:pds:tndo_context_pds3:pds:data_set_pds3::1.0;
  rdfs:range pds4:urn:nasa:pds:0001_nasa_pds_1:pds:tndo_context:pds:other::1.0.
 
pds4:urn:nasa:pds:0001_nasa_pds_1:pds:product_components:pds:discipline_facets::has_group_facet2::1.0 rdf:type rdf:Property;
  rdfs:label "has_Group_Facet2";
  rdfs:domain pds4:urn:nasa:pds:0001_nasa_pds_1:pds:product_components:pds:discipline_facets::1.0;
  rdfs:range pds4:urn:nasa:pds:0001_nasa_pds_1:pds:product_components:pds:group_facet2::1.0.
 
pds4:urn:nasa:pds:0001_nasa_pds_1:pds:product_components:pds:discipline_facets::has_group_facet1::1.0 rdf:type rdf:Property;
  rdfs:label "has_Group_Facet1";
  rdfs:domain pds4:urn:nasa:pds:0001_nasa_pds_1:pds:product_components:pds:discipline_facets::1.0;
  rdfs:range pds4:urn:nasa:pds:0001_nasa_pds_1:pds:product_components:pds:group_facet1::1.0.
 
pds4:urn:nasa:pds:0001_nasa_pds_1:pds:tndo_supplemental:pds:document::data_object::1.0 rdf:type rdf:Property;
  rdfs:label "data_object";
  rdfs:domain pds4:urn:nasa:pds:0001_nasa_pds_1:pds:tndo_supplemental:pds:document::1.0;
  rdfs:range pds4:urn:nasa:pds:0001_nasa_pds_1:pds:tndo_context:pds:other::1.0.
 
pds4:urn:nasa:pds:0001_nasa_pds_1:pds:tndo_supplemental:pds:document::has_document_edition::1.0 rdf:type rdf:Property;
  rdfs:label "has_document_edition";
  rdfs:domain pds4:urn:nasa:pds:0001_nasa_pds_1:pds:tndo_supplemental:pds:document::1.0;
  rdfs:range pds4:urn:nasa:pds:0001_nasa_pds_1:pds:tagged_nondigital_child:pds:document_edition::1.0.
 
pds4:urn:nasa:pds:0001_nasa_pds_1:pds:tagged_nondigital_child:pds:document_edition::has_document_file::1.0 rdf:type rdf:Property;
  rdfs:label "has_document_file";
  rdfs:domain pds4:urn:nasa:pds:0001_nasa_pds_1:pds:tagged_nondigital_child:pds:document_edition::1.0;
  rdfs:range pds4:urn:nasa:pds:0001_nasa_pds_1:pds:file:pds:document_file::1.0.
 
pds4:urn:nasa:pds:0001_nasa_pds_1:pds:byte_stream:pds:encoded_byte_stream::data_object::1.0 rdf:type rdf:Property;
  rdfs:label "data_object";
  rdfs:domain pds4:urn:nasa:pds:0001_nasa_pds_1:pds:byte_stream:pds:encoded_byte_stream::1.0;
  rdfs:range pds4:urn:nasa:pds:0001_nasa_pds_1:pds:tndo_context:pds:other::1.0.
 
pds4:urn:nasa:pds:0001_nasa_pds_1:pds:tndo_context:pds:facility::data_object::1.0 rdf:type rdf:Property;
  rdfs:label "data_object";
  rdfs:domain pds4:urn:nasa:pds:0001_nasa_pds_1:pds:tndo_context:pds:facility::1.0;
  rdfs:range pds4:urn:nasa:pds:0001_nasa_pds_1:pds:tndo_context:pds:other::1.0.
 
pds4:urn:nasa:pds:0001_nasa_pds_1:pds:field:pds:field_binary::associated_statistics::1.0 rdf:type rdf:Property;
  rdfs:label "associated_Statistics";
  rdfs:domain pds4:urn:nasa:pds:0001_nasa_pds_1:pds:field:pds:field_binary::1.0;
  rdfs:range pds4:urn:nasa:pds:0001_nasa_pds_1:pds:tndo_supplemental:pds:field_statistics::1.0.
 
pds4:urn:nasa:pds:0001_nasa_pds_1:pds:field:pds:field_binary::associated_special_constants::1.0 rdf:type rdf:Property;
  rdfs:label "associated_Special_Constants";
  rdfs:domain pds4:urn:nasa:pds:0001_nasa_pds_1:pds:field:pds:field_binary::1.0;
  rdfs:range pds4:urn:nasa:pds:0001_nasa_pds_1:pds:tagged_digital_child:pds:special_constants::1.0.
 
pds4:urn:nasa:pds:0001_nasa_pds_1:pds:field:pds:field_binary::has_packed_data_fields::1.0 rdf:type rdf:Property;
  rdfs:label "has_Packed_Data_Fields";
  rdfs:domain pds4:urn:nasa:pds:0001_nasa_pds_1:pds:field:pds:field_binary::1.0;
  rdfs:range pds4:urn:nasa:pds:0001_nasa_pds_1:pds:tagged_digital_child:pds:packed_data_fields::1.0.
 
pds4:urn:nasa:pds:0001_nasa_pds_1:pds:field:pds:field_bit::associated_special_constants::1.0 rdf:type rdf:Property;
  rdfs:label "associated_Special_Constants";
  rdfs:domain pds4:urn:nasa:pds:0001_nasa_pds_1:pds:field:pds:field_bit::1.0;
  rdfs:range pds4:urn:nasa:pds:0001_nasa_pds_1:pds:tagged_digital_child:pds:special_constants::1.0.
 
pds4:urn:nasa:pds:0001_nasa_pds_1:pds:field:pds:field_character::associated_statistics::1.0 rdf:type rdf:Property;
  rdfs:label "associated_Statistics";
  rdfs:domain pds4:urn:nasa:pds:0001_nasa_pds_1:pds:field:pds:field_character::1.0;
  rdfs:range pds4:urn:nasa:pds:0001_nasa_pds_1:pds:tndo_supplemental:pds:field_statistics::1.0.
 
pds4:urn:nasa:pds:0001_nasa_pds_1:pds:field:pds:field_character::associated_special_constants::1.0 rdf:type rdf:Property;
  rdfs:label "associated_Special_Constants";
  rdfs:domain pds4:urn:nasa:pds:0001_nasa_pds_1:pds:field:pds:field_character::1.0;
  rdfs:range pds4:urn:nasa:pds:0001_nasa_pds_1:pds:tagged_digital_child:pds:special_constants::1.0.
 
pds4:urn:nasa:pds:0001_nasa_pds_1:pds:field:pds:field_delimited::associated_statistics::1.0 rdf:type rdf:Property;
  rdfs:label "associated_Statistics";
  rdfs:domain pds4:urn:nasa:pds:0001_nasa_pds_1:pds:field:pds:field_delimited::1.0;
  rdfs:range pds4:urn:nasa:pds:0001_nasa_pds_1:pds:tndo_supplemental:pds:field_statistics::1.0.
 
pds4:urn:nasa:pds:0001_nasa_pds_1:pds:field:pds:field_delimited::associated_special_constants::1.0 rdf:type rdf:Property;
  rdfs:label "associated_Special_Constants";
  rdfs:domain pds4:urn:nasa:pds:0001_nasa_pds_1:pds:field:pds:field_delimited::1.0;
  rdfs:range pds4:urn:nasa:pds:0001_nasa_pds_1:pds:tagged_digital_child:pds:special_constants::1.0.
 
pds4:urn:nasa:pds:0001_nasa_pds_1:pds:tndo_supplemental:pds:field_statistics::data_object::1.0 rdf:type rdf:Property;
  rdfs:label "data_object";
  rdfs:domain pds4:urn:nasa:pds:0001_nasa_pds_1:pds:tndo_supplemental:pds:field_statistics::1.0;
  rdfs:range pds4:urn:nasa:pds:0001_nasa_pds_1:pds:tndo_context:pds:other::1.0.
 
pds4:urn:nasa:pds:0001_nasa_pds_1:pds:tagged_digital_object:pds:file::data_object::1.0 rdf:type rdf:Property;
  rdfs:label "data_object";
  rdfs:domain pds4:urn:nasa:pds:0001_nasa_pds_1:pds:tagged_digital_object:pds:file::1.0;
  rdfs:range pds4:urn:nasa:pds:0001_nasa_pds_1:pds:tndo_context:pds:other::1.0.
 
pds4:urn:nasa:pds:0001_nasa_pds_1:pds:file_area:pds:file_area_ancillary::has_tagged_data_object::1.0 rdf:type rdf:Property;
  rdfs:label "has_tagged_data_object";
  rdfs:domain pds4:urn:nasa:pds:0001_nasa_pds_1:pds:file_area:pds:file_area_ancillary::1.0;
  rdfs:range pds4:urn:nasa:pds:0001_nasa_pds_1:pds:byte_stream:pds:array::1.0.
 
pds4:urn:nasa:pds:0001_nasa_pds_1:pds:file_area:pds:file_area_ancillary::has_tagged_data_object::1.0 rdf:type rdf:Property;
  rdfs:label "has_tagged_data_object";
  rdfs:domain pds4:urn:nasa:pds:0001_nasa_pds_1:pds:file_area:pds:file_area_ancillary::1.0;
  rdfs:range pds4:urn:nasa:pds:0001_nasa_pds_1:pds:array:pds:array_1d::1.0.
 
pds4:urn:nasa:pds:0001_nasa_pds_1:pds:file_area:pds:file_area_ancillary::has_tagged_data_object::1.0 rdf:type rdf:Property;
  rdfs:label "has_tagged_data_object";
  rdfs:domain pds4:urn:nasa:pds:0001_nasa_pds_1:pds:file_area:pds:file_area_ancillary::1.0;
  rdfs:range pds4:urn:nasa:pds:0001_nasa_pds_1:pds:array:pds:array_2d::1.0.
 
pds4:urn:nasa:pds:0001_nasa_pds_1:pds:file_area:pds:file_area_ancillary::has_tagged_data_object::1.0 rdf:type rdf:Property;
  rdfs:label "has_tagged_data_object";
  rdfs:domain pds4:urn:nasa:pds:0001_nasa_pds_1:pds:file_area:pds:file_area_ancillary::1.0;
  rdfs:range pds4:urn:nasa:pds:0001_nasa_pds_1:pds:array_2d:pds:array_2d_image::1.0.
 
pds4:urn:nasa:pds:0001_nasa_pds_1:pds:file_area:pds:file_area_ancillary::has_tagged_data_object::1.0 rdf:type rdf:Property;
  rdfs:label "has_tagged_data_object";
  rdfs:domain pds4:urn:nasa:pds:0001_nasa_pds_1:pds:file_area:pds:file_area_ancillary::1.0;
  rdfs:range pds4:urn:nasa:pds:0001_nasa_pds_1:pds:array_2d:pds:array_2d_map::1.0.
 
pds4:urn:nasa:pds:0001_nasa_pds_1:pds:file_area:pds:file_area_ancillary::has_tagged_data_object::1.0 rdf:type rdf:Property;
  rdfs:label "has_tagged_data_object";
  rdfs:domain pds4:urn:nasa:pds:0001_nasa_pds_1:pds:file_area:pds:file_area_ancillary::1.0;
  rdfs:range pds4:urn:nasa:pds:0001_nasa_pds_1:pds:array_2d:pds:array_2d_spectrum::1.0.
 
pds4:urn:nasa:pds:0001_nasa_pds_1:pds:file_area:pds:file_area_ancillary::has_tagged_data_object::1.0 rdf:type rdf:Property;
  rdfs:label "has_tagged_data_object";
  rdfs:domain pds4:urn:nasa:pds:0001_nasa_pds_1:pds:file_area:pds:file_area_ancillary::1.0;
  rdfs:range pds4:urn:nasa:pds:0001_nasa_pds_1:pds:array:pds:array_3d::1.0.
 
pds4:urn:nasa:pds:0001_nasa_pds_1:pds:file_area:pds:file_area_ancillary::has_tagged_data_object::1.0 rdf:type rdf:Property;
  rdfs:label "has_tagged_data_object";
  rdfs:domain pds4:urn:nasa:pds:0001_nasa_pds_1:pds:file_area:pds:file_area_ancillary::1.0;
  rdfs:range pds4:urn:nasa:pds:0001_nasa_pds_1:pds:array_3d:pds:array_3d_image::1.0.
 
pds4:urn:nasa:pds:0001_nasa_pds_1:pds:file_area:pds:file_area_ancillary::has_tagged_data_object::1.0 rdf:type rdf:Property;
  rdfs:label "has_tagged_data_object";
  rdfs:domain pds4:urn:nasa:pds:0001_nasa_pds_1:pds:file_area:pds:file_area_ancillary::1.0;
  rdfs:range pds4:urn:nasa:pds:0001_nasa_pds_1:pds:array_3d:pds:array_3d_movie::1.0.
 
pds4:urn:nasa:pds:0001_nasa_pds_1:pds:file_area:pds:file_area_ancillary::has_tagged_data_object::1.0 rdf:type rdf:Property;
  rdfs:label "has_tagged_data_object";
  rdfs:domain pds4:urn:nasa:pds:0001_nasa_pds_1:pds:file_area:pds:file_area_ancillary::1.0;
  rdfs:range pds4:urn:nasa:pds:0001_nasa_pds_1:pds:array_3d:pds:array_3d_spectrum::1.0.
 
pds4:urn:nasa:pds:0001_nasa_pds_1:pds:file_area:pds:file_area_ancillary::has_tagged_data_object::1.0 rdf:type rdf:Property;
  rdfs:label "has_tagged_data_object";
  rdfs:domain pds4:urn:nasa:pds:0001_nasa_pds_1:pds:file_area:pds:file_area_ancillary::1.0;
  rdfs:range pds4:urn:nasa:pds:0001_nasa_pds_1:pds:parsable_byte_stream:pds:checksum_manifest::1.0.
 
pds4:urn:nasa:pds:0001_nasa_pds_1:pds:file_area:pds:file_area_ancillary::has_tagged_data_object::1.0 rdf:type rdf:Property;
  rdfs:label "has_tagged_data_object";
  rdfs:domain pds4:urn:nasa:pds:0001_nasa_pds_1:pds:file_area:pds:file_area_ancillary::1.0;
  rdfs:range pds4:urn:nasa:pds:0001_nasa_pds_1:pds:encoded_byte_stream:pds:encoded_audio::1.0.
 
pds4:urn:nasa:pds:0001_nasa_pds_1:pds:file_area:pds:file_area_ancillary::has_tagged_data_object::1.0 rdf:type rdf:Property;
  rdfs:label "has_tagged_data_object";
  rdfs:domain pds4:urn:nasa:pds:0001_nasa_pds_1:pds:file_area:pds:file_area_ancillary::1.0;
  rdfs:range pds4:urn:nasa:pds:0001_nasa_pds_1:pds:encoded_byte_stream:pds:encoded_header::1.0.
 
pds4:urn:nasa:pds:0001_nasa_pds_1:pds:file_area:pds:file_area_ancillary::has_tagged_data_object::1.0 rdf:type rdf:Property;
  rdfs:label "has_tagged_data_object";
  rdfs:domain pds4:urn:nasa:pds:0001_nasa_pds_1:pds:file_area:pds:file_area_ancillary::1.0;
  rdfs:range pds4:urn:nasa:pds:0001_nasa_pds_1:pds:encoded_byte_stream:pds:encoded_image::1.0.
 
pds4:urn:nasa:pds:0001_nasa_pds_1:pds:file_area:pds:file_area_ancillary::has_tagged_data_object::1.0 rdf:type rdf:Property;
  rdfs:label "has_tagged_data_object";
  rdfs:domain pds4:urn:nasa:pds:0001_nasa_pds_1:pds:file_area:pds:file_area_ancillary::1.0;
  rdfs:range pds4:urn:nasa:pds:0001_nasa_pds_1:pds:parsable_byte_stream:pds:header::1.0.
 
pds4:urn:nasa:pds:0001_nasa_pds_1:pds:file_area:pds:file_area_ancillary::has_tagged_data_object::1.0 rdf:type rdf:Property;
  rdfs:label "has_tagged_data_object";
  rdfs:domain pds4:urn:nasa:pds:0001_nasa_pds_1:pds:file_area:pds:file_area_ancillary::1.0;
  rdfs:range pds4:urn:nasa:pds:0001_nasa_pds_1:pds:parsable_byte_stream:pds:stream_text::1.0.
 
pds4:urn:nasa:pds:0001_nasa_pds_1:pds:file_area:pds:file_area_ancillary::has_tagged_data_object::1.0 rdf:type rdf:Property;
  rdfs:label "has_tagged_data_object";
  rdfs:domain pds4:urn:nasa:pds:0001_nasa_pds_1:pds:file_area:pds:file_area_ancillary::1.0;
  rdfs:range pds4:urn:nasa:pds:0001_nasa_pds_1:pds:table_base:pds:table_binary::1.0.
 
pds4:urn:nasa:pds:0001_nasa_pds_1:pds:file_area:pds:file_area_ancillary::has_tagged_data_object::1.0 rdf:type rdf:Property;
  rdfs:label "has_tagged_data_object";
  rdfs:domain pds4:urn:nasa:pds:0001_nasa_pds_1:pds:file_area:pds:file_area_ancillary::1.0;
  rdfs:range pds4:urn:nasa:pds:0001_nasa_pds_1:pds:table_base:pds:table_character::1.0.
 
pds4:urn:nasa:pds:0001_nasa_pds_1:pds:file_area:pds:file_area_ancillary::has_tagged_data_object::1.0 rdf:type rdf:Property;
  rdfs:label "has_tagged_data_object";
  rdfs:domain pds4:urn:nasa:pds:0001_nasa_pds_1:pds:file_area:pds:file_area_ancillary::1.0;
  rdfs:range pds4:urn:nasa:pds:0001_nasa_pds_1:pds:parsable_byte_stream:pds:table_delimited::1.0.
 
pds4:urn:nasa:pds:0001_nasa_pds_1:pds:file_area:pds:file_area_ancillary::has_file::1.0 rdf:type rdf:Property;
  rdfs:label "has_File";
  rdfs:domain pds4:urn:nasa:pds:0001_nasa_pds_1:pds:file_area:pds:file_area_ancillary::1.0;
  rdfs:range pds4:urn:nasa:pds:0001_nasa_pds_1:pds:tagged_digital_object:pds:file::1.0.
 
pds4:urn:nasa:pds:0001_nasa_pds_1:pds:file_area:pds:file_area_binary::has_tagged_data_object::1.0 rdf:type rdf:Property;
  rdfs:label "has_tagged_data_object";
  rdfs:domain pds4:urn:nasa:pds:0001_nasa_pds_1:pds:file_area:pds:file_area_binary::1.0;
  rdfs:range pds4:urn:nasa:pds:0001_nasa_pds_1:pds:encoded_byte_stream:pds:encoded_binary::1.0.
 
pds4:urn:nasa:pds:0001_nasa_pds_1:pds:file_area:pds:file_area_binary::has_file::1.0 rdf:type rdf:Property;
  rdfs:label "has_File";
  rdfs:domain pds4:urn:nasa:pds:0001_nasa_pds_1:pds:file_area:pds:file_area_binary::1.0;
  rdfs:range pds4:urn:nasa:pds:0001_nasa_pds_1:pds:tagged_digital_object:pds:file::1.0.
 
pds4:urn:nasa:pds:0001_nasa_pds_1:pds:file_area:pds:file_area_browse::has_tagged_data_object::1.0 rdf:type rdf:Property;
  rdfs:label "has_tagged_data_object";
  rdfs:domain pds4:urn:nasa:pds:0001_nasa_pds_1:pds:file_area:pds:file_area_browse::1.0;
  rdfs:range pds4:urn:nasa:pds:0001_nasa_pds_1:pds:byte_stream:pds:array::1.0.
 
pds4:urn:nasa:pds:0001_nasa_pds_1:pds:file_area:pds:file_area_browse::has_tagged_data_object::1.0 rdf:type rdf:Property;
  rdfs:label "has_tagged_data_object";
  rdfs:domain pds4:urn:nasa:pds:0001_nasa_pds_1:pds:file_area:pds:file_area_browse::1.0;
  rdfs:range pds4:urn:nasa:pds:0001_nasa_pds_1:pds:array:pds:array_1d::1.0.
 
pds4:urn:nasa:pds:0001_nasa_pds_1:pds:file_area:pds:file_area_browse::has_tagged_data_object::1.0 rdf:type rdf:Property;
  rdfs:label "has_tagged_data_object";
  rdfs:domain pds4:urn:nasa:pds:0001_nasa_pds_1:pds:file_area:pds:file_area_browse::1.0;
  rdfs:range pds4:urn:nasa:pds:0001_nasa_pds_1:pds:array:pds:array_2d::1.0.
 
pds4:urn:nasa:pds:0001_nasa_pds_1:pds:file_area:pds:file_area_browse::has_tagged_data_object::1.0 rdf:type rdf:Property;
  rdfs:label "has_tagged_data_object";
  rdfs:domain pds4:urn:nasa:pds:0001_nasa_pds_1:pds:file_area:pds:file_area_browse::1.0;
  rdfs:range pds4:urn:nasa:pds:0001_nasa_pds_1:pds:array_2d:pds:array_2d_image::1.0.
 
pds4:urn:nasa:pds:0001_nasa_pds_1:pds:file_area:pds:file_area_browse::has_tagged_data_object::1.0 rdf:type rdf:Property;
  rdfs:label "has_tagged_data_object";
  rdfs:domain pds4:urn:nasa:pds:0001_nasa_pds_1:pds:file_area:pds:file_area_browse::1.0;
  rdfs:range pds4:urn:nasa:pds:0001_nasa_pds_1:pds:array_2d:pds:array_2d_map::1.0.
 
pds4:urn:nasa:pds:0001_nasa_pds_1:pds:file_area:pds:file_area_browse::has_tagged_data_object::1.0 rdf:type rdf:Property;
  rdfs:label "has_tagged_data_object";
  rdfs:domain pds4:urn:nasa:pds:0001_nasa_pds_1:pds:file_area:pds:file_area_browse::1.0;
  rdfs:range pds4:urn:nasa:pds:0001_nasa_pds_1:pds:array_2d:pds:array_2d_spectrum::1.0.
 
pds4:urn:nasa:pds:0001_nasa_pds_1:pds:file_area:pds:file_area_browse::has_tagged_data_object::1.0 rdf:type rdf:Property;
  rdfs:label "has_tagged_data_object";
  rdfs:domain pds4:urn:nasa:pds:0001_nasa_pds_1:pds:file_area:pds:file_area_browse::1.0;
  rdfs:range pds4:urn:nasa:pds:0001_nasa_pds_1:pds:array:pds:array_3d::1.0.
 
pds4:urn:nasa:pds:0001_nasa_pds_1:pds:file_area:pds:file_area_browse::has_tagged_data_object::1.0 rdf:type rdf:Property;
  rdfs:label "has_tagged_data_object";
  rdfs:domain pds4:urn:nasa:pds:0001_nasa_pds_1:pds:file_area:pds:file_area_browse::1.0;
  rdfs:range pds4:urn:nasa:pds:0001_nasa_pds_1:pds:array_3d:pds:array_3d_image::1.0.
 
pds4:urn:nasa:pds:0001_nasa_pds_1:pds:file_area:pds:file_area_browse::has_tagged_data_object::1.0 rdf:type rdf:Property;
  rdfs:label "has_tagged_data_object";
  rdfs:domain pds4:urn:nasa:pds:0001_nasa_pds_1:pds:file_area:pds:file_area_browse::1.0;
  rdfs:range pds4:urn:nasa:pds:0001_nasa_pds_1:pds:array_3d:pds:array_3d_movie::1.0.
 
pds4:urn:nasa:pds:0001_nasa_pds_1:pds:file_area:pds:file_area_browse::has_tagged_data_object::1.0 rdf:type rdf:Property;
  rdfs:label "has_tagged_data_object";
  rdfs:domain pds4:urn:nasa:pds:0001_nasa_pds_1:pds:file_area:pds:file_area_browse::1.0;
  rdfs:range pds4:urn:nasa:pds:0001_nasa_pds_1:pds:array_3d:pds:array_3d_spectrum::1.0.
 
pds4:urn:nasa:pds:0001_nasa_pds_1:pds:file_area:pds:file_area_browse::has_tagged_data_object::1.0 rdf:type rdf:Property;
  rdfs:label "has_tagged_data_object";
  rdfs:domain pds4:urn:nasa:pds:0001_nasa_pds_1:pds:file_area:pds:file_area_browse::1.0;
  rdfs:range pds4:urn:nasa:pds:0001_nasa_pds_1:pds:encoded_byte_stream:pds:encoded_audio::1.0.
 
pds4:urn:nasa:pds:0001_nasa_pds_1:pds:file_area:pds:file_area_browse::has_tagged_data_object::1.0 rdf:type rdf:Property;
  rdfs:label "has_tagged_data_object";
  rdfs:domain pds4:urn:nasa:pds:0001_nasa_pds_1:pds:file_area:pds:file_area_browse::1.0;
  rdfs:range pds4:urn:nasa:pds:0001_nasa_pds_1:pds:encoded_byte_stream:pds:encoded_header::1.0.
 
pds4:urn:nasa:pds:0001_nasa_pds_1:pds:file_area:pds:file_area_browse::has_tagged_data_object::1.0 rdf:type rdf:Property;
  rdfs:label "has_tagged_data_object";
  rdfs:domain pds4:urn:nasa:pds:0001_nasa_pds_1:pds:file_area:pds:file_area_browse::1.0;
  rdfs:range pds4:urn:nasa:pds:0001_nasa_pds_1:pds:encoded_byte_stream:pds:encoded_image::1.0.
 
pds4:urn:nasa:pds:0001_nasa_pds_1:pds:file_area:pds:file_area_browse::has_tagged_data_object::1.0 rdf:type rdf:Property;
  rdfs:label "has_tagged_data_object";
  rdfs:domain pds4:urn:nasa:pds:0001_nasa_pds_1:pds:file_area:pds:file_area_browse::1.0;
  rdfs:range pds4:urn:nasa:pds:0001_nasa_pds_1:pds:parsable_byte_stream:pds:header::1.0.
 
pds4:urn:nasa:pds:0001_nasa_pds_1:pds:file_area:pds:file_area_browse::has_tagged_data_object::1.0 rdf:type rdf:Property;
  rdfs:label "has_tagged_data_object";
  rdfs:domain pds4:urn:nasa:pds:0001_nasa_pds_1:pds:file_area:pds:file_area_browse::1.0;
  rdfs:range pds4:urn:nasa:pds:0001_nasa_pds_1:pds:parsable_byte_stream:pds:stream_text::1.0.
 
pds4:urn:nasa:pds:0001_nasa_pds_1:pds:file_area:pds:file_area_browse::has_tagged_data_object::1.0 rdf:type rdf:Property;
  rdfs:label "has_tagged_data_object";
  rdfs:domain pds4:urn:nasa:pds:0001_nasa_pds_1:pds:file_area:pds:file_area_browse::1.0;
  rdfs:range pds4:urn:nasa:pds:0001_nasa_pds_1:pds:table_base:pds:table_binary::1.0.
 
pds4:urn:nasa:pds:0001_nasa_pds_1:pds:file_area:pds:file_area_browse::has_tagged_data_object::1.0 rdf:type rdf:Property;
  rdfs:label "has_tagged_data_object";
  rdfs:domain pds4:urn:nasa:pds:0001_nasa_pds_1:pds:file_area:pds:file_area_browse::1.0;
  rdfs:range pds4:urn:nasa:pds:0001_nasa_pds_1:pds:table_base:pds:table_character::1.0.
 
pds4:urn:nasa:pds:0001_nasa_pds_1:pds:file_area:pds:file_area_browse::has_tagged_data_object::1.0 rdf:type rdf:Property;
  rdfs:label "has_tagged_data_object";
  rdfs:domain pds4:urn:nasa:pds:0001_nasa_pds_1:pds:file_area:pds:file_area_browse::1.0;
  rdfs:range pds4:urn:nasa:pds:0001_nasa_pds_1:pds:parsable_byte_stream:pds:table_delimited::1.0.
 
pds4:urn:nasa:pds:0001_nasa_pds_1:pds:file_area:pds:file_area_browse::has_file::1.0 rdf:type rdf:Property;
  rdfs:label "has_File";
  rdfs:domain pds4:urn:nasa:pds:0001_nasa_pds_1:pds:file_area:pds:file_area_browse::1.0;
  rdfs:range pds4:urn:nasa:pds:0001_nasa_pds_1:pds:tagged_digital_object:pds:file::1.0.
 
pds4:urn:nasa:pds:0001_nasa_pds_1:pds:file_area:pds:file_area_checksum_manifest::has_tagged_data_object::1.0 rdf:type rdf:Property;
  rdfs:label "has_tagged_data_object";
  rdfs:domain pds4:urn:nasa:pds:0001_nasa_pds_1:pds:file_area:pds:file_area_checksum_manifest::1.0;
  rdfs:range pds4:urn:nasa:pds:0001_nasa_pds_1:pds:parsable_byte_stream:pds:checksum_manifest::1.0.
 
pds4:urn:nasa:pds:0001_nasa_pds_1:pds:file_area:pds:file_area_checksum_manifest::has_file::1.0 rdf:type rdf:Property;
  rdfs:label "has_File";
  rdfs:domain pds4:urn:nasa:pds:0001_nasa_pds_1:pds:file_area:pds:file_area_checksum_manifest::1.0;
  rdfs:range pds4:urn:nasa:pds:0001_nasa_pds_1:pds:tagged_digital_object:pds:file::1.0.
 
pds4:urn:nasa:pds:0001_nasa_pds_1:pds:file_area:pds:file_area_encoded_image::has_tagged_data_object::1.0 rdf:type rdf:Property;
  rdfs:label "has_tagged_data_object";
  rdfs:domain pds4:urn:nasa:pds:0001_nasa_pds_1:pds:file_area:pds:file_area_encoded_image::1.0;
  rdfs:range pds4:urn:nasa:pds:0001_nasa_pds_1:pds:encoded_byte_stream:pds:encoded_image::1.0.
 
pds4:urn:nasa:pds:0001_nasa_pds_1:pds:file_area:pds:file_area_encoded_image::has_file::1.0 rdf:type rdf:Property;
  rdfs:label "has_File";
  rdfs:domain pds4:urn:nasa:pds:0001_nasa_pds_1:pds:file_area:pds:file_area_encoded_image::1.0;
  rdfs:range pds4:urn:nasa:pds:0001_nasa_pds_1:pds:tagged_digital_object:pds:file::1.0.
 
pds4:urn:nasa:pds:0001_nasa_pds_1:pds:file_area:pds:file_area_inventory::has_tagged_data_object::1.0 rdf:type rdf:Property;
  rdfs:label "has_tagged_data_object";
  rdfs:domain pds4:urn:nasa:pds:0001_nasa_pds_1:pds:file_area:pds:file_area_inventory::1.0;
  rdfs:range pds4:urn:nasa:pds:0001_nasa_pds_1:pds:table_delimited:pds:inventory::1.0.
 
pds4:urn:nasa:pds:0001_nasa_pds_1:pds:file_area:pds:file_area_inventory::has_file::1.0 rdf:type rdf:Property;
  rdfs:label "has_File";
  rdfs:domain pds4:urn:nasa:pds:0001_nasa_pds_1:pds:file_area:pds:file_area_inventory::1.0;
  rdfs:range pds4:urn:nasa:pds:0001_nasa_pds_1:pds:tagged_digital_object:pds:file::1.0.
 
pds4:urn:nasa:pds:0001_nasa_pds_1:pds:file_area:pds:file_area_metadata::has_tagged_data_object2::1.0 rdf:type rdf:Property;
  rdfs:label "has_tagged_data_object2";
  rdfs:domain pds4:urn:nasa:pds:0001_nasa_pds_1:pds:file_area:pds:file_area_metadata::1.0;
  rdfs:range pds4:urn:nasa:pds:0001_nasa_pds_1:pds:parsable_byte_stream:pds:header::1.0.
 
pds4:urn:nasa:pds:0001_nasa_pds_1:pds:file_area:pds:file_area_metadata::has_tagged_data_object::1.0 rdf:type rdf:Property;
  rdfs:label "has_tagged_data_object";
  rdfs:domain pds4:urn:nasa:pds:0001_nasa_pds_1:pds:file_area:pds:file_area_metadata::1.0;
  rdfs:range pds4:urn:nasa:pds:0001_nasa_pds_1:pds:table_base:pds:table_character::1.0.
 
pds4:urn:nasa:pds:0001_nasa_pds_1:pds:file_area:pds:file_area_metadata::has_tagged_data_object::1.0 rdf:type rdf:Property;
  rdfs:label "has_tagged_data_object";
  rdfs:domain pds4:urn:nasa:pds:0001_nasa_pds_1:pds:file_area:pds:file_area_metadata::1.0;
  rdfs:range pds4:urn:nasa:pds:0001_nasa_pds_1:pds:parsable_byte_stream:pds:table_delimited::1.0.
 
pds4:urn:nasa:pds:0001_nasa_pds_1:pds:file_area:pds:file_area_metadata::has_file::1.0 rdf:type rdf:Property;
  rdfs:label "has_File";
  rdfs:domain pds4:urn:nasa:pds:0001_nasa_pds_1:pds:file_area:pds:file_area_metadata::1.0;
  rdfs:range pds4:urn:nasa:pds:0001_nasa_pds_1:pds:tagged_digital_object:pds:file::1.0.
 
pds4:urn:nasa:pds:0001_nasa_pds_1:pds:file_area:pds:file_area_native::has_tagged_data_object::1.0 rdf:type rdf:Property;
  rdfs:label "has_tagged_data_object";
  rdfs:domain pds4:urn:nasa:pds:0001_nasa_pds_1:pds:file_area:pds:file_area_native::1.0;
  rdfs:range pds4:urn:nasa:pds:0001_nasa_pds_1:pds:encoded_byte_stream:pds:encoded_native::1.0.
 
pds4:urn:nasa:pds:0001_nasa_pds_1:pds:file_area:pds:file_area_native::has_file::1.0 rdf:type rdf:Property;
  rdfs:label "has_File";
  rdfs:domain pds4:urn:nasa:pds:0001_nasa_pds_1:pds:file_area:pds:file_area_native::1.0;
  rdfs:range pds4:urn:nasa:pds:0001_nasa_pds_1:pds:tagged_digital_object:pds:file::1.0.
 
pds4:urn:nasa:pds:0001_nasa_pds_1:pds:file_area:pds:file_area_observational::has_tagged_data_object::1.0 rdf:type rdf:Property;
  rdfs:label "has_tagged_data_object";
  rdfs:domain pds4:urn:nasa:pds:0001_nasa_pds_1:pds:file_area:pds:file_area_observational::1.0;
  rdfs:range pds4:urn:nasa:pds:0001_nasa_pds_1:pds:byte_stream:pds:array::1.0.
 
pds4:urn:nasa:pds:0001_nasa_pds_1:pds:file_area:pds:file_area_observational::has_tagged_data_object::1.0 rdf:type rdf:Property;
  rdfs:label "has_tagged_data_object";
  rdfs:domain pds4:urn:nasa:pds:0001_nasa_pds_1:pds:file_area:pds:file_area_observational::1.0;
  rdfs:range pds4:urn:nasa:pds:0001_nasa_pds_1:pds:array:pds:array_1d::1.0.
 
pds4:urn:nasa:pds:0001_nasa_pds_1:pds:file_area:pds:file_area_observational::has_tagged_data_object::1.0 rdf:type rdf:Property;
  rdfs:label "has_tagged_data_object";
  rdfs:domain pds4:urn:nasa:pds:0001_nasa_pds_1:pds:file_area:pds:file_area_observational::1.0;
  rdfs:range pds4:urn:nasa:pds:0001_nasa_pds_1:pds:array:pds:array_2d::1.0.
 
pds4:urn:nasa:pds:0001_nasa_pds_1:pds:file_area:pds:file_area_observational::has_tagged_data_object::1.0 rdf:type rdf:Property;
  rdfs:label "has_tagged_data_object";
  rdfs:domain pds4:urn:nasa:pds:0001_nasa_pds_1:pds:file_area:pds:file_area_observational::1.0;
  rdfs:range pds4:urn:nasa:pds:0001_nasa_pds_1:pds:array_2d:pds:array_2d_image::1.0.
 
pds4:urn:nasa:pds:0001_nasa_pds_1:pds:file_area:pds:file_area_observational::has_tagged_data_object::1.0 rdf:type rdf:Property;
  rdfs:label "has_tagged_data_object";
  rdfs:domain pds4:urn:nasa:pds:0001_nasa_pds_1:pds:file_area:pds:file_area_observational::1.0;
  rdfs:range pds4:urn:nasa:pds:0001_nasa_pds_1:pds:array_2d:pds:array_2d_map::1.0.
 
pds4:urn:nasa:pds:0001_nasa_pds_1:pds:file_area:pds:file_area_observational::has_tagged_data_object::1.0 rdf:type rdf:Property;
  rdfs:label "has_tagged_data_object";
  rdfs:domain pds4:urn:nasa:pds:0001_nasa_pds_1:pds:file_area:pds:file_area_observational::1.0;
  rdfs:range pds4:urn:nasa:pds:0001_nasa_pds_1:pds:array_2d:pds:array_2d_spectrum::1.0.
 
pds4:urn:nasa:pds:0001_nasa_pds_1:pds:file_area:pds:file_area_observational::has_tagged_data_object::1.0 rdf:type rdf:Property;
  rdfs:label "has_tagged_data_object";
  rdfs:domain pds4:urn:nasa:pds:0001_nasa_pds_1:pds:file_area:pds:file_area_observational::1.0;
  rdfs:range pds4:urn:nasa:pds:0001_nasa_pds_1:pds:array:pds:array_3d::1.0.
 
pds4:urn:nasa:pds:0001_nasa_pds_1:pds:file_area:pds:file_area_observational::has_tagged_data_object::1.0 rdf:type rdf:Property;
  rdfs:label "has_tagged_data_object";
  rdfs:domain pds4:urn:nasa:pds:0001_nasa_pds_1:pds:file_area:pds:file_area_observational::1.0;
  rdfs:range pds4:urn:nasa:pds:0001_nasa_pds_1:pds:array_3d:pds:array_3d_image::1.0.
 
pds4:urn:nasa:pds:0001_nasa_pds_1:pds:file_area:pds:file_area_observational::has_tagged_data_object::1.0 rdf:type rdf:Property;
  rdfs:label "has_tagged_data_object";
  rdfs:domain pds4:urn:nasa:pds:0001_nasa_pds_1:pds:file_area:pds:file_area_observational::1.0;
  rdfs:range pds4:urn:nasa:pds:0001_nasa_pds_1:pds:array_3d:pds:array_3d_movie::1.0.
 
pds4:urn:nasa:pds:0001_nasa_pds_1:pds:file_area:pds:file_area_observational::has_tagged_data_object::1.0 rdf:type rdf:Property;
  rdfs:label "has_tagged_data_object";
  rdfs:domain pds4:urn:nasa:pds:0001_nasa_pds_1:pds:file_area:pds:file_area_observational::1.0;
  rdfs:range pds4:urn:nasa:pds:0001_nasa_pds_1:pds:array_3d:pds:array_3d_spectrum::1.0.
 
pds4:urn:nasa:pds:0001_nasa_pds_1:pds:file_area:pds:file_area_observational::has_tagged_data_object::1.0 rdf:type rdf:Property;
  rdfs:label "has_tagged_data_object";
  rdfs:domain pds4:urn:nasa:pds:0001_nasa_pds_1:pds:file_area:pds:file_area_observational::1.0;
  rdfs:range pds4:urn:nasa:pds:0001_nasa_pds_1:pds:encoded_byte_stream:pds:encoded_header::1.0.
 
pds4:urn:nasa:pds:0001_nasa_pds_1:pds:file_area:pds:file_area_observational::has_tagged_data_object::1.0 rdf:type rdf:Property;
  rdfs:label "has_tagged_data_object";
  rdfs:domain pds4:urn:nasa:pds:0001_nasa_pds_1:pds:file_area:pds:file_area_observational::1.0;
  rdfs:range pds4:urn:nasa:pds:0001_nasa_pds_1:pds:parsable_byte_stream:pds:header::1.0.
 
pds4:urn:nasa:pds:0001_nasa_pds_1:pds:file_area:pds:file_area_observational::has_tagged_data_object::1.0 rdf:type rdf:Property;
  rdfs:label "has_tagged_data_object";
  rdfs:domain pds4:urn:nasa:pds:0001_nasa_pds_1:pds:file_area:pds:file_area_observational::1.0;
  rdfs:range pds4:urn:nasa:pds:0001_nasa_pds_1:pds:parsable_byte_stream:pds:stream_text::1.0.
 
pds4:urn:nasa:pds:0001_nasa_pds_1:pds:file_area:pds:file_area_observational::has_tagged_data_object::1.0 rdf:type rdf:Property;
  rdfs:label "has_tagged_data_object";
  rdfs:domain pds4:urn:nasa:pds:0001_nasa_pds_1:pds:file_area:pds:file_area_observational::1.0;
  rdfs:range pds4:urn:nasa:pds:0001_nasa_pds_1:pds:table_base:pds:table_binary::1.0.
 
pds4:urn:nasa:pds:0001_nasa_pds_1:pds:file_area:pds:file_area_observational::has_tagged_data_object::1.0 rdf:type rdf:Property;
  rdfs:label "has_tagged_data_object";
  rdfs:domain pds4:urn:nasa:pds:0001_nasa_pds_1:pds:file_area:pds:file_area_observational::1.0;
  rdfs:range pds4:urn:nasa:pds:0001_nasa_pds_1:pds:table_base:pds:table_character::1.0.
 
pds4:urn:nasa:pds:0001_nasa_pds_1:pds:file_area:pds:file_area_observational::has_tagged_data_object::1.0 rdf:type rdf:Property;
  rdfs:label "has_tagged_data_object";
  rdfs:domain pds4:urn:nasa:pds:0001_nasa_pds_1:pds:file_area:pds:file_area_observational::1.0;
  rdfs:range pds4:urn:nasa:pds:0001_nasa_pds_1:pds:parsable_byte_stream:pds:table_delimited::1.0.
 
pds4:urn:nasa:pds:0001_nasa_pds_1:pds:file_area:pds:file_area_observational::has_composite_structure::1.0 rdf:type rdf:Property;
  rdfs:label "has_composite_structure";
  rdfs:domain pds4:urn:nasa:pds:0001_nasa_pds_1:pds:file_area:pds:file_area_observational::1.0;
  rdfs:range pds4:urn:nasa:pds:0001_nasa_pds_1:pds:tagged_digital_object:pds:composite_structure::1.0.
 
pds4:urn:nasa:pds:0001_nasa_pds_1:pds:file_area:pds:file_area_observational::has_file::1.0 rdf:type rdf:Property;
  rdfs:label "has_File";
  rdfs:domain pds4:urn:nasa:pds:0001_nasa_pds_1:pds:file_area:pds:file_area_observational::1.0;
  rdfs:range pds4:urn:nasa:pds:0001_nasa_pds_1:pds:tagged_digital_object:pds:file::1.0.
 
pds4:urn:nasa:pds:0001_nasa_pds_1:pds:file_area:pds:file_area_observational_supplemental::has_tagged_data_object::1.0 rdf:type rdf:Property;
  rdfs:label "has_tagged_data_object";
  rdfs:domain pds4:urn:nasa:pds:0001_nasa_pds_1:pds:file_area:pds:file_area_observational_supplemental::1.0;
  rdfs:range pds4:urn:nasa:pds:0001_nasa_pds_1:pds:byte_stream:pds:array::1.0.
 
pds4:urn:nasa:pds:0001_nasa_pds_1:pds:file_area:pds:file_area_observational_supplemental::has_tagged_data_object::1.0 rdf:type rdf:Property;
  rdfs:label "has_tagged_data_object";
  rdfs:domain pds4:urn:nasa:pds:0001_nasa_pds_1:pds:file_area:pds:file_area_observational_supplemental::1.0;
  rdfs:range pds4:urn:nasa:pds:0001_nasa_pds_1:pds:array:pds:array_1d::1.0.
 
pds4:urn:nasa:pds:0001_nasa_pds_1:pds:file_area:pds:file_area_observational_supplemental::has_tagged_data_object::1.0 rdf:type rdf:Property;
  rdfs:label "has_tagged_data_object";
  rdfs:domain pds4:urn:nasa:pds:0001_nasa_pds_1:pds:file_area:pds:file_area_observational_supplemental::1.0;
  rdfs:range pds4:urn:nasa:pds:0001_nasa_pds_1:pds:array:pds:array_2d::1.0.
 
pds4:urn:nasa:pds:0001_nasa_pds_1:pds:file_area:pds:file_area_observational_supplemental::has_tagged_data_object::1.0 rdf:type rdf:Property;
  rdfs:label "has_tagged_data_object";
  rdfs:domain pds4:urn:nasa:pds:0001_nasa_pds_1:pds:file_area:pds:file_area_observational_supplemental::1.0;
  rdfs:range pds4:urn:nasa:pds:0001_nasa_pds_1:pds:array_2d:pds:array_2d_image::1.0.
 
pds4:urn:nasa:pds:0001_nasa_pds_1:pds:file_area:pds:file_area_observational_supplemental::has_tagged_data_object::1.0 rdf:type rdf:Property;
  rdfs:label "has_tagged_data_object";
  rdfs:domain pds4:urn:nasa:pds:0001_nasa_pds_1:pds:file_area:pds:file_area_observational_supplemental::1.0;
  rdfs:range pds4:urn:nasa:pds:0001_nasa_pds_1:pds:array_2d:pds:array_2d_map::1.0.
 
pds4:urn:nasa:pds:0001_nasa_pds_1:pds:file_area:pds:file_area_observational_supplemental::has_tagged_data_object::1.0 rdf:type rdf:Property;
  rdfs:label "has_tagged_data_object";
  rdfs:domain pds4:urn:nasa:pds:0001_nasa_pds_1:pds:file_area:pds:file_area_observational_supplemental::1.0;
  rdfs:range pds4:urn:nasa:pds:0001_nasa_pds_1:pds:array_2d:pds:array_2d_spectrum::1.0.
 
pds4:urn:nasa:pds:0001_nasa_pds_1:pds:file_area:pds:file_area_observational_supplemental::has_tagged_data_object::1.0 rdf:type rdf:Property;
  rdfs:label "has_tagged_data_object";
  rdfs:domain pds4:urn:nasa:pds:0001_nasa_pds_1:pds:file_area:pds:file_area_observational_supplemental::1.0;
  rdfs:range pds4:urn:nasa:pds:0001_nasa_pds_1:pds:array:pds:array_3d::1.0.
 
pds4:urn:nasa:pds:0001_nasa_pds_1:pds:file_area:pds:file_area_observational_supplemental::has_tagged_data_object::1.0 rdf:type rdf:Property;
  rdfs:label "has_tagged_data_object";
  rdfs:domain pds4:urn:nasa:pds:0001_nasa_pds_1:pds:file_area:pds:file_area_observational_supplemental::1.0;
  rdfs:range pds4:urn:nasa:pds:0001_nasa_pds_1:pds:array_3d:pds:array_3d_image::1.0.
 
pds4:urn:nasa:pds:0001_nasa_pds_1:pds:file_area:pds:file_area_observational_supplemental::has_tagged_data_object::1.0 rdf:type rdf:Property;
  rdfs:label "has_tagged_data_object";
  rdfs:domain pds4:urn:nasa:pds:0001_nasa_pds_1:pds:file_area:pds:file_area_observational_supplemental::1.0;
  rdfs:range pds4:urn:nasa:pds:0001_nasa_pds_1:pds:array_3d:pds:array_3d_movie::1.0.
 
pds4:urn:nasa:pds:0001_nasa_pds_1:pds:file_area:pds:file_area_observational_supplemental::has_tagged_data_object::1.0 rdf:type rdf:Property;
  rdfs:label "has_tagged_data_object";
  rdfs:domain pds4:urn:nasa:pds:0001_nasa_pds_1:pds:file_area:pds:file_area_observational_supplemental::1.0;
  rdfs:range pds4:urn:nasa:pds:0001_nasa_pds_1:pds:array_3d:pds:array_3d_spectrum::1.0.
 
pds4:urn:nasa:pds:0001_nasa_pds_1:pds:file_area:pds:file_area_observational_supplemental::has_tagged_data_object::1.0 rdf:type rdf:Property;
  rdfs:label "has_tagged_data_object";
  rdfs:domain pds4:urn:nasa:pds:0001_nasa_pds_1:pds:file_area:pds:file_area_observational_supplemental::1.0;
  rdfs:range pds4:urn:nasa:pds:0001_nasa_pds_1:pds:encoded_byte_stream:pds:encoded_binary::1.0.
 
pds4:urn:nasa:pds:0001_nasa_pds_1:pds:file_area:pds:file_area_observational_supplemental::has_tagged_data_object::1.0 rdf:type rdf:Property;
  rdfs:label "has_tagged_data_object";
  rdfs:domain pds4:urn:nasa:pds:0001_nasa_pds_1:pds:file_area:pds:file_area_observational_supplemental::1.0;
  rdfs:range pds4:urn:nasa:pds:0001_nasa_pds_1:pds:byte_stream:pds:encoded_byte_stream::1.0.
 
pds4:urn:nasa:pds:0001_nasa_pds_1:pds:file_area:pds:file_area_observational_supplemental::has_tagged_data_object::1.0 rdf:type rdf:Property;
  rdfs:label "has_tagged_data_object";
  rdfs:domain pds4:urn:nasa:pds:0001_nasa_pds_1:pds:file_area:pds:file_area_observational_supplemental::1.0;
  rdfs:range pds4:urn:nasa:pds:0001_nasa_pds_1:pds:encoded_byte_stream:pds:encoded_header::1.0.
 
pds4:urn:nasa:pds:0001_nasa_pds_1:pds:file_area:pds:file_area_observational_supplemental::has_tagged_data_object::1.0 rdf:type rdf:Property;
  rdfs:label "has_tagged_data_object";
  rdfs:domain pds4:urn:nasa:pds:0001_nasa_pds_1:pds:file_area:pds:file_area_observational_supplemental::1.0;
  rdfs:range pds4:urn:nasa:pds:0001_nasa_pds_1:pds:encoded_byte_stream:pds:encoded_image::1.0.
 
pds4:urn:nasa:pds:0001_nasa_pds_1:pds:file_area:pds:file_area_observational_supplemental::has_tagged_data_object::1.0 rdf:type rdf:Property;
  rdfs:label "has_tagged_data_object";
  rdfs:domain pds4:urn:nasa:pds:0001_nasa_pds_1:pds:file_area:pds:file_area_observational_supplemental::1.0;
  rdfs:range pds4:urn:nasa:pds:0001_nasa_pds_1:pds:parsable_byte_stream:pds:header::1.0.
 
pds4:urn:nasa:pds:0001_nasa_pds_1:pds:file_area:pds:file_area_observational_supplemental::has_tagged_data_object::1.0 rdf:type rdf:Property;
  rdfs:label "has_tagged_data_object";
  rdfs:domain pds4:urn:nasa:pds:0001_nasa_pds_1:pds:file_area:pds:file_area_observational_supplemental::1.0;
  rdfs:range pds4:urn:nasa:pds:0001_nasa_pds_1:pds:byte_stream:pds:parsable_byte_stream::1.0.
 
pds4:urn:nasa:pds:0001_nasa_pds_1:pds:file_area:pds:file_area_observational_supplemental::has_tagged_data_object::1.0 rdf:type rdf:Property;
  rdfs:label "has_tagged_data_object";
  rdfs:domain pds4:urn:nasa:pds:0001_nasa_pds_1:pds:file_area:pds:file_area_observational_supplemental::1.0;
  rdfs:range pds4:urn:nasa:pds:0001_nasa_pds_1:pds:parsable_byte_stream:pds:stream_text::1.0.
 
pds4:urn:nasa:pds:0001_nasa_pds_1:pds:file_area:pds:file_area_observational_supplemental::has_tagged_data_object::1.0 rdf:type rdf:Property;
  rdfs:label "has_tagged_data_object";
  rdfs:domain pds4:urn:nasa:pds:0001_nasa_pds_1:pds:file_area:pds:file_area_observational_supplemental::1.0;
  rdfs:range pds4:urn:nasa:pds:0001_nasa_pds_1:pds:table_base:pds:table_binary::1.0.
 
pds4:urn:nasa:pds:0001_nasa_pds_1:pds:file_area:pds:file_area_observational_supplemental::has_tagged_data_object::1.0 rdf:type rdf:Property;
  rdfs:label "has_tagged_data_object";
  rdfs:domain pds4:urn:nasa:pds:0001_nasa_pds_1:pds:file_area:pds:file_area_observational_supplemental::1.0;
  rdfs:range pds4:urn:nasa:pds:0001_nasa_pds_1:pds:table_base:pds:table_character::1.0.
 
pds4:urn:nasa:pds:0001_nasa_pds_1:pds:file_area:pds:file_area_observational_supplemental::has_tagged_data_object::1.0 rdf:type rdf:Property;
  rdfs:label "has_tagged_data_object";
  rdfs:domain pds4:urn:nasa:pds:0001_nasa_pds_1:pds:file_area:pds:file_area_observational_supplemental::1.0;
  rdfs:range pds4:urn:nasa:pds:0001_nasa_pds_1:pds:parsable_byte_stream:pds:table_delimited::1.0.
 
pds4:urn:nasa:pds:0001_nasa_pds_1:pds:file_area:pds:file_area_observational_supplemental::has_tagged_data_object::1.0 rdf:type rdf:Property;
  rdfs:label "has_tagged_data_object";
  rdfs:domain pds4:urn:nasa:pds:0001_nasa_pds_1:pds:file_area:pds:file_area_observational_supplemental::1.0;
  rdfs:range pds4:urn:nasa:pds:0001_nasa_pds_1:pds:table_delimited:pds:table_delimited_source_product_external::1.0.
 
pds4:urn:nasa:pds:0001_nasa_pds_1:pds:file_area:pds:file_area_observational_supplemental::has_tagged_data_object::1.0 rdf:type rdf:Property;
  rdfs:label "has_tagged_data_object";
  rdfs:domain pds4:urn:nasa:pds:0001_nasa_pds_1:pds:file_area:pds:file_area_observational_supplemental::1.0;
  rdfs:range pds4:urn:nasa:pds:0001_nasa_pds_1:pds:table_delimited:pds:table_delimited_source_product_internal::1.0.
 
pds4:urn:nasa:pds:0001_nasa_pds_1:pds:file_area:pds:file_area_observational_supplemental::has_composite_structure::1.0 rdf:type rdf:Property;
  rdfs:label "has_composite_structure";
  rdfs:domain pds4:urn:nasa:pds:0001_nasa_pds_1:pds:file_area:pds:file_area_observational_supplemental::1.0;
  rdfs:range pds4:urn:nasa:pds:0001_nasa_pds_1:pds:tagged_digital_object:pds:composite_structure::1.0.
 
pds4:urn:nasa:pds:0001_nasa_pds_1:pds:file_area:pds:file_area_observational_supplemental::has_file::1.0 rdf:type rdf:Property;
  rdfs:label "has_File";
  rdfs:domain pds4:urn:nasa:pds:0001_nasa_pds_1:pds:file_area:pds:file_area_observational_supplemental::1.0;
  rdfs:range pds4:urn:nasa:pds:0001_nasa_pds_1:pds:tagged_digital_object:pds:file::1.0.
 
pds4:urn:nasa:pds:0001_nasa_pds_1:pds:file_area:pds:file_area_sip_deep_archive::has_tagged_data_object::1.0 rdf:type rdf:Property;
  rdfs:label "has_tagged_data_object";
  rdfs:domain pds4:urn:nasa:pds:0001_nasa_pds_1:pds:file_area:pds:file_area_sip_deep_archive::1.0;
  rdfs:range pds4:urn:nasa:pds:0001_nasa_pds_1:pds:table_delimited:pds:manifest_sip_deep_archive::1.0.
 
pds4:urn:nasa:pds:0001_nasa_pds_1:pds:file_area:pds:file_area_sip_deep_archive::has_file::1.0 rdf:type rdf:Property;
  rdfs:label "has_File";
  rdfs:domain pds4:urn:nasa:pds:0001_nasa_pds_1:pds:file_area:pds:file_area_sip_deep_archive::1.0;
  rdfs:range pds4:urn:nasa:pds:0001_nasa_pds_1:pds:tagged_digital_object:pds:file::1.0.
 
pds4:urn:nasa:pds:0001_nasa_pds_1:pds:file_area:pds:file_area_spice_kernel::has_tagged_data_object::1.0 rdf:type rdf:Property;
  rdfs:label "has_tagged_data_object";
  rdfs:domain pds4:urn:nasa:pds:0001_nasa_pds_1:pds:file_area:pds:file_area_spice_kernel::1.0;
  rdfs:range pds4:urn:nasa:pds:0001_nasa_pds_1:pds:parsable_byte_stream:pds:spice_kernel::1.0.
 
pds4:urn:nasa:pds:0001_nasa_pds_1:pds:file_area:pds:file_area_spice_kernel::has_file::1.0 rdf:type rdf:Property;
  rdfs:label "has_File";
  rdfs:domain pds4:urn:nasa:pds:0001_nasa_pds_1:pds:file_area:pds:file_area_spice_kernel::1.0;
  rdfs:range pds4:urn:nasa:pds:0001_nasa_pds_1:pds:tagged_digital_object:pds:file::1.0.
 
pds4:urn:nasa:pds:0001_nasa_pds_1:pds:file_area:pds:file_area_service_description::has_tagged_data_object::1.0 rdf:type rdf:Property;
  rdfs:label "has_tagged_data_object";
  rdfs:domain pds4:urn:nasa:pds:0001_nasa_pds_1:pds:file_area:pds:file_area_service_description::1.0;
  rdfs:range pds4:urn:nasa:pds:0001_nasa_pds_1:pds:parsable_byte_stream:pds:service_description::1.0.
 
pds4:urn:nasa:pds:0001_nasa_pds_1:pds:file_area:pds:file_area_service_description::has_file::1.0 rdf:type rdf:Property;
  rdfs:label "has_File";
  rdfs:domain pds4:urn:nasa:pds:0001_nasa_pds_1:pds:file_area:pds:file_area_service_description::1.0;
  rdfs:range pds4:urn:nasa:pds:0001_nasa_pds_1:pds:tagged_digital_object:pds:file::1.0.
 
pds4:urn:nasa:pds:0001_nasa_pds_1:pds:file_area:pds:file_area_text::has_tagged_data_object::1.0 rdf:type rdf:Property;
  rdfs:label "has_tagged_data_object";
  rdfs:domain pds4:urn:nasa:pds:0001_nasa_pds_1:pds:file_area:pds:file_area_text::1.0;
  rdfs:range pds4:urn:nasa:pds:0001_nasa_pds_1:pds:parsable_byte_stream:pds:stream_text::1.0.
 
pds4:urn:nasa:pds:0001_nasa_pds_1:pds:file_area:pds:file_area_text::has_file::1.0 rdf:type rdf:Property;
  rdfs:label "has_File";
  rdfs:domain pds4:urn:nasa:pds:0001_nasa_pds_1:pds:file_area:pds:file_area_text::1.0;
  rdfs:range pds4:urn:nasa:pds:0001_nasa_pds_1:pds:tagged_digital_object:pds:file::1.0.
 
pds4:urn:nasa:pds:0001_nasa_pds_1:pds:file_area:pds:file_area_transfer_manifest::has_tagged_data_object::1.0 rdf:type rdf:Property;
  rdfs:label "has_tagged_data_object";
  rdfs:domain pds4:urn:nasa:pds:0001_nasa_pds_1:pds:file_area:pds:file_area_transfer_manifest::1.0;
  rdfs:range pds4:urn:nasa:pds:0001_nasa_pds_1:pds:table_character:pds:transfer_manifest::1.0.
 
pds4:urn:nasa:pds:0001_nasa_pds_1:pds:file_area:pds:file_area_transfer_manifest::has_file::1.0 rdf:type rdf:Property;
  rdfs:label "has_File";
  rdfs:domain pds4:urn:nasa:pds:0001_nasa_pds_1:pds:file_area:pds:file_area_transfer_manifest::1.0;
  rdfs:range pds4:urn:nasa:pds:0001_nasa_pds_1:pds:tagged_digital_object:pds:file::1.0.
 
pds4:urn:nasa:pds:0001_nasa_pds_1:pds:file_area:pds:file_area_update::has_tagged_data_object2::1.0 rdf:type rdf:Property;
  rdfs:label "has_tagged_data_object2";
  rdfs:domain pds4:urn:nasa:pds:0001_nasa_pds_1:pds:file_area:pds:file_area_update::1.0;
  rdfs:range pds4:urn:nasa:pds:0001_nasa_pds_1:pds:parsable_byte_stream:pds:header::1.0.
 
pds4:urn:nasa:pds:0001_nasa_pds_1:pds:file_area:pds:file_area_update::has_tagged_data_object::1.0 rdf:type rdf:Property;
  rdfs:label "has_tagged_data_object";
  rdfs:domain pds4:urn:nasa:pds:0001_nasa_pds_1:pds:file_area:pds:file_area_update::1.0;
  rdfs:range pds4:urn:nasa:pds:0001_nasa_pds_1:pds:table_base:pds:table_character::1.0.
 
pds4:urn:nasa:pds:0001_nasa_pds_1:pds:file_area:pds:file_area_update::has_tagged_data_object::1.0 rdf:type rdf:Property;
  rdfs:label "has_tagged_data_object";
  rdfs:domain pds4:urn:nasa:pds:0001_nasa_pds_1:pds:file_area:pds:file_area_update::1.0;
  rdfs:range pds4:urn:nasa:pds:0001_nasa_pds_1:pds:parsable_byte_stream:pds:table_delimited::1.0.
 
pds4:urn:nasa:pds:0001_nasa_pds_1:pds:file_area:pds:file_area_update::has_file::1.0 rdf:type rdf:Property;
  rdfs:label "has_File";
  rdfs:domain pds4:urn:nasa:pds:0001_nasa_pds_1:pds:file_area:pds:file_area_update::1.0;
  rdfs:range pds4:urn:nasa:pds:0001_nasa_pds_1:pds:tagged_digital_object:pds:file::1.0.
 
pds4:urn:nasa:pds:0001_nasa_pds_1:pds:file_area:pds:file_area_xml_schema::has_tagged_data_object::1.0 rdf:type rdf:Property;
  rdfs:label "has_tagged_data_object";
  rdfs:domain pds4:urn:nasa:pds:0001_nasa_pds_1:pds:file_area:pds:file_area_xml_schema::1.0;
  rdfs:range pds4:urn:nasa:pds:0001_nasa_pds_1:pds:parsable_byte_stream:pds:xml_schema::1.0.
 
pds4:urn:nasa:pds:0001_nasa_pds_1:pds:file_area:pds:file_area_xml_schema::has_file::1.0 rdf:type rdf:Property;
  rdfs:label "has_File";
  rdfs:domain pds4:urn:nasa:pds:0001_nasa_pds_1:pds:file_area:pds:file_area_xml_schema::1.0;
  rdfs:range pds4:urn:nasa:pds:0001_nasa_pds_1:pds:tagged_digital_object:pds:file::1.0.
 
pds4:urn:nasa:pds:0001_nasa_pds_1:pds:group:pds:group_field_binary::has_group_field_binary::1.0 rdf:type rdf:Property;
  rdfs:label "has_Group_Field_Binary";
  rdfs:domain pds4:urn:nasa:pds:0001_nasa_pds_1:pds:group:pds:group_field_binary::1.0;
  rdfs:range pds4:urn:nasa:pds:0001_nasa_pds_1:pds:field:pds:field_binary::1.0.
 
pds4:urn:nasa:pds:0001_nasa_pds_1:pds:group:pds:group_field_binary::has_group_field_binary::1.0 rdf:type rdf:Property;
  rdfs:label "has_Group_Field_Binary";
  rdfs:domain pds4:urn:nasa:pds:0001_nasa_pds_1:pds:group:pds:group_field_binary::1.0;
  rdfs:range pds4:urn:nasa:pds:0001_nasa_pds_1:pds:group:pds:group_field_binary::1.0.
 
pds4:urn:nasa:pds:0001_nasa_pds_1:pds:group:pds:group_field_character::has_group_field_character::1.0 rdf:type rdf:Property;
  rdfs:label "has_Group_Field_Character";
  rdfs:domain pds4:urn:nasa:pds:0001_nasa_pds_1:pds:group:pds:group_field_character::1.0;
  rdfs:range pds4:urn:nasa:pds:0001_nasa_pds_1:pds:field:pds:field_character::1.0.
 
pds4:urn:nasa:pds:0001_nasa_pds_1:pds:group:pds:group_field_character::has_group_field_character::1.0 rdf:type rdf:Property;
  rdfs:label "has_Group_Field_Character";
  rdfs:domain pds4:urn:nasa:pds:0001_nasa_pds_1:pds:group:pds:group_field_character::1.0;
  rdfs:range pds4:urn:nasa:pds:0001_nasa_pds_1:pds:group:pds:group_field_character::1.0.
 
pds4:urn:nasa:pds:0001_nasa_pds_1:pds:group:pds:group_field_delimited::has_delimited_field_grouped::1.0 rdf:type rdf:Property;
  rdfs:label "has_Delimited_Field_Grouped";
  rdfs:domain pds4:urn:nasa:pds:0001_nasa_pds_1:pds:group:pds:group_field_delimited::1.0;
  rdfs:range pds4:urn:nasa:pds:0001_nasa_pds_1:pds:field:pds:field_delimited::1.0.
 
pds4:urn:nasa:pds:0001_nasa_pds_1:pds:group:pds:group_field_delimited::has_delimited_field_grouped::1.0 rdf:type rdf:Property;
  rdfs:label "has_Delimited_Field_Grouped";
  rdfs:domain pds4:urn:nasa:pds:0001_nasa_pds_1:pds:group:pds:group_field_delimited::1.0;
  rdfs:range pds4:urn:nasa:pds:0001_nasa_pds_1:pds:group:pds:group_field_delimited::1.0.
 
pds4:urn:nasa:pds:0001_nasa_pds_1:pds:product_components:pds:identification_area::modification_history::1.0 rdf:type rdf:Property;
  rdfs:label "modification_history";
  rdfs:domain pds4:urn:nasa:pds:0001_nasa_pds_1:pds:product_components:pds:identification_area::1.0;
  rdfs:range pds4:urn:nasa:pds:0001_nasa_pds_1:pds:product_components:pds:modification_history::1.0.
 
pds4:urn:nasa:pds:0001_nasa_pds_1:pds:product_components:pds:identification_area::alias_list::1.0 rdf:type rdf:Property;
  rdfs:label "alias_list";
  rdfs:domain pds4:urn:nasa:pds:0001_nasa_pds_1:pds:product_components:pds:identification_area::1.0;
  rdfs:range pds4:urn:nasa:pds:0001_nasa_pds_1:pds:product_components:pds:alias_list::1.0.
 
pds4:urn:nasa:pds:0001_nasa_pds_1:pds:product_components:pds:identification_area::citation_information::1.0 rdf:type rdf:Property;
  rdfs:label "citation_information";
  rdfs:domain pds4:urn:nasa:pds:0001_nasa_pds_1:pds:product_components:pds:identification_area::1.0;
  rdfs:range pds4:urn:nasa:pds:0001_nasa_pds_1:pds:product_components:pds:citation_information::1.0.
 
pds4:urn:nasa:pds:0001_nasa_pds_1:pds:tndo_supplemental:pds:information_package_component::has_transfer_manifest::1.0 rdf:type rdf:Property;
  rdfs:label "has_Transfer_Manifest";
  rdfs:domain pds4:urn:nasa:pds:0001_nasa_pds_1:pds:tndo_supplemental:pds:information_package_component::1.0;
  rdfs:range pds4:urn:nasa:pds:0001_nasa_pds_1:pds:file_area:pds:file_area_transfer_manifest::1.0.
 
pds4:urn:nasa:pds:0001_nasa_pds_1:pds:tndo_supplemental:pds:information_package_component::has_checksum_manifest::1.0 rdf:type rdf:Property;
  rdfs:label "has_Checksum_Manifest";
  rdfs:domain pds4:urn:nasa:pds:0001_nasa_pds_1:pds:tndo_supplemental:pds:information_package_component::1.0;
  rdfs:range pds4:urn:nasa:pds:0001_nasa_pds_1:pds:file_area:pds:file_area_checksum_manifest::1.0.
 
pds4:urn:nasa:pds:0001_nasa_pds_1:pds:tndo_supplemental:pds:information_package_component::internal_reference::1.0 rdf:type rdf:Property;
  rdfs:label "internal_reference";
  rdfs:domain pds4:urn:nasa:pds:0001_nasa_pds_1:pds:tndo_supplemental:pds:information_package_component::1.0;
  rdfs:range pds4:urn:nasa:pds:0001_nasa_pds_1:pds:product_components:pds:internal_reference::1.0.
 
pds4:urn:nasa:pds:0001_nasa_pds_1:pds:tndo_supplemental:pds:information_package_component_deep_archive::internal_reference::1.0 rdf:type rdf:Property;
  rdfs:label "internal_reference";
  rdfs:domain pds4:urn:nasa:pds:0001_nasa_pds_1:pds:tndo_supplemental:pds:information_package_component_deep_archive::1.0;
  rdfs:range pds4:urn:nasa:pds:0001_nasa_pds_1:pds:product_components:pds:internal_reference::1.0.
 
pds4:urn:nasa:pds:0001_nasa_pds_1:pds:tndo_supplemental:pds:information_package_component_deep_archive::has_manifest::1.0 rdf:type rdf:Property;
  rdfs:label "has_manifest";
  rdfs:domain pds4:urn:nasa:pds:0001_nasa_pds_1:pds:tndo_supplemental:pds:information_package_component_deep_archive::1.0;
  rdfs:range pds4:urn:nasa:pds:0001_nasa_pds_1:pds:file_area:pds:file_area_sip_deep_archive::1.0.
 
pds4:urn:nasa:pds:0001_nasa_pds_1:pds:tndo_supplemental:pds:ingest_ldd::local_rule::1.0 rdf:type rdf:Property;
  rdfs:label "local_rule";
  rdfs:domain pds4:urn:nasa:pds:0001_nasa_pds_1:pds:tndo_supplemental:pds:ingest_ldd::1.0;
  rdfs:range pds4:urn:nasa:pds:0001_nasa_pds_1:pds:tndo_supplemental:pds:dd_rule::1.0.
 
pds4:urn:nasa:pds:0001_nasa_pds_1:pds:tndo_supplemental:pds:ingest_ldd::local_class::1.0 rdf:type rdf:Property;
  rdfs:label "local_class";
  rdfs:domain pds4:urn:nasa:pds:0001_nasa_pds_1:pds:tndo_supplemental:pds:ingest_ldd::1.0;
  rdfs:range pds4:urn:nasa:pds:0001_nasa_pds_1:pds:tndo_supplemental:pds:dd_class::1.0.
 
pds4:urn:nasa:pds:0001_nasa_pds_1:pds:tndo_supplemental:pds:ingest_ldd::data_object::1.0 rdf:type rdf:Property;
  rdfs:label "data_object";
  rdfs:domain pds4:urn:nasa:pds:0001_nasa_pds_1:pds:tndo_supplemental:pds:ingest_ldd::1.0;
  rdfs:range pds4:urn:nasa:pds:0001_nasa_pds_1:pds:tndo_context:pds:other::1.0.
 
pds4:urn:nasa:pds:0001_nasa_pds_1:pds:tndo_supplemental:pds:ingest_ldd::local_attribute::1.0 rdf:type rdf:Property;
  rdfs:label "local_attribute";
  rdfs:domain pds4:urn:nasa:pds:0001_nasa_pds_1:pds:tndo_supplemental:pds:ingest_ldd::1.0;
  rdfs:range pds4:urn:nasa:pds:0001_nasa_pds_1:pds:tndo_supplemental:pds:dd_attribute::1.0.
 
pds4:urn:nasa:pds:0001_nasa_pds_1:pds:tndo_supplemental:pds:ingest_ldd::has_property_maps::1.0 rdf:type rdf:Property;
  rdfs:label "has_Property_Maps";
  rdfs:domain pds4:urn:nasa:pds:0001_nasa_pds_1:pds:tndo_supplemental:pds:ingest_ldd::1.0;
  rdfs:range pds4:urn:nasa:pds:0001_nasa_pds_1:pds:tndo_supplemental:pds:property_maps::1.0.
 
pds4:urn:nasa:pds:0001_nasa_pds_1:pds:tndo_context:pds:instrument::data_object::1.0 rdf:type rdf:Property;
  rdfs:label "data_object";
  rdfs:domain pds4:urn:nasa:pds:0001_nasa_pds_1:pds:tndo_context:pds:instrument::1.0;
  rdfs:range pds4:urn:nasa:pds:0001_nasa_pds_1:pds:tndo_context:pds:other::1.0.
 
pds4:urn:nasa:pds:0001_nasa_pds_1:pds:tndo_context:pds:instrument::has_type_list_area::1.0 rdf:type rdf:Property;
  rdfs:label "has_type_list_area";
  rdfs:domain pds4:urn:nasa:pds:0001_nasa_pds_1:pds:tndo_context:pds:instrument::1.0;
  rdfs:range pds4:urn:nasa:pds:0001_nasa_pds_1:pds:tndo_context:pds:type_list_area::1.0.
 
pds4:urn:nasa:pds:0001_nasa_pds_1:pds:tndo_context:pds:instrument_host::data_object::1.0 rdf:type rdf:Property;
  rdfs:label "data_object";
  rdfs:domain pds4:urn:nasa:pds:0001_nasa_pds_1:pds:tndo_context:pds:instrument_host::1.0;
  rdfs:range pds4:urn:nasa:pds:0001_nasa_pds_1:pds:tndo_context:pds:other::1.0.
 
pds4:urn:nasa:pds:0001_nasa_pds_1:pds:tndo_context_pds3:pds:instrument_host_pds3::data_object::1.0 rdf:type rdf:Property;
  rdfs:label "data_object";
  rdfs:domain pds4:urn:nasa:pds:0001_nasa_pds_1:pds:tndo_context_pds3:pds:instrument_host_pds3::1.0;
  rdfs:range pds4:urn:nasa:pds:0001_nasa_pds_1:pds:tndo_context:pds:other::1.0.
 
pds4:urn:nasa:pds:0001_nasa_pds_1:pds:tndo_context_pds3:pds:instrument_pds3::data_object::1.0 rdf:type rdf:Property;
  rdfs:label "data_object";
  rdfs:domain pds4:urn:nasa:pds:0001_nasa_pds_1:pds:tndo_context_pds3:pds:instrument_pds3::1.0;
  rdfs:range pds4:urn:nasa:pds:0001_nasa_pds_1:pds:tndo_context:pds:other::1.0.
 
pds4:urn:nasa:pds:0001_nasa_pds_1:pds:tndo_context:pds:investigation::data_object::1.0 rdf:type rdf:Property;
  rdfs:label "data_object";
  rdfs:domain pds4:urn:nasa:pds:0001_nasa_pds_1:pds:tndo_context:pds:investigation::1.0;
  rdfs:range pds4:urn:nasa:pds:0001_nasa_pds_1:pds:tndo_context:pds:other::1.0.
 
pds4:urn:nasa:pds:0001_nasa_pds_1:pds:product_components:pds:investigation_area::internal_reference::1.0 rdf:type rdf:Property;
  rdfs:label "internal_reference";
  rdfs:domain pds4:urn:nasa:pds:0001_nasa_pds_1:pds:product_components:pds:investigation_area::1.0;
  rdfs:range pds4:urn:nasa:pds:0001_nasa_pds_1:pds:product_components:pds:internal_reference::1.0.
 
pds4:urn:nasa:pds:0001_nasa_pds_1:pds:tndo_context_pds3:pds:mission_pds3::data_object::1.0 rdf:type rdf:Property;
  rdfs:label "data_object";
  rdfs:domain pds4:urn:nasa:pds:0001_nasa_pds_1:pds:tndo_context_pds3:pds:mission_pds3::1.0;
  rdfs:range pds4:urn:nasa:pds:0001_nasa_pds_1:pds:tndo_context:pds:other::1.0.
 
pds4:urn:nasa:pds:0001_nasa_pds_1:pds:product_components:pds:modification_history::modification_detail::1.0 rdf:type rdf:Property;
  rdfs:label "modification_detail";
  rdfs:domain pds4:urn:nasa:pds:0001_nasa_pds_1:pds:product_components:pds:modification_history::1.0;
  rdfs:range pds4:urn:nasa:pds:0001_nasa_pds_1:pds:product_components:pds:modification_detail::1.0.
 
pds4:urn:nasa:pds:0001_nasa_pds_1:pds:tndo_context:pds:node::data_object::1.0 rdf:type rdf:Property;
  rdfs:label "data_object";
  rdfs:domain pds4:urn:nasa:pds:0001_nasa_pds_1:pds:tndo_context:pds:node::1.0;
  rdfs:range pds4:urn:nasa:pds:0001_nasa_pds_1:pds:tndo_context:pds:other::1.0.
 
pds4:urn:nasa:pds:0001_nasa_pds_1:pds:tndo_supplemental:pds:object_statistics::data_object::1.0 rdf:type rdf:Property;
  rdfs:label "data_object";
  rdfs:domain pds4:urn:nasa:pds:0001_nasa_pds_1:pds:tndo_supplemental:pds:object_statistics::1.0;
  rdfs:range pds4:urn:nasa:pds:0001_nasa_pds_1:pds:tndo_context:pds:other::1.0.
 
pds4:urn:nasa:pds:0001_nasa_pds_1:pds:context_area:pds:observation_area::has_investigation_area::1.0 rdf:type rdf:Property;
  rdfs:label "has_investigation_area";
  rdfs:domain pds4:urn:nasa:pds:0001_nasa_pds_1:pds:context_area:pds:observation_area::1.0;
  rdfs:range pds4:urn:nasa:pds:0001_nasa_pds_1:pds:product_components:pds:investigation_area::1.0.
 
pds4:urn:nasa:pds:0001_nasa_pds_1:pds:context_area:pds:observation_area::has_time_coordinates::1.0 rdf:type rdf:Property;
  rdfs:label "has_time_coordinates";
  rdfs:domain pds4:urn:nasa:pds:0001_nasa_pds_1:pds:context_area:pds:observation_area::1.0;
  rdfs:range pds4:urn:nasa:pds:0001_nasa_pds_1:pds:product_components:pds:time_coordinates::1.0.
 
pds4:urn:nasa:pds:0001_nasa_pds_1:pds:context_area:pds:observation_area::has_observing_system::1.0 rdf:type rdf:Property;
  rdfs:label "has_observing_system";
  rdfs:domain pds4:urn:nasa:pds:0001_nasa_pds_1:pds:context_area:pds:observation_area::1.0;
  rdfs:range pds4:urn:nasa:pds:0001_nasa_pds_1:pds:tndo_context:pds:observing_system::1.0.
 
pds4:urn:nasa:pds:0001_nasa_pds_1:pds:context_area:pds:observation_area::has_target_identification::1.0 rdf:type rdf:Property;
  rdfs:label "has_target_identification";
  rdfs:domain pds4:urn:nasa:pds:0001_nasa_pds_1:pds:context_area:pds:observation_area::1.0;
  rdfs:range pds4:urn:nasa:pds:0001_nasa_pds_1:pds:product_components:pds:target_identification::1.0.
 
pds4:urn:nasa:pds:0001_nasa_pds_1:pds:tndo_context:pds:observing_system::data_object::1.0 rdf:type rdf:Property;
  rdfs:label "data_object";
  rdfs:domain pds4:urn:nasa:pds:0001_nasa_pds_1:pds:tndo_context:pds:observing_system::1.0;
  rdfs:range pds4:urn:nasa:pds:0001_nasa_pds_1:pds:tndo_context:pds:other::1.0.
 
pds4:urn:nasa:pds:0001_nasa_pds_1:pds:tndo_context:pds:observing_system::data_object::1.0 rdf:type rdf:Property;
  rdfs:label "data_object";
  rdfs:domain pds4:urn:nasa:pds:0001_nasa_pds_1:pds:tndo_context:pds:observing_system::1.0;
  rdfs:range pds4:urn:nasa:pds:0001_nasa_pds_1:pds:tndo_context:pds:other::1.0.
 
pds4:urn:nasa:pds:0001_nasa_pds_1:pds:tndo_context:pds:observing_system::observing_system_component::1.0 rdf:type rdf:Property;
  rdfs:label "observing_system_component";
  rdfs:domain pds4:urn:nasa:pds:0001_nasa_pds_1:pds:tndo_context:pds:observing_system::1.0;
  rdfs:range pds4:urn:nasa:pds:0001_nasa_pds_1:pds:tagged_nondigital_child:pds:observing_system_component::1.0.
 
pds4:urn:nasa:pds:0001_nasa_pds_1:pds:tagged_nondigital_child:pds:observing_system_component::external_reference::1.0 rdf:type rdf:Property;
  rdfs:label "external_reference";
  rdfs:domain pds4:urn:nasa:pds:0001_nasa_pds_1:pds:tagged_nondigital_child:pds:observing_system_component::1.0;
  rdfs:range pds4:urn:nasa:pds:0001_nasa_pds_1:pds:product_components:pds:external_reference::1.0.
 
pds4:urn:nasa:pds:0001_nasa_pds_1:pds:tagged_nondigital_child:pds:observing_system_component::internal_reference::1.0 rdf:type rdf:Property;
  rdfs:label "internal_reference";
  rdfs:domain pds4:urn:nasa:pds:0001_nasa_pds_1:pds:tagged_nondigital_child:pds:observing_system_component::1.0;
  rdfs:range pds4:urn:nasa:pds:0001_nasa_pds_1:pds:product_components:pds:internal_reference::1.0.
 
pds4:urn:nasa:pds:0001_nasa_pds_1:pds:tndo_context:pds:other::data_object::1.0 rdf:type rdf:Property;
  rdfs:label "data_object";
  rdfs:domain pds4:urn:nasa:pds:0001_nasa_pds_1:pds:tndo_context:pds:other::1.0;
  rdfs:range pds4:urn:nasa:pds:0001_nasa_pds_1:pds:tndo_context:pds:other::1.0.
 
pds4:urn:nasa:pds:0001_nasa_pds_1:pds:tndo_context:pds:pds_affiliate::data_object::1.0 rdf:type rdf:Property;
  rdfs:label "data_object";
  rdfs:domain pds4:urn:nasa:pds:0001_nasa_pds_1:pds:tndo_context:pds:pds_affiliate::1.0;
  rdfs:range pds4:urn:nasa:pds:0001_nasa_pds_1:pds:tndo_context:pds:other::1.0.
 
pds4:urn:nasa:pds:0001_nasa_pds_1:pds:tndo_context:pds:pds_guest::data_object::1.0 rdf:type rdf:Property;
  rdfs:label "data_object";
  rdfs:domain pds4:urn:nasa:pds:0001_nasa_pds_1:pds:tndo_context:pds:pds_guest::1.0;
  rdfs:range pds4:urn:nasa:pds:0001_nasa_pds_1:pds:tndo_context:pds:other::1.0.
 
pds4:urn:nasa:pds:0001_nasa_pds_1:pds:tagged_digital_child:pds:packed_data_fields::has_field_bit::1.0 rdf:type rdf:Property;
  rdfs:label "has_Field_Bit";
  rdfs:domain pds4:urn:nasa:pds:0001_nasa_pds_1:pds:tagged_digital_child:pds:packed_data_fields::1.0;
  rdfs:range pds4:urn:nasa:pds:0001_nasa_pds_1:pds:field:pds:field_bit::1.0.
 
pds4:urn:nasa:pds:0001_nasa_pds_1:pds:byte_stream:pds:parsable_byte_stream::data_object::1.0 rdf:type rdf:Property;
  rdfs:label "data_object";
  rdfs:domain pds4:urn:nasa:pds:0001_nasa_pds_1:pds:byte_stream:pds:parsable_byte_stream::1.0;
  rdfs:range pds4:urn:nasa:pds:0001_nasa_pds_1:pds:tndo_context:pds:other::1.0.
 
pds4:urn:nasa:pds:0001_nasa_pds_1:pds:product_components:pds:primary_result_summary::has_science_facet::1.0 rdf:type rdf:Property;
  rdfs:label "has_Science_Facet";
  rdfs:domain pds4:urn:nasa:pds:0001_nasa_pds_1:pds:product_components:pds:primary_result_summary::1.0;
  rdfs:range pds4:urn:nasa:pds:0001_nasa_pds_1:pds:product_components:pds:science_facets::1.0.
 
pds4:urn:nasa:pds:0001_nasa_pds_1:all:user:pds:product::has_identification_area::1.0 rdf:type rdf:Property;
  rdfs:label "has_identification_area";
  rdfs:domain pds4:urn:nasa:pds:0001_nasa_pds_1:all:user:pds:product::1.0;
  rdfs:range pds4:urn:nasa:pds:0001_nasa_pds_1:pds:product_components:pds:identification_area::1.0.
 
pds4:urn:nasa:pds:0001_nasa_pds_1:pds:product:pds:product_aip::reference_list::1.0 rdf:type rdf:Property;
  rdfs:label "reference_list";
  rdfs:domain pds4:urn:nasa:pds:0001_nasa_pds_1:pds:product:pds:product_aip::1.0;
  rdfs:range pds4:urn:nasa:pds:0001_nasa_pds_1:pds:product_components:pds:reference_list::1.0.
 
pds4:urn:nasa:pds:0001_nasa_pds_1:pds:product:pds:product_aip::has_information_package_component::1.0 rdf:type rdf:Property;
  rdfs:label "has_Information_Package_Component";
  rdfs:domain pds4:urn:nasa:pds:0001_nasa_pds_1:pds:product:pds:product_aip::1.0;
  rdfs:range pds4:urn:nasa:pds:0001_nasa_pds_1:pds:tndo_supplemental:pds:information_package_component::1.0.
 
pds4:urn:nasa:pds:0001_nasa_pds_1:pds:product:pds:product_aip::product_data_object::1.0 rdf:type rdf:Property;
  rdfs:label "product_data_object";
  rdfs:domain pds4:urn:nasa:pds:0001_nasa_pds_1:pds:product:pds:product_aip::1.0;
  rdfs:range pds4:urn:nasa:pds:0001_nasa_pds_1:pds:information_package:pds:archival_information_package::1.0.
 
pds4:urn:nasa:pds:0001_nasa_pds_1:pds:product:pds:product_ancillary::context_area::1.0 rdf:type rdf:Property;
  rdfs:label "context_area";
  rdfs:domain pds4:urn:nasa:pds:0001_nasa_pds_1:pds:product:pds:product_ancillary::1.0;
  rdfs:range pds4:urn:nasa:pds:0001_nasa_pds_1:pds:product_components:pds:context_area::1.0.
 
pds4:urn:nasa:pds:0001_nasa_pds_1:pds:product:pds:product_ancillary::reference_list::1.0 rdf:type rdf:Property;
  rdfs:label "reference_list";
  rdfs:domain pds4:urn:nasa:pds:0001_nasa_pds_1:pds:product:pds:product_ancillary::1.0;
  rdfs:range pds4:urn:nasa:pds:0001_nasa_pds_1:pds:product_components:pds:reference_list::1.0.
 
pds4:urn:nasa:pds:0001_nasa_pds_1:pds:product:pds:product_ancillary::file_area::1.0 rdf:type rdf:Property;
  rdfs:label "file_area";
  rdfs:domain pds4:urn:nasa:pds:0001_nasa_pds_1:pds:product:pds:product_ancillary::1.0;
  rdfs:range pds4:urn:nasa:pds:0001_nasa_pds_1:pds:file_area:pds:file_area_ancillary::1.0.
 
pds4:urn:nasa:pds:0001_nasa_pds_1:pds:product:pds:product_attribute_definition::reference_list::1.0 rdf:type rdf:Property;
  rdfs:label "reference_list";
  rdfs:domain pds4:urn:nasa:pds:0001_nasa_pds_1:pds:product:pds:product_attribute_definition::1.0;
  rdfs:range pds4:urn:nasa:pds:0001_nasa_pds_1:pds:product_components:pds:reference_list::1.0.
 
pds4:urn:nasa:pds:0001_nasa_pds_1:pds:product:pds:product_attribute_definition::product_data_object::1.0 rdf:type rdf:Property;
  rdfs:label "product_data_object";
  rdfs:domain pds4:urn:nasa:pds:0001_nasa_pds_1:pds:product:pds:product_attribute_definition::1.0;
  rdfs:range pds4:urn:nasa:pds:0001_nasa_pds_1:pds:tndo_supplemental:pds:dd_attribute_full::1.0.
 
pds4:urn:nasa:pds:0001_nasa_pds_1:pds:product:pds:product_browse::context_area::1.0 rdf:type rdf:Property;
  rdfs:label "context_area";
  rdfs:domain pds4:urn:nasa:pds:0001_nasa_pds_1:pds:product:pds:product_browse::1.0;
  rdfs:range pds4:urn:nasa:pds:0001_nasa_pds_1:pds:product_components:pds:context_area::1.0.
 
pds4:urn:nasa:pds:0001_nasa_pds_1:pds:product:pds:product_browse::reference_list::1.0 rdf:type rdf:Property;
  rdfs:label "reference_list";
  rdfs:domain pds4:urn:nasa:pds:0001_nasa_pds_1:pds:product:pds:product_browse::1.0;
  rdfs:range pds4:urn:nasa:pds:0001_nasa_pds_1:pds:product_components:pds:reference_list::1.0.
 
pds4:urn:nasa:pds:0001_nasa_pds_1:pds:product:pds:product_browse::file_area::1.0 rdf:type rdf:Property;
  rdfs:label "file_area";
  rdfs:domain pds4:urn:nasa:pds:0001_nasa_pds_1:pds:product:pds:product_browse::1.0;
  rdfs:range pds4:urn:nasa:pds:0001_nasa_pds_1:pds:file_area:pds:file_area_browse::1.0.
 
pds4:urn:nasa:pds:0001_nasa_pds_1:pds:product:pds:product_bundle::context_area::1.0 rdf:type rdf:Property;
  rdfs:label "context_area";
  rdfs:domain pds4:urn:nasa:pds:0001_nasa_pds_1:pds:product:pds:product_bundle::1.0;
  rdfs:range pds4:urn:nasa:pds:0001_nasa_pds_1:pds:product_components:pds:context_area::1.0.
 
pds4:urn:nasa:pds:0001_nasa_pds_1:pds:product:pds:product_bundle::member_entry::1.0 rdf:type rdf:Property;
  rdfs:label "member_entry";
  rdfs:domain pds4:urn:nasa:pds:0001_nasa_pds_1:pds:product:pds:product_bundle::1.0;
  rdfs:range pds4:urn:nasa:pds:0001_nasa_pds_1:pds:product_components:pds:bundle_member_entry::1.0.
 
pds4:urn:nasa:pds:0001_nasa_pds_1:pds:product:pds:product_bundle::reference_list::1.0 rdf:type rdf:Property;
  rdfs:label "reference_list";
  rdfs:domain pds4:urn:nasa:pds:0001_nasa_pds_1:pds:product:pds:product_bundle::1.0;
  rdfs:range pds4:urn:nasa:pds:0001_nasa_pds_1:pds:product_components:pds:reference_list::1.0.
 
pds4:urn:nasa:pds:0001_nasa_pds_1:pds:product:pds:product_bundle::file_area::1.0 rdf:type rdf:Property;
  rdfs:label "file_area";
  rdfs:domain pds4:urn:nasa:pds:0001_nasa_pds_1:pds:product:pds:product_bundle::1.0;
  rdfs:range pds4:urn:nasa:pds:0001_nasa_pds_1:pds:file_area:pds:file_area_text::1.0.
 
pds4:urn:nasa:pds:0001_nasa_pds_1:pds:product:pds:product_bundle::product_data_object::1.0 rdf:type rdf:Property;
  rdfs:label "product_data_object";
  rdfs:domain pds4:urn:nasa:pds:0001_nasa_pds_1:pds:product:pds:product_bundle::1.0;
  rdfs:range pds4:urn:nasa:pds:0001_nasa_pds_1:pds:tndo_supplemental:pds:bundle::1.0.
 
pds4:urn:nasa:pds:0001_nasa_pds_1:pds:product:pds:product_class_definition::reference_list::1.0 rdf:type rdf:Property;
  rdfs:label "reference_list";
  rdfs:domain pds4:urn:nasa:pds:0001_nasa_pds_1:pds:product:pds:product_class_definition::1.0;
  rdfs:range pds4:urn:nasa:pds:0001_nasa_pds_1:pds:product_components:pds:reference_list::1.0.
 
pds4:urn:nasa:pds:0001_nasa_pds_1:pds:product:pds:product_class_definition::product_data_object::1.0 rdf:type rdf:Property;
  rdfs:label "product_data_object";
  rdfs:domain pds4:urn:nasa:pds:0001_nasa_pds_1:pds:product:pds:product_class_definition::1.0;
  rdfs:range pds4:urn:nasa:pds:0001_nasa_pds_1:pds:tndo_supplemental:pds:dd_class_full::1.0.
 
pds4:urn:nasa:pds:0001_nasa_pds_1:pds:product:pds:product_collection::context_area::1.0 rdf:type rdf:Property;
  rdfs:label "context_area";
  rdfs:domain pds4:urn:nasa:pds:0001_nasa_pds_1:pds:product:pds:product_collection::1.0;
  rdfs:range pds4:urn:nasa:pds:0001_nasa_pds_1:pds:product_components:pds:context_area::1.0.
 
pds4:urn:nasa:pds:0001_nasa_pds_1:pds:product:pds:product_collection::reference_list::1.0 rdf:type rdf:Property;
  rdfs:label "reference_list";
  rdfs:domain pds4:urn:nasa:pds:0001_nasa_pds_1:pds:product:pds:product_collection::1.0;
  rdfs:range pds4:urn:nasa:pds:0001_nasa_pds_1:pds:product_components:pds:reference_list::1.0.
 
pds4:urn:nasa:pds:0001_nasa_pds_1:pds:product:pds:product_collection::product_data_object::1.0 rdf:type rdf:Property;
  rdfs:label "product_data_object";
  rdfs:domain pds4:urn:nasa:pds:0001_nasa_pds_1:pds:product:pds:product_collection::1.0;
  rdfs:range pds4:urn:nasa:pds:0001_nasa_pds_1:pds:tndo_supplemental:pds:collection::1.0.
 
pds4:urn:nasa:pds:0001_nasa_pds_1:pds:product:pds:product_collection::file_area_inventory::1.0 rdf:type rdf:Property;
  rdfs:label "file_area_inventory";
  rdfs:domain pds4:urn:nasa:pds:0001_nasa_pds_1:pds:product:pds:product_collection::1.0;
  rdfs:range pds4:urn:nasa:pds:0001_nasa_pds_1:pds:file_area:pds:file_area_inventory::1.0.
 
pds4:urn:nasa:pds:0001_nasa_pds_1:pds:product:pds:product_context::reference_list::1.0 rdf:type rdf:Property;
  rdfs:label "reference_list";
  rdfs:domain pds4:urn:nasa:pds:0001_nasa_pds_1:pds:product:pds:product_context::1.0;
  rdfs:range pds4:urn:nasa:pds:0001_nasa_pds_1:pds:product_components:pds:reference_list::1.0.
 
pds4:urn:nasa:pds:0001_nasa_pds_1:pds:product:pds:product_context::product_data_object::1.0 rdf:type rdf:Property;
  rdfs:label "product_data_object";
  rdfs:domain pds4:urn:nasa:pds:0001_nasa_pds_1:pds:product:pds:product_context::1.0;
  rdfs:range pds4:urn:nasa:pds:0001_nasa_pds_1:pds:tndo_context:pds:agency::1.0.
 
pds4:urn:nasa:pds:0001_nasa_pds_1:pds:product:pds:product_context::product_data_object::1.0 rdf:type rdf:Property;
  rdfs:label "product_data_object";
  rdfs:domain pds4:urn:nasa:pds:0001_nasa_pds_1:pds:product:pds:product_context::1.0;
  rdfs:range pds4:urn:nasa:pds:0001_nasa_pds_1:pds:tndo_context:pds:airborne::1.0.
 
pds4:urn:nasa:pds:0001_nasa_pds_1:pds:product:pds:product_context::product_data_object::1.0 rdf:type rdf:Property;
  rdfs:label "product_data_object";
  rdfs:domain pds4:urn:nasa:pds:0001_nasa_pds_1:pds:product:pds:product_context::1.0;
  rdfs:range pds4:urn:nasa:pds:0001_nasa_pds_1:pds:tndo_context:pds:facility::1.0.
 
pds4:urn:nasa:pds:0001_nasa_pds_1:pds:product:pds:product_context::product_data_object::1.0 rdf:type rdf:Property;
  rdfs:label "product_data_object";
  rdfs:domain pds4:urn:nasa:pds:0001_nasa_pds_1:pds:product:pds:product_context::1.0;
  rdfs:range pds4:urn:nasa:pds:0001_nasa_pds_1:pds:tndo_context:pds:instrument::1.0.
 
pds4:urn:nasa:pds:0001_nasa_pds_1:pds:product:pds:product_context::product_data_object::1.0 rdf:type rdf:Property;
  rdfs:label "product_data_object";
  rdfs:domain pds4:urn:nasa:pds:0001_nasa_pds_1:pds:product:pds:product_context::1.0;
  rdfs:range pds4:urn:nasa:pds:0001_nasa_pds_1:pds:tndo_context:pds:instrument_host::1.0.
 
pds4:urn:nasa:pds:0001_nasa_pds_1:pds:product:pds:product_context::product_data_object::1.0 rdf:type rdf:Property;
  rdfs:label "product_data_object";
  rdfs:domain pds4:urn:nasa:pds:0001_nasa_pds_1:pds:product:pds:product_context::1.0;
  rdfs:range pds4:urn:nasa:pds:0001_nasa_pds_1:pds:tndo_context:pds:investigation::1.0.
 
pds4:urn:nasa:pds:0001_nasa_pds_1:pds:product:pds:product_context::product_data_object::1.0 rdf:type rdf:Property;
  rdfs:label "product_data_object";
  rdfs:domain pds4:urn:nasa:pds:0001_nasa_pds_1:pds:product:pds:product_context::1.0;
  rdfs:range pds4:urn:nasa:pds:0001_nasa_pds_1:pds:tndo_context:pds:node::1.0.
 
pds4:urn:nasa:pds:0001_nasa_pds_1:pds:product:pds:product_context::product_data_object::1.0 rdf:type rdf:Property;
  rdfs:label "product_data_object";
  rdfs:domain pds4:urn:nasa:pds:0001_nasa_pds_1:pds:product:pds:product_context::1.0;
  rdfs:range pds4:urn:nasa:pds:0001_nasa_pds_1:pds:tndo_context:pds:other::1.0.
 
pds4:urn:nasa:pds:0001_nasa_pds_1:pds:product:pds:product_context::product_data_object::1.0 rdf:type rdf:Property;
  rdfs:label "product_data_object";
  rdfs:domain pds4:urn:nasa:pds:0001_nasa_pds_1:pds:product:pds:product_context::1.0;
  rdfs:range pds4:urn:nasa:pds:0001_nasa_pds_1:pds:tndo_context:pds:pds_affiliate::1.0.
 
pds4:urn:nasa:pds:0001_nasa_pds_1:pds:product:pds:product_context::product_data_object::1.0 rdf:type rdf:Property;
  rdfs:label "product_data_object";
  rdfs:domain pds4:urn:nasa:pds:0001_nasa_pds_1:pds:product:pds:product_context::1.0;
  rdfs:range pds4:urn:nasa:pds:0001_nasa_pds_1:pds:tndo_context:pds:pds_guest::1.0.
 
pds4:urn:nasa:pds:0001_nasa_pds_1:pds:product:pds:product_context::product_data_object::1.0 rdf:type rdf:Property;
  rdfs:label "product_data_object";
  rdfs:domain pds4:urn:nasa:pds:0001_nasa_pds_1:pds:product:pds:product_context::1.0;
  rdfs:range pds4:urn:nasa:pds:0001_nasa_pds_1:pds:tndo_context:pds:resource::1.0.
 
pds4:urn:nasa:pds:0001_nasa_pds_1:pds:product:pds:product_context::product_data_object::1.0 rdf:type rdf:Property;
  rdfs:label "product_data_object";
  rdfs:domain pds4:urn:nasa:pds:0001_nasa_pds_1:pds:product:pds:product_context::1.0;
  rdfs:range pds4:urn:nasa:pds:0001_nasa_pds_1:pds:tndo_context:pds:target::1.0.
 
pds4:urn:nasa:pds:0001_nasa_pds_1:pds:product:pds:product_context::product_data_object::1.0 rdf:type rdf:Property;
  rdfs:label "product_data_object";
  rdfs:domain pds4:urn:nasa:pds:0001_nasa_pds_1:pds:product:pds:product_context::1.0;
  rdfs:range pds4:urn:nasa:pds:0001_nasa_pds_1:pds:tndo_context:pds:telescope::1.0.
 
pds4:urn:nasa:pds:0001_nasa_pds_1:pds:product:pds:product_context::has_discipline_area::1.0 rdf:type rdf:Property;
  rdfs:label "has_discipline_area";
  rdfs:domain pds4:urn:nasa:pds:0001_nasa_pds_1:pds:product:pds:product_context::1.0;
  rdfs:range pds4:urn:nasa:pds:0001_nasa_pds_1:pds:product_components:pds:discipline_area::1.0.
 
pds4:urn:nasa:pds:0001_nasa_pds_1:pds:product:pds:product_dip::reference_list::1.0 rdf:type rdf:Property;
  rdfs:label "reference_list";
  rdfs:domain pds4:urn:nasa:pds:0001_nasa_pds_1:pds:product:pds:product_dip::1.0;
  rdfs:range pds4:urn:nasa:pds:0001_nasa_pds_1:pds:product_components:pds:reference_list::1.0.
 
pds4:urn:nasa:pds:0001_nasa_pds_1:pds:product:pds:product_dip::has_information_package_component::1.0 rdf:type rdf:Property;
  rdfs:label "has_Information_Package_Component";
  rdfs:domain pds4:urn:nasa:pds:0001_nasa_pds_1:pds:product:pds:product_dip::1.0;
  rdfs:range pds4:urn:nasa:pds:0001_nasa_pds_1:pds:tndo_supplemental:pds:information_package_component::1.0.
 
pds4:urn:nasa:pds:0001_nasa_pds_1:pds:product:pds:product_dip::product_data_object::1.0 rdf:type rdf:Property;
  rdfs:label "product_data_object";
  rdfs:domain pds4:urn:nasa:pds:0001_nasa_pds_1:pds:product:pds:product_dip::1.0;
  rdfs:range pds4:urn:nasa:pds:0001_nasa_pds_1:pds:information_package:pds:dissemination_information_package::1.0.
 
pds4:urn:nasa:pds:0001_nasa_pds_1:pds:product:pds:product_dip_deep_archive::reference_list::1.0 rdf:type rdf:Property;
  rdfs:label "reference_list";
  rdfs:domain pds4:urn:nasa:pds:0001_nasa_pds_1:pds:product:pds:product_dip_deep_archive::1.0;
  rdfs:range pds4:urn:nasa:pds:0001_nasa_pds_1:pds:product_components:pds:reference_list::1.0.
 
pds4:urn:nasa:pds:0001_nasa_pds_1:pds:product:pds:product_dip_deep_archive::has_information_package_component::1.0 rdf:type rdf:Property;
  rdfs:label "has_Information_Package_Component";
  rdfs:domain pds4:urn:nasa:pds:0001_nasa_pds_1:pds:product:pds:product_dip_deep_archive::1.0;
  rdfs:range pds4:urn:nasa:pds:0001_nasa_pds_1:pds:tndo_supplemental:pds:information_package_component::1.0.
 
pds4:urn:nasa:pds:0001_nasa_pds_1:pds:product:pds:product_dip_deep_archive::product_data_object::1.0 rdf:type rdf:Property;
  rdfs:label "product_data_object";
  rdfs:domain pds4:urn:nasa:pds:0001_nasa_pds_1:pds:product:pds:product_dip_deep_archive::1.0;
  rdfs:range pds4:urn:nasa:pds:0001_nasa_pds_1:pds:information_package:pds:dip_deep_archive::1.0.
 
pds4:urn:nasa:pds:0001_nasa_pds_1:pds:product:pds:product_data_set_pds3::reference_list::1.0 rdf:type rdf:Property;
  rdfs:label "reference_list";
  rdfs:domain pds4:urn:nasa:pds:0001_nasa_pds_1:pds:product:pds:product_data_set_pds3::1.0;
  rdfs:range pds4:urn:nasa:pds:0001_nasa_pds_1:pds:product_components:pds:reference_list::1.0.
 
pds4:urn:nasa:pds:0001_nasa_pds_1:pds:product:pds:product_data_set_pds3::product_data_object::1.0 rdf:type rdf:Property;
  rdfs:label "product_data_object";
  rdfs:domain pds4:urn:nasa:pds:0001_nasa_pds_1:pds:product:pds:product_data_set_pds3::1.0;
  rdfs:range pds4:urn:nasa:pds:0001_nasa_pds_1:pds:tndo_context_pds3:pds:data_set_pds3::1.0.
 
pds4:urn:nasa:pds:0001_nasa_pds_1:pds:product:pds:product_document::context_area::1.0 rdf:type rdf:Property;
  rdfs:label "context_area";
  rdfs:domain pds4:urn:nasa:pds:0001_nasa_pds_1:pds:product:pds:product_document::1.0;
  rdfs:range pds4:urn:nasa:pds:0001_nasa_pds_1:pds:product_components:pds:context_area::1.0.
 
pds4:urn:nasa:pds:0001_nasa_pds_1:pds:product:pds:product_document::reference_list::1.0 rdf:type rdf:Property;
  rdfs:label "reference_list";
  rdfs:domain pds4:urn:nasa:pds:0001_nasa_pds_1:pds:product:pds:product_document::1.0;
  rdfs:range pds4:urn:nasa:pds:0001_nasa_pds_1:pds:product_components:pds:reference_list::1.0.
 
pds4:urn:nasa:pds:0001_nasa_pds_1:pds:product:pds:product_document::has_document::1.0 rdf:type rdf:Property;
  rdfs:label "has_document";
  rdfs:domain pds4:urn:nasa:pds:0001_nasa_pds_1:pds:product:pds:product_document::1.0;
  rdfs:range pds4:urn:nasa:pds:0001_nasa_pds_1:pds:tndo_supplemental:pds:document::1.0.
 
pds4:urn:nasa:pds:0001_nasa_pds_1:pds:product:pds:product_file_repository::reference_list::1.0 rdf:type rdf:Property;
  rdfs:label "reference_list";
  rdfs:domain pds4:urn:nasa:pds:0001_nasa_pds_1:pds:product:pds:product_file_repository::1.0;
  rdfs:range pds4:urn:nasa:pds:0001_nasa_pds_1:pds:product_components:pds:reference_list::1.0.
 
pds4:urn:nasa:pds:0001_nasa_pds_1:pds:product:pds:product_file_repository::file_area::1.0 rdf:type rdf:Property;
  rdfs:label "file_area";
  rdfs:domain pds4:urn:nasa:pds:0001_nasa_pds_1:pds:product:pds:product_file_repository::1.0;
  rdfs:range pds4:urn:nasa:pds:0001_nasa_pds_1:pds:file_area:pds:file_area_binary::1.0.
 
pds4:urn:nasa:pds:0001_nasa_pds_1:pds:product:pds:product_file_text::reference_list::1.0 rdf:type rdf:Property;
  rdfs:label "reference_list";
  rdfs:domain pds4:urn:nasa:pds:0001_nasa_pds_1:pds:product:pds:product_file_text::1.0;
  rdfs:range pds4:urn:nasa:pds:0001_nasa_pds_1:pds:product_components:pds:reference_list::1.0.
 
pds4:urn:nasa:pds:0001_nasa_pds_1:pds:product:pds:product_file_text::file_area::1.0 rdf:type rdf:Property;
  rdfs:label "file_area";
  rdfs:domain pds4:urn:nasa:pds:0001_nasa_pds_1:pds:product:pds:product_file_text::1.0;
  rdfs:range pds4:urn:nasa:pds:0001_nasa_pds_1:pds:file_area:pds:file_area_text::1.0.
 
pds4:urn:nasa:pds:0001_nasa_pds_1:pds:product:pds:product_instrument_host_pds3::reference_list::1.0 rdf:type rdf:Property;
  rdfs:label "reference_list";
  rdfs:domain pds4:urn:nasa:pds:0001_nasa_pds_1:pds:product:pds:product_instrument_host_pds3::1.0;
  rdfs:range pds4:urn:nasa:pds:0001_nasa_pds_1:pds:product_components:pds:reference_list::1.0.
 
pds4:urn:nasa:pds:0001_nasa_pds_1:pds:product:pds:product_instrument_host_pds3::product_data_object::1.0 rdf:type rdf:Property;
  rdfs:label "product_data_object";
  rdfs:domain pds4:urn:nasa:pds:0001_nasa_pds_1:pds:product:pds:product_instrument_host_pds3::1.0;
  rdfs:range pds4:urn:nasa:pds:0001_nasa_pds_1:pds:tndo_context_pds3:pds:instrument_host_pds3::1.0.
 
pds4:urn:nasa:pds:0001_nasa_pds_1:pds:product:pds:product_instrument_pds3::reference_list::1.0 rdf:type rdf:Property;
  rdfs:label "reference_list";
  rdfs:domain pds4:urn:nasa:pds:0001_nasa_pds_1:pds:product:pds:product_instrument_pds3::1.0;
  rdfs:range pds4:urn:nasa:pds:0001_nasa_pds_1:pds:product_components:pds:reference_list::1.0.
 
pds4:urn:nasa:pds:0001_nasa_pds_1:pds:product:pds:product_instrument_pds3::product_data_object::1.0 rdf:type rdf:Property;
  rdfs:label "product_data_object";
  rdfs:domain pds4:urn:nasa:pds:0001_nasa_pds_1:pds:product:pds:product_instrument_pds3::1.0;
  rdfs:range pds4:urn:nasa:pds:0001_nasa_pds_1:pds:tndo_context_pds3:pds:instrument_pds3::1.0.
 
pds4:urn:nasa:pds:0001_nasa_pds_1:pds:product:pds:product_metadata_supplemental::reference_list::1.0 rdf:type rdf:Property;
  rdfs:label "reference_list";
  rdfs:domain pds4:urn:nasa:pds:0001_nasa_pds_1:pds:product:pds:product_metadata_supplemental::1.0;
  rdfs:range pds4:urn:nasa:pds:0001_nasa_pds_1:pds:product_components:pds:reference_list::1.0.
 
pds4:urn:nasa:pds:0001_nasa_pds_1:pds:product:pds:product_metadata_supplemental::file_area::1.0 rdf:type rdf:Property;
  rdfs:label "file_area";
  rdfs:domain pds4:urn:nasa:pds:0001_nasa_pds_1:pds:product:pds:product_metadata_supplemental::1.0;
  rdfs:range pds4:urn:nasa:pds:0001_nasa_pds_1:pds:file_area:pds:file_area_metadata::1.0.
 
pds4:urn:nasa:pds:0001_nasa_pds_1:pds:product:pds:product_mission_pds3::reference_list::1.0 rdf:type rdf:Property;
  rdfs:label "reference_list";
  rdfs:domain pds4:urn:nasa:pds:0001_nasa_pds_1:pds:product:pds:product_mission_pds3::1.0;
  rdfs:range pds4:urn:nasa:pds:0001_nasa_pds_1:pds:product_components:pds:reference_list::1.0.
 
pds4:urn:nasa:pds:0001_nasa_pds_1:pds:product:pds:product_mission_pds3::product_data_object::1.0 rdf:type rdf:Property;
  rdfs:label "product_data_object";
  rdfs:domain pds4:urn:nasa:pds:0001_nasa_pds_1:pds:product:pds:product_mission_pds3::1.0;
  rdfs:range pds4:urn:nasa:pds:0001_nasa_pds_1:pds:tndo_context_pds3:pds:mission_pds3::1.0.
 
pds4:urn:nasa:pds:0001_nasa_pds_1:pds:product:pds:product_native::context_area::1.0 rdf:type rdf:Property;
  rdfs:label "context_area";
  rdfs:domain pds4:urn:nasa:pds:0001_nasa_pds_1:pds:product:pds:product_native::1.0;
  rdfs:range pds4:urn:nasa:pds:0001_nasa_pds_1:pds:product_components:pds:context_area::1.0.
 
pds4:urn:nasa:pds:0001_nasa_pds_1:pds:product:pds:product_native::reference_list::1.0 rdf:type rdf:Property;
  rdfs:label "reference_list";
  rdfs:domain pds4:urn:nasa:pds:0001_nasa_pds_1:pds:product:pds:product_native::1.0;
  rdfs:range pds4:urn:nasa:pds:0001_nasa_pds_1:pds:product_components:pds:reference_list::1.0.
 
pds4:urn:nasa:pds:0001_nasa_pds_1:pds:product:pds:product_native::file_area::1.0 rdf:type rdf:Property;
  rdfs:label "file_area";
  rdfs:domain pds4:urn:nasa:pds:0001_nasa_pds_1:pds:product:pds:product_native::1.0;
  rdfs:range pds4:urn:nasa:pds:0001_nasa_pds_1:pds:file_area:pds:file_area_native::1.0.
 
pds4:urn:nasa:pds:0001_nasa_pds_1:pds:product:pds:product_observational::reference_list::1.0 rdf:type rdf:Property;
  rdfs:label "reference_list";
  rdfs:domain pds4:urn:nasa:pds:0001_nasa_pds_1:pds:product:pds:product_observational::1.0;
  rdfs:range pds4:urn:nasa:pds:0001_nasa_pds_1:pds:product_components:pds:reference_list::1.0.
 
pds4:urn:nasa:pds:0001_nasa_pds_1:pds:product:pds:product_observational::file_area::1.0 rdf:type rdf:Property;
  rdfs:label "file_area";
  rdfs:domain pds4:urn:nasa:pds:0001_nasa_pds_1:pds:product:pds:product_observational::1.0;
  rdfs:range pds4:urn:nasa:pds:0001_nasa_pds_1:pds:file_area:pds:file_area_observational::1.0.
 
pds4:urn:nasa:pds:0001_nasa_pds_1:pds:product:pds:product_observational::observation_area::1.0 rdf:type rdf:Property;
  rdfs:label "observation_area";
  rdfs:domain pds4:urn:nasa:pds:0001_nasa_pds_1:pds:product:pds:product_observational::1.0;
  rdfs:range pds4:urn:nasa:pds:0001_nasa_pds_1:pds:context_area:pds:observation_area::1.0.
 
pds4:urn:nasa:pds:0001_nasa_pds_1:pds:product:pds:product_observational::file_area_supplemental::1.0 rdf:type rdf:Property;
  rdfs:label "file_area_supplemental";
  rdfs:domain pds4:urn:nasa:pds:0001_nasa_pds_1:pds:product:pds:product_observational::1.0;
  rdfs:range pds4:urn:nasa:pds:0001_nasa_pds_1:pds:file_area:pds:file_area_observational_supplemental::1.0.
 
pds4:urn:nasa:pds:0001_nasa_pds_1:pds:product:pds:product_proxy_pds3::reference_list::1.0 rdf:type rdf:Property;
  rdfs:label "reference_list";
  rdfs:domain pds4:urn:nasa:pds:0001_nasa_pds_1:pds:product:pds:product_proxy_pds3::1.0;
  rdfs:range pds4:urn:nasa:pds:0001_nasa_pds_1:pds:product_components:pds:reference_list::1.0.
 
pds4:urn:nasa:pds:0001_nasa_pds_1:pds:product:pds:product_proxy_pds3::file_area::1.0 rdf:type rdf:Property;
  rdfs:label "file_area";
  rdfs:domain pds4:urn:nasa:pds:0001_nasa_pds_1:pds:product:pds:product_proxy_pds3::1.0;
  rdfs:range pds4:urn:nasa:pds:0001_nasa_pds_1:pds:file_area:pds:file_area_binary::1.0.
 
pds4:urn:nasa:pds:0001_nasa_pds_1:pds:product:pds:product_sip::reference_list::1.0 rdf:type rdf:Property;
  rdfs:label "reference_list";
  rdfs:domain pds4:urn:nasa:pds:0001_nasa_pds_1:pds:product:pds:product_sip::1.0;
  rdfs:range pds4:urn:nasa:pds:0001_nasa_pds_1:pds:product_components:pds:reference_list::1.0.
 
pds4:urn:nasa:pds:0001_nasa_pds_1:pds:product:pds:product_sip::has_information_package_component::1.0 rdf:type rdf:Property;
  rdfs:label "has_Information_Package_Component";
  rdfs:domain pds4:urn:nasa:pds:0001_nasa_pds_1:pds:product:pds:product_sip::1.0;
  rdfs:range pds4:urn:nasa:pds:0001_nasa_pds_1:pds:tndo_supplemental:pds:information_package_component::1.0.
 
pds4:urn:nasa:pds:0001_nasa_pds_1:pds:product:pds:product_sip::product_data_object::1.0 rdf:type rdf:Property;
  rdfs:label "product_data_object";
  rdfs:domain pds4:urn:nasa:pds:0001_nasa_pds_1:pds:product:pds:product_sip::1.0;
  rdfs:range pds4:urn:nasa:pds:0001_nasa_pds_1:pds:information_package:pds:submission_information_package::1.0.
 
pds4:urn:nasa:pds:0001_nasa_pds_1:pds:product:pds:product_sip_deep_archive::reference_list::1.0 rdf:type rdf:Property;
  rdfs:label "reference_list";
  rdfs:domain pds4:urn:nasa:pds:0001_nasa_pds_1:pds:product:pds:product_sip_deep_archive::1.0;
  rdfs:range pds4:urn:nasa:pds:0001_nasa_pds_1:pds:product_components:pds:reference_list::1.0.
 
pds4:urn:nasa:pds:0001_nasa_pds_1:pds:product:pds:product_sip_deep_archive::has_information_package_component::1.0 rdf:type rdf:Property;
  rdfs:label "has_Information_Package_Component";
  rdfs:domain pds4:urn:nasa:pds:0001_nasa_pds_1:pds:product:pds:product_sip_deep_archive::1.0;
  rdfs:range pds4:urn:nasa:pds:0001_nasa_pds_1:pds:tndo_supplemental:pds:information_package_component_deep_archive::1.0.
 
pds4:urn:nasa:pds:0001_nasa_pds_1:pds:product:pds:product_sip_deep_archive::product_data_object::1.0 rdf:type rdf:Property;
  rdfs:label "product_data_object";
  rdfs:domain pds4:urn:nasa:pds:0001_nasa_pds_1:pds:product:pds:product_sip_deep_archive::1.0;
  rdfs:range pds4:urn:nasa:pds:0001_nasa_pds_1:pds:information_package:pds:sip_deep_archive::1.0.
 
pds4:urn:nasa:pds:0001_nasa_pds_1:pds:product:pds:product_spice_kernel::context_area::1.0 rdf:type rdf:Property;
  rdfs:label "context_area";
  rdfs:domain pds4:urn:nasa:pds:0001_nasa_pds_1:pds:product:pds:product_spice_kernel::1.0;
  rdfs:range pds4:urn:nasa:pds:0001_nasa_pds_1:pds:product_components:pds:context_area::1.0.
 
pds4:urn:nasa:pds:0001_nasa_pds_1:pds:product:pds:product_spice_kernel::reference_list::1.0 rdf:type rdf:Property;
  rdfs:label "reference_list";
  rdfs:domain pds4:urn:nasa:pds:0001_nasa_pds_1:pds:product:pds:product_spice_kernel::1.0;
  rdfs:range pds4:urn:nasa:pds:0001_nasa_pds_1:pds:product_components:pds:reference_list::1.0.
 
pds4:urn:nasa:pds:0001_nasa_pds_1:pds:product:pds:product_spice_kernel::file_area::1.0 rdf:type rdf:Property;
  rdfs:label "file_area";
  rdfs:domain pds4:urn:nasa:pds:0001_nasa_pds_1:pds:product:pds:product_spice_kernel::1.0;
  rdfs:range pds4:urn:nasa:pds:0001_nasa_pds_1:pds:file_area:pds:file_area_spice_kernel::1.0.
 
pds4:urn:nasa:pds:0001_nasa_pds_1:pds:product:pds:product_service::reference_list::1.0 rdf:type rdf:Property;
  rdfs:label "reference_list";
  rdfs:domain pds4:urn:nasa:pds:0001_nasa_pds_1:pds:product:pds:product_service::1.0;
  rdfs:range pds4:urn:nasa:pds:0001_nasa_pds_1:pds:product_components:pds:reference_list::1.0.
 
pds4:urn:nasa:pds:0001_nasa_pds_1:pds:product:pds:product_service::file_area::1.0 rdf:type rdf:Property;
  rdfs:label "file_area";
  rdfs:domain pds4:urn:nasa:pds:0001_nasa_pds_1:pds:product:pds:product_service::1.0;
  rdfs:range pds4:urn:nasa:pds:0001_nasa_pds_1:pds:file_area:pds:file_area_service_description::1.0.
 
pds4:urn:nasa:pds:0001_nasa_pds_1:pds:product:pds:product_service::product_data_object::1.0 rdf:type rdf:Property;
  rdfs:label "product_data_object";
  rdfs:domain pds4:urn:nasa:pds:0001_nasa_pds_1:pds:product:pds:product_service::1.0;
  rdfs:range pds4:urn:nasa:pds:0001_nasa_pds_1:pds:tndo_context:pds:service::1.0.
 
pds4:urn:nasa:pds:0001_nasa_pds_1:pds:product:pds:product_software::product_description::1.0 rdf:type rdf:Property;
  rdfs:label "product_description";
  rdfs:domain pds4:urn:nasa:pds:0001_nasa_pds_1:pds:product:pds:product_software::1.0;
  rdfs:range pds4:urn:nasa:pds:0001_nasa_pds_1:pds:tndo_supplemental:pds:software::1.0.
 
pds4:urn:nasa:pds:0001_nasa_pds_1:pds:product:pds:product_software::reference_list::1.0 rdf:type rdf:Property;
  rdfs:label "reference_list";
  rdfs:domain pds4:urn:nasa:pds:0001_nasa_pds_1:pds:product:pds:product_software::1.0;
  rdfs:range pds4:urn:nasa:pds:0001_nasa_pds_1:pds:product_components:pds:reference_list::1.0.
 
pds4:urn:nasa:pds:0001_nasa_pds_1:pds:product:pds:product_software::software_format_set::1.0 rdf:type rdf:Property;
  rdfs:label "software_format_set";
  rdfs:domain pds4:urn:nasa:pds:0001_nasa_pds_1:pds:product:pds:product_software::1.0;
  rdfs:range pds4:urn:nasa:pds:0001_nasa_pds_1:pds:tndo_supplemental:pds:software_binary::1.0.
 
pds4:urn:nasa:pds:0001_nasa_pds_1:pds:product:pds:product_software::software_format_set::1.0 rdf:type rdf:Property;
  rdfs:label "software_format_set";
  rdfs:domain pds4:urn:nasa:pds:0001_nasa_pds_1:pds:product:pds:product_software::1.0;
  rdfs:range pds4:urn:nasa:pds:0001_nasa_pds_1:pds:tndo_supplemental:pds:software_script::1.0.
 
pds4:urn:nasa:pds:0001_nasa_pds_1:pds:product:pds:product_software::software_format_set::1.0 rdf:type rdf:Property;
  rdfs:label "software_format_set";
  rdfs:domain pds4:urn:nasa:pds:0001_nasa_pds_1:pds:product:pds:product_software::1.0;
  rdfs:range pds4:urn:nasa:pds:0001_nasa_pds_1:pds:tndo_supplemental:pds:software_source::1.0.
 
pds4:urn:nasa:pds:0001_nasa_pds_1:pds:product:pds:product_subscription_pds3::reference_list::1.0 rdf:type rdf:Property;
  rdfs:label "reference_list";
  rdfs:domain pds4:urn:nasa:pds:0001_nasa_pds_1:pds:product:pds:product_subscription_pds3::1.0;
  rdfs:range pds4:urn:nasa:pds:0001_nasa_pds_1:pds:product_components:pds:reference_list::1.0.
 
pds4:urn:nasa:pds:0001_nasa_pds_1:pds:product:pds:product_subscription_pds3::subscriber::1.0 rdf:type rdf:Property;
  rdfs:label "subscriber";
  rdfs:domain pds4:urn:nasa:pds:0001_nasa_pds_1:pds:product:pds:product_subscription_pds3::1.0;
  rdfs:range pds4:urn:nasa:pds:0001_nasa_pds_1:pds:tndo_context_pds3:pds:subscriber_pds3::1.0.
 
pds4:urn:nasa:pds:0001_nasa_pds_1:pds:product:pds:product_target_pds3::reference_list::1.0 rdf:type rdf:Property;
  rdfs:label "reference_list";
  rdfs:domain pds4:urn:nasa:pds:0001_nasa_pds_1:pds:product:pds:product_target_pds3::1.0;
  rdfs:range pds4:urn:nasa:pds:0001_nasa_pds_1:pds:product_components:pds:reference_list::1.0.
 
pds4:urn:nasa:pds:0001_nasa_pds_1:pds:product:pds:product_target_pds3::product_data_object::1.0 rdf:type rdf:Property;
  rdfs:label "product_data_object";
  rdfs:domain pds4:urn:nasa:pds:0001_nasa_pds_1:pds:product:pds:product_target_pds3::1.0;
  rdfs:range pds4:urn:nasa:pds:0001_nasa_pds_1:pds:tndo_context_pds3:pds:target_pds3::1.0.
 
pds4:urn:nasa:pds:0001_nasa_pds_1:pds:product:pds:product_thumbnail::reference_list::1.0 rdf:type rdf:Property;
  rdfs:label "reference_list";
  rdfs:domain pds4:urn:nasa:pds:0001_nasa_pds_1:pds:product:pds:product_thumbnail::1.0;
  rdfs:range pds4:urn:nasa:pds:0001_nasa_pds_1:pds:product_components:pds:reference_list::1.0.
 
pds4:urn:nasa:pds:0001_nasa_pds_1:pds:product:pds:product_thumbnail::file_area::1.0 rdf:type rdf:Property;
  rdfs:label "file_area";
  rdfs:domain pds4:urn:nasa:pds:0001_nasa_pds_1:pds:product:pds:product_thumbnail::1.0;
  rdfs:range pds4:urn:nasa:pds:0001_nasa_pds_1:pds:file_area:pds:file_area_encoded_image::1.0.
 
pds4:urn:nasa:pds:0001_nasa_pds_1:pds:product:pds:product_update::reference_list::1.0 rdf:type rdf:Property;
  rdfs:label "reference_list";
  rdfs:domain pds4:urn:nasa:pds:0001_nasa_pds_1:pds:product:pds:product_update::1.0;
  rdfs:range pds4:urn:nasa:pds:0001_nasa_pds_1:pds:product_components:pds:reference_list::1.0.
 
pds4:urn:nasa:pds:0001_nasa_pds_1:pds:product:pds:product_update::file_area::1.0 rdf:type rdf:Property;
  rdfs:label "file_area";
  rdfs:domain pds4:urn:nasa:pds:0001_nasa_pds_1:pds:product:pds:product_update::1.0;
  rdfs:range pds4:urn:nasa:pds:0001_nasa_pds_1:pds:file_area:pds:file_area_update::1.0.
 
pds4:urn:nasa:pds:0001_nasa_pds_1:pds:product:pds:product_update::product_data_object::1.0 rdf:type rdf:Property;
  rdfs:label "product_data_object";
  rdfs:domain pds4:urn:nasa:pds:0001_nasa_pds_1:pds:product:pds:product_update::1.0;
  rdfs:range pds4:urn:nasa:pds:0001_nasa_pds_1:pds:tndo_supplemental:pds:update::1.0.
 
pds4:urn:nasa:pds:0001_nasa_pds_1:pds:product:pds:product_volume_pds3::reference_list::1.0 rdf:type rdf:Property;
  rdfs:label "reference_list";
  rdfs:domain pds4:urn:nasa:pds:0001_nasa_pds_1:pds:product:pds:product_volume_pds3::1.0;
  rdfs:range pds4:urn:nasa:pds:0001_nasa_pds_1:pds:product_components:pds:reference_list::1.0.
 
pds4:urn:nasa:pds:0001_nasa_pds_1:pds:product:pds:product_volume_pds3::product_data_object::1.0 rdf:type rdf:Property;
  rdfs:label "product_data_object";
  rdfs:domain pds4:urn:nasa:pds:0001_nasa_pds_1:pds:product:pds:product_volume_pds3::1.0;
  rdfs:range pds4:urn:nasa:pds:0001_nasa_pds_1:pds:tndo_context_pds3:pds:volume_pds3::1.0.
 
pds4:urn:nasa:pds:0001_nasa_pds_1:pds:product:pds:product_volume_set_pds3::reference_list::1.0 rdf:type rdf:Property;
  rdfs:label "reference_list";
  rdfs:domain pds4:urn:nasa:pds:0001_nasa_pds_1:pds:product:pds:product_volume_set_pds3::1.0;
  rdfs:range pds4:urn:nasa:pds:0001_nasa_pds_1:pds:product_components:pds:reference_list::1.0.
 
pds4:urn:nasa:pds:0001_nasa_pds_1:pds:product:pds:product_volume_set_pds3::product_data_object::1.0 rdf:type rdf:Property;
  rdfs:label "product_data_object";
  rdfs:domain pds4:urn:nasa:pds:0001_nasa_pds_1:pds:product:pds:product_volume_set_pds3::1.0;
  rdfs:range pds4:urn:nasa:pds:0001_nasa_pds_1:pds:tndo_context_pds3:pds:volume_set_pds3::1.0.
 
pds4:urn:nasa:pds:0001_nasa_pds_1:pds:product:pds:product_xml_schema::context_area::1.0 rdf:type rdf:Property;
  rdfs:label "context_area";
  rdfs:domain pds4:urn:nasa:pds:0001_nasa_pds_1:pds:product:pds:product_xml_schema::1.0;
  rdfs:range pds4:urn:nasa:pds:0001_nasa_pds_1:pds:product_components:pds:context_area::1.0.
 
pds4:urn:nasa:pds:0001_nasa_pds_1:pds:product:pds:product_xml_schema::reference_list::1.0 rdf:type rdf:Property;
  rdfs:label "reference_list";
  rdfs:domain pds4:urn:nasa:pds:0001_nasa_pds_1:pds:product:pds:product_xml_schema::1.0;
  rdfs:range pds4:urn:nasa:pds:0001_nasa_pds_1:pds:product_components:pds:reference_list::1.0.
 
pds4:urn:nasa:pds:0001_nasa_pds_1:pds:product:pds:product_xml_schema::file_area::1.0 rdf:type rdf:Property;
  rdfs:label "file_area";
  rdfs:domain pds4:urn:nasa:pds:0001_nasa_pds_1:pds:product:pds:product_xml_schema::1.0;
  rdfs:range pds4:urn:nasa:pds:0001_nasa_pds_1:pds:file_area:pds:file_area_xml_schema::1.0.
 
pds4:urn:nasa:pds:0001_nasa_pds_1:pds:product:pds:product_zipped::file::1.0 rdf:type rdf:Property;
  rdfs:label "file";
  rdfs:domain pds4:urn:nasa:pds:0001_nasa_pds_1:pds:product:pds:product_zipped::1.0;
  rdfs:range pds4:urn:nasa:pds:0001_nasa_pds_1:pds:tagged_digital_object:pds:file::1.0.
 
pds4:urn:nasa:pds:0001_nasa_pds_1:pds:product:pds:product_zipped::internal_reference::1.0 rdf:type rdf:Property;
  rdfs:label "internal_reference";
  rdfs:domain pds4:urn:nasa:pds:0001_nasa_pds_1:pds:product:pds:product_zipped::1.0;
  rdfs:range pds4:urn:nasa:pds:0001_nasa_pds_1:pds:product_components:pds:internal_reference::1.0.
 
pds4:urn:nasa:pds:0001_nasa_pds_1:pds:product:pds:product_zipped::has_zip::1.0 rdf:type rdf:Property;
  rdfs:label "has_zip";
  rdfs:domain pds4:urn:nasa:pds:0001_nasa_pds_1:pds:product:pds:product_zipped::1.0;
  rdfs:range pds4:urn:nasa:pds:0001_nasa_pds_1:pds:tndo_supplemental:pds:zip::1.0.
 
pds4:urn:nasa:pds:0001_nasa_pds_1:pds:tndo_supplemental:pds:property_map::has_property_map_entry::1.0 rdf:type rdf:Property;
  rdfs:label "has_Property_Map_Entry";
  rdfs:domain pds4:urn:nasa:pds:0001_nasa_pds_1:pds:tndo_supplemental:pds:property_map::1.0;
  rdfs:range pds4:urn:nasa:pds:0001_nasa_pds_1:pds:tndo_supplemental:pds:property_map_entry::1.0.
 
pds4:urn:nasa:pds:0001_nasa_pds_1:pds:tndo_supplemental:pds:property_maps::has_property_map::1.0 rdf:type rdf:Property;
  rdfs:label "has_property_map";
  rdfs:domain pds4:urn:nasa:pds:0001_nasa_pds_1:pds:tndo_supplemental:pds:property_maps::1.0;
  rdfs:range pds4:urn:nasa:pds:0001_nasa_pds_1:pds:tndo_supplemental:pds:property_map::1.0.
 
pds4:urn:nasa:pds:0001_nasa_pds_1:pds:tndo_supplemental:pds:quaternion::data_object::1.0 rdf:type rdf:Property;
  rdfs:label "data_object";
  rdfs:domain pds4:urn:nasa:pds:0001_nasa_pds_1:pds:tndo_supplemental:pds:quaternion::1.0;
  rdfs:range pds4:urn:nasa:pds:0001_nasa_pds_1:pds:tndo_context:pds:other::1.0.
 
pds4:urn:nasa:pds:0001_nasa_pds_1:pds:tndo_supplemental:pds:quaternion::quaternion_component::1.0 rdf:type rdf:Property;
  rdfs:label "quaternion_component";
  rdfs:domain pds4:urn:nasa:pds:0001_nasa_pds_1:pds:tndo_supplemental:pds:quaternion::1.0;
  rdfs:range pds4:urn:nasa:pds:0001_nasa_pds_1:pds:tagged_nondigital_child:pds:quaternion_component::1.0.
 
pds4:urn:nasa:pds:0001_nasa_pds_1:pds:record:pds:record_binary::has_table_field::1.0 rdf:type rdf:Property;
  rdfs:label "has_Table_Field";
  rdfs:domain pds4:urn:nasa:pds:0001_nasa_pds_1:pds:record:pds:record_binary::1.0;
  rdfs:range pds4:urn:nasa:pds:0001_nasa_pds_1:pds:field:pds:field_binary::1.0.
 
pds4:urn:nasa:pds:0001_nasa_pds_1:pds:record:pds:record_binary::has_table_field::1.0 rdf:type rdf:Property;
  rdfs:label "has_Table_Field";
  rdfs:domain pds4:urn:nasa:pds:0001_nasa_pds_1:pds:record:pds:record_binary::1.0;
  rdfs:range pds4:urn:nasa:pds:0001_nasa_pds_1:pds:group:pds:group_field_binary::1.0.
 
pds4:urn:nasa:pds:0001_nasa_pds_1:pds:record:pds:record_character::has_character_field::1.0 rdf:type rdf:Property;
  rdfs:label "has_Character_Field";
  rdfs:domain pds4:urn:nasa:pds:0001_nasa_pds_1:pds:record:pds:record_character::1.0;
  rdfs:range pds4:urn:nasa:pds:0001_nasa_pds_1:pds:field:pds:field_character::1.0.
 
pds4:urn:nasa:pds:0001_nasa_pds_1:pds:record:pds:record_character::has_character_field::1.0 rdf:type rdf:Property;
  rdfs:label "has_Character_Field";
  rdfs:domain pds4:urn:nasa:pds:0001_nasa_pds_1:pds:record:pds:record_character::1.0;
  rdfs:range pds4:urn:nasa:pds:0001_nasa_pds_1:pds:group:pds:group_field_character::1.0.
 
pds4:urn:nasa:pds:0001_nasa_pds_1:pds:record:pds:record_delimited::has_delimited_field::1.0 rdf:type rdf:Property;
  rdfs:label "has_Delimited_Field";
  rdfs:domain pds4:urn:nasa:pds:0001_nasa_pds_1:pds:record:pds:record_delimited::1.0;
  rdfs:range pds4:urn:nasa:pds:0001_nasa_pds_1:pds:field:pds:field_delimited::1.0.
 
pds4:urn:nasa:pds:0001_nasa_pds_1:pds:record:pds:record_delimited::has_delimited_field::1.0 rdf:type rdf:Property;
  rdfs:label "has_Delimited_Field";
  rdfs:domain pds4:urn:nasa:pds:0001_nasa_pds_1:pds:record:pds:record_delimited::1.0;
  rdfs:range pds4:urn:nasa:pds:0001_nasa_pds_1:pds:group:pds:group_field_delimited::1.0.
 
pds4:urn:nasa:pds:0001_nasa_pds_1:pds:product_components:pds:reference_list::external_reference::1.0 rdf:type rdf:Property;
  rdfs:label "external_reference";
  rdfs:domain pds4:urn:nasa:pds:0001_nasa_pds_1:pds:product_components:pds:reference_list::1.0;
  rdfs:range pds4:urn:nasa:pds:0001_nasa_pds_1:pds:product_components:pds:external_reference::1.0.
 
pds4:urn:nasa:pds:0001_nasa_pds_1:pds:product_components:pds:reference_list::source_product_external::1.0 rdf:type rdf:Property;
  rdfs:label "source_product_external";
  rdfs:domain pds4:urn:nasa:pds:0001_nasa_pds_1:pds:product_components:pds:reference_list::1.0;
  rdfs:range pds4:urn:nasa:pds:0001_nasa_pds_1:pds:tagged_nondigital_child:pds:source_product_external::1.0.
 
pds4:urn:nasa:pds:0001_nasa_pds_1:pds:product_components:pds:reference_list::internal_reference::1.0 rdf:type rdf:Property;
  rdfs:label "internal_reference";
  rdfs:domain pds4:urn:nasa:pds:0001_nasa_pds_1:pds:product_components:pds:reference_list::1.0;
  rdfs:range pds4:urn:nasa:pds:0001_nasa_pds_1:pds:product_components:pds:internal_reference::1.0.
 
pds4:urn:nasa:pds:0001_nasa_pds_1:pds:product_components:pds:reference_list::source_product_internal::1.0 rdf:type rdf:Property;
  rdfs:label "source_product_internal";
  rdfs:domain pds4:urn:nasa:pds:0001_nasa_pds_1:pds:product_components:pds:reference_list::1.0;
  rdfs:range pds4:urn:nasa:pds:0001_nasa_pds_1:pds:tagged_nondigital_child:pds:source_product_internal::1.0.
 
pds4:urn:nasa:pds:0001_nasa_pds_1:pds:tndo_context:pds:resource::data_object::1.0 rdf:type rdf:Property;
  rdfs:label "data_object";
  rdfs:domain pds4:urn:nasa:pds:0001_nasa_pds_1:pds:tndo_context:pds:resource::1.0;
  rdfs:range pds4:urn:nasa:pds:0001_nasa_pds_1:pds:tndo_context:pds:other::1.0.
 
pds4:urn:nasa:pds:0001_nasa_pds_1:pds:product_components:pds:science_facets::has_discipline_facets::1.0 rdf:type rdf:Property;
  rdfs:label "has_Discipline_Facets";
  rdfs:domain pds4:urn:nasa:pds:0001_nasa_pds_1:pds:product_components:pds:science_facets::1.0;
  rdfs:range pds4:urn:nasa:pds:0001_nasa_pds_1:pds:product_components:pds:discipline_facets::1.0.
 
pds4:urn:nasa:pds:0001_nasa_pds_1:pds:tndo_context:pds:service::data_object::1.0 rdf:type rdf:Property;
  rdfs:label "data_object";
  rdfs:domain pds4:urn:nasa:pds:0001_nasa_pds_1:pds:tndo_context:pds:service::1.0;
  rdfs:range pds4:urn:nasa:pds:0001_nasa_pds_1:pds:tndo_context:pds:other::1.0.
 
pds4:urn:nasa:pds:0001_nasa_pds_1:pds:tndo_supplemental:pds:software::data_object::1.0 rdf:type rdf:Property;
  rdfs:label "data_object";
  rdfs:domain pds4:urn:nasa:pds:0001_nasa_pds_1:pds:tndo_supplemental:pds:software::1.0;
  rdfs:range pds4:urn:nasa:pds:0001_nasa_pds_1:pds:tndo_context:pds:other::1.0.
 
pds4:urn:nasa:pds:0001_nasa_pds_1:pds:tndo_supplemental:pds:software_binary::data_object::1.0 rdf:type rdf:Property;
  rdfs:label "data_object";
  rdfs:domain pds4:urn:nasa:pds:0001_nasa_pds_1:pds:tndo_supplemental:pds:software_binary::1.0;
  rdfs:range pds4:urn:nasa:pds:0001_nasa_pds_1:pds:tndo_context:pds:other::1.0.
 
pds4:urn:nasa:pds:0001_nasa_pds_1:pds:tndo_supplemental:pds:software_script::data_object::1.0 rdf:type rdf:Property;
  rdfs:label "data_object";
  rdfs:domain pds4:urn:nasa:pds:0001_nasa_pds_1:pds:tndo_supplemental:pds:software_script::1.0;
  rdfs:range pds4:urn:nasa:pds:0001_nasa_pds_1:pds:tndo_context:pds:other::1.0.
 
pds4:urn:nasa:pds:0001_nasa_pds_1:pds:tndo_supplemental:pds:software_source::data_object::1.0 rdf:type rdf:Property;
  rdfs:label "data_object";
  rdfs:domain pds4:urn:nasa:pds:0001_nasa_pds_1:pds:tndo_supplemental:pds:software_source::1.0;
  rdfs:range pds4:urn:nasa:pds:0001_nasa_pds_1:pds:tndo_context:pds:other::1.0.
 
pds4:urn:nasa:pds:0001_nasa_pds_1:pds:byte_stream:pds:table_base::data_object::1.0 rdf:type rdf:Property;
  rdfs:label "data_object";
  rdfs:domain pds4:urn:nasa:pds:0001_nasa_pds_1:pds:byte_stream:pds:table_base::1.0;
  rdfs:range pds4:urn:nasa:pds:0001_nasa_pds_1:pds:tndo_context:pds:other::1.0.
 
pds4:urn:nasa:pds:0001_nasa_pds_1:pds:table_base:pds:table_binary::uniformly_sampled::1.0 rdf:type rdf:Property;
  rdfs:label "uniformly_sampled";
  rdfs:domain pds4:urn:nasa:pds:0001_nasa_pds_1:pds:table_base:pds:table_binary::1.0;
  rdfs:range pds4:urn:nasa:pds:0001_nasa_pds_1:pds:tagged_digital_child:pds:uniformly_sampled::1.0.
 
pds4:urn:nasa:pds:0001_nasa_pds_1:pds:table_base:pds:table_binary::has_record::1.0 rdf:type rdf:Property;
  rdfs:label "has_Record";
  rdfs:domain pds4:urn:nasa:pds:0001_nasa_pds_1:pds:table_base:pds:table_binary::1.0;
  rdfs:range pds4:urn:nasa:pds:0001_nasa_pds_1:pds:record:pds:record_binary::1.0.
 
pds4:urn:nasa:pds:0001_nasa_pds_1:pds:table_base:pds:table_character::uniformly_sampled::1.0 rdf:type rdf:Property;
  rdfs:label "uniformly_sampled";
  rdfs:domain pds4:urn:nasa:pds:0001_nasa_pds_1:pds:table_base:pds:table_character::1.0;
  rdfs:range pds4:urn:nasa:pds:0001_nasa_pds_1:pds:tagged_digital_child:pds:uniformly_sampled::1.0.
 
pds4:urn:nasa:pds:0001_nasa_pds_1:pds:table_base:pds:table_character::has_record::1.0 rdf:type rdf:Property;
  rdfs:label "has_Record";
  rdfs:domain pds4:urn:nasa:pds:0001_nasa_pds_1:pds:table_base:pds:table_character::1.0;
  rdfs:range pds4:urn:nasa:pds:0001_nasa_pds_1:pds:record:pds:record_character::1.0.
 
pds4:urn:nasa:pds:0001_nasa_pds_1:pds:parsable_byte_stream:pds:table_delimited::uniformly_sampled::1.0 rdf:type rdf:Property;
  rdfs:label "uniformly_sampled";
  rdfs:domain pds4:urn:nasa:pds:0001_nasa_pds_1:pds:parsable_byte_stream:pds:table_delimited::1.0;
  rdfs:range pds4:urn:nasa:pds:0001_nasa_pds_1:pds:tagged_digital_child:pds:uniformly_sampled::1.0.
 
pds4:urn:nasa:pds:0001_nasa_pds_1:pds:parsable_byte_stream:pds:table_delimited::has_delimited_record::1.0 rdf:type rdf:Property;
  rdfs:label "has_delimited_record";
  rdfs:domain pds4:urn:nasa:pds:0001_nasa_pds_1:pds:parsable_byte_stream:pds:table_delimited::1.0;
  rdfs:range pds4:urn:nasa:pds:0001_nasa_pds_1:pds:record:pds:record_delimited::1.0.
 
pds4:urn:nasa:pds:0001_nasa_pds_1:pds:tndo_context:pds:target::data_object::1.0 rdf:type rdf:Property;
  rdfs:label "data_object";
  rdfs:domain pds4:urn:nasa:pds:0001_nasa_pds_1:pds:tndo_context:pds:target::1.0;
  rdfs:range pds4:urn:nasa:pds:0001_nasa_pds_1:pds:tndo_context:pds:other::1.0.
 
pds4:urn:nasa:pds:0001_nasa_pds_1:pds:product_components:pds:target_identification::internal_reference::1.0 rdf:type rdf:Property;
  rdfs:label "internal_reference";
  rdfs:domain pds4:urn:nasa:pds:0001_nasa_pds_1:pds:product_components:pds:target_identification::1.0;
  rdfs:range pds4:urn:nasa:pds:0001_nasa_pds_1:pds:product_components:pds:internal_reference::1.0.
 
pds4:urn:nasa:pds:0001_nasa_pds_1:pds:tndo_context_pds3:pds:target_pds3::data_object::1.0 rdf:type rdf:Property;
  rdfs:label "data_object";
  rdfs:domain pds4:urn:nasa:pds:0001_nasa_pds_1:pds:tndo_context_pds3:pds:target_pds3::1.0;
  rdfs:range pds4:urn:nasa:pds:0001_nasa_pds_1:pds:tndo_context:pds:other::1.0.
 
pds4:urn:nasa:pds:0001_nasa_pds_1:pds:tndo_context:pds:telescope::data_object::1.0 rdf:type rdf:Property;
  rdfs:label "data_object";
  rdfs:domain pds4:urn:nasa:pds:0001_nasa_pds_1:pds:tndo_context:pds:telescope::1.0;
  rdfs:range pds4:urn:nasa:pds:0001_nasa_pds_1:pds:tndo_context:pds:other::1.0.
 
pds4:urn:nasa:pds:0001_nasa_pds_1:pds:tndo_supplemental:pds:term_map_skos::term_map_skos_to_term_entry_skos::1.0 rdf:type rdf:Property;
  rdfs:label "Term_Map_SKOS_to_Term_Entry_SKOS";
  rdfs:domain pds4:urn:nasa:pds:0001_nasa_pds_1:pds:tndo_supplemental:pds:term_map_skos::1.0;
  rdfs:range pds4:urn:nasa:pds:0001_nasa_pds_1:pds:tagged_nondigital_child:pds:terminological_entry_skos::1.0.
 
pds4:urn:nasa:pds:0001_nasa_pds_1:pds:tagged_nondigital_child:pds:terminological_entry::source::1.0 rdf:type rdf:Property;
  rdfs:label "source";
  rdfs:domain pds4:urn:nasa:pds:0001_nasa_pds_1:pds:tagged_nondigital_child:pds:terminological_entry::1.0;
  rdfs:range pds4:urn:nasa:pds:0001_nasa_pds_1:pds:external_reference:pds:external_reference_extended::1.0.
 
pds4:urn:nasa:pds:0001_nasa_pds_1:pds:tndo_supplemental:pds:update::data_object::1.0 rdf:type rdf:Property;
  rdfs:label "data_object";
  rdfs:domain pds4:urn:nasa:pds:0001_nasa_pds_1:pds:tndo_supplemental:pds:update::1.0;
  rdfs:range pds4:urn:nasa:pds:0001_nasa_pds_1:pds:tndo_context:pds:other::1.0.
 
pds4:urn:nasa:pds:0001_nasa_pds_1:pds:tndo_supplemental:pds:update::update_entry::1.0 rdf:type rdf:Property;
  rdfs:label "update_entry";
  rdfs:domain pds4:urn:nasa:pds:0001_nasa_pds_1:pds:tndo_supplemental:pds:update::1.0;
  rdfs:range pds4:urn:nasa:pds:0001_nasa_pds_1:pds:product_components:pds:update_entry::1.0.
 
pds4:urn:nasa:pds:0001_nasa_pds_1:pds:product_components:pds:update_entry::internal_reference::1.0 rdf:type rdf:Property;
  rdfs:label "internal_reference";
  rdfs:domain pds4:urn:nasa:pds:0001_nasa_pds_1:pds:product_components:pds:update_entry::1.0;
  rdfs:range pds4:urn:nasa:pds:0001_nasa_pds_1:pds:product_components:pds:internal_reference::1.0.
 
pds4:urn:nasa:pds:0001_nasa_pds_1:pds:tndo_supplemental:pds:vector::data_object::1.0 rdf:type rdf:Property;
  rdfs:label "data_object";
  rdfs:domain pds4:urn:nasa:pds:0001_nasa_pds_1:pds:tndo_supplemental:pds:vector::1.0;
  rdfs:range pds4:urn:nasa:pds:0001_nasa_pds_1:pds:tndo_context:pds:other::1.0.
 
pds4:urn:nasa:pds:0001_nasa_pds_1:pds:tndo_supplemental:pds:vector::vector_component::1.0 rdf:type rdf:Property;
  rdfs:label "vector_component";
  rdfs:domain pds4:urn:nasa:pds:0001_nasa_pds_1:pds:tndo_supplemental:pds:vector::1.0;
  rdfs:range pds4:urn:nasa:pds:0001_nasa_pds_1:pds:tagged_nondigital_child:pds:vector_component::1.0.
 
pds4:urn:nasa:pds:0001_nasa_pds_1:pds:tndo_context_pds3:pds:volume_pds3::data_object::1.0 rdf:type rdf:Property;
  rdfs:label "data_object";
  rdfs:domain pds4:urn:nasa:pds:0001_nasa_pds_1:pds:tndo_context_pds3:pds:volume_pds3::1.0;
  rdfs:range pds4:urn:nasa:pds:0001_nasa_pds_1:pds:tndo_context:pds:other::1.0.
 
pds4:urn:nasa:pds:0001_nasa_pds_1:pds:tndo_context_pds3:pds:volume_pds3::data_object::1.0 rdf:type rdf:Property;
  rdfs:label "data_object";
  rdfs:domain pds4:urn:nasa:pds:0001_nasa_pds_1:pds:tndo_context_pds3:pds:volume_pds3::1.0;
  rdfs:range pds4:urn:nasa:pds:0001_nasa_pds_1:pds:tndo_context:pds:other::1.0.
 
pds4:urn:nasa:pds:0001_nasa_pds_1:pds:tndo_context_pds3:pds:volume_set_pds3::data_object::1.0 rdf:type rdf:Property;
  rdfs:label "data_object";
  rdfs:domain pds4:urn:nasa:pds:0001_nasa_pds_1:pds:tndo_context_pds3:pds:volume_set_pds3::1.0;
  rdfs:range pds4:urn:nasa:pds:0001_nasa_pds_1:pds:tndo_context:pds:other::1.0.
 
pds4:urn:nasa:pds:0001_nasa_pds_1:pds:tndo_context_pds3:pds:volume_set_pds3::data_object::1.0 rdf:type rdf:Property;
  rdfs:label "data_object";
  rdfs:domain pds4:urn:nasa:pds:0001_nasa_pds_1:pds:tndo_context_pds3:pds:volume_set_pds3::1.0;
  rdfs:range pds4:urn:nasa:pds:0001_nasa_pds_1:pds:tndo_context:pds:other::1.0.
 
pds4:urn:nasa:pds:0001_nasa_pds_1:all:user:proc:input_product::internal_reference::1.0 rdf:type rdf:Property;
  rdfs:label "Internal_Reference";
  rdfs:domain pds4:urn:nasa:pds:0001_nasa_pds_1:all:user:proc:input_product::1.0;
  rdfs:range pds4:urn:nasa:pds:0001_nasa_pds_1:pds:product_components:pds:internal_reference::1.0.
 
pds4:urn:nasa:pds:0001_nasa_pds_1:all:user:proc:input_product::local_internal_reference::1.0 rdf:type rdf:Property;
  rdfs:label "Local_Internal_Reference";
  rdfs:domain pds4:urn:nasa:pds:0001_nasa_pds_1:all:user:proc:input_product::1.0;
  rdfs:range pds4:urn:nasa:pds:0001_nasa_pds_1:pds:product_components:pds:local_internal_reference::1.0.
 
pds4:urn:nasa:pds:0001_nasa_pds_1:all:user:proc:input_product::external_reference::1.0 rdf:type rdf:Property;
  rdfs:label "External_Reference";
  rdfs:domain pds4:urn:nasa:pds:0001_nasa_pds_1:all:user:proc:input_product::1.0;
  rdfs:range pds4:urn:nasa:pds:0001_nasa_pds_1:pds:product_components:pds:external_reference::1.0.
 
pds4:urn:nasa:pds:0001_nasa_pds_1:all:user:proc:input_product_list::internal_reference::1.0 rdf:type rdf:Property;
  rdfs:label "Internal_Reference";
  rdfs:domain pds4:urn:nasa:pds:0001_nasa_pds_1:all:user:proc:input_product_list::1.0;
  rdfs:range pds4:urn:nasa:pds:0001_nasa_pds_1:pds:product_components:pds:internal_reference::1.0.
 
pds4:urn:nasa:pds:0001_nasa_pds_1:all:user:proc:input_product_list::local_internal_reference::1.0 rdf:type rdf:Property;
  rdfs:label "Local_Internal_Reference";
  rdfs:domain pds4:urn:nasa:pds:0001_nasa_pds_1:all:user:proc:input_product_list::1.0;
  rdfs:range pds4:urn:nasa:pds:0001_nasa_pds_1:pds:product_components:pds:local_internal_reference::1.0.
 
pds4:urn:nasa:pds:0001_nasa_pds_1:all:user:proc:input_product_list::input_product::1.0 rdf:type rdf:Property;
  rdfs:label "Input_Product";
  rdfs:domain pds4:urn:nasa:pds:0001_nasa_pds_1:all:user:proc:input_product_list::1.0;
  rdfs:range pds4:urn:nasa:pds:0001_nasa_pds_1:all:user:proc:input_product::1.0.
 
pds4:urn:nasa:pds:0001_nasa_pds_1:all:user:proc:parameter::internal_reference::1.0 rdf:type rdf:Property;
  rdfs:label "Internal_Reference";
  rdfs:domain pds4:urn:nasa:pds:0001_nasa_pds_1:all:user:proc:parameter::1.0;
  rdfs:range pds4:urn:nasa:pds:0001_nasa_pds_1:pds:product_components:pds:internal_reference::1.0.
 
pds4:urn:nasa:pds:0001_nasa_pds_1:all:user:proc:parameter::local_internal_reference::1.0 rdf:type rdf:Property;
  rdfs:label "Local_Internal_Reference";
  rdfs:domain pds4:urn:nasa:pds:0001_nasa_pds_1:all:user:proc:parameter::1.0;
  rdfs:range pds4:urn:nasa:pds:0001_nasa_pds_1:pds:product_components:pds:local_internal_reference::1.0.
 
pds4:urn:nasa:pds:0001_nasa_pds_1:all:user:proc:parameter::external_reference::1.0 rdf:type rdf:Property;
  rdfs:label "External_Reference";
  rdfs:domain pds4:urn:nasa:pds:0001_nasa_pds_1:all:user:proc:parameter::1.0;
  rdfs:range pds4:urn:nasa:pds:0001_nasa_pds_1:pds:product_components:pds:external_reference::1.0.
 
pds4:urn:nasa:pds:0001_nasa_pds_1:all:user:proc:process::software::1.0 rdf:type rdf:Property;
  rdfs:label "Software";
  rdfs:domain pds4:urn:nasa:pds:0001_nasa_pds_1:all:user:proc:process::1.0;
  rdfs:range pds4:urn:nasa:pds:0001_nasa_pds_1:all:user:proc:software::1.0.
 
pds4:urn:nasa:pds:0001_nasa_pds_1:all:user:proc:processing_information::local_internal_reference::1.0 rdf:type rdf:Property;
  rdfs:label "Local_Internal_Reference";
  rdfs:domain pds4:urn:nasa:pds:0001_nasa_pds_1:all:user:proc:processing_information::1.0;
  rdfs:range pds4:urn:nasa:pds:0001_nasa_pds_1:pds:product_components:pds:local_internal_reference::1.0.
 
pds4:urn:nasa:pds:0001_nasa_pds_1:all:user:proc:processing_information::input_product_list::1.0 rdf:type rdf:Property;
  rdfs:label "Input_Product_List";
  rdfs:domain pds4:urn:nasa:pds:0001_nasa_pds_1:all:user:proc:processing_information::1.0;
  rdfs:range pds4:urn:nasa:pds:0001_nasa_pds_1:all:user:proc:input_product_list::1.0.
 
pds4:urn:nasa:pds:0001_nasa_pds_1:all:user:proc:processing_information::process::1.0 rdf:type rdf:Property;
  rdfs:label "Process";
  rdfs:domain pds4:urn:nasa:pds:0001_nasa_pds_1:all:user:proc:processing_information::1.0;
  rdfs:range pds4:urn:nasa:pds:0001_nasa_pds_1:all:user:proc:process::1.0.
 
pds4:urn:nasa:pds:0001_nasa_pds_1:all:user:proc:software::internal_reference::1.0 rdf:type rdf:Property;
  rdfs:label "Internal_Reference";
  rdfs:domain pds4:urn:nasa:pds:0001_nasa_pds_1:all:user:proc:software::1.0;
  rdfs:range pds4:urn:nasa:pds:0001_nasa_pds_1:pds:product_components:pds:internal_reference::1.0.
 
pds4:urn:nasa:pds:0001_nasa_pds_1:all:user:proc:software::software_program::1.0 rdf:type rdf:Property;
  rdfs:label "Software_Program";
  rdfs:domain pds4:urn:nasa:pds:0001_nasa_pds_1:all:user:proc:software::1.0;
  rdfs:range pds4:urn:nasa:pds:0001_nasa_pds_1:all:user:proc:software_program::1.0.
 
pds4:urn:nasa:pds:0001_nasa_pds_1:all:user:proc:software_program::software_program_parameters::1.0 rdf:type rdf:Property;
  rdfs:label "Software_Program_Parameters";
  rdfs:domain pds4:urn:nasa:pds:0001_nasa_pds_1:all:user:proc:software_program::1.0;
  rdfs:range pds4:urn:nasa:pds:0001_nasa_pds_1:all:user:proc:software_program_parameters::1.0.
 
pds4:urn:nasa:pds:0001_nasa_pds_1:all:user:proc:software_program_parameters::parameter::1.0 rdf:type rdf:Property;
  rdfs:label "Parameter";
  rdfs:domain pds4:urn:nasa:pds:0001_nasa_pds_1:all:user:proc:software_program_parameters::1.0;
  rdfs:range pds4:urn:nasa:pds:0001_nasa_pds_1:all:user:proc:parameter::1.0.
 
pds4:urn:nasa:pds:0001_nasa_pds_1:all:user:rings:global_model_parameters::reference_frame_ident::1.0 rdf:type rdf:Property;
  rdfs:label "Reference_Frame_Ident";
  rdfs:domain pds4:urn:nasa:pds:0001_nasa_pds_1:all:user:rings:global_model_parameters::1.0;
  rdfs:range pds4:urn:nasa:pds:0001_nasa_pds_1:rings:frame_ident_base:rings:reference_frame_ident::1.0.
 
pds4:urn:nasa:pds:0001_nasa_pds_1:all:user:rings:ring_model::global_model_parameters::1.0 rdf:type rdf:Property;
  rdfs:label "Global_Model_Parameters";
  rdfs:domain pds4:urn:nasa:pds:0001_nasa_pds_1:all:user:rings:ring_model::1.0;
  rdfs:range pds4:urn:nasa:pds:0001_nasa_pds_1:all:user:rings:global_model_parameters::1.0.
 
pds4:urn:nasa:pds:0001_nasa_pds_1:all:user:rings:ring_model::central_body_parameters::1.0 rdf:type rdf:Property;
  rdfs:label "Central_Body_Parameters";
  rdfs:domain pds4:urn:nasa:pds:0001_nasa_pds_1:all:user:rings:ring_model::1.0;
  rdfs:range pds4:urn:nasa:pds:0001_nasa_pds_1:rings:central_body_ident:rings:central_body_parameters::1.0.
 
pds4:urn:nasa:pds:0001_nasa_pds_1:all:user:rings:ring_model::satellite_parameters::1.0 rdf:type rdf:Property;
  rdfs:label "Satellite_Parameters";
  rdfs:domain pds4:urn:nasa:pds:0001_nasa_pds_1:all:user:rings:ring_model::1.0;
  rdfs:range pds4:urn:nasa:pds:0001_nasa_pds_1:all:user:rings:satellite_parameters::1.0.
 
pds4:urn:nasa:pds:0001_nasa_pds_1:all:user:rings:ring_model::ring_orbital_elements::1.0 rdf:type rdf:Property;
  rdfs:label "Ring_Orbital_Elements";
  rdfs:domain pds4:urn:nasa:pds:0001_nasa_pds_1:all:user:rings:ring_model::1.0;
  rdfs:range pds4:urn:nasa:pds:0001_nasa_pds_1:all:user:rings:ring_orbital_elements::1.0.
 
pds4:urn:nasa:pds:0001_nasa_pds_1:all:user:rings:ring_moon_systems::occultation_ring_profile::1.0 rdf:type rdf:Property;
  rdfs:label "Occultation_Ring_Profile";
  rdfs:domain pds4:urn:nasa:pds:0001_nasa_pds_1:all:user:rings:ring_moon_systems::1.0;
  rdfs:range pds4:urn:nasa:pds:0001_nasa_pds_1:all:user:rings:occultation_ring_profile::1.0.
 
pds4:urn:nasa:pds:0001_nasa_pds_1:all:user:rings:ring_moon_systems::occultation_time_series::1.0 rdf:type rdf:Property;
  rdfs:label "Occultation_Time_Series";
  rdfs:domain pds4:urn:nasa:pds:0001_nasa_pds_1:all:user:rings:ring_moon_systems::1.0;
  rdfs:range pds4:urn:nasa:pds:0001_nasa_pds_1:all:user:rings:occultation_time_series::1.0.
 
pds4:urn:nasa:pds:0001_nasa_pds_1:all:user:rings:ring_moon_systems::occultation_supplement::1.0 rdf:type rdf:Property;
  rdfs:label "Occultation_Supplement";
  rdfs:domain pds4:urn:nasa:pds:0001_nasa_pds_1:all:user:rings:ring_moon_systems::1.0;
  rdfs:range pds4:urn:nasa:pds:0001_nasa_pds_1:all:user:rings:occultation_supplement::1.0.
 
pds4:urn:nasa:pds:0001_nasa_pds_1:all:user:rings:ring_moon_systems::ring_model::1.0 rdf:type rdf:Property;
  rdfs:label "Ring_Model";
  rdfs:domain pds4:urn:nasa:pds:0001_nasa_pds_1:all:user:rings:ring_moon_systems::1.0;
  rdfs:range pds4:urn:nasa:pds:0001_nasa_pds_1:all:user:rings:ring_model::1.0.
 
pds4:urn:nasa:pds:0001_nasa_pds_1:all:user:rings:ring_moon_systems::ring_reprojection::1.0 rdf:type rdf:Property;
  rdfs:label "Ring_Reprojection";
  rdfs:domain pds4:urn:nasa:pds:0001_nasa_pds_1:all:user:rings:ring_moon_systems::1.0;
  rdfs:range pds4:urn:nasa:pds:0001_nasa_pds_1:all:user:rings:ring_reprojection::1.0.
 
pds4:urn:nasa:pds:0001_nasa_pds_1:all:user:rings:ring_moon_systems::ring_spectrum::1.0 rdf:type rdf:Property;
  rdfs:label "Ring_Spectrum";
  rdfs:domain pds4:urn:nasa:pds:0001_nasa_pds_1:all:user:rings:ring_moon_systems::1.0;
  rdfs:range pds4:urn:nasa:pds:0001_nasa_pds_1:all:user:rings:ring_spectrum::1.0.
 
pds4:urn:nasa:pds:0001_nasa_pds_1:all:user:rings:ring_orbital_elements::ring_identification::1.0 rdf:type rdf:Property;
  rdfs:label "Ring_Identification";
  rdfs:domain pds4:urn:nasa:pds:0001_nasa_pds_1:all:user:rings:ring_orbital_elements::1.0;
  rdfs:range pds4:urn:nasa:pds:0001_nasa_pds_1:rings:body_ident_base:rings:ring_identification::1.0.
 
pds4:urn:nasa:pds:0001_nasa_pds_1:all:user:rings:ring_orbital_elements::normal_mode_parameters::1.0 rdf:type rdf:Property;
  rdfs:label "Normal_Mode_Parameters";
  rdfs:domain pds4:urn:nasa:pds:0001_nasa_pds_1:all:user:rings:ring_orbital_elements::1.0;
  rdfs:range pds4:urn:nasa:pds:0001_nasa_pds_1:all:user:rings:normal_mode_parameters::1.0.
 
pds4:urn:nasa:pds:0001_nasa_pds_1:all:user:rings:ring_reprojection::display_direction::1.0 rdf:type rdf:Property;
  rdfs:label "Display_Direction";
  rdfs:domain pds4:urn:nasa:pds:0001_nasa_pds_1:all:user:rings:ring_reprojection::1.0;
  rdfs:range pds4:urn:nasa:pds:0001_nasa_pds_1:all:user:rings:display_direction::1.0.
 
pds4:urn:nasa:pds:0001_nasa_pds_1:all:user:rings:ring_reprojection::central_body_parameters::1.0 rdf:type rdf:Property;
  rdfs:label "Central_Body_Parameters";
  rdfs:domain pds4:urn:nasa:pds:0001_nasa_pds_1:all:user:rings:ring_reprojection::1.0;
  rdfs:range pds4:urn:nasa:pds:0001_nasa_pds_1:rings:central_body_ident:rings:central_body_parameters::1.0.
 
pds4:urn:nasa:pds:0001_nasa_pds_1:all:user:rings:ring_reprojection::ring_orbital_elements::1.0 rdf:type rdf:Property;
  rdfs:label "Ring_Orbital_Elements";
  rdfs:domain pds4:urn:nasa:pds:0001_nasa_pds_1:all:user:rings:ring_reprojection::1.0;
  rdfs:range pds4:urn:nasa:pds:0001_nasa_pds_1:all:user:rings:ring_orbital_elements::1.0.
 
pds4:urn:nasa:pds:0001_nasa_pds_1:all:user:rings:ring_reprojection::reprojection_geometry::1.0 rdf:type rdf:Property;
  rdfs:label "Reprojection_Geometry";
  rdfs:domain pds4:urn:nasa:pds:0001_nasa_pds_1:all:user:rings:ring_reprojection::1.0;
  rdfs:range pds4:urn:nasa:pds:0001_nasa_pds_1:all:user:rings:reprojection_geometry::1.0.
 
pds4:urn:nasa:pds:0001_nasa_pds_1:all:user:rings:ring_spectrum::display_direction::1.0 rdf:type rdf:Property;
  rdfs:label "Display_Direction";
  rdfs:domain pds4:urn:nasa:pds:0001_nasa_pds_1:all:user:rings:ring_spectrum::1.0;
  rdfs:range pds4:urn:nasa:pds:0001_nasa_pds_1:all:user:rings:display_direction::1.0.
 
pds4:urn:nasa:pds:0001_nasa_pds_1:all:user:rings:satellite_parameters::satellite_identification::1.0 rdf:type rdf:Property;
  rdfs:label "Satellite_Identification";
  rdfs:domain pds4:urn:nasa:pds:0001_nasa_pds_1:all:user:rings:satellite_parameters::1.0;
  rdfs:range pds4:urn:nasa:pds:0001_nasa_pds_1:rings:body_ident_base:rings:satellite_identification::1.0.
 
pds4:urn:nasa:pds:0001_nasa_pds_1:all:user:rings:uniformly_sampled_radius::local_internal_reference::1.0 rdf:type rdf:Property;
  rdfs:label "Local_Internal_Reference";
  rdfs:domain pds4:urn:nasa:pds:0001_nasa_pds_1:all:user:rings:uniformly_sampled_radius::1.0;
  rdfs:range pds4:urn:nasa:pds:0001_nasa_pds_1:pds:product_components:pds:local_internal_reference::1.0.
 
pds4:urn:nasa:pds:0001_nasa_pds_1:all:user:sp:axis_bin_set_energy::bin_energy::1.0 rdf:type rdf:Property;
  rdfs:label "Bin_Energy";
  rdfs:domain pds4:urn:nasa:pds:0001_nasa_pds_1:all:user:sp:axis_bin_set_energy::1.0;
  rdfs:range pds4:urn:nasa:pds:0001_nasa_pds_1:all:user:sp:bin_energy::1.0.
 
pds4:urn:nasa:pds:0001_nasa_pds_1:all:user:sp:axis_bin_set_frequency::bin_frequency::1.0 rdf:type rdf:Property;
  rdfs:label "Bin_Frequency";
  rdfs:domain pds4:urn:nasa:pds:0001_nasa_pds_1:all:user:sp:axis_bin_set_frequency::1.0;
  rdfs:range pds4:urn:nasa:pds:0001_nasa_pds_1:all:user:sp:bin_frequency::1.0.
 
pds4:urn:nasa:pds:0001_nasa_pds_1:all:user:sp:axis_bin_set_wavelength::bin_wavelength::1.0 rdf:type rdf:Property;
  rdfs:label "Bin_Wavelength";
  rdfs:domain pds4:urn:nasa:pds:0001_nasa_pds_1:all:user:sp:axis_bin_set_wavelength::1.0;
  rdfs:range pds4:urn:nasa:pds:0001_nasa_pds_1:all:user:sp:bin_wavelength::1.0.
 
pds4:urn:nasa:pds:0001_nasa_pds_1:all:user:sp:axis_bin_set_wavenumber::bin_wavenumber::1.0 rdf:type rdf:Property;
  rdfs:label "Bin_Wavenumber";
  rdfs:domain pds4:urn:nasa:pds:0001_nasa_pds_1:all:user:sp:axis_bin_set_wavenumber::1.0;
  rdfs:range pds4:urn:nasa:pds:0001_nasa_pds_1:all:user:sp:bin_wavenumber::1.0.
 
pds4:urn:nasa:pds:0001_nasa_pds_1:all:user:sp:bin_center_lookup::local_internal_reference::1.0 rdf:type rdf:Property;
  rdfs:label "Local_Internal_Reference";
  rdfs:domain pds4:urn:nasa:pds:0001_nasa_pds_1:all:user:sp:bin_center_lookup::1.0;
  rdfs:range pds4:urn:nasa:pds:0001_nasa_pds_1:pds:product_components:pds:local_internal_reference::1.0.
 
pds4:urn:nasa:pds:0001_nasa_pds_1:all:user:sp:bin_center_lookup::internal_reference::1.0 rdf:type rdf:Property;
  rdfs:label "Internal_Reference";
  rdfs:domain pds4:urn:nasa:pds:0001_nasa_pds_1:all:user:sp:bin_center_lookup::1.0;
  rdfs:range pds4:urn:nasa:pds:0001_nasa_pds_1:pds:product_components:pds:internal_reference::1.0.
 
pds4:urn:nasa:pds:0001_nasa_pds_1:all:user:sp:bin_description::uniformly_sampled_frequency::1.0 rdf:type rdf:Property;
  rdfs:label "Uniformly_Sampled_Frequency";
  rdfs:domain pds4:urn:nasa:pds:0001_nasa_pds_1:all:user:sp:bin_description::1.0;
  rdfs:range pds4:urn:nasa:pds:0001_nasa_pds_1:all:user:sp:uniformly_sampled_frequency::1.0.
 
pds4:urn:nasa:pds:0001_nasa_pds_1:all:user:sp:bin_description::uniformly_sampled_wavelength::1.0 rdf:type rdf:Property;
  rdfs:label "Uniformly_Sampled_Wavelength";
  rdfs:domain pds4:urn:nasa:pds:0001_nasa_pds_1:all:user:sp:bin_description::1.0;
  rdfs:range pds4:urn:nasa:pds:0001_nasa_pds_1:all:user:sp:uniformly_sampled_wavelength::1.0.
 
pds4:urn:nasa:pds:0001_nasa_pds_1:all:user:sp:bin_description::uniformly_sampled_wavenumber::1.0 rdf:type rdf:Property;
  rdfs:label "Uniformly_Sampled_Wavenumber";
  rdfs:domain pds4:urn:nasa:pds:0001_nasa_pds_1:all:user:sp:bin_description::1.0;
  rdfs:range pds4:urn:nasa:pds:0001_nasa_pds_1:all:user:sp:uniformly_sampled_wavenumber::1.0.
 
pds4:urn:nasa:pds:0001_nasa_pds_1:all:user:sp:bin_description::axis_bin_set_frequency::1.0 rdf:type rdf:Property;
  rdfs:label "Axis_Bin_Set_Frequency";
  rdfs:domain pds4:urn:nasa:pds:0001_nasa_pds_1:all:user:sp:bin_description::1.0;
  rdfs:range pds4:urn:nasa:pds:0001_nasa_pds_1:all:user:sp:axis_bin_set_frequency::1.0.
 
pds4:urn:nasa:pds:0001_nasa_pds_1:all:user:sp:bin_description::axis_bin_set_wavelength::1.0 rdf:type rdf:Property;
  rdfs:label "Axis_Bin_Set_Wavelength";
  rdfs:domain pds4:urn:nasa:pds:0001_nasa_pds_1:all:user:sp:bin_description::1.0;
  rdfs:range pds4:urn:nasa:pds:0001_nasa_pds_1:all:user:sp:axis_bin_set_wavelength::1.0.
 
pds4:urn:nasa:pds:0001_nasa_pds_1:all:user:sp:bin_description::axis_bin_set_wavenumber::1.0 rdf:type rdf:Property;
  rdfs:label "Axis_Bin_Set_Wavenumber";
  rdfs:domain pds4:urn:nasa:pds:0001_nasa_pds_1:all:user:sp:bin_description::1.0;
  rdfs:range pds4:urn:nasa:pds:0001_nasa_pds_1:all:user:sp:axis_bin_set_wavenumber::1.0.
 
pds4:urn:nasa:pds:0001_nasa_pds_1:all:user:sp:bin_description::spectral_lookup::1.0 rdf:type rdf:Property;
  rdfs:label "Spectral_Lookup";
  rdfs:domain pds4:urn:nasa:pds:0001_nasa_pds_1:all:user:sp:bin_description::1.0;
  rdfs:range pds4:urn:nasa:pds:0001_nasa_pds_1:all:user:sp:spectral_lookup::1.0.
 
pds4:urn:nasa:pds:0001_nasa_pds_1:all:user:sp:bin_energy::filter::1.0 rdf:type rdf:Property;
  rdfs:label "Filter";
  rdfs:domain pds4:urn:nasa:pds:0001_nasa_pds_1:all:user:sp:bin_energy::1.0;
  rdfs:range pds4:urn:nasa:pds:0001_nasa_pds_1:all:user:sp:filter::1.0.
 
pds4:urn:nasa:pds:0001_nasa_pds_1:all:user:sp:bin_frequency::filter::1.0 rdf:type rdf:Property;
  rdfs:label "Filter";
  rdfs:domain pds4:urn:nasa:pds:0001_nasa_pds_1:all:user:sp:bin_frequency::1.0;
  rdfs:range pds4:urn:nasa:pds:0001_nasa_pds_1:all:user:sp:filter::1.0.
 
pds4:urn:nasa:pds:0001_nasa_pds_1:all:user:sp:bin_wavelength::filter::1.0 rdf:type rdf:Property;
  rdfs:label "Filter";
  rdfs:domain pds4:urn:nasa:pds:0001_nasa_pds_1:all:user:sp:bin_wavelength::1.0;
  rdfs:range pds4:urn:nasa:pds:0001_nasa_pds_1:all:user:sp:filter::1.0.
 
pds4:urn:nasa:pds:0001_nasa_pds_1:all:user:sp:bin_wavenumber::filter::1.0 rdf:type rdf:Property;
  rdfs:label "Filter";
  rdfs:domain pds4:urn:nasa:pds:0001_nasa_pds_1:all:user:sp:bin_wavenumber::1.0;
  rdfs:range pds4:urn:nasa:pds:0001_nasa_pds_1:all:user:sp:filter::1.0.
 
pds4:urn:nasa:pds:0001_nasa_pds_1:all:user:sp:bin_width_lookup::local_internal_reference::1.0 rdf:type rdf:Property;
  rdfs:label "Local_Internal_Reference";
  rdfs:domain pds4:urn:nasa:pds:0001_nasa_pds_1:all:user:sp:bin_width_lookup::1.0;
  rdfs:range pds4:urn:nasa:pds:0001_nasa_pds_1:pds:product_components:pds:local_internal_reference::1.0.
 
pds4:urn:nasa:pds:0001_nasa_pds_1:all:user:sp:bin_width_lookup::internal_reference::1.0 rdf:type rdf:Property;
  rdfs:label "Internal_Reference";
  rdfs:domain pds4:urn:nasa:pds:0001_nasa_pds_1:all:user:sp:bin_width_lookup::1.0;
  rdfs:range pds4:urn:nasa:pds:0001_nasa_pds_1:pds:product_components:pds:internal_reference::1.0.
 
pds4:urn:nasa:pds:0001_nasa_pds_1:all:user:sp:field_of_view::circular_fov::1.0 rdf:type rdf:Property;
  rdfs:label "Circular_FOV";
  rdfs:domain pds4:urn:nasa:pds:0001_nasa_pds_1:all:user:sp:field_of_view::1.0;
  rdfs:range pds4:urn:nasa:pds:0001_nasa_pds_1:all:user:sp:circular_fov::1.0.
 
pds4:urn:nasa:pds:0001_nasa_pds_1:all:user:sp:field_of_view::rectangular_fov::1.0 rdf:type rdf:Property;
  rdfs:label "Rectangular_FOV";
  rdfs:domain pds4:urn:nasa:pds:0001_nasa_pds_1:all:user:sp:field_of_view::1.0;
  rdfs:range pds4:urn:nasa:pds:0001_nasa_pds_1:all:user:sp:rectangular_fov::1.0.
 
pds4:urn:nasa:pds:0001_nasa_pds_1:all:user:sp:field_of_view::complex_fov::1.0 rdf:type rdf:Property;
  rdfs:label "Complex_FOV";
  rdfs:domain pds4:urn:nasa:pds:0001_nasa_pds_1:all:user:sp:field_of_view::1.0;
  rdfs:range pds4:urn:nasa:pds:0001_nasa_pds_1:all:user:sp:complex_fov::1.0.
 
pds4:urn:nasa:pds:0001_nasa_pds_1:all:user:sp:field_of_view::internal_reference::1.0 rdf:type rdf:Property;
  rdfs:label "Internal_Reference";
  rdfs:domain pds4:urn:nasa:pds:0001_nasa_pds_1:all:user:sp:field_of_view::1.0;
  rdfs:range pds4:urn:nasa:pds:0001_nasa_pds_1:pds:product_components:pds:internal_reference::1.0.
 
pds4:urn:nasa:pds:0001_nasa_pds_1:all:user:sp:spectral_characteristics::local_internal_reference::1.0 rdf:type rdf:Property;
  rdfs:label "Local_Internal_Reference";
  rdfs:domain pds4:urn:nasa:pds:0001_nasa_pds_1:all:user:sp:spectral_characteristics::1.0;
  rdfs:range pds4:urn:nasa:pds:0001_nasa_pds_1:pds:product_components:pds:local_internal_reference::1.0.
 
pds4:urn:nasa:pds:0001_nasa_pds_1:all:user:sp:spectral_characteristics::observation_parameters::1.0 rdf:type rdf:Property;
  rdfs:label "Observation_Parameters";
  rdfs:domain pds4:urn:nasa:pds:0001_nasa_pds_1:all:user:sp:spectral_characteristics::1.0;
  rdfs:range pds4:urn:nasa:pds:0001_nasa_pds_1:all:user:sp:observation_parameters::1.0.
 
pds4:urn:nasa:pds:0001_nasa_pds_1:all:user:sp:spectral_characteristics::field_of_view::1.0 rdf:type rdf:Property;
  rdfs:label "Field_of_View";
  rdfs:domain pds4:urn:nasa:pds:0001_nasa_pds_1:all:user:sp:spectral_characteristics::1.0;
  rdfs:range pds4:urn:nasa:pds:0001_nasa_pds_1:all:user:sp:field_of_view::1.0.
 
pds4:urn:nasa:pds:0001_nasa_pds_1:all:user:sp:spectral_characteristics::bin_description::1.0 rdf:type rdf:Property;
  rdfs:label "Bin_Description";
  rdfs:domain pds4:urn:nasa:pds:0001_nasa_pds_1:all:user:sp:spectral_characteristics::1.0;
  rdfs:range pds4:urn:nasa:pds:0001_nasa_pds_1:all:user:sp:bin_description::1.0.
 
pds4:urn:nasa:pds:0001_nasa_pds_1:all:user:sp:spectral_lookup::bin_center_lookup::1.0 rdf:type rdf:Property;
  rdfs:label "Bin_Center_Lookup";
  rdfs:domain pds4:urn:nasa:pds:0001_nasa_pds_1:all:user:sp:spectral_lookup::1.0;
  rdfs:range pds4:urn:nasa:pds:0001_nasa_pds_1:all:user:sp:bin_center_lookup::1.0.
 
pds4:urn:nasa:pds:0001_nasa_pds_1:all:user:sp:spectral_lookup::bin_width_lookup::1.0 rdf:type rdf:Property;
  rdfs:label "Bin_Width_Lookup";
  rdfs:domain pds4:urn:nasa:pds:0001_nasa_pds_1:all:user:sp:spectral_lookup::1.0;
  rdfs:range pds4:urn:nasa:pds:0001_nasa_pds_1:all:user:sp:bin_width_lookup::1.0.
 
pds4:urn:nasa:pds:0001_nasa_pds_1:all:user:sp:spectral_lookup::bin_width_constant::1.0 rdf:type rdf:Property;
  rdfs:label "Bin_Width_Constant";
  rdfs:domain pds4:urn:nasa:pds:0001_nasa_pds_1:all:user:sp:spectral_lookup::1.0;
  rdfs:range pds4:urn:nasa:pds:0001_nasa_pds_1:all:user:sp:bin_width_constant::1.0.
 
pds4:urn:nasa:pds:0001_nasa_pds_1:all:user:speclib:ancillary_product::internal_reference::1.0 rdf:type rdf:Property;
  rdfs:label "Internal_Reference";
  rdfs:domain pds4:urn:nasa:pds:0001_nasa_pds_1:all:user:speclib:ancillary_product::1.0;
  rdfs:range pds4:urn:nasa:pds:0001_nasa_pds_1:pds:product_components:pds:internal_reference::1.0.
 
pds4:urn:nasa:pds:0001_nasa_pds_1:all:user:speclib:measurement_instrument::internal_reference::1.0 rdf:type rdf:Property;
  rdfs:label "Internal_Reference";
  rdfs:domain pds4:urn:nasa:pds:0001_nasa_pds_1:all:user:speclib:measurement_instrument::1.0;
  rdfs:range pds4:urn:nasa:pds:0001_nasa_pds_1:pds:product_components:pds:internal_reference::1.0.
 
pds4:urn:nasa:pds:0001_nasa_pds_1:all:user:speclib:measurement_parameters::measurement_instrument::1.0 rdf:type rdf:Property;
  rdfs:label "Measurement_Instrument";
  rdfs:domain pds4:urn:nasa:pds:0001_nasa_pds_1:all:user:speclib:measurement_parameters::1.0;
  rdfs:range pds4:urn:nasa:pds:0001_nasa_pds_1:all:user:speclib:measurement_instrument::1.0.
 
pds4:urn:nasa:pds:0001_nasa_pds_1:all:user:speclib:spectral_library_product::specimen_parameters::1.0 rdf:type rdf:Property;
  rdfs:label "Specimen_Parameters";
  rdfs:domain pds4:urn:nasa:pds:0001_nasa_pds_1:all:user:speclib:spectral_library_product::1.0;
  rdfs:range pds4:urn:nasa:pds:0001_nasa_pds_1:all:user:speclib:specimen_parameters::1.0.
 
pds4:urn:nasa:pds:0001_nasa_pds_1:all:user:speclib:spectral_library_product::specimen_classification::1.0 rdf:type rdf:Property;
  rdfs:label "Specimen_Classification";
  rdfs:domain pds4:urn:nasa:pds:0001_nasa_pds_1:all:user:speclib:spectral_library_product::1.0;
  rdfs:range pds4:urn:nasa:pds:0001_nasa_pds_1:all:user:speclib:specimen_classification::1.0.
 
pds4:urn:nasa:pds:0001_nasa_pds_1:all:user:speclib:spectral_library_product::measurement_parameters::1.0 rdf:type rdf:Property;
  rdfs:label "Measurement_Parameters";
  rdfs:domain pds4:urn:nasa:pds:0001_nasa_pds_1:all:user:speclib:spectral_library_product::1.0;
  rdfs:range pds4:urn:nasa:pds:0001_nasa_pds_1:all:user:speclib:measurement_parameters::1.0.
 
pds4:urn:nasa:pds:0001_nasa_pds_1:all:user:speclib:spectral_library_product::ancillary_product::1.0 rdf:type rdf:Property;
  rdfs:label "Ancillary_Product";
  rdfs:domain pds4:urn:nasa:pds:0001_nasa_pds_1:all:user:speclib:spectral_library_product::1.0;
  rdfs:range pds4:urn:nasa:pds:0001_nasa_pds_1:all:user:speclib:ancillary_product::1.0.
 
pds4:urn:nasa:pds:0001_nasa_pds_1:all:user:survey:corner_position::coordinate::1.0 rdf:type rdf:Property;
  rdfs:label "Coordinate";
  rdfs:domain pds4:urn:nasa:pds:0001_nasa_pds_1:all:user:survey:corner_position::1.0;
  rdfs:range pds4:urn:nasa:pds:0001_nasa_pds_1:all:user:survey:coordinate::1.0.
 
pds4:urn:nasa:pds:0001_nasa_pds_1:all:user:survey:image_corners::corner_position::1.0 rdf:type rdf:Property;
  rdfs:label "Corner_Position";
  rdfs:domain pds4:urn:nasa:pds:0001_nasa_pds_1:all:user:survey:image_corners::1.0;
  rdfs:range pds4:urn:nasa:pds:0001_nasa_pds_1:all:user:survey:corner_position::1.0.
 
pds4:urn:nasa:pds:0001_nasa_pds_1:all:user:survey:limiting_magnitudes::n_sigma_limit::1.0 rdf:type rdf:Property;
  rdfs:label "N_Sigma_Limit";
  rdfs:domain pds4:urn:nasa:pds:0001_nasa_pds_1:all:user:survey:limiting_magnitudes::1.0;
  rdfs:range pds4:urn:nasa:pds:0001_nasa_pds_1:all:user:survey:n_sigma_limit::1.0.
 
pds4:urn:nasa:pds:0001_nasa_pds_1:all:user:survey:limiting_magnitudes::percentage_limit::1.0 rdf:type rdf:Property;
  rdfs:label "Percentage_Limit";
  rdfs:domain pds4:urn:nasa:pds:0001_nasa_pds_1:all:user:survey:limiting_magnitudes::1.0;
  rdfs:range pds4:urn:nasa:pds:0001_nasa_pds_1:all:user:survey:percentage_limit::1.0.
 
pds4:urn:nasa:pds:0001_nasa_pds_1:all:user:survey:survey::image_corners::1.0 rdf:type rdf:Property;
  rdfs:label "Image_Corners";
  rdfs:domain pds4:urn:nasa:pds:0001_nasa_pds_1:all:user:survey:survey::1.0;
  rdfs:range pds4:urn:nasa:pds:0001_nasa_pds_1:all:user:survey:image_corners::1.0.
 
pds4:urn:nasa:pds:0001_nasa_pds_1:all:user:survey:survey::limiting_magnitudes::1.0 rdf:type rdf:Property;
  rdfs:label "Limiting_Magnitudes";
  rdfs:domain pds4:urn:nasa:pds:0001_nasa_pds_1:all:user:survey:survey::1.0;
  rdfs:range pds4:urn:nasa:pds:0001_nasa_pds_1:all:user:survey:limiting_magnitudes::1.0.
 
pds4:urn:nasa:pds:0001_nasa_pds_1:all:user:survey:survey::rollover::1.0 rdf:type rdf:Property;
  rdfs:label "Rollover";
  rdfs:domain pds4:urn:nasa:pds:0001_nasa_pds_1:all:user:survey:survey::1.0;
  rdfs:range pds4:urn:nasa:pds:0001_nasa_pds_1:all:user:survey:rollover::1.0.
  
